@prefix fat: <http://emmo.info/emmo/domain/mechanical-testing/fatigue#> .
@prefix isq: <http://emmo.info/emmo/middle/isq#> .
@prefix isql: <http://emmo.info/emmo/middle/isql#> .
@prefix owl: <http://www.w3.org/2002/07/owl#> .
@prefix rdf: <http://www.w3.org/1999/02/22-rdf-syntax-ns#> .
@prefix top: <http://emmo.info/emmo/top#> .
@prefix xml: <http://www.w3.org/XML/1998/namespace> .
@prefix xsd: <http://www.w3.org/2001/XMLSchema#> .
@prefix math: <http://emmo.info/emmo/middle/math#> .
@prefix rdfs: <http://www.w3.org/2000/01/rdf-schema#> .
@prefix mechanical-testing: <http://emmo.info/emmo/domain/mechanical-testing/1.0.0#> .
@prefix mechtesting: <http://emmo.info/emmo/domain/mechanical-testing#> .
@prefix models: <http://emmo.info/emmo/middle/models#> .
@prefix siunits: <http://emmo.info/emmo/middle/siunits#> .
@prefix holistic: <http://emmo.info/emmo/middle/holistic#> .
@prefix physical: <http://emmo.info/emmo/top/physical#> .
@prefix materials: <http://emmo.info/emmo/middle/materials#> .
@prefix metrology: <http://emmo.info/emmo/middle/metrology#> .
@prefix semiotics: <http://emmo.info/emmo/middle/semiotics#> .
@prefix perceptual: <http://emmo.info/emmo/middle/perceptual#> .
@prefix properties: <http://emmo.info/emmo/middle/properties#> .
@prefix annotations: <http://emmo.info/emmo/top/annotations#> .
@prefix emmo: <http://emmo.info/emmo#> .
@prefix manufacturing: <http://emmo.info/emmo/middle/manufacturing#> .
@prefix mereotopology: <http://emmo.info/emmo/top/mereotopology#> .
@prefix physicalistic: <http://emmo.info/emmo/middle/physicalistic#> .
@prefix reductionistic: <http://emmo.info/emmo/middle/reductionistic#> .
@prefix units-extension: <http://emmo.info/emmo/middle/units-extension#> .
@prefix chemistry: <http://emmo.info/emmo/middle/chemistry#> .
@prefix turtle: <http://www.semanticweb.org/owl/owlapi/turtle#>.
@base <http://emmo.info/emmo/domain/mechanical-testing/fatigue> .

<http://emmo.info/emmo/domain/mechanical-testing/fatigue> rdf:type owl:Ontology ;
                                                           <http://purl.org/dc/terms/abstract> "A domain ontology for Mechanical Testing based on EMMO."@en ,
                                                                                               """European Materials & Modelling Ontology (EMMO)

EMMO is a multidisciplinary effort to develop a standard representational framework (the ontology) based on current materials modelling knowledge, including physical sciences, analytical philosophy and information and communication technologies.

It provides the connection between the physical world, materials characterisation world and materials modelling world.

EMMO is released under a Creative Commons license Attribution 4.0 International (CC BY 4.0)."""@en ;
                                                           <http://purl.org/dc/terms/contributor> "Access, DE" ,
                                                                                                  "Fraunhofer IWM, DE" ,
                                                                                                  "Goldbeck Consulting Ltd (UK)" ,
                                                                                                  "SINTEF, NO" ,
                                                                                                  "University of Bologna, IT" ;
                                                           <http://purl.org/dc/terms/creator> "Adham Hashibon" ,
                                                                                              "Daniele Toti" ,
                                                                                              "Emanuele Ghedini" ,
                                                                                              "Georg Schmitz" ,
                                                                                              "Gerhard Goldbeck" ,
                                                                                              "Jesper Friis" ,
                                                                                              "Joana Francisco Morgado" ,
                                                                                              "Yoav Nahshon" ;
                                                           <http://purl.org/dc/terms/license> "https://creativecommons.org/licenses/by/4.0/legalcode" ;
                                                           <http://purl.org/dc/terms/publisher> "EMMC ASBL" ;
                                                           <http://purl.org/dc/terms/title> "Domain Mechanical Testing"@en ,
                                                                                            "European Materials & Modelling Ontology"@en ;
                                                           rdfs:comment """Contacts:
Gerhard Goldbeck
Goldbeck Consulting Ltd (UK)
email: gerhard@goldbeck-consulting.com

Emanuele Ghedini
University of Bologna (IT)
email: emanuele.ghedini@unibo.it"""@en ,
                                                                        "The EMMO requires FacT++ reasoner plugin in order to visualize all inferences and class hierarchy (ctrl+R hotkey in Protege)."@en ,
                                                                        "This ontology is a joint colaboration between different projects: OYSTER, UrWerk and MarketPlace."@en ;
                                                           owl:versionInfo "1.0.0" ,
                                                                           "1.0.0-alpha2" .

#################################################################
#    Annotation properties
#################################################################

###  http://emmo.info/emmo/middle/chemistry#elucidation
<http://emmo.info/emmo/middle/chemistry#elucidation> rdf:type owl:AnnotationProperty .


###  http://emmo.info/emmo/middle/chemistry#example
<http://emmo.info/emmo/middle/chemistry#example> rdf:type owl:AnnotationProperty .


###  http://emmo.info/emmo/middle/chemistry#iupacDoi
<http://emmo.info/emmo/middle/chemistry#iupacDoi> rdf:type owl:AnnotationProperty .


###  http://emmo.info/emmo/middle/chemistry#wikipediaEntry
<http://emmo.info/emmo/middle/chemistry#wikipediaEntry> rdf:type owl:AnnotationProperty .


###  http://emmo.info/emmo/middle/isq#EMMO_de178b12_5d35_4bca_8efa_a4193162571d
<http://emmo.info/emmo/middle/isq#EMMO_de178b12_5d35_4bca_8efa_a4193162571d> rdf:type owl:AnnotationProperty ;
                                                                             rdfs:comment """A unique string describing the physical dimensionality of a physical quantity. 

See the comments of PhysicalDimension for a description of this \"regex\" string."""@en ;
                                                                             <http://www.w3.org/2004/02/skos/core#prefLabel> "physicalDimension"@en .


###  http://emmo.info/emmo/middle/isq#physicalDimension
<http://emmo.info/emmo/middle/isq#physicalDimension> rdf:type owl:AnnotationProperty .


###  http://emmo.info/emmo/top/annotations#EMMO_1f1b164d_ec6a_4faa_8d5e_88bda62316cc
<http://emmo.info/emmo/top/annotations#EMMO_1f1b164d_ec6a_4faa_8d5e_88bda62316cc> rdf:type owl:AnnotationProperty ;
                                                                                  rdfs:comment "URL to corresponing entity in QUDT."@en ;
                                                                                  rdfs:seeAlso "http://www.qudt.org/2.1/catalog/qudt-catalog.html"^^xsd:anyURI ;
                                                                                  <http://www.w3.org/2004/02/skos/core#prefLabel> "qudtEntry"@en .


###  http://emmo.info/emmo/top/annotations#EMMO_50c298c2_55a2_4068_b3ac_4e948c33181f
<http://emmo.info/emmo/top/annotations#EMMO_50c298c2_55a2_4068_b3ac_4e948c33181f> rdf:type owl:AnnotationProperty ;
                                                                                  rdfs:comment "URL to corresponding entry in the IEC Electropedia online database of ISO 80000 terms and definitions of quantities and units available at http://www.electropedia.org/."@en ;
                                                                                  rdfs:seeAlso "http://www.electropedia.org/"^^xsd:anyURI ;
                                                                                  <http://www.w3.org/2004/02/skos/core#prefLabel> "IECEntry"@en .


###  http://emmo.info/emmo/top/annotations#EMMO_6dd685dd_1895_46e4_b227_be9f7d643c25
<http://emmo.info/emmo/top/annotations#EMMO_6dd685dd_1895_46e4_b227_be9f7d643c25> rdf:type owl:AnnotationProperty ;
                                                                                  rdfs:comment "URL to corresponding concept in DBpedia."@en ;
                                                                                  rdfs:seeAlso "https://wiki.dbpedia.org/"^^xsd:anyURI ;
                                                                                  <http://www.w3.org/2004/02/skos/core#prefLabel> "dbpediaEntry"@en .


###  http://emmo.info/emmo/top/annotations#EMMO_70fe84ff_99b6_4206_a9fc_9a8931836d84
<http://emmo.info/emmo/top/annotations#EMMO_70fe84ff_99b6_4206_a9fc_9a8931836d84> rdf:type owl:AnnotationProperty ;
                                                                                  rdfs:comment "Human readable definition of a concept."@en ;
                                                                                  <http://www.w3.org/2004/02/skos/core#prefLabel> "definition"@en .


###  http://emmo.info/emmo/top/annotations#EMMO_8de5d5bf_db1c_40ac_b698_095ba3b18578
<http://emmo.info/emmo/top/annotations#EMMO_8de5d5bf_db1c_40ac_b698_095ba3b18578> rdf:type owl:AnnotationProperty ;
                                                                                  <http://emmo.info/emmo/top/annotations#EMMO_b432d2d5_25f4_4165_99c5_5935a7763c1a> "3-1.1  (refers to length)"@en ;
                                                                                  rdfs:comment "Corresponding item number in ISO 80 000."@en ;
                                                                                  rdfs:seeAlso "https://www.iso.org/obp/ui/#iso:std:iso:80000:-1:ed-1:v1:en"^^xsd:anyURI ;
                                                                                  <http://www.w3.org/2004/02/skos/core#prefLabel> "ISO80000Ref"@en .


###  http://emmo.info/emmo/top/annotations#EMMO_967080e5_2f42_4eb2_a3a9_c58143e835f9
<http://emmo.info/emmo/top/annotations#EMMO_967080e5_2f42_4eb2_a3a9_c58143e835f9> rdf:type owl:AnnotationProperty ;
                                                                                  rdfs:comment "Short enlightening explanation of a concept."@en ;
                                                                                  <http://www.w3.org/2004/02/skos/core#prefLabel> "elucidation"@en .


###  http://emmo.info/emmo/top/annotations#EMMO_a9b3d04c_7ceb_40a2_b8d3_28d514a770a8
<http://emmo.info/emmo/top/annotations#EMMO_a9b3d04c_7ceb_40a2_b8d3_28d514a770a8> rdf:type owl:AnnotationProperty ;
                                                                                  rdfs:comment "URL to CODATA Internationally recommended 2018 values of physical constants."@en ;
                                                                                  rdfs:seeAlso "https://physics.nist.gov/cuu/Constants/index.html"^^xsd:anyURI ;
                                                                                  <http://www.w3.org/2004/02/skos/core#prefLabel> "codataEntry"@en .


###  http://emmo.info/emmo/top/annotations#EMMO_b432d2d5_25f4_4165_99c5_5935a7763c1a
<http://emmo.info/emmo/top/annotations#EMMO_b432d2d5_25f4_4165_99c5_5935a7763c1a> rdf:type owl:AnnotationProperty ;
                                                                                  rdfs:comment "Illustrative example of how the entity is used."@en ;
                                                                                  <http://www.w3.org/2004/02/skos/core#prefLabel> "example"@en .


###  http://emmo.info/emmo/top/annotations#EMMO_c84c6752_6d64_48cc_9500_e54a3c34898d
<http://emmo.info/emmo/top/annotations#EMMO_c84c6752_6d64_48cc_9500_e54a3c34898d> rdf:type owl:AnnotationProperty ;
                                                                                  rdfs:comment "URL to corresponding Wikipedia entry."@en ;
                                                                                  rdfs:seeAlso "https://www.wikipedia.org/" ;
                                                                                  <http://www.w3.org/2004/02/skos/core#prefLabel> "wikipediaEntry"@en .


###  http://emmo.info/emmo/top/annotations#EMMO_e55f2d7c_9893_48cd_b4a4_fdf38253bd20
<http://emmo.info/emmo/top/annotations#EMMO_e55f2d7c_9893_48cd_b4a4_fdf38253bd20> rdf:type owl:AnnotationProperty ;
                                                                                  rdfs:comment "IRI to corresponding concept in the Ontology of units of Measure"@en ;
                                                                                  rdfs:seeAlso "https://enterpriseintegrationlab.github.io/icity/OM/doc/index-en.html"^^xsd:anyURI ,
                                                                                               "https://github.com/HajoRijgersberg/OM"^^xsd:anyURI ;
                                                                                  <http://www.w3.org/2004/02/skos/core#prefLabel> "omMatch"@en .


###  http://emmo.info/emmo/top/annotations#EMMO_fe015383_afb3_44a6_ae86_043628697aa2
<http://emmo.info/emmo/top/annotations#EMMO_fe015383_afb3_44a6_ae86_043628697aa2> rdf:type owl:AnnotationProperty ;
                                                                                  rdfs:comment "DOI to corresponding concept in IUPAC"@en ;
                                                                                  rdfs:seeAlso "https://goldbook.iupac.org/"^^xsd:anyURI ;
                                                                                  <http://www.w3.org/2004/02/skos/core#prefLabel> "iupacEntry"@en .


###  http://emmo.info/emmo/top/annotations#elucidation
<http://emmo.info/emmo/top/annotations#elucidation> rdf:type owl:AnnotationProperty .


###  http://purl.org/dc/terms/abstract
<http://purl.org/dc/terms/abstract> rdf:type owl:AnnotationProperty .


###  http://purl.org/dc/terms/contributor
<http://purl.org/dc/terms/contributor> rdf:type owl:AnnotationProperty .


###  http://purl.org/dc/terms/creator
<http://purl.org/dc/terms/creator> rdf:type owl:AnnotationProperty .


###  http://purl.org/dc/terms/license
<http://purl.org/dc/terms/license> rdf:type owl:AnnotationProperty .


###  http://purl.org/dc/terms/publisher
<http://purl.org/dc/terms/publisher> rdf:type owl:AnnotationProperty .


###  http://purl.org/dc/terms/title
<http://purl.org/dc/terms/title> rdf:type owl:AnnotationProperty .


###  http://www.w3.org/2000/01/rdf-schema#seeAlso
rdfs:seeAlso rdfs:comment """EMMO applies the naming convension to its sub-properties of rdfs:seeAlso that their label must end with one of the following terms:
  - 'Match': resolvable URLs to corresponding entity in another ontology
  - 'Entry': resolvable URLs to a human readable resource describing the subject
  - 'Ref': non-resolvable reference to a human readable resource describing the subject"""@en ,
                          "Indicate a resource that might provide additional information about the subject resource."@en .


###  http://www.w3.org/2002/07/owl#minQualifiedCardinality
owl:minQualifiedCardinality rdf:type owl:AnnotationProperty .


###  http://www.w3.org/2002/07/owl#qualifiedCardinality
owl:qualifiedCardinality rdf:type owl:AnnotationProperty .


###  http://www.w3.org/2004/02/skos/core#altLabel
<http://www.w3.org/2004/02/skos/core#altLabel> rdf:type owl:AnnotationProperty .


###  http://www.w3.org/2004/02/skos/core#prefLabel
<http://www.w3.org/2004/02/skos/core#prefLabel> rdf:type owl:AnnotationProperty .


#################################################################
#    Object Properties
#################################################################

###  http://emmo.info/emmo/domain/mechanical-testing#EMMO_a079cf37_e495_41f1_af01_d544e886eacb
<http://emmo.info/emmo/domain/mechanical-testing#EMMO_a079cf37_e495_41f1_af01_d544e886eacb> rdf:type owl:ObjectProperty ;
                                                                                            rdfs:subPropertyOf <http://emmo.info/emmo/middle/holistic#EMMO_c5aae418_1622_4d02_93c5_21159e28e6c1> ;
                                                                                            rdfs:comment "Relates a Process to its direct outputs." ;
                                                                                            <http://www.w3.org/2004/02/skos/core#prefLabel> "hasOutput"@en .


###  http://emmo.info/emmo/domain/mechanical-testing#EMMO_dc4c5477_e02e_40ac_b5a4_0d4e8e36c74d
<http://emmo.info/emmo/domain/mechanical-testing#EMMO_dc4c5477_e02e_40ac_b5a4_0d4e8e36c74d> rdf:type owl:ObjectProperty ;
                                                                                            rdfs:subPropertyOf <http://emmo.info/emmo/middle/holistic#EMMO_c5aae418_1622_4d02_93c5_21159e28e6c1> ;
                                                                                            rdfs:comment "Relates a process to its inputs." ;
                                                                                            <http://www.w3.org/2004/02/skos/core#prefLabel> "hasInput"@en .


###  http://emmo.info/emmo/middle/holistic#EMMO_ae2d1a96_bfa1_409a_a7d2_03d69e8a125a
<http://emmo.info/emmo/middle/holistic#EMMO_ae2d1a96_bfa1_409a_a7d2_03d69e8a125a> rdf:type owl:ObjectProperty ;
                                                                                  rdfs:subPropertyOf <http://emmo.info/emmo/top/mereotopology#EMMO_17e27c22_37e1_468c_9dd7_95e137f73e7f> ;
                                                                                  <http://emmo.info/emmo/top/annotations#EMMO_967080e5_2f42_4eb2_a3a9_c58143e835f9> "The relation between a process and an object participating to it."@en ;
                                                                                  rdfs:comment "Participation is a parthood relation: you must be part (and then be connected) of the process to contribute to it."@en ,
                                                                                               "Participation is not under direct parthood since a process is not strictly related to reductionism, but it's a way to categorize temporal regions by the interpreters."@en ;
                                                                                  <http://www.w3.org/2004/02/skos/core#prefLabel> "hasParticipant"@en .


###  http://emmo.info/emmo/middle/holistic#EMMO_c5aae418_1622_4d02_93c5_21159e28e6c1
<http://emmo.info/emmo/middle/holistic#EMMO_c5aae418_1622_4d02_93c5_21159e28e6c1> rdf:type owl:ObjectProperty ;
                                                                                  rdfs:subPropertyOf <http://emmo.info/emmo/middle/holistic#EMMO_ae2d1a96_bfa1_409a_a7d2_03d69e8a125a> ,
                                                                                                     <http://emmo.info/emmo/top/mereotopology#EMMO_9380ab64_0363_4804_b13f_3a8a94119a76> ;
                                                                                  <http://www.w3.org/2004/02/skos/core#prefLabel> "hasProperParticipant"@en .


###  http://emmo.info/emmo/middle/math#EMMO_3446e167_c576_49d6_846c_215bb8878a55
<http://emmo.info/emmo/middle/math#EMMO_3446e167_c576_49d6_846c_215bb8878a55> rdf:type owl:ObjectProperty ;
                                                                              rdfs:subPropertyOf <http://emmo.info/emmo/middle/semiotics#EMMO_eb3518bf_f799_4f9e_8c3e_ce59af11453b> ;
                                                                              <http://www.w3.org/2004/02/skos/core#prefLabel> "hasVariable"@en .


###  http://emmo.info/emmo/middle/metrology#EMMO_67fc0a36_8dcb_4ffa_9a43_31074efa3296
<http://emmo.info/emmo/middle/metrology#EMMO_67fc0a36_8dcb_4ffa_9a43_31074efa3296> rdf:type owl:ObjectProperty ;
                                                                                   rdfs:subPropertyOf <http://emmo.info/emmo/middle/reductionistic#EMMO_b2282816_b7a3_44c6_b2cb_3feff1ceb7fe> ;
                                                                                   rdfs:comment "Relates the physical quantity to its unit through spatial direct parthood."@en ;
                                                                                   owl:versionInfo """In EMMO version 1.0.0-alpha2, physical quantities used the hasReferenceUnit object property to relate them to their units via physical dimensionality. This was simplified in 1.0.0-alpha3 in order to make reasoning faster.

The restriction (e.g. for the physical quantity Length)

    Length hasReferenceUnit only (hasPhysicsDimension only LengthDimension)

was in 1.0.0-alpha3 changed to

    Length hasPhysicsDimension some LengthDimension

Likewise were the universal restrictions on the corresponding unit changed to excistential. E.g.

    Metre hasPhysicsDimension only LengthDimension

was changed to

    Metre hasPhysicsDimension some LengthDimension

The label of this class was also changed from PhysicsDimension to PhysicalDimension.""" ;
                                                                                   <http://www.w3.org/2004/02/skos/core#prefLabel> "hasReferenceUnit"@en .


###  http://emmo.info/emmo/middle/metrology#EMMO_8ef3cd6d_ae58_4a8d_9fc0_ad8f49015cd0
<http://emmo.info/emmo/middle/metrology#EMMO_8ef3cd6d_ae58_4a8d_9fc0_ad8f49015cd0> rdf:type owl:ObjectProperty ;
                                                                                   rdfs:subPropertyOf <http://emmo.info/emmo/middle/reductionistic#EMMO_b2282816_b7a3_44c6_b2cb_3feff1ceb7fe> ;
                                                                                   rdfs:comment "Relates a quantity to its reference unit through spatial direct parthood."@en ;
                                                                                   <http://www.w3.org/2004/02/skos/core#prefLabel> "hasQuantityValue"@en .


###  http://emmo.info/emmo/middle/metrology#EMMO_bed1d005_b04e_4a90_94cf_02bc678a8569
<http://emmo.info/emmo/middle/metrology#EMMO_bed1d005_b04e_4a90_94cf_02bc678a8569> rdf:type owl:ObjectProperty ;
                                                                                   rdfs:subPropertyOf <http://emmo.info/emmo/middle/properties#EMMO_e1097637_70d2_4895_973f_2396f04fa204> ;
                                                                                   <http://www.w3.org/2004/02/skos/core#prefLabel> "hasPhysicalDimension"@en .


###  http://emmo.info/emmo/middle/models#EMMO_24c71baf_6db6_48b9_86c8_8c70cf36db0c
<http://emmo.info/emmo/middle/models#EMMO_24c71baf_6db6_48b9_86c8_8c70cf36db0c> rdf:type owl:ObjectProperty ;
                                                                                rdfs:subPropertyOf <http://emmo.info/emmo/middle/semiotics#EMMO_39c3815d_8cae_4c8f_b2ff_eeba24bec455> ;
                                                                                <http://www.w3.org/2004/02/skos/core#prefLabel> "hasModel"@en .


###  http://emmo.info/emmo/middle/properties#EMMO_e1097637_70d2_4895_973f_2396f04fa204
<http://emmo.info/emmo/middle/properties#EMMO_e1097637_70d2_4895_973f_2396f04fa204> rdf:type owl:ObjectProperty ;
                                                                                    rdfs:subPropertyOf <http://emmo.info/emmo/middle/semiotics#EMMO_eb3518bf_f799_4f9e_8c3e_ce59af11453b> ;
                                                                                    <http://www.w3.org/2004/02/skos/core#prefLabel> "hasProperty"@en .


###  http://emmo.info/emmo/middle/reductionistic#EMMO_65a2c5b8_e4d8_4a51_b2f8_e55effc0547d
<http://emmo.info/emmo/middle/reductionistic#EMMO_65a2c5b8_e4d8_4a51_b2f8_e55effc0547d> rdf:type owl:ObjectProperty ;
                                                                                        rdfs:subPropertyOf <http://emmo.info/emmo/top/physical#EMMO_7afbed84_7593_4a23_bd88_9d9c6b04e8f6> ;
                                                                                        <http://www.w3.org/2004/02/skos/core#prefLabel> "hasTemporalDirectPart"@en .


###  http://emmo.info/emmo/middle/reductionistic#EMMO_663859e5_add3_4c9e_96fb_c99399de278d
<http://emmo.info/emmo/middle/reductionistic#EMMO_663859e5_add3_4c9e_96fb_c99399de278d> rdf:type owl:ObjectProperty ;
                                                                                        rdfs:subPropertyOf <http://emmo.info/emmo/top/physical#EMMO_6e046dd0_9634_4013_b2b1_9cc468087c83> ;
                                                                                        <http://www.w3.org/2004/02/skos/core#prefLabel> "hasSpatioTemporalDirectPart"@en .


###  http://emmo.info/emmo/middle/reductionistic#EMMO_b2282816_b7a3_44c6_b2cb_3feff1ceb7fe
<http://emmo.info/emmo/middle/reductionistic#EMMO_b2282816_b7a3_44c6_b2cb_3feff1ceb7fe> rdf:type owl:ObjectProperty ;
                                                                                        rdfs:subPropertyOf <http://emmo.info/emmo/top/physical#EMMO_f68030be_94b8_4c61_a161_886468558054> ;
                                                                                        <http://www.w3.org/2004/02/skos/core#prefLabel> "hasSpatialDirectPart"@en .


###  http://emmo.info/emmo/middle/semiotics#EMMO_2337e25c_3c60_43fc_a8f9_b11a3f974291
<http://emmo.info/emmo/middle/semiotics#EMMO_2337e25c_3c60_43fc_a8f9_b11a3f974291> rdf:type owl:ObjectProperty ;
                                                                                   rdfs:subPropertyOf <http://emmo.info/emmo/top/mereotopology#EMMO_ec2472ae_cf4a_46a5_8555_1556f5a6c3c5> ,
                                                                                                      [ owl:inverseOf <http://emmo.info/emmo/top/mereotopology#EMMO_ec2472ae_cf4a_46a5_8555_1556f5a6c3c5>
                                                                                                      ] ;
                                                                                   <http://emmo.info/emmo/top/annotations#EMMO_967080e5_2f42_4eb2_a3a9_c58143e835f9> "The generic EMMO semiotical relation."@en ;
                                                                                   <http://www.w3.org/2004/02/skos/core#prefLabel> "semiotical"@en .


###  http://emmo.info/emmo/middle/semiotics#EMMO_297999d6_c9e4_4262_9536_bd524d1c6e21
<http://emmo.info/emmo/middle/semiotics#EMMO_297999d6_c9e4_4262_9536_bd524d1c6e21> rdf:type owl:ObjectProperty ;
                                                                                   rdfs:subPropertyOf <http://emmo.info/emmo/middle/semiotics#EMMO_60577dea_9019_4537_ac41_80b0fb563d41> ;
                                                                                   <http://www.w3.org/2004/02/skos/core#prefLabel> "hasIndex"@en .


###  http://emmo.info/emmo/middle/semiotics#EMMO_39c3815d_8cae_4c8f_b2ff_eeba24bec455
<http://emmo.info/emmo/middle/semiotics#EMMO_39c3815d_8cae_4c8f_b2ff_eeba24bec455> rdf:type owl:ObjectProperty ;
                                                                                   rdfs:subPropertyOf <http://emmo.info/emmo/middle/semiotics#EMMO_60577dea_9019_4537_ac41_80b0fb563d41> ;
                                                                                   <http://www.w3.org/2004/02/skos/core#prefLabel> "hasIcon"@en .


###  http://emmo.info/emmo/middle/semiotics#EMMO_60577dea_9019_4537_ac41_80b0fb563d41
<http://emmo.info/emmo/middle/semiotics#EMMO_60577dea_9019_4537_ac41_80b0fb563d41> rdf:type owl:ObjectProperty ;
                                                                                   rdfs:subPropertyOf <http://emmo.info/emmo/middle/semiotics#EMMO_2337e25c_3c60_43fc_a8f9_b11a3f974291> ;
                                                                                   <http://www.w3.org/2004/02/skos/core#prefLabel> "hasSign"@en .


###  http://emmo.info/emmo/middle/semiotics#EMMO_7fb7fe7e_bdf9_4eeb_adad_e384dd5285c6
<http://emmo.info/emmo/middle/semiotics#EMMO_7fb7fe7e_bdf9_4eeb_adad_e384dd5285c6> rdf:type owl:ObjectProperty ;
                                                                                   rdfs:subPropertyOf <http://emmo.info/emmo/middle/semiotics#EMMO_60577dea_9019_4537_ac41_80b0fb563d41> ;
                                                                                   <http://www.w3.org/2004/02/skos/core#prefLabel> "hasInterpretant"@en .


###  http://emmo.info/emmo/middle/semiotics#EMMO_eb3518bf_f799_4f9e_8c3e_ce59af11453b
<http://emmo.info/emmo/middle/semiotics#EMMO_eb3518bf_f799_4f9e_8c3e_ce59af11453b> rdf:type owl:ObjectProperty ;
                                                                                   rdfs:subPropertyOf <http://emmo.info/emmo/middle/semiotics#EMMO_60577dea_9019_4537_ac41_80b0fb563d41> ;
                                                                                   <http://www.w3.org/2004/02/skos/core#prefLabel> "hasConvention"@en .


###  http://emmo.info/emmo/top/mereotopology#EMMO_03212fd7_abfd_4828_9c8e_62c293052d4b
<http://emmo.info/emmo/top/mereotopology#EMMO_03212fd7_abfd_4828_9c8e_62c293052d4b> rdf:type owl:ObjectProperty ;
                                                                                    rdfs:subPropertyOf <http://emmo.info/emmo/top/mereotopology#EMMO_ec2472ae_cf4a_46a5_8555_1556f5a6c3c5> ,
                                                                                                       [ owl:inverseOf <http://emmo.info/emmo/top/mereotopology#EMMO_ec2472ae_cf4a_46a5_8555_1556f5a6c3c5>
                                                                                                       ] ;
                                                                                    <http://emmo.info/emmo/top/annotations#EMMO_967080e5_2f42_4eb2_a3a9_c58143e835f9> "The superclass for all EMMO mereotopological relations."@en ;
                                                                                    rdfs:comment "Mereotopology merges mereological and topological concepts and provides relations between wholes, parts, boundaries, etc."@en ;
                                                                                    <http://www.w3.org/2004/02/skos/core#prefLabel> "mereotopological"@en .


###  http://emmo.info/emmo/top/mereotopology#EMMO_17e27c22_37e1_468c_9dd7_95e137f73e7f
<http://emmo.info/emmo/top/mereotopology#EMMO_17e27c22_37e1_468c_9dd7_95e137f73e7f> rdf:type owl:ObjectProperty ;
                                                                                    rdfs:subPropertyOf <http://emmo.info/emmo/top/mereotopology#EMMO_8c898653_1118_4682_9bbf_6cc334d16a99> ,
                                                                                                       <http://emmo.info/emmo/top/mereotopology#EMMO_d893d373_b579_4867_841e_1c2b31a8d2c6> ,
                                                                                                       [ owl:inverseOf <http://emmo.info/emmo/top/mereotopology#EMMO_d893d373_b579_4867_841e_1c2b31a8d2c6>
                                                                                                       ] ;
                                                                                    <http://www.w3.org/2004/02/skos/core#prefLabel> "hasPart"@en .


###  http://emmo.info/emmo/top/mereotopology#EMMO_4d6504f1_c470_4ce9_b941_bbbebc9ab05d
<http://emmo.info/emmo/top/mereotopology#EMMO_4d6504f1_c470_4ce9_b941_bbbebc9ab05d> rdf:type owl:ObjectProperty ;
                                                                                    rdfs:subPropertyOf <http://emmo.info/emmo/top/mereotopology#EMMO_6703954e_34c4_4a15_a9e7_f313760ae1a8> ,
                                                                                                       [ owl:inverseOf <http://emmo.info/emmo/top/mereotopology#EMMO_6703954e_34c4_4a15_a9e7_f313760ae1a8>
                                                                                                       ] ;
                                                                                    <http://www.w3.org/2004/02/skos/core#prefLabel> "hasContactWith"@en .


###  http://emmo.info/emmo/top/mereotopology#EMMO_517dfaf9_4970_41ac_81ee_d031627d2c7c
<http://emmo.info/emmo/top/mereotopology#EMMO_517dfaf9_4970_41ac_81ee_d031627d2c7c> rdf:type owl:ObjectProperty ;
                                                                                    rdfs:subPropertyOf <http://emmo.info/emmo/top/mereotopology#EMMO_03212fd7_abfd_4828_9c8e_62c293052d4b> ,
                                                                                                       [ owl:inverseOf <http://emmo.info/emmo/top/mereotopology#EMMO_03212fd7_abfd_4828_9c8e_62c293052d4b>
                                                                                                       ] ;
                                                                                    <http://www.w3.org/2004/02/skos/core#prefLabel> "disconnected"@en .


###  http://emmo.info/emmo/top/mereotopology#EMMO_6703954e_34c4_4a15_a9e7_f313760ae1a8
<http://emmo.info/emmo/top/mereotopology#EMMO_6703954e_34c4_4a15_a9e7_f313760ae1a8> rdf:type owl:ObjectProperty ;
                                                                                    rdfs:subPropertyOf <http://emmo.info/emmo/top/mereotopology#EMMO_03212fd7_abfd_4828_9c8e_62c293052d4b> ,
                                                                                                       [ owl:inverseOf <http://emmo.info/emmo/top/mereotopology#EMMO_03212fd7_abfd_4828_9c8e_62c293052d4b>
                                                                                                       ] ;
                                                                                    rdfs:comment "Causality is a topological property between connected items."@en ,
                                                                                                 "Items being connected means that there is a topological contact or \"interaction\" between them."@en ;
                                                                                    <http://www.w3.org/2004/02/skos/core#prefLabel> "connected"@en .


###  http://emmo.info/emmo/top/mereotopology#EMMO_6b7276a4_4b9d_440a_b577_0277539c0fc4
<http://emmo.info/emmo/top/mereotopology#EMMO_6b7276a4_4b9d_440a_b577_0277539c0fc4> rdf:type owl:ObjectProperty ;
                                                                                    rdfs:subPropertyOf <http://emmo.info/emmo/top/mereotopology#EMMO_9380ab64_0363_4804_b13f_3a8a94119a76> ;
                                                                                    <http://www.w3.org/2004/02/skos/core#prefLabel> "hasMember"@en .


###  http://emmo.info/emmo/top/mereotopology#EMMO_8c898653_1118_4682_9bbf_6cc334d16a99
<http://emmo.info/emmo/top/mereotopology#EMMO_8c898653_1118_4682_9bbf_6cc334d16a99> rdf:type owl:ObjectProperty ;
                                                                                    rdfs:subPropertyOf <http://emmo.info/emmo/top/mereotopology#EMMO_6703954e_34c4_4a15_a9e7_f313760ae1a8> ,
                                                                                                       [ owl:inverseOf <http://emmo.info/emmo/top/mereotopology#EMMO_6703954e_34c4_4a15_a9e7_f313760ae1a8>
                                                                                                       ] ;
                                                                                    rdfs:comment "Enclosure is reflexive and transitive."@en ;
                                                                                    <http://www.w3.org/2004/02/skos/core#prefLabel> "encloses"@en .


###  http://emmo.info/emmo/top/mereotopology#EMMO_9380ab64_0363_4804_b13f_3a8a94119a76
<http://emmo.info/emmo/top/mereotopology#EMMO_9380ab64_0363_4804_b13f_3a8a94119a76> rdf:type owl:ObjectProperty ;
                                                                                    rdfs:subPropertyOf <http://emmo.info/emmo/top/mereotopology#EMMO_17e27c22_37e1_468c_9dd7_95e137f73e7f> ;
                                                                                    <http://www.w3.org/2004/02/skos/core#prefLabel> "hasProperPart"@en .


###  http://emmo.info/emmo/top/mereotopology#EMMO_9cb984ca_48ad_4864_b09e_50d3fff19420
<http://emmo.info/emmo/top/mereotopology#EMMO_9cb984ca_48ad_4864_b09e_50d3fff19420> rdf:type owl:ObjectProperty ;
                                                                                    rdfs:subPropertyOf <http://emmo.info/emmo/top/mereotopology#EMMO_d893d373_b579_4867_841e_1c2b31a8d2c6> ,
                                                                                                       [ owl:inverseOf <http://emmo.info/emmo/top/mereotopology#EMMO_d893d373_b579_4867_841e_1c2b31a8d2c6>
                                                                                                       ] ;
                                                                                    <http://www.w3.org/2004/02/skos/core#prefLabel> "overcrosses"@en .


###  http://emmo.info/emmo/top/mereotopology#EMMO_d893d373_b579_4867_841e_1c2b31a8d2c6
<http://emmo.info/emmo/top/mereotopology#EMMO_d893d373_b579_4867_841e_1c2b31a8d2c6> rdf:type owl:ObjectProperty ;
                                                                                    rdfs:subPropertyOf <http://emmo.info/emmo/top/mereotopology#EMMO_6703954e_34c4_4a15_a9e7_f313760ae1a8> ,
                                                                                                       [ owl:inverseOf <http://emmo.info/emmo/top/mereotopology#EMMO_6703954e_34c4_4a15_a9e7_f313760ae1a8>
                                                                                                       ] ;
                                                                                    <http://www.w3.org/2004/02/skos/core#prefLabel> "hasOverlapWith"@en .


###  http://emmo.info/emmo/top/mereotopology#EMMO_ec2472ae_cf4a_46a5_8555_1556f5a6c3c5
<http://emmo.info/emmo/top/mereotopology#EMMO_ec2472ae_cf4a_46a5_8555_1556f5a6c3c5> rdf:type owl:ObjectProperty ;
                                                                                    <http://emmo.info/emmo/top/annotations#EMMO_967080e5_2f42_4eb2_a3a9_c58143e835f9> "The superclass for all relations used by the EMMO."@en ;
                                                                                    <http://www.w3.org/2004/02/skos/core#prefLabel> "EMMORelation"@en .


###  http://emmo.info/emmo/top/physical#EMMO_6e046dd0_9634_4013_b2b1_9cc468087c83
<http://emmo.info/emmo/top/physical#EMMO_6e046dd0_9634_4013_b2b1_9cc468087c83> rdf:type owl:ObjectProperty ;
                                                                               rdfs:subPropertyOf <http://emmo.info/emmo/top/mereotopology#EMMO_9380ab64_0363_4804_b13f_3a8a94119a76> ;
                                                                               <http://emmo.info/emmo/top/annotations#EMMO_967080e5_2f42_4eb2_a3a9_c58143e835f9> "A relation that isolates a proper part that extends itself in time through a portion of the lifetime whole." ;
                                                                               <http://www.w3.org/2004/02/skos/core#prefLabel> "hasSpatioTemporalPart"@en .


###  http://emmo.info/emmo/top/physical#EMMO_7afbed84_7593_4a23_bd88_9d9c6b04e8f6
<http://emmo.info/emmo/top/physical#EMMO_7afbed84_7593_4a23_bd88_9d9c6b04e8f6> rdf:type owl:ObjectProperty ;
                                                                               rdfs:subPropertyOf <http://emmo.info/emmo/top/mereotopology#EMMO_9380ab64_0363_4804_b13f_3a8a94119a76> ;
                                                                               <http://emmo.info/emmo/top/annotations#EMMO_967080e5_2f42_4eb2_a3a9_c58143e835f9> "A relation that isolate a proper part that covers the total spatial extension of a whole within a time interval." ;
                                                                               <http://www.w3.org/2004/02/skos/core#prefLabel> "hasTemporalPart"@en .


###  http://emmo.info/emmo/top/physical#EMMO_f68030be_94b8_4c61_a161_886468558054
<http://emmo.info/emmo/top/physical#EMMO_f68030be_94b8_4c61_a161_886468558054> rdf:type owl:ObjectProperty ;
                                                                               rdfs:subPropertyOf <http://emmo.info/emmo/top/mereotopology#EMMO_9380ab64_0363_4804_b13f_3a8a94119a76> ;
                                                                               <http://emmo.info/emmo/top/annotations#EMMO_967080e5_2f42_4eb2_a3a9_c58143e835f9> "A relation that isolates a proper part that extends itself in time within the overall lifetime of the whole, without covering the full spatial extension of the 4D whole (i.e. is not a temporal part)." ;
                                                                               <http://www.w3.org/2004/02/skos/core#prefLabel> "hasSpatialPart"@en .


#################################################################
#    Classes
#################################################################

###  http://emmo.info/emmo/domain/mechanical-testing#CableBundleUseCase
<http://emmo.info/emmo/domain/mechanical-testing#CableBundleUseCase> rdf:type owl:Class ;
                                                                     rdfs:subClassOf <http://emmo.info/emmo/domain/mechanical-testing#MechanicalTestingOntology> ;
                                                                     rdfs:comment "This is the artificial parent concept of the classes related to the Cable Bundle Use Case within this ontology." ;
                                                                     <http://www.w3.org/2004/02/skos/core#prefLabel> "CableBundleUseCase"@en .


###  http://emmo.info/emmo/domain/mechanical-testing#EMMO_0059f168_0cf0_4a84_8bab_ab313a2d27d7
<http://emmo.info/emmo/domain/mechanical-testing#EMMO_0059f168_0cf0_4a84_8bab_ab313a2d27d7> rdf:type owl:Class ;
                                                                                            rdfs:subClassOf <http://emmo.info/emmo/domain/mechanical-testing#EMMO_e5d45f40_f9e9_47b9_934b_4c463a38b08e> ,
                                                                                                            <http://emmo.info/emmo/middle/chemistry#EMMO_4f40def1_3cd7_4067_9596_541e9a5134cf> ;
                                                                                            <http://www.w3.org/2004/02/skos/core#prefLabel> "NiobiumSymbol"@en .


###  http://emmo.info/emmo/domain/mechanical-testing#EMMO_01751749_c384_4a73_b1f1_291447712a92
<http://emmo.info/emmo/domain/mechanical-testing#EMMO_01751749_c384_4a73_b1f1_291447712a92> rdf:type owl:Class ;
                                                                                            rdfs:subClassOf <http://emmo.info/emmo/domain/mechanical-testing#EMMO_e5d45f40_f9e9_47b9_934b_4c463a38b08e> ,
                                                                                                            <http://emmo.info/emmo/middle/math#EMMO_18d180e4_5e3e_42f7_820c_e08951223486> ,
                                                                                                            <http://emmo.info/emmo/middle/properties#EMMO_b7bcff25_ffc3_474e_9ab5_01b1664bd4ba> ;
                                                                                            rdfs:comment "Slope k of the SN curve in high cycle fatigue regime (HCF). High cycle fatigue is the range of fatigue life Nf between 10^4 and approximately 10^6 cycles (depending on the material)." ;
                                                                                            <http://www.w3.org/2004/02/skos/core#prefLabel> "SNCurveSlope"@en .


###  http://emmo.info/emmo/domain/mechanical-testing#EMMO_01a098aa_19c5_46f7_83bc_4dd01f8e0d4b
<http://emmo.info/emmo/domain/mechanical-testing#EMMO_01a098aa_19c5_46f7_83bc_4dd01f8e0d4b> rdf:type owl:Class ;
                                                                                            rdfs:subClassOf <http://emmo.info/emmo/domain/mechanical-testing#EMMO_442c0fb7_09d4_4dae_b45c_8eb1522da38f> ;
                                                                                            rdfs:comment "Method that performs multiple nanoindentation tests in different locations at extremely high- throughputs(2-5 s between one test and the subsequent)." ;
                                                                                            <http://www.w3.org/2004/02/skos/core#prefLabel> "HighSpeedNanoindentation"@en .


###  http://emmo.info/emmo/domain/mechanical-testing#EMMO_03dd3972_9de0_4872_a0f5_c6ff0cacf241
<http://emmo.info/emmo/domain/mechanical-testing#EMMO_03dd3972_9de0_4872_a0f5_c6ff0cacf241> rdf:type owl:Class ;
                                                                                            rdfs:subClassOf <http://emmo.info/emmo/domain/mechanical-testing#EMMO_7dc73553_7d3f_4dc2_bb7b_f47775207457> ,
                                                                                                            <http://emmo.info/emmo/domain/mechanical-testing#EMMO_f0ad542d_ff13_4998_9e7f_ea27583c5f31> ;
                                                                                            rdfs:comment "The modulus calculated from dynamics and the Oliver and Pharr method." ;
                                                                                            <http://www.w3.org/2004/02/skos/core#prefLabel> "DynamicModulus"@en .


###  http://emmo.info/emmo/domain/mechanical-testing#EMMO_03e264fd_ee9f_4ac0_a9f4_b0a975ddaded
<http://emmo.info/emmo/domain/mechanical-testing#EMMO_03e264fd_ee9f_4ac0_a9f4_b0a975ddaded> rdf:type owl:Class ;
                                                                                            rdfs:subClassOf <http://emmo.info/emmo/domain/mechanical-testing#NanoindentationUseCase> ,
                                                                                                            <http://emmo.info/emmo/middle/manufacturing#EMMO_494b372c_cfdf_47d3_a4de_5e037c540de8> ;
                                                                                            rdfs:comment "The hardware set consisting of the indenter column, indenter tip, the support springs, the displacement capacitive sensor, the actuation coil the metal case and the interface with the control electronics." ;
                                                                                            <http://www.w3.org/2004/02/skos/core#prefLabel> "IndenterHead"@en .


###  http://emmo.info/emmo/domain/mechanical-testing#EMMO_03ed6a50_3b04_4189_a939_dad066ece197
<http://emmo.info/emmo/domain/mechanical-testing#EMMO_03ed6a50_3b04_4189_a939_dad066ece197> rdf:type owl:Class ;
                                                                                            rdfs:subClassOf <http://emmo.info/emmo/domain/mechanical-testing#EMMO_91e9c813_b277_48ad_b5b0_a781a05b9c1f> ,
                                                                                                            <http://emmo.info/emmo/middle/isq#EMMO_d4f7d378_5e3b_468a_baa1_a7e98358cda7> ;
                                                                                            rdfs:comment "The time constant used to measure the Dynamic displacement (time over which the RMS value of the displacement is computed). Generally equivalent to at least five waves at the target frequency and being an integer number of waves. This dramatically reduces noise ." ;
                                                                                            <http://www.w3.org/2004/02/skos/core#prefLabel> "DynamicTimeConstant"@en .


###  http://emmo.info/emmo/domain/mechanical-testing#EMMO_04de9b50_35ef_4531_afbd_ded7ce5fffa1
<http://emmo.info/emmo/domain/mechanical-testing#EMMO_04de9b50_35ef_4531_afbd_ded7ce5fffa1> rdf:type owl:Class ;
                                                                                            rdfs:subClassOf <http://emmo.info/emmo/domain/mechanical-testing#EMMO_23273603_7ee7_4012_a0bb_d484433083de> ;
                                                                                            <http://www.w3.org/2004/02/skos/core#prefLabel> "StaircaseMethod" .


###  http://emmo.info/emmo/domain/mechanical-testing#EMMO_04f76b8a_0cb9_4a9e_8c94_dab5eb82d0e8
<http://emmo.info/emmo/domain/mechanical-testing#EMMO_04f76b8a_0cb9_4a9e_8c94_dab5eb82d0e8> rdf:type owl:Class ;
                                                                                            rdfs:subClassOf <http://emmo.info/emmo/domain/mechanical-testing#NanoindentationUseCase> ,
                                                                                                            <http://emmo.info/emmo/middle/materials#EMMO_7509da43_56b1_4d7f_887a_65d1663df4ba> ;
                                                                                            <http://www.w3.org/2004/02/skos/core#prefLabel> "LiquidDroplet"@en .


###  http://emmo.info/emmo/domain/mechanical-testing#EMMO_0527f1f8_41d4_4414_b1fa_8afbc8651ecb
<http://emmo.info/emmo/domain/mechanical-testing#EMMO_0527f1f8_41d4_4414_b1fa_8afbc8651ecb> rdf:type owl:Class ;
                                                                                            rdfs:subClassOf <http://emmo.info/emmo/domain/mechanical-testing#EMMO_e5d45f40_f9e9_47b9_934b_4c463a38b08e> ,
                                                                                                            <http://emmo.info/emmo/middle/isq#EMMO_ba882f34_0d71_4e4f_9d92_0c076c633a2c> ;
                                                                                            rdfs:comment "Number of cycles until the fatigue test stopped due to failure or run out." ;
                                                                                            <http://www.w3.org/2004/02/skos/core#prefLabel> "Cycles"@en .


###  http://emmo.info/emmo/domain/mechanical-testing#EMMO_05dbcd32_bdf0_44d2_94c4_78ea47fec79a
<http://emmo.info/emmo/domain/mechanical-testing#EMMO_05dbcd32_bdf0_44d2_94c4_78ea47fec79a> rdf:type owl:Class ;
                                                                                            rdfs:subClassOf <http://emmo.info/emmo/domain/mechanical-testing#CableBundleUseCase> ,
                                                                                                            <http://emmo.info/emmo/middle/metrology#EMMO_71f6ab56_342c_484b_bbe0_de86b7367cb3> ;
                                                                                            <http://emmo.info/emmo/middle/isq#physicalDimension> "T0 L-1 M+1 I0 T0 N0 J0" ;
                                                                                            rdfs:comment "The length density is a physical quantity that represents the is mass per unit length." ;
                                                                                            <http://www.w3.org/2004/02/skos/core#prefLabel> "LengthDensity"@en .


###  http://emmo.info/emmo/domain/mechanical-testing#EMMO_06390646_6edb_4410_b22b_f7adbd6025c4
<http://emmo.info/emmo/domain/mechanical-testing#EMMO_06390646_6edb_4410_b22b_f7adbd6025c4> rdf:type owl:Class ;
                                                                                            rdfs:subClassOf <http://emmo.info/emmo/domain/mechanical-testing#EMMO_e5d45f40_f9e9_47b9_934b_4c463a38b08e> ,
                                                                                                            <http://emmo.info/emmo/middle/perceptual#EMMO_c74da218_9147_4f03_92d1_8894abca55f3> ;
                                                                                            rdfs:comment "Microstructures are compositional/structural inhomogeneities that may consist of spatially distributed phases of different compositions/structures, grains of different orientations, structural defects." ;
                                                                                            <http://www.w3.org/2004/02/skos/core#prefLabel> "Microstructure"@en .


###  http://emmo.info/emmo/domain/mechanical-testing#EMMO_0747262d_9356_4b7b_ac5d_90e2504e0968
<http://emmo.info/emmo/domain/mechanical-testing#EMMO_0747262d_9356_4b7b_ac5d_90e2504e0968> rdf:type owl:Class ;
                                                                                            rdfs:subClassOf <http://emmo.info/emmo/domain/mechanical-testing#EMMO_f210d615_89a5_483f_a8b2_923ff6fcf4ab> ;
                                                                                            rdfs:comment "Bending test post processing is a generic class that holds for description of bending tests post-processing approaches." ;
                                                                                            <http://www.w3.org/2004/02/skos/core#prefLabel> "BendingTestPostProcessing"@en .


###  http://emmo.info/emmo/domain/mechanical-testing#EMMO_07696442_2e6d_416a_b4f0_81c4aff90de8
<http://emmo.info/emmo/domain/mechanical-testing#EMMO_07696442_2e6d_416a_b4f0_81c4aff90de8> rdf:type owl:Class ;
                                                                                            rdfs:subClassOf <http://emmo.info/emmo/domain/mechanical-testing#NanoindentationUseCase> ,
                                                                                                            <http://emmo.info/emmo/middle/manufacturing#EMMO_494b372c_cfdf_47d3_a4de_5e037c540de8> ,
                                                                                                            <http://emmo.info/emmo/middle/properties#EMMO_f2d5d3ad_2e00_417f_8849_686f3988d929> ;
                                                                                            <http://www.w3.org/2004/02/skos/core#prefLabel> "ContactAngleMeter"@en .


###  http://emmo.info/emmo/domain/mechanical-testing#EMMO_08cb5a5f_ae54_4ad0_a63f_8170f3852f02
<http://emmo.info/emmo/domain/mechanical-testing#EMMO_08cb5a5f_ae54_4ad0_a63f_8170f3852f02> rdf:type owl:Class ;
                                                                                            rdfs:subClassOf <http://emmo.info/emmo/domain/mechanical-testing#EMMO_c799b443_c70f_4351_bb0f_e4ab29073481> ;
                                                                                            rdfs:comment "Is a derived quantity that is determined using a standard Vickers Hardness test." ;
                                                                                            <http://www.w3.org/2004/02/skos/core#prefLabel> "VickersHardness"@en .


###  http://emmo.info/emmo/domain/mechanical-testing#EMMO_099c40dc_9ddb_4ee1_b7c8_1e14d9a19fbb
<http://emmo.info/emmo/domain/mechanical-testing#EMMO_099c40dc_9ddb_4ee1_b7c8_1e14d9a19fbb> rdf:type owl:Class ;
                                                                                            rdfs:subClassOf <http://emmo.info/emmo/domain/mechanical-testing#EMMO_2e9a014f_9337_42f7_ad91_b73f150a9901> ;
                                                                                            rdfs:comment "Induction hardening is a type of surface hardening in which a metal part is induction-heated and then quenched. The quenched metal undergoes a martensitic transformation, increasing the hardness and brittleness of the part. Induction hardening is used to selectively harden areas of a part or assembly without affecting the properties of the part as a whole." ;
                                                                                            <http://www.w3.org/2004/02/skos/core#prefLabel> "InductionHardening"@en .


###  http://emmo.info/emmo/domain/mechanical-testing#EMMO_09ed4e02_7485_425b_a9bc_a610b67d3ef8
<http://emmo.info/emmo/domain/mechanical-testing#EMMO_09ed4e02_7485_425b_a9bc_a610b67d3ef8> rdf:type owl:Class ;
                                                                                            rdfs:subClassOf <http://emmo.info/emmo/domain/mechanical-testing#EMMO_e32ab9e8_a962_42df_afc0_a45e1ec00e1b> ;
                                                                                            rdfs:comment """Steel category according to DIN standard:
Stainless steels with special additives (DIN 10027-2)""" ;
                                                                                            rdfs:label "Stainless steels with special additives (DIN 10027-2)"@en ;
                                                                                            <http://www.w3.org/2004/02/skos/core#prefLabel> "StainlessSteelsWithSpecialAdditivesDIN10027"@en .


###  http://emmo.info/emmo/domain/mechanical-testing#EMMO_0ae01f99_b2ed_4dd0_959d_60baad0ab475
<http://emmo.info/emmo/domain/mechanical-testing#EMMO_0ae01f99_b2ed_4dd0_959d_60baad0ab475> rdf:type owl:Class ;
                                                                                            rdfs:subClassOf <http://emmo.info/emmo/domain/mechanical-testing#NanoindentationUseCase> ,
                                                                                                            <http://emmo.info/emmo/middle/metrology#EMMO_79751276_b2d0_4e2f_bbd4_99d412f43d55> ;
                                                                                            rdfs:comment "The amplitude of the displacement value oscillation reading while in contact with the sample, with respect to its quasi static value." ;
                                                                                            <http://www.w3.org/2004/02/skos/core#prefLabel> "AmplitudeOfOscillatoryDepthReading"@en .


###  http://emmo.info/emmo/domain/mechanical-testing#EMMO_0b47a9ad_2854_43d0_9707_ff5f81f5b7d8
<http://emmo.info/emmo/domain/mechanical-testing#EMMO_0b47a9ad_2854_43d0_9707_ff5f81f5b7d8> rdf:type owl:Class ;
                                                                                            rdfs:subClassOf <http://emmo.info/emmo/domain/mechanical-testing#EMMO_3c7c1148_40e2_4ec2_a0ac_8720d03e356f> ;
                                                                                            <http://emmo.info/emmo/middle/isq#physicalDimension> "T-2 L+2 M+1 I0 T0 N0 J0" ;
                                                                                            <http://www.w3.org/2004/02/skos/core#prefLabel> "TorsionalStiffness"@en .


###  http://emmo.info/emmo/domain/mechanical-testing#EMMO_0ba19cad_5314_452c_9410_76183326694d
<http://emmo.info/emmo/domain/mechanical-testing#EMMO_0ba19cad_5314_452c_9410_76183326694d> rdf:type owl:Class ;
                                                                                            rdfs:subClassOf <http://emmo.info/emmo/domain/mechanical-testing#EMMO_2e9a014f_9337_42f7_ad91_b73f150a9901> ;
                                                                                            <http://www.w3.org/2004/02/skos/core#prefLabel> "BainiteHardening"@en .


###  http://emmo.info/emmo/domain/mechanical-testing#EMMO_0d41e0d2_f6d3_4d76_97b3_0367b546f492
<http://emmo.info/emmo/domain/mechanical-testing#EMMO_0d41e0d2_f6d3_4d76_97b3_0367b546f492> rdf:type owl:Class ;
                                                                                            rdfs:subClassOf <http://emmo.info/emmo/domain/mechanical-testing#EMMO_24af8df2_9438_44f6_8c5f_755beb459a49> ;
                                                                                            rdfs:comment "Corresponds to the Yield stress at 1% plastic strain." ;
                                                                                            <http://www.w3.org/2004/02/skos/core#prefLabel> "RP1.0"@en .


###  http://emmo.info/emmo/domain/mechanical-testing#EMMO_0d867829_e08b_46b4_9549_0e158d2b6a35
<http://emmo.info/emmo/domain/mechanical-testing#EMMO_0d867829_e08b_46b4_9549_0e158d2b6a35> rdf:type owl:Class ;
                                                                                            rdfs:subClassOf <http://emmo.info/emmo/domain/mechanical-testing#NanoindentationUseCase> ,
                                                                                                            <http://emmo.info/emmo/middle/properties#EMMO_463bcfda_867b_41d9_a967_211d4d437cfb> ;
                                                                                            <http://www.w3.org/2004/02/skos/core#prefLabel> "ContactAngleMeasurement"@en .


###  http://emmo.info/emmo/domain/mechanical-testing#EMMO_0d9c3564_5955_4804_9d96_dd15ff7ba441
<http://emmo.info/emmo/domain/mechanical-testing#EMMO_0d9c3564_5955_4804_9d96_dd15ff7ba441> rdf:type owl:Class ;
                                                                                            rdfs:subClassOf <http://emmo.info/emmo/domain/mechanical-testing#EMMO_3c93b3eb_f08f_4c25_940c_fac690e012c6> ;
                                                                                            rdfs:comment "Label secified following the Society of Automotive Engineers (SAE) standards." ;
                                                                                            <http://www.w3.org/2004/02/skos/core#prefLabel> "SAE"@en .


###  http://emmo.info/emmo/domain/mechanical-testing#EMMO_0e0b318d_d7f3_4d35_852c_9d4385019612
<http://emmo.info/emmo/domain/mechanical-testing#EMMO_0e0b318d_d7f3_4d35_852c_9d4385019612> rdf:type owl:Class ;
                                                                                            rdfs:subClassOf <http://emmo.info/emmo/domain/mechanical-testing#EMMO_e5d45f40_f9e9_47b9_934b_4c463a38b08e> ,
                                                                                                            <http://emmo.info/emmo/middle/isq#EMMO_cd2cd0de_e0cc_4ef1_b27e_2e88db027bac> ;
                                                                                            <http://www.w3.org/2004/02/skos/core#prefLabel> "Width"@en .


###  http://emmo.info/emmo/domain/mechanical-testing#EMMO_0e30b15f_1b1e_4ff7_8699_a2fffdbc80d2
<http://emmo.info/emmo/domain/mechanical-testing#EMMO_0e30b15f_1b1e_4ff7_8699_a2fffdbc80d2> rdf:type owl:Class ;
                                                                                            rdfs:subClassOf <http://emmo.info/emmo/domain/mechanical-testing#EMMO_bf5ed681_bd31_4994_a05b_85d1443d23b1> ;
                                                                                            <http://www.w3.org/2004/02/skos/core#prefLabel> "Nitration"@en .


###  http://emmo.info/emmo/domain/mechanical-testing#EMMO_0e559791_8595_4d85_b666_3d75baba8cc8
<http://emmo.info/emmo/domain/mechanical-testing#EMMO_0e559791_8595_4d85_b666_3d75baba8cc8> rdf:type owl:Class ;
                                                                                            rdfs:subClassOf <http://emmo.info/emmo/domain/mechanical-testing#EMMO_3c7c1148_40e2_4ec2_a0ac_8720d03e356f> ;
                                                                                            <http://emmo.info/emmo/middle/isq#physicalDimension> "T-2 L+2 M+1 I0 T0 N0 J0" ;
                                                                                            rdfs:comment "The value of the stiffness that takes into account the appropriate calculation for both dynamic and non-dynamic portions of the experiment." ;
                                                                                            <http://www.w3.org/2004/02/skos/core#prefLabel> "DynamicStiffness"@en .


###  http://emmo.info/emmo/domain/mechanical-testing#EMMO_0ece9cba_617c_4452_bbdc_1c564129e393
<http://emmo.info/emmo/domain/mechanical-testing#EMMO_0ece9cba_617c_4452_bbdc_1c564129e393> rdf:type owl:Class ;
                                                                                            rdfs:subClassOf <http://emmo.info/emmo/domain/mechanical-testing#EMMO_e3665cba_b1a8_4fcf_8194_493187fcd25a> ,
                                                                                                            <http://emmo.info/emmo/domain/mechanical-testing#EMMO_f210d615_89a5_483f_a8b2_923ff6fcf4ab> ;
                                                                                            <http://www.w3.org/2004/02/skos/core#prefLabel> "ContactAngleMeasurementPostProcessing"@en .


###  http://emmo.info/emmo/domain/mechanical-testing#EMMO_0edc8739_b8c7_4bcc_a37d_5cc02a2bd572
<http://emmo.info/emmo/domain/mechanical-testing#EMMO_0edc8739_b8c7_4bcc_a37d_5cc02a2bd572> rdf:type owl:Class ;
                                                                                            rdfs:subClassOf <http://emmo.info/emmo/domain/mechanical-testing#EMMO_06390646_6edb_4410_b22b_f7adbd6025c4> ;
                                                                                            rdfs:comment "In iron and steelmetallurgy,ledeburiteis a mixture of 4.3% carbon in iron and is aeutecticmixture ofausteniteandcementite. Ledeburite is not a type ofsteelas the carbon level is too high although it may occur as a separate constituent in some high carbon steels. It is mostly found with cementite orpearlitein a range of cast irons." ;
                                                                                            rdfs:label "Ledeburite"@en ;
                                                                                            <http://www.w3.org/2004/02/skos/core#prefLabel> "Ledeburite" .


###  http://emmo.info/emmo/domain/mechanical-testing#EMMO_0f73321c_c4fd_40ed_9b58_eccd9b7d8e15
<http://emmo.info/emmo/domain/mechanical-testing#EMMO_0f73321c_c4fd_40ed_9b58_eccd9b7d8e15> rdf:type owl:Class ;
                                                                                            rdfs:subClassOf <http://emmo.info/emmo/domain/mechanical-testing#NanoindentationUseCase> ,
                                                                                                            <http://emmo.info/emmo/middle/holistic#EMMO_43e9a05d_98af_41b4_92f6_00f79a09bfce> ;
                                                                                            rdfs:comment "Represents a Process (or the sequence of processes) by which the metrological chain is defined or in other words a full recipe describing the workflow of an entire indentation experiment." ;
                                                                                            <http://www.w3.org/2004/02/skos/core#prefLabel> "Method"@en .


###  http://emmo.info/emmo/domain/mechanical-testing#EMMO_10e7f26e_4cb6_4fb8_84e8_f90fec466e75
<http://emmo.info/emmo/domain/mechanical-testing#EMMO_10e7f26e_4cb6_4fb8_84e8_f90fec466e75> rdf:type owl:Class ;
                                                                                            rdfs:subClassOf <http://emmo.info/emmo/domain/mechanical-testing#EMMO_91e9c813_b277_48ad_b5b0_a781a05b9c1f> ,
                                                                                                            <http://emmo.info/emmo/middle/isq#EMMO_d4f7d378_5e3b_468a_baa1_a7e98358cda7> ;
                                                                                            rdfs:comment "The time over which the drift rate is measured." ;
                                                                                            <http://www.w3.org/2004/02/skos/core#prefLabel> "DriftDeterminationTime"@en .


###  http://emmo.info/emmo/domain/mechanical-testing#EMMO_10f4d440_33d0_456d_b27c_83bf1d9811c0
<http://emmo.info/emmo/domain/mechanical-testing#EMMO_10f4d440_33d0_456d_b27c_83bf1d9811c0> rdf:type owl:Class ;
                                                                                            rdfs:subClassOf <http://emmo.info/emmo/domain/mechanical-testing#CableBundleUseCase> ,
                                                                                                            <http://emmo.info/emmo/middle/properties#EMMO_463bcfda_867b_41d9_a967_211d4d437cfb> ;
                                                                                            rdfs:comment "Bending measurement is a measurement that follows a bending test method and is carried out for testing materials in terms of their bending strength and other important properties." ;
                                                                                            <http://www.w3.org/2004/02/skos/core#prefLabel> "BendingMeasurement"@en .


###  http://emmo.info/emmo/domain/mechanical-testing#EMMO_12c76f15_6daa_43a9_b535_c2df84dbf9e1
<http://emmo.info/emmo/domain/mechanical-testing#EMMO_12c76f15_6daa_43a9_b535_c2df84dbf9e1> rdf:type owl:Class ;
                                                                                            rdfs:subClassOf <http://emmo.info/emmo/domain/mechanical-testing#EMMO_e5d45f40_f9e9_47b9_934b_4c463a38b08e> ,
                                                                                                            <http://emmo.info/emmo/middle/chemistry#EMMO_4f40def1_3cd7_4067_9596_541e9a5134cf> ;
                                                                                            <http://www.w3.org/2004/02/skos/core#prefLabel> "CobaltSymbol"@en .


###  http://emmo.info/emmo/domain/mechanical-testing#EMMO_12e5e93b_764f_476f_8532_7aab62291399
<http://emmo.info/emmo/domain/mechanical-testing#EMMO_12e5e93b_764f_476f_8532_7aab62291399> rdf:type owl:Class ;
                                                                                            rdfs:subClassOf <http://emmo.info/emmo/domain/mechanical-testing#EMMO_e5d45f40_f9e9_47b9_934b_4c463a38b08e> ,
                                                                                                            <http://emmo.info/emmo/middle/isq#EMMO_acf636d4_9ac2_4ce3_960a_d54338e6cae3> ;
                                                                                            <http://www.w3.org/2004/02/skos/core#prefLabel> "FatigueStrain"@en .


###  http://emmo.info/emmo/domain/mechanical-testing#EMMO_13a8ef22_4ade_4c89_af34_0b4c7044517d
<http://emmo.info/emmo/domain/mechanical-testing#EMMO_13a8ef22_4ade_4c89_af34_0b4c7044517d> rdf:type owl:Class ;
                                                                                            rdfs:subClassOf <http://emmo.info/emmo/domain/mechanical-testing#EMMO_e5d45f40_f9e9_47b9_934b_4c463a38b08e> ,
                                                                                                            <http://emmo.info/emmo/middle/isq#EMMO_d1917609_db5e_4b8a_9b76_ef1d6f860a81> ;
                                                                                            rdfs:comment "The mean stress S_m is the averaged value of the stresses during fatigue testing (S_m = (S_min + S_max)/2)." ;
                                                                                            <http://www.w3.org/2004/02/skos/core#prefLabel> "MeanStress"@en .


###  http://emmo.info/emmo/domain/mechanical-testing#EMMO_142c4b97_9011_4608_849b_08d1fdd642ce
<http://emmo.info/emmo/domain/mechanical-testing#EMMO_142c4b97_9011_4608_849b_08d1fdd642ce> rdf:type owl:Class ;
                                                                                            rdfs:subClassOf <http://emmo.info/emmo/domain/mechanical-testing#EMMO_e5d45f40_f9e9_47b9_934b_4c463a38b08e> ,
                                                                                                            <http://emmo.info/emmo/middle/isq#EMMO_d1917609_db5e_4b8a_9b76_ef1d6f860a81> ;
                                                                                            rdfs:comment "Residual stresses are stresses that remain in a solid material after the original cause of the stresses has been removed." ;
                                                                                            <http://www.w3.org/2004/02/skos/core#prefLabel> "ResidualStress"@en .


###  http://emmo.info/emmo/domain/mechanical-testing#EMMO_1481b773_15d8_4f1a_bf37_3a704958c9d3
<http://emmo.info/emmo/domain/mechanical-testing#EMMO_1481b773_15d8_4f1a_bf37_3a704958c9d3> rdf:type owl:Class ;
                                                                                            rdfs:subClassOf <http://emmo.info/emmo/domain/mechanical-testing#EMMO_3c93b3eb_f08f_4c25_940c_fac690e012c6> ;
                                                                                            <http://emmo.info/emmo/top/annotations#EMMO_967080e5_2f42_4eb2_a3a9_c58143e835f9> "Label after DIN EN 10027-2. This label is the unique material number. Applies only if the material is defined according to DIN standard. For other standards, this cell is left empty." ;
                                                                                            rdfs:comment "European Standards (abbreviated ENs owing to the more literal translation from French/German as European Norms)" ;
                                                                                            rdfs:seeAlso "https://www.beuth.de/en/standard/din-en-10027-2/223407681" ;
                                                                                            <http://www.w3.org/2004/02/skos/core#prefLabel> "MaterialNumber"@en .


###  http://emmo.info/emmo/domain/mechanical-testing#EMMO_167562c3_4474_40a1_a07d_5ec8e21f3fef
<http://emmo.info/emmo/domain/mechanical-testing#EMMO_167562c3_4474_40a1_a07d_5ec8e21f3fef> rdf:type owl:Class ;
                                                                                            rdfs:subClassOf <http://emmo.info/emmo/domain/mechanical-testing#EMMO_e5d45f40_f9e9_47b9_934b_4c463a38b08e> ,
                                                                                                            <http://emmo.info/emmo/middle/properties#EMMO_463bcfda_867b_41d9_a967_211d4d437cfb> ;
                                                                                            <http://www.w3.org/2004/02/skos/core#prefLabel> "ChemicalCompositionMeasurement"@en .


###  http://emmo.info/emmo/domain/mechanical-testing#EMMO_169db6cf_3388_48f6_8d13_3848f69f84a5
<http://emmo.info/emmo/domain/mechanical-testing#EMMO_169db6cf_3388_48f6_8d13_3848f69f84a5> rdf:type owl:Class ;
                                                                                            rdfs:subClassOf <http://emmo.info/emmo/domain/mechanical-testing#EMMO_8e959570_c1a5_436f_bc54_08b423f4568d> ;
                                                                                            rdfs:comment "Vacuum arc remelting (VAR) is a secondary melting process for production of metal ingots with elevated chemical and mechanical homogeneity for highly demanding applications. The alloy to undergo VAR is formed into a cylinder typically by vacuum induction melting (VIM)." ;
                                                                                            <http://www.w3.org/2004/02/skos/core#prefLabel> "VIMVAR" .


###  http://emmo.info/emmo/domain/mechanical-testing#EMMO_16b98788_0d34_47d8_9cec_91511a9ef000
<http://emmo.info/emmo/domain/mechanical-testing#EMMO_16b98788_0d34_47d8_9cec_91511a9ef000> rdf:type owl:Class ;
                                                                                            rdfs:subClassOf <http://emmo.info/emmo/domain/mechanical-testing#EMMO_c8e9f573_1b9a_48f6_a274_61a441f3a7c4> ;
                                                                                            rdfs:comment """Steel category according to JIS standard:
High speed tool steels (JIS)""" ;
                                                                                            rdfs:label "High speed tool steels (JIS)"@en ;
                                                                                            <http://www.w3.org/2004/02/skos/core#prefLabel> "HighSpeedToolSteelsJIS"@en .


###  http://emmo.info/emmo/domain/mechanical-testing#EMMO_16cfb313_1fea_414f_99ca_aec999e93e0c
<http://emmo.info/emmo/domain/mechanical-testing#EMMO_16cfb313_1fea_414f_99ca_aec999e93e0c> rdf:type owl:Class ;
                                                                                            rdfs:subClassOf <http://emmo.info/emmo/middle/chemistry#EMMO_abf7efbe_6b04_41b8_8326_4dd0f6be753e> ;
                                                                                            rdfs:comment "Steel nomenclature contains steel groups / categories as defined in the standards DIN, SAE and JIS and superclasses in which the categories from the different standards are combined" ;
                                                                                            rdfs:label "SteelNomenclature"@en ;
                                                                                            <http://www.w3.org/2004/02/skos/core#prefLabel> "SteelNomenclature"@en .


###  http://emmo.info/emmo/domain/mechanical-testing#EMMO_16d31733_248f_4e55_b870_dfc96d3e2c3b
<http://emmo.info/emmo/domain/mechanical-testing#EMMO_16d31733_248f_4e55_b870_dfc96d3e2c3b> rdf:type owl:Class ;
                                                                                            rdfs:subClassOf <http://emmo.info/emmo/domain/mechanical-testing#EMMO_e5d45f40_f9e9_47b9_934b_4c463a38b08e> ,
                                                                                                            <http://emmo.info/emmo/middle/perceptual#EMMO_89a0c87c_0804_4013_937a_6fe234d9499c> ;
                                                                                            <http://www.w3.org/2004/02/skos/core#prefLabel> "DataSet"@en .


###  http://emmo.info/emmo/domain/mechanical-testing#EMMO_1834f628_a7ad_460a_b858_3112c906ef00
<http://emmo.info/emmo/domain/mechanical-testing#EMMO_1834f628_a7ad_460a_b858_3112c906ef00> rdf:type owl:Class ;
                                                                                            rdfs:subClassOf <http://emmo.info/emmo/domain/mechanical-testing#EMMO_e5d45f40_f9e9_47b9_934b_4c463a38b08e> ,
                                                                                                            <http://emmo.info/emmo/middle/chemistry#EMMO_4f40def1_3cd7_4067_9596_541e9a5134cf> ;
                                                                                            <http://www.w3.org/2004/02/skos/core#prefLabel> "BerylliumSymbol"@en .


###  http://emmo.info/emmo/domain/mechanical-testing#EMMO_18be2e24_9665_4349_8dd3_6335c921a0ef
<http://emmo.info/emmo/domain/mechanical-testing#EMMO_18be2e24_9665_4349_8dd3_6335c921a0ef> rdf:type owl:Class ;
                                                                                            rdfs:subClassOf <http://emmo.info/emmo/domain/mechanical-testing#EMMO_ee09aa64_f477_4e8f_8b0c_f5d30177ba8d> ;
                                                                                            rdfs:comment "The depth of the indentation when dynamics are in use. It is the zeroed value of the Filtered Displacement corrected for load frame stiffness, drift rate and the Dynamic Displacement. It is zero prior to surface detection." ;
                                                                                            <http://www.w3.org/2004/02/skos/core#prefLabel> "FilteredDepthWithDynamics"@en .


###  http://emmo.info/emmo/domain/mechanical-testing#EMMO_197b6afe_74cb_41bd_83a4_54fda6bea1e4
<http://emmo.info/emmo/domain/mechanical-testing#EMMO_197b6afe_74cb_41bd_83a4_54fda6bea1e4> rdf:type owl:Class ;
                                                                                            rdfs:subClassOf <http://emmo.info/emmo/domain/mechanical-testing#EMMO_da87d0e5_8e93_4fc3_81b9_53f8568d4cc4> ;
                                                                                            rdfs:comment "A pore is a very small opening, cavity or depression. Pores occur in metals during melting and casting processes. Gases dissolved in the melt still escape while the melt solidifies, so the gas bubbles remain trapped and form pores in the material." ;
                                                                                            <http://www.w3.org/2004/02/skos/core#prefLabel> "Pore"@en .


###  http://emmo.info/emmo/domain/mechanical-testing#EMMO_19afc39b_eb5c_46e0_b880_8e08ec831ebc
<http://emmo.info/emmo/domain/mechanical-testing#EMMO_19afc39b_eb5c_46e0_b880_8e08ec831ebc> rdf:type owl:Class ;
                                                                                            rdfs:subClassOf <http://emmo.info/emmo/domain/mechanical-testing#EMMO_a30a7cdc_f652_4b01_b8c2_cd056f3e3d85> ;
                                                                                            <http://www.w3.org/2004/02/skos/core#prefLabel> "IndentationMachine"@en .


###  http://emmo.info/emmo/domain/mechanical-testing#EMMO_19d0ed3f_38b8_4879_9ba1_7ce54c8443fd
<http://emmo.info/emmo/domain/mechanical-testing#EMMO_19d0ed3f_38b8_4879_9ba1_7ce54c8443fd> rdf:type owl:Class ;
                                                                                            rdfs:subClassOf <http://emmo.info/emmo/domain/mechanical-testing#EMMO_8e959570_c1a5_436f_bc54_08b423f4568d> ;
                                                                                            rdfs:comment "Spray forming, also known as spray casting, is a method of casting near net shape metal components with homogeneous microstructures via the deposition of semi-solid sprayed droplets onto a shaped substrate. The spray-forming subprocess is part of the metallurgy process and has the output material after spray-forming." ;
                                                                                            <http://www.w3.org/2004/02/skos/core#prefLabel> "SprayForming" .


###  http://emmo.info/emmo/domain/mechanical-testing#EMMO_1a019aef_e953_46dc_86c3_b70aa159ba59
<http://emmo.info/emmo/domain/mechanical-testing#EMMO_1a019aef_e953_46dc_86c3_b70aa159ba59> rdf:type owl:Class ;
                                                                                            rdfs:subClassOf <http://emmo.info/emmo/domain/mechanical-testing#EMMO_e5d45f40_f9e9_47b9_934b_4c463a38b08e> ,
                                                                                                            <http://emmo.info/emmo/middle/semiotics#EMMO_6f5af708_f825_4feb_a0d1_a8d813d3022b> ;
                                                                                            <http://www.w3.org/2004/02/skos/core#prefLabel> "SpecimenNotch"@en .


###  http://emmo.info/emmo/domain/mechanical-testing#EMMO_1afcac36_c92e_439b_a4e2_ed24fc6c60d4
<http://emmo.info/emmo/domain/mechanical-testing#EMMO_1afcac36_c92e_439b_a4e2_ed24fc6c60d4> rdf:type owl:Class ;
                                                                                            rdfs:subClassOf <http://emmo.info/emmo/domain/mechanical-testing#EMMO_e8c8c152_484e_4053_8e35_82346b3fc927> ;
                                                                                            <http://www.w3.org/2004/02/skos/core#prefLabel> "ElongatedCrossSection"@en .


###  http://emmo.info/emmo/domain/mechanical-testing#EMMO_1b0a92ef_c509_40ee_8abe_408181aafaad
<http://emmo.info/emmo/domain/mechanical-testing#EMMO_1b0a92ef_c509_40ee_8abe_408181aafaad> rdf:type owl:Class ;
                                                                                            rdfs:subClassOf <http://emmo.info/emmo/domain/mechanical-testing#CableBundleUseCase> ,
                                                                                                            <http://emmo.info/emmo/domain/mechanical-testing#EMMO_e5d45f40_f9e9_47b9_934b_4c463a38b08e> ,
                                                                                                            <http://emmo.info/emmo/domain/mechanical-testing#NanoindentationUseCase> ,
                                                                                                            <http://emmo.info/emmo/middle/manufacturing#EMMO_494b372c_cfdf_47d3_a4de_5e037c540de8> ,
                                                                                                            <http://emmo.info/emmo/middle/properties#EMMO_f2d5d3ad_2e00_417f_8849_686f3988d929> ;
                                                                                            <http://www.w3.org/2004/02/skos/core#prefLabel> "TestingMachine"@en .


###  http://emmo.info/emmo/domain/mechanical-testing#EMMO_1cbdb7f5_47e4_468a_8d87_b25093803b8e
<http://emmo.info/emmo/domain/mechanical-testing#EMMO_1cbdb7f5_47e4_468a_8d87_b25093803b8e> rdf:type owl:Class ;
                                                                                            rdfs:subClassOf <http://emmo.info/emmo/domain/mechanical-testing#EMMO_535baaec_5360_48e8_ada4_72c6e6848957> ;
                                                                                            <http://www.w3.org/2004/02/skos/core#prefLabel> "MechanicalTestingSpecimen"@en .


###  http://emmo.info/emmo/domain/mechanical-testing#EMMO_1f213db4_5e4d_45d3_963e_8b7c7693707b
<http://emmo.info/emmo/domain/mechanical-testing#EMMO_1f213db4_5e4d_45d3_963e_8b7c7693707b> rdf:type owl:Class ;
                                                                                            rdfs:subClassOf <http://emmo.info/emmo/domain/mechanical-testing#EMMO_cc6faafc_5942_4724_9af8_14c2be17a64a> ;
                                                                                            rdfs:comment "{1..N} Elements the inclusion consists of." ;
                                                                                            <http://www.w3.org/2004/02/skos/core#prefLabel> "InclusionElements"@en .


###  http://emmo.info/emmo/domain/mechanical-testing#EMMO_1f2e03be_012a_4560_9d1b_417f530fdf3b
<http://emmo.info/emmo/domain/mechanical-testing#EMMO_1f2e03be_012a_4560_9d1b_417f530fdf3b> rdf:type owl:Class ;
                                                                                            rdfs:subClassOf <http://emmo.info/emmo/domain/mechanical-testing#EMMO_c21ab500_db9a_43a3_a7ef_d43fb64bf856> ;
                                                                                            rdfs:comment "A digital object identifier represents a persistent identifier or handle used to identify objects uniquely, standardized by the International Organization for Standardization (ISO)." ;
                                                                                            rdfs:seeAlso "https://www.iso.org/obp/ui/#iso:std:iso:26324:ed-1:v1:en" ;
                                                                                            <http://www.w3.org/2004/02/skos/core#prefLabel> "DigitalObjectIdentifier"@en .


###  http://emmo.info/emmo/domain/mechanical-testing#EMMO_207b3e76_c121_47f6_8278_7871292ce73f
<http://emmo.info/emmo/domain/mechanical-testing#EMMO_207b3e76_c121_47f6_8278_7871292ce73f> rdf:type owl:Class ;
                                                                                            rdfs:subClassOf <http://emmo.info/emmo/domain/mechanical-testing#EMMO_e5d45f40_f9e9_47b9_934b_4c463a38b08e> ,
                                                                                                            <http://emmo.info/emmo/middle/properties#EMMO_463bcfda_867b_41d9_a967_211d4d437cfb> ;
                                                                                            rdfs:comment """Mechanical testing covers a wide range of tests, which can be divided broadly into two types:
1. those that aim to determine a material's mechanical properties, independent of geometry.
2. those that determine the response of a structure to a given action, e.g. testing of composite beams, aircraft structures to destruction, etc.""" ;
                                                                                            <http://www.w3.org/2004/02/skos/core#prefLabel> "MechanicalTesting"@en .


###  http://emmo.info/emmo/domain/mechanical-testing#EMMO_21d06317_5b59_4940_8d02_804279fe07ad
<http://emmo.info/emmo/domain/mechanical-testing#EMMO_21d06317_5b59_4940_8d02_804279fe07ad> rdf:type owl:Class ;
                                                                                            rdfs:subClassOf <http://emmo.info/emmo/domain/mechanical-testing#EMMO_1cbdb7f5_47e4_468a_8d87_b25093803b8e> ;
                                                                                            rdfs:comment "UnnotchedSpecimen is a MechanicalTestingSpecimen that has homogeneous. An unnotched specimen has a stress concentration factor equal to 1." ;
                                                                                            <http://www.w3.org/2004/02/skos/core#prefLabel> "UnnotchedSpecimen"@en .


###  http://emmo.info/emmo/domain/mechanical-testing#EMMO_23273603_7ee7_4012_a0bb_d484433083de
<http://emmo.info/emmo/domain/mechanical-testing#EMMO_23273603_7ee7_4012_a0bb_d484433083de> rdf:type owl:Class ;
                                                                                            rdfs:subClassOf <http://emmo.info/emmo/domain/mechanical-testing#EMMO_207b3e76_c121_47f6_8278_7871292ce73f> ;
                                                                                            rdfs:comment "Fatigue testing is a specialised form of mechanical testing that is performed by applying cyclic loading to a coupon or structure. These tests are used either to generate fatigue life and crack growth data, identify critical locations or demonstrate the safety of a structure that may be susceptible to fatigue." ;
                                                                                            <http://www.w3.org/2004/02/skos/core#prefLabel> "FatigueTesting"@en .


###  http://emmo.info/emmo/domain/mechanical-testing#EMMO_24af8df2_9438_44f6_8c5f_755beb459a49
<http://emmo.info/emmo/domain/mechanical-testing#EMMO_24af8df2_9438_44f6_8c5f_755beb459a49> rdf:type owl:Class ;
                                                                                            rdfs:subClassOf <http://emmo.info/emmo/domain/mechanical-testing#EMMO_e5d45f40_f9e9_47b9_934b_4c463a38b08e> ,
                                                                                                            <http://emmo.info/emmo/middle/isq#EMMO_d1917609_db5e_4b8a_9b76_ef1d6f860a81> ;
                                                                                            rdfs:comment "The Yield Point also known by by yield stress or yield strength corresponds to the stress above which the material starts deforming plastically. It indicates the limit of elastic behaviour and the beginning of plastic behaviour." ;
                                                                                            <http://www.w3.org/2004/02/skos/core#prefLabel> "YieldPoint"@en .


###  http://emmo.info/emmo/domain/mechanical-testing#EMMO_25dd29ab_7e1e_46a0_b565_5ea5a9c7bed3
<http://emmo.info/emmo/domain/mechanical-testing#EMMO_25dd29ab_7e1e_46a0_b565_5ea5a9c7bed3> rdf:type owl:Class ;
                                                                                            rdfs:subClassOf <http://emmo.info/emmo/domain/mechanical-testing#EMMO_06390646_6edb_4410_b22b_f7adbd6025c4> ;
                                                                                            rdfs:comment "Ferrite or alpha-ferrite isa body-centered cubic structure phase of iron which exists below temperatures of 912C for low concentrations of carbon in iron." ;
                                                                                            rdfs:label "Ferrite"@en ;
                                                                                            <http://www.w3.org/2004/02/skos/core#prefLabel> "Ferrite" .


###  http://emmo.info/emmo/domain/mechanical-testing#EMMO_26707f23_c0f3_462a_91d7_5db51cd14cf4
<http://emmo.info/emmo/domain/mechanical-testing#EMMO_26707f23_c0f3_462a_91d7_5db51cd14cf4> rdf:type owl:Class ;
                                                                                            rdfs:subClassOf <http://emmo.info/emmo/domain/mechanical-testing#EMMO_e5d45f40_f9e9_47b9_934b_4c463a38b08e> ,
                                                                                                            <http://emmo.info/emmo/middle/siunits#EMMO_d41ce84b_4317_41fb_a5d1_6cd281fca106> ;
                                                                                            <http://www.w3.org/2004/02/skos/core#prefLabel> "MegaPascal"@en .


###  http://emmo.info/emmo/domain/mechanical-testing#EMMO_26708d5b_4bf7_4059_969f_3ba03c587051
<http://emmo.info/emmo/domain/mechanical-testing#EMMO_26708d5b_4bf7_4059_969f_3ba03c587051> rdf:type owl:Class ;
                                                                                            rdfs:subClassOf <http://emmo.info/emmo/domain/mechanical-testing#EMMO_442c0fb7_09d4_4dae_b45c_8eb1522da38f> ;
                                                                                            rdfs:comment "A method that is fully compliant with ISO 14577 standard." ;
                                                                                            <http://www.w3.org/2004/02/skos/core#prefLabel> "StandardNanoindentationMeasurementMethod"@en .


###  http://emmo.info/emmo/domain/mechanical-testing#EMMO_2697e9d2_e173_411c_8c4b_2b400ab6b1b9
<http://emmo.info/emmo/domain/mechanical-testing#EMMO_2697e9d2_e173_411c_8c4b_2b400ab6b1b9> rdf:type owl:Class ;
                                                                                            rdfs:subClassOf <http://emmo.info/emmo/domain/mechanical-testing#EMMO_37824926_963f_4e3d_ac3c_7c323e969ff6> ;
                                                                                            <http://www.w3.org/2004/02/skos/core#prefLabel> "Bending"@en .


###  http://emmo.info/emmo/domain/mechanical-testing#EMMO_2a706af8_27ae_468f_9688_fbbe4ca13a86
<http://emmo.info/emmo/domain/mechanical-testing#EMMO_2a706af8_27ae_468f_9688_fbbe4ca13a86> rdf:type owl:Class ;
                                                                                            rdfs:subClassOf <http://emmo.info/emmo/domain/mechanical-testing#EMMO_e5d45f40_f9e9_47b9_934b_4c463a38b08e> ,
                                                                                                            <http://emmo.info/emmo/middle/perceptual#EMMO_c74da218_9147_4f03_92d1_8894abca55f3> ;
                                                                                            rdfs:comment "Specifies, where the crack started on the cross section." ;
                                                                                            <http://www.w3.org/2004/02/skos/core#prefLabel> "FailureType"@en .


###  http://emmo.info/emmo/domain/mechanical-testing#EMMO_2a7951e2_0f3d_4fe7_bf8a_0ce97b4cbab1
<http://emmo.info/emmo/domain/mechanical-testing#EMMO_2a7951e2_0f3d_4fe7_bf8a_0ce97b4cbab1> rdf:type owl:Class ;
                                                                                            rdfs:subClassOf <http://emmo.info/emmo/domain/mechanical-testing#EMMO_35a4d47f_452e_4234_9183_3b835ca02091> ;
                                                                                            <http://www.w3.org/2004/02/skos/core#prefLabel> "ContinuousStiffnessMeasurementOliverPharrPostProcessing"@en .


###  http://emmo.info/emmo/domain/mechanical-testing#EMMO_2aa65ba7_afb2_4deb_b566_3e2c25a89feb
<http://emmo.info/emmo/domain/mechanical-testing#EMMO_2aa65ba7_afb2_4deb_b566_3e2c25a89feb> rdf:type owl:Class ;
                                                                                            rdfs:subClassOf <http://emmo.info/emmo/domain/mechanical-testing#EMMO_e5d45f40_f9e9_47b9_934b_4c463a38b08e> ,
                                                                                                            <http://emmo.info/emmo/middle/isq#EMMO_acf636d4_9ac2_4ce3_960a_d54338e6cae3> ;
                                                                                            rdfs:comment "Elongation at break, also known as fracture strain, is the ratio between changed length and initial length after breakage of the test specimen. Plastic strain at fracture." ;
                                                                                            <http://www.w3.org/2004/02/skos/core#prefLabel> "FractureStrain"@en .


###  http://emmo.info/emmo/domain/mechanical-testing#EMMO_2b89063d_6ed4_4bf0_9443_e0d3dcb265b8
<http://emmo.info/emmo/domain/mechanical-testing#EMMO_2b89063d_6ed4_4bf0_9443_e0d3dcb265b8> rdf:type owl:Class ;
                                                                                            rdfs:subClassOf <http://emmo.info/emmo/domain/mechanical-testing#EMMO_c16d56fc_ad1f_420d_9d61_edbe4a28136a> ;
                                                                                            rdfs:comment "An indentation test where both the applied load and resulting displacement are monitored during the test." ;
                                                                                            <http://www.w3.org/2004/02/skos/core#prefLabel> "DepthSensingIndentation"@en .


###  http://emmo.info/emmo/domain/mechanical-testing#EMMO_2bd00836_2e7a_4e95_ad4e_50cb370c288c
<http://emmo.info/emmo/domain/mechanical-testing#EMMO_2bd00836_2e7a_4e95_ad4e_50cb370c288c> rdf:type owl:Class ;
                                                                                            rdfs:subClassOf <http://emmo.info/emmo/domain/mechanical-testing#EMMO_8630b1ff_7985_444e_8572_373816c0d3b5> ;
                                                                                            rdfs:comment """Steel category according to SAE standard:
Metals with special properties (SAE)""" ;
                                                                                            rdfs:label "Metals with special properties (SAE)"@en ;
                                                                                            <http://www.w3.org/2004/02/skos/core#prefLabel> "MetalsWithSpecialPropertiesSAE"@en .


###  http://emmo.info/emmo/domain/mechanical-testing#EMMO_2d48b136_0b7f_4c7c_86a8_cb9a1a287893
<http://emmo.info/emmo/domain/mechanical-testing#EMMO_2d48b136_0b7f_4c7c_86a8_cb9a1a287893> rdf:type owl:Class ;
                                                                                            rdfs:subClassOf <http://emmo.info/emmo/domain/mechanical-testing#EMMO_76dba92f_a761_409f_83d8_5a0c9c73b349> ;
                                                                                            <http://www.w3.org/2004/02/skos/core#prefLabel> "IndentationDepthCalibration"@en .


###  http://emmo.info/emmo/domain/mechanical-testing#EMMO_2db2865b_2cd9_4c96_ab3e_6e81964f7436
<http://emmo.info/emmo/domain/mechanical-testing#EMMO_2db2865b_2cd9_4c96_ab3e_6e81964f7436> rdf:type owl:Class ;
                                                                                            rdfs:subClassOf <http://emmo.info/emmo/domain/mechanical-testing#EMMO_48e3eddc_de6b_4e9e_891d_99169d9f0883> ;
                                                                                            <http://www.w3.org/2004/02/skos/core#prefLabel> "Rolling"@en .


###  http://emmo.info/emmo/domain/mechanical-testing#EMMO_2e9a014f_9337_42f7_ad91_b73f150a9901
<http://emmo.info/emmo/domain/mechanical-testing#EMMO_2e9a014f_9337_42f7_ad91_b73f150a9901> rdf:type owl:Class ;
                                                                                            rdfs:subClassOf <http://emmo.info/emmo/domain/mechanical-testing#EMMO_4c57e181_8205_4e51_a164_d17c4bea891d> ;
                                                                                            <http://www.w3.org/2004/02/skos/core#prefLabel> "BulkHardening"@en .


###  http://emmo.info/emmo/domain/mechanical-testing#EMMO_2ebac53b_0902_43c3_abe5_fc110fbec98f
<http://emmo.info/emmo/domain/mechanical-testing#EMMO_2ebac53b_0902_43c3_abe5_fc110fbec98f> rdf:type owl:Class ;
                                                                                            rdfs:subClassOf <http://emmo.info/emmo/domain/mechanical-testing#EMMO_ca42ed31_3983_4e1a_84f9_a84cab2cdb59> ,
                                                                                                            <http://emmo.info/emmo/domain/mechanical-testing#EMMO_eda29fc2_7d48_4997_8593_38fd9b344fe2> ;
                                                                                            rdfs:comment "The displacement difference between the beginning of the pull-off phenomenon and its end during an adhesion experiment." ;
                                                                                            <http://www.w3.org/2004/02/skos/core#prefLabel> "PulloffDisplacement"@en .


###  http://emmo.info/emmo/domain/mechanical-testing#EMMO_2f9a266b_ffe6_4b3e_8222_eca6001174a2
<http://emmo.info/emmo/domain/mechanical-testing#EMMO_2f9a266b_ffe6_4b3e_8222_eca6001174a2> rdf:type owl:Class ;
                                                                                            rdfs:subClassOf <http://emmo.info/emmo/domain/mechanical-testing#EMMO_0f73321c_c4fd_40ed_9b58_eccd9b7d8e15> ;
                                                                                            <http://www.w3.org/2004/02/skos/core#prefLabel> "ContactAngleMethod"@en .


###  http://emmo.info/emmo/domain/mechanical-testing#EMMO_2ff88734_1272_45d0_a720_0e476b55af26
<http://emmo.info/emmo/domain/mechanical-testing#EMMO_2ff88734_1272_45d0_a720_0e476b55af26> rdf:type owl:Class ;
                                                                                            rdfs:subClassOf <http://emmo.info/emmo/domain/mechanical-testing#EMMO_b71e5f70_227c_4798_8a8a_ee7b70afd10f> ;
                                                                                            rdfs:comment "Grindingis a type ofabrasive machiningprocess which usesgrinding wheelascutting tool. Grinding is a subset of cutting, as grinding is a true metal-cutting process." ;
                                                                                            <http://www.w3.org/2004/02/skos/core#prefLabel> "Grinding"@en .


###  http://emmo.info/emmo/domain/mechanical-testing#EMMO_301113f2_d390_4b1d_8cff_4d4ef9c1fc55
<http://emmo.info/emmo/domain/mechanical-testing#EMMO_301113f2_d390_4b1d_8cff_4d4ef9c1fc55> rdf:type owl:Class ;
                                                                                            rdfs:subClassOf <http://emmo.info/emmo/domain/mechanical-testing#EMMO_ba4f6d96_699f_48ba_a432_6676521587f1> ;
                                                                                            <http://www.w3.org/2004/02/skos/core#prefLabel> "MaximumIndentationTime"@en .


###  http://emmo.info/emmo/domain/mechanical-testing#EMMO_3226bd7c_b9d8_436d_ae5f_8a69a92ea128
<http://emmo.info/emmo/domain/mechanical-testing#EMMO_3226bd7c_b9d8_436d_ae5f_8a69a92ea128> rdf:type owl:Class ;
                                                                                            rdfs:subClassOf <http://emmo.info/emmo/domain/mechanical-testing#NanoindentationUseCase> ,
                                                                                                            <http://emmo.info/emmo/middle/metrology#EMMO_79751276_b2d0_4e2f_bbd4_99d412f43d55> ;
                                                                                            rdfs:comment "Constant strain rate testing involves the application of load so that the depth measurements follow a pre-defined relationship. Set the loading rate to give a constant rate of strain within the specimen material." ;
                                                                                            <http://www.w3.org/2004/02/skos/core#prefLabel> "ConstantStrainRate"@en .


###  http://emmo.info/emmo/domain/mechanical-testing#EMMO_3261d0d2_d0f7_4ec5_bd5a_0e0ad8372311
<http://emmo.info/emmo/domain/mechanical-testing#EMMO_3261d0d2_d0f7_4ec5_bd5a_0e0ad8372311> rdf:type owl:Class ;
                                                                                            rdfs:subClassOf <http://emmo.info/emmo/domain/mechanical-testing#EMMO_e5d45f40_f9e9_47b9_934b_4c463a38b08e> ,
                                                                                                            <http://emmo.info/emmo/middle/chemistry#EMMO_4f40def1_3cd7_4067_9596_541e9a5134cf> ;
                                                                                            <http://www.w3.org/2004/02/skos/core#prefLabel> "PhosphorusSymbol"@en .


###  http://emmo.info/emmo/domain/mechanical-testing#EMMO_326d02f6_8ca0_42ac_9658_ba041231574a
<http://emmo.info/emmo/domain/mechanical-testing#EMMO_326d02f6_8ca0_42ac_9658_ba041231574a> rdf:type owl:Class ;
                                                                                            rdfs:subClassOf <http://emmo.info/emmo/domain/mechanical-testing#EMMO_e5d45f40_f9e9_47b9_934b_4c463a38b08e> ,
                                                                                                            <http://emmo.info/emmo/middle/chemistry#EMMO_4f40def1_3cd7_4067_9596_541e9a5134cf> ;
                                                                                            <http://www.w3.org/2004/02/skos/core#prefLabel> "IronSymbol"@en .


###  http://emmo.info/emmo/domain/mechanical-testing#EMMO_3361ecb7_0340_4475_8e42_b2ae29af2420
<http://emmo.info/emmo/domain/mechanical-testing#EMMO_3361ecb7_0340_4475_8e42_b2ae29af2420> rdf:type owl:Class ;
                                                                                            rdfs:subClassOf <http://emmo.info/emmo/domain/mechanical-testing#EMMO_7452b52c_82ea_47da_b84f_493317c8f03e> ;
                                                                                            rdfs:comment "Steel nomenclature contains steel groups / categories as defined in the standards DIN, SAE and JIS and superclasses in which the categories from the different standards are combined" ;
                                                                                            rdfs:label "Roller bearing steels"@en ;
                                                                                            <http://www.w3.org/2004/02/skos/core#prefLabel> "RollerBearingSteels"@en .


###  http://emmo.info/emmo/domain/mechanical-testing#EMMO_3407d408_5d15_4090_8161_43d5e288a864
<http://emmo.info/emmo/domain/mechanical-testing#EMMO_3407d408_5d15_4090_8161_43d5e288a864> rdf:type owl:Class ;
                                                                                            rdfs:subClassOf <http://emmo.info/emmo/domain/mechanical-testing#EMMO_3c7c1148_40e2_4ec2_a0ac_8720d03e356f> ;
                                                                                            <http://emmo.info/emmo/middle/isq#physicalDimension> "T-2 L+2 M+1 I0 T0 N0 J0" ;
                                                                                            <http://www.w3.org/2004/02/skos/core#prefLabel> "TensileStiffness"@en .


###  http://emmo.info/emmo/domain/mechanical-testing#EMMO_35a4d47f_452e_4234_9183_3b835ca02091
<http://emmo.info/emmo/domain/mechanical-testing#EMMO_35a4d47f_452e_4234_9183_3b835ca02091> rdf:type owl:Class ;
                                                                                            rdfs:subClassOf <http://emmo.info/emmo/domain/mechanical-testing#EMMO_76dba92f_a761_409f_83d8_5a0c9c73b349> ;
                                                                                            <http://www.w3.org/2004/02/skos/core#prefLabel> "OliverPharrPostProcessing"@en .


###  http://emmo.info/emmo/domain/mechanical-testing#EMMO_35d0fcf5_b574_4e43_94ae_874a6117aab3
<http://emmo.info/emmo/domain/mechanical-testing#EMMO_35d0fcf5_b574_4e43_94ae_874a6117aab3> rdf:type owl:Class ;
                                                                                            rdfs:subClassOf <http://emmo.info/emmo/domain/mechanical-testing#CableBundleUseCase> ,
                                                                                                            <http://emmo.info/emmo/domain/mechanical-testing#EMMO_e5d45f40_f9e9_47b9_934b_4c463a38b08e> ,
                                                                                                            <http://emmo.info/emmo/domain/mechanical-testing#NanoindentationUseCase> ,
                                                                                                            <http://emmo.info/emmo/middle/semiotics#EMMO_6f5af708_f825_4feb_a0d1_a8d813d3022b> ;
                                                                                            <http://www.w3.org/2004/02/skos/core#prefLabel> "Sample"@en .


###  http://emmo.info/emmo/domain/mechanical-testing#EMMO_3650a56b_7f3d_4f44_90e7_c08cfd7d3fdd
<http://emmo.info/emmo/domain/mechanical-testing#EMMO_3650a56b_7f3d_4f44_90e7_c08cfd7d3fdd> rdf:type owl:Class ;
                                                                                            rdfs:subClassOf <http://emmo.info/emmo/domain/mechanical-testing#EMMO_91e9c813_b277_48ad_b5b0_a781a05b9c1f> ;
                                                                                            rdfs:comment "The rate of change in the displacement measured in contact with the specimen." ;
                                                                                            <http://www.w3.org/2004/02/skos/core#prefLabel> "DriftRate"@en .


###  http://emmo.info/emmo/domain/mechanical-testing#EMMO_376c6456_5601_41c2_987c_3063f14408d4
<http://emmo.info/emmo/domain/mechanical-testing#EMMO_376c6456_5601_41c2_987c_3063f14408d4> rdf:type owl:Class ;
                                                                                            rdfs:subClassOf <http://emmo.info/emmo/domain/mechanical-testing#NanoindentationUseCase> ,
                                                                                                            <http://emmo.info/emmo/middle/isq#EMMO_1f087811_06cb_42d5_90fb_25d0e7e068ef> ;
                                                                                            rdfs:comment "The Load applied to the sample. It is the zeroed value of the Force corrected for spring deflection. It is zero prior to surface detection Dynamics are not considered." ;
                                                                                            <http://www.w3.org/2004/02/skos/core#prefLabel> "Load"@en .


###  http://emmo.info/emmo/domain/mechanical-testing#EMMO_37824926_963f_4e3d_ac3c_7c323e969ff6
<http://emmo.info/emmo/domain/mechanical-testing#EMMO_37824926_963f_4e3d_ac3c_7c323e969ff6> rdf:type owl:Class ;
                                                                                            rdfs:subClassOf <http://emmo.info/emmo/domain/mechanical-testing#EMMO_646b0170_e349_4382_8291_4fa2cca982ea> ;
                                                                                            rdfs:comment "A symbolic that identifies the differnt types of loading applied that should be part of teh series (tension/compression, bending, shearing, torsion)." ;
                                                                                            <http://www.w3.org/2004/02/skos/core#prefLabel> "LoadingType"@en .


###  http://emmo.info/emmo/domain/mechanical-testing#EMMO_38b58e82_8019_4d19_978a_d47901acce17
<http://emmo.info/emmo/domain/mechanical-testing#EMMO_38b58e82_8019_4d19_978a_d47901acce17> rdf:type owl:Class ;
                                                                                            rdfs:subClassOf <http://emmo.info/emmo/domain/mechanical-testing#EMMO_87985f48_7967_4ed1_b23f_33357576c47d> ;
                                                                                            rdfs:comment "Milling is the process of machining using rotary cutters to remove material by advancing a cutter into a workpiece. This may be done varying direction on one or several axes, cutter head speed, and pressure." ;
                                                                                            <http://www.w3.org/2004/02/skos/core#prefLabel> "Milling"@en .


###  http://emmo.info/emmo/domain/mechanical-testing#EMMO_3b07c236_fcaa_4d7f_9b2b_b59e247a1922
<http://emmo.info/emmo/domain/mechanical-testing#EMMO_3b07c236_fcaa_4d7f_9b2b_b59e247a1922> rdf:type owl:Class ;
                                                                                            rdfs:subClassOf <http://emmo.info/emmo/domain/mechanical-testing#EMMO_c799b443_c70f_4351_bb0f_e4ab29073481> ;
                                                                                            rdfs:comment "Value of the hardness, measured at the specimen surface." ;
                                                                                            <http://www.w3.org/2004/02/skos/core#prefLabel> "SurfaceHardness"@en .


###  http://emmo.info/emmo/domain/mechanical-testing#EMMO_3bc8656e_07db_406b_9847_46f44c458958
<http://emmo.info/emmo/domain/mechanical-testing#EMMO_3bc8656e_07db_406b_9847_46f44c458958> rdf:type owl:Class ;
                                                                                            rdfs:subClassOf <http://emmo.info/emmo/domain/mechanical-testing#EMMO_3407d408_5d15_4090_8161_43d5e288a864> ,
                                                                                                            <http://emmo.info/emmo/middle/holistic#EMMO_49804605_c0fe_4538_abda_f70ba1dc8a5d> ;
                                                                                            rdfs:comment "Averaged Tensile Stifness is a phyiscal quantity of the type of tensile stiffness that results from a calculation of the type arithmetic mean." ;
                                                                                            <http://www.w3.org/2004/02/skos/core#prefLabel> "AveragedTensileStiffness"@en .


###  http://emmo.info/emmo/domain/mechanical-testing#EMMO_3c7c1148_40e2_4ec2_a0ac_8720d03e356f
<http://emmo.info/emmo/domain/mechanical-testing#EMMO_3c7c1148_40e2_4ec2_a0ac_8720d03e356f> rdf:type owl:Class ;
                                                                                            rdfs:subClassOf <http://emmo.info/emmo/domain/mechanical-testing#CableBundleUseCase> ,
                                                                                                            <http://emmo.info/emmo/domain/mechanical-testing#EMMO_e5d45f40_f9e9_47b9_934b_4c463a38b08e> ,
                                                                                                            <http://emmo.info/emmo/domain/mechanical-testing#NanoindentationUseCase> ,
                                                                                                            <http://emmo.info/emmo/middle/metrology#EMMO_71f6ab56_342c_484b_bbe0_de86b7367cb3> ;
                                                                                            rdfs:comment "Stiffness is the extent to which an object resists deformation in response to an applied force. The complementary concept is flexibility or pliability: the more flexible an object is, the less stiff it is." ;
                                                                                            rdfs:seeAlso "http://dbpedia.org/page/Stiffness" ;
                                                                                            <http://www.w3.org/2004/02/skos/core#prefLabel> "Stiffness"@en .


###  http://emmo.info/emmo/domain/mechanical-testing#EMMO_3c835c69_11a9_458d_9b3f_bc68c0348c7d
<http://emmo.info/emmo/domain/mechanical-testing#EMMO_3c835c69_11a9_458d_9b3f_bc68c0348c7d> rdf:type owl:Class ;
                                                                                            rdfs:subClassOf <http://emmo.info/emmo/domain/mechanical-testing#CableBundleUseCase> ,
                                                                                                            <http://emmo.info/emmo/domain/mechanical-testing#EMMO_e5d45f40_f9e9_47b9_934b_4c463a38b08e> ,
                                                                                                            <http://emmo.info/emmo/domain/mechanical-testing#NanoindentationUseCase> ,
                                                                                                            <http://emmo.info/emmo/middle/holistic#EMMO_43e9a05d_98af_41b4_92f6_00f79a09bfce> ;
                                                                                            rdfs:comment "Is a type of activity/computation that is part of a process or in other words a participant in a process and a process itself that involves the transformation of inputs into results (outputs). The calculation defines in more detail very specific tasks within a process (simulation) that are executed. Each of this tasks or calculations have a specific role within the simulation." ;
                                                                                            <http://www.w3.org/2004/02/skos/core#prefLabel> "Calculation"@en .


###  http://emmo.info/emmo/domain/mechanical-testing#EMMO_3c93b3eb_f08f_4c25_940c_fac690e012c6
<http://emmo.info/emmo/domain/mechanical-testing#EMMO_3c93b3eb_f08f_4c25_940c_fac690e012c6> rdf:type owl:Class ;
                                                                                            rdfs:subClassOf <http://emmo.info/emmo/middle/chemistry#EMMO_d357e0dd_3497_4590_af6f_7954db7fecf7> ;
                                                                                            <http://emmo.info/emmo/top/annotations#EMMO_967080e5_2f42_4eb2_a3a9_c58143e835f9> "This name is a label according to local rules like DIN, EN, ISO, SAE or JIS, e.g \"100Cr6\", \"20MnCr5\" or \"SKD 61\", \"4150\"." ;
                                                                                            rdfs:comment "A language object following a specific rules for specifying the chemical composition of chemical species." ;
                                                                                            <http://www.w3.org/2004/02/skos/core#prefLabel> "MaterialName"@en .


###  http://emmo.info/emmo/domain/mechanical-testing#EMMO_3c970e96_4876_4d83_bafa_c79cf5b5916b
<http://emmo.info/emmo/domain/mechanical-testing#EMMO_3c970e96_4876_4d83_bafa_c79cf5b5916b> rdf:type owl:Class ;
                                                                                            rdfs:subClassOf <http://emmo.info/emmo/domain/mechanical-testing#EMMO_7dc73553_7d3f_4dc2_bb7b_f47775207457> ,
                                                                                                            <http://emmo.info/emmo/domain/mechanical-testing#EMMO_f0ad542d_ff13_4998_9e7f_ea27583c5f31> ;
                                                                                            rdfs:comment "The modulus of the specimen as calculated from the maximum load, the maximum depth and the unloading data following the Oliver and Pharr calculation steps." ;
                                                                                            <http://www.w3.org/2004/02/skos/core#prefLabel> "ElasticModulusFromUnload"@en .


###  http://emmo.info/emmo/domain/mechanical-testing#EMMO_3cd2f82b_e17f_4098_b014_dd773e8de8c1
<http://emmo.info/emmo/domain/mechanical-testing#EMMO_3cd2f82b_e17f_4098_b014_dd773e8de8c1> rdf:type owl:Class ;
                                                                                            rdfs:subClassOf <http://emmo.info/emmo/domain/mechanical-testing#EMMO_e5d45f40_f9e9_47b9_934b_4c463a38b08e> ,
                                                                                                            <http://emmo.info/emmo/middle/isq#EMMO_cd2cd0de_e0cc_4ef1_b27e_2e88db027bac> ;
                                                                                            <http://www.w3.org/2004/02/skos/core#prefLabel> "Thickness"@en .


###  http://emmo.info/emmo/domain/mechanical-testing#EMMO_3d31d98b_0620_4f58_858e_8aeedaf70dad
<http://emmo.info/emmo/domain/mechanical-testing#EMMO_3d31d98b_0620_4f58_858e_8aeedaf70dad> rdf:type owl:Class ;
                                                                                            owl:equivalentClass <http://emmo.info/emmo/domain/mechanical-testing#EMMO_f80d451a_9146_47db_bd9a_41e9f7e4b88e> ;
                                                                                            rdfs:subClassOf <http://emmo.info/emmo/domain/mechanical-testing#EMMO_a30a7cdc_f652_4b01_b8c2_cd056f3e3d85> ;
                                                                                            <http://www.w3.org/2004/02/skos/core#prefLabel> "UniversalTestingMachine"@en .


###  http://emmo.info/emmo/domain/mechanical-testing#EMMO_3f227fda_ccf8_4cac_8eec_cd074a006b06
<http://emmo.info/emmo/domain/mechanical-testing#EMMO_3f227fda_ccf8_4cac_8eec_cd074a006b06> rdf:type owl:Class ;
                                                                                            rdfs:subClassOf <http://emmo.info/emmo/domain/mechanical-testing#EMMO_e5d45f40_f9e9_47b9_934b_4c463a38b08e> ,
                                                                                                            <http://emmo.info/emmo/middle/metrology#EMMO_50a3552e_859a_4ff7_946d_76d537cabce6> ,
                                                                                                            <http://emmo.info/emmo/middle/metrology#EMMO_c9c8f824_9127_4f93_bc21_69fe78a7f6f2> ;
                                                                                            rdfs:comment "Brinell Hardness unit" ;
                                                                                            <http://www.w3.org/2004/02/skos/core#prefLabel> "BrinellHardnessUnit"@en .


###  http://emmo.info/emmo/domain/mechanical-testing#EMMO_3fdd2c2f_762b_4d0f_b883_4cf47a2da2f9
<http://emmo.info/emmo/domain/mechanical-testing#EMMO_3fdd2c2f_762b_4d0f_b883_4cf47a2da2f9> rdf:type owl:Class ;
                                                                                            rdfs:subClassOf <http://emmo.info/emmo/domain/mechanical-testing#EMMO_eda29fc2_7d48_4997_8593_38fd9b344fe2> ,
                                                                                                            <http://emmo.info/emmo/middle/isq#EMMO_1f087811_06cb_42d5_90fb_25d0e7e068ef> ;
                                                                                            rdfs:comment "The force needed to overcome the adhesion phenomena between indenter tip and material under investigation." ;
                                                                                            <http://www.w3.org/2004/02/skos/core#prefLabel> "PulloffForce"@en .


###  http://emmo.info/emmo/domain/mechanical-testing#EMMO_3fe87ba8_b79f_4c33_ad30_bf81eaaee46b
<http://emmo.info/emmo/domain/mechanical-testing#EMMO_3fe87ba8_b79f_4c33_ad30_bf81eaaee46b> rdf:type owl:Class ;
                                                                                            rdfs:subClassOf <http://emmo.info/emmo/domain/mechanical-testing#EMMO_e5d45f40_f9e9_47b9_934b_4c463a38b08e> ,
                                                                                                            <http://emmo.info/emmo/middle/perceptual#EMMO_89a0c87c_0804_4013_937a_6fe234d9499c> ,
                                                                                                            <http://emmo.info/emmo/middle/reductionistic#EMMO_36c79456_e29c_400d_8bd3_0eedddb82652> ;
                                                                                            rdfs:comment "The fatigue properties are determined by fatigue testing according to predefined test parameters. The fatigue properties may be direct data resulting from a experiment itself (specimen level) or data that is derived from the test result of many specimens (series level). The test result is input for the fatigue / series properties." ;
                                                                                            <http://www.w3.org/2004/02/skos/core#prefLabel> "FatigueTestResult"@en .


###  http://emmo.info/emmo/domain/mechanical-testing#EMMO_400fa2bf_a1b9_4e03_b6bd_7540c8fe5b4a
<http://emmo.info/emmo/domain/mechanical-testing#EMMO_400fa2bf_a1b9_4e03_b6bd_7540c8fe5b4a> rdf:type owl:Class ;
                                                                                            rdfs:subClassOf <http://emmo.info/emmo/domain/mechanical-testing#EMMO_3c7c1148_40e2_4ec2_a0ac_8720d03e356f> ;
                                                                                            <http://emmo.info/emmo/middle/isq#physicalDimension> "T-2 L+3 M+1 I0 T0 N0 J0" ;
                                                                                            rdfs:comment "In beam theory, a bending stiffness describes the effective stiffness of the beam for bending deformation. Formally, it is given as product of Youngs modulus and the second moment of inertia. But in practice, the bending stiffness is an individual effective parameter, that must not be separated into a material and a geometrical property." ;
                                                                                            <http://www.w3.org/2004/02/skos/core#prefLabel> "BendingStiffness"@en .


###  http://emmo.info/emmo/domain/mechanical-testing#EMMO_40af5a74_ab01_4457_83aa_216a5d7889ee
<http://emmo.info/emmo/domain/mechanical-testing#EMMO_40af5a74_ab01_4457_83aa_216a5d7889ee> rdf:type owl:Class ;
                                                                                            rdfs:subClassOf <http://emmo.info/emmo/domain/mechanical-testing#EMMO_c799b443_c70f_4351_bb0f_e4ab29073481> ,
                                                                                                            <http://emmo.info/emmo/domain/mechanical-testing#EMMO_eda29fc2_7d48_4997_8593_38fd9b344fe2> ;
                                                                                            rdfs:comment "The hardness of the specimen as calculated form the maximum load, the maximum depth and the unloading data following the Oliver and Pharr calculation steps." ;
                                                                                            <http://www.w3.org/2004/02/skos/core#prefLabel> "HardnessFromUnload"@en .


###  http://emmo.info/emmo/domain/mechanical-testing#EMMO_40c2449f_3a12_4c31_bb87_895e24ebb8a8
<http://emmo.info/emmo/domain/mechanical-testing#EMMO_40c2449f_3a12_4c31_bb87_895e24ebb8a8> rdf:type owl:Class ;
                                                                                            rdfs:subClassOf <http://emmo.info/emmo/domain/mechanical-testing#EMMO_d27a86dd_6e4d_4f89_979f_c7500876928a> ;
                                                                                            <http://www.w3.org/2004/02/skos/core#prefLabel> "TensionCompression"@en .


###  http://emmo.info/emmo/domain/mechanical-testing#EMMO_4136ef18_9624_4f92_b556_c9295b088806
<http://emmo.info/emmo/domain/mechanical-testing#EMMO_4136ef18_9624_4f92_b556_c9295b088806> rdf:type owl:Class ;
                                                                                            rdfs:subClassOf <http://emmo.info/emmo/domain/mechanical-testing#EMMO_e5d45f40_f9e9_47b9_934b_4c463a38b08e> ,
                                                                                                            <http://emmo.info/emmo/middle/isq#EMMO_d1917609_db5e_4b8a_9b76_ef1d6f860a81> ;
                                                                                            rdfs:comment "The maximum stress S_max is the highest occuring stress during fatigue testing." ;
                                                                                            <http://www.w3.org/2004/02/skos/core#prefLabel> "MaximumStress"@en .


###  http://emmo.info/emmo/domain/mechanical-testing#EMMO_416da557_8833_4161_b469_7cc7373399a1
<http://emmo.info/emmo/domain/mechanical-testing#EMMO_416da557_8833_4161_b469_7cc7373399a1> rdf:type owl:Class ;
                                                                                            rdfs:subClassOf <http://emmo.info/emmo/domain/mechanical-testing#EMMO_e5d45f40_f9e9_47b9_934b_4c463a38b08e> ,
                                                                                                            <http://emmo.info/emmo/middle/chemistry#EMMO_4f40def1_3cd7_4067_9596_541e9a5134cf> ;
                                                                                            <http://www.w3.org/2004/02/skos/core#prefLabel> "ArsenicSymbol"@en .


###  http://emmo.info/emmo/domain/mechanical-testing#EMMO_43db3609_c443_4f24_8bc2_0b7cf27ac12a
<http://emmo.info/emmo/domain/mechanical-testing#EMMO_43db3609_c443_4f24_8bc2_0b7cf27ac12a> rdf:type owl:Class ;
                                                                                            rdfs:subClassOf <http://emmo.info/emmo/domain/mechanical-testing#EMMO_e5d45f40_f9e9_47b9_934b_4c463a38b08e> ,
                                                                                                            <http://emmo.info/emmo/middle/chemistry#EMMO_4f40def1_3cd7_4067_9596_541e9a5134cf> ;
                                                                                            <http://www.w3.org/2004/02/skos/core#prefLabel> "StrontiumSymbol"@en .


###  http://emmo.info/emmo/domain/mechanical-testing#EMMO_442c0fb7_09d4_4dae_b45c_8eb1522da38f
<http://emmo.info/emmo/domain/mechanical-testing#EMMO_442c0fb7_09d4_4dae_b45c_8eb1522da38f> rdf:type owl:Class ;
                                                                                            rdfs:subClassOf <http://emmo.info/emmo/domain/mechanical-testing#EMMO_2b89063d_6ed4_4bf0_9443_e0d3dcb265b8> ;
                                                                                            rdfs:comment "A depth sensing indentation test where measured displacement is in the nanometer range (0-1000 nm)." ;
                                                                                            <http://www.w3.org/2004/02/skos/core#prefLabel> "Nanoindentation"@en .


###  http://emmo.info/emmo/domain/mechanical-testing#EMMO_44389354_4c50_4a74_b315_83cdc69d326d
<http://emmo.info/emmo/domain/mechanical-testing#EMMO_44389354_4c50_4a74_b315_83cdc69d326d> rdf:type owl:Class ;
                                                                                            rdfs:subClassOf <http://emmo.info/emmo/domain/mechanical-testing#EMMO_19afc39b_eb5c_46e0_b880_8e08ec831ebc> ;
                                                                                            <http://www.w3.org/2004/02/skos/core#prefLabel> "NanoindentationMachine"@en .


###  http://emmo.info/emmo/domain/mechanical-testing#EMMO_44c9b071_54a1_4366_84e4_b14b055ec633
<http://emmo.info/emmo/domain/mechanical-testing#EMMO_44c9b071_54a1_4366_84e4_b14b055ec633> rdf:type owl:Class ;
                                                                                            rdfs:subClassOf <http://emmo.info/emmo/domain/mechanical-testing#EMMO_24af8df2_9438_44f6_8c5f_755beb459a49> ;
                                                                                            rdfs:comment "Corresponds to the Yield stress at 0.2% plastic strain." ;
                                                                                            <http://www.w3.org/2004/02/skos/core#prefLabel> "RP0.2"@en .


###  http://emmo.info/emmo/domain/mechanical-testing#EMMO_44e81349_11f5_406c_beb1_457184586cf8
<http://emmo.info/emmo/domain/mechanical-testing#EMMO_44e81349_11f5_406c_beb1_457184586cf8> rdf:type owl:Class ;
                                                                                            rdfs:subClassOf <http://emmo.info/emmo/domain/mechanical-testing#EMMO_16d31733_248f_4e55_b870_dfc96d3e2c3b> ,
                                                                                                            <http://emmo.info/emmo/middle/reductionistic#EMMO_36c79456_e29c_400d_8bd3_0eedddb82652> ,
                                                                                                            <http://emmo.info/emmo/middle/semiotics#EMMO_6f5af708_f825_4feb_a0d1_a8d813d3022b> ;
                                                                                            rdfs:comment "This label should be made more specific since it represents a very specific series to the FatigueTestUseCase" ,
                                                                                                         "Typically a series contains data from multiple experiments/specimens of similar type and material, but at different stress amplitude aiming at determination of a SN curve. Furthermore, a series contains secondary data such as the fatigue strength and slope of the SN-curve which puts the results of the individual experiments in a context." ;
                                                                                            <http://www.w3.org/2004/02/skos/core#prefLabel> "Series"@en .


###  http://emmo.info/emmo/domain/mechanical-testing#EMMO_4533a4e3_b817_46b1_8784_d8ba08b70910
<http://emmo.info/emmo/domain/mechanical-testing#EMMO_4533a4e3_b817_46b1_8784_d8ba08b70910> rdf:type owl:Class ;
                                                                                            rdfs:subClassOf <http://emmo.info/emmo/domain/mechanical-testing#EMMO_ce1fea85_f31d_4ad4_a717_8ef7612f651f> ;
                                                                                            rdfs:comment """Steel category according to DIN standard:
Alloyed construction, engineering and pressure vessel steels (DIN 10027-2)""" ;
                                                                                            rdfs:label "Alloyed construction, engineering and pressure vessel steels (DIN 10027-2)"@en ;
                                                                                            <http://www.w3.org/2004/02/skos/core#prefLabel> "AlloyedConstructionEngineeringAndPressureVesselSteelsDIN10027"@en .


###  http://emmo.info/emmo/domain/mechanical-testing#EMMO_460d3ba4_a8e5_449d_8423_7d4d1cca6d76
<http://emmo.info/emmo/domain/mechanical-testing#EMMO_460d3ba4_a8e5_449d_8423_7d4d1cca6d76> rdf:type owl:Class ;
                                                                                            rdfs:subClassOf <http://emmo.info/emmo/domain/mechanical-testing#EMMO_a30a7cdc_f652_4b01_b8c2_cd056f3e3d85> ;
                                                                                            rdfs:comment "Mechanical testing machine that is designed for a a very specific purpose." ;
                                                                                            <http://www.w3.org/2004/02/skos/core#prefLabel> "SpecialPurposeTestingMachine"@en .


###  http://emmo.info/emmo/domain/mechanical-testing#EMMO_46d03bc9_dc95_4fa3_82e5_25b499393275
<http://emmo.info/emmo/domain/mechanical-testing#EMMO_46d03bc9_dc95_4fa3_82e5_25b499393275> rdf:type owl:Class ;
                                                                                            rdfs:subClassOf <http://emmo.info/emmo/domain/mechanical-testing#EMMO_0527f1f8_41d4_4414_b1fa_8afbc8651ecb> ,
                                                                                                            <http://emmo.info/emmo/domain/mechanical-testing#EMMO_646b0170_e349_4382_8291_4fa2cca982ea> ;
                                                                                            rdfs:comment "Number of load cycles after which the test is terminated and the specimen is treated as a run out." ;
                                                                                            <http://www.w3.org/2004/02/skos/core#prefLabel> "CycleLimit"@en .


###  http://emmo.info/emmo/domain/mechanical-testing#EMMO_473ac6ab_620f_4195_97ed_23591b27a5ef
<http://emmo.info/emmo/domain/mechanical-testing#EMMO_473ac6ab_620f_4195_97ed_23591b27a5ef> rdf:type owl:Class ;
                                                                                            rdfs:subClassOf <http://emmo.info/emmo/domain/mechanical-testing#EMMO_e5d45f40_f9e9_47b9_934b_4c463a38b08e> ,
                                                                                                            <http://emmo.info/emmo/middle/isq#EMMO_faab3f84_e475_4a46_af9c_7d249f0b9aef> ;
                                                                                            rdfs:comment """The mean stress sensitivity is a numerical value that indicates how sensible a steel is reacting to mean stress influence. It is calculated via the parameters/constants a_M and b_M (which are specified further in \"FKM-Richtlinie - Rechnerischer Festigkeitsnachweis (2012)\" and the tensile strength of the material. 
mean stress sensitivity M_sig = f(Rm, a_M, b_M)"""@en ;
                                                                                            <http://www.w3.org/2004/02/skos/core#prefLabel> "MeanStressSensitivity"@en .


###  http://emmo.info/emmo/domain/mechanical-testing#EMMO_48e3eddc_de6b_4e9e_891d_99169d9f0883
<http://emmo.info/emmo/domain/mechanical-testing#EMMO_48e3eddc_de6b_4e9e_891d_99169d9f0883> rdf:type owl:Class ;
                                                                                            rdfs:subClassOf <http://emmo.info/emmo/domain/mechanical-testing#EMMO_e5d45f40_f9e9_47b9_934b_4c463a38b08e> ,
                                                                                                            <http://emmo.info/emmo/middle/manufacturing#EMMO_a4d66059_5dd3_4b90_b4cb_10960559441b> ;
                                                                                            <http://www.w3.org/2004/02/skos/core#prefLabel> "Metalworking"@en .


###  http://emmo.info/emmo/domain/mechanical-testing#EMMO_4b1174a6_bf6f_488e_978d_26ee2542d119
<http://emmo.info/emmo/domain/mechanical-testing#EMMO_4b1174a6_bf6f_488e_978d_26ee2542d119> rdf:type owl:Class ;
                                                                                            rdfs:subClassOf <http://emmo.info/emmo/domain/mechanical-testing#EMMO_89be8d21_79a7_4970_9b0a_ee18cec63e62> ;
                                                                                            rdfs:comment """Steel category according to DIN standard:
Unalloyed construction, engineering and pressure vessel steels with C < 0,5 % (DIN 10027-2)""" ;
                                                                                            rdfs:label "Unalloyed construction, engineering and pressure vessel steels with C < 0,5 % (DIN 10027-2)"@en ;
                                                                                            <http://www.w3.org/2004/02/skos/core#prefLabel> "UnalloyedConstructionEngineeringAndPressureVesselSteelsWithCBelow0p5PercentDIN10027"@en .


###  http://emmo.info/emmo/domain/mechanical-testing#EMMO_4ba72a55_218b_4ead_8a55_2ca1ac5fea33
<http://emmo.info/emmo/domain/mechanical-testing#EMMO_4ba72a55_218b_4ead_8a55_2ca1ac5fea33> rdf:type owl:Class ;
                                                                                            rdfs:subClassOf <http://emmo.info/emmo/domain/mechanical-testing#EMMO_c21ab500_db9a_43a3_a7ef_d43fb64bf856> ;
                                                                                            rdfs:seeAlso "Represents a label (symbolic) that uniquely identifies a series." ;
                                                                                            <http://www.w3.org/2004/02/skos/core#prefLabel> "SeriesID"@en .


###  http://emmo.info/emmo/domain/mechanical-testing#EMMO_4c25ab1b_462c_49a6_bb27_ea3bd020ab2a
<http://emmo.info/emmo/domain/mechanical-testing#EMMO_4c25ab1b_462c_49a6_bb27_ea3bd020ab2a> rdf:type owl:Class ;
                                                                                            rdfs:subClassOf <http://emmo.info/emmo/domain/mechanical-testing#EMMO_48e3eddc_de6b_4e9e_891d_99169d9f0883> ;
                                                                                            rdfs:comment "Heat treatment is the process of heating metal without letting it reach its molten, or melting, stage, and then cooling the metal in a controlled way to select desired mechanical properties." ;
                                                                                            <http://www.w3.org/2004/02/skos/core#prefLabel> "HeatTreatment"@en .


###  http://emmo.info/emmo/domain/mechanical-testing#EMMO_4c57e181_8205_4e51_a164_d17c4bea891d
<http://emmo.info/emmo/domain/mechanical-testing#EMMO_4c57e181_8205_4e51_a164_d17c4bea891d> rdf:type owl:Class ;
                                                                                            rdfs:subClassOf <http://emmo.info/emmo/domain/mechanical-testing#EMMO_4c25ab1b_462c_49a6_bb27_ea3bd020ab2a> ;
                                                                                            rdfs:comment "Hardening is a metalurgical metalworking process used to increase the hardness of a metal. It requires heating the material above a certain temperature and quenchening it afterwards." ;
                                                                                            <http://www.w3.org/2004/02/skos/core#prefLabel> "Hardening"@en .


###  http://emmo.info/emmo/domain/mechanical-testing#EMMO_4d068e58_f7d2_4629_bb8c_e3f8251cdf07
<http://emmo.info/emmo/domain/mechanical-testing#EMMO_4d068e58_f7d2_4629_bb8c_e3f8251cdf07> rdf:type owl:Class ;
                                                                                            rdfs:subClassOf <http://emmo.info/emmo/domain/mechanical-testing#EMMO_76471eff_11f6_4b51_a6e0_3923a7ecfa2e> ;
                                                                                            rdfs:comment """Steel category according to JIS standard:
Construction steels (JIS)""" ;
                                                                                            rdfs:label "Construction steels (JIS)"@en ;
                                                                                            <http://www.w3.org/2004/02/skos/core#prefLabel> "ConstructionSteelsJIS"@en .


###  http://emmo.info/emmo/domain/mechanical-testing#EMMO_4d5b1eee_cda4_4bc7_8a0e_612fcf7f0c82
<http://emmo.info/emmo/domain/mechanical-testing#EMMO_4d5b1eee_cda4_4bc7_8a0e_612fcf7f0c82> rdf:type owl:Class ;
                                                                                            rdfs:subClassOf <http://emmo.info/emmo/domain/mechanical-testing#EMMO_c21ab500_db9a_43a3_a7ef_d43fb64bf856> ;
                                                                                            rdfs:comment "Represents a label (symbolic) that uniquely identifies a specimen." ;
                                                                                            <http://www.w3.org/2004/02/skos/core#prefLabel> "SpecimenID"@en .


###  http://emmo.info/emmo/domain/mechanical-testing#EMMO_4e0b694c_0a16_4cac_b5e3_991aa7f282eb
<http://emmo.info/emmo/domain/mechanical-testing#EMMO_4e0b694c_0a16_4cac_b5e3_991aa7f282eb> rdf:type owl:Class ;
                                                                                            rdfs:subClassOf <http://emmo.info/emmo/domain/mechanical-testing#EMMO_e5d45f40_f9e9_47b9_934b_4c463a38b08e> ,
                                                                                                            <http://emmo.info/emmo/middle/chemistry#EMMO_4f40def1_3cd7_4067_9596_541e9a5134cf> ;
                                                                                            <http://www.w3.org/2004/02/skos/core#prefLabel> "TitaniumSymbol"@en .


###  http://emmo.info/emmo/domain/mechanical-testing#EMMO_4ea93487_28ea_4e1b_8973_12b73e895c64
<http://emmo.info/emmo/domain/mechanical-testing#EMMO_4ea93487_28ea_4e1b_8973_12b73e895c64> rdf:type owl:Class ;
                                                                                            rdfs:subClassOf <http://emmo.info/emmo/domain/mechanical-testing#EMMO_207b3e76_c121_47f6_8278_7871292ce73f> ;
                                                                                            rdfs:comment "Tensile testing, also known as tension testing, is a fundamental materials science and engineering test in which a sample is subjected to a controlled tension until failure. Properties that are directly measured via a tensile test are ultimate tensile strength, breaking strength, maximum elongation and reduction in area. From these measurements the following properties can also be determined: Young's modulus, Poisson's ratio, yield strength, and strain-hardening characteristics. Uniaxial tensile testing is the most commonly used for obtaining the mechanical characteristics of isotropic materials. Some materials use biaxial tensile testing. The main difference between these testing machines being how load is applied on the materials." ;
                                                                                            <http://www.w3.org/2004/02/skos/core#prefLabel> "TensileTesting"@en .


###  http://emmo.info/emmo/domain/mechanical-testing#EMMO_4fca07ce_cc0f_412c_907f_c2ba9fa05fcc
<http://emmo.info/emmo/domain/mechanical-testing#EMMO_4fca07ce_cc0f_412c_907f_c2ba9fa05fcc> rdf:type owl:Class ;
                                                                                            rdfs:subClassOf <http://emmo.info/emmo/domain/mechanical-testing#EMMO_c799b443_c70f_4351_bb0f_e4ab29073481> ;
                                                                                            rdfs:comment "Brinnel hardness is a derived quantity that is determined using a standard Brinnel Hardness test." ;
                                                                                            <http://www.w3.org/2004/02/skos/core#prefLabel> "BrinnelHardness"@en .


###  http://emmo.info/emmo/domain/mechanical-testing#EMMO_5053c512_2431_4fc5_9782_c85e94519495
<http://emmo.info/emmo/domain/mechanical-testing#EMMO_5053c512_2431_4fc5_9782_c85e94519495> rdf:type owl:Class ;
                                                                                            rdfs:subClassOf <http://emmo.info/emmo/domain/mechanical-testing#EMMO_93c88738_64bc_49d7_9d43_f4c177a3b72e> ;
                                                                                            rdfs:comment """Steel category according to DIN standard:
Construction, engineering and pressure vessel steels, Cr-Mo with Mo < 0,35 % Cr-Mo-B (DIN 10027-2)""" ;
                                                                                            rdfs:label "Construction, engineering and pressure vessel steels, Cr-Mo with Mo < 0,35 % Cr-Mo-B (DIN 10027-2)"@en ;
                                                                                            <http://www.w3.org/2004/02/skos/core#prefLabel> "ConstructionEngineeringAndPressureVesselSteelsCrMoWithMoBelow0p35PercentDIN10027"@en .


###  http://emmo.info/emmo/domain/mechanical-testing#EMMO_509e1730_f02e_432c_87d8_7a553a9d93ac
<http://emmo.info/emmo/domain/mechanical-testing#EMMO_509e1730_f02e_432c_87d8_7a553a9d93ac> rdf:type owl:Class ;
                                                                                            rdfs:subClassOf <http://emmo.info/emmo/domain/mechanical-testing#EMMO_7dc73553_7d3f_4dc2_bb7b_f47775207457> ,
                                                                                                            <http://emmo.info/emmo/domain/mechanical-testing#EMMO_f0ad542d_ff13_4998_9e7f_ea27583c5f31> ;
                                                                                            rdfs:comment "The reduced modulus calculated form dynamics and the Oliver and Pharr method." ;
                                                                                            <http://www.w3.org/2004/02/skos/core#prefLabel> "DynamicReducedModulus"@en .


###  http://emmo.info/emmo/domain/mechanical-testing#EMMO_50c344b9_35d9_4029_a68b_a713b0bcc6ad
<http://emmo.info/emmo/domain/mechanical-testing#EMMO_50c344b9_35d9_4029_a68b_a713b0bcc6ad> rdf:type owl:Class ;
                                                                                            rdfs:subClassOf <http://emmo.info/emmo/domain/mechanical-testing#EMMO_7dc73553_7d3f_4dc2_bb7b_f47775207457> ,
                                                                                                            <http://emmo.info/emmo/domain/mechanical-testing#EMMO_f0ad542d_ff13_4998_9e7f_ea27583c5f31> ;
                                                                                            rdfs:comment "The average value of the modulus measured using the Continuous Stiffness Measurement technique. It is calculated by averaging the elastic modulus coming from the calculations performed according to the Oliver and Pharr method over a specific, user-selected, penetration depth range." ;
                                                                                            <http://www.w3.org/2004/02/skos/core#prefLabel> "AverageDynamicModulus"@en .


###  http://emmo.info/emmo/domain/mechanical-testing#EMMO_535baaec_5360_48e8_ada4_72c6e6848957
<http://emmo.info/emmo/domain/mechanical-testing#EMMO_535baaec_5360_48e8_ada4_72c6e6848957> rdf:type owl:Class ;
                                                                                            rdfs:subClassOf <http://emmo.info/emmo/domain/mechanical-testing#CableBundleUseCase> ,
                                                                                                            <http://emmo.info/emmo/domain/mechanical-testing#EMMO_e5d45f40_f9e9_47b9_934b_4c463a38b08e> ,
                                                                                                            <http://emmo.info/emmo/domain/mechanical-testing#NanoindentationUseCase> ,
                                                                                                            <http://emmo.info/emmo/middle/manufacturing#EMMO_ec7464a9_d99d_45f8_965b_4e9230ea8356> ,
                                                                                                            <http://emmo.info/emmo/middle/semiotics#EMMO_6f5af708_f825_4feb_a0d1_a8d813d3022b> ;
                                                                                            rdfs:comment "Specimen is a limited quantity of a real world object which is intended to be similar to and represent a larger amount of it. It can be defined as a sample or a portion of a real world object that has been prepared based on the measureemnt protocol." ;
                                                                                            <http://www.w3.org/2004/02/skos/core#prefLabel> "Specimen"@en .


###  http://emmo.info/emmo/domain/mechanical-testing#EMMO_543888aa_a923_4968_9a14_aece66106772
<http://emmo.info/emmo/domain/mechanical-testing#EMMO_543888aa_a923_4968_9a14_aece66106772> rdf:type owl:Class ;
                                                                                            rdfs:subClassOf <http://emmo.info/emmo/domain/mechanical-testing#EMMO_400fa2bf_a1b9_4e03_b6bd_7540c8fe5b4a> ,
                                                                                                            <http://emmo.info/emmo/middle/holistic#EMMO_49804605_c0fe_4538_abda_f70ba1dc8a5d> ;
                                                                                            rdfs:comment "Averaged bending stifness is a phyiscal quantity of the type of bending stiffness that results from a calculation of the type arithmetic mean." ;
                                                                                            <http://www.w3.org/2004/02/skos/core#prefLabel> "AveragedBendingStiffness"@en .


###  http://emmo.info/emmo/domain/mechanical-testing#EMMO_5589aa4e_6cb7_4194_b549_73854ab8aaa6
<http://emmo.info/emmo/domain/mechanical-testing#EMMO_5589aa4e_6cb7_4194_b549_73854ab8aaa6> rdf:type owl:Class ;
                                                                                            rdfs:subClassOf <http://emmo.info/emmo/domain/mechanical-testing#EMMO_376c6456_5601_41c2_987c_3063f14408d4> ,
                                                                                                            <http://emmo.info/emmo/domain/mechanical-testing#EMMO_91e9c813_b277_48ad_b5b0_a781a05b9c1f> ;
                                                                                            rdfs:comment "The maximum load attained during a nanoindentation test." ;
                                                                                            <http://www.w3.org/2004/02/skos/core#prefLabel> "MaximumLoad"@en .


###  http://emmo.info/emmo/domain/mechanical-testing#EMMO_57b66075_0a4b_46a3_a19b_7a7acdd2f28a
<http://emmo.info/emmo/domain/mechanical-testing#EMMO_57b66075_0a4b_46a3_a19b_7a7acdd2f28a> rdf:type owl:Class ;
                                                                                            rdfs:subClassOf <http://emmo.info/emmo/domain/mechanical-testing#EMMO_f210d615_89a5_483f_a8b2_923ff6fcf4ab> ;
                                                                                            <http://www.w3.org/2004/02/skos/core#prefLabel> "TensileTestPostProcessing"@en .


###  http://emmo.info/emmo/domain/mechanical-testing#EMMO_580f1bd6_5505_4f31_9a8a_b4e9a17bc604
<http://emmo.info/emmo/domain/mechanical-testing#EMMO_580f1bd6_5505_4f31_9a8a_b4e9a17bc604> rdf:type owl:Class ;
                                                                                            rdfs:subClassOf <http://emmo.info/emmo/domain/mechanical-testing#CableBundleUseCase> ,
                                                                                                            <http://emmo.info/emmo/middle/manufacturing#EMMO_ec7464a9_d99d_45f8_965b_4e9230ea8356> ;
                                                                                            rdfs:comment "Represents the cover of a Cable Bundle and it describes how it is spacially distributed across the cable bundle length." ;
                                                                                            <http://www.w3.org/2004/02/skos/core#prefLabel> "BundleCover"@en .


###  http://emmo.info/emmo/domain/mechanical-testing#EMMO_58da328c_f504_44f9_9a78_ef62e50bb6b1
<http://emmo.info/emmo/domain/mechanical-testing#EMMO_58da328c_f504_44f9_9a78_ef62e50bb6b1> rdf:type owl:Class ;
                                                                                            rdfs:subClassOf <http://emmo.info/emmo/domain/mechanical-testing#EMMO_c83ab749_46e6_46fa_be0f_12575a28a30f> ;
                                                                                            <http://www.w3.org/2004/02/skos/core#prefLabel> "Forging"@en .


###  http://emmo.info/emmo/domain/mechanical-testing#EMMO_59a24d10_ed15_4d81_b8b6_1e3d4744a38c
<http://emmo.info/emmo/domain/mechanical-testing#EMMO_59a24d10_ed15_4d81_b8b6_1e3d4744a38c> rdf:type owl:Class ;
                                                                                            rdfs:subClassOf <http://emmo.info/emmo/domain/mechanical-testing#EMMO_3c7c1148_40e2_4ec2_a0ac_8720d03e356f> ;
                                                                                            rdfs:comment "The stiffness of the support springs. It is calibrated as a function of the displacement." ;
                                                                                            <http://www.w3.org/2004/02/skos/core#prefLabel> "NanoindentationMachineSpringStiffness"@en .


###  http://emmo.info/emmo/domain/mechanical-testing#EMMO_5ae58bc1_85e1_45e4_be56_c1331bee7d75
<http://emmo.info/emmo/domain/mechanical-testing#EMMO_5ae58bc1_85e1_45e4_be56_c1331bee7d75> rdf:type owl:Class ;
                                                                                            rdfs:subClassOf <http://emmo.info/emmo/domain/mechanical-testing#EMMO_6e37e2b7_8cce_487c_ad40_36b4b7f030e3> ,
                                                                                                            <http://emmo.info/emmo/middle/math#EMMO_54ee6b5e_5261_44a8_86eb_5717e7fdb9d0> ;
                                                                                            rdfs:comment "It is a measure of central tendency in a data set. It is defined as the sum of a collection of numbers divided by the count of numbers in the collection." ;
                                                                                            <http://www.w3.org/2004/02/skos/core#prefLabel> "ArithmeticMean"@en .


###  http://emmo.info/emmo/domain/mechanical-testing#EMMO_5d4ab23c_859a_4def_844c_c57b82fea44d
<http://emmo.info/emmo/domain/mechanical-testing#EMMO_5d4ab23c_859a_4def_844c_c57b82fea44d> rdf:type owl:Class ;
                                                                                            rdfs:subClassOf <http://emmo.info/emmo/domain/mechanical-testing#EMMO_1cbdb7f5_47e4_468a_8d87_b25093803b8e> ;
                                                                                            <http://www.w3.org/2004/02/skos/core#prefLabel> "NanoindentationSpecimen"@en .


###  http://emmo.info/emmo/domain/mechanical-testing#EMMO_5dc819b6_0173_41ab_84b4_f4cc73a10a29
<http://emmo.info/emmo/domain/mechanical-testing#EMMO_5dc819b6_0173_41ab_84b4_f4cc73a10a29> rdf:type owl:Class ;
                                                                                            rdfs:subClassOf <http://emmo.info/emmo/domain/mechanical-testing#EMMO_e5d45f40_f9e9_47b9_934b_4c463a38b08e> ,
                                                                                                            <http://emmo.info/emmo/middle/isq#EMMO_cd2cd0de_e0cc_4ef1_b27e_2e88db027bac> ;
                                                                                            <http://www.w3.org/2004/02/skos/core#prefLabel> "Diameter"@en .


###  http://emmo.info/emmo/domain/mechanical-testing#EMMO_5dffae98_f5b7_4287_96ce_94f2314b8bae
<http://emmo.info/emmo/domain/mechanical-testing#EMMO_5dffae98_f5b7_4287_96ce_94f2314b8bae> rdf:type owl:Class ;
                                                                                            rdfs:subClassOf <http://emmo.info/emmo/domain/mechanical-testing#NanoindentationUseCase> ,
                                                                                                            <http://emmo.info/emmo/middle/metrology#EMMO_79751276_b2d0_4e2f_bbd4_99d412f43d55> ;
                                                                                            rdfs:comment "The loading rate required to achieve the Surface approach velocity. It depends on the value of the support springs stiffness (Spring stiffness)." ;
                                                                                            <http://www.w3.org/2004/02/skos/core#prefLabel> "ApproachLoadingRate"@en .


###  http://emmo.info/emmo/domain/mechanical-testing#EMMO_5f4390fd_cc6a_4f20_8af4_fe76d54af476
<http://emmo.info/emmo/domain/mechanical-testing#EMMO_5f4390fd_cc6a_4f20_8af4_fe76d54af476> rdf:type owl:Class ;
                                                                                            rdfs:subClassOf <http://emmo.info/emmo/domain/mechanical-testing#EMMO_e5d45f40_f9e9_47b9_934b_4c463a38b08e> ,
                                                                                                            <http://emmo.info/emmo/middle/chemistry#EMMO_4f40def1_3cd7_4067_9596_541e9a5134cf> ;
                                                                                            <http://www.w3.org/2004/02/skos/core#prefLabel> "ChromiumSymbol"@en .


###  http://emmo.info/emmo/domain/mechanical-testing#EMMO_5f5b81c8_f10a_409c_8ae7_20924f801826
<http://emmo.info/emmo/domain/mechanical-testing#EMMO_5f5b81c8_f10a_409c_8ae7_20924f801826> rdf:type owl:Class ;
                                                                                            rdfs:subClassOf <http://emmo.info/emmo/domain/mechanical-testing#EMMO_2e9a014f_9337_42f7_ad91_b73f150a9901> ;
                                                                                            <http://www.w3.org/2004/02/skos/core#prefLabel> "MartensiteHardening"@en .


###  http://emmo.info/emmo/domain/mechanical-testing#EMMO_606f7573_61f6_4bbd_8d42_1d86ab1caadb
<http://emmo.info/emmo/domain/mechanical-testing#EMMO_606f7573_61f6_4bbd_8d42_1d86ab1caadb> rdf:type owl:Class ;
                                                                                            rdfs:subClassOf <http://emmo.info/emmo/domain/mechanical-testing#EMMO_48e3eddc_de6b_4e9e_891d_99169d9f0883> ;
                                                                                            <http://www.w3.org/2004/02/skos/core#prefLabel> "SheetForming"@en .


###  http://emmo.info/emmo/domain/mechanical-testing#EMMO_6294b181_baf5_460a_9880_7f183bba9aae
<http://emmo.info/emmo/domain/mechanical-testing#EMMO_6294b181_baf5_460a_9880_7f183bba9aae> rdf:type owl:Class ;
                                                                                            rdfs:subClassOf <http://emmo.info/emmo/domain/mechanical-testing#EMMO_e5d45f40_f9e9_47b9_934b_4c463a38b08e> ,
                                                                                                            <http://emmo.info/emmo/middle/isq#EMMO_faab3f84_e475_4a46_af9c_7d249f0b9aef> ;
                                                                                            rdfs:comment """Stress ratio is defined as the ratio of minimum stress to maximum stress.
(need to add further logics)
Relation of S_min to S_max (R = S_min / S_max).
0 < R < 1 describes tension-tension loading,
R = 0 describes pulsating stress (S_m = S_a = S_max),
-1 < R < 0 describes partly reversed tension-compression loading,
R = -1 describes fully reversed loading,
-\"infinte\" < R < -1 describes partly reversed compression  loading,
R = -\"infinite\" is compression pulsating stress,
R > 1 describes compression-compression loading""" ;
                                                                                            <http://www.w3.org/2004/02/skos/core#prefLabel> "StressRatio"@en .


###  http://emmo.info/emmo/domain/mechanical-testing#EMMO_62bba151_6db3_4cb1_b3f7_ca42fe98f849
<http://emmo.info/emmo/domain/mechanical-testing#EMMO_62bba151_6db3_4cb1_b3f7_ca42fe98f849> rdf:type owl:Class ;
                                                                                            rdfs:subClassOf <http://emmo.info/emmo/domain/mechanical-testing#EMMO_48e3eddc_de6b_4e9e_891d_99169d9f0883> ;
                                                                                            <http://www.w3.org/2004/02/skos/core#prefLabel> "ColdWorking"@en .


###  http://emmo.info/emmo/domain/mechanical-testing#EMMO_6354c7de_cb63_446e_a6d0_f832844f0633
<http://emmo.info/emmo/domain/mechanical-testing#EMMO_6354c7de_cb63_446e_a6d0_f832844f0633> rdf:type owl:Class ;
                                                                                            rdfs:subClassOf <http://emmo.info/emmo/domain/mechanical-testing#EMMO_e5d45f40_f9e9_47b9_934b_4c463a38b08e> ,
                                                                                                            <http://emmo.info/emmo/middle/chemistry#EMMO_4f40def1_3cd7_4067_9596_541e9a5134cf> ;
                                                                                            <http://www.w3.org/2004/02/skos/core#prefLabel> "SulfurSymbol"@en .


###  http://emmo.info/emmo/domain/mechanical-testing#EMMO_63a2b220_31d4_4e65_92d4_82b2959a2949
<http://emmo.info/emmo/domain/mechanical-testing#EMMO_63a2b220_31d4_4e65_92d4_82b2959a2949> rdf:type owl:Class ;
                                                                                            rdfs:subClassOf <http://emmo.info/emmo/domain/mechanical-testing#EMMO_89be8d21_79a7_4970_9b0a_ee18cec63e62> ;
                                                                                            rdfs:comment """Steel category according to DIN standard:
Unalloyed construction, engineering and pressure vessel steels with
special requirements (DIN 10027-2)""" ;
                                                                                            rdfs:label "Unalloyed construction, engineering and pressure vessel steels with special requirements (DIN 10027-2)"@en ;
                                                                                            <http://www.w3.org/2004/02/skos/core#prefLabel> "UnalloyedConstructionEngineeringAndPressureVesselSteelsWithSpecialRequirementsDIN10027"@en .


###  http://emmo.info/emmo/domain/mechanical-testing#EMMO_646b0170_e349_4382_8291_4fa2cca982ea
<http://emmo.info/emmo/domain/mechanical-testing#EMMO_646b0170_e349_4382_8291_4fa2cca982ea> rdf:type owl:Class ;
                                                                                            rdfs:subClassOf <http://emmo.info/emmo/domain/mechanical-testing#EMMO_e5d45f40_f9e9_47b9_934b_4c463a38b08e> ,
                                                                                                            <http://emmo.info/emmo/middle/perceptual#EMMO_d8d2144e_5c8d_455d_a643_5caf4d8d9df8> ;
                                                                                            <http://www.w3.org/2004/02/skos/core#prefLabel> "LoadingEntity"@en .


###  http://emmo.info/emmo/domain/mechanical-testing#EMMO_66f6b324_8190_44d6_a504_0388d74c86be
<http://emmo.info/emmo/domain/mechanical-testing#EMMO_66f6b324_8190_44d6_a504_0388d74c86be> rdf:type owl:Class ;
                                                                                            rdfs:subClassOf <http://emmo.info/emmo/middle/chemistry#EMMO_a293f923_954c_4af5_9f97_9600ebd362cb> ,
                                                                                                            <http://emmo.info/emmo/middle/isq#EMMO_faab3f84_e475_4a46_af9c_7d249f0b9aef> ;
                                                                                            rdfs:comment "Austenite that does not transform to martensite upon quenching is called retained austenite.  This retained austenite occurs when the steel is not quenched to  a temperature low enough to form 100% martensite. Amount of austenite present in the microstructure after the hardening process is completed." ;
                                                                                            <http://www.w3.org/2004/02/skos/core#prefLabel> "RetainedAustenite"@en .


###  http://emmo.info/emmo/domain/mechanical-testing#EMMO_67869907_8e6e_45ac_87f7_41520e861b68
<http://emmo.info/emmo/domain/mechanical-testing#EMMO_67869907_8e6e_45ac_87f7_41520e861b68> rdf:type owl:Class ;
                                                                                            rdfs:subClassOf <http://emmo.info/emmo/domain/mechanical-testing#EMMO_c799b443_c70f_4351_bb0f_e4ab29073481> ;
                                                                                            rdfs:comment "Value of the hardness, measured along the cross section of the material." ;
                                                                                            <http://www.w3.org/2004/02/skos/core#prefLabel> "CoreHardness"@en .


###  http://emmo.info/emmo/domain/mechanical-testing#EMMO_67c583bf_57d9_4580_b68c_d16b40564b23
<http://emmo.info/emmo/domain/mechanical-testing#EMMO_67c583bf_57d9_4580_b68c_d16b40564b23> rdf:type owl:Class ;
                                                                                            rdfs:subClassOf <http://emmo.info/emmo/domain/mechanical-testing#EMMO_c8e9f573_1b9a_48f6_a274_61a441f3a7c4> ;
                                                                                            rdfs:comment """Steel category according to DIN standard:
Cr-Mo-V Tool Steels (DIN 10027-2)"""@en ;
                                                                                            <http://www.w3.org/2004/02/skos/core#prefLabel> "CrMoVToolSteelsDIN10027"@en .


###  http://emmo.info/emmo/domain/mechanical-testing#EMMO_68856430_66a2_49fb_b93f_e7124effb6bd
<http://emmo.info/emmo/domain/mechanical-testing#EMMO_68856430_66a2_49fb_b93f_e7124effb6bd> rdf:type owl:Class ;
                                                                                            rdfs:subClassOf <http://emmo.info/emmo/domain/mechanical-testing#EMMO_91e9c813_b277_48ad_b5b0_a781a05b9c1f> ,
                                                                                                            <http://emmo.info/emmo/middle/isq#EMMO_cd2cd0de_e0cc_4ef1_b27e_2e88db027bac> ;
                                                                                            rdfs:comment "The distance from the last known value of the displacement associated with the surface at which the system will establish the Approach Velocity and start looking for the surface." ;
                                                                                            <http://www.w3.org/2004/02/skos/core#prefLabel> "SurfaceApproachDistance"@en .


###  http://emmo.info/emmo/domain/mechanical-testing#EMMO_68bc845c_5943_47da_ba95_b265bb3780a2
<http://emmo.info/emmo/domain/mechanical-testing#EMMO_68bc845c_5943_47da_ba95_b265bb3780a2> rdf:type owl:Class ;
                                                                                            rdfs:subClassOf <http://emmo.info/emmo/domain/mechanical-testing#CableBundleUseCase> ,
                                                                                                            <http://emmo.info/emmo/domain/mechanical-testing#EMMO_e5d45f40_f9e9_47b9_934b_4c463a38b08e> ,
                                                                                                            <http://emmo.info/emmo/domain/mechanical-testing#NanoindentationUseCase> ,
                                                                                                            <http://emmo.info/emmo/middle/manufacturing#EMMO_ec7464a9_d99d_45f8_965b_4e9230ea8356> ;
                                                                                            <http://www.w3.org/2004/02/skos/core#prefLabel> "MetalSheet"@en .


###  http://emmo.info/emmo/domain/mechanical-testing#EMMO_68ee637e_eee7_4edc_ab24_1fe4135fb71c
<http://emmo.info/emmo/domain/mechanical-testing#EMMO_68ee637e_eee7_4edc_ab24_1fe4135fb71c> rdf:type owl:Class ;
                                                                                            rdfs:subClassOf <http://emmo.info/emmo/domain/mechanical-testing#EMMO_e5d45f40_f9e9_47b9_934b_4c463a38b08e> ,
                                                                                                            <http://emmo.info/emmo/middle/isq#EMMO_faab3f84_e475_4a46_af9c_7d249f0b9aef> ;
                                                                                            rdfs:comment "The stress concentration factor Kt expresses the ratio of the highest stress to a nominal stress of the cross cross section (Kt = S_max/S_nominal). For an unnotched specimen, K_t = 1, for notched specimens K_t > 1" ;
                                                                                            <http://www.w3.org/2004/02/skos/core#prefLabel> "StressConcentrationFactor"@en .


###  http://emmo.info/emmo/domain/mechanical-testing#EMMO_68efbbca_549a_4209_bdfc_cf0ddfd27dc9
<http://emmo.info/emmo/domain/mechanical-testing#EMMO_68efbbca_549a_4209_bdfc_cf0ddfd27dc9> rdf:type owl:Class ;
                                                                                            rdfs:subClassOf <http://emmo.info/emmo/domain/mechanical-testing#EMMO_91e9c813_b277_48ad_b5b0_a781a05b9c1f> ,
                                                                                                            <http://emmo.info/emmo/middle/isq#EMMO_0329f1f5_8339_4ce4_8505_a264c6d606ba> ;
                                                                                            rdfs:comment "The velocity of the probe as it approaches the surface." ;
                                                                                            <http://www.w3.org/2004/02/skos/core#prefLabel> "SurfaceApproachVelocity"@en .


###  http://emmo.info/emmo/domain/mechanical-testing#EMMO_698316f5_e359_4774_b7fb_a0967be129bb
<http://emmo.info/emmo/domain/mechanical-testing#EMMO_698316f5_e359_4774_b7fb_a0967be129bb> rdf:type owl:Class ;
                                                                                            rdfs:subClassOf <http://emmo.info/emmo/domain/mechanical-testing#EMMO_c8e9f573_1b9a_48f6_a274_61a441f3a7c4> ;
                                                                                            rdfs:comment """Steel category according to JIS standard:
Alloyed tool steels (JIS)""" ;
                                                                                            rdfs:label "Alloyed tool steels (JIS)"@en ;
                                                                                            <http://www.w3.org/2004/02/skos/core#prefLabel> "AlloyedToolSteelsJIS"@en .


###  http://emmo.info/emmo/domain/mechanical-testing#EMMO_6a8bfa0e_ef96_4f38_b892_40389eb7d69d
<http://emmo.info/emmo/domain/mechanical-testing#EMMO_6a8bfa0e_ef96_4f38_b892_40389eb7d69d> rdf:type owl:Class ;
                                                                                            rdfs:subClassOf <http://emmo.info/emmo/domain/mechanical-testing#EMMO_91e9c813_b277_48ad_b5b0_a781a05b9c1f> ,
                                                                                                            <http://emmo.info/emmo/domain/mechanical-testing#EMMO_ee09aa64_f477_4e8f_8b0c_f5d30177ba8d> ;
                                                                                            rdfs:comment "The targeted maximum depth. The experiment will stop loading at this point or if the maximum target load is reached." ;
                                                                                            <http://www.w3.org/2004/02/skos/core#prefLabel> "TargetDepth"@en .


###  http://emmo.info/emmo/domain/mechanical-testing#EMMO_6b218da5_9a74_43fe_a71d_72c13dae4551
<http://emmo.info/emmo/domain/mechanical-testing#EMMO_6b218da5_9a74_43fe_a71d_72c13dae4551> rdf:type owl:Class ;
                                                                                            rdfs:subClassOf <http://emmo.info/emmo/domain/mechanical-testing#NanoindentationUseCase> ,
                                                                                                            <http://emmo.info/emmo/middle/isq#EMMO_cd2cd0de_e0cc_4ef1_b27e_2e88db027bac> ;
                                                                                            rdfs:comment "The position of the actuator relative to the last point at which it was zeroed." ;
                                                                                            <http://www.w3.org/2004/02/skos/core#prefLabel> "Extension"@en .


###  http://emmo.info/emmo/domain/mechanical-testing#EMMO_6b496d19_be97_4391_bd71_7e1f003989f6
<http://emmo.info/emmo/domain/mechanical-testing#EMMO_6b496d19_be97_4391_bd71_7e1f003989f6> rdf:type owl:Class ;
                                                                                            rdfs:subClassOf <http://emmo.info/emmo/domain/mechanical-testing#EMMO_89be8d21_79a7_4970_9b0a_ee18cec63e62> ;
                                                                                            rdfs:comment """Steel category according to DIN standard:
Unalloyed construction, engineering and pressure vessel steels with C > 0,5 % (DIN 10027-2)""" ;
                                                                                            rdfs:label "Unalloyed construction, engineering and pressure vessel steels with C > 0,5 % (DIN 10027-2)"@en ;
                                                                                            <http://www.w3.org/2004/02/skos/core#prefLabel> "UnalloyedConstructionEngineeringAndPressureVesselSteelsWithCAbove0p5PercentDIN10027"@en .


###  http://emmo.info/emmo/domain/mechanical-testing#EMMO_6bc4fa0e_67f8_4638_bfa4_6f660a00c687
<http://emmo.info/emmo/domain/mechanical-testing#EMMO_6bc4fa0e_67f8_4638_bfa4_6f660a00c687> rdf:type owl:Class ;
                                                                                            rdfs:subClassOf <http://emmo.info/emmo/middle/metrology#EMMO_3ee80521_3c23_4dd1_935d_9d522614a3e2> ;
                                                                                            <http://www.w3.org/2004/02/skos/core#prefLabel> "Pascal"@en .


###  http://emmo.info/emmo/domain/mechanical-testing#EMMO_6d7b5fe0_36a2_4638_8c1c_a1bf399624c1
<http://emmo.info/emmo/domain/mechanical-testing#EMMO_6d7b5fe0_36a2_4638_8c1c_a1bf399624c1> rdf:type owl:Class ;
                                                                                            rdfs:subClassOf <http://emmo.info/emmo/domain/mechanical-testing#EMMO_91e9c813_b277_48ad_b5b0_a781a05b9c1f> ,
                                                                                                            <http://emmo.info/emmo/middle/isq#EMMO_852b4ab8_fc29_4749_a8c7_b92d4fca7d5a> ;
                                                                                            rdfs:comment "The frequency used to excite the contact for dynamic testing. The dynamic force will be oscillated at this frequency." ;
                                                                                            <http://www.w3.org/2004/02/skos/core#prefLabel> "TargetFrequency"@en .


###  http://emmo.info/emmo/domain/mechanical-testing#EMMO_6dee097b_7b39_4299_a322_b83eb2948428
<http://emmo.info/emmo/domain/mechanical-testing#EMMO_6dee097b_7b39_4299_a322_b83eb2948428> rdf:type owl:Class ;
                                                                                            rdfs:subClassOf <http://emmo.info/emmo/domain/mechanical-testing#EMMO_91e9c813_b277_48ad_b5b0_a781a05b9c1f> ;
                                                                                            rdfs:comment "This value is used to control Dynamic Force to obtain a constant value of Dynamic Displacement." ;
                                                                                            <http://www.w3.org/2004/02/skos/core#prefLabel> "DynamicLoadRequired"@en .


###  http://emmo.info/emmo/domain/mechanical-testing#EMMO_6e37e2b7_8cce_487c_ad40_36b4b7f030e3
<http://emmo.info/emmo/domain/mechanical-testing#EMMO_6e37e2b7_8cce_487c_ad40_36b4b7f030e3> rdf:type owl:Class ;
                                                                                            rdfs:subClassOf <http://emmo.info/emmo/domain/mechanical-testing#EMMO_0747262d_9356_4b7b_ac5d_90e2504e0968> ;
                                                                                            rdfs:comment "Mesomics bending analysis is a general class that is used to represent the set of Mesomics bensing analysis post-processing calculations." ;
                                                                                            <http://www.w3.org/2004/02/skos/core#prefLabel> "MesomicsBendingAnalysis"@en .


###  http://emmo.info/emmo/domain/mechanical-testing#EMMO_6e59c5d5_6b2c_46a6_a598_ae692a35a4dc
<http://emmo.info/emmo/domain/mechanical-testing#EMMO_6e59c5d5_6b2c_46a6_a598_ae692a35a4dc> rdf:type owl:Class ;
                                                                                            rdfs:subClassOf <http://emmo.info/emmo/domain/mechanical-testing#EMMO_23273603_7ee7_4012_a0bb_d484433083de> ;
                                                                                            <http://www.w3.org/2004/02/skos/core#prefLabel> "SingleStepLoading" .


###  http://emmo.info/emmo/domain/mechanical-testing#EMMO_6e5dfdf2_c936_479c_a4dd_2eb50084c4a1
<http://emmo.info/emmo/domain/mechanical-testing#EMMO_6e5dfdf2_c936_479c_a4dd_2eb50084c4a1> rdf:type owl:Class ;
                                                                                            rdfs:subClassOf <http://emmo.info/emmo/domain/mechanical-testing#EMMO_e5d45f40_f9e9_47b9_934b_4c463a38b08e> ,
                                                                                                            <http://emmo.info/emmo/middle/isq#EMMO_f3dd74c0_f480_49e8_9764_33b78638c235> ;
                                                                                            rdfs:comment "Specification of the rolling direction. Metal stock is passed through one or more pairs of rolls to reduce thickness, to make the thickness uniform, and/or to impart a desired mechanical property." ;
                                                                                            <http://www.w3.org/2004/02/skos/core#prefLabel> "RollingDirection"@en .


###  http://emmo.info/emmo/domain/mechanical-testing#EMMO_6f5deb88_b02f_48a1_b177_ea123082d703
<http://emmo.info/emmo/domain/mechanical-testing#EMMO_6f5deb88_b02f_48a1_b177_ea123082d703> rdf:type owl:Class ;
                                                                                            rdfs:subClassOf <http://emmo.info/emmo/domain/mechanical-testing#EMMO_4c25ab1b_462c_49a6_bb27_ea3bd020ab2a> ;
                                                                                            rdfs:comment "Annealing is a heat treatment that alters the physical and sometimes chemical properties of a material to increase ist ductility and reduce ist hardness, making it more workable. It involves heating a material above ist recrystallization temperature, maintaining a suitable temperature for an appropriate amount of time and then cooling." ;
                                                                                            <http://www.w3.org/2004/02/skos/core#prefLabel> "Annealing"@en .


###  http://emmo.info/emmo/domain/mechanical-testing#EMMO_6f7c111f_ac09_48e9_9a26_575bf4ed878e
<http://emmo.info/emmo/domain/mechanical-testing#EMMO_6f7c111f_ac09_48e9_9a26_575bf4ed878e> rdf:type owl:Class ;
                                                                                            rdfs:subClassOf <http://emmo.info/emmo/domain/mechanical-testing#EMMO_91e9c813_b277_48ad_b5b0_a781a05b9c1f> ,
                                                                                                            <http://emmo.info/emmo/domain/mechanical-testing#EMMO_ca42ed31_3983_4e1a_84f9_a84cab2cdb59> ;
                                                                                            rdfs:comment "The system will try to maintain this value of the Dynamic displacement as long as the Dynamic load is less than Dynamic max fraction of load fraction of the applied load." ;
                                                                                            <http://www.w3.org/2004/02/skos/core#prefLabel> "TargetDynamicDisplacement"@en .


###  http://emmo.info/emmo/domain/mechanical-testing#EMMO_6f7f288a_ec43_41f7_ac6c_8e4941d2d29d
<http://emmo.info/emmo/domain/mechanical-testing#EMMO_6f7f288a_ec43_41f7_ac6c_8e4941d2d29d> rdf:type owl:Class ;
                                                                                            rdfs:subClassOf <http://emmo.info/emmo/domain/mechanical-testing#CableBundleUseCase> ,
                                                                                                            <http://emmo.info/emmo/middle/manufacturing#EMMO_494b372c_cfdf_47d3_a4de_5e037c540de8> ;
                                                                                            rdfs:comment "An optional description of single cable details. The cable core usually corresponds to the conducting metal part." ;
                                                                                            <http://www.w3.org/2004/02/skos/core#prefLabel> "CableCore"@en .


###  http://emmo.info/emmo/domain/mechanical-testing#EMMO_709d4e04_e972_4f57_9589_bf99ea08d2ea
<http://emmo.info/emmo/domain/mechanical-testing#EMMO_709d4e04_e972_4f57_9589_bf99ea08d2ea> rdf:type owl:Class ;
                                                                                            rdfs:subClassOf <http://emmo.info/emmo/domain/mechanical-testing#CableBundleUseCase> ,
                                                                                                            <http://emmo.info/emmo/middle/manufacturing#EMMO_ec7464a9_d99d_45f8_965b_4e9230ea8356> ;
                                                                                            rdfs:comment "An electrical insulating material is a material that reduces or prevents the transmission of heat, sound or electricity. For instance, an electrical insulating material prevents electricity  voltage-carrying conductors against one another as well as against earth." ;
                                                                                            <http://www.w3.org/2004/02/skos/core#prefLabel> "InsulatingMaterial"@en .


###  http://emmo.info/emmo/domain/mechanical-testing#EMMO_71200c24_44fe_4533_96be_55ecb299681c
<http://emmo.info/emmo/domain/mechanical-testing#EMMO_71200c24_44fe_4533_96be_55ecb299681c> rdf:type owl:Class ;
                                                                                            rdfs:subClassOf <http://emmo.info/emmo/domain/mechanical-testing#EMMO_3c93b3eb_f08f_4c25_940c_fac690e012c6> ;
                                                                                            <http://emmo.info/emmo/top/annotations#EMMO_967080e5_2f42_4eb2_a3a9_c58143e835f9> "Label after DIN EN 10027-1, often short form of material name." ;
                                                                                            rdfs:comment "Deutsches Institut fr Normung" ;
                                                                                            rdfs:seeAlso "https://www.beuth.de/en/standard/din-en-10027-1/262540217" ;
                                                                                            <http://www.w3.org/2004/02/skos/core#prefLabel> "ShortName"@en .


###  http://emmo.info/emmo/domain/mechanical-testing#EMMO_71f86460_7451_43be_9e29_bb653724e231
<http://emmo.info/emmo/domain/mechanical-testing#EMMO_71f86460_7451_43be_9e29_bb653724e231> rdf:type owl:Class ;
                                                                                            rdfs:subClassOf <http://emmo.info/emmo/domain/mechanical-testing#EMMO_2a706af8_27ae_468f_9688_fbbe4ca13a86> ;
                                                                                            rdfs:comment "Crack-origin at specimen surface." ;
                                                                                            <http://www.w3.org/2004/02/skos/core#prefLabel> "SurfaceFailure"@en .


###  http://emmo.info/emmo/domain/mechanical-testing#EMMO_73e0c7f8_20db_46c7_af69_22ad5616f8dc
<http://emmo.info/emmo/domain/mechanical-testing#EMMO_73e0c7f8_20db_46c7_af69_22ad5616f8dc> rdf:type owl:Class ;
                                                                                            rdfs:subClassOf <http://emmo.info/emmo/domain/mechanical-testing#EMMO_91e9c813_b277_48ad_b5b0_a781a05b9c1f> ;
                                                                                            rdfs:comment "The displacement resolution is typically found by dividing the maximum displacement voltage reading by the number of bits in the data acquisition system." ;
                                                                                            <http://www.w3.org/2004/02/skos/core#prefLabel> "DisplacementResolution"@en .


###  http://emmo.info/emmo/domain/mechanical-testing#EMMO_740dc009_8db5_4a11_b063_206016ec6cc9
<http://emmo.info/emmo/domain/mechanical-testing#EMMO_740dc009_8db5_4a11_b063_206016ec6cc9> rdf:type owl:Class ;
                                                                                            rdfs:subClassOf <http://emmo.info/emmo/domain/mechanical-testing#EMMO_e5d45f40_f9e9_47b9_934b_4c463a38b08e> ;
                                                                                            rdfs:comment "Comment on unique features of the failure" ;
                                                                                            <http://www.w3.org/2004/02/skos/core#prefLabel> "FailureComment"@en .


###  http://emmo.info/emmo/domain/mechanical-testing#EMMO_7452b52c_82ea_47da_b84f_493317c8f03e
<http://emmo.info/emmo/domain/mechanical-testing#EMMO_7452b52c_82ea_47da_b84f_493317c8f03e> rdf:type owl:Class ;
                                                                                            rdfs:subClassOf <http://emmo.info/emmo/domain/mechanical-testing#EMMO_16cfb313_1fea_414f_99ca_aec999e93e0c> ;
                                                                                            rdfs:comment "Steel nomenclature contains steel groups / categories as defined in the standards DIN, SAE and JIS and superclasses in which the categories from the different standards are combined" ;
                                                                                            rdfs:label "Alloyed steels"@en ;
                                                                                            <http://www.w3.org/2004/02/skos/core#prefLabel> "AlloyedSteels"@en .


###  http://emmo.info/emmo/domain/mechanical-testing#EMMO_7461cbb7_9056_48ba_87fc_a2693a086c71
<http://emmo.info/emmo/domain/mechanical-testing#EMMO_7461cbb7_9056_48ba_87fc_a2693a086c71> rdf:type owl:Class ;
                                                                                            rdfs:subClassOf <http://emmo.info/emmo/domain/mechanical-testing#EMMO_9d621c9b_9c52_4084_af20_b2dfda89fe6c> ;
                                                                                            <http://www.w3.org/2004/02/skos/core#prefLabel> "NanoindentationMeasurement"@en .


###  http://emmo.info/emmo/domain/mechanical-testing#EMMO_74c9f630_5e5e_4503_9f03_d84228ed405f
<http://emmo.info/emmo/domain/mechanical-testing#EMMO_74c9f630_5e5e_4503_9f03_d84228ed405f> rdf:type owl:Class ;
                                                                                            rdfs:subClassOf <http://emmo.info/emmo/domain/mechanical-testing#EMMO_06390646_6edb_4410_b22b_f7adbd6025c4> ;
                                                                                            rdfs:comment "Cementite (or iron carbide) is a compound of iron and carbon, more precisely an intermediate transition metal carbide with the formula Fe3C. By weight, it is 6.67% carbon and 93.3% iron. It has an orthorhombic crystal structure." ;
                                                                                            rdfs:label "Cementite"@en ;
                                                                                            <http://www.w3.org/2004/02/skos/core#prefLabel> "Cementite" .


###  http://emmo.info/emmo/domain/mechanical-testing#EMMO_76471eff_11f6_4b51_a6e0_3923a7ecfa2e
<http://emmo.info/emmo/domain/mechanical-testing#EMMO_76471eff_11f6_4b51_a6e0_3923a7ecfa2e> rdf:type owl:Class ;
                                                                                            rdfs:subClassOf <http://emmo.info/emmo/domain/mechanical-testing#EMMO_7452b52c_82ea_47da_b84f_493317c8f03e> ;
                                                                                            rdfs:comment "Steel nomenclature contains steel groups / categories as defined in the standards DIN, SAE and JIS and superclasses in which the categories from the different standards are combined" ;
                                                                                            rdfs:label "Construction steels"@en ;
                                                                                            <http://www.w3.org/2004/02/skos/core#prefLabel> "ConstructionSteels"@en .


###  http://emmo.info/emmo/domain/mechanical-testing#EMMO_76dba92f_a761_409f_83d8_5a0c9c73b349
<http://emmo.info/emmo/domain/mechanical-testing#EMMO_76dba92f_a761_409f_83d8_5a0c9c73b349> rdf:type owl:Class ;
                                                                                            rdfs:subClassOf <http://emmo.info/emmo/domain/mechanical-testing#EMMO_f210d615_89a5_483f_a8b2_923ff6fcf4ab> ;
                                                                                            <http://www.w3.org/2004/02/skos/core#prefLabel> "IndentationTestPostProcessing"@en .


###  http://emmo.info/emmo/domain/mechanical-testing#EMMO_77cfb822_431d_436f_8617_ceb4a461b403
<http://emmo.info/emmo/domain/mechanical-testing#EMMO_77cfb822_431d_436f_8617_ceb4a461b403> rdf:type owl:Class ;
                                                                                            rdfs:subClassOf <http://emmo.info/emmo/domain/mechanical-testing#EMMO_8630b1ff_7985_444e_8572_373816c0d3b5> ;
                                                                                            rdfs:comment """Steel category according to JIS standard:
High carbon steel wire rods (JIS)""" ;
                                                                                            rdfs:label "High carbon steel wire rods (JIS)"@en ;
                                                                                            <http://www.w3.org/2004/02/skos/core#prefLabel> "HighCarbonSteelWireRodsJIS"@en .


###  http://emmo.info/emmo/domain/mechanical-testing#EMMO_78ddc826_66d5_4be3_8eeb_d8b39e02c9d6
<http://emmo.info/emmo/domain/mechanical-testing#EMMO_78ddc826_66d5_4be3_8eeb_d8b39e02c9d6> rdf:type owl:Class ;
                                                                                            rdfs:subClassOf <http://emmo.info/emmo/domain/mechanical-testing#EMMO_e5d45f40_f9e9_47b9_934b_4c463a38b08e> ,
                                                                                                            <http://emmo.info/emmo/middle/isq#EMMO_faab3f84_e475_4a46_af9c_7d249f0b9aef> ;
                                                                                            rdfs:comment """The mean stress factor is a numerical value calculated by the mean stress sensitivity and the stress ratio. The formula is depending on the stress ratio value. The mean stress factor indicates the influence of mean stress on the fatigue strength of a material (see \"FKM-Richtlinie - Rechnerischer Festigkeitsnachweis (2012)\")
mean stress factor K_AK = f(M_sig, R)"""@en ;
                                                                                            <http://www.w3.org/2004/02/skos/core#prefLabel> "MeanStressFactor"@en .


###  http://emmo.info/emmo/domain/mechanical-testing#EMMO_795fa324_2330_44ee_90c7_5bbf59c1ec53
<http://emmo.info/emmo/domain/mechanical-testing#EMMO_795fa324_2330_44ee_90c7_5bbf59c1ec53> rdf:type owl:Class ;
                                                                                            rdfs:subClassOf <http://emmo.info/emmo/domain/mechanical-testing#EMMO_e5d45f40_f9e9_47b9_934b_4c463a38b08e> ,
                                                                                                            <http://emmo.info/emmo/middle/chemistry#EMMO_4f40def1_3cd7_4067_9596_541e9a5134cf> ;
                                                                                            <http://www.w3.org/2004/02/skos/core#prefLabel> "CopperSymbol"@en .


###  http://emmo.info/emmo/domain/mechanical-testing#EMMO_7aa20434_165d_414f_a945_b57bd849e43b
<http://emmo.info/emmo/domain/mechanical-testing#EMMO_7aa20434_165d_414f_a945_b57bd849e43b> rdf:type owl:Class ;
                                                                                            rdfs:subClassOf <http://emmo.info/emmo/domain/mechanical-testing#NanoindentationUseCase> ,
                                                                                                            <http://emmo.info/emmo/middle/math#EMMO_4bc29b0f_8fcc_4026_a291_f9774a66d9b8> ;
                                                                                            rdfs:comment "The area function that describes the geometry according to which the indenter tip diamond end is cut: three sided pyramids, four sided pyramids, wedges, cones, cylinders or spheres. The tip end of the indenter can be made sharp, flat, or rounded to a cylindrical or spherical shape. All these features of the indenter tip can be described with a mathematical function." ;
                                                                                            <http://www.w3.org/2004/02/skos/core#prefLabel> "IndenterTipAreaFunction"@en .


###  http://emmo.info/emmo/domain/mechanical-testing#EMMO_7ac33acb_e6b5_4660_86d3_3a174c3486b7
<http://emmo.info/emmo/domain/mechanical-testing#EMMO_7ac33acb_e6b5_4660_86d3_3a174c3486b7> rdf:type owl:Class ;
                                                                                            rdfs:subClassOf <http://emmo.info/emmo/domain/mechanical-testing#EMMO_e5d45f40_f9e9_47b9_934b_4c463a38b08e> ,
                                                                                                            <http://emmo.info/emmo/middle/chemistry#EMMO_4f40def1_3cd7_4067_9596_541e9a5134cf> ;
                                                                                            <http://www.w3.org/2004/02/skos/core#prefLabel> "ManganeseSymbol"@en .


###  http://emmo.info/emmo/domain/mechanical-testing#EMMO_7bbc9593_ad1d_4e80_a957_815b7daca408
<http://emmo.info/emmo/domain/mechanical-testing#EMMO_7bbc9593_ad1d_4e80_a957_815b7daca408> rdf:type owl:Class ;
                                                                                            rdfs:subClassOf <http://emmo.info/emmo/domain/mechanical-testing#EMMO_2f9a266b_ffe6_4b3e_8222_eca6001174a2> ;
                                                                                            <http://www.w3.org/2004/02/skos/core#prefLabel> "PendantDropMethod"@en .


###  http://emmo.info/emmo/domain/mechanical-testing#EMMO_7dc73553_7d3f_4dc2_bb7b_f47775207457
<http://emmo.info/emmo/domain/mechanical-testing#EMMO_7dc73553_7d3f_4dc2_bb7b_f47775207457> rdf:type owl:Class ;
                                                                                            owl:equivalentClass <http://emmo.info/emmo/domain/mechanical-testing#EMMO_f0ad542d_ff13_4998_9e7f_ea27583c5f31> ;
                                                                                            rdfs:subClassOf <http://emmo.info/emmo/domain/mechanical-testing#NanoindentationUseCase> ,
                                                                                                            <http://emmo.info/emmo/middle/metrology#EMMO_71f6ab56_342c_484b_bbe0_de86b7367cb3> ;
                                                                                            rdfs:comment "Describes the stiffness, which is the ability of a material to withstand elastic deformation." ;
                                                                                            <http://www.w3.org/2004/02/skos/core#prefLabel> "YoungsModulus"@en .


###  http://emmo.info/emmo/domain/mechanical-testing#EMMO_7de63ea0_5f60_4818_8dba_5df52ac11c77
<http://emmo.info/emmo/domain/mechanical-testing#EMMO_7de63ea0_5f60_4818_8dba_5df52ac11c77> rdf:type owl:Class ;
                                                                                            rdfs:subClassOf <http://emmo.info/emmo/domain/mechanical-testing#EMMO_8630b1ff_7985_444e_8572_373816c0d3b5> ;
                                                                                            rdfs:comment """Steel category according to DIN standard:
Materials with increased temperature properties (DIN 10027-2)""" ;
                                                                                            rdfs:label "Materials with increased temperature properties (DIN 10027-2)"@en ;
                                                                                            <http://www.w3.org/2004/02/skos/core#prefLabel> "MaterialsWithIncreasedTemperaturePropertiesDIN10027"@en .


###  http://emmo.info/emmo/domain/mechanical-testing#EMMO_804ada5e_70bf_451f_b3dc_868631b22b05
<http://emmo.info/emmo/domain/mechanical-testing#EMMO_804ada5e_70bf_451f_b3dc_868631b22b05> rdf:type owl:Class ;
                                                                                            rdfs:subClassOf <http://emmo.info/emmo/domain/mechanical-testing#EMMO_e5d45f40_f9e9_47b9_934b_4c463a38b08e> ,
                                                                                                            <http://emmo.info/emmo/middle/properties#EMMO_463bcfda_867b_41d9_a967_211d4d437cfb> ;
                                                                                            <http://www.w3.org/2004/02/skos/core#prefLabel> "TensileTestMeasurement"@en .


###  http://emmo.info/emmo/domain/mechanical-testing#EMMO_80a5c2f7_deda_411a_842a_9e023bddde65
<http://emmo.info/emmo/domain/mechanical-testing#EMMO_80a5c2f7_deda_411a_842a_9e023bddde65> rdf:type owl:Class ;
                                                                                            rdfs:subClassOf <http://emmo.info/emmo/domain/mechanical-testing#EMMO_24af8df2_9438_44f6_8c5f_755beb459a49> ;
                                                                                            rdfs:comment "Corresponds to the Yield stress at 0.1% plastic strain." ;
                                                                                            <http://www.w3.org/2004/02/skos/core#prefLabel> "RP0.1"@en .


###  http://emmo.info/emmo/domain/mechanical-testing#EMMO_8101f160_1b9c_49cc_8e37_6eb832f85b4b
<http://emmo.info/emmo/domain/mechanical-testing#EMMO_8101f160_1b9c_49cc_8e37_6eb832f85b4b> rdf:type owl:Class ;
                                                                                            rdfs:subClassOf <http://emmo.info/emmo/domain/mechanical-testing#EMMO_e5d45f40_f9e9_47b9_934b_4c463a38b08e> ,
                                                                                                            <http://emmo.info/emmo/middle/chemistry#EMMO_4f40def1_3cd7_4067_9596_541e9a5134cf> ;
                                                                                            <http://www.w3.org/2004/02/skos/core#prefLabel> "CarbonSymbol"@en .


###  http://emmo.info/emmo/domain/mechanical-testing#EMMO_81c57565_463f_4281_bd64_59eb7a56c952
<http://emmo.info/emmo/domain/mechanical-testing#EMMO_81c57565_463f_4281_bd64_59eb7a56c952> rdf:type owl:Class ;
                                                                                            rdfs:subClassOf <http://emmo.info/emmo/domain/mechanical-testing#EMMO_b71e5f70_227c_4798_8a8a_ee7b70afd10f> ;
                                                                                            rdfs:comment "Polishingandbuffingarefinishingprocesses for smoothing a workpiece's surface. While used less extensively than traditional mechanical polishing, electropolishing is an alternative form of polishing that uses the principles of electrochemistry to remove microscopic layers of metal from a base surface." ;
                                                                                            <http://www.w3.org/2004/02/skos/core#altLabel> "Buffing" ;
                                                                                            <http://www.w3.org/2004/02/skos/core#prefLabel> "Polishing" .


###  http://emmo.info/emmo/domain/mechanical-testing#EMMO_81dd7f19_073d_4153_9517_823edac9fac7
<http://emmo.info/emmo/domain/mechanical-testing#EMMO_81dd7f19_073d_4153_9517_823edac9fac7> rdf:type owl:Class ;
                                                                                            rdfs:subClassOf <http://emmo.info/emmo/domain/mechanical-testing#EMMO_580f1bd6_5505_4f31_9a8a_b4e9a17bc604> ;
                                                                                            rdfs:comment "Represents a cable bundle cover based on Tape and how the tape is placed across the bundle." ;
                                                                                            <http://www.w3.org/2004/02/skos/core#prefLabel> "Taping"@en .


###  http://emmo.info/emmo/domain/mechanical-testing#EMMO_82723ac0_2abd_46d4_a850_7616d1ac2fa0
<http://emmo.info/emmo/domain/mechanical-testing#EMMO_82723ac0_2abd_46d4_a850_7616d1ac2fa0> rdf:type owl:Class ;
                                                                                            rdfs:subClassOf <http://emmo.info/emmo/domain/mechanical-testing#EMMO_442c0fb7_09d4_4dae_b45c_8eb1522da38f> ;
                                                                                            rdfs:comment "Technique for obtaining elastic modulus and hardness data continuously during a nanoindentation process." ;
                                                                                            <http://www.w3.org/2004/02/skos/core#prefLabel> "ContinuousStiffnessMeasurementMethod"@en .


###  http://emmo.info/emmo/domain/mechanical-testing#EMMO_841ccb1b_518f_4277_baf5_8f97529dfb00
<http://emmo.info/emmo/domain/mechanical-testing#EMMO_841ccb1b_518f_4277_baf5_8f97529dfb00> rdf:type owl:Class ;
                                                                                            rdfs:subClassOf <http://emmo.info/emmo/domain/mechanical-testing#EMMO_e5d45f40_f9e9_47b9_934b_4c463a38b08e> ,
                                                                                                            <http://emmo.info/emmo/middle/chemistry#EMMO_4f40def1_3cd7_4067_9596_541e9a5134cf> ;
                                                                                            <http://www.w3.org/2004/02/skos/core#prefLabel> "NickelSymbol"@en .


###  http://emmo.info/emmo/domain/mechanical-testing#EMMO_851f6719_2e5c_454b_b0d1_439fbdac11b5
<http://emmo.info/emmo/domain/mechanical-testing#EMMO_851f6719_2e5c_454b_b0d1_439fbdac11b5> rdf:type owl:Class ;
                                                                                            rdfs:subClassOf <http://emmo.info/emmo/domain/mechanical-testing#EMMO_81dd7f19_073d_4153_9517_823edac9fac7> ;
                                                                                            rdfs:comment "Taping that covers half of he cable bundle lateral surface area." ;
                                                                                            <http://www.w3.org/2004/02/skos/core#prefLabel> "HalfTaping"@en .


###  http://emmo.info/emmo/domain/mechanical-testing#EMMO_8571817a_da81_42c2_b97d_ba974d0119b1
<http://emmo.info/emmo/domain/mechanical-testing#EMMO_8571817a_da81_42c2_b97d_ba974d0119b1> rdf:type owl:Class ;
                                                                                            rdfs:subClassOf <http://emmo.info/emmo/domain/mechanical-testing#EMMO_cc1df6d0_cf70_41e1_b757_7bdad7cc459e> ;
                                                                                            rdfs:comment """Steel category according to JIS standard:
Spring steels (JIS)""" ;
                                                                                            rdfs:label "Spring steels (JIS)"@en ;
                                                                                            <http://www.w3.org/2004/02/skos/core#prefLabel> "SpringSteelsJIS"@en .


###  http://emmo.info/emmo/domain/mechanical-testing#EMMO_8630b1ff_7985_444e_8572_373816c0d3b5
<http://emmo.info/emmo/domain/mechanical-testing#EMMO_8630b1ff_7985_444e_8572_373816c0d3b5> rdf:type owl:Class ;
                                                                                            rdfs:subClassOf <http://emmo.info/emmo/domain/mechanical-testing#EMMO_7452b52c_82ea_47da_b84f_493317c8f03e> ;
                                                                                            rdfs:comment "Steel nomenclature contains steel groups / categories as defined in the standards DIN, SAE and JIS and superclasses in which the categories from the different standards are combined" ;
                                                                                            rdfs:label "Other steels"@en ;
                                                                                            <http://www.w3.org/2004/02/skos/core#prefLabel> "OtherSteels"@en .


###  http://emmo.info/emmo/domain/mechanical-testing#EMMO_86a5bfa9_fb77_4365_9894_81c0454ad7d0
<http://emmo.info/emmo/domain/mechanical-testing#EMMO_86a5bfa9_fb77_4365_9894_81c0454ad7d0> rdf:type owl:Class ;
                                                                                            rdfs:subClassOf <http://emmo.info/emmo/domain/mechanical-testing#EMMO_ca42ed31_3983_4e1a_84f9_a84cab2cdb59> ;
                                                                                            rdfs:comment "The RMS value of the displacement at the target frequency when dynamics are switched on during the test (e.g. Continuous Stiffness Measurement )." ;
                                                                                            <http://www.w3.org/2004/02/skos/core#prefLabel> "DynamicDisplacement"@en .


###  http://emmo.info/emmo/domain/mechanical-testing#EMMO_87286423_f048_47ac_b8df_3235e824f277
<http://emmo.info/emmo/domain/mechanical-testing#EMMO_87286423_f048_47ac_b8df_3235e824f277> rdf:type owl:Class ;
                                                                                            rdfs:subClassOf <http://emmo.info/emmo/domain/mechanical-testing#EMMO_e5d45f40_f9e9_47b9_934b_4c463a38b08e> ,
                                                                                                            <http://emmo.info/emmo/middle/manufacturing#EMMO_a4d66059_5dd3_4b90_b4cb_10960559441b> ;
                                                                                            rdfs:comment "Machining is a process in which a material (often metal) is cut to a desired final shape and size by a controlled material-removal process. The processes that have this common theme are collectively called subtractive manufacturing." ;
                                                                                            <http://www.w3.org/2004/02/skos/core#prefLabel> "Machining"@en .


###  http://emmo.info/emmo/domain/mechanical-testing#EMMO_87985f48_7967_4ed1_b23f_33357576c47d
<http://emmo.info/emmo/domain/mechanical-testing#EMMO_87985f48_7967_4ed1_b23f_33357576c47d> rdf:type owl:Class ;
                                                                                            rdfs:subClassOf <http://emmo.info/emmo/domain/mechanical-testing#EMMO_87286423_f048_47ac_b8df_3235e824f277> ;
                                                                                            rdfs:comment "Roughing cuts are used to remove large amount of material from the starting workpart as rapidly as possible, i.e. with a large Material Removal Rate (MRR), in order to produce a shape close to the desired form, but leaving some material on the piece for a subsequent finishing operation." ;
                                                                                            <http://www.w3.org/2004/02/skos/core#prefLabel> "Roughing" .


###  http://emmo.info/emmo/domain/mechanical-testing#EMMO_87cf41f0_9efa_47da_9826_57eeb34a33f1
<http://emmo.info/emmo/domain/mechanical-testing#EMMO_87cf41f0_9efa_47da_9826_57eeb34a33f1> rdf:type owl:Class ;
                                                                                            rdfs:subClassOf <http://emmo.info/emmo/domain/mechanical-testing#EMMO_91e9c813_b277_48ad_b5b0_a781a05b9c1f> ,
                                                                                                            <http://emmo.info/emmo/middle/isq#EMMO_d4f7d378_5e3b_468a_baa1_a7e98358cda7> ;
                                                                                            rdfs:comment "This is the time needed by the instrument to stabilize after initial power up. This time is usually dependent on the thermal characteristics of the measurement system." ;
                                                                                            <http://www.w3.org/2004/02/skos/core#prefLabel> "MachineStabilizationTime"@en .


###  http://emmo.info/emmo/domain/mechanical-testing#EMMO_87d31968_0753_420f_bc7d_23a83438e13f
<http://emmo.info/emmo/domain/mechanical-testing#EMMO_87d31968_0753_420f_bc7d_23a83438e13f> rdf:type owl:Class ;
                                                                                            rdfs:subClassOf <http://emmo.info/emmo/domain/mechanical-testing#EMMO_376c6456_5601_41c2_987c_3063f14408d4> ,
                                                                                                            <http://emmo.info/emmo/domain/mechanical-testing#EMMO_91e9c813_b277_48ad_b5b0_a781a05b9c1f> ;
                                                                                            rdfs:comment "The targeted maximum load to be applied. The experiment will stop loading at this point or if the Target Depth is reached." ;
                                                                                            <http://www.w3.org/2004/02/skos/core#prefLabel> "TargetLoad"@en .


###  http://emmo.info/emmo/domain/mechanical-testing#EMMO_8828c7d2_8f7d_4804_8e13_336d37d94ec2
<http://emmo.info/emmo/domain/mechanical-testing#EMMO_8828c7d2_8f7d_4804_8e13_336d37d94ec2> rdf:type owl:Class ;
                                                                                            rdfs:subClassOf <http://emmo.info/emmo/domain/mechanical-testing#CableBundleUseCase> ,
                                                                                                            <http://emmo.info/emmo/middle/manufacturing#EMMO_494b372c_cfdf_47d3_a4de_5e037c540de8> ,
                                                                                                            <http://emmo.info/emmo/middle/semiotics#EMMO_6f5af708_f825_4feb_a0d1_a8d813d3022b> ;
                                                                                            rdfs:comment "A cable system is a generic term to represent different types of cable systems such as a cable bundle or a single cable." ;
                                                                                            <http://www.w3.org/2004/02/skos/core#prefLabel> "CableSystem"@en .


###  http://emmo.info/emmo/domain/mechanical-testing#EMMO_897678f5_488b_4489_8b84_1ab548db1512
<http://emmo.info/emmo/domain/mechanical-testing#EMMO_897678f5_488b_4489_8b84_1ab548db1512> rdf:type owl:Class ;
                                                                                            rdfs:subClassOf <http://emmo.info/emmo/domain/mechanical-testing#EMMO_35a4d47f_452e_4234_9183_3b835ca02091> ;
                                                                                            <http://www.w3.org/2004/02/skos/core#prefLabel> "StandardNanoindentationMeasurementOliverPharrPostProcessing"@en .


###  http://emmo.info/emmo/domain/mechanical-testing#EMMO_89be8d21_79a7_4970_9b0a_ee18cec63e62
<http://emmo.info/emmo/domain/mechanical-testing#EMMO_89be8d21_79a7_4970_9b0a_ee18cec63e62> rdf:type owl:Class ;
                                                                                            rdfs:subClassOf <http://emmo.info/emmo/domain/mechanical-testing#EMMO_bb2485f3_e956_489b_8434_6f71333ae16c> ;
                                                                                            rdfs:comment "Steel nomenclature contains steel groups / categories as defined in the standards DIN, SAE and JIS and superclasses in which the categories from the different standards are combined" ;
                                                                                            rdfs:label "Unalloyed construction, engineering and pressure vessel steels"@en ;
                                                                                            <http://www.w3.org/2004/02/skos/core#prefLabel> "UnalloyedConstructionEngineeringAndPressureVesselSteels"@en .


###  http://emmo.info/emmo/domain/mechanical-testing#EMMO_8a5f8323_d356_44a8_9840_af3bfac84505
<http://emmo.info/emmo/domain/mechanical-testing#EMMO_8a5f8323_d356_44a8_9840_af3bfac84505> rdf:type owl:Class ;
                                                                                            rdfs:subClassOf <http://emmo.info/emmo/domain/mechanical-testing#EMMO_b50db598_cfea_4582_9168_46fbc0b9ec4f> ;
                                                                                            rdfs:comment "Represents the distance between the ouside edge of a circular cross section and its center." ;
                                                                                            <http://www.w3.org/2004/02/skos/core#prefLabel> "OuterRadius"@en .


###  http://emmo.info/emmo/domain/mechanical-testing#EMMO_8aa746fa_0cfa_4be7_9e5b_a691a860032e
<http://emmo.info/emmo/domain/mechanical-testing#EMMO_8aa746fa_0cfa_4be7_9e5b_a691a860032e> rdf:type owl:Class ;
                                                                                            rdfs:subClassOf <http://emmo.info/emmo/domain/mechanical-testing#EMMO_91e9c813_b277_48ad_b5b0_a781a05b9c1f> ;
                                                                                            rdfs:comment "In load frames of finite stiffness, the load applied via the indenter induces displacement in both the sample and the load frame. Frame compliance must be identified and subtracted from the total indenter displacement to account properly for sample deformation." ;
                                                                                            <http://www.w3.org/2004/02/skos/core#prefLabel> "LoadFrameCompliance"@en .


###  http://emmo.info/emmo/domain/mechanical-testing#EMMO_8beaaf27_f05f_4235_ae3d_6af594eadf87
<http://emmo.info/emmo/domain/mechanical-testing#EMMO_8beaaf27_f05f_4235_ae3d_6af594eadf87> rdf:type owl:Class ;
                                                                                            rdfs:subClassOf <http://emmo.info/emmo/domain/mechanical-testing#EMMO_c799b443_c70f_4351_bb0f_e4ab29073481> ,
                                                                                                            <http://emmo.info/emmo/domain/mechanical-testing#EMMO_eda29fc2_7d48_4997_8593_38fd9b344fe2> ;
                                                                                            rdfs:comment "The average value of the hardness measured using the Continuous Stiffness Measurement technique. It is calculated by averaging, over the user selected penetration depth range, the ratio between the load applied to the sample (also considering its dynamic component) and the tip contact area. (according to the Oliver and Pharr method)" ;
                                                                                            <http://www.w3.org/2004/02/skos/core#prefLabel> "AverageDynamicHardness"@en .


###  http://emmo.info/emmo/domain/mechanical-testing#EMMO_8e789c90_a34a_425a_a685_36865e342c82
<http://emmo.info/emmo/domain/mechanical-testing#EMMO_8e789c90_a34a_425a_a685_36865e342c82> rdf:type owl:Class ;
                                                                                            rdfs:subClassOf <http://emmo.info/emmo/domain/mechanical-testing#EMMO_da87d0e5_8e93_4fc3_81b9_53f8568d4cc4> ;
                                                                                            rdfs:comment "No special feature detected at crack-origin." ;
                                                                                            <http://www.w3.org/2004/02/skos/core#prefLabel> "Featureless"@en .


###  http://emmo.info/emmo/domain/mechanical-testing#EMMO_8e959570_c1a5_436f_bc54_08b423f4568d
<http://emmo.info/emmo/domain/mechanical-testing#EMMO_8e959570_c1a5_436f_bc54_08b423f4568d> rdf:type owl:Class ;
                                                                                            rdfs:subClassOf <http://emmo.info/emmo/domain/mechanical-testing#EMMO_e5d45f40_f9e9_47b9_934b_4c463a38b08e> ,
                                                                                                            <http://emmo.info/emmo/middle/manufacturing#EMMO_a4d66059_5dd3_4b90_b4cb_10960559441b> ;
                                                                                            rdfs:comment "In production engineering, metallurgy is concerned with the production of metallic components for use in consumer or engineering products." ;
                                                                                            <http://www.w3.org/2004/02/skos/core#prefLabel> "Metallurgy"@en .


###  http://emmo.info/emmo/domain/mechanical-testing#EMMO_8f7eb52b_6435_4c8f_99cc_f24d84b547a9
<http://emmo.info/emmo/domain/mechanical-testing#EMMO_8f7eb52b_6435_4c8f_99cc_f24d84b547a9> rdf:type owl:Class ;
                                                                                            rdfs:subClassOf <http://emmo.info/emmo/domain/mechanical-testing#EMMO_93c88738_64bc_49d7_9d43_f4c177a3b72e> ;
                                                                                            rdfs:comment """Steel category according to JIS standard:
Low-alloyed steels for machine structural use (JIS)""" ;
                                                                                            rdfs:label "Low-alloyed steels for machine structural use (JIS)"@en ;
                                                                                            <http://www.w3.org/2004/02/skos/core#prefLabel> "LowAlloyedSteelsForMachineStructuralUseJIS"@en .


###  http://emmo.info/emmo/domain/mechanical-testing#EMMO_8fab8d45_c53b_475f_997a_125646067051
<http://emmo.info/emmo/domain/mechanical-testing#EMMO_8fab8d45_c53b_475f_997a_125646067051> rdf:type owl:Class ;
                                                                                            rdfs:subClassOf <http://emmo.info/emmo/domain/mechanical-testing#EMMO_e5d45f40_f9e9_47b9_934b_4c463a38b08e> ,
                                                                                                            <http://emmo.info/emmo/middle/chemistry#EMMO_4f40def1_3cd7_4067_9596_541e9a5134cf> ;
                                                                                            <http://www.w3.org/2004/02/skos/core#prefLabel> "MagnesiumSymbol"@en .


###  http://emmo.info/emmo/domain/mechanical-testing#EMMO_8fb5442e_d864_4d85_aad1_8d638f6a5fd3
<http://emmo.info/emmo/domain/mechanical-testing#EMMO_8fb5442e_d864_4d85_aad1_8d638f6a5fd3> rdf:type owl:Class ;
                                                                                            rdfs:subClassOf <http://emmo.info/emmo/domain/mechanical-testing#EMMO_e5d45f40_f9e9_47b9_934b_4c463a38b08e> ,
                                                                                                            <http://emmo.info/emmo/middle/properties#EMMO_463bcfda_867b_41d9_a967_211d4d437cfb> ;
                                                                                            rdfs:comment "Fractography describes all data resulting from examination of the fracture surface after fatigue testing. The goal is to find the information necessary to describe the failure behaviour and reason." ;
                                                                                            <http://www.w3.org/2004/02/skos/core#prefLabel> "Fractography"@en .


###  http://emmo.info/emmo/domain/mechanical-testing#EMMO_8fc8a9e8_e8c3_476c_a417_031267a0206a
<http://emmo.info/emmo/domain/mechanical-testing#EMMO_8fc8a9e8_e8c3_476c_a417_031267a0206a> rdf:type owl:Class ;
                                                                                            rdfs:subClassOf <http://emmo.info/emmo/domain/mechanical-testing#EMMO_e5d45f40_f9e9_47b9_934b_4c463a38b08e> ,
                                                                                                            <http://emmo.info/emmo/middle/metrology#EMMO_50a3552e_859a_4ff7_946d_76d537cabce6> ,
                                                                                                            <http://emmo.info/emmo/middle/metrology#EMMO_c9c8f824_9127_4f93_bc21_69fe78a7f6f2> ;
                                                                                            rdfs:comment "Rockwell C Hardness unit" ;
                                                                                            <http://www.w3.org/2004/02/skos/core#prefLabel> "RockwellCHardnessUnit"@en .


###  http://emmo.info/emmo/domain/mechanical-testing#EMMO_91e9c813_b277_48ad_b5b0_a781a05b9c1f
<http://emmo.info/emmo/domain/mechanical-testing#EMMO_91e9c813_b277_48ad_b5b0_a781a05b9c1f> rdf:type owl:Class ;
                                                                                            rdfs:subClassOf <http://emmo.info/emmo/domain/mechanical-testing#NanoindentationUseCase> ,
                                                                                                            <http://emmo.info/emmo/middle/perceptual#EMMO_d8d2144e_5c8d_455d_a643_5caf4d8d9df8> ,
                                                                                                            <http://emmo.info/emmo/middle/properties#EMMO_b7bcff25_ffc3_474e_9ab5_01b1664bd4ba> ;
                                                                                            rdfs:comment "Represents the Nanoindentation method specification." ;
                                                                                            <http://www.w3.org/2004/02/skos/core#prefLabel> "NanoindentationMethodSpecification"@en .


###  http://emmo.info/emmo/domain/mechanical-testing#EMMO_91fd8d2f_af9a_47e7_b26d_01946f952e49
<http://emmo.info/emmo/domain/mechanical-testing#EMMO_91fd8d2f_af9a_47e7_b26d_01946f952e49> rdf:type owl:Class ;
                                                                                            rdfs:subClassOf <http://emmo.info/emmo/domain/mechanical-testing#EMMO_91e9c813_b277_48ad_b5b0_a781a05b9c1f> ,
                                                                                                            <http://emmo.info/emmo/middle/isq#EMMO_d4f7d378_5e3b_468a_baa1_a7e98358cda7> ;
                                                                                            rdfs:comment "The time at constant load prior to taking drift data." ;
                                                                                            <http://www.w3.org/2004/02/skos/core#prefLabel> "DriftSettleTime"@en .


###  http://emmo.info/emmo/domain/mechanical-testing#EMMO_926d14c7_4f78_4c37_99b4_dfb0a531db64
<http://emmo.info/emmo/domain/mechanical-testing#EMMO_926d14c7_4f78_4c37_99b4_dfb0a531db64> rdf:type owl:Class ;
                                                                                            rdfs:subClassOf <http://emmo.info/emmo/domain/mechanical-testing#EMMO_e5d45f40_f9e9_47b9_934b_4c463a38b08e> ,
                                                                                                            <http://emmo.info/emmo/middle/isq#EMMO_d1917609_db5e_4b8a_9b76_ef1d6f860a81> ;
                                                                                            rdfs:comment "Tensile strength is the maximum tensile stress a material can withstand prior to fracture." ;
                                                                                            <http://www.w3.org/2004/02/skos/core#prefLabel> "TensileStrength"@en .


###  http://emmo.info/emmo/domain/mechanical-testing#EMMO_9294b602_0926_4063_9c68_7d541728856d
<http://emmo.info/emmo/domain/mechanical-testing#EMMO_9294b602_0926_4063_9c68_7d541728856d> rdf:type owl:Class ;
                                                                                            rdfs:subClassOf <http://emmo.info/emmo/domain/mechanical-testing#EMMO_e5d45f40_f9e9_47b9_934b_4c463a38b08e> ,
                                                                                                            <http://emmo.info/emmo/middle/chemistry#EMMO_4f40def1_3cd7_4067_9596_541e9a5134cf> ;
                                                                                            <http://www.w3.org/2004/02/skos/core#prefLabel> "ZirconiumSymbol"@en .


###  http://emmo.info/emmo/domain/mechanical-testing#EMMO_929f8ef1_ff51_49c5_ab3e_c654b156960c
<http://emmo.info/emmo/domain/mechanical-testing#EMMO_929f8ef1_ff51_49c5_ab3e_c654b156960c> rdf:type owl:Class ;
                                                                                            rdfs:subClassOf <http://emmo.info/emmo/domain/mechanical-testing#EMMO_87985f48_7967_4ed1_b23f_33357576c47d> ;
                                                                                            rdfs:comment "Cutting is manufacturing by removal of material (DIN 8580; CIRP Dictionary 2004). Particles of material, the chips, are mechanically removed from the raw material or from an unfinished part by cutting edges of a tool. The tool has one or several cutting edges, which can be geometrically defined by number, shape, and position (cutting by geometrically defined cutting edges), whereas in abrasive processes the separation of chips takes place by numerous cutting edges which have to be statistically described and which are randomly distributed inside the tool (cutting by geometrically undefined cutting edges)." ;
                                                                                            rdfs:isDefinedBy "https://www.beuth.de/de/norm/din-8580/65031153" ;
                                                                                            <http://www.w3.org/2004/02/skos/core#prefLabel> "Cutting"@en .


###  http://emmo.info/emmo/domain/mechanical-testing#EMMO_93c88738_64bc_49d7_9d43_f4c177a3b72e
<http://emmo.info/emmo/domain/mechanical-testing#EMMO_93c88738_64bc_49d7_9d43_f4c177a3b72e> rdf:type owl:Class ;
                                                                                            rdfs:subClassOf <http://emmo.info/emmo/domain/mechanical-testing#EMMO_bb2485f3_e956_489b_8434_6f71333ae16c> ;
                                                                                            rdfs:comment "Steel nomenclature contains steel groups / categories as defined in the standards DIN, SAE and JIS and superclasses in which the categories from the different standards are combined" ;
                                                                                            rdfs:label "Low-alloyed construction, engineering and pressure vessel steels"@en ;
                                                                                            <http://www.w3.org/2004/02/skos/core#prefLabel> "LowAlloyedConstructionEngineeringAndPressureVesselSteels"@en .


###  http://emmo.info/emmo/domain/mechanical-testing#EMMO_94376acf_9d21_497a_85e4_12c84dba4645
<http://emmo.info/emmo/domain/mechanical-testing#EMMO_94376acf_9d21_497a_85e4_12c84dba4645> rdf:type owl:Class ;
                                                                                            rdfs:subClassOf <http://emmo.info/emmo/domain/mechanical-testing#EMMO_bd8e17c8_167a_4c72_b4ab_e8b2f69034f1> ,
                                                                                                            <http://emmo.info/emmo/domain/mechanical-testing#EMMO_d5b0d9de_0ce0_4e28_8c17_9e5706baba43> ;
                                                                                            <http://www.w3.org/2004/02/skos/core#prefLabel> "FlatNotchedSpecimen"@en .


###  http://emmo.info/emmo/domain/mechanical-testing#EMMO_94bbba62_9b14_4c2a_a2dd_b7474d1d53cd
<http://emmo.info/emmo/domain/mechanical-testing#EMMO_94bbba62_9b14_4c2a_a2dd_b7474d1d53cd> rdf:type owl:Class ;
                                                                                            rdfs:subClassOf <http://emmo.info/emmo/domain/mechanical-testing#NanoindentationUseCase> ,
                                                                                                            <http://emmo.info/emmo/middle/isq#EMMO_96f39f77_44dc_491b_8fa7_30d887fe0890> ;
                                                                                            rdfs:comment "The contact area calculated form dynamics and the Oliver and Pharr method." ;
                                                                                            <http://www.w3.org/2004/02/skos/core#prefLabel> "DynamicContactArea"@en .


###  http://emmo.info/emmo/domain/mechanical-testing#EMMO_9560b3d4_c573_458a_a9c4_5e00383979cf
<http://emmo.info/emmo/domain/mechanical-testing#EMMO_9560b3d4_c573_458a_a9c4_5e00383979cf> rdf:type owl:Class ;
                                                                                            rdfs:subClassOf <http://emmo.info/emmo/domain/mechanical-testing#NanoindentationUseCase> ,
                                                                                                            <http://emmo.info/emmo/middle/semiotics#EMMO_d7788d1a_020d_4c78_85a1_13563fcec168> ;
                                                                                            <http://www.w3.org/2004/02/skos/core#prefLabel> "ContactAngleMeasurementStateImage"@en .


###  http://emmo.info/emmo/domain/mechanical-testing#EMMO_959181b4_1765_4fee_8ca7_139d4728b2a5
<http://emmo.info/emmo/domain/mechanical-testing#EMMO_959181b4_1765_4fee_8ca7_139d4728b2a5> rdf:type owl:Class ;
                                                                                            rdfs:subClassOf <http://emmo.info/emmo/domain/mechanical-testing#EMMO_e5d45f40_f9e9_47b9_934b_4c463a38b08e> ,
                                                                                                            <http://emmo.info/emmo/middle/siunits#EMMO_d41ce84b_4317_41fb_a5d1_6cd281fca106> ;
                                                                                            <http://www.w3.org/2004/02/skos/core#prefLabel> "Millimetre"@en .


###  http://emmo.info/emmo/domain/mechanical-testing#EMMO_962bea7f_4fd4_4a16_8dc0_183efcc620bb
<http://emmo.info/emmo/domain/mechanical-testing#EMMO_962bea7f_4fd4_4a16_8dc0_183efcc620bb> rdf:type owl:Class ;
                                                                                            rdfs:subClassOf <http://emmo.info/emmo/domain/mechanical-testing#EMMO_e5d45f40_f9e9_47b9_934b_4c463a38b08e> ,
                                                                                                            <http://emmo.info/emmo/middle/chemistry#EMMO_4f40def1_3cd7_4067_9596_541e9a5134cf> ;
                                                                                            <http://www.w3.org/2004/02/skos/core#prefLabel> "BoronSymbol"@en .


###  http://emmo.info/emmo/domain/mechanical-testing#EMMO_9731faf5_4cb1_46bd_891c_686e6340c83f
<http://emmo.info/emmo/domain/mechanical-testing#EMMO_9731faf5_4cb1_46bd_891c_686e6340c83f> rdf:type owl:Class ;
                                                                                            rdfs:subClassOf <http://emmo.info/emmo/domain/mechanical-testing#EMMO_e5d45f40_f9e9_47b9_934b_4c463a38b08e> ,
                                                                                                            <http://emmo.info/emmo/middle/chemistry#EMMO_a293f923_954c_4af5_9f97_9600ebd362cb> ,
                                                                                                            <http://emmo.info/emmo/middle/isq#EMMO_faab3f84_e475_4a46_af9c_7d249f0b9aef> ;
                                                                                            rdfs:comment "Represents the percentage by volume (vol%) that is used to express the composition of a mixture." ;
                                                                                            <http://www.w3.org/2004/02/skos/core#prefLabel> "VolumePercent"@en .


###  http://emmo.info/emmo/domain/mechanical-testing#EMMO_9b84bd4e_adfa_48b6_b4f7_f597bb40dae1
<http://emmo.info/emmo/domain/mechanical-testing#EMMO_9b84bd4e_adfa_48b6_b4f7_f597bb40dae1> rdf:type owl:Class ;
                                                                                            rdfs:subClassOf <http://emmo.info/emmo/domain/mechanical-testing#EMMO_c21ab500_db9a_43a3_a7ef_d43fb64bf856> ;
                                                                                            rdfs:comment "A simbolic symbolic representation of the source of infomation (e.g.: a string that represents the path to a file)." ;
                                                                                            <http://www.w3.org/2004/02/skos/core#prefLabel> "Reference"@en .


###  http://emmo.info/emmo/domain/mechanical-testing#EMMO_9b8fd21c_cf02_40bd_8d0b_748556612573
<http://emmo.info/emmo/domain/mechanical-testing#EMMO_9b8fd21c_cf02_40bd_8d0b_748556612573> rdf:type owl:Class ;
                                                                                            rdfs:subClassOf <http://emmo.info/emmo/domain/mechanical-testing#EMMO_460d3ba4_a8e5_449d_8423_7d4d1cca6d76> ;
                                                                                            rdfs:comment "MeSOMICS, stands for Measurement System for the Optically Monitored Identification of Cable Stiffnesses. The mesomics measurement enables the determination of the bending stiffness of a cable bundle using a MeSOMICS machine." ;
                                                                                            rdfs:seeAlso "https://www.itwm.fraunhofer.de/content/dam/itwm/de/documents/MDF_Infomaterial/mdf_flyer_MeSOMICS_EN.pdf" ;
                                                                                            <http://www.w3.org/2004/02/skos/core#prefLabel> "Mesomics"@en .


###  http://emmo.info/emmo/domain/mechanical-testing#EMMO_9c3dfc81_ccd9_4c91_a4ca_e52153f9e4e0
<http://emmo.info/emmo/domain/mechanical-testing#EMMO_9c3dfc81_ccd9_4c91_a4ca_e52153f9e4e0> rdf:type owl:Class ;
                                                                                            rdfs:subClassOf <http://emmo.info/emmo/domain/mechanical-testing#EMMO_3361ecb7_0340_4475_8e42_b2ae29af2420> ;
                                                                                            rdfs:comment """Steel category according to DIN standard:
Roller bearing steels (DIN 10027-2)""" ;
                                                                                            rdfs:label "Roller bearing steels (DIN 10027-2)"@en ;
                                                                                            <http://www.w3.org/2004/02/skos/core#prefLabel> "RollerBearingSteelsDIN10027"@en .


###  http://emmo.info/emmo/domain/mechanical-testing#EMMO_9d12d5ce_2af4_4784_a2b0_6c19db27d8ce
<http://emmo.info/emmo/domain/mechanical-testing#EMMO_9d12d5ce_2af4_4784_a2b0_6c19db27d8ce> rdf:type owl:Class ;
                                                                                            rdfs:subClassOf <http://emmo.info/emmo/domain/mechanical-testing#EMMO_e5d45f40_f9e9_47b9_934b_4c463a38b08e> ,
                                                                                                            <http://emmo.info/emmo/middle/chemistry#EMMO_4f40def1_3cd7_4067_9596_541e9a5134cf> ;
                                                                                            <http://www.w3.org/2004/02/skos/core#prefLabel> "LeadSymbol"@en .


###  http://emmo.info/emmo/domain/mechanical-testing#EMMO_9d621c9b_9c52_4084_af20_b2dfda89fe6c
<http://emmo.info/emmo/domain/mechanical-testing#EMMO_9d621c9b_9c52_4084_af20_b2dfda89fe6c> rdf:type owl:Class ;
                                                                                            rdfs:subClassOf <http://emmo.info/emmo/domain/mechanical-testing#NanoindentationUseCase> ,
                                                                                                            <http://emmo.info/emmo/middle/properties#EMMO_463bcfda_867b_41d9_a967_211d4d437cfb> ;
                                                                                            <http://www.w3.org/2004/02/skos/core#prefLabel> "IndentationMeasurement"@en .


###  http://emmo.info/emmo/domain/mechanical-testing#EMMO_9ecbe4c2_0fdd_4ee9_8f68_31c290be4bde
<http://emmo.info/emmo/domain/mechanical-testing#EMMO_9ecbe4c2_0fdd_4ee9_8f68_31c290be4bde> rdf:type owl:Class ;
                                                                                            rdfs:subClassOf <http://emmo.info/emmo/domain/mechanical-testing#EMMO_8828c7d2_8f7d_4804_8e13_336d37d94ec2> ,
                                                                                                            <http://emmo.info/emmo/middle/reductionistic#EMMO_36c79456_e29c_400d_8bd3_0eedddb82652> ;
                                                                                            rdfs:comment "A component containing several single cables, that are bundled together by a certain type of taping. A cable bundle has simple effective properties (bending stiffness, etc.) describing the macroscopic structure." ;
                                                                                            <http://www.w3.org/2004/02/skos/core#prefLabel> "CableBundle"@en .


###  http://emmo.info/emmo/domain/mechanical-testing#EMMO_9ee6424d_55a9_4645_891d_58dac89c5ee6
<http://emmo.info/emmo/domain/mechanical-testing#EMMO_9ee6424d_55a9_4645_891d_58dac89c5ee6> rdf:type owl:Class ;
                                                                                            rdfs:subClassOf <http://emmo.info/emmo/domain/mechanical-testing#EMMO_e5d45f40_f9e9_47b9_934b_4c463a38b08e> ,
                                                                                                            <http://emmo.info/emmo/middle/chemistry#EMMO_4f40def1_3cd7_4067_9596_541e9a5134cf> ;
                                                                                            <http://www.w3.org/2004/02/skos/core#prefLabel> "OxygenSymbol"@en .


###  http://emmo.info/emmo/domain/mechanical-testing#EMMO_a0d796f3_02e1_47d4_b9c0_9995ebf6e7a4
<http://emmo.info/emmo/domain/mechanical-testing#EMMO_a0d796f3_02e1_47d4_b9c0_9995ebf6e7a4> rdf:type owl:Class ;
                                                                                            rdfs:subClassOf <http://emmo.info/emmo/domain/mechanical-testing#EMMO_8630b1ff_7985_444e_8572_373816c0d3b5> ;
                                                                                            rdfs:comment """Steel category according to DIN standard:
Materials with special physical properties including Ni (DIN 10027-2)""" ;
                                                                                            rdfs:label "Materials with special physical properties including Ni (DIN 10027-2)"@en ;
                                                                                            <http://www.w3.org/2004/02/skos/core#prefLabel> "MaterialsWithSpecialPhysicalPropertiesIncludingNiDIN10027"@en .


###  http://emmo.info/emmo/domain/mechanical-testing#EMMO_a11352bc_9b81_4c0c_92e8_f47ea2c5c68b
<http://emmo.info/emmo/domain/mechanical-testing#EMMO_a11352bc_9b81_4c0c_92e8_f47ea2c5c68b> rdf:type owl:Class ;
                                                                                            rdfs:subClassOf <http://emmo.info/emmo/domain/mechanical-testing#EMMO_e5d45f40_f9e9_47b9_934b_4c463a38b08e> ,
                                                                                                            <http://emmo.info/emmo/middle/perceptual#EMMO_50ea1ec5_f157_41b0_b46b_a9032f17ca10> ,
                                                                                                            <http://emmo.info/emmo/middle/perceptual#EMMO_a1083d0a_c1fb_471f_8e20_a98f881ad527> ;
                                                                                            rdfs:comment "A symbolic that represents the type of environment in which a measurement has been carried out." ;
                                                                                            <http://www.w3.org/2004/02/skos/core#prefLabel> "Environment"@en .


###  http://emmo.info/emmo/domain/mechanical-testing#EMMO_a1c92b74_411d_414c_85e0_36ddd8c8afb6
<http://emmo.info/emmo/domain/mechanical-testing#EMMO_a1c92b74_411d_414c_85e0_36ddd8c8afb6> rdf:type owl:Class ;
                                                                                            rdfs:subClassOf <http://emmo.info/emmo/domain/mechanical-testing#EMMO_91e9c813_b277_48ad_b5b0_a781a05b9c1f> ,
                                                                                                            <http://emmo.info/emmo/middle/isq#EMMO_d4f7d378_5e3b_468a_baa1_a7e98358cda7> ;
                                                                                            rdfs:comment "This is the time specified to linearly reduce the load on the contact form its maximum value to zero." ;
                                                                                            <http://www.w3.org/2004/02/skos/core#prefLabel> "TargetUnloadTime"@en .


###  http://emmo.info/emmo/domain/mechanical-testing#EMMO_a1fb2461_3dc8_45bd_a7f3_4c1cff1ba432
<http://emmo.info/emmo/domain/mechanical-testing#EMMO_a1fb2461_3dc8_45bd_a7f3_4c1cff1ba432> rdf:type owl:Class ;
                                                                                            rdfs:subClassOf <http://emmo.info/emmo/domain/mechanical-testing#EMMO_e5d45f40_f9e9_47b9_934b_4c463a38b08e> ,
                                                                                                            <http://emmo.info/emmo/middle/chemistry#EMMO_4f40def1_3cd7_4067_9596_541e9a5134cf> ;
                                                                                            <http://www.w3.org/2004/02/skos/core#prefLabel> "SiliconElement"@en .


###  http://emmo.info/emmo/domain/mechanical-testing#EMMO_a30a7cdc_f652_4b01_b8c2_cd056f3e3d85
<http://emmo.info/emmo/domain/mechanical-testing#EMMO_a30a7cdc_f652_4b01_b8c2_cd056f3e3d85> rdf:type owl:Class ;
                                                                                            rdfs:subClassOf <http://emmo.info/emmo/domain/mechanical-testing#EMMO_1b0a92ef_c509_40ee_8abe_408181aafaad> ;
                                                                                            rdfs:comment "Is a device that is used to determine mechanical properties of materials in paricular it is used to test the tensile strength and compressive strength of materials. It represents a measuremt device that is used in mechanical testing experiments." ;
                                                                                            <http://www.w3.org/2004/02/skos/core#prefLabel> "MechanicalTestingMachine"@en .


###  http://emmo.info/emmo/domain/mechanical-testing#EMMO_a522e3fa_fde7_4d20_9246_ee6b0f073d6d
<http://emmo.info/emmo/domain/mechanical-testing#EMMO_a522e3fa_fde7_4d20_9246_ee6b0f073d6d> rdf:type owl:Class ;
                                                                                            rdfs:subClassOf <http://emmo.info/emmo/domain/mechanical-testing#EMMO_e5d45f40_f9e9_47b9_934b_4c463a38b08e> ;
                                                                                            <http://www.w3.org/2004/02/skos/core#prefLabel> "FailureOrigin"@en .


###  http://emmo.info/emmo/domain/mechanical-testing#EMMO_a579af48_7803_4f5f_8f5f_ae1198b3eb85
<http://emmo.info/emmo/domain/mechanical-testing#EMMO_a579af48_7803_4f5f_8f5f_ae1198b3eb85> rdf:type owl:Class ;
                                                                                            rdfs:subClassOf <http://emmo.info/emmo/domain/mechanical-testing#EMMO_06390646_6edb_4410_b22b_f7adbd6025c4> ;
                                                                                            rdfs:comment "Martensite is a non-equilibrium phase of the iron-carbon system. It is formed in carbon steels by the rapid cooling (quenching) of the austenite form of iron at such a high rate that carbon atoms do not have time to diffuse out of the crystal structure in large enough quantities to form cementite (Fe3C). Austenite is gamma-phase iron, a solid solution of iron and alloying elements. As a result of the quenching, the face-centered cubic austenite transforms to a highly strained body-centered tetragonal form called martensite that is supersaturated with carbon. The shear deformations that result produce a large number of dislocations, which is a primary strengthening mechanism of steels." ;
                                                                                            <http://www.w3.org/2004/02/skos/core#prefLabel> "Martensite"@en .


###  http://emmo.info/emmo/domain/mechanical-testing#EMMO_a5fb2228_53f8_4d1a_a929_ae166b9ea7ac
<http://emmo.info/emmo/domain/mechanical-testing#EMMO_a5fb2228_53f8_4d1a_a929_ae166b9ea7ac> rdf:type owl:Class ;
                                                                                            rdfs:subClassOf <http://emmo.info/emmo/domain/mechanical-testing#EMMO_646b0170_e349_4382_8291_4fa2cca982ea> ,
                                                                                                            <http://emmo.info/emmo/middle/metrology#EMMO_71f6ab56_342c_484b_bbe0_de86b7367cb3> ;
                                                                                            rdfs:comment "One half the algebraic difference between the maximum and minimum stress in one fatigue test cycle." ;
                                                                                            <http://www.w3.org/2004/02/skos/core#prefLabel> "StressAmplitude"@en .


###  http://emmo.info/emmo/domain/mechanical-testing#EMMO_a7841c32_22a5_46ee_8298_fe4f4d6473b0
<http://emmo.info/emmo/domain/mechanical-testing#EMMO_a7841c32_22a5_46ee_8298_fe4f4d6473b0> rdf:type owl:Class ;
                                                                                            rdfs:subClassOf <http://emmo.info/emmo/domain/mechanical-testing#EMMO_e5d45f40_f9e9_47b9_934b_4c463a38b08e> ,
                                                                                                            <http://emmo.info/emmo/middle/chemistry#EMMO_4f40def1_3cd7_4067_9596_541e9a5134cf> ;
                                                                                            <http://www.w3.org/2004/02/skos/core#prefLabel> "MolybdenumSymbol"@en .


###  http://emmo.info/emmo/domain/mechanical-testing#EMMO_a8df9a6f_36ee_4396_9e3d_732a86318386
<http://emmo.info/emmo/domain/mechanical-testing#EMMO_a8df9a6f_36ee_4396_9e3d_732a86318386> rdf:type owl:Class ;
                                                                                            rdfs:subClassOf <http://emmo.info/emmo/domain/mechanical-testing#EMMO_8e959570_c1a5_436f_bc54_08b423f4568d> ;
                                                                                            rdfs:comment "Deoxidization is a method used in metallurgy to remove the oxygen content during steel manufacturing. Deoxidation is important in the steelmaking process as oxygen is often detrimental to the quality of steel produced. Deoxidization is mainly achieved by adding a separate chemical species to neutralize the effects of oxygen or by directly removing the oxygen." ;
                                                                                            <http://www.w3.org/2004/02/skos/core#prefLabel> "Deoxidization" .


###  http://emmo.info/emmo/domain/mechanical-testing#EMMO_a9974b61_d31e_4f5c_9fee_13c777ad93ff
<http://emmo.info/emmo/domain/mechanical-testing#EMMO_a9974b61_d31e_4f5c_9fee_13c777ad93ff> rdf:type owl:Class ;
                                                                                            rdfs:subClassOf <http://emmo.info/emmo/domain/mechanical-testing#EMMO_81dd7f19_073d_4153_9517_823edac9fac7> ;
                                                                                            rdfs:comment "Taping that covers only at specific discrete locations across the cable bundle overall length." ;
                                                                                            <http://www.w3.org/2004/02/skos/core#prefLabel> "PartialTaping"@en .


###  http://emmo.info/emmo/domain/mechanical-testing#EMMO_ab528a3a_cb4b_40de_acaa_7752ccd968b9
<http://emmo.info/emmo/domain/mechanical-testing#EMMO_ab528a3a_cb4b_40de_acaa_7752ccd968b9> rdf:type owl:Class ;
                                                                                            rdfs:subClassOf <http://emmo.info/emmo/domain/mechanical-testing#EMMO_7dc73553_7d3f_4dc2_bb7b_f47775207457> ,
                                                                                                            <http://emmo.info/emmo/domain/mechanical-testing#EMMO_f0ad542d_ff13_4998_9e7f_ea27583c5f31> ;
                                                                                            rdfs:comment "The reduced modulus of the specimen and indenter tip as calculated from the maximum load, the maximum depth and the unloading data following the Oliver and Pharr calculation steps." ;
                                                                                            <http://www.w3.org/2004/02/skos/core#prefLabel> "ReducedModulusFromUnload"@en .


###  http://emmo.info/emmo/domain/mechanical-testing#EMMO_ab7acd0c_c199_47f7_ae2a_0ea5f579771b
<http://emmo.info/emmo/domain/mechanical-testing#EMMO_ab7acd0c_c199_47f7_ae2a_0ea5f579771b> rdf:type owl:Class ;
                                                                                            rdfs:subClassOf <http://emmo.info/emmo/domain/mechanical-testing#EMMO_e5d45f40_f9e9_47b9_934b_4c463a38b08e> ,
                                                                                                            <http://emmo.info/emmo/middle/chemistry#EMMO_4f40def1_3cd7_4067_9596_541e9a5134cf> ;
                                                                                            <http://www.w3.org/2004/02/skos/core#prefLabel> "CalciumSymbol"@en .


###  http://emmo.info/emmo/domain/mechanical-testing#EMMO_ac324c09_8830_4b04_bda5_8646a8dee0d4
<http://emmo.info/emmo/domain/mechanical-testing#EMMO_ac324c09_8830_4b04_bda5_8646a8dee0d4> rdf:type owl:Class ;
                                                                                            rdfs:subClassOf <http://emmo.info/emmo/middle/units-extension#EMMO_c2f5ee66_579c_44c6_a2e9_fa2eaa9fa4da> ;
                                                                                            <http://emmo.info/emmo/top/annotations#EMMO_1f1b164d_ec6a_4faa_8d5e_88bda62316cc> "http://qudt.org/vocab/unit/PERCENT" ;
                                                                                            <http://www.w3.org/2004/02/skos/core#prefLabel> "Percent"@en .


###  http://emmo.info/emmo/domain/mechanical-testing#EMMO_acc0ae8c_0726_461d_acab_834e84eaad69
<http://emmo.info/emmo/domain/mechanical-testing#EMMO_acc0ae8c_0726_461d_acab_834e84eaad69> rdf:type owl:Class ;
                                                                                            rdfs:subClassOf <http://emmo.info/emmo/domain/mechanical-testing#EMMO_06390646_6edb_4410_b22b_f7adbd6025c4> ;
                                                                                            rdfs:comment "Pearliteis atwo-phased,lamellar(or layered) structure composed of alternating layers offerrite(87.5 wt%) andcementite(12.5 wt%) that occurs in somesteelsandcast irons. During slow cooling of an iron-carbon alloy, pearlite forms by aeutectoidreaction asaustenitecools below 723C (1,333F) (the eutectoid temperature). Pearlite is a microstructure occurring in many common grades of steels." ;
                                                                                            <http://www.w3.org/2004/02/skos/core#prefLabel> "Pearlite"@en .


###  http://emmo.info/emmo/domain/mechanical-testing#EMMO_adff8854_b8f6_4943_99b4_6e3619b6c552
<http://emmo.info/emmo/domain/mechanical-testing#EMMO_adff8854_b8f6_4943_99b4_6e3619b6c552> rdf:type owl:Class ;
                                                                                            rdfs:subClassOf <http://emmo.info/emmo/domain/mechanical-testing#NanoindentationUseCase> ,
                                                                                                            <http://emmo.info/emmo/middle/isq#EMMO_1f087811_06cb_42d5_90fb_25d0e7e068ef> ;
                                                                                            rdfs:comment "The RMS value of the Force at the target frequency." ;
                                                                                            <http://www.w3.org/2004/02/skos/core#prefLabel> "DynamicForce"@en .


###  http://emmo.info/emmo/domain/mechanical-testing#EMMO_af7886a4_c996_469b_a0ed_23bb31448a19
<http://emmo.info/emmo/domain/mechanical-testing#EMMO_af7886a4_c996_469b_a0ed_23bb31448a19> rdf:type owl:Class ;
                                                                                            rdfs:subClassOf <http://emmo.info/emmo/domain/mechanical-testing#EMMO_e5d45f40_f9e9_47b9_934b_4c463a38b08e> ,
                                                                                                            <http://emmo.info/emmo/middle/isq#EMMO_d1917609_db5e_4b8a_9b76_ef1d6f860a81> ;
                                                                                            <http://emmo.info/emmo/middle/isq#physicalDimension> "T-2 L-1 M+1 I0 T0 N0 J0" ;
                                                                                            rdfs:comment "Corresponding strength value to a given number of cycles as determined from an S-N diagram (usually given for 50 % probability of survival)." ;
                                                                                            rdfs:isDefinedBy "https://www.astm.org/Standards/E1823.htm" ;
                                                                                            <http://www.w3.org/2004/02/skos/core#prefLabel> "FatigueStrength"@en .


###  http://emmo.info/emmo/domain/mechanical-testing#EMMO_b2a234a8_579a_422c_9305_b8f7e72c76cd
<http://emmo.info/emmo/domain/mechanical-testing#EMMO_b2a234a8_579a_422c_9305_b8f7e72c76cd> rdf:type owl:Class ;
                                                                                            rdfs:subClassOf <http://emmo.info/emmo/domain/mechanical-testing#EMMO_e8c8c152_484e_4053_8e35_82346b3fc927> ;
                                                                                            rdfs:comment "Circular cross section is a cross section with circular shape." ;
                                                                                            <http://www.w3.org/2004/02/skos/core#prefLabel> "CirclularCrossSection"@en .


###  http://emmo.info/emmo/domain/mechanical-testing#EMMO_b39aa045_49f3_4c29_a197_c2d65f352cfb
<http://emmo.info/emmo/domain/mechanical-testing#EMMO_b39aa045_49f3_4c29_a197_c2d65f352cfb> rdf:type owl:Class ;
                                                                                            rdfs:subClassOf <http://emmo.info/emmo/domain/mechanical-testing#EMMO_91e9c813_b277_48ad_b5b0_a781a05b9c1f> ,
                                                                                                            <http://emmo.info/emmo/middle/isq#EMMO_d4f7d378_5e3b_468a_baa1_a7e98358cda7> ;
                                                                                            rdfs:comment "When the \"Target Load\" or the \"Target Depth\" is reached, the \"Load\" is held constant for this time." ;
                                                                                            <http://www.w3.org/2004/02/skos/core#prefLabel> "MaximumLoadHoldingTime"@en .


###  http://emmo.info/emmo/domain/mechanical-testing#EMMO_b3ad6907_7206_4cc9_952b_2cdf34b578ea
<http://emmo.info/emmo/domain/mechanical-testing#EMMO_b3ad6907_7206_4cc9_952b_2cdf34b578ea> rdf:type owl:Class ;
                                                                                            rdfs:subClassOf <http://emmo.info/emmo/domain/mechanical-testing#EMMO_e5d45f40_f9e9_47b9_934b_4c463a38b08e> ,
                                                                                                            <http://emmo.info/emmo/middle/chemistry#EMMO_4f40def1_3cd7_4067_9596_541e9a5134cf> ;
                                                                                            <http://www.w3.org/2004/02/skos/core#prefLabel> "NitrogenSymbol"@en .


###  http://emmo.info/emmo/domain/mechanical-testing#EMMO_b424de87_996f_4117_b4bf_b5e52fe5b4d3
<http://emmo.info/emmo/domain/mechanical-testing#EMMO_b424de87_996f_4117_b4bf_b5e52fe5b4d3> rdf:type owl:Class ;
                                                                                            rdfs:subClassOf <http://emmo.info/emmo/domain/mechanical-testing#EMMO_3c7c1148_40e2_4ec2_a0ac_8720d03e356f> ;
                                                                                            rdfs:comment "The squared value of the stiffness from unloading divided by the maximum load. Is a parameter that should be insensitive to the area function. It can be used to determine load frame stiffness." ;
                                                                                            <http://www.w3.org/2004/02/skos/core#prefLabel> "SquaredStiffnessOverLoad"@en .


###  http://emmo.info/emmo/domain/mechanical-testing#EMMO_b4d92a5c_5267_46ab_abed_f000b890b9db
<http://emmo.info/emmo/domain/mechanical-testing#EMMO_b4d92a5c_5267_46ab_abed_f000b890b9db> rdf:type owl:Class ;
                                                                                            rdfs:subClassOf <http://emmo.info/emmo/domain/mechanical-testing#EMMO_e5d45f40_f9e9_47b9_934b_4c463a38b08e> ,
                                                                                                            <http://emmo.info/emmo/middle/isq#EMMO_d1917609_db5e_4b8a_9b76_ef1d6f860a81> ;
                                                                                            <http://emmo.info/emmo/middle/isq#physicalDimension> "T-2 L-1 M+1 I0 T0 N0 J0" ;
                                                                                            rdfs:comment """According to \"FKM-Richtlinie - Rechnerischer Festigkeitsnachweis (2012)\", the alternating strength is a numerical value that is calculated via the fatigue strength of a material and the mean stress factor. The alternating strength allows the engineer to compare fatigue strengths obtained from tests with different stress ratios (mean stress). It converts the fatigue strength value to an alternate strength value for R=-1.
alternating strength S_WK = fatigue strength / K_AK."""@en ;
                                                                                            <http://www.w3.org/2004/02/skos/core#prefLabel> "AlternatingStrength"@en .


###  http://emmo.info/emmo/domain/mechanical-testing#EMMO_b50db598_cfea_4582_9168_46fbc0b9ec4f
<http://emmo.info/emmo/domain/mechanical-testing#EMMO_b50db598_cfea_4582_9168_46fbc0b9ec4f> rdf:type owl:Class ;
                                                                                            rdfs:subClassOf <http://emmo.info/emmo/domain/mechanical-testing#CableBundleUseCase> ,
                                                                                                            <http://emmo.info/emmo/middle/isq#EMMO_cd2cd0de_e0cc_4ef1_b27e_2e88db027bac> ;
                                                                                            rdfs:comment "In classical geometry, a radius of a circle or sphere is any of the line segments from its center to its perimeter." ;
                                                                                            <http://www.w3.org/2004/02/skos/core#prefLabel> "Radius"@en .


###  http://emmo.info/emmo/domain/mechanical-testing#EMMO_b5e76617_a340_4ab5_8fee_4c9de18db6c6
<http://emmo.info/emmo/domain/mechanical-testing#EMMO_b5e76617_a340_4ab5_8fee_4c9de18db6c6> rdf:type owl:Class ;
                                                                                            rdfs:subClassOf <http://emmo.info/emmo/domain/mechanical-testing#EMMO_eda29fc2_7d48_4997_8593_38fd9b344fe2> ;
                                                                                            rdfs:comment "The temperature of the copper housing of the sample heater assembly." ;
                                                                                            <http://www.w3.org/2004/02/skos/core#prefLabel> "SampleHousingTemperature"@en .


###  http://emmo.info/emmo/domain/mechanical-testing#EMMO_b70a0653_b4aa_4cc5_81a7_594fa04d0730
<http://emmo.info/emmo/domain/mechanical-testing#EMMO_b70a0653_b4aa_4cc5_81a7_594fa04d0730> rdf:type owl:Class ;
                                                                                            rdfs:subClassOf <http://emmo.info/emmo/domain/mechanical-testing#EMMO_e5d45f40_f9e9_47b9_934b_4c463a38b08e> ,
                                                                                                            <http://emmo.info/emmo/middle/chemistry#EMMO_4f40def1_3cd7_4067_9596_541e9a5134cf> ;
                                                                                            <http://www.w3.org/2004/02/skos/core#prefLabel> "SilverSymbol"@en .


###  http://emmo.info/emmo/domain/mechanical-testing#EMMO_b71e5f70_227c_4798_8a8a_ee7b70afd10f
<http://emmo.info/emmo/domain/mechanical-testing#EMMO_b71e5f70_227c_4798_8a8a_ee7b70afd10f> rdf:type owl:Class ;
                                                                                            rdfs:subClassOf <http://emmo.info/emmo/domain/mechanical-testing#EMMO_87286423_f048_47ac_b8df_3235e824f277> ;
                                                                                            rdfs:comment "Finishing cuts are used to complete the part and achieve the final dimension,tolerances, and surface finish." ;
                                                                                            <http://www.w3.org/2004/02/skos/core#prefLabel> "Finishing" .


###  http://emmo.info/emmo/domain/mechanical-testing#EMMO_b82033a4_faa1_4f97_8c31_ee9148e120be
<http://emmo.info/emmo/domain/mechanical-testing#EMMO_b82033a4_faa1_4f97_8c31_ee9148e120be> rdf:type owl:Class ;
                                                                                            rdfs:subClassOf <http://emmo.info/emmo/domain/mechanical-testing#EMMO_c3c23bd2_2720_4acb_9f76_e1bb6579afca> ;
                                                                                            rdfs:comment "Surface roughness as a result from machining process (e.g. turning, milling, grinding, polishing etc.) given in terms of Rz. Average Rz value over assessement length (Rzi=maximum peak to valley height of profile, within a single sampling length i). This is equivalent to Ry5." ;
                                                                                            <http://www.w3.org/2004/02/skos/core#prefLabel> "RoughnessRz"@en .


###  http://emmo.info/emmo/domain/mechanical-testing#EMMO_ba4f6d96_699f_48ba_a432_6676521587f1
<http://emmo.info/emmo/domain/mechanical-testing#EMMO_ba4f6d96_699f_48ba_a432_6676521587f1> rdf:type owl:Class ;
                                                                                            rdfs:subClassOf <http://emmo.info/emmo/domain/mechanical-testing#EMMO_91e9c813_b277_48ad_b5b0_a781a05b9c1f> ,
                                                                                                            <http://emmo.info/emmo/middle/isq#EMMO_d4f7d378_5e3b_468a_baa1_a7e98358cda7> ;
                                                                                            rdfs:comment "This is the average time of a typical indentation cycle from load to full unload." ;
                                                                                            <http://www.w3.org/2004/02/skos/core#prefLabel> "IndentationTime"@en .


###  http://emmo.info/emmo/domain/mechanical-testing#EMMO_baf5bb96_05ea_4f78_bdb7_a556342c8b6a
<http://emmo.info/emmo/domain/mechanical-testing#EMMO_baf5bb96_05ea_4f78_bdb7_a556342c8b6a> rdf:type owl:Class ;
                                                                                            rdfs:subClassOf <http://emmo.info/emmo/domain/mechanical-testing#EMMO_e5d45f40_f9e9_47b9_934b_4c463a38b08e> ,
                                                                                                            <http://emmo.info/emmo/middle/siunits#EMMO_d41ce84b_4317_41fb_a5d1_6cd281fca106> ;
                                                                                            <http://www.w3.org/2004/02/skos/core#prefLabel> "MicroMetre"@en .


###  http://emmo.info/emmo/domain/mechanical-testing#EMMO_bb2485f3_e956_489b_8434_6f71333ae16c
<http://emmo.info/emmo/domain/mechanical-testing#EMMO_bb2485f3_e956_489b_8434_6f71333ae16c> rdf:type owl:Class ;
                                                                                            rdfs:subClassOf <http://emmo.info/emmo/domain/mechanical-testing#EMMO_16cfb313_1fea_414f_99ca_aec999e93e0c> ;
                                                                                            rdfs:comment "Steel nomenclature contains steel groups / categories as defined in the standards DIN, SAE and JIS and superclasses in which the categories from the different standards are combined" ;
                                                                                            rdfs:label "Low-alloyed steels"@en ;
                                                                                            <http://www.w3.org/2004/02/skos/core#prefLabel> "LowAlloyedSteels"@en .


###  http://emmo.info/emmo/domain/mechanical-testing#EMMO_bc7a1ff8_9c74_4147_a417_08e7867aac77
<http://emmo.info/emmo/domain/mechanical-testing#EMMO_bc7a1ff8_9c74_4147_a417_08e7867aac77> rdf:type owl:Class ;
                                                                                            rdfs:subClassOf <http://emmo.info/emmo/domain/mechanical-testing#EMMO_e8c8c152_484e_4053_8e35_82346b3fc927> ;
                                                                                            rdfs:comment "Rectangular cross section is a cross section with rectangualr shape." ;
                                                                                            <http://www.w3.org/2004/02/skos/core#prefLabel> "RectanglularCrossSection"@en .


###  http://emmo.info/emmo/domain/mechanical-testing#EMMO_bcfa65e9_ddf4_4a16_81ff_b02ae29c0a27
<http://emmo.info/emmo/domain/mechanical-testing#EMMO_bcfa65e9_ddf4_4a16_81ff_b02ae29c0a27> rdf:type owl:Class ;
                                                                                            rdfs:subClassOf <http://emmo.info/emmo/domain/mechanical-testing#EMMO_e5d45f40_f9e9_47b9_934b_4c463a38b08e> ,
                                                                                                            <http://emmo.info/emmo/middle/chemistry#EMMO_a293f923_954c_4af5_9f97_9600ebd362cb> ,
                                                                                                            <http://emmo.info/emmo/middle/isq#EMMO_faab3f84_e475_4a46_af9c_7d249f0b9aef> ;
                                                                                            <http://emmo.info/emmo/top/annotations#EMMO_967080e5_2f42_4eb2_a3a9_c58143e835f9> "The idea is to convert the percentage of alloying elements other than carbon to the equivalent carbon percentage. CEV = C + Mn/6 + (Cu + Ni)/15 + (Cr + Mo + V)/5 ." ;
                                                                                            rdfs:comment "The equivalent carbon content concept it used on ferrous materials, to determine various properties of the alloy when more than just carbon is used as an alloyant." ;
                                                                                            <http://www.w3.org/2004/02/skos/core#altLabel> "CEV" ;
                                                                                            <http://www.w3.org/2004/02/skos/core#prefLabel> "EquivalentCarbonContent"@en .


###  http://emmo.info/emmo/domain/mechanical-testing#EMMO_bd59ce5c_09a5_4912_961b_91cfbbd087f2
<http://emmo.info/emmo/domain/mechanical-testing#EMMO_bd59ce5c_09a5_4912_961b_91cfbbd087f2> rdf:type owl:Class ;
                                                                                            rdfs:subClassOf <http://emmo.info/emmo/domain/mechanical-testing#EMMO_e5d45f40_f9e9_47b9_934b_4c463a38b08e> ,
                                                                                                            <http://emmo.info/emmo/middle/metrology#EMMO_50a3552e_859a_4ff7_946d_76d537cabce6> ,
                                                                                                            <http://emmo.info/emmo/middle/metrology#EMMO_c9c8f824_9127_4f93_bc21_69fe78a7f6f2> ;
                                                                                            rdfs:comment "Vickers Hardness unit" ;
                                                                                            <http://www.w3.org/2004/02/skos/core#prefLabel> "VickersHardnessUnit"@en .


###  http://emmo.info/emmo/domain/mechanical-testing#EMMO_bd8e17c8_167a_4c72_b4ab_e8b2f69034f1
<http://emmo.info/emmo/domain/mechanical-testing#EMMO_bd8e17c8_167a_4c72_b4ab_e8b2f69034f1> rdf:type owl:Class ;
                                                                                            rdfs:subClassOf <http://emmo.info/emmo/domain/mechanical-testing#EMMO_1cbdb7f5_47e4_468a_8d87_b25093803b8e> ;
                                                                                            rdfs:comment "FlatSpecimen represents a mechanical testing specimen that has rectangular cross section." ;
                                                                                            <http://www.w3.org/2004/02/skos/core#prefLabel> "FlatSpecimen"@en .


###  http://emmo.info/emmo/domain/mechanical-testing#EMMO_bf5ed681_bd31_4994_a05b_85d1443d23b1
<http://emmo.info/emmo/domain/mechanical-testing#EMMO_bf5ed681_bd31_4994_a05b_85d1443d23b1> rdf:type owl:Class ;
                                                                                            rdfs:subClassOf <http://emmo.info/emmo/domain/mechanical-testing#EMMO_4c57e181_8205_4e51_a164_d17c4bea891d> ;
                                                                                            <http://www.w3.org/2004/02/skos/core#prefLabel> "SurfaceHardening"@en .


###  http://emmo.info/emmo/domain/mechanical-testing#EMMO_c0b46f83_fd24_420e_8cda_642fb7bf3e49
<http://emmo.info/emmo/domain/mechanical-testing#EMMO_c0b46f83_fd24_420e_8cda_642fb7bf3e49> rdf:type owl:Class ;
                                                                                            rdfs:subClassOf <http://emmo.info/emmo/domain/mechanical-testing#EMMO_ecb41be6_be55_4d5a_9c23_f5a1063cf74d> ;
                                                                                            <http://www.w3.org/2004/02/skos/core#prefLabel> "OutputParameterSet"@en .


###  http://emmo.info/emmo/domain/mechanical-testing#EMMO_c141a264_e73e_49a9_bc16_9c77b8e856bf
<http://emmo.info/emmo/domain/mechanical-testing#EMMO_c141a264_e73e_49a9_bc16_9c77b8e856bf> rdf:type owl:Class ;
                                                                                            rdfs:subClassOf <http://emmo.info/emmo/domain/mechanical-testing#EMMO_ecb41be6_be55_4d5a_9c23_f5a1063cf74d> ;
                                                                                            <http://www.w3.org/2004/02/skos/core#prefLabel> "InputParameterSet"@en .


###  http://emmo.info/emmo/domain/mechanical-testing#EMMO_c16d56fc_ad1f_420d_9d61_edbe4a28136a
<http://emmo.info/emmo/domain/mechanical-testing#EMMO_c16d56fc_ad1f_420d_9d61_edbe4a28136a> rdf:type owl:Class ;
                                                                                            rdfs:subClassOf <http://emmo.info/emmo/domain/mechanical-testing#EMMO_0f73321c_c4fd_40ed_9b58_eccd9b7d8e15> ;
                                                                                            rdfs:comment "A single indentation experiment." ;
                                                                                            <http://www.w3.org/2004/02/skos/core#prefLabel> "IndentationTest"@en .


###  http://emmo.info/emmo/domain/mechanical-testing#EMMO_c183c000_5475_4f13_96ff_fb95d627f983
<http://emmo.info/emmo/domain/mechanical-testing#EMMO_c183c000_5475_4f13_96ff_fb95d627f983> rdf:type owl:Class ;
                                                                                            rdfs:subClassOf <http://emmo.info/emmo/domain/mechanical-testing#EMMO_e32ab9e8_a962_42df_afc0_a45e1ec00e1b> ;
                                                                                            rdfs:comment """Steel category according to SAE standard:
Heat-resisting stainless steels (SAE)""" ;
                                                                                            rdfs:label "Heat-resisting stainless steels (SAE)"@en ;
                                                                                            <http://www.w3.org/2004/02/skos/core#prefLabel> "HeatResistingStainlessSteelsSAE"@en .


###  http://emmo.info/emmo/domain/mechanical-testing#EMMO_c1a5ffe0_4b14_45c4_9777_5b74a2f7eb1e
<http://emmo.info/emmo/domain/mechanical-testing#EMMO_c1a5ffe0_4b14_45c4_9777_5b74a2f7eb1e> rdf:type owl:Class ;
                                                                                            rdfs:subClassOf <http://emmo.info/emmo/domain/mechanical-testing#EMMO_2f9a266b_ffe6_4b3e_8222_eca6001174a2> ;
                                                                                            <http://www.w3.org/2004/02/skos/core#prefLabel> "SessileDropMethod"@en .


###  http://emmo.info/emmo/domain/mechanical-testing#EMMO_c21ab500_db9a_43a3_a7ef_d43fb64bf856
<http://emmo.info/emmo/domain/mechanical-testing#EMMO_c21ab500_db9a_43a3_a7ef_d43fb64bf856> rdf:type owl:Class ;
                                                                                            rdfs:subClassOf <http://emmo.info/emmo/domain/mechanical-testing#EMMO_e5d45f40_f9e9_47b9_934b_4c463a38b08e> ,
                                                                                                            <http://emmo.info/emmo/middle/perceptual#EMMO_a1083d0a_c1fb_471f_8e20_a98f881ad527> ,
                                                                                                            <http://emmo.info/emmo/middle/perceptual#EMMO_d8d2144e_5c8d_455d_a643_5caf4d8d9df8> ;
                                                                                            rdfs:comment "An identifier is a name that identifies (that is, labels the identity of) either a unique object or a unique class of objects." ;
                                                                                            rdfs:seeAlso "https://en.wikipedia.org/wiki/Identifier" ;
                                                                                            <http://www.w3.org/2004/02/skos/core#prefLabel> "Identifier"@en .


###  http://emmo.info/emmo/domain/mechanical-testing#EMMO_c3c23bd2_2720_4acb_9f76_e1bb6579afca
<http://emmo.info/emmo/domain/mechanical-testing#EMMO_c3c23bd2_2720_4acb_9f76_e1bb6579afca> rdf:type owl:Class ;
                                                                                            rdfs:subClassOf <http://emmo.info/emmo/domain/mechanical-testing#EMMO_e5d45f40_f9e9_47b9_934b_4c463a38b08e> ,
                                                                                                            <http://emmo.info/emmo/middle/metrology#EMMO_71f6ab56_342c_484b_bbe0_de86b7367cb3> ;
                                                                                            <http://www.w3.org/2004/02/skos/core#prefLabel> "Roughness"@en .


###  http://emmo.info/emmo/domain/mechanical-testing#EMMO_c43a755d_f7c7_4699_8498_4d84f92bf6df
<http://emmo.info/emmo/domain/mechanical-testing#EMMO_c43a755d_f7c7_4699_8498_4d84f92bf6df> rdf:type owl:Class ;
                                                                                            rdfs:subClassOf <http://emmo.info/emmo/domain/mechanical-testing#EMMO_2e9a014f_9337_42f7_ad91_b73f150a9901> ;
                                                                                            <http://www.w3.org/2004/02/skos/core#prefLabel> "PearliteHardening"@en .


###  http://emmo.info/emmo/domain/mechanical-testing#EMMO_c4532221_a9f8_41bd_b8d4_3869164aaf4f
<http://emmo.info/emmo/domain/mechanical-testing#EMMO_c4532221_a9f8_41bd_b8d4_3869164aaf4f> rdf:type owl:Class ;
                                                                                            rdfs:subClassOf <http://emmo.info/emmo/domain/mechanical-testing#EMMO_8e959570_c1a5_436f_bc54_08b423f4568d> ;
                                                                                            rdfs:comment "Melt processes convert a liquid melt into a solid article with a defined structure and shape." ;
                                                                                            <http://www.w3.org/2004/02/skos/core#prefLabel> "Melting" .


###  http://emmo.info/emmo/domain/mechanical-testing#EMMO_c4cb32e6_69d4_4807_b781_b1dcc867eef1
<http://emmo.info/emmo/domain/mechanical-testing#EMMO_c4cb32e6_69d4_4807_b781_b1dcc867eef1> rdf:type owl:Class ;
                                                                                            rdfs:subClassOf <http://emmo.info/emmo/domain/mechanical-testing#EMMO_e5d45f40_f9e9_47b9_934b_4c463a38b08e> ,
                                                                                                            <http://emmo.info/emmo/middle/math#EMMO_e56ee3eb_7609_4ae1_8bed_51974f0960a6> ,
                                                                                                            <http://emmo.info/emmo/middle/perceptual#EMMO_b5957cef_a287_442d_a3ce_fd39f20ba1cd> ,
                                                                                                            <http://emmo.info/emmo/middle/semiotics#EMMO_6f5af708_f825_4feb_a0d1_a8d813d3022b> ;
                                                                                            <http://www.w3.org/2004/02/skos/core#prefLabel> "SNCurve"@en .


###  http://emmo.info/emmo/domain/mechanical-testing#EMMO_c799b443_c70f_4351_bb0f_e4ab29073481
<http://emmo.info/emmo/domain/mechanical-testing#EMMO_c799b443_c70f_4351_bb0f_e4ab29073481> rdf:type owl:Class ;
                                                                                            rdfs:subClassOf <http://emmo.info/emmo/domain/mechanical-testing#EMMO_e5d45f40_f9e9_47b9_934b_4c463a38b08e> ,
                                                                                                            <http://emmo.info/emmo/middle/metrology#EMMO_71f6ab56_342c_484b_bbe0_de86b7367cb3> ;
                                                                                            <http://www.w3.org/2004/02/skos/core#prefLabel> "Hardness"@en .


###  http://emmo.info/emmo/domain/mechanical-testing#EMMO_c83ab749_46e6_46fa_be0f_12575a28a30f
<http://emmo.info/emmo/domain/mechanical-testing#EMMO_c83ab749_46e6_46fa_be0f_12575a28a30f> rdf:type owl:Class ;
                                                                                            rdfs:subClassOf <http://emmo.info/emmo/domain/mechanical-testing#EMMO_48e3eddc_de6b_4e9e_891d_99169d9f0883> ;
                                                                                            <http://www.w3.org/2004/02/skos/core#prefLabel> "Forming"@en .


###  http://emmo.info/emmo/domain/mechanical-testing#EMMO_c8e9f573_1b9a_48f6_a274_61a441f3a7c4
<http://emmo.info/emmo/domain/mechanical-testing#EMMO_c8e9f573_1b9a_48f6_a274_61a441f3a7c4> rdf:type owl:Class ;
                                                                                            rdfs:subClassOf <http://emmo.info/emmo/domain/mechanical-testing#EMMO_7452b52c_82ea_47da_b84f_493317c8f03e> ;
                                                                                            rdfs:comment "Steel nomenclature contains steel groups / categories as defined in the standards DIN, SAE and JIS and superclasses in which the categories from the different standards are combined" ;
                                                                                            rdfs:label "Tool steels"@en ;
                                                                                            <http://www.w3.org/2004/02/skos/core#prefLabel> "ToolSteels"@en .


###  http://emmo.info/emmo/domain/mechanical-testing#EMMO_c9167163_ac7f_46b0_a523_a9842f05c29c
<http://emmo.info/emmo/domain/mechanical-testing#EMMO_c9167163_ac7f_46b0_a523_a9842f05c29c> rdf:type owl:Class ;
                                                                                            rdfs:subClassOf <http://emmo.info/emmo/domain/mechanical-testing#EMMO_93c88738_64bc_49d7_9d43_f4c177a3b72e> ;
                                                                                            rdfs:comment """Steel category according to DIN standard:
Construction, engineering and pressure vessel steels, Cr-Mo with Mo < 0,4 % and Ni < 2 % (DIN 10027-2)""" ;
                                                                                            rdfs:label "Construction, engineering and pressure vessel steels, Cr-Mo with Mo < 0,4 % and Ni < 2 % (DIN 10027-2)"@en ;
                                                                                            <http://www.w3.org/2004/02/skos/core#prefLabel> "ConstructionEngineeringAndPressureVesselSteelsCrMoWithMoBelow0p4PercentAndNiBelow2PercentDIN10027"@en .


###  http://emmo.info/emmo/domain/mechanical-testing#EMMO_c9cc79d7_37cd_4b8b_b4e4_95b09ffa20b3
<http://emmo.info/emmo/domain/mechanical-testing#EMMO_c9cc79d7_37cd_4b8b_b4e4_95b09ffa20b3> rdf:type owl:Class ;
                                                                                            rdfs:subClassOf <http://emmo.info/emmo/domain/mechanical-testing#EMMO_e5d45f40_f9e9_47b9_934b_4c463a38b08e> ,
                                                                                                            <http://emmo.info/emmo/middle/chemistry#EMMO_4f40def1_3cd7_4067_9596_541e9a5134cf> ;
                                                                                            <http://www.w3.org/2004/02/skos/core#prefLabel> "TinSymbol"@en .


###  http://emmo.info/emmo/domain/mechanical-testing#EMMO_c9e3e11c_a837_4b6f_a0f6_48f1a3447616
<http://emmo.info/emmo/domain/mechanical-testing#EMMO_c9e3e11c_a837_4b6f_a0f6_48f1a3447616> rdf:type owl:Class ;
                                                                                            rdfs:subClassOf <http://emmo.info/emmo/domain/mechanical-testing#EMMO_e5d45f40_f9e9_47b9_934b_4c463a38b08e> ,
                                                                                                            <http://emmo.info/emmo/middle/chemistry#EMMO_4f40def1_3cd7_4067_9596_541e9a5134cf> ;
                                                                                            <http://www.w3.org/2004/02/skos/core#prefLabel> "ZincSymbol"@en .


###  http://emmo.info/emmo/domain/mechanical-testing#EMMO_ca42ed31_3983_4e1a_84f9_a84cab2cdb59
<http://emmo.info/emmo/domain/mechanical-testing#EMMO_ca42ed31_3983_4e1a_84f9_a84cab2cdb59> rdf:type owl:Class ;
                                                                                            rdfs:subClassOf <http://emmo.info/emmo/domain/mechanical-testing#NanoindentationUseCase> ,
                                                                                                            <http://emmo.info/emmo/middle/isq#EMMO_cd2cd0de_e0cc_4ef1_b27e_2e88db027bac> ;
                                                                                            rdfs:comment "The displacement from the center of travel of the indenter column as measured by the capacitive sensor, it is calibrated as a function of the voltage reading from the sensor." ;
                                                                                            <http://www.w3.org/2004/02/skos/core#prefLabel> "Displacement"@en .


###  http://emmo.info/emmo/domain/mechanical-testing#EMMO_cbd4cff7_fc88_43f3_882c_acc604c6d853
<http://emmo.info/emmo/domain/mechanical-testing#EMMO_cbd4cff7_fc88_43f3_882c_acc604c6d853> rdf:type owl:Class ;
                                                                                            rdfs:subClassOf <http://emmo.info/emmo/domain/mechanical-testing#EMMO_37824926_963f_4e3d_ac3c_7c323e969ff6> ;
                                                                                            <http://www.w3.org/2004/02/skos/core#prefLabel> "Shearing"@en .


###  http://emmo.info/emmo/domain/mechanical-testing#EMMO_cc1df6d0_cf70_41e1_b757_7bdad7cc459e
<http://emmo.info/emmo/domain/mechanical-testing#EMMO_cc1df6d0_cf70_41e1_b757_7bdad7cc459e> rdf:type owl:Class ;
                                                                                            rdfs:subClassOf <http://emmo.info/emmo/domain/mechanical-testing#EMMO_7452b52c_82ea_47da_b84f_493317c8f03e> ;
                                                                                            rdfs:comment "Steel nomenclature contains steel groups / categories as defined in the standards DIN, SAE and JIS and superclasses in which the categories from the different standards are combined" ;
                                                                                            rdfs:label "Spring steels"@en ;
                                                                                            <http://www.w3.org/2004/02/skos/core#prefLabel> "SpringSteels"@en .


###  http://emmo.info/emmo/domain/mechanical-testing#EMMO_cc6faafc_5942_4724_9af8_14c2be17a64a
<http://emmo.info/emmo/domain/mechanical-testing#EMMO_cc6faafc_5942_4724_9af8_14c2be17a64a> rdf:type owl:Class ;
                                                                                            rdfs:subClassOf <http://emmo.info/emmo/domain/mechanical-testing#EMMO_da87d0e5_8e93_4fc3_81b9_53f8568d4cc4> ;
                                                                                            rdfs:comment "Non-metallic inclusions are chemical compounds and nonmetals that are present in steel and other alloys. They are the product of chemical reactions, physical effects, and contamination that occurs during the melting and pouring process." ;
                                                                                            <http://www.w3.org/2004/02/skos/core#prefLabel> "Inclusion"@en .


###  http://emmo.info/emmo/domain/mechanical-testing#EMMO_cd736720_7091_493d_a1ae_3fd31721ff36
<http://emmo.info/emmo/domain/mechanical-testing#EMMO_cd736720_7091_493d_a1ae_3fd31721ff36> rdf:type owl:Class ;
                                                                                            rdfs:subClassOf <http://emmo.info/emmo/domain/mechanical-testing#EMMO_8e959570_c1a5_436f_bc54_08b423f4568d> ;
                                                                                            rdfs:comment "Casting is a process in which a liquid metal is delivered into a mold that contains a negative impression of the intended shape (in this case an ingot). The metal is poured into the mold through a hollow channel called a sprue. The metal and mold are then cooled, and the metal part (the casting) is extracted. Ingots usually require a second procedure of shaping, such as cold/hot working, cutting, or milling to produce a useful final product." ;
                                                                                            <http://www.w3.org/2004/02/skos/core#prefLabel> "IngotCasting" .


###  http://emmo.info/emmo/domain/mechanical-testing#EMMO_ce1fea85_f31d_4ad4_a717_8ef7612f651f
<http://emmo.info/emmo/domain/mechanical-testing#EMMO_ce1fea85_f31d_4ad4_a717_8ef7612f651f> rdf:type owl:Class ;
                                                                                            rdfs:subClassOf <http://emmo.info/emmo/domain/mechanical-testing#EMMO_7452b52c_82ea_47da_b84f_493317c8f03e> ;
                                                                                            rdfs:comment "Steel nomenclature contains steel groups / categories as defined in the standards DIN, SAE and JIS and superclasses in which the categories from the different standards are combined" ;
                                                                                            rdfs:label "Alloyed construction, engineering and pressure vessel steels"@en ;
                                                                                            <http://www.w3.org/2004/02/skos/core#prefLabel> "AlloyedConstructionEngineeringAndPressureVesselSteels"@en .


###  http://emmo.info/emmo/domain/mechanical-testing#EMMO_cfc07446_bcc0_4697_b854_f9ec00240297
<http://emmo.info/emmo/domain/mechanical-testing#EMMO_cfc07446_bcc0_4697_b854_f9ec00240297> rdf:type owl:Class ;
                                                                                            rdfs:subClassOf <http://emmo.info/emmo/domain/mechanical-testing#EMMO_87985f48_7967_4ed1_b23f_33357576c47d> ;
                                                                                            rdfs:comment "Turningis amachiningprocess in which acutting tool, typically a non-rotarytool bit, describes ahelixtoolpath by moving more or less linearly while the workpiecerotates." ;
                                                                                            <http://www.w3.org/2004/02/skos/core#prefLabel> "Turning" .


###  http://emmo.info/emmo/domain/mechanical-testing#EMMO_cfcbcb56_e951_4377_bd80_0c51a9d6fe6f
<http://emmo.info/emmo/domain/mechanical-testing#EMMO_cfcbcb56_e951_4377_bd80_0c51a9d6fe6f> rdf:type owl:Class ;
                                                                                            rdfs:subClassOf <http://emmo.info/emmo/domain/mechanical-testing#EMMO_4c57e181_8205_4e51_a164_d17c4bea891d> ;
                                                                                            rdfs:comment "Quenching after austenitizing is used to suppress the normal breakdown of austenite into ferrite and cementite, and to cause a partial decomposition at such a low temperature to produce martensite. To obtain this, steel requires a critical cooling velocity, which is greatly reduced by the presence of alloying elements, which therefore cause hardening with mild quenching (e.g. oil and hardening steels)." ;
                                                                                            <http://www.w3.org/2004/02/skos/core#prefLabel> "Quenching" .


###  http://emmo.info/emmo/domain/mechanical-testing#EMMO_d0a86d56_1b66_4562_bc96_4075527463ed
<http://emmo.info/emmo/domain/mechanical-testing#EMMO_d0a86d56_1b66_4562_bc96_4075527463ed> rdf:type owl:Class ;
                                                                                            rdfs:subClassOf <http://emmo.info/emmo/domain/mechanical-testing#EMMO_10f4d440_33d0_456d_b27c_83bf1d9811c0> ;
                                                                                            rdfs:comment "A measurement performed using the MeSOMICS machine." ;
                                                                                            <http://www.w3.org/2004/02/skos/core#prefLabel> "MesomicsMeasurement"@en .


###  http://emmo.info/emmo/domain/mechanical-testing#EMMO_d23111fa_d8e5_43a9_a0fe_53c322362196
<http://emmo.info/emmo/domain/mechanical-testing#EMMO_d23111fa_d8e5_43a9_a0fe_53c322362196> rdf:type owl:Class ;
                                                                                            rdfs:subClassOf <http://emmo.info/emmo/domain/mechanical-testing#EMMO_10f4d440_33d0_456d_b27c_83bf1d9811c0> ;
                                                                                            <http://www.w3.org/2004/02/skos/core#prefLabel> "TwoPointBending"@en .


###  http://emmo.info/emmo/domain/mechanical-testing#EMMO_d27a86dd_6e4d_4f89_979f_c7500876928a
<http://emmo.info/emmo/domain/mechanical-testing#EMMO_d27a86dd_6e4d_4f89_979f_c7500876928a> rdf:type owl:Class ;
                                                                                            rdfs:subClassOf <http://emmo.info/emmo/domain/mechanical-testing#EMMO_37824926_963f_4e3d_ac3c_7c323e969ff6> ;
                                                                                            <http://www.w3.org/2004/02/skos/core#prefLabel> "Tension"@en .


###  http://emmo.info/emmo/domain/mechanical-testing#EMMO_d291bbdb_322f_4758_a9cd_39ad0b91fac5
<http://emmo.info/emmo/domain/mechanical-testing#EMMO_d291bbdb_322f_4758_a9cd_39ad0b91fac5> rdf:type owl:Class ;
                                                                                            rdfs:subClassOf <http://emmo.info/emmo/domain/mechanical-testing#EMMO_2a706af8_27ae_468f_9688_fbbe4ca13a86> ;
                                                                                            rdfs:comment "Crack-origin in specimen volume." ;
                                                                                            <http://www.w3.org/2004/02/skos/core#prefLabel> "VolumeFailure"@en .


###  http://emmo.info/emmo/domain/mechanical-testing#EMMO_d39c0421_949a_41ad_96aa_bbf055760668
<http://emmo.info/emmo/domain/mechanical-testing#EMMO_d39c0421_949a_41ad_96aa_bbf055760668> rdf:type owl:Class ;
                                                                                            rdfs:subClassOf <http://emmo.info/emmo/domain/mechanical-testing#EMMO_4c57e181_8205_4e51_a164_d17c4bea891d> ,
                                                                                                            <http://emmo.info/emmo/domain/mechanical-testing#EMMO_6f5deb88_b02f_48a1_b177_ea123082d703> ;
                                                                                            rdfs:comment """Quenching is the rapid cooling of a workpiece in water, oil or air in order to obtain certain material properties. It is most commonly used to harden steel by inducing a martensite transformation.
Tempering is a heat treatment technique applied to ferrous alloys, such as steel or cast iron, to achieve greater tougness by decreasing the hardness of the alloy. The reduction in hardness is usually accompanied by an increase in ductility, thereby decreasing the brittleness of the metal. It is usually applied after quenching.""" ;
                                                                                            <http://www.w3.org/2004/02/skos/core#prefLabel> "QuenchingAndTempering"@en .


###  http://emmo.info/emmo/domain/mechanical-testing#EMMO_d4d0a51f_3b70_49ca_aca4_20b3f4648958
<http://emmo.info/emmo/domain/mechanical-testing#EMMO_d4d0a51f_3b70_49ca_aca4_20b3f4648958> rdf:type owl:Class ;
                                                                                            rdfs:subClassOf <http://emmo.info/emmo/domain/mechanical-testing#NanoindentationUseCase> ,
                                                                                                            <http://emmo.info/emmo/middle/isq#EMMO_f3dd74c0_f480_49e8_9764_33b78638c235> ;
                                                                                            <http://www.w3.org/2004/02/skos/core#prefLabel> "ContactAngle"@en .


###  http://emmo.info/emmo/domain/mechanical-testing#EMMO_d502b7c5_e898_4dfe_a0fe_6c64e922d14b
<http://emmo.info/emmo/domain/mechanical-testing#EMMO_d502b7c5_e898_4dfe_a0fe_6c64e922d14b> rdf:type owl:Class ;
                                                                                            rdfs:subClassOf <http://emmo.info/emmo/domain/mechanical-testing#EMMO_48e3eddc_de6b_4e9e_891d_99169d9f0883> ;
                                                                                            <http://www.w3.org/2004/02/skos/core#prefLabel> "MetalJoining"@en .


###  http://emmo.info/emmo/domain/mechanical-testing#EMMO_d552bbb0_ea25_40dc_bb74_ed8ff63b7998
<http://emmo.info/emmo/domain/mechanical-testing#EMMO_d552bbb0_ea25_40dc_bb74_ed8ff63b7998> rdf:type owl:Class ;
                                                                                            rdfs:subClassOf <http://emmo.info/emmo/domain/mechanical-testing#NanoindentationUseCase> ,
                                                                                                            <http://emmo.info/emmo/middle/metrology#EMMO_79751276_b2d0_4e2f_bbd4_99d412f43d55> ;
                                                                                            <http://www.w3.org/2004/02/skos/core#prefLabel> "DataAcquisitionRate"@en .


###  http://emmo.info/emmo/domain/mechanical-testing#EMMO_d5b0d9de_0ce0_4e28_8c17_9e5706baba43
<http://emmo.info/emmo/domain/mechanical-testing#EMMO_d5b0d9de_0ce0_4e28_8c17_9e5706baba43> rdf:type owl:Class ;
                                                                                            rdfs:subClassOf <http://emmo.info/emmo/domain/mechanical-testing#EMMO_1cbdb7f5_47e4_468a_8d87_b25093803b8e> ,
                                                                                                            <http://emmo.info/emmo/middle/reductionistic#EMMO_36c79456_e29c_400d_8bd3_0eedddb82652> ;
                                                                                            rdfs:comment "Notched Specimen is a MechanicalTestingSpecimen that has a notch or in other words a change in the cross section that results in an uneven stress distribution. A notched specimen has a Stress concentration factor higher than 1." ;
                                                                                            <http://www.w3.org/2004/02/skos/core#prefLabel> "NotchedSpecimen"@en .


###  http://emmo.info/emmo/domain/mechanical-testing#EMMO_d7029930_e902_418a_91b1_76040840d977
<http://emmo.info/emmo/domain/mechanical-testing#EMMO_d7029930_e902_418a_91b1_76040840d977> rdf:type owl:Class ;
                                                                                            rdfs:subClassOf <http://emmo.info/emmo/domain/mechanical-testing#EMMO_e5d45f40_f9e9_47b9_934b_4c463a38b08e> ,
                                                                                                            <http://emmo.info/emmo/middle/chemistry#EMMO_4f40def1_3cd7_4067_9596_541e9a5134cf> ;
                                                                                            <http://www.w3.org/2004/02/skos/core#prefLabel> "VanadiumSymbol"@en .


###  http://emmo.info/emmo/domain/mechanical-testing#EMMO_d7744a44_6cfe_47cd_9e10_9ec3be7f8d0c
<http://emmo.info/emmo/domain/mechanical-testing#EMMO_d7744a44_6cfe_47cd_9e10_9ec3be7f8d0c> rdf:type owl:Class ;
                                                                                            rdfs:subClassOf <http://emmo.info/emmo/middle/math#EMMO_18d180e4_5e3e_42f7_820c_e08951223486> ,
                                                                                                            <http://emmo.info/emmo/middle/properties#EMMO_b7bcff25_ffc3_474e_9ab5_01b1664bd4ba> ;
                                                                                            rdfs:comment "Depending on the type of the SN-curve model, one or several knee points exist, where the SN curve changes its slope. For ferritic steels, there is usually a constant, non-zero slope of the SN-curve in the high cycle fatigue regime (e.g. 10^4 < n < 10^6), followed by a horizontal shape of the SN curve after reaching the fatigue strength / endurance limit. In this case the knee point corresponds to the endurance limit. For other materials (e.g. aluminium or austenitic steels), a horizontal slope is never reached, but there are at least two regions with different slope, which are separated by the knee point (in terms of cycles)." ;
                                                                                            <http://www.w3.org/2004/02/skos/core#prefLabel> "KneePoint"@en .


###  http://emmo.info/emmo/domain/mechanical-testing#EMMO_d87db143_a9d9_4fe4_a61b_05ea26355783
<http://emmo.info/emmo/domain/mechanical-testing#EMMO_d87db143_a9d9_4fe4_a61b_05ea26355783> rdf:type owl:Class ;
                                                                                            rdfs:subClassOf <http://emmo.info/emmo/domain/mechanical-testing#EMMO_e5d45f40_f9e9_47b9_934b_4c463a38b08e> ,
                                                                                                            <http://emmo.info/emmo/middle/isq#EMMO_d1917609_db5e_4b8a_9b76_ef1d6f860a81> ;
                                                                                            rdfs:comment "The minimum stress S_min is the lowest occuring stress during fatigue testing." ;
                                                                                            <http://www.w3.org/2004/02/skos/core#prefLabel> "MinimumStress"@en .


###  http://emmo.info/emmo/domain/mechanical-testing#EMMO_da0493fd_72f9_4fc2_8650_2a2965606188
<http://emmo.info/emmo/domain/mechanical-testing#EMMO_da0493fd_72f9_4fc2_8650_2a2965606188> rdf:type owl:Class ;
                                                                                            rdfs:subClassOf <http://emmo.info/emmo/domain/mechanical-testing#EMMO_4c57e181_8205_4e51_a164_d17c4bea891d> ;
                                                                                            rdfs:comment "Tempering is a process of heat treating, which is used to increase the toughness of iron-based alloys. Tempering is usually performed after hardening, to reduce some of the excess hardness, and is done by heating the metal to some temperature below the critical point for a certain period of time, then allowing it to cool in still air." ;
                                                                                            <http://www.w3.org/2004/02/skos/core#prefLabel> "Tempering" .


###  http://emmo.info/emmo/domain/mechanical-testing#EMMO_da87d0e5_8e93_4fc3_81b9_53f8568d4cc4
<http://emmo.info/emmo/domain/mechanical-testing#EMMO_da87d0e5_8e93_4fc3_81b9_53f8568d4cc4> rdf:type owl:Class ;
                                                                                            rdfs:subClassOf <http://emmo.info/emmo/domain/mechanical-testing#EMMO_e5d45f40_f9e9_47b9_934b_4c463a38b08e> ;
                                                                                            rdfs:comment "Explanation for crack-initiation at origin." ;
                                                                                            <http://www.w3.org/2004/02/skos/core#prefLabel> "FailureReason"@en .


###  http://emmo.info/emmo/domain/mechanical-testing#EMMO_dad694df_6f58_4f5f_bb1d_6eb9dea25fb1
<http://emmo.info/emmo/domain/mechanical-testing#EMMO_dad694df_6f58_4f5f_bb1d_6eb9dea25fb1> rdf:type owl:Class ;
                                                                                            rdfs:subClassOf <http://emmo.info/emmo/domain/mechanical-testing#NanoindentationUseCase> ,
                                                                                                            <http://emmo.info/emmo/middle/isq#EMMO_cd2cd0de_e0cc_4ef1_b27e_2e88db027bac> ;
                                                                                            rdfs:comment "The contact depth calculated from dynamics and the Oliver and Pharr method." ;
                                                                                            <http://www.w3.org/2004/02/skos/core#prefLabel> "DynamicContactDepth"@en .


###  http://emmo.info/emmo/domain/mechanical-testing#EMMO_dbeee072_237a_42f9_845b_5f2bd3da5222
<http://emmo.info/emmo/domain/mechanical-testing#EMMO_dbeee072_237a_42f9_845b_5f2bd3da5222> rdf:type owl:Class ;
                                                                                            rdfs:subClassOf <http://emmo.info/emmo/domain/mechanical-testing#EMMO_0b47a9ad_2854_43d0_9707_ff5f81f5b7d8> ,
                                                                                                            <http://emmo.info/emmo/middle/holistic#EMMO_49804605_c0fe_4538_abda_f70ba1dc8a5d> ;
                                                                                            rdfs:comment "AveragedTorsionalStifness is a phyiscal quantity of the type of torsional stiffness that results from a calculation of the type arithmetic mean." ;
                                                                                            <http://www.w3.org/2004/02/skos/core#prefLabel> "AveragedTorsionalStiffness"@en .


###  http://emmo.info/emmo/domain/mechanical-testing#EMMO_dc56a625_9376_4434_a554_2d1153348c97
<http://emmo.info/emmo/domain/mechanical-testing#EMMO_dc56a625_9376_4434_a554_2d1153348c97> rdf:type owl:Class ;
                                                                                            rdfs:subClassOf <http://emmo.info/emmo/domain/mechanical-testing#EMMO_91e9c813_b277_48ad_b5b0_a781a05b9c1f> ,
                                                                                                            <http://emmo.info/emmo/domain/mechanical-testing#EMMO_ee09aa64_f477_4e8f_8b0c_f5d30177ba8d> ;
                                                                                            rdfs:comment "The maximum penetration depth attained during a nanoindentation test." ;
                                                                                            <http://www.w3.org/2004/02/skos/core#prefLabel> "MaximumDepth"@en .


###  http://emmo.info/emmo/domain/mechanical-testing#EMMO_dc637a06_1988_4f9a_a2b4_05dfbf7e246c
<http://emmo.info/emmo/domain/mechanical-testing#EMMO_dc637a06_1988_4f9a_a2b4_05dfbf7e246c> rdf:type owl:Class ;
                                                                                            rdfs:subClassOf <http://emmo.info/emmo/domain/mechanical-testing#CableBundleUseCase> ,
                                                                                                            <http://emmo.info/emmo/middle/manufacturing#EMMO_ec7464a9_d99d_45f8_965b_4e9230ea8356> ;
                                                                                            rdfs:comment "Tape represents an engineered material. It is defined as a strip of material, typically used to hold something." ;
                                                                                            <http://www.w3.org/2004/02/skos/core#prefLabel> "Tape"@en .


###  http://emmo.info/emmo/domain/mechanical-testing#EMMO_de2e853c_c30e_4710_9c8a_671dba758955
<http://emmo.info/emmo/domain/mechanical-testing#EMMO_de2e853c_c30e_4710_9c8a_671dba758955> rdf:type owl:Class ;
                                                                                            rdfs:subClassOf <http://emmo.info/emmo/domain/mechanical-testing#NanoindentationUseCase> ,
                                                                                                            <http://emmo.info/emmo/middle/manufacturing#EMMO_494b372c_cfdf_47d3_a4de_5e037c540de8> ;
                                                                                            <http://www.w3.org/2004/02/skos/core#prefLabel> "IndenterDevice"@en .


###  http://emmo.info/emmo/domain/mechanical-testing#EMMO_de956783_463e_40d2_b84c_4c493eadb3d4
<http://emmo.info/emmo/domain/mechanical-testing#EMMO_de956783_463e_40d2_b84c_4c493eadb3d4> rdf:type owl:Class ;
                                                                                            rdfs:subClassOf <http://emmo.info/emmo/domain/mechanical-testing#EMMO_58da328c_f504_44f9_9a78_ef62e50bb6b1> ;
                                                                                            <http://www.w3.org/2004/02/skos/core#prefLabel> "HotForging"@en .


###  http://emmo.info/emmo/domain/mechanical-testing#EMMO_df1db910_9601_4420_82b0_3a6ddaf93094
<http://emmo.info/emmo/domain/mechanical-testing#EMMO_df1db910_9601_4420_82b0_3a6ddaf93094> rdf:type owl:Class ;
                                                                                            rdfs:subClassOf <http://emmo.info/emmo/domain/mechanical-testing#CableBundleUseCase> ,
                                                                                                            <http://emmo.info/emmo/domain/mechanical-testing#EMMO_e5d45f40_f9e9_47b9_934b_4c463a38b08e> ,
                                                                                                            <http://emmo.info/emmo/domain/mechanical-testing#NanoindentationUseCase> ,
                                                                                                            <http://emmo.info/emmo/middle/semiotics#EMMO_6f5af708_f825_4feb_a0d1_a8d813d3022b> ;
                                                                                            <http://emmo.info/emmo/top/annotations#elucidation> """A typical substrate might be a metal, onto which a coating might be deposited.
For instance, in the contact angle meadurement, the substrate is the sample to be examined concerning its wettability.""" ;
                                                                                            rdfs:comment "Substrate is a term used in materials science to describe the base material on which processing is conducted to produce new film or layers of material such as deposited coatings." ;
                                                                                            rdfs:isDefinedBy "https://en.wikipedia.org/wiki/Substrate_(materials_science)" ;
                                                                                            <http://www.w3.org/2004/02/skos/core#prefLabel> "Substrate"@en .


###  http://emmo.info/emmo/domain/mechanical-testing#EMMO_e199bfdb_f084_4ab0_8951_706248d15c32
<http://emmo.info/emmo/domain/mechanical-testing#EMMO_e199bfdb_f084_4ab0_8951_706248d15c32> rdf:type owl:Class ;
                                                                                            rdfs:subClassOf <http://emmo.info/emmo/domain/mechanical-testing#EMMO_8828c7d2_8f7d_4804_8e13_336d37d94ec2> ,
                                                                                                            <http://emmo.info/emmo/middle/reductionistic#EMMO_36c79456_e29c_400d_8bd3_0eedddb82652> ;
                                                                                            rdfs:comment "One single cable, e.g. a sensor cable with effective properties (e.g. bending stiffness)." ;
                                                                                            <http://www.w3.org/2004/02/skos/core#prefLabel> "SingleCable"@en .


###  http://emmo.info/emmo/domain/mechanical-testing#EMMO_e30fc4f3_fbb6_4bf0_afc3_d3aeb802f2e0
<http://emmo.info/emmo/domain/mechanical-testing#EMMO_e30fc4f3_fbb6_4bf0_afc3_d3aeb802f2e0> rdf:type owl:Class ;
                                                                                            rdfs:subClassOf <http://emmo.info/emmo/domain/mechanical-testing#EMMO_e5d45f40_f9e9_47b9_934b_4c463a38b08e> ,
                                                                                                            <http://emmo.info/emmo/middle/chemistry#EMMO_4f40def1_3cd7_4067_9596_541e9a5134cf> ;
                                                                                            <http://www.w3.org/2004/02/skos/core#prefLabel> "AluminiumSymbol"@en .


###  http://emmo.info/emmo/domain/mechanical-testing#EMMO_e32ab9e8_a962_42df_afc0_a45e1ec00e1b
<http://emmo.info/emmo/domain/mechanical-testing#EMMO_e32ab9e8_a962_42df_afc0_a45e1ec00e1b> rdf:type owl:Class ;
                                                                                            rdfs:subClassOf <http://emmo.info/emmo/domain/mechanical-testing#EMMO_fe655c2d_4f4c_43ce_9528_8bcb2a81485d> ;
                                                                                            rdfs:comment "Steel nomenclature contains steel groups / categories as defined in the standards DIN, SAE and JIS and superclasses in which the categories from the different standards are combined" ;
                                                                                            rdfs:label "Heat-resisting and stainless steels"@en ;
                                                                                            <http://www.w3.org/2004/02/skos/core#prefLabel> "HeatResistingAndStainlessSteels"@en .


###  http://emmo.info/emmo/domain/mechanical-testing#EMMO_e3665cba_b1a8_4fcf_8194_493187fcd25a
<http://emmo.info/emmo/domain/mechanical-testing#EMMO_e3665cba_b1a8_4fcf_8194_493187fcd25a> rdf:type owl:Class ;
                                                                                            rdfs:subClassOf <http://emmo.info/emmo/domain/mechanical-testing#MechanicalTestingOntology> ;
                                                                                            <http://www.w3.org/2004/02/skos/core#prefLabel> "ContactAngleUseCase"@en .


###  http://emmo.info/emmo/domain/mechanical-testing#EMMO_e5d45f40_f9e9_47b9_934b_4c463a38b08e
<http://emmo.info/emmo/domain/mechanical-testing#EMMO_e5d45f40_f9e9_47b9_934b_4c463a38b08e> rdf:type owl:Class ;
                                                                                            rdfs:subClassOf <http://emmo.info/emmo/domain/mechanical-testing#MechanicalTestingOntology> ;
                                                                                            rdfs:comment "This is the artificial parent concept of the classes related to the Fatigue Use Case within this ontology." ;
                                                                                            <http://www.w3.org/2004/02/skos/core#prefLabel> "FatigueUseCase"@en .


###  http://emmo.info/emmo/domain/mechanical-testing#EMMO_e6d1f1d4_6280_4c52_9a09_288c4b58e416
<http://emmo.info/emmo/domain/mechanical-testing#EMMO_e6d1f1d4_6280_4c52_9a09_288c4b58e416> rdf:type owl:Class ;
                                                                                            rdfs:subClassOf <http://emmo.info/emmo/domain/mechanical-testing#EMMO_4c57e181_8205_4e51_a164_d17c4bea891d> ;
                                                                                            rdfs:comment "Austenitizing describes the process of heating a steel above the austenitizing temperature (GSE line in the iron carbon diagram). This process changes the lattice structure from a body centered cubic structure (BCC) to a face centered cubic structure (FCC), allowing a martensitic transformation via quenching." ;
                                                                                            <http://www.w3.org/2004/02/skos/core#altLabel> "Austenitizing" ;
                                                                                            <http://www.w3.org/2004/02/skos/core#prefLabel> "Austenitising" .


###  http://emmo.info/emmo/domain/mechanical-testing#EMMO_e723d828_7090_4685_ac7b_b3c2c5f091f1
<http://emmo.info/emmo/domain/mechanical-testing#EMMO_e723d828_7090_4685_ac7b_b3c2c5f091f1> rdf:type owl:Class ;
                                                                                            rdfs:subClassOf <http://emmo.info/emmo/domain/mechanical-testing#EMMO_06390646_6edb_4410_b22b_f7adbd6025c4> ;
                                                                                            rdfs:comment "Austenite, also known asgamma-phase iron, is a metallic, non-magneticallotrope of ironor asolid solutionofiron, with analloyingelement. Inplain-carbon steel, austenite exists above the criticaleutectoidtemperature of 1000 K (727C); other alloys ofsteelhave different eutectoid temperatures." ;
                                                                                            rdfs:label "Austenite"@en ;
                                                                                            <http://www.w3.org/2004/02/skos/core#prefLabel> "Austenite" .


###  http://emmo.info/emmo/domain/mechanical-testing#EMMO_e767adc2_9823_4cdd_88c7_6b698d89b720
<http://emmo.info/emmo/domain/mechanical-testing#EMMO_e767adc2_9823_4cdd_88c7_6b698d89b720> rdf:type owl:Class ;
                                                                                            rdfs:subClassOf <http://emmo.info/emmo/domain/mechanical-testing#EMMO_58da328c_f504_44f9_9a78_ef62e50bb6b1> ;
                                                                                            <http://www.w3.org/2004/02/skos/core#prefLabel> "ColdForging"@en .


###  http://emmo.info/emmo/domain/mechanical-testing#EMMO_e77aec7f_c6cb_40f1_834c_df04d0822305
<http://emmo.info/emmo/domain/mechanical-testing#EMMO_e77aec7f_c6cb_40f1_834c_df04d0822305> rdf:type owl:Class ;
                                                                                            rdfs:subClassOf <http://emmo.info/emmo/domain/mechanical-testing#EMMO_37824926_963f_4e3d_ac3c_7c323e969ff6> ;
                                                                                            <http://www.w3.org/2004/02/skos/core#prefLabel> "Superposition"@en .


###  http://emmo.info/emmo/domain/mechanical-testing#EMMO_e8c8c152_484e_4053_8e35_82346b3fc927
<http://emmo.info/emmo/domain/mechanical-testing#EMMO_e8c8c152_484e_4053_8e35_82346b3fc927> rdf:type owl:Class ;
                                                                                            rdfs:subClassOf <http://emmo.info/emmo/domain/mechanical-testing#EMMO_e5d45f40_f9e9_47b9_934b_4c463a38b08e> ,
                                                                                                            <http://emmo.info/emmo/middle/perceptual#EMMO_b5957cef_a287_442d_a3ce_fd39f20ba1cd> ;
                                                                                            rdfs:comment "Represents the geometry/shape of the cross section" ;
                                                                                            <http://www.w3.org/2004/02/skos/core#prefLabel> "CrossSectionGeometry"@en .


###  http://emmo.info/emmo/domain/mechanical-testing#EMMO_e8ed26aa_3a68_4ca0_b064_ca6c4dad1140
<http://emmo.info/emmo/domain/mechanical-testing#EMMO_e8ed26aa_3a68_4ca0_b064_ca6c4dad1140> rdf:type owl:Class ;
                                                                                            rdfs:subClassOf <http://emmo.info/emmo/domain/mechanical-testing#EMMO_c8e9f573_1b9a_48f6_a274_61a441f3a7c4> ;
                                                                                            rdfs:comment """Steel category according to JIS standard:
Carbon tool steels (JIS)""" ;
                                                                                            rdfs:label "Carbon tool steels (JIS)"@en ;
                                                                                            <http://www.w3.org/2004/02/skos/core#prefLabel> "CarbonToolSteelsJIS"@en .


###  http://emmo.info/emmo/domain/mechanical-testing#EMMO_e938bea8_eb34_4c90_877c_481d6ed9fa08
<http://emmo.info/emmo/domain/mechanical-testing#EMMO_e938bea8_eb34_4c90_877c_481d6ed9fa08> rdf:type owl:Class ;
                                                                                            rdfs:subClassOf <http://emmo.info/emmo/domain/mechanical-testing#EMMO_e32ab9e8_a962_42df_afc0_a45e1ec00e1b> ;
                                                                                            rdfs:comment """Steel category according to JIS standard:
Heat-resisting steel bars and wire rods (JIS)""" ;
                                                                                            rdfs:label "Heat-resisting steel bars and wire rods (JIS)"@en ;
                                                                                            <http://www.w3.org/2004/02/skos/core#prefLabel> "HeatResistingSteelBarsAndWireRodsJIS"@en .


###  http://emmo.info/emmo/domain/mechanical-testing#EMMO_ebb3c390_173a_4c23_a338_12b6a75ddab2
<http://emmo.info/emmo/domain/mechanical-testing#EMMO_ebb3c390_173a_4c23_a338_12b6a75ddab2> rdf:type owl:Class ;
                                                                                            rdfs:subClassOf <http://emmo.info/emmo/domain/mechanical-testing#EMMO_91e9c813_b277_48ad_b5b0_a781a05b9c1f> ;
                                                                                            rdfs:comment "The noise floor in the displacement measurement system will determine what the minimum useable indentation depth." ;
                                                                                            <http://www.w3.org/2004/02/skos/core#prefLabel> "DisplacementNoiseFloor"@en .


###  http://emmo.info/emmo/domain/mechanical-testing#EMMO_ecb41be6_be55_4d5a_9c23_f5a1063cf74d
<http://emmo.info/emmo/domain/mechanical-testing#EMMO_ecb41be6_be55_4d5a_9c23_f5a1063cf74d> rdf:type owl:Class ;
                                                                                            rdfs:subClassOf <http://emmo.info/emmo/domain/mechanical-testing#EMMO_e5d45f40_f9e9_47b9_934b_4c463a38b08e> ;
                                                                                            <http://www.w3.org/2004/02/skos/core#prefLabel> "ParameterSet"@en .


###  http://emmo.info/emmo/domain/mechanical-testing#EMMO_ecc66886_7f39_42a5_99f4_c260b74ed7f5
<http://emmo.info/emmo/domain/mechanical-testing#EMMO_ecc66886_7f39_42a5_99f4_c260b74ed7f5> rdf:type owl:Class ;
                                                                                            rdfs:subClassOf <http://emmo.info/emmo/domain/mechanical-testing#EMMO_c16d56fc_ad1f_420d_9d61_edbe4a28136a> ;
                                                                                            rdfs:comment "An indentation test where only the maximum applied load is controlled." ;
                                                                                            <http://www.w3.org/2004/02/skos/core#prefLabel> "StaticIndentation"@en .


###  http://emmo.info/emmo/domain/mechanical-testing#EMMO_eda29fc2_7d48_4997_8593_38fd9b344fe2
<http://emmo.info/emmo/domain/mechanical-testing#EMMO_eda29fc2_7d48_4997_8593_38fd9b344fe2> rdf:type owl:Class ;
                                                                                            rdfs:subClassOf <http://emmo.info/emmo/domain/mechanical-testing#NanoindentationUseCase> ,
                                                                                                            <http://emmo.info/emmo/middle/properties#EMMO_b7bcff25_ffc3_474e_9ab5_01b1664bd4ba> ;
                                                                                            rdfs:comment "Represents the properties properties of the NanoindentationSpecimen." ;
                                                                                            <http://www.w3.org/2004/02/skos/core#prefLabel> "NanoindentationSpecimenProperty"@en .


###  http://emmo.info/emmo/domain/mechanical-testing#EMMO_ee09aa64_f477_4e8f_8b0c_f5d30177ba8d
<http://emmo.info/emmo/domain/mechanical-testing#EMMO_ee09aa64_f477_4e8f_8b0c_f5d30177ba8d> rdf:type owl:Class ;
                                                                                            rdfs:subClassOf <http://emmo.info/emmo/domain/mechanical-testing#NanoindentationUseCase> ,
                                                                                                            <http://emmo.info/emmo/middle/isq#EMMO_cd2cd0de_e0cc_4ef1_b27e_2e88db027bac> ;
                                                                                            rdfs:comment "The depth of the indentation. It is the zeroed value of the displacement corrected for load frame stiffness and drift rate- It is zero prior to surface detection." ;
                                                                                            <http://www.w3.org/2004/02/skos/core#prefLabel> "Depth"@en .


###  http://emmo.info/emmo/domain/mechanical-testing#EMMO_ee7743e6_9de1_4a64_a784_c49a49f4be25
<http://emmo.info/emmo/domain/mechanical-testing#EMMO_ee7743e6_9de1_4a64_a784_c49a49f4be25> rdf:type owl:Class ;
                                                                                            rdfs:subClassOf <http://emmo.info/emmo/domain/mechanical-testing#EMMO_06390646_6edb_4410_b22b_f7adbd6025c4> ;
                                                                                            rdfs:comment "Bainite is a plate-like microstructure that forms in steels at temperatures of 125550C (depending on alloy content). It is one of the products that may form when austenite (the face-centered cubic crystal structure of iron) is cooled past a temperature where it no longer is thermodynamically stable with respect to ferrite, cementite, or ferrite and cementite." ;
                                                                                            <http://www.w3.org/2004/02/skos/core#prefLabel> "Bainite"@en .


###  http://emmo.info/emmo/domain/mechanical-testing#EMMO_f01503f3_f77d_49ec_b97f_56440ea8e2a2
<http://emmo.info/emmo/domain/mechanical-testing#EMMO_f01503f3_f77d_49ec_b97f_56440ea8e2a2> rdf:type owl:Class ;
                                                                                            rdfs:subClassOf <http://emmo.info/emmo/domain/mechanical-testing#EMMO_bf5ed681_bd31_4994_a05b_85d1443d23b1> ;
                                                                                            rdfs:comment "Surface hardening (or case-hardening) is the process of hardening the surface of a metal object while allowing the metal deeper underneath to remain soft, thus forming a thin layer of harder metal at the surface. This creates a hardness profile across the cross section of the material. In the end, increased hardness at the surface is combined with a ductile core, which prevents the material from becoming brittle." ;
                                                                                            <http://www.w3.org/2004/02/skos/core#prefLabel> "CaseHardening"@en .


###  http://emmo.info/emmo/domain/mechanical-testing#EMMO_f0ad542d_ff13_4998_9e7f_ea27583c5f31
<http://emmo.info/emmo/domain/mechanical-testing#EMMO_f0ad542d_ff13_4998_9e7f_ea27583c5f31> rdf:type owl:Class ;
                                                                                            rdfs:subClassOf <http://emmo.info/emmo/domain/mechanical-testing#NanoindentationUseCase> ,
                                                                                                            <http://emmo.info/emmo/middle/metrology#EMMO_71f6ab56_342c_484b_bbe0_de86b7367cb3> ;
                                                                                            <http://www.w3.org/2004/02/skos/core#prefLabel> "ElasticModulus"@en .


###  http://emmo.info/emmo/domain/mechanical-testing#EMMO_f210d615_89a5_483f_a8b2_923ff6fcf4ab
<http://emmo.info/emmo/domain/mechanical-testing#EMMO_f210d615_89a5_483f_a8b2_923ff6fcf4ab> rdf:type owl:Class ;
                                                                                            rdfs:subClassOf <http://emmo.info/emmo/domain/mechanical-testing#EMMO_3c835c69_11a9_458d_9b3f_bc68c0348c7d> ;
                                                                                            rdfs:comment "Post processing is a process/operation on the data set that enables extrating useful information from the data.  There are diffrent type of post-processors such as visualizers, converters, extractors." ;
                                                                                            <http://www.w3.org/2004/02/skos/core#prefLabel> "DataPostProcessing"@en .


###  http://emmo.info/emmo/domain/mechanical-testing#EMMO_f229418b_b1f5_41bd_8aad_ae690b380d29
<http://emmo.info/emmo/domain/mechanical-testing#EMMO_f229418b_b1f5_41bd_8aad_ae690b380d29> rdf:type owl:Class ;
                                                                                            rdfs:subClassOf <http://emmo.info/emmo/domain/mechanical-testing#EMMO_10f4d440_33d0_456d_b27c_83bf1d9811c0> ;
                                                                                            <http://www.w3.org/2004/02/skos/core#prefLabel> "CantileverBending"@en .


###  http://emmo.info/emmo/domain/mechanical-testing#EMMO_f234208c_b6ce_4890_9535_254b3a67edb7
<http://emmo.info/emmo/domain/mechanical-testing#EMMO_f234208c_b6ce_4890_9535_254b3a67edb7> rdf:type owl:Class ;
                                                                                            rdfs:subClassOf <http://emmo.info/emmo/domain/mechanical-testing#EMMO_37824926_963f_4e3d_ac3c_7c323e969ff6> ;
                                                                                            <http://www.w3.org/2004/02/skos/core#prefLabel> "Torsion"@en .


###  http://emmo.info/emmo/domain/mechanical-testing#EMMO_f2d6622f_83f7_4b66_b75c_d4576ad5d986
<http://emmo.info/emmo/domain/mechanical-testing#EMMO_f2d6622f_83f7_4b66_b75c_d4576ad5d986> rdf:type owl:Class ;
                                                                                            rdfs:subClassOf <http://emmo.info/emmo/domain/mechanical-testing#NanoindentationUseCase> ,
                                                                                                            <http://emmo.info/emmo/middle/manufacturing#EMMO_494b372c_cfdf_47d3_a4de_5e037c540de8> ,
                                                                                                            <http://emmo.info/emmo/middle/semiotics#EMMO_6f5af708_f825_4feb_a0d1_a8d813d3022b> ;
                                                                                            rdfs:comment """The probe used during an indentation test, generally composed by three parts:
1.	The diamond;
2.	The holder;
3.	The bond;""" ;
                                                                                            <http://www.w3.org/2004/02/skos/core#prefLabel> "IndenterTip"@en .


###  http://emmo.info/emmo/domain/mechanical-testing#EMMO_f386fe2e_f871_4dcb_ba95_90663bcd6129
<http://emmo.info/emmo/domain/mechanical-testing#EMMO_f386fe2e_f871_4dcb_ba95_90663bcd6129> rdf:type owl:Class ;
                                                                                            rdfs:subClassOf <http://emmo.info/emmo/domain/mechanical-testing#EMMO_709d4e04_e972_4f57_9589_bf99ea08d2ea> ,
                                                                                                            <http://emmo.info/emmo/domain/mechanical-testing#EMMO_dc637a06_1988_4f9a_a2b4_05dfbf7e246c> ;
                                                                                            rdfs:comment "Insulating tape (electrical insulating tape) is a type of pressure-sensitive tape used to insulate electrical wires and other materials that conduct electricity. It describes the type of tape as insulating material in cable bundles." ;
                                                                                            <http://www.w3.org/2004/02/skos/core#prefLabel> "InsulatingTape"@en .


###  http://emmo.info/emmo/domain/mechanical-testing#EMMO_f42ef6fc_110b_4491_8534_80bd6cfa80cb
<http://emmo.info/emmo/domain/mechanical-testing#EMMO_f42ef6fc_110b_4491_8534_80bd6cfa80cb> rdf:type owl:Class ;
                                                                                            rdfs:subClassOf <http://emmo.info/emmo/domain/mechanical-testing#EMMO_bf5ed681_bd31_4994_a05b_85d1443d23b1> ;
                                                                                            <http://www.w3.org/2004/02/skos/core#prefLabel> "Nitrocarburizing"@en .


###  http://emmo.info/emmo/domain/mechanical-testing#EMMO_f45d46c8_1ee5_4e71_a666_12e5eedc2770
<http://emmo.info/emmo/domain/mechanical-testing#EMMO_f45d46c8_1ee5_4e71_a666_12e5eedc2770> rdf:type owl:Class ;
                                                                                            rdfs:subClassOf <http://emmo.info/emmo/domain/mechanical-testing#NanoindentationUseCase> ,
                                                                                                            <http://emmo.info/emmo/middle/isq#EMMO_96f39f77_44dc_491b_8fa7_30d887fe0890> ;
                                                                                            rdfs:comment "The area of contact between the tip and the specimen calculated from the maximum applied load, the maximum depth of penetration and the unloading data using the Oliver and Pharr technique." ;
                                                                                            <http://www.w3.org/2004/02/skos/core#prefLabel> "ContactAreaFromUnload"@en .


###  http://emmo.info/emmo/domain/mechanical-testing#EMMO_f77b52b9_0750_4dbf_a131_faecbbb7f6a4
<http://emmo.info/emmo/domain/mechanical-testing#EMMO_f77b52b9_0750_4dbf_a131_faecbbb7f6a4> rdf:type owl:Class ;
                                                                                            rdfs:subClassOf <http://emmo.info/emmo/domain/mechanical-testing#EMMO_1cbdb7f5_47e4_468a_8d87_b25093803b8e> ;
                                                                                            rdfs:comment "Mesomics specimen is a mechanical testing specimen, sample that is used in a mesomics measurement. A mesomics specimen consists of a cable sample." ;
                                                                                            <http://www.w3.org/2004/02/skos/core#prefLabel> "MesomicsSpecimen"@en .


###  http://emmo.info/emmo/domain/mechanical-testing#EMMO_f7ce04b7_d252_4e30_b3ce_eb2346951a6b
<http://emmo.info/emmo/domain/mechanical-testing#EMMO_f7ce04b7_d252_4e30_b3ce_eb2346951a6b> rdf:type owl:Class ;
                                                                                            rdfs:subClassOf <http://emmo.info/emmo/domain/mechanical-testing#EMMO_76471eff_11f6_4b51_a6e0_3923a7ecfa2e> ;
                                                                                            rdfs:comment """Steel category (no specific standard):
Construction steels (Misc.)""" ;
                                                                                            rdfs:label "Construction steels (Misc.)"@en ;
                                                                                            <http://www.w3.org/2004/02/skos/core#prefLabel> "ConstructionSteelsMisc"@en .


###  http://emmo.info/emmo/domain/mechanical-testing#EMMO_f80b05af_5a68_495f_b722_25b4ac3fdfa9
<http://emmo.info/emmo/domain/mechanical-testing#EMMO_f80b05af_5a68_495f_b722_25b4ac3fdfa9> rdf:type owl:Class ;
                                                                                            rdfs:subClassOf <http://emmo.info/emmo/domain/mechanical-testing#EMMO_2697e9d2_e173_411c_8c4b_2b400ab6b1b9> ;
                                                                                            <http://www.w3.org/2004/02/skos/core#prefLabel> "RotatingBending"@en .


###  http://emmo.info/emmo/domain/mechanical-testing#EMMO_f80d451a_9146_47db_bd9a_41e9f7e4b88e
<http://emmo.info/emmo/domain/mechanical-testing#EMMO_f80d451a_9146_47db_bd9a_41e9f7e4b88e> rdf:type owl:Class ;
                                                                                            rdfs:subClassOf <http://emmo.info/emmo/domain/mechanical-testing#EMMO_a30a7cdc_f652_4b01_b8c2_cd056f3e3d85> ;
                                                                                            <http://www.w3.org/2004/02/skos/core#prefLabel> "TensileTestingMachine"@en .


###  http://emmo.info/emmo/domain/mechanical-testing#EMMO_f8448aef_c62e_448a_87e3_b7e670566de3
<http://emmo.info/emmo/domain/mechanical-testing#EMMO_f8448aef_c62e_448a_87e3_b7e670566de3> rdf:type owl:Class ;
                                                                                            rdfs:subClassOf <http://emmo.info/emmo/domain/mechanical-testing#EMMO_81dd7f19_073d_4153_9517_823edac9fac7> ;
                                                                                            rdfs:comment "Taping that covers the cable bundle entire lateral surface area." ;
                                                                                            <http://www.w3.org/2004/02/skos/core#prefLabel> "FullyTaping"@en .


###  http://emmo.info/emmo/domain/mechanical-testing#EMMO_fa443ad2_dac1_418e_b7ff_8051096e27e4
<http://emmo.info/emmo/domain/mechanical-testing#EMMO_fa443ad2_dac1_418e_b7ff_8051096e27e4> rdf:type owl:Class ;
                                                                                            rdfs:subClassOf <http://emmo.info/emmo/domain/mechanical-testing#EMMO_b50db598_cfea_4582_9168_46fbc0b9ec4f> ;
                                                                                            <http://www.w3.org/2004/02/skos/core#prefLabel> "InnerRadius"@en .


###  http://emmo.info/emmo/domain/mechanical-testing#EMMO_fb0dd8d8_1dc7_489d_b3f5_7c04ba7df433
<http://emmo.info/emmo/domain/mechanical-testing#EMMO_fb0dd8d8_1dc7_489d_b3f5_7c04ba7df433> rdf:type owl:Class ;
                                                                                            rdfs:subClassOf <http://emmo.info/emmo/domain/mechanical-testing#NanoindentationUseCase> ,
                                                                                                            <http://emmo.info/emmo/middle/metrology#EMMO_79751276_b2d0_4e2f_bbd4_99d412f43d55> ;
                                                                                            <http://emmo.info/emmo/middle/isq#physicalDimension> "T-2 L+1 M+1 I0 T0 N0 J0" ;
                                                                                            rdfs:comment "The amplitude of the force value oscillation reading, with respect to its quasi static value." ;
                                                                                            <http://www.w3.org/2004/02/skos/core#prefLabel> "AmplitudeOfOscillatoryForce"@en .


###  http://emmo.info/emmo/domain/mechanical-testing#EMMO_fb32d59e_b09b_4bdc_ba0a_5a927be64f27
<http://emmo.info/emmo/domain/mechanical-testing#EMMO_fb32d59e_b09b_4bdc_ba0a_5a927be64f27> rdf:type owl:Class ;
                                                                                            rdfs:subClassOf <http://emmo.info/emmo/domain/mechanical-testing#EMMO_1cbdb7f5_47e4_468a_8d87_b25093803b8e> ;
                                                                                            rdfs:comment "RoundSpecimen represents a mechanical testing specimen that has circular cross section." ;
                                                                                            <http://www.w3.org/2004/02/skos/core#prefLabel> "RoundSpecimen"@en .


###  http://emmo.info/emmo/domain/mechanical-testing#EMMO_fd952898_9cf1_447b_8b81_95b8773ace8f
<http://emmo.info/emmo/domain/mechanical-testing#EMMO_fd952898_9cf1_447b_8b81_95b8773ace8f> rdf:type owl:Class ;
                                                                                            rdfs:subClassOf <http://emmo.info/emmo/domain/mechanical-testing#EMMO_e32ab9e8_a962_42df_afc0_a45e1ec00e1b> ;
                                                                                            rdfs:comment """Steel category according to JIS standard:
Stainless steels (JIS)""" ;
                                                                                            rdfs:label "Stainless steels (JIS)"@en ;
                                                                                            <http://www.w3.org/2004/02/skos/core#prefLabel> "StainlessSteelsJIS"@en .


###  http://emmo.info/emmo/domain/mechanical-testing#EMMO_fe13168c_8e04_4cbf_8462_641669a4b7f3
<http://emmo.info/emmo/domain/mechanical-testing#EMMO_fe13168c_8e04_4cbf_8462_641669a4b7f3> rdf:type owl:Class ;
                                                                                            rdfs:subClassOf <http://emmo.info/emmo/domain/mechanical-testing#EMMO_a30a7cdc_f652_4b01_b8c2_cd056f3e3d85> ;
                                                                                            <http://www.w3.org/2004/02/skos/core#prefLabel> "FatigueTestingMachine"@en .


###  http://emmo.info/emmo/domain/mechanical-testing#EMMO_fe655c2d_4f4c_43ce_9528_8bcb2a81485d
<http://emmo.info/emmo/domain/mechanical-testing#EMMO_fe655c2d_4f4c_43ce_9528_8bcb2a81485d> rdf:type owl:Class ;
                                                                                            rdfs:subClassOf <http://emmo.info/emmo/domain/mechanical-testing#EMMO_16cfb313_1fea_414f_99ca_aec999e93e0c> ;
                                                                                            rdfs:comment "Steel nomenclature contains steel groups / categories as defined in the standards DIN, SAE and JIS and superclasses in which the categories from the different standards are combined" ;
                                                                                            rdfs:label "Stainless steels"@en ;
                                                                                            <http://www.w3.org/2004/02/skos/core#prefLabel> "StainlessSteels"@en .


###  http://emmo.info/emmo/domain/mechanical-testing#EMMO_fffa2163_8ecd_4775_a908_c5eb6af6be45
<http://emmo.info/emmo/domain/mechanical-testing#EMMO_fffa2163_8ecd_4775_a908_c5eb6af6be45> rdf:type owl:Class ;
                                                                                            rdfs:subClassOf <http://emmo.info/emmo/domain/mechanical-testing#EMMO_c799b443_c70f_4351_bb0f_e4ab29073481> ;
                                                                                            rdfs:comment "Rockwell hardness is a derived quantity that is determined using an apparatus called the Rockwell hardness tester." ;
                                                                                            <http://www.w3.org/2004/02/skos/core#prefLabel> "RockwellCHardness"@en .


###  http://emmo.info/emmo/domain/mechanical-testing#MechanicalTestingOntology
<http://emmo.info/emmo/domain/mechanical-testing#MechanicalTestingOntology> rdf:type owl:Class ;
                                                                            rdfs:comment "This is the root class of the Mechanical Testing Ontology." ;
                                                                            <http://www.w3.org/2004/02/skos/core#prefLabel> "MechanicalTestingOntology"@en .


###  http://emmo.info/emmo/domain/mechanical-testing#NanoindentationUseCase
<http://emmo.info/emmo/domain/mechanical-testing#NanoindentationUseCase> rdf:type owl:Class ;
                                                                         rdfs:subClassOf <http://emmo.info/emmo/domain/mechanical-testing#MechanicalTestingOntology> ;
                                                                         rdfs:comment "This is the artificial parent concept of the classes related to the Nanoindentation Use Case within this ontology." ;
                                                                         <http://www.w3.org/2004/02/skos/core#prefLabel> "NanoindentationUseCase"@en .


###  http://emmo.info/emmo/middle/chemistry#EMMO_0eabfde6_c6c5_4b1f_bf10_e4e0e06e9b2e
<http://emmo.info/emmo/middle/chemistry#EMMO_0eabfde6_c6c5_4b1f_bf10_e4e0e06e9b2e> rdf:type owl:Class ;
                                                                                   rdfs:subClassOf <http://emmo.info/emmo/middle/chemistry#EMMO_7efd64d1_05a1_49cd_a7f0_783ca050d4f3> ;
                                                                                   <http://www.w3.org/2004/02/skos/core#prefLabel> "TotalComposition"@en .


###  http://emmo.info/emmo/middle/chemistry#EMMO_16a3bd5c_75f0_42b3_b000_cb0d018f840e
<http://emmo.info/emmo/middle/chemistry#EMMO_16a3bd5c_75f0_42b3_b000_cb0d018f840e> rdf:type owl:Class ;
                                                                                   rdfs:subClassOf <http://emmo.info/emmo/middle/chemistry#EMMO_26586828_3b8c_4d8b_9c6c_0bc2502f26ae> ,
                                                                                                   <http://emmo.info/emmo/middle/chemistry#EMMO_91a0635a_a89a_46de_8928_04a777d145c7> ;
                                                                                   <http://www.w3.org/2004/02/skos/core#prefLabel> "IUPACName"@en .


###  http://emmo.info/emmo/middle/chemistry#EMMO_172e2c96_180b_40f8_a3e7_b624471f40c2
<http://emmo.info/emmo/middle/chemistry#EMMO_172e2c96_180b_40f8_a3e7_b624471f40c2> rdf:type owl:Class ;
                                                                                   rdfs:subClassOf <http://emmo.info/emmo/middle/chemistry#EMMO_7efd64d1_05a1_49cd_a7f0_783ca050d4f3> ;
                                                                                   <http://www.w3.org/2004/02/skos/core#prefLabel> "SingleComponentComposition"@en .


###  http://emmo.info/emmo/middle/chemistry#EMMO_21205421_5783_4d3e_81e5_10c5d894a88a
<http://emmo.info/emmo/middle/chemistry#EMMO_21205421_5783_4d3e_81e5_10c5d894a88a> rdf:type owl:Class ;
                                                                                   rdfs:subClassOf <http://emmo.info/emmo/middle/chemistry#EMMO_47338839_6cca_4a8e_b565_3c4d5517e2c0> .


###  http://emmo.info/emmo/middle/chemistry#EMMO_26586828_3b8c_4d8b_9c6c_0bc2502f26ae
<http://emmo.info/emmo/middle/chemistry#EMMO_26586828_3b8c_4d8b_9c6c_0bc2502f26ae> rdf:type owl:Class ;
                                                                                   rdfs:subClassOf <http://emmo.info/emmo/middle/chemistry#EMMO_643d99dd_fae6_4121_a76f_47f486a4480b> ;
                                                                                   <http://www.w3.org/2004/02/skos/core#prefLabel> "ChemicalName"@en .


###  http://emmo.info/emmo/middle/chemistry#EMMO_4208f937_8bad_47cf_af46_4ada75e63adb
<http://emmo.info/emmo/middle/chemistry#EMMO_4208f937_8bad_47cf_af46_4ada75e63adb> rdf:type owl:Class ;
                                                                                   rdfs:subClassOf <http://emmo.info/emmo/middle/chemistry#EMMO_9236d0aa_cb39_43a1_bbdd_6a2a714951c8> ;
                                                                                   <http://emmo.info/emmo/middle/chemistry#elucidation> "An expression that provides information about the element types that constiture a molecule or a molecular substance and their number." ;
                                                                                   <http://emmo.info/emmo/middle/chemistry#example> "Hydrogen peroxide is H2O2" ;
                                                                                   <http://www.w3.org/2004/02/skos/core#prefLabel> "MolecularFormula"@en .


###  http://emmo.info/emmo/middle/chemistry#EMMO_436b11bd_1756_4821_9f14_c9ed6b67552e
<http://emmo.info/emmo/middle/chemistry#EMMO_436b11bd_1756_4821_9f14_c9ed6b67552e> rdf:type owl:Class ;
                                                                                   rdfs:subClassOf <http://emmo.info/emmo/middle/chemistry#EMMO_df96cbb6_b5ee_4222_8eab_b3675df24bea> ;
                                                                                   <http://emmo.info/emmo/middle/chemistry#elucidation> "A chemical substance composed of atoms with the same number of protons in the atomic nucleus." ;
                                                                                   <http://emmo.info/emmo/middle/chemistry#iupacDoi> "https://doi.org/10.1351/goldbook.C01022" ;
                                                                                   <http://www.w3.org/2004/02/skos/core#altLabel> "PureSubstance"@en ;
                                                                                   <http://www.w3.org/2004/02/skos/core#prefLabel> "ElementalSubstance" .


###  http://emmo.info/emmo/middle/chemistry#EMMO_47338839_6cca_4a8e_b565_3c4d5517e2c0
<http://emmo.info/emmo/middle/chemistry#EMMO_47338839_6cca_4a8e_b565_3c4d5517e2c0> rdf:type owl:Class ;
                                                                                   rdfs:subClassOf <http://emmo.info/emmo/middle/physicalistic#EMMO_5b2222df_4da6_442f_8244_96e9e45887d1> ;
                                                                                   rdfs:comment """A chemical entity comprises the two different ways to represents matter: as single recognizable particle entity (molecular entity) and as a composition of particle entities (substance).

This distinction is not well assessed in actual chemical nomenclature, in which an element name refers to both the pure elemental substance or the atom.

In the EMMO we force the adoption of a more strict categorization based on mereotopology.

The class Material hosts the subclasses for which a substance can be identified without necessarily considering its nature of molecule/atom or substance (e.g. hydrocarbon is the class of both hydrocarbon molecules or gases).""" ;
                                                                                   <http://www.w3.org/2004/02/skos/core#prefLabel> "ChemicalEntity"@en .


###  http://emmo.info/emmo/middle/chemistry#EMMO_4e659c69_ca2d_4569_8a96_f99857a1fa32
<http://emmo.info/emmo/middle/chemistry#EMMO_4e659c69_ca2d_4569_8a96_f99857a1fa32> rdf:type owl:Class ;
                                                                                   rdfs:subClassOf <http://emmo.info/emmo/middle/chemistry#EMMO_e2b11f6a_4191_427e_9844_2e0ac88dfc8b> ;
                                                                                   <http://www.w3.org/2004/02/skos/core#prefLabel> "InorganicCompound"@en .


###  http://emmo.info/emmo/middle/chemistry#EMMO_4f40def1_3cd7_4067_9596_541e9a5134cf
<http://emmo.info/emmo/middle/chemistry#EMMO_4f40def1_3cd7_4067_9596_541e9a5134cf> rdf:type owl:Class ;
                                                                                   rdfs:subClassOf <http://emmo.info/emmo/middle/chemistry#EMMO_cbcf8fe6_6da6_49e0_ab4d_00f737ea9689> ,
                                                                                                   <http://emmo.info/emmo/middle/chemistry#EMMO_d357e0dd_3497_4590_af6f_7954db7fecf7> ;
                                                                                   <http://emmo.info/emmo/middle/chemistry#elucidation> "The symbol for a specific chemical element, that can stand both for an atom or a substance." ;
                                                                                   <http://emmo.info/emmo/middle/chemistry#iupacDoi> "https://doi.org/10.1351/goldbook.C01022" ;
                                                                                   rdfs:comment """The IUPAC Gold Book defines the a chemical element both as:
- a species of atoms; all atoms with the same number of protons in the atomic nucleus
-  a pure chemical substance composed of atoms with the same number of protons in the atomic nucleus

This qualifies a chemical element as a name and not a matter obejct that can stand for an atom or a substance.""" ;
                                                                                   rdfs:seeAlso "http://publications.iupac.org/ci/2005/2701/ud.html" ;
                                                                                   <http://www.w3.org/2004/02/skos/core#prefLabel> "ChemicalElement"@en .


###  http://emmo.info/emmo/middle/chemistry#EMMO_50967f46_51f9_462a_b1e4_e63365b4a184
<http://emmo.info/emmo/middle/chemistry#EMMO_50967f46_51f9_462a_b1e4_e63365b4a184> rdf:type owl:Class ;
                                                                                   rdfs:subClassOf <http://emmo.info/emmo/middle/materials#EMMO_3397f270_dfc1_4500_8f6f_4d0d85ac5f71> ;
                                                                                   <http://www.w3.org/2004/02/skos/core#prefLabel> "Heteronuclear"@en .


###  http://emmo.info/emmo/middle/chemistry#EMMO_643d99dd_fae6_4121_a76f_47f486a4480b
<http://emmo.info/emmo/middle/chemistry#EMMO_643d99dd_fae6_4121_a76f_47f486a4480b> rdf:type owl:Class ;
                                                                                   rdfs:subClassOf <http://emmo.info/emmo/middle/chemistry#EMMO_cbcf8fe6_6da6_49e0_ab4d_00f737ea9689> ;
                                                                                   <http://emmo.info/emmo/middle/chemistry#elucidation> "A language object following a specific nomenclature rules for defining univocal names of chemical compounds." ;
                                                                                   rdfs:comment "A chemical numenclature should not be confused with the chemical formula." ;
                                                                                   <http://www.w3.org/2004/02/skos/core#prefLabel> "ChemicalNomenclature"@en .


###  http://emmo.info/emmo/middle/chemistry#EMMO_6756e9c2_8b89_40b2_bee7_52cd1dad3395
<http://emmo.info/emmo/middle/chemistry#EMMO_6756e9c2_8b89_40b2_bee7_52cd1dad3395> rdf:type owl:Class ;
                                                                                   rdfs:subClassOf <http://emmo.info/emmo/middle/chemistry#EMMO_4f40def1_3cd7_4067_9596_541e9a5134cf> ;
                                                                                   <http://www.w3.org/2004/02/skos/core#prefLabel> "HydrogenSymbol"@en .


###  http://emmo.info/emmo/middle/chemistry#EMMO_6afdb7e8_2a0b_444d_bde3_8d67d98180c0
<http://emmo.info/emmo/middle/chemistry#EMMO_6afdb7e8_2a0b_444d_bde3_8d67d98180c0> rdf:type owl:Class ;
                                                                                   rdfs:subClassOf <http://emmo.info/emmo/middle/chemistry#EMMO_9236d0aa_cb39_43a1_bbdd_6a2a714951c8> ;
                                                                                   <http://emmo.info/emmo/middle/chemistry#elucidation> "An expression that provide information about the element type of a compound and their relative ratio." ;
                                                                                   <http://emmo.info/emmo/middle/chemistry#example> "Hydrogen peroxide is HO" ;
                                                                                   <http://www.w3.org/2004/02/skos/core#prefLabel> "EmpiricalFormula"@en .


###  http://emmo.info/emmo/middle/chemistry#EMMO_704630b8_fee3_49b9_baca_40e2dd276370
<http://emmo.info/emmo/middle/chemistry#EMMO_704630b8_fee3_49b9_baca_40e2dd276370> rdf:type owl:Class ;
                                                                                   rdfs:subClassOf <http://emmo.info/emmo/middle/chemistry#EMMO_e2b11f6a_4191_427e_9844_2e0ac88dfc8b> ;
                                                                                   <http://www.w3.org/2004/02/skos/core#prefLabel> "OrganicCompound"@en .


###  http://emmo.info/emmo/middle/chemistry#EMMO_7efd64d1_05a1_49cd_a7f0_783ca050d4f3
<http://emmo.info/emmo/middle/chemistry#EMMO_7efd64d1_05a1_49cd_a7f0_783ca050d4f3> rdf:type owl:Class ;
                                                                                   rdfs:subClassOf <http://emmo.info/emmo/middle/chemistry#EMMO_bd8db028_aec2_4a44_ad93_1a9f8270f72c> ,
                                                                                                   <http://emmo.info/emmo/middle/reductionistic#EMMO_36c79456_e29c_400d_8bd3_0eedddb82652> ;
                                                                                   <http://emmo.info/emmo/middle/chemistry#elucidation> "A language construct that provides information about the consitutents of a substance and their fractions or amounts." ;
                                                                                   <http://www.w3.org/2004/02/skos/core#prefLabel> "ChemicalComposition"@en .


###  http://emmo.info/emmo/middle/chemistry#EMMO_844d1ded_2ede_43fd_a3c0_d33f332b2da6
<http://emmo.info/emmo/middle/chemistry#EMMO_844d1ded_2ede_43fd_a3c0_d33f332b2da6> rdf:type owl:Class ;
                                                                                   rdfs:subClassOf <http://emmo.info/emmo/middle/chemistry#EMMO_4f40def1_3cd7_4067_9596_541e9a5134cf> ;
                                                                                   <http://www.w3.org/2004/02/skos/core#prefLabel> "UraniumSymbol"@en .


###  http://emmo.info/emmo/middle/chemistry#EMMO_86f34276_7ab7_4609_94ea_16a15c0bc9fb
<http://emmo.info/emmo/middle/chemistry#EMMO_86f34276_7ab7_4609_94ea_16a15c0bc9fb> rdf:type owl:Class ;
                                                                                   rdfs:subClassOf <http://emmo.info/emmo/middle/chemistry#EMMO_4f40def1_3cd7_4067_9596_541e9a5134cf> ;
                                                                                   <http://www.w3.org/2004/02/skos/core#prefLabel> "ArgonSymbol"@en .


###  http://emmo.info/emmo/middle/chemistry#EMMO_8a41ed1b_64f9_4be7_9b60_01fcece45075
<http://emmo.info/emmo/middle/chemistry#EMMO_8a41ed1b_64f9_4be7_9b60_01fcece45075> rdf:type owl:Class ;
                                                                                   rdfs:subClassOf <http://emmo.info/emmo/middle/physicalistic#EMMO_4207e895_8b83_4318_996a_72cfb32acd94> ;
                                                                                   <http://www.w3.org/2004/02/skos/core#prefLabel> "ChemicalMaterial"@en .


###  http://emmo.info/emmo/middle/chemistry#EMMO_90963312_d9a9_4474_8d10_835aef5b168e
<http://emmo.info/emmo/middle/chemistry#EMMO_90963312_d9a9_4474_8d10_835aef5b168e> rdf:type owl:Class ;
                                                                                   rdfs:subClassOf <http://emmo.info/emmo/middle/chemistry#EMMO_7efd64d1_05a1_49cd_a7f0_783ca050d4f3> ;
                                                                                   <http://www.w3.org/2004/02/skos/core#prefLabel> "PartialComposition"@en .


###  http://emmo.info/emmo/middle/chemistry#EMMO_91a0635a_a89a_46de_8928_04a777d145c7
<http://emmo.info/emmo/middle/chemistry#EMMO_91a0635a_a89a_46de_8928_04a777d145c7> rdf:type owl:Class ;
                                                                                   rdfs:subClassOf <http://emmo.info/emmo/middle/chemistry#EMMO_643d99dd_fae6_4121_a76f_47f486a4480b> ;
                                                                                   <http://www.w3.org/2004/02/skos/core#prefLabel> "IUPACNomencalture"@en .


###  http://emmo.info/emmo/middle/chemistry#EMMO_9236d0aa_cb39_43a1_bbdd_6a2a714951c8
<http://emmo.info/emmo/middle/chemistry#EMMO_9236d0aa_cb39_43a1_bbdd_6a2a714951c8> rdf:type owl:Class ;
                                                                                   rdfs:subClassOf <http://emmo.info/emmo/middle/chemistry#EMMO_cbcf8fe6_6da6_49e0_ab4d_00f737ea9689> ,
                                                                                                   <http://emmo.info/emmo/middle/reductionistic#EMMO_36c79456_e29c_400d_8bd3_0eedddb82652> ;
                                                                                   <http://emmo.info/emmo/middle/chemistry#elucidation> "A symbolic construct that provides informations about the chemical proportions of the elements that constitute a chemical compound or a specific molecule." ;
                                                                                   rdfs:comment "A chemical formula may also include other symbols such as parentheses, plus and minus signs, brackets" ;
                                                                                   <http://www.w3.org/2004/02/skos/core#prefLabel> "ChemicalFormula"@en .


###  http://emmo.info/emmo/middle/chemistry#EMMO_9fa966c7_5231_409e_841f_b4c5fd33732a
<http://emmo.info/emmo/middle/chemistry#EMMO_9fa966c7_5231_409e_841f_b4c5fd33732a> rdf:type owl:Class ;
                                                                                   rdfs:subClassOf <http://emmo.info/emmo/middle/materials#EMMO_21205421_5783_4d3e_81e5_10c5d894a88a> ;
                                                                                   <http://www.w3.org/2004/02/skos/core#prefLabel> "PolyatomicEntity"@en .


###  http://emmo.info/emmo/middle/chemistry#EMMO_a086af15_a7c3_404c_b4ce_c8e4466f1b4b
<http://emmo.info/emmo/middle/chemistry#EMMO_a086af15_a7c3_404c_b4ce_c8e4466f1b4b> rdf:type owl:Class ;
                                                                                   rdfs:subClassOf <http://emmo.info/emmo/middle/chemistry#EMMO_8a41ed1b_64f9_4be7_9b60_01fcece45075> ;
                                                                                   <http://www.w3.org/2004/02/skos/core#prefLabel> "ElementalMaterial"@en .


###  http://emmo.info/emmo/middle/chemistry#EMMO_a14dd591_8b7a_4847_8c91_3a2f421a45b4
<http://emmo.info/emmo/middle/chemistry#EMMO_a14dd591_8b7a_4847_8c91_3a2f421a45b4> rdf:type owl:Class ;
                                                                                   rdfs:subClassOf <http://emmo.info/emmo/middle/chemistry#EMMO_9fa966c7_5231_409e_841f_b4c5fd33732a> ;
                                                                                   <http://www.w3.org/2004/02/skos/core#prefLabel> "Macromolecule"@en .


###  http://emmo.info/emmo/middle/chemistry#EMMO_a293f923_954c_4af5_9f97_9600ebd362cb
<http://emmo.info/emmo/middle/chemistry#EMMO_a293f923_954c_4af5_9f97_9600ebd362cb> rdf:type owl:Class ;
                                                                                   rdfs:subClassOf <http://emmo.info/emmo/middle/metrology#EMMO_daf05011_df3f_44a0_bb31_f8d565d7a854> ;
                                                                                   <http://www.w3.org/2004/02/skos/core#prefLabel> "ChemicalCompositionQuantity"@en .


###  http://emmo.info/emmo/middle/chemistry#EMMO_a466b60b_d973_4b8f_897f_d0b837a59df3
<http://emmo.info/emmo/middle/chemistry#EMMO_a466b60b_d973_4b8f_897f_d0b837a59df3> rdf:type owl:Class ;
                                                                                   rdfs:subClassOf <http://emmo.info/emmo/middle/chemistry#EMMO_ecc4efe9_77a2_47e3_8190_f9a883d54ac6> ;
                                                                                   <http://emmo.info/emmo/middle/chemistry#elucidation> "A graphical representation of a molecular structure showing the relative position in space of the atomic constituents and their bonds." ;
                                                                                   <http://www.w3.org/2004/02/skos/core#prefLabel> "StructuralFormula"@en .


###  http://emmo.info/emmo/middle/chemistry#EMMO_abf7efbe_6b04_41b8_8326_4dd0f6be753e
<http://emmo.info/emmo/middle/chemistry#EMMO_abf7efbe_6b04_41b8_8326_4dd0f6be753e> rdf:type owl:Class ;
                                                                                   rdfs:subClassOf <http://emmo.info/emmo/middle/perceptual#EMMO_d8d2144e_5c8d_455d_a643_5caf4d8d9df8> ;
                                                                                   <http://emmo.info/emmo/middle/chemistry#elucidation> "A language object that follows the syntactic rules used in the chemical field." ;
                                                                                   <http://www.w3.org/2004/02/skos/core#prefLabel> "Chemical"@en .


###  http://emmo.info/emmo/middle/chemistry#EMMO_bd8db028_aec2_4a44_ad93_1a9f8270f72c
<http://emmo.info/emmo/middle/chemistry#EMMO_bd8db028_aec2_4a44_ad93_1a9f8270f72c> rdf:type owl:Class ;
                                                                                   rdfs:subClassOf <http://emmo.info/emmo/middle/chemistry#EMMO_abf7efbe_6b04_41b8_8326_4dd0f6be753e> ,
                                                                                                   <http://emmo.info/emmo/middle/perceptual#EMMO_89a0c87c_0804_4013_937a_6fe234d9499c> ;
                                                                                   <http://www.w3.org/2004/02/skos/core#prefLabel> "ChemicalSymbolicConstruct"@en .


###  http://emmo.info/emmo/middle/chemistry#EMMO_bf836c2b_7800_474d_b674_f5d629fa0bb1
<http://emmo.info/emmo/middle/chemistry#EMMO_bf836c2b_7800_474d_b674_f5d629fa0bb1> rdf:type owl:Class ;
                                                                                   rdfs:subClassOf <http://emmo.info/emmo/middle/chemistry#EMMO_9236d0aa_cb39_43a1_bbdd_6a2a714951c8> ;
                                                                                   <http://emmo.info/emmo/middle/chemistry#example> "An expression that provides information about the element types that constiture a molecule or a molecular substance and their number, together with simple information about the connectivity of its groups by using parenthesis or by goruping element names according to its molecular structure." ;
                                                                                   <http://www.w3.org/2004/02/skos/core#prefLabel> "CondensedFormula"@en .


###  http://emmo.info/emmo/middle/chemistry#EMMO_cbcf8fe6_6da6_49e0_ab4d_00f737ea9689
<http://emmo.info/emmo/middle/chemistry#EMMO_cbcf8fe6_6da6_49e0_ab4d_00f737ea9689> rdf:type owl:Class ;
                                                                                   rdfs:subClassOf <http://emmo.info/emmo/middle/chemistry#EMMO_abf7efbe_6b04_41b8_8326_4dd0f6be753e> ;
                                                                                   <http://emmo.info/emmo/middle/chemistry#elucidation> """Specific form of an element defined as to isotopic composition, electronic or oxidation state, and/or complex or molecular structure.

Chemical species is the macroscopic equivalent of molecular entity and refers to sets or ensembles of molecular entities.""" ;
                                                                                   <http://emmo.info/emmo/middle/chemistry#iupacDoi> "https://doi.org/10.1351/goldbook.CT06859" ;
                                                                                   rdfs:comment """Following nominalistic approach a species is simply a name that can point to an element name, a chemical formula or a chemical compound.

So everything addressed by these classes of names can be calleded a chemical species.""" ,
                                                                                                """N2
Methane
CH4
Fe
Sodium Chloride""" ;
                                                                                   <http://www.w3.org/2004/02/skos/core#prefLabel> "ChemicalSpecies"@en .


###  http://emmo.info/emmo/middle/chemistry#EMMO_d2a47cd8_662f_438f_855a_b4378eb992ff
<http://emmo.info/emmo/middle/chemistry#EMMO_d2a47cd8_662f_438f_855a_b4378eb992ff> rdf:type owl:Class ;
                                                                                   rdfs:subClassOf <http://emmo.info/emmo/middle/chemistry#EMMO_643d99dd_fae6_4121_a76f_47f486a4480b> ;
                                                                                   <http://emmo.info/emmo/middle/chemistry#elucidation> "Chemical Abstact Service registry number for a chemical substance from the American Chemical Society" ;
                                                                                   <http://emmo.info/emmo/middle/chemistry#example> "Water is 7732-18-5" ;
                                                                                   <http://www.w3.org/2004/02/skos/core#prefLabel> "CASRN"@en .


###  http://emmo.info/emmo/middle/chemistry#EMMO_d357e0dd_3497_4590_af6f_7954db7fecf7
<http://emmo.info/emmo/middle/chemistry#EMMO_d357e0dd_3497_4590_af6f_7954db7fecf7> rdf:type owl:Class ;
                                                                                   rdfs:subClassOf <http://emmo.info/emmo/middle/chemistry#EMMO_abf7efbe_6b04_41b8_8326_4dd0f6be753e> ,
                                                                                                   <http://emmo.info/emmo/middle/perceptual#EMMO_a1083d0a_c1fb_471f_8e20_a98f881ad527> ;
                                                                                   <http://www.w3.org/2004/02/skos/core#prefLabel> "ChemicalSymbol"@en .


###  http://emmo.info/emmo/middle/chemistry#EMMO_d74ed682_894f_46c5_87cb_167f60926965
<http://emmo.info/emmo/middle/chemistry#EMMO_d74ed682_894f_46c5_87cb_167f60926965> rdf:type owl:Class ;
                                                                                   rdfs:subClassOf <http://emmo.info/emmo/middle/chemistry#EMMO_91a0635a_a89a_46de_8928_04a777d145c7> ;
                                                                                   <http://emmo.info/emmo/middle/chemistry#elucidation> "The International Chemical Identifier (InChI) textual identifier proposed by IUPAC to provide a standard encoding for databases of molecular information." ;
                                                                                   <http://www.w3.org/2004/02/skos/core#prefLabel> "InChI"@en .


###  http://emmo.info/emmo/middle/chemistry#EMMO_df96cbb6_b5ee_4222_8eab_b3675df24bea
<http://emmo.info/emmo/middle/chemistry#EMMO_df96cbb6_b5ee_4222_8eab_b3675df24bea> rdf:type owl:Class ;
                                                                                   rdfs:subClassOf <http://emmo.info/emmo/middle/chemistry#EMMO_47338839_6cca_4a8e_b565_3c4d5517e2c0> ;
                                                                                   <http://emmo.info/emmo/middle/chemistry#elucidation> "Matter of constant composition best characterized by the entities (molecules, formula units, atoms) it is composed of." ;
                                                                                   <http://emmo.info/emmo/middle/chemistry#iupacDoi> "https://doi.org/10.1351/goldbook.C01039" ;
                                                                                   rdfs:comment "A substance is always composed of more than one molecular entity. It lays in the continuum or mesoscopic domain." ;
                                                                                   <http://www.w3.org/2004/02/skos/core#prefLabel> "ChemicalSubstance"@en .


###  http://emmo.info/emmo/middle/chemistry#EMMO_e024544d_e374_45b7_9340_1982040bc6b7
<http://emmo.info/emmo/middle/chemistry#EMMO_e024544d_e374_45b7_9340_1982040bc6b7> rdf:type owl:Class ;
                                                                                   rdfs:subClassOf <http://emmo.info/emmo/middle/materials#EMMO_3397f270_dfc1_4500_8f6f_4d0d85ac5f71> ;
                                                                                   <http://www.w3.org/2004/02/skos/core#altLabel> "ElementalMolecule" ;
                                                                                   <http://www.w3.org/2004/02/skos/core#prefLabel> "Homonuclear"@en .


###  http://emmo.info/emmo/middle/chemistry#EMMO_e2b11f6a_4191_427e_9844_2e0ac88dfc8b
<http://emmo.info/emmo/middle/chemistry#EMMO_e2b11f6a_4191_427e_9844_2e0ac88dfc8b> rdf:type owl:Class ;
                                                                                   rdfs:subClassOf <http://emmo.info/emmo/middle/chemistry#EMMO_df96cbb6_b5ee_4222_8eab_b3675df24bea> ;
                                                                                   <http://emmo.info/emmo/middle/chemistry#elucidation> "A chemical substance composed of many identical molecules (or molecular entities) composed of atoms from more than one element held together by chemical bonds." ;
                                                                                   <http://emmo.info/emmo/middle/chemistry#wikipediaEntry> "https://en.wikipedia.org/wiki/Chemical_compound" ;
                                                                                   <http://www.w3.org/2004/02/skos/core#prefLabel> "ChemicalCompound"@en .


###  http://emmo.info/emmo/middle/chemistry#EMMO_eb7de1a1_c30e_4f0d_94c6_fe70414d7e61
<http://emmo.info/emmo/middle/chemistry#EMMO_eb7de1a1_c30e_4f0d_94c6_fe70414d7e61> rdf:type owl:Class ;
                                                                                   rdfs:subClassOf <http://emmo.info/emmo/middle/perceptual#EMMO_c74da218_9147_4f03_92d1_8894abca55f3> ;
                                                                                   <http://emmo.info/emmo/middle/chemistry#elucidation> "A graphical object aimed to represent schematically the conceptual, tempral or spatial structure of another object." ;
                                                                                   <http://www.w3.org/2004/02/skos/core#prefLabel> "Representation"@en .


###  http://emmo.info/emmo/middle/chemistry#EMMO_ecc4efe9_77a2_47e3_8190_f9a883d54ac6
<http://emmo.info/emmo/middle/chemistry#EMMO_ecc4efe9_77a2_47e3_8190_f9a883d54ac6> rdf:type owl:Class ;
                                                                                   rdfs:subClassOf <http://emmo.info/emmo/middle/chemistry#EMMO_eb7de1a1_c30e_4f0d_94c6_fe70414d7e61> ;
                                                                                   <http://emmo.info/emmo/middle/chemistry#elucidation> "A representation of objects belonging to the chemistry field." ;
                                                                                   <http://www.w3.org/2004/02/skos/core#prefLabel> "ChemicalRepresentation"@en .


###  http://emmo.info/emmo/middle/holistic#EMMO_0277f24a_ea7f_4917_81b7_fb0406c8fc62
<http://emmo.info/emmo/middle/holistic#EMMO_0277f24a_ea7f_4917_81b7_fb0406c8fc62> rdf:type owl:Class ;
                                                                                  rdfs:subClassOf <http://emmo.info/emmo/top#EMMO_49267eba_5548_4163_8f36_518d65b583f9> ;
                                                                                  <http://emmo.info/emmo/top/annotations#EMMO_967080e5_2f42_4eb2_a3a9_c58143e835f9> "A union of classes that categorize physicals under a holistic perspective: the interest is on the whole 4D object (process) and the role of its 4D parts (participants) without going further into specifying the spatial hierarchy or the temporal position of each part."@en ;
                                                                                  rdfs:comment """An holistic perspective considers each part of the whole as equally important, without the need of a granularity hierarchy (in time or space).

A molecule of a body can have role in the body evolution, without caring if its part of a specific organ and without specifying the time interval in which this role occurred.

This class allows the picking of parts without necessarily going trough a rigid hierarchy of spatial compositions (e.g. body -> organ -> cell -> molecule) or temporal composition."""@en ,
                                                                                               "Holism (from Greek ???? holos \"all, whole, entire\")"@en ;
                                                                                  <http://www.w3.org/2004/02/skos/core#prefLabel> "Holistic"@en .


###  http://emmo.info/emmo/middle/holistic#EMMO_43e9a05d_98af_41b4_92f6_00f79a09bfce
<http://emmo.info/emmo/middle/holistic#EMMO_43e9a05d_98af_41b4_92f6_00f79a09bfce> rdf:type owl:Class ;
                                                                                  rdfs:subClassOf <http://emmo.info/emmo/middle/holistic#EMMO_0277f24a_ea7f_4917_81b7_fb0406c8fc62> ;
                                                                                  <http://emmo.info/emmo/top/annotations#EMMO_967080e5_2f42_4eb2_a3a9_c58143e835f9> "A temporal part of a physical that identifies a particular type of evolution in time."@en ;
                                                                                  rdfs:comment "A 'Process' is always a 'Physical', since a 'Void' does not have elements that evolves in time."@en ,
                                                                                               """Following the common definition of process, the reader may think that every 'Physical' should be a process, since every 4D object always has a time dimension. 

However, in the EMMO we restrict the meaning of the word process to 'Physical'-s whose evolution in time have a particular meaning for the ontologist (i.e. every 4D object unfolds in time, but not every 4D object may be of interest for the ontologist). 

A 'Process' is not only something that unfolds in time (which is automatically represented in a 4D ontology), but something that has a meaning for the ontologist (i.e. that the ontologist can separate from the rest of the 4D physical for any reason)."""@en ;
                                                                                  <http://www.w3.org/2004/02/skos/core#prefLabel> "Process"@en .


###  http://emmo.info/emmo/middle/holistic#EMMO_49804605_c0fe_4538_abda_f70ba1dc8a5d
<http://emmo.info/emmo/middle/holistic#EMMO_49804605_c0fe_4538_abda_f70ba1dc8a5d> rdf:type owl:Class ;
                                                                                  rdfs:subClassOf <http://emmo.info/emmo/middle/holistic#EMMO_0277f24a_ea7f_4917_81b7_fb0406c8fc62> ;
                                                                                  <http://emmo.info/emmo/top/annotations#EMMO_967080e5_2f42_4eb2_a3a9_c58143e835f9> "A portion of a 'Process' that participates to the process with a specific role."@en ;
                                                                                  rdfs:comment """In the EMMO the relation of participation to a process falls under mereotopology.

Since topological connection means causality, then the only way for a real world object to participate to a process is to be a part of it."""@en ;
                                                                                  <http://www.w3.org/2004/02/skos/core#prefLabel> "Participant"@en .


###  http://emmo.info/emmo/middle/isq#EMMO_02e894c3_b793_4197_b120_3442e08f58d1
<http://emmo.info/emmo/middle/isq#EMMO_02e894c3_b793_4197_b120_3442e08f58d1> rdf:type owl:Class ;
                                                                             rdfs:subClassOf <http://emmo.info/emmo/middle/metrology#EMMO_9895a1b4_f0a5_4167_ac5e_97db40b8bfcc> ;
                                                                             <http://www.w3.org/2004/02/skos/core#prefLabel> "TimeDimension"@en .


###  http://emmo.info/emmo/middle/isq#EMMO_0329f1f5_8339_4ce4_8505_a264c6d606ba
<http://emmo.info/emmo/middle/isq#EMMO_0329f1f5_8339_4ce4_8505_a264c6d606ba> rdf:type owl:Class ;
                                                                             rdfs:subClassOf <http://emmo.info/emmo/middle/isq#EMMO_81369540_1b0e_471b_9bae_6801af22800e> ;
                                                                             <http://emmo.info/emmo/middle/isq#EMMO_de178b12_5d35_4bca_8efa_a4193162571d> "T-1 L+1 M0 I0 T0 N0 J0" ;
                                                                             <http://emmo.info/emmo/top/annotations#EMMO_1f1b164d_ec6a_4faa_8d5e_88bda62316cc> "http://qudt.org/vocab/quantitykind/Velocity" ;
                                                                             <http://emmo.info/emmo/top/annotations#EMMO_50c298c2_55a2_4068_b3ac_4e948c33181f> "http://www.electropedia.org/iev/iev.nsf/display?openform&ievref=113-01-32" ;
                                                                             <http://emmo.info/emmo/top/annotations#EMMO_70fe84ff_99b6_4206_a9fc_9a8931836d84> """Vector quantity giving the rate of change of a position vector.

-- ISO 80000-3"""@en ;
                                                                             <http://emmo.info/emmo/top/annotations#EMMO_8de5d5bf_db1c_40ac_b698_095ba3b18578> "3-10.1" ;
                                                                             rdfs:comment """The velocity depends on the choice of the reference frame. Proper transformation between frames must be used: Galilean for non-relativistic description, Lorentzian for relativistic description.

-- IEC, note 2"""@en ,
                                                                                          """The velocity is related to a point described by its position vector. The point may localize a particle, or be attached to any other object such as a body or a wave.

-- IEC, note 1"""@en ;
                                                                             <http://www.w3.org/2004/02/skos/core#prefLabel> "Velocity"@en .


###  http://emmo.info/emmo/middle/isq#EMMO_04b3300c_98bd_42dc_a3b5_e6c29d69f1ac
<http://emmo.info/emmo/middle/isq#EMMO_04b3300c_98bd_42dc_a3b5_e6c29d69f1ac> rdf:type owl:Class ;
                                                                             rdfs:subClassOf <http://emmo.info/emmo/middle/chemistry#EMMO_a293f923_954c_4af5_9f97_9600ebd362cb> ,
                                                                                             <http://emmo.info/emmo/middle/isq#EMMO_faab3f84_e475_4a46_af9c_7d249f0b9aef> ;
                                                                             <http://emmo.info/emmo/middle/isq#EMMO_de178b12_5d35_4bca_8efa_a4193162571d> "T0 L0 M0 I0 T0 N0 J0" ;
                                                                             <http://emmo.info/emmo/top/annotations#EMMO_1f1b164d_ec6a_4faa_8d5e_88bda62316cc> "http://qudt.org/vocab/quantitykind/MoleFraction" ;
                                                                             <http://emmo.info/emmo/top/annotations#EMMO_6dd685dd_1895_46e4_b227_be9f7d643c25> "http://dbpedia.org/page/Mole_fraction" ;
                                                                             <http://emmo.info/emmo/top/annotations#EMMO_70fe84ff_99b6_4206_a9fc_9a8931836d84> "The amount of a constituent divided by the total amount of all constituents in a mixture."@en ;
                                                                             <http://emmo.info/emmo/top/annotations#EMMO_e55f2d7c_9893_48cd_b4a4_fdf38253bd20> "http://www.ontology-of-units-of-measure.org/resource/om-2/AmountOfSubstanceFraction" ;
                                                                             <http://emmo.info/emmo/top/annotations#EMMO_fe015383_afb3_44a6_ae86_043628697aa2> "https://doi.org/10.1351/goldbook.A00296" ;
                                                                             <http://www.w3.org/2004/02/skos/core#altLabel> "MoleFraction"@en ;
                                                                             <http://www.w3.org/2004/02/skos/core#prefLabel> "AmountFraction"@en .


###  http://emmo.info/emmo/middle/isq#EMMO_04cc9451_5306_45d0_8554_22cee4d6e785
<http://emmo.info/emmo/middle/isq#EMMO_04cc9451_5306_45d0_8554_22cee4d6e785> rdf:type owl:Class ;
                                                                             rdfs:subClassOf <http://emmo.info/emmo/middle/isq#EMMO_2946d40b_24a1_47fa_8176_e3f79bb45064> ;
                                                                             <http://emmo.info/emmo/middle/isq#EMMO_de178b12_5d35_4bca_8efa_a4193162571d> "T-2 L+2 M+1 I-2 T0 N0 J0" ;
                                                                             <http://emmo.info/emmo/top/annotations#EMMO_1f1b164d_ec6a_4faa_8d5e_88bda62316cc> "http://qudt.org/vocab/quantitykind/Inductance" ;
                                                                             <http://emmo.info/emmo/top/annotations#EMMO_6dd685dd_1895_46e4_b227_be9f7d643c25> "http://dbpedia.org/page/Inductance" ;
                                                                             <http://emmo.info/emmo/top/annotations#EMMO_967080e5_2f42_4eb2_a3a9_c58143e835f9> "A property of an electrical conductor by which a change in current through it induces an electromotive force in both the conductor itself and in any nearby conductors by mutual inductance."@en ;
                                                                             <http://emmo.info/emmo/top/annotations#EMMO_fe015383_afb3_44a6_ae86_043628697aa2> "https://doi.org/10.1351/goldbook.M04076" ;
                                                                             <http://www.w3.org/2004/02/skos/core#altLabel> "Inductance"@en ;
                                                                             <http://www.w3.org/2004/02/skos/core#prefLabel> "ElectricInductance"@en .


###  http://emmo.info/emmo/middle/isq#EMMO_04cf0295_3e8f_4693_a87f_3130d125cf05
<http://emmo.info/emmo/middle/isq#EMMO_04cf0295_3e8f_4693_a87f_3130d125cf05> rdf:type owl:Class ;
                                                                             rdfs:subClassOf <http://emmo.info/emmo/middle/isq#EMMO_1f087811_06cb_42d5_90fb_25d0e7e068ef> ;
                                                                             <http://emmo.info/emmo/middle/isq#EMMO_de178b12_5d35_4bca_8efa_a4193162571d> "T-2 L+1 M+1 I0 T0 N0 J0" ;
                                                                             <http://emmo.info/emmo/top/annotations#EMMO_1f1b164d_ec6a_4faa_8d5e_88bda62316cc> "http://qudt.org/vocab/quantitykind/Weight" ;
                                                                             <http://emmo.info/emmo/top/annotations#EMMO_6dd685dd_1895_46e4_b227_be9f7d643c25> "http://dbpedia.org/page/Weight" ;
                                                                             <http://emmo.info/emmo/top/annotations#EMMO_fe015383_afb3_44a6_ae86_043628697aa2> "https://doi.org/10.1351/goldbook.W06668" ;
                                                                             rdfs:comment "Force of gravity acting on a body."@en ;
                                                                             <http://www.w3.org/2004/02/skos/core#prefLabel> "Weight"@en .


###  http://emmo.info/emmo/middle/isq#EMMO_06448f64_8db6_4304_8b2c_e785dba82044
<http://emmo.info/emmo/middle/isq#EMMO_06448f64_8db6_4304_8b2c_e785dba82044> rdf:type owl:Class ;
                                                                             rdfs:subClassOf <http://emmo.info/emmo/middle/isq#EMMO_2946d40b_24a1_47fa_8176_e3f79bb45064> ;
                                                                             <http://emmo.info/emmo/middle/isq#EMMO_de178b12_5d35_4bca_8efa_a4193162571d> "T0 L-3 M+1 I0 T0 N0 J0" ;
                                                                             <http://emmo.info/emmo/top/annotations#EMMO_1f1b164d_ec6a_4faa_8d5e_88bda62316cc> "http://qudt.org/vocab/quantitykind/Density" ;
                                                                             <http://emmo.info/emmo/top/annotations#EMMO_6dd685dd_1895_46e4_b227_be9f7d643c25> "http://dbpedia.org/page/Density" ;
                                                                             <http://emmo.info/emmo/top/annotations#EMMO_fe015383_afb3_44a6_ae86_043628697aa2> "https://doi.org/10.1351/goldbook.D01590" ;
                                                                             rdfs:comment "Mass per volume."@en ;
                                                                             <http://www.w3.org/2004/02/skos/core#prefLabel> "Density"@en .


###  http://emmo.info/emmo/middle/isq#EMMO_07de47e0_6bb6_45b9_b55a_4f238efbb105
<http://emmo.info/emmo/middle/isq#EMMO_07de47e0_6bb6_45b9_b55a_4f238efbb105> rdf:type owl:Class ;
                                                                             rdfs:subClassOf <http://emmo.info/emmo/middle/isq#EMMO_ba882f34_0d71_4e4f_9d92_0c076c633a2c> ;
                                                                             <http://emmo.info/emmo/middle/isq#EMMO_de178b12_5d35_4bca_8efa_a4193162571d> "T0 L0 M0 I0 T0 N0 J0" ;
                                                                             <http://emmo.info/emmo/top/annotations#EMMO_1f1b164d_ec6a_4faa_8d5e_88bda62316cc> "http://qudt.org/vocab/quantitykind/AtomicNumber" ;
                                                                             <http://emmo.info/emmo/top/annotations#EMMO_6dd685dd_1895_46e4_b227_be9f7d643c25> "http://dbpedia.org/page/Atomic_number" ;
                                                                             <http://emmo.info/emmo/top/annotations#EMMO_70fe84ff_99b6_4206_a9fc_9a8931836d84> "Number of protons in an atomic nucleus."@en ;
                                                                             <http://emmo.info/emmo/top/annotations#EMMO_fe015383_afb3_44a6_ae86_043628697aa2> "https://doi.org/10.1351/goldbook.A00499" ;
                                                                             <http://www.w3.org/2004/02/skos/core#prefLabel> "AtomicNumber"@en .


###  http://emmo.info/emmo/middle/isq#EMMO_09663630_1b84_4202_91e6_e641104f579e
<http://emmo.info/emmo/middle/isq#EMMO_09663630_1b84_4202_91e6_e641104f579e> rdf:type owl:Class ;
                                                                             rdfs:subClassOf <http://emmo.info/emmo/middle/isq#EMMO_2946d40b_24a1_47fa_8176_e3f79bb45064> ;
                                                                             <http://emmo.info/emmo/middle/isq#EMMO_de178b12_5d35_4bca_8efa_a4193162571d> "T-2 L+1 M+1 I-2 T0 N0 J0" ;
                                                                             <http://emmo.info/emmo/top/annotations#EMMO_1f1b164d_ec6a_4faa_8d5e_88bda62316cc> "http://qudt.org/vocab/quantitykind/ElectromagneticPermeability" ;
                                                                             <http://emmo.info/emmo/top/annotations#EMMO_6dd685dd_1895_46e4_b227_be9f7d643c25> "http://dbpedia.org/page/Permeability_(electromagnetism)" ;
                                                                             <http://emmo.info/emmo/top/annotations#EMMO_fe015383_afb3_44a6_ae86_043628697aa2> "https://doi.org/10.1351/goldbook.P04503" ;
                                                                             rdfs:comment "Measure for how the magnetization of material is affected by the application of an external magnetic field ."@en ;
                                                                             <http://www.w3.org/2004/02/skos/core#altLabel> "ElectromagneticPermeability" ;
                                                                             <http://www.w3.org/2004/02/skos/core#prefLabel> "Permeability"@en .


###  http://emmo.info/emmo/middle/isq#EMMO_09b9021b_f97b_43eb_b83d_0a764b472bc2
<http://emmo.info/emmo/middle/isq#EMMO_09b9021b_f97b_43eb_b83d_0a764b472bc2> rdf:type owl:Class ;
                                                                             rdfs:subClassOf <http://emmo.info/emmo/middle/isq#EMMO_2946d40b_24a1_47fa_8176_e3f79bb45064> ;
                                                                             <http://emmo.info/emmo/middle/isq#EMMO_de178b12_5d35_4bca_8efa_a4193162571d> "T-3 L+2 M+1 I0 T0 N0 J0" ;
                                                                             <http://emmo.info/emmo/top/annotations#EMMO_1f1b164d_ec6a_4faa_8d5e_88bda62316cc> "http://qudt.org/vocab/quantitykind/Power" ;
                                                                             <http://emmo.info/emmo/top/annotations#EMMO_6dd685dd_1895_46e4_b227_be9f7d643c25> "http://dbpedia.org/page/Power_(physics)" ;
                                                                             <http://emmo.info/emmo/top/annotations#EMMO_967080e5_2f42_4eb2_a3a9_c58143e835f9> "Rate of transfer of energy per unit time."@en ;
                                                                             <http://emmo.info/emmo/top/annotations#EMMO_fe015383_afb3_44a6_ae86_043628697aa2> "https://doi.org/10.1351/goldbook.P04792" ;
                                                                             <http://www.w3.org/2004/02/skos/core#prefLabel> "Power"@en .


###  http://emmo.info/emmo/middle/isq#EMMO_0a88be81_343d_4388_92c1_09228ff95ada
<http://emmo.info/emmo/middle/isq#EMMO_0a88be81_343d_4388_92c1_09228ff95ada> rdf:type owl:Class ;
                                                                             rdfs:subClassOf <http://emmo.info/emmo/middle/isq#EMMO_faab3f84_e475_4a46_af9c_7d249f0b9aef> ;
                                                                             <http://emmo.info/emmo/middle/isq#EMMO_de178b12_5d35_4bca_8efa_a4193162571d> "T0 L0 M0 I0 T0 N0 J0" ;
                                                                             <http://emmo.info/emmo/top/annotations#EMMO_967080e5_2f42_4eb2_a3a9_c58143e835f9> "Probability is a dimensionless quantity that can attain values between 0 and 1; zero denotes the impossible event and 1 denotes a certain event."@en ;
                                                                             <http://emmo.info/emmo/top/annotations#EMMO_fe015383_afb3_44a6_ae86_043628697aa2> "https://doi.org/10.1351/goldbook.P04855" ;
                                                                             rdfs:comment "The propability for a certain outcome, is the ratio between the number of events leading to the given outcome and the total number of events."@en ;
                                                                             <http://www.w3.org/2004/02/skos/core#prefLabel> "Probability"@en .


###  http://emmo.info/emmo/middle/isq#EMMO_0ee5779e_d798_4ee5_9bfe_c392d5bea112
<http://emmo.info/emmo/middle/isq#EMMO_0ee5779e_d798_4ee5_9bfe_c392d5bea112> rdf:type owl:Class ;
                                                                             rdfs:subClassOf <http://emmo.info/emmo/middle/isq#EMMO_2946d40b_24a1_47fa_8176_e3f79bb45064> ;
                                                                             <http://emmo.info/emmo/middle/isq#EMMO_de178b12_5d35_4bca_8efa_a4193162571d> "T+4 L-3 M-1 I+2 T0 N0 J0" ;
                                                                             <http://emmo.info/emmo/top/annotations#EMMO_1f1b164d_ec6a_4faa_8d5e_88bda62316cc> "http://qudt.org/vocab/quantitykind/Permittivity" ;
                                                                             <http://emmo.info/emmo/top/annotations#EMMO_6dd685dd_1895_46e4_b227_be9f7d643c25> "http://dbpedia.org/page/Permittivity" ;
                                                                             <http://emmo.info/emmo/top/annotations#EMMO_e55f2d7c_9893_48cd_b4a4_fdf38253bd20> "http://www.ontology-of-units-of-measure.org/resource/om-2/Permittivity" ;
                                                                             <http://emmo.info/emmo/top/annotations#EMMO_fe015383_afb3_44a6_ae86_043628697aa2> "https://doi.org/10.1351/goldbook.P04507" ;
                                                                             rdfs:comment "Measure for how the polarization of a material is affected by the application of an external electric field."@en ;
                                                                             <http://www.w3.org/2004/02/skos/core#prefLabel> "Permittivity"@en .


###  http://emmo.info/emmo/middle/isq#EMMO_12d4ba9b_2f89_4ea3_b206_cd376f96c875
<http://emmo.info/emmo/middle/isq#EMMO_12d4ba9b_2f89_4ea3_b206_cd376f96c875> rdf:type owl:Class ;
                                                                             rdfs:subClassOf <http://emmo.info/emmo/middle/isq#EMMO_31ec09ba_1713_42cb_83c7_b38bf6f9ced2> ;
                                                                             <http://emmo.info/emmo/middle/isq#EMMO_de178b12_5d35_4bca_8efa_a4193162571d> "T-2 L+2 M+1 I0 T0 N0 J0" ;
                                                                             <http://emmo.info/emmo/top/annotations#EMMO_1f1b164d_ec6a_4faa_8d5e_88bda62316cc> "http://qudt.org/vocab/quantitykind/Heat" ;
                                                                             <http://emmo.info/emmo/top/annotations#EMMO_fe015383_afb3_44a6_ae86_043628697aa2> "https://doi.org/10.1351/goldbook.H02752" ;
                                                                             rdfs:comment "Heat is energy in transfer to or from a thermodynamic system, by mechanisms other than thermodynamic work or transfer of matter."@en ;
                                                                             <http://www.w3.org/2004/02/skos/core#prefLabel> "Heat"@en .


###  http://emmo.info/emmo/middle/isq#EMMO_14ff4393_0f28_4fb4_abc7_c2cc00bc761d
<http://emmo.info/emmo/middle/isq#EMMO_14ff4393_0f28_4fb4_abc7_c2cc00bc761d> rdf:type owl:Class ;
                                                                             rdfs:subClassOf <http://emmo.info/emmo/middle/metrology#EMMO_9895a1b4_f0a5_4167_ac5e_97db40b8bfcc> ;
                                                                             <http://www.w3.org/2004/02/skos/core#prefLabel> "LuminousIntensityDimension"@en .


###  http://emmo.info/emmo/middle/isq#EMMO_1604f495_328a_4f28_9962_f4cc210739dd
<http://emmo.info/emmo/middle/isq#EMMO_1604f495_328a_4f28_9962_f4cc210739dd> rdf:type owl:Class ;
                                                                             rdfs:subClassOf <http://emmo.info/emmo/middle/isq#EMMO_2946d40b_24a1_47fa_8176_e3f79bb45064> ;
                                                                             <http://emmo.info/emmo/middle/isq#EMMO_de178b12_5d35_4bca_8efa_a4193162571d> "T+1 L0 M0 I+1 T0 N0 J0" ;
                                                                             <http://emmo.info/emmo/top/annotations#EMMO_1f1b164d_ec6a_4faa_8d5e_88bda62316cc> "http://qudt.org/vocab/quantitykind/ElectricCharge" ;
                                                                             <http://emmo.info/emmo/top/annotations#EMMO_6dd685dd_1895_46e4_b227_be9f7d643c25> "http://dbpedia.org/page/Electric_charge" ;
                                                                             <http://emmo.info/emmo/top/annotations#EMMO_967080e5_2f42_4eb2_a3a9_c58143e835f9> "The physical property of matter that causes it to experience a force when placed in an electromagnetic field."@en ;
                                                                             <http://emmo.info/emmo/top/annotations#EMMO_fe015383_afb3_44a6_ae86_043628697aa2> "https://doi.org/10.1351/goldbook.E01923" ;
                                                                             <http://www.w3.org/2004/02/skos/core#altLabel> "Charge"@en ;
                                                                             <http://www.w3.org/2004/02/skos/core#prefLabel> "ElectricCharge"@en .


###  http://emmo.info/emmo/middle/isq#EMMO_16f2fe60_2db7_43ca_8fee_5b3e416bfe87
<http://emmo.info/emmo/middle/isq#EMMO_16f2fe60_2db7_43ca_8fee_5b3e416bfe87> rdf:type owl:Class ;
                                                                             rdfs:subClassOf <http://emmo.info/emmo/middle/chemistry#EMMO_a293f923_954c_4af5_9f97_9600ebd362cb> ,
                                                                                             <http://emmo.info/emmo/middle/isq#EMMO_06448f64_8db6_4304_8b2c_e785dba82044> ;
                                                                             <http://emmo.info/emmo/middle/isq#EMMO_de178b12_5d35_4bca_8efa_a4193162571d> "T0 L-3 M+1 I0 T0 N0 J0" ;
                                                                             <http://emmo.info/emmo/top/annotations#EMMO_1f1b164d_ec6a_4faa_8d5e_88bda62316cc> "http://qudt.org/vocab/quantitykind/MassConcentration" ;
                                                                             <http://emmo.info/emmo/top/annotations#EMMO_6dd685dd_1895_46e4_b227_be9f7d643c25> "http://dbpedia.org/page/Mass_concentration_(chemistry)" ;
                                                                             <http://emmo.info/emmo/top/annotations#EMMO_fe015383_afb3_44a6_ae86_043628697aa2> "https://doi.org/10.1351/goldbook.M03713" ;
                                                                             rdfs:comment "Mass of a constituent divided by the volume of the mixture."@en ;
                                                                             <http://www.w3.org/2004/02/skos/core#prefLabel> "MassConcentration"@en .


###  http://emmo.info/emmo/middle/isq#EMMO_176cae33_b83e_4cd2_a6bc_281f42f0ccc8
<http://emmo.info/emmo/middle/isq#EMMO_176cae33_b83e_4cd2_a6bc_281f42f0ccc8> rdf:type owl:Class ;
                                                                             rdfs:subClassOf <http://emmo.info/emmo/middle/isq#EMMO_f2ca6dd0_0e5f_4392_a92d_cafdae6cfc95> ;
                                                                             <http://emmo.info/emmo/middle/isq#EMMO_de178b12_5d35_4bca_8efa_a4193162571d> "T0 L0 M0 I0 T0 N-1 J0" ;
                                                                             <http://emmo.info/emmo/top/annotations#EMMO_1f1b164d_ec6a_4faa_8d5e_88bda62316cc> "http://qudt.org/vocab/constant/AvogadroConstant" ;
                                                                             <http://emmo.info/emmo/top/annotations#EMMO_967080e5_2f42_4eb2_a3a9_c58143e835f9> """The number of constituent particles, usually atoms or molecules, that are contained in the amount of substance given by one mole.

It defines the base unit mole in the SI system."""@en ;
                                                                             <http://emmo.info/emmo/top/annotations#EMMO_a9b3d04c_7ceb_40a2_b8d3_28d514a770a8> "https://physics.nist.gov/cgi-bin/cuu/Value?na" ;
                                                                             <http://emmo.info/emmo/top/annotations#EMMO_fe015383_afb3_44a6_ae86_043628697aa2> "https://doi.org/10.1351/goldbook.A00543" ;
                                                                             rdfs:comment "The DBpedia definition (http://dbpedia.org/page/Avogadro_constant) is outdated as May 20, 2019. It is now an exact quantity."@en ;
                                                                             <http://www.w3.org/2004/02/skos/core#prefLabel> "AvogadroConstant"@en .


###  http://emmo.info/emmo/middle/isq#EMMO_1a179ce4_3724_47f8_bee5_6292e3ac9942
<http://emmo.info/emmo/middle/isq#EMMO_1a179ce4_3724_47f8_bee5_6292e3ac9942> rdf:type owl:Class ;
                                                                             rdfs:subClassOf <http://emmo.info/emmo/middle/isq#EMMO_2946d40b_24a1_47fa_8176_e3f79bb45064> ;
                                                                             <http://emmo.info/emmo/middle/isq#EMMO_de178b12_5d35_4bca_8efa_a4193162571d> "T+1 L+1 M0 I+1 T0 N0 J0" ;
                                                                             <http://emmo.info/emmo/top/annotations#EMMO_1f1b164d_ec6a_4faa_8d5e_88bda62316cc> "http://qudt.org/vocab/quantitykind/ElectricDipoleMoment" ;
                                                                             <http://emmo.info/emmo/top/annotations#EMMO_50c298c2_55a2_4068_b3ac_4e948c33181f> "http://www.electropedia.org/iev/iev.nsf/display?openform&ievref=121-11-35" ,
                                                                                                                                                               "http://www.electropedia.org/iev/iev.nsf/display?openform&ievref=121-11-36" ;
                                                                             <http://emmo.info/emmo/top/annotations#EMMO_6dd685dd_1895_46e4_b227_be9f7d643c25> "http://dbpedia.org/page/Electric_dipole_moment" ;
                                                                             <http://emmo.info/emmo/top/annotations#EMMO_967080e5_2f42_4eb2_a3a9_c58143e835f9> "An electric dipole, vector quantity of magnitude equal to the product of the positive charge and the distance between the charges and directed from the negative charge to the positive charge."@en ;
                                                                             <http://emmo.info/emmo/top/annotations#EMMO_e55f2d7c_9893_48cd_b4a4_fdf38253bd20> "http://www.ontology-of-units-of-measure.org/resource/om-2/ElectricDipoleMoment" ;
                                                                             <http://emmo.info/emmo/top/annotations#EMMO_fe015383_afb3_44a6_ae86_043628697aa2> "https://doi.org/10.1351/goldbook.E01929" ;
                                                                             <http://www.w3.org/2004/02/skos/core#prefLabel> "ElectricDipoleMoment"@en .


###  http://emmo.info/emmo/middle/isq#EMMO_1a4c1a97_88a7_4d8e_b2f9_2ca58e92dde4
<http://emmo.info/emmo/middle/isq#EMMO_1a4c1a97_88a7_4d8e_b2f9_2ca58e92dde4> rdf:type owl:Class ;
                                                                             rdfs:subClassOf <http://emmo.info/emmo/middle/isq#EMMO_f35cff4d_dc09_44cf_a729_22fb79e3bfb2> ,
                                                                                             <http://emmo.info/emmo/middle/metrology#EMMO_acaaa124_3dde_48b6_86e6_6ec6f364f408> ;
                                                                             <http://emmo.info/emmo/top/annotations#EMMO_967080e5_2f42_4eb2_a3a9_c58143e835f9> "Base quantities defined in the International System of Quantities (ISQ)."@en ;
                                                                             <http://emmo.info/emmo/top/annotations#EMMO_c84c6752_6d64_48cc_9500_e54a3c34898d> "https://en.wikipedia.org/wiki/International_System_of_Quantities" ;
                                                                             <http://www.w3.org/2004/02/skos/core#prefLabel> "ISQBaseQuantity"@en .


###  http://emmo.info/emmo/middle/isq#EMMO_1c2226a9_22f0_40c8_8928_5a01d398f96e
<http://emmo.info/emmo/middle/isq#EMMO_1c2226a9_22f0_40c8_8928_5a01d398f96e> rdf:type owl:Class ;
                                                                             rdfs:subClassOf <http://emmo.info/emmo/middle/metrology#EMMO_9895a1b4_f0a5_4167_ac5e_97db40b8bfcc> ;
                                                                             <http://www.w3.org/2004/02/skos/core#prefLabel> "MagneticDipoleMomentDimension"@en .


###  http://emmo.info/emmo/middle/isq#EMMO_1e7603a7_1365_49b8_b5e5_3711c8e6b904
<http://emmo.info/emmo/middle/isq#EMMO_1e7603a7_1365_49b8_b5e5_3711c8e6b904> rdf:type owl:Class ;
                                                                             rdfs:subClassOf <http://emmo.info/emmo/middle/isq#EMMO_2946d40b_24a1_47fa_8176_e3f79bb45064> ;
                                                                             <http://emmo.info/emmo/middle/isq#EMMO_de178b12_5d35_4bca_8efa_a4193162571d> "T0 L-1 M0 I0 T0 N0 J0" ;
                                                                             <http://emmo.info/emmo/top/annotations#EMMO_6dd685dd_1895_46e4_b227_be9f7d643c25> "http://dbpedia.org/page/Vergence" ;
                                                                             rdfs:comment "In geometrical optics, vergence describes the curvature of optical wavefronts."@en ;
                                                                             <http://www.w3.org/2004/02/skos/core#prefLabel> "Vergence"@en .


###  http://emmo.info/emmo/middle/isq#EMMO_1f087811_06cb_42d5_90fb_25d0e7e068ef
<http://emmo.info/emmo/middle/isq#EMMO_1f087811_06cb_42d5_90fb_25d0e7e068ef> rdf:type owl:Class ;
                                                                             rdfs:subClassOf <http://emmo.info/emmo/middle/isq#EMMO_2946d40b_24a1_47fa_8176_e3f79bb45064> ;
                                                                             <http://emmo.info/emmo/middle/isq#EMMO_de178b12_5d35_4bca_8efa_a4193162571d> "T-2 L+1 M+1 I0 T0 N0 J0" ;
                                                                             <http://emmo.info/emmo/top/annotations#EMMO_1f1b164d_ec6a_4faa_8d5e_88bda62316cc> "http://qudt.org/vocab/quantitykind/Force" ;
                                                                             <http://emmo.info/emmo/top/annotations#EMMO_6dd685dd_1895_46e4_b227_be9f7d643c25> "http://dbpedia.org/page/Force" ;
                                                                             <http://emmo.info/emmo/top/annotations#EMMO_967080e5_2f42_4eb2_a3a9_c58143e835f9> "Any interaction that, when unopposed, will change the motion of an object."@en ;
                                                                             <http://emmo.info/emmo/top/annotations#EMMO_fe015383_afb3_44a6_ae86_043628697aa2> "https://doi.org/10.1351/goldbook.F02480" ;
                                                                             <http://www.w3.org/2004/02/skos/core#prefLabel> "Force"@en .


###  http://emmo.info/emmo/middle/isq#EMMO_27367073_ed8a_481a_9b07_f836dfe31f7f
<http://emmo.info/emmo/middle/isq#EMMO_27367073_ed8a_481a_9b07_f836dfe31f7f> rdf:type owl:Class ;
                                                                             rdfs:subClassOf <http://emmo.info/emmo/middle/isq#EMMO_ed4af7ae_63a2_497e_bb88_2309619ea405> ;
                                                                             <http://emmo.info/emmo/middle/isq#EMMO_de178b12_5d35_4bca_8efa_a4193162571d> "T0 L0 M+1 I0 T0 N0 J0" ;
                                                                             <http://emmo.info/emmo/top/annotations#EMMO_70fe84ff_99b6_4206_a9fc_9a8931836d84> "The mass of an atom in the ground state."@en ;
                                                                             <http://emmo.info/emmo/top/annotations#EMMO_c84c6752_6d64_48cc_9500_e54a3c34898d> "https://en.wikipedia.org/wiki/Atomic_mass" ;
                                                                             <http://emmo.info/emmo/top/annotations#EMMO_fe015383_afb3_44a6_ae86_043628697aa2> "https://doi.org/10.1351/goldbook.A00496" ;
                                                                             rdfs:comment "Since the nucleus account for nearly all of the total mass of atoms  (with the electrons and nuclear binding energy making minor contributions), the atomic mass measured in Da has nearly the same value as the mass number."@en ,
                                                                                          "The atomic mass is often expressed as an average of the commonly found isotopes."@en ;
                                                                             <http://www.w3.org/2004/02/skos/core#prefLabel> "AtomicMass"@en .


###  http://emmo.info/emmo/middle/isq#EMMO_2946d40b_24a1_47fa_8176_e3f79bb45064
<http://emmo.info/emmo/middle/isq#EMMO_2946d40b_24a1_47fa_8176_e3f79bb45064> rdf:type owl:Class ;
                                                                             rdfs:subClassOf <http://emmo.info/emmo/middle/isq#EMMO_f35cff4d_dc09_44cf_a729_22fb79e3bfb2> ,
                                                                                             <http://emmo.info/emmo/middle/metrology#EMMO_71f6ab56_342c_484b_bbe0_de86b7367cb3> ;
                                                                             <http://emmo.info/emmo/top/annotations#EMMO_967080e5_2f42_4eb2_a3a9_c58143e835f9> "Derived quantities defined in the International System of Quantities (ISQ)."@en ;
                                                                             <http://www.w3.org/2004/02/skos/core#prefLabel> "ISQDerivedQuantity"@en .


###  http://emmo.info/emmo/middle/isq#EMMO_2e7e5796_4a80_4d73_bb84_f31138446c0c
<http://emmo.info/emmo/middle/isq#EMMO_2e7e5796_4a80_4d73_bb84_f31138446c0c> rdf:type owl:Class ;
                                                                             rdfs:subClassOf <http://emmo.info/emmo/middle/metrology#EMMO_9895a1b4_f0a5_4167_ac5e_97db40b8bfcc> ;
                                                                             <http://www.w3.org/2004/02/skos/core#prefLabel> "ElectricPotentialDimension"@en .


###  http://emmo.info/emmo/middle/isq#EMMO_31ec09ba_1713_42cb_83c7_b38bf6f9ced2
<http://emmo.info/emmo/middle/isq#EMMO_31ec09ba_1713_42cb_83c7_b38bf6f9ced2> rdf:type owl:Class ;
                                                                             rdfs:subClassOf <http://emmo.info/emmo/middle/isq#EMMO_2946d40b_24a1_47fa_8176_e3f79bb45064> ;
                                                                             <http://emmo.info/emmo/middle/isq#EMMO_de178b12_5d35_4bca_8efa_a4193162571d> "T-2 L+2 M+1 I0 T0 N0 J0" ;
                                                                             <http://emmo.info/emmo/top/annotations#EMMO_1f1b164d_ec6a_4faa_8d5e_88bda62316cc> "http://qudt.org/vocab/quantitykind/Energy" ;
                                                                             <http://emmo.info/emmo/top/annotations#EMMO_6dd685dd_1895_46e4_b227_be9f7d643c25> "http://dbpedia.org/page/Energy" ;
                                                                             <http://emmo.info/emmo/top/annotations#EMMO_967080e5_2f42_4eb2_a3a9_c58143e835f9> "A property of objects which can be transferred to other objects or converted into different forms."@en ;
                                                                             <http://emmo.info/emmo/top/annotations#EMMO_fe015383_afb3_44a6_ae86_043628697aa2> "https://doi.org/10.1351/goldbook.E02101" ;
                                                                             rdfs:comment "Energy is often defined as \"ability of a system to perform work\", but it might be misleading since is not necessarily available to do work."@en ;
                                                                             <http://www.w3.org/2004/02/skos/core#prefLabel> "Energy"@en .


###  http://emmo.info/emmo/middle/isq#EMMO_321af35f_f0cc_4a5c_b4fe_8c2c0303fb0c
<http://emmo.info/emmo/middle/isq#EMMO_321af35f_f0cc_4a5c_b4fe_8c2c0303fb0c> rdf:type owl:Class ;
                                                                             rdfs:subClassOf <http://emmo.info/emmo/middle/metrology#EMMO_9895a1b4_f0a5_4167_ac5e_97db40b8bfcc> ;
                                                                             <http://www.w3.org/2004/02/skos/core#prefLabel> "ElectricConductanceDimension"@en .


###  http://emmo.info/emmo/middle/isq#EMMO_33433bb1_c68f_45ee_a466_f01e2c57b214
<http://emmo.info/emmo/middle/isq#EMMO_33433bb1_c68f_45ee_a466_f01e2c57b214> rdf:type owl:Class ;
                                                                             rdfs:subClassOf <http://emmo.info/emmo/middle/metrology#EMMO_9895a1b4_f0a5_4167_ac5e_97db40b8bfcc> ;
                                                                             <http://www.w3.org/2004/02/skos/core#prefLabel> "AreaDimension"@en .


###  http://emmo.info/emmo/middle/isq#EMMO_3b931698_937e_49be_ab1b_36fa52d91181
<http://emmo.info/emmo/middle/isq#EMMO_3b931698_937e_49be_ab1b_36fa52d91181> rdf:type owl:Class ;
                                                                             rdfs:subClassOf <http://emmo.info/emmo/middle/isq#EMMO_2946d40b_24a1_47fa_8176_e3f79bb45064> ;
                                                                             <http://emmo.info/emmo/middle/isq#EMMO_de178b12_5d35_4bca_8efa_a4193162571d> "T-2 L+2 M+1 I-1 T0 N0 J0" ;
                                                                             <http://emmo.info/emmo/top/annotations#EMMO_1f1b164d_ec6a_4faa_8d5e_88bda62316cc> "http://qudt.org/vocab/quantitykind/MagneticFlux" ;
                                                                             <http://emmo.info/emmo/top/annotations#EMMO_6dd685dd_1895_46e4_b227_be9f7d643c25> "http://dbpedia.org/page/Magnetic_flux" ;
                                                                             <http://emmo.info/emmo/top/annotations#EMMO_967080e5_2f42_4eb2_a3a9_c58143e835f9> "Measure of magnetism, taking account of the strength and the extent of a magnetic field."@en ;
                                                                             <http://emmo.info/emmo/top/annotations#EMMO_fe015383_afb3_44a6_ae86_043628697aa2> "https://doi.org/10.1351/goldbook.M03684" ;
                                                                             <http://www.w3.org/2004/02/skos/core#prefLabel> "MagneticFlux"@en .


###  http://emmo.info/emmo/middle/isq#EMMO_3df10765_f6ff_4c9e_be3d_10b1809d78bd
<http://emmo.info/emmo/middle/isq#EMMO_3df10765_f6ff_4c9e_be3d_10b1809d78bd> rdf:type owl:Class ;
                                                                             rdfs:subClassOf <http://emmo.info/emmo/middle/isq#EMMO_2946d40b_24a1_47fa_8176_e3f79bb45064> ;
                                                                             <http://emmo.info/emmo/middle/isq#EMMO_de178b12_5d35_4bca_8efa_a4193162571d> "T-2 L+2 M0 I0 T0 N0 J0" ;
                                                                             <http://emmo.info/emmo/top/annotations#EMMO_1f1b164d_ec6a_4faa_8d5e_88bda62316cc> "http://qudt.org/vocab/quantitykind/DoseEquivalent" ;
                                                                             <http://emmo.info/emmo/top/annotations#EMMO_6dd685dd_1895_46e4_b227_be9f7d643c25> "http://dbpedia.org/page/Energy" ;
                                                                             <http://emmo.info/emmo/top/annotations#EMMO_967080e5_2f42_4eb2_a3a9_c58143e835f9> "A dose quantity used in the International Commission on Radiological Protection (ICRP) system of radiological protection."@en ;
                                                                             <http://emmo.info/emmo/top/annotations#EMMO_fe015383_afb3_44a6_ae86_043628697aa2> "https://doi.org/10.1351/goldbook.E02101" ;
                                                                             <http://www.w3.org/2004/02/skos/core#prefLabel> "DoseEquivalent"@en .


###  http://emmo.info/emmo/middle/isq#EMMO_3ecff38b_b3cf_4a78_b49f_8580abf8715b
<http://emmo.info/emmo/middle/isq#EMMO_3ecff38b_b3cf_4a78_b49f_8580abf8715b> rdf:type owl:Class ;
                                                                             rdfs:subClassOf <http://emmo.info/emmo/middle/metrology#EMMO_9895a1b4_f0a5_4167_ac5e_97db40b8bfcc> ;
                                                                             <http://www.w3.org/2004/02/skos/core#prefLabel> "EntropyDimension"@en .


###  http://emmo.info/emmo/middle/isq#EMMO_4091d5ec_a4df_42b9_a073_9a090839279f
<http://emmo.info/emmo/middle/isq#EMMO_4091d5ec_a4df_42b9_a073_9a090839279f> rdf:type owl:Class ;
                                                                             rdfs:subClassOf <http://emmo.info/emmo/middle/isq#EMMO_31ec09ba_1713_42cb_83c7_b38bf6f9ced2> ;
                                                                             <http://emmo.info/emmo/middle/isq#EMMO_de178b12_5d35_4bca_8efa_a4193162571d> "T-2 L+2 M+1 I0 T0 N0 J0" ;
                                                                             <http://emmo.info/emmo/top/annotations#EMMO_1f1b164d_ec6a_4faa_8d5e_88bda62316cc> "http://qudt.org/vocab/quantitykind/Enthalpy" ;
                                                                             <http://emmo.info/emmo/top/annotations#EMMO_6dd685dd_1895_46e4_b227_be9f7d643c25> "http://dbpedia.org/page/Enthalpy" ;
                                                                             <http://emmo.info/emmo/top/annotations#EMMO_fe015383_afb3_44a6_ae86_043628697aa2> "https://doi.org/10.1351/goldbook.E02141" ;
                                                                             rdfs:comment "Measurement of energy in a thermodynamic system."@en ;
                                                                             <http://www.w3.org/2004/02/skos/core#prefLabel> "Enthalpy"@en .


###  http://emmo.info/emmo/middle/isq#EMMO_43776fc9_d712_4571_85f0_72183678039a
<http://emmo.info/emmo/middle/isq#EMMO_43776fc9_d712_4571_85f0_72183678039a> rdf:type owl:Class ;
                                                                             rdfs:subClassOf <http://emmo.info/emmo/middle/isq#EMMO_2946d40b_24a1_47fa_8176_e3f79bb45064> ;
                                                                             <http://emmo.info/emmo/middle/isq#EMMO_de178b12_5d35_4bca_8efa_a4193162571d> "T-1 L+1 M+1 I0 T0 N0 J0" ;
                                                                             <http://emmo.info/emmo/top/annotations#EMMO_1f1b164d_ec6a_4faa_8d5e_88bda62316cc> "http://qudt.org/vocab/quantitykind/Momentum" ;
                                                                             <http://emmo.info/emmo/top/annotations#EMMO_6dd685dd_1895_46e4_b227_be9f7d643c25> "http://dbpedia.org/page/Momentum" ;
                                                                             <http://emmo.info/emmo/top/annotations#EMMO_fe015383_afb3_44a6_ae86_043628697aa2> "https://doi.org/10.1351/goldbook.M04007" ;
                                                                             rdfs:comment "Product of mass and velocity."@en ;
                                                                             <http://www.w3.org/2004/02/skos/core#prefLabel> "Momentum"@en .


###  http://emmo.info/emmo/middle/isq#EMMO_44da6d75_54a4_4aa8_bd3a_156f6e9abb8e
<http://emmo.info/emmo/middle/isq#EMMO_44da6d75_54a4_4aa8_bd3a_156f6e9abb8e> rdf:type owl:Class ;
                                                                             rdfs:subClassOf <http://emmo.info/emmo/middle/isq#EMMO_cd2cd0de_e0cc_4ef1_b27e_2e88db027bac> ;
                                                                             <http://emmo.info/emmo/middle/isq#EMMO_de178b12_5d35_4bca_8efa_a4193162571d> "T0 L+1 M0 I0 T0 N0 J0" ;
                                                                             <http://emmo.info/emmo/top/annotations#EMMO_50c298c2_55a2_4068_b3ac_4e948c33181f> "http://www.electropedia.org/iev/iev.nsf/display?openform&ievref=113-03-12" ;
                                                                             <http://emmo.info/emmo/top/annotations#EMMO_70fe84ff_99b6_4206_a9fc_9a8931836d84> "Vector r characterizing a point P in a point space with a given origin point O."@en ;
                                                                             rdfs:comment """In the usual geometrical three-dimensional space, position vectors are quantities of the dimension length. 

-- IEC"""@en ,
                                                                                          """Position vectors are so-called bounded vectors, i.e. their magnitude and direction depend on the particular coordinate system used.

-- ISO 80000-3"""@en ;
                                                                             <http://www.w3.org/2004/02/skos/core#altLabel> "Position"@en ;
                                                                             <http://www.w3.org/2004/02/skos/core#prefLabel> "PositionVector"@en .


###  http://emmo.info/emmo/middle/isq#EMMO_44fc8c60_7a9c_49af_a046_e1878c88862c
<http://emmo.info/emmo/middle/isq#EMMO_44fc8c60_7a9c_49af_a046_e1878c88862c> rdf:type owl:Class ;
                                                                             rdfs:subClassOf <http://emmo.info/emmo/middle/isq#EMMO_ed4af7ae_63a2_497e_bb88_2309619ea405> ,
                                                                                             <http://emmo.info/emmo/middle/metrology#EMMO_3f15d200_c97b_42c8_8ac0_d81d150361e2> ;
                                                                             <http://emmo.info/emmo/middle/isq#EMMO_de178b12_5d35_4bca_8efa_a4193162571d> "T0 L0 M+1 I0 T0 N0 J0" ;
                                                                             <http://emmo.info/emmo/top/annotations#EMMO_1f1b164d_ec6a_4faa_8d5e_88bda62316cc> "http://qudt.org/vocab/constant/ElectronMass" ;
                                                                             <http://emmo.info/emmo/top/annotations#EMMO_6dd685dd_1895_46e4_b227_be9f7d643c25> "http://dbpedia.org/page/Electron_rest_mass" ;
                                                                             <http://emmo.info/emmo/top/annotations#EMMO_a9b3d04c_7ceb_40a2_b8d3_28d514a770a8> "https://physics.nist.gov/cgi-bin/cuu/Value?me" ;
                                                                             <http://emmo.info/emmo/top/annotations#EMMO_fe015383_afb3_44a6_ae86_043628697aa2> "https://doi.org/10.1351/goldbook.E02008" ;
                                                                             rdfs:comment "The rest mass of an electron."@en ;
                                                                             <http://www.w3.org/2004/02/skos/core#prefLabel> "ElectronMass"@en .


###  http://emmo.info/emmo/middle/isq#EMMO_4c151909_6f26_4ef9_b43d_7c9e9514883a
<http://emmo.info/emmo/middle/isq#EMMO_4c151909_6f26_4ef9_b43d_7c9e9514883a> rdf:type owl:Class ;
                                                                             rdfs:subClassOf <http://emmo.info/emmo/middle/isq#EMMO_31ec09ba_1713_42cb_83c7_b38bf6f9ced2> ;
                                                                             <http://emmo.info/emmo/middle/isq#EMMO_de178b12_5d35_4bca_8efa_a4193162571d> "T-2 L+2 M+1 I0 T0 N0 J0" ;
                                                                             <http://emmo.info/emmo/top/annotations#EMMO_1f1b164d_ec6a_4faa_8d5e_88bda62316cc> "http://qudt.org/vocab/quantitykind/PotentialEnergy" ;
                                                                             <http://emmo.info/emmo/top/annotations#EMMO_50c298c2_55a2_4068_b3ac_4e948c33181f> "http://www.electropedia.org/iev/iev.nsf/display?openform&ievref=113-03-48" ;
                                                                             <http://emmo.info/emmo/top/annotations#EMMO_6dd685dd_1895_46e4_b227_be9f7d643c25> "http://dbpedia.org/page/Potential_energy" ;
                                                                             <http://emmo.info/emmo/top/annotations#EMMO_967080e5_2f42_4eb2_a3a9_c58143e835f9> "The energy possessed by a body by virtue of its position or orientation in a potential field."@en ;
                                                                             <http://emmo.info/emmo/top/annotations#EMMO_e55f2d7c_9893_48cd_b4a4_fdf38253bd20> "http://www.ontology-of-units-of-measure.org/resource/om-2/PotentialEnergy" ;
                                                                             <http://emmo.info/emmo/top/annotations#EMMO_fe015383_afb3_44a6_ae86_043628697aa2> "https://doi.org/10.1351/goldbook.P04778" ;
                                                                             <http://www.w3.org/2004/02/skos/core#prefLabel> "PotentialEnergy"@en .


###  http://emmo.info/emmo/middle/isq#EMMO_4c49ab58_a6f6_409e_b849_f873ae1dcbee
<http://emmo.info/emmo/middle/isq#EMMO_4c49ab58_a6f6_409e_b849_f873ae1dcbee> rdf:type owl:Class ;
                                                                             rdfs:subClassOf <http://emmo.info/emmo/middle/metrology#EMMO_9895a1b4_f0a5_4167_ac5e_97db40b8bfcc> ;
                                                                             <http://www.w3.org/2004/02/skos/core#prefLabel> "MagneticFluxDimension"@en .


###  http://emmo.info/emmo/middle/isq#EMMO_4f2d3939_91b1_4001_b8ab_7d19074bf845
<http://emmo.info/emmo/middle/isq#EMMO_4f2d3939_91b1_4001_b8ab_7d19074bf845> rdf:type owl:Class ;
                                                                             rdfs:subClassOf <http://emmo.info/emmo/middle/isq#EMMO_2946d40b_24a1_47fa_8176_e3f79bb45064> ;
                                                                             <http://emmo.info/emmo/middle/isq#EMMO_de178b12_5d35_4bca_8efa_a4193162571d> "T-3 L+2 M+1 I-1 T0 N0 J0" ;
                                                                             <http://emmo.info/emmo/top/annotations#EMMO_1f1b164d_ec6a_4faa_8d5e_88bda62316cc> "http://qudt.org/vocab/quantitykind/Voltage" ;
                                                                             <http://emmo.info/emmo/top/annotations#EMMO_6dd685dd_1895_46e4_b227_be9f7d643c25> "http://dbpedia.org/page/Voltage" ;
                                                                             <http://emmo.info/emmo/top/annotations#EMMO_967080e5_2f42_4eb2_a3a9_c58143e835f9> "Energy required to move a unit charge through an electric field from a reference point."@en ;
                                                                             <http://emmo.info/emmo/top/annotations#EMMO_fe015383_afb3_44a6_ae86_043628697aa2> "https://doi.org/10.1351/goldbook.A00424" ;
                                                                             <http://www.w3.org/2004/02/skos/core#altLabel> "Voltage"@en ;
                                                                             <http://www.w3.org/2004/02/skos/core#prefLabel> "ElectricPotential"@en .


###  http://emmo.info/emmo/middle/isq#EMMO_4f5c7c54_1c63_4d17_b12b_ea0792c2b187
<http://emmo.info/emmo/middle/isq#EMMO_4f5c7c54_1c63_4d17_b12b_ea0792c2b187> rdf:type owl:Class ;
                                                                             owl:equivalentClass <http://emmo.info/emmo/middle/isq#EMMO_f84792eb_ec64_4a6b_941f_c9f3e9ef052c> ;
                                                                             rdfs:subClassOf <http://emmo.info/emmo/middle/metrology#EMMO_9895a1b4_f0a5_4167_ac5e_97db40b8bfcc> ;
                                                                             <http://www.w3.org/2004/02/skos/core#prefLabel> "SpeedDimension"@en .


###  http://emmo.info/emmo/middle/isq#EMMO_501f9b3a_c469_48f7_9281_2e6a8d805d7a
<http://emmo.info/emmo/middle/isq#EMMO_501f9b3a_c469_48f7_9281_2e6a8d805d7a> rdf:type owl:Class ;
                                                                             rdfs:subClassOf <http://emmo.info/emmo/middle/metrology#EMMO_9895a1b4_f0a5_4167_ac5e_97db40b8bfcc> ;
                                                                             <http://www.w3.org/2004/02/skos/core#prefLabel> "AngularMomentumDimension"@en .


###  http://emmo.info/emmo/middle/isq#EMMO_506f7823_52bc_40cb_be07_b3b1e10cce13
<http://emmo.info/emmo/middle/isq#EMMO_506f7823_52bc_40cb_be07_b3b1e10cce13> rdf:type owl:Class ;
                                                                             rdfs:subClassOf <http://emmo.info/emmo/middle/isq#EMMO_f2ca6dd0_0e5f_4392_a92d_cafdae6cfc95> ;
                                                                             <http://emmo.info/emmo/middle/isq#EMMO_de178b12_5d35_4bca_8efa_a4193162571d> "T+3 L-1 M-1 I0 T0 N0 J+1" ;
                                                                             <http://emmo.info/emmo/top/annotations#EMMO_967080e5_2f42_4eb2_a3a9_c58143e835f9> "The luminous efficacy of monochromatic radiation of frequency 540  10 12 Hz, K cd , is a technical constant that gives an exact numerical relationship between the purely physical characteristics of the radiant power stimulating the human eye (W) and its photobiological response defined by the luminous flux due to the spectral responsivity of a standard observer (lm) at a frequency of 540  10 12 hertz."@en ;
                                                                             <http://emmo.info/emmo/top/annotations#EMMO_a9b3d04c_7ceb_40a2_b8d3_28d514a770a8> "https://physics.nist.gov/cgi-bin/cuu/Value?kcd" ;
                                                                             rdfs:comment "Defines the Candela base unit in the SI system."@en ;
                                                                             <http://www.w3.org/2004/02/skos/core#prefLabel> "LuminousEfficacyOf540THzRadiation"@en .


###  http://emmo.info/emmo/middle/isq#EMMO_50a44256_9dc5_434b_bad4_74a4d9a29989
<http://emmo.info/emmo/middle/isq#EMMO_50a44256_9dc5_434b_bad4_74a4d9a29989> rdf:type owl:Class ;
                                                                             rdfs:subClassOf <http://emmo.info/emmo/middle/isq#EMMO_2946d40b_24a1_47fa_8176_e3f79bb45064> ;
                                                                             <http://emmo.info/emmo/middle/isq#EMMO_de178b12_5d35_4bca_8efa_a4193162571d> "T-2 L-1 M+1 I0 T0 N0 J0" ;
                                                                             <http://emmo.info/emmo/top/annotations#EMMO_1f1b164d_ec6a_4faa_8d5e_88bda62316cc> "http://qudt.org/vocab/quantitykind/Pressure" ;
                                                                             <http://emmo.info/emmo/top/annotations#EMMO_6dd685dd_1895_46e4_b227_be9f7d643c25> "http://dbpedia.org/page/Pressure" ;
                                                                             <http://emmo.info/emmo/top/annotations#EMMO_967080e5_2f42_4eb2_a3a9_c58143e835f9> "The force applied perpendicular to the surface of an object per unit area over which that force is distributed."@en ;
                                                                             <http://emmo.info/emmo/top/annotations#EMMO_fe015383_afb3_44a6_ae86_043628697aa2> "https://doi.org/10.1351/goldbook.P04819" ;
                                                                             <http://www.w3.org/2004/02/skos/core#prefLabel> "Pressure"@en .


###  http://emmo.info/emmo/middle/isq#EMMO_50bf79a6_a48b_424d_9d2c_813bd631231a
<http://emmo.info/emmo/middle/isq#EMMO_50bf79a6_a48b_424d_9d2c_813bd631231a> rdf:type owl:Class ;
                                                                             rdfs:subClassOf <http://emmo.info/emmo/middle/isq#EMMO_1a4c1a97_88a7_4d8e_b2f9_2ca58e92dde4> ;
                                                                             <http://emmo.info/emmo/middle/isq#EMMO_de178b12_5d35_4bca_8efa_a4193162571d> "T0 L0 M0 I0 T0 N0 J+1" ;
                                                                             <http://emmo.info/emmo/top/annotations#EMMO_1f1b164d_ec6a_4faa_8d5e_88bda62316cc> "http://qudt.org/vocab/quantitykind/Length" ;
                                                                             <http://emmo.info/emmo/top/annotations#EMMO_6dd685dd_1895_46e4_b227_be9f7d643c25> "http://dbpedia.org/page/Luminous_intensity" ;
                                                                             <http://emmo.info/emmo/top/annotations#EMMO_967080e5_2f42_4eb2_a3a9_c58143e835f9> "A measure of the wavelength-weighted power emitted by a light source in a particular direction per unit solid angle. It is based on the luminosity function, which is a standardized model of the sensitivity of the human eye."@en ;
                                                                             <http://www.w3.org/2004/02/skos/core#prefLabel> "LuminousIntensity"@en .


###  http://emmo.info/emmo/middle/isq#EMMO_515b5579_d526_4842_9e6f_ecc34db6f368
<http://emmo.info/emmo/middle/isq#EMMO_515b5579_d526_4842_9e6f_ecc34db6f368> rdf:type owl:Class ;
                                                                             rdfs:subClassOf <http://emmo.info/emmo/middle/metrology#EMMO_9895a1b4_f0a5_4167_ac5e_97db40b8bfcc> ;
                                                                             <http://www.w3.org/2004/02/skos/core#prefLabel> "FrequencyDimension"@en .


###  http://emmo.info/emmo/middle/isq#EMMO_53bd0c90_41c3_46e2_8779_cd2a80f7e18b
<http://emmo.info/emmo/middle/isq#EMMO_53bd0c90_41c3_46e2_8779_cd2a80f7e18b> rdf:type owl:Class ;
                                                                             rdfs:subClassOf <http://emmo.info/emmo/middle/metrology#EMMO_9895a1b4_f0a5_4167_ac5e_97db40b8bfcc> ;
                                                                             <http://www.w3.org/2004/02/skos/core#prefLabel> "PressureDimension"@en .


###  http://emmo.info/emmo/middle/isq#EMMO_53e825d9_1a09_483c_baa7_37501ebfbe1c
<http://emmo.info/emmo/middle/isq#EMMO_53e825d9_1a09_483c_baa7_37501ebfbe1c> rdf:type owl:Class ;
                                                                             rdfs:subClassOf <http://emmo.info/emmo/middle/metrology#EMMO_9895a1b4_f0a5_4167_ac5e_97db40b8bfcc> ;
                                                                             <http://www.w3.org/2004/02/skos/core#prefLabel> "ForceDimension"@en .


###  http://emmo.info/emmo/middle/isq#EMMO_585e0ff0_9429_4d3c_b578_58abb1ba21d1
<http://emmo.info/emmo/middle/isq#EMMO_585e0ff0_9429_4d3c_b578_58abb1ba21d1> rdf:type owl:Class ;
                                                                             rdfs:subClassOf <http://emmo.info/emmo/middle/metrology#EMMO_9895a1b4_f0a5_4167_ac5e_97db40b8bfcc> ;
                                                                             <http://www.w3.org/2004/02/skos/core#prefLabel> "InductanceDimension"@en .


###  http://emmo.info/emmo/middle/isq#EMMO_58a650f0_a638_4743_8439_535a325e5c4c
<http://emmo.info/emmo/middle/isq#EMMO_58a650f0_a638_4743_8439_535a325e5c4c> rdf:type owl:Class ;
                                                                             rdfs:subClassOf <http://emmo.info/emmo/middle/isq#EMMO_1604f495_328a_4f28_9962_f4cc210739dd> ,
                                                                                             <http://emmo.info/emmo/middle/isq#EMMO_f2ca6dd0_0e5f_4392_a92d_cafdae6cfc95> ;
                                                                             <http://emmo.info/emmo/middle/isq#EMMO_de178b12_5d35_4bca_8efa_a4193162571d> "T+1 L0 M0 I+1 T0 N0 J0" ;
                                                                             <http://emmo.info/emmo/top/annotations#EMMO_1f1b164d_ec6a_4faa_8d5e_88bda62316cc> "http://qudt.org/vocab/quantitykind/ElementaryCharge" ;
                                                                             <http://emmo.info/emmo/top/annotations#EMMO_6dd685dd_1895_46e4_b227_be9f7d643c25> "http://dbpedia.org/page/Elementary_charge" ;
                                                                             <http://emmo.info/emmo/top/annotations#EMMO_967080e5_2f42_4eb2_a3a9_c58143e835f9> "The magnitude of the electric charge carried by a single electron. It defines the base unit Ampere in the SI system."@en ;
                                                                             <http://emmo.info/emmo/top/annotations#EMMO_a9b3d04c_7ceb_40a2_b8d3_28d514a770a8> "https://physics.nist.gov/cgi-bin/cuu/Value?e" ;
                                                                             <http://emmo.info/emmo/top/annotations#EMMO_fe015383_afb3_44a6_ae86_043628697aa2> "https://doi.org/10.1351/goldbook.E02032" ;
                                                                             rdfs:comment "The DBpedia definition (http://dbpedia.org/page/Elementary_charge) is outdated as May 20, 2019. It is now an exact quantity."@en ;
                                                                             <http://www.w3.org/2004/02/skos/core#prefLabel> "ElementaryCharge"@en .


###  http://emmo.info/emmo/middle/isq#EMMO_5c003f53_20a2_4bd7_8445_58187e582578
<http://emmo.info/emmo/middle/isq#EMMO_5c003f53_20a2_4bd7_8445_58187e582578> rdf:type owl:Class ;
                                                                             rdfs:subClassOf <http://emmo.info/emmo/middle/metrology#EMMO_9895a1b4_f0a5_4167_ac5e_97db40b8bfcc> ;
                                                                             <http://www.w3.org/2004/02/skos/core#prefLabel> "LuminousEfficacyDimension"@en .


###  http://emmo.info/emmo/middle/isq#EMMO_5eedba4d_105b_44d8_b1bc_e33606276ea2
<http://emmo.info/emmo/middle/isq#EMMO_5eedba4d_105b_44d8_b1bc_e33606276ea2> rdf:type owl:Class ;
                                                                             rdfs:subClassOf <http://emmo.info/emmo/middle/isq#EMMO_faab3f84_e475_4a46_af9c_7d249f0b9aef> ;
                                                                             <http://emmo.info/emmo/middle/isq#EMMO_de178b12_5d35_4bca_8efa_a4193162571d> "T0 L0 M0 I0 T0 N0 J0" ;
                                                                             <http://emmo.info/emmo/top/annotations#EMMO_1f1b164d_ec6a_4faa_8d5e_88bda62316cc> "http://qudt.org/vocab/quantitykind/RefractiveIndex" ;
                                                                             <http://emmo.info/emmo/top/annotations#EMMO_6dd685dd_1895_46e4_b227_be9f7d643c25> "http://dbpedia.org/page/Refractive_index" ;
                                                                             <http://emmo.info/emmo/top/annotations#EMMO_fe015383_afb3_44a6_ae86_043628697aa2> "https://doi.org/10.1351/goldbook.R05240" ;
                                                                             rdfs:comment "Factor by which the phase velocity of light is reduced in a medium."@en ;
                                                                             <http://www.w3.org/2004/02/skos/core#prefLabel> "RefractiveIndex"@en .


###  http://emmo.info/emmo/middle/isq#EMMO_61a32ae9_8200_473a_bd55_59a9899996f4
<http://emmo.info/emmo/middle/isq#EMMO_61a32ae9_8200_473a_bd55_59a9899996f4> rdf:type owl:Class ;
                                                                             rdfs:subClassOf <http://emmo.info/emmo/middle/isq#EMMO_0ee5779e_d798_4ee5_9bfe_c392d5bea112> ,
                                                                                             <http://emmo.info/emmo/middle/metrology#EMMO_3f15d200_c97b_42c8_8ac0_d81d150361e2> ;
                                                                             <http://emmo.info/emmo/middle/isq#EMMO_de178b12_5d35_4bca_8efa_a4193162571d> "T+4 L-3 M-1 I+2 T0 N0 J0" ;
                                                                             <http://emmo.info/emmo/top/annotations#EMMO_1f1b164d_ec6a_4faa_8d5e_88bda62316cc> "http://qudt.org/vocab/constant/PermittivityOfVacuum" ;
                                                                             <http://emmo.info/emmo/top/annotations#EMMO_a9b3d04c_7ceb_40a2_b8d3_28d514a770a8> "https://physics.nist.gov/cgi-bin/cuu/Value?ep0" ;
                                                                             <http://emmo.info/emmo/top/annotations#EMMO_fe015383_afb3_44a6_ae86_043628697aa2> "https://doi.org/10.1351/goldbook.P04508" ;
                                                                             rdfs:comment "The DBpedia definition (http://dbpedia.org/page/Vacuum_permittivity) is outdated since May 20, 2019. It is now a measured constant."@en ,
                                                                                          "The value of the absolute dielectric permittivity of classical vacuum."@en ;
                                                                             <http://www.w3.org/2004/02/skos/core#prefLabel> "VacuumElectricPermittivity"@en .


###  http://emmo.info/emmo/middle/isq#EMMO_624d72ee_e676_4470_9434_c22b4190d3d5
<http://emmo.info/emmo/middle/isq#EMMO_624d72ee_e676_4470_9434_c22b4190d3d5> rdf:type owl:Class ;
                                                                             rdfs:subClassOf <http://emmo.info/emmo/middle/isq#EMMO_31ec09ba_1713_42cb_83c7_b38bf6f9ced2> ;
                                                                             <http://emmo.info/emmo/middle/isq#EMMO_de178b12_5d35_4bca_8efa_a4193162571d> "T-2 L+2 M+1 I0 T0 N0 J0" ;
                                                                             <http://emmo.info/emmo/top/annotations#EMMO_1f1b164d_ec6a_4faa_8d5e_88bda62316cc> "http://qudt.org/vocab/quantitykind/Work" ;
                                                                             <http://emmo.info/emmo/top/annotations#EMMO_6dd685dd_1895_46e4_b227_be9f7d643c25> "http://dbpedia.org/page/Heat" ,
                                                                                                                                                               "http://dbpedia.org/page/Work_(physics)" ;
                                                                             <http://emmo.info/emmo/top/annotations#EMMO_70fe84ff_99b6_4206_a9fc_9a8931836d84> "Product of force and displacement."@en ;
                                                                             <http://emmo.info/emmo/top/annotations#EMMO_fe015383_afb3_44a6_ae86_043628697aa2> "https://doi.org/10.1351/goldbook.W06684" ;
                                                                             <http://www.w3.org/2004/02/skos/core#prefLabel> "Work"@en .


###  http://emmo.info/emmo/middle/isq#EMMO_668e6ead_1530_40cc_ad5e_24b880edff50
<http://emmo.info/emmo/middle/isq#EMMO_668e6ead_1530_40cc_ad5e_24b880edff50> rdf:type owl:Class ;
                                                                             rdfs:subClassOf <http://emmo.info/emmo/middle/metrology#EMMO_9895a1b4_f0a5_4167_ac5e_97db40b8bfcc> ;
                                                                             <http://www.w3.org/2004/02/skos/core#prefLabel> "IlluminanceDimension"@en .


###  http://emmo.info/emmo/middle/isq#EMMO_66bc9029_f473_45ff_bab9_c3509ff37a22
<http://emmo.info/emmo/middle/isq#EMMO_66bc9029_f473_45ff_bab9_c3509ff37a22> rdf:type owl:Class ;
                                                                             rdfs:subClassOf <http://emmo.info/emmo/middle/isq#EMMO_2946d40b_24a1_47fa_8176_e3f79bb45064> ;
                                                                             <http://emmo.info/emmo/middle/isq#EMMO_de178b12_5d35_4bca_8efa_a4193162571d> "T-1 L0 M0 I0 T0 N+1 J0" ;
                                                                             <http://emmo.info/emmo/top/annotations#EMMO_6dd685dd_1895_46e4_b227_be9f7d643c25> "http://dbpedia.org/page/Temperature" ;
                                                                             <http://emmo.info/emmo/top/annotations#EMMO_967080e5_2f42_4eb2_a3a9_c58143e835f9> """An objective comparative measure of hot or cold. 

Temperature is a relative quantity that can be used to express temperature differences. Unlike ThermodynamicTemperature, it cannot express absolute temperatures."""@en ;
                                                                             <http://emmo.info/emmo/top/annotations#EMMO_fe015383_afb3_44a6_ae86_043628697aa2> "https://doi.org/10.1351/goldbook.T06261" ;
                                                                             <http://www.w3.org/2004/02/skos/core#prefLabel> "CelsiusTemperature"@en .


###  http://emmo.info/emmo/middle/isq#EMMO_66d01570_36dd_42fd_844d_29b81b029cd5
<http://emmo.info/emmo/middle/isq#EMMO_66d01570_36dd_42fd_844d_29b81b029cd5> rdf:type owl:Class ;
                                                                             rdfs:subClassOf <http://emmo.info/emmo/middle/isq#EMMO_2946d40b_24a1_47fa_8176_e3f79bb45064> ;
                                                                             <http://emmo.info/emmo/middle/isq#EMMO_de178b12_5d35_4bca_8efa_a4193162571d> "T-1 L+2 M+1 I0 T0 N0 J0" ;
                                                                             <http://emmo.info/emmo/top/annotations#EMMO_1f1b164d_ec6a_4faa_8d5e_88bda62316cc> "http://qudt.org/vocab/quantitykind/AngularMomentum" ;
                                                                             <http://emmo.info/emmo/top/annotations#EMMO_6dd685dd_1895_46e4_b227_be9f7d643c25> "http://dbpedia.org/page/Angular_momentum" ;
                                                                             <http://emmo.info/emmo/top/annotations#EMMO_fe015383_afb3_44a6_ae86_043628697aa2> "https://doi.org/10.1351/goldbook.A00353" ;
                                                                             rdfs:comment "Measure of the extent and direction an object rotates about a reference point."@en ;
                                                                             <http://www.w3.org/2004/02/skos/core#prefLabel> "AngularMomentum"@en .


###  http://emmo.info/emmo/middle/isq#EMMO_7610efb8_c7c6_4684_abc1_774783c62472
<http://emmo.info/emmo/middle/isq#EMMO_7610efb8_c7c6_4684_abc1_774783c62472> rdf:type owl:Class ;
                                                                             rdfs:subClassOf <http://emmo.info/emmo/middle/metrology#EMMO_9895a1b4_f0a5_4167_ac5e_97db40b8bfcc> ;
                                                                             <http://www.w3.org/2004/02/skos/core#prefLabel> "ElectricResistanceDimension"@en .


###  http://emmo.info/emmo/middle/isq#EMMO_76cc4efc_231e_42b4_be83_2547681caed6
<http://emmo.info/emmo/middle/isq#EMMO_76cc4efc_231e_42b4_be83_2547681caed6> rdf:type owl:Class ;
                                                                             rdfs:subClassOf <http://emmo.info/emmo/middle/isq#EMMO_66d01570_36dd_42fd_844d_29b81b029cd5> ,
                                                                                             <http://emmo.info/emmo/middle/isq#EMMO_f2ca6dd0_0e5f_4392_a92d_cafdae6cfc95> ;
                                                                             <http://emmo.info/emmo/middle/isq#EMMO_de178b12_5d35_4bca_8efa_a4193162571d> "T-1 L+2 M+1 I0 T0 N0 J0" ;
                                                                             <http://emmo.info/emmo/top/annotations#EMMO_1f1b164d_ec6a_4faa_8d5e_88bda62316cc> "http://qudt.org/vocab/constant/PlanckConstant" ;
                                                                             <http://emmo.info/emmo/top/annotations#EMMO_6dd685dd_1895_46e4_b227_be9f7d643c25> "http://dbpedia.org/page/Planck_constant" ;
                                                                             <http://emmo.info/emmo/top/annotations#EMMO_967080e5_2f42_4eb2_a3a9_c58143e835f9> "The quantum of action. It defines the kg base unit in the SI system."@en ;
                                                                             <http://emmo.info/emmo/top/annotations#EMMO_a9b3d04c_7ceb_40a2_b8d3_28d514a770a8> "https://physics.nist.gov/cgi-bin/cuu/Value?h" ;
                                                                             <http://emmo.info/emmo/top/annotations#EMMO_fe015383_afb3_44a6_ae86_043628697aa2> "https://doi.org/10.1351/goldbook.P04685" ;
                                                                             <http://www.w3.org/2004/02/skos/core#prefLabel> "PlanckConstant"@en .


###  http://emmo.info/emmo/middle/isq#EMMO_77e9dc31_5b19_463e_b000_44c6e79f98aa
<http://emmo.info/emmo/middle/isq#EMMO_77e9dc31_5b19_463e_b000_44c6e79f98aa> rdf:type owl:Class ;
                                                                             rdfs:subClassOf <http://emmo.info/emmo/middle/metrology#EMMO_9895a1b4_f0a5_4167_ac5e_97db40b8bfcc> ;
                                                                             <http://www.w3.org/2004/02/skos/core#prefLabel> "MassDimension"@en .


###  http://emmo.info/emmo/middle/isq#EMMO_79a02de5_b884_4eab_bc18_f67997d597a2
<http://emmo.info/emmo/middle/isq#EMMO_79a02de5_b884_4eab_bc18_f67997d597a2> rdf:type owl:Class ;
                                                                             rdfs:subClassOf <http://emmo.info/emmo/middle/isq#EMMO_e88f75d6_9a17_4cfc_bdf7_43d7cea5a9a1> ;
                                                                             <http://emmo.info/emmo/middle/isq#EMMO_de178b12_5d35_4bca_8efa_a4193162571d> "T-3 L+2 M+1 I-2 T0 N0 J0" ;
                                                                             <http://emmo.info/emmo/top/annotations#EMMO_1f1b164d_ec6a_4faa_8d5e_88bda62316cc> "http://qudt.org/vocab/quantitykind/Impedance" ;
                                                                             <http://emmo.info/emmo/top/annotations#EMMO_6dd685dd_1895_46e4_b227_be9f7d643c25> "http://dbpedia.org/page/Electrical_impedance" ;
                                                                             rdfs:comment "Measure of the opposition that a circuit presents to a current when a voltage is applied."@en ;
                                                                             <http://www.w3.org/2004/02/skos/core#altLabel> "Impedance" ;
                                                                             <http://www.w3.org/2004/02/skos/core#prefLabel> "ElectricImpedance"@en .


###  http://emmo.info/emmo/middle/isq#EMMO_7c055d65_2929_40e1_af4f_4bf10995ad50
<http://emmo.info/emmo/middle/isq#EMMO_7c055d65_2929_40e1_af4f_4bf10995ad50> rdf:type owl:Class ;
                                                                             rdfs:subClassOf <http://emmo.info/emmo/middle/chemistry#EMMO_a293f923_954c_4af5_9f97_9600ebd362cb> ,
                                                                                             <http://emmo.info/emmo/middle/isq#EMMO_faab3f84_e475_4a46_af9c_7d249f0b9aef> ;
                                                                             <http://emmo.info/emmo/middle/isq#EMMO_de178b12_5d35_4bca_8efa_a4193162571d> "T0 L0 M0 I0 T0 N0 J0" ;
                                                                             <http://emmo.info/emmo/top/annotations#EMMO_1f1b164d_ec6a_4faa_8d5e_88bda62316cc> "http://qudt.org/vocab/quantitykind/MassFraction" ;
                                                                             <http://emmo.info/emmo/top/annotations#EMMO_6dd685dd_1895_46e4_b227_be9f7d643c25> "http://dbpedia.org/page/Mass_fraction_(chemistry)" ;
                                                                             <http://emmo.info/emmo/top/annotations#EMMO_e55f2d7c_9893_48cd_b4a4_fdf38253bd20> "http://www.ontology-of-units-of-measure.org/resource/om-2/MassFraction" ;
                                                                             <http://emmo.info/emmo/top/annotations#EMMO_fe015383_afb3_44a6_ae86_043628697aa2> "https://doi.org/10.1351/goldbook.M03722" ;
                                                                             rdfs:comment "Mass of a constituent divided by the total mass of all constituents in the mixture."@en ;
                                                                             <http://www.w3.org/2004/02/skos/core#prefLabel> "MassFraction"@en .


###  http://emmo.info/emmo/middle/isq#EMMO_7c8007b0_58a7_4486_bf1c_4772852caca0
<http://emmo.info/emmo/middle/isq#EMMO_7c8007b0_58a7_4486_bf1c_4772852caca0> rdf:type owl:Class ;
                                                                             rdfs:subClassOf <http://emmo.info/emmo/middle/isq#EMMO_2946d40b_24a1_47fa_8176_e3f79bb45064> ;
                                                                             <http://emmo.info/emmo/middle/isq#EMMO_de178b12_5d35_4bca_8efa_a4193162571d> "T0 L-2 M0 I+1 T0 N0 J0" ;
                                                                             <http://emmo.info/emmo/top/annotations#EMMO_1f1b164d_ec6a_4faa_8d5e_88bda62316cc> "http://qudt.org/vocab/quantitykind/ElectricCurrentDensity" ;
                                                                             <http://emmo.info/emmo/top/annotations#EMMO_6dd685dd_1895_46e4_b227_be9f7d643c25> "http://dbpedia.org/page/Current_density" ;
                                                                             <http://emmo.info/emmo/top/annotations#EMMO_fe015383_afb3_44a6_ae86_043628697aa2> "https://doi.org/10.1351/goldbook.E01928" ;
                                                                             rdfs:comment "Electric current divided by the cross-sectional area it is passing through."@en ;
                                                                             <http://www.w3.org/2004/02/skos/core#prefLabel> "CurrentDensity"@en .


###  http://emmo.info/emmo/middle/isq#EMMO_81369540_1b0e_471b_9bae_6801af22800e
<http://emmo.info/emmo/middle/isq#EMMO_81369540_1b0e_471b_9bae_6801af22800e> rdf:type owl:Class ;
                                                                             rdfs:subClassOf <http://emmo.info/emmo/middle/isq#EMMO_2946d40b_24a1_47fa_8176_e3f79bb45064> ;
                                                                             <http://emmo.info/emmo/middle/isq#EMMO_de178b12_5d35_4bca_8efa_a4193162571d> "T-1 L+1 M0 I0 T0 N0 J0" ;
                                                                             <http://emmo.info/emmo/top/annotations#EMMO_1f1b164d_ec6a_4faa_8d5e_88bda62316cc> "http://qudt.org/vocab/quantitykind/Speed" ;
                                                                             <http://emmo.info/emmo/top/annotations#EMMO_6dd685dd_1895_46e4_b227_be9f7d643c25> "http://dbpedia.org/page/Speed" ;
                                                                             <http://emmo.info/emmo/top/annotations#EMMO_e55f2d7c_9893_48cd_b4a4_fdf38253bd20> "http://www.ontology-of-units-of-measure.org/resource/om-2/Speed" ;
                                                                             <http://emmo.info/emmo/top/annotations#EMMO_fe015383_afb3_44a6_ae86_043628697aa2> "https://doi.org/10.1351/goldbook.S05852" ;
                                                                             rdfs:comment """Length per unit time. 

Speed in the absolute value of the velocity."""@en ;
                                                                             <http://www.w3.org/2004/02/skos/core#prefLabel> "Speed"@en .


###  http://emmo.info/emmo/middle/isq#EMMO_8159c26a_494b_4fa0_9959_10888f152298
<http://emmo.info/emmo/middle/isq#EMMO_8159c26a_494b_4fa0_9959_10888f152298> rdf:type owl:Class ;
                                                                             rdfs:subClassOf <http://emmo.info/emmo/middle/isq#EMMO_1a4c1a97_88a7_4d8e_b2f9_2ca58e92dde4> ;
                                                                             <http://emmo.info/emmo/middle/isq#EMMO_de178b12_5d35_4bca_8efa_a4193162571d> "T0 L0 M0 I0 T0 N+1 J0" ;
                                                                             <http://emmo.info/emmo/top/annotations#EMMO_1f1b164d_ec6a_4faa_8d5e_88bda62316cc> "http://qudt.org/vocab/quantitykind/AmountOfSubstance" ;
                                                                             <http://emmo.info/emmo/top/annotations#EMMO_6dd685dd_1895_46e4_b227_be9f7d643c25> "http://dbpedia.org/page/Amount_of_substance" ;
                                                                             <http://emmo.info/emmo/top/annotations#EMMO_967080e5_2f42_4eb2_a3a9_c58143e835f9> "The number of elementary entities present."@en ;
                                                                             <http://emmo.info/emmo/top/annotations#EMMO_fe015383_afb3_44a6_ae86_043628697aa2> "https://doi.org/10.1351/goldbook.A00297" ;
                                                                             rdfs:comment """\"In the name amount of substance, the word substance will typically be replaced by words to specify the substance concerned in any particular application, for example amount of hydrogen chloride, HCl, or amount of benzene, C6H6 . It is important to give a precise definition of the entity involved (as emphasized in the definition of the mole); this should preferably be done by specifying the molecular chemical formula of the material involved. Although the word amount has a more general dictionary definition, the abbreviation of the full name amount of substance to amount may be used for brevity.\"

-- SI Brochure"""@en ;
                                                                             <http://www.w3.org/2004/02/skos/core#prefLabel> "AmountOfSubstance"@en .


###  http://emmo.info/emmo/middle/isq#EMMO_81e767f1_59b1_4d7a_bf69_17f322241831
<http://emmo.info/emmo/middle/isq#EMMO_81e767f1_59b1_4d7a_bf69_17f322241831> rdf:type owl:Class ;
                                                                             rdfs:subClassOf <http://emmo.info/emmo/middle/isq#EMMO_2946d40b_24a1_47fa_8176_e3f79bb45064> ;
                                                                             <http://emmo.info/emmo/middle/isq#EMMO_de178b12_5d35_4bca_8efa_a4193162571d> "T0 L+2 M0 I+1 T0 N0 J0" ;
                                                                             <http://emmo.info/emmo/top/annotations#EMMO_1f1b164d_ec6a_4faa_8d5e_88bda62316cc> "http://qudt.org/vocab/quantitykind/MagneticDipoleMoment" ;
                                                                             <http://emmo.info/emmo/top/annotations#EMMO_50c298c2_55a2_4068_b3ac_4e948c33181f> "http://www.electropedia.org/iev/iev.nsf/display?openform&ievref=121-11-55" ;
                                                                             <http://emmo.info/emmo/top/annotations#EMMO_6dd685dd_1895_46e4_b227_be9f7d643c25> "http://dbpedia.org/page/Magnetic_moment" ;
                                                                             <http://emmo.info/emmo/top/annotations#EMMO_8de5d5bf_db1c_40ac_b698_095ba3b18578> "10-9.1" ;
                                                                             <http://emmo.info/emmo/top/annotations#EMMO_967080e5_2f42_4eb2_a3a9_c58143e835f9> """Vector quantity  causing a change to its energy ?W in an external magnetic field of field flux density B:

    ?W = -  B"""@en ;
                                                                             <http://emmo.info/emmo/top/annotations#EMMO_fe015383_afb3_44a6_ae86_043628697aa2> "http://goldbook.iupac.org/terms/view/M03688" ;
                                                                             rdfs:comment """For an atom or nucleus, this energy is quantized and can be written as:

    W = g  M B

where g is the appropriate g factor,  is mostly the Bohr magneton or nuclear magneton, M is magnetic quantum number, and B is magnitude of the magnetic flux density.

-- ISO 80000"""@en ;
                                                                             <http://www.w3.org/2004/02/skos/core#prefLabel> "MagneticDipoleMoment"@en .


###  http://emmo.info/emmo/middle/isq#EMMO_830b59f7_d047_438c_90cd_62845749efcb
<http://emmo.info/emmo/middle/isq#EMMO_830b59f7_d047_438c_90cd_62845749efcb> rdf:type owl:Class ;
                                                                             rdfs:subClassOf <http://emmo.info/emmo/middle/isq#EMMO_31ec09ba_1713_42cb_83c7_b38bf6f9ced2> ;
                                                                             <http://emmo.info/emmo/middle/isq#EMMO_de178b12_5d35_4bca_8efa_a4193162571d> "T-2 L+2 M+1 I0 T0 N0 J0" ;
                                                                             <http://emmo.info/emmo/top/annotations#EMMO_1f1b164d_ec6a_4faa_8d5e_88bda62316cc> "http://qudt.org/vocab/quantitykind/InternalEnergy" ;
                                                                             <http://emmo.info/emmo/top/annotations#EMMO_50c298c2_55a2_4068_b3ac_4e948c33181f> "http://www.electropedia.org/iev/iev.nsf/display?openform&ievref=113-04-20" ;
                                                                             <http://emmo.info/emmo/top/annotations#EMMO_6dd685dd_1895_46e4_b227_be9f7d643c25> "http://dbpedia.org/page/Internal_energy" ;
                                                                             <http://emmo.info/emmo/top/annotations#EMMO_967080e5_2f42_4eb2_a3a9_c58143e835f9> "A state quantity equal to the difference between the total energy of a system and the sum of the macroscopic kinetic and potential energies of the system."@en ;
                                                                             <http://emmo.info/emmo/top/annotations#EMMO_e55f2d7c_9893_48cd_b4a4_fdf38253bd20> "http://www.ontology-of-units-of-measure.org/resource/om-2/InternalEnergy" ;
                                                                             <http://emmo.info/emmo/top/annotations#EMMO_fe015383_afb3_44a6_ae86_043628697aa2> "https://doi.org/10.1351/goldbook.I03103" ;
                                                                             <http://www.w3.org/2004/02/skos/core#altLabel> "ThermodynamicEnergy"@en ;
                                                                             <http://www.w3.org/2004/02/skos/core#prefLabel> "InternalEnergy"@en .


###  http://emmo.info/emmo/middle/isq#EMMO_847f1d9f_205e_46c1_8cb6_a9e479421f88
<http://emmo.info/emmo/middle/isq#EMMO_847f1d9f_205e_46c1_8cb6_a9e479421f88> rdf:type owl:Class ;
                                                                             rdfs:subClassOf <http://emmo.info/emmo/middle/metrology#EMMO_9895a1b4_f0a5_4167_ac5e_97db40b8bfcc> ;
                                                                             <http://www.w3.org/2004/02/skos/core#prefLabel> "AbsorbedDoseDimension"@en .


###  http://emmo.info/emmo/middle/isq#EMMO_852b4ab8_fc29_4749_a8c7_b92d4fca7d5a
<http://emmo.info/emmo/middle/isq#EMMO_852b4ab8_fc29_4749_a8c7_b92d4fca7d5a> rdf:type owl:Class ;
                                                                             rdfs:subClassOf <http://emmo.info/emmo/middle/isq#EMMO_2946d40b_24a1_47fa_8176_e3f79bb45064> ;
                                                                             <http://emmo.info/emmo/middle/isq#EMMO_de178b12_5d35_4bca_8efa_a4193162571d> "T-1 L0 M0 I0 T0 N0 J0" ;
                                                                             <http://emmo.info/emmo/top/annotations#EMMO_1f1b164d_ec6a_4faa_8d5e_88bda62316cc> "http://qudt.org/vocab/quantitykind/Frequency" ;
                                                                             <http://emmo.info/emmo/top/annotations#EMMO_6dd685dd_1895_46e4_b227_be9f7d643c25> "http://dbpedia.org/page/Frequency" ;
                                                                             <http://emmo.info/emmo/top/annotations#EMMO_967080e5_2f42_4eb2_a3a9_c58143e835f9> "Number of periods per time interval."@en ;
                                                                             <http://emmo.info/emmo/top/annotations#EMMO_fe015383_afb3_44a6_ae86_043628697aa2> "https://doi.org/10.1351/goldbook.FT07383" ;
                                                                             <http://www.w3.org/2004/02/skos/core#prefLabel> "Frequency"@en .


###  http://emmo.info/emmo/middle/isq#EMMO_88fc5d1b_d3ab_4626_b24c_915ebe7400ca
<http://emmo.info/emmo/middle/isq#EMMO_88fc5d1b_d3ab_4626_b24c_915ebe7400ca> rdf:type owl:Class ;
                                                                             rdfs:subClassOf <http://emmo.info/emmo/middle/isq#EMMO_2946d40b_24a1_47fa_8176_e3f79bb45064> ;
                                                                             <http://emmo.info/emmo/middle/isq#EMMO_de178b12_5d35_4bca_8efa_a4193162571d> "T-2 L+2 M+1 I0 T0 N-1 J0" ;
                                                                             <http://emmo.info/emmo/top/annotations#EMMO_1f1b164d_ec6a_4faa_8d5e_88bda62316cc> "http://qudt.org/vocab/quantitykind/ChemicalPotential" ;
                                                                             <http://emmo.info/emmo/top/annotations#EMMO_6dd685dd_1895_46e4_b227_be9f7d643c25> "http://dbpedia.org/page/Chemical_potential" ;
                                                                             <http://emmo.info/emmo/top/annotations#EMMO_fe015383_afb3_44a6_ae86_043628697aa2> "https://doi.org/10.1351/goldbook.C01032" ;
                                                                             rdfs:comment "Energy per unit change in amount of substance."@en ;
                                                                             <http://www.w3.org/2004/02/skos/core#prefLabel> "ChemicalPotential"@en .


###  http://emmo.info/emmo/middle/isq#EMMO_8d3da9ac_2265_4382_bee5_db72046722f8
<http://emmo.info/emmo/middle/isq#EMMO_8d3da9ac_2265_4382_bee5_db72046722f8> rdf:type owl:Class ;
                                                                             rdfs:subClassOf <http://emmo.info/emmo/middle/isq#EMMO_2946d40b_24a1_47fa_8176_e3f79bb45064> ;
                                                                             <http://emmo.info/emmo/middle/isq#EMMO_de178b12_5d35_4bca_8efa_a4193162571d> "T-1 L0 M0 I0 T0 N0 J0" ;
                                                                             <http://emmo.info/emmo/top/annotations#EMMO_1f1b164d_ec6a_4faa_8d5e_88bda62316cc> "http://qudt.org/vocab/quantitykind/SpecificActivity" ;
                                                                             <http://emmo.info/emmo/top/annotations#EMMO_967080e5_2f42_4eb2_a3a9_c58143e835f9> "Decays per unit time."@en ;
                                                                             <http://emmo.info/emmo/top/annotations#EMMO_fe015383_afb3_44a6_ae86_043628697aa2> "https://doi.org/10.1351/goldbook.A00114" ;
                                                                             <http://www.w3.org/2004/02/skos/core#prefLabel> "Radioactivity"@en .


###  http://emmo.info/emmo/middle/isq#EMMO_8d689295_7d84_421b_bc01_d5cceb2c2086
<http://emmo.info/emmo/middle/isq#EMMO_8d689295_7d84_421b_bc01_d5cceb2c2086> rdf:type owl:Class ;
                                                                             rdfs:subClassOf <http://emmo.info/emmo/middle/isq#EMMO_ed4af7ae_63a2_497e_bb88_2309619ea405> ,
                                                                                             <http://emmo.info/emmo/middle/metrology#EMMO_3f15d200_c97b_42c8_8ac0_d81d150361e2> ;
                                                                             <http://emmo.info/emmo/middle/isq#EMMO_de178b12_5d35_4bca_8efa_a4193162571d> "T0 L0 M+1 I0 T0 N0 J0" ;
                                                                             <http://emmo.info/emmo/top/annotations#EMMO_1f1b164d_ec6a_4faa_8d5e_88bda62316cc> "http://qudt.org/vocab/constant/ProtonMass" ;
                                                                             <http://emmo.info/emmo/top/annotations#EMMO_a9b3d04c_7ceb_40a2_b8d3_28d514a770a8> "https://physics.nist.gov/cgi-bin/cuu/Value?mp" ;
                                                                             <http://emmo.info/emmo/top/annotations#EMMO_fe015383_afb3_44a6_ae86_043628697aa2> "https://doi.org/10.1351/goldbook.P04914" ;
                                                                             rdfs:comment "The rest mass of a proton."@en ;
                                                                             <http://www.w3.org/2004/02/skos/core#prefLabel> "ProtonMass"@en .


###  http://emmo.info/emmo/middle/isq#EMMO_8e5dd473_808b_4a8a_b7cd_63068c12ff57
<http://emmo.info/emmo/middle/isq#EMMO_8e5dd473_808b_4a8a_b7cd_63068c12ff57> rdf:type owl:Class ;
                                                                             rdfs:subClassOf <http://emmo.info/emmo/middle/isq#EMMO_2946d40b_24a1_47fa_8176_e3f79bb45064> ;
                                                                             <http://emmo.info/emmo/middle/isq#EMMO_de178b12_5d35_4bca_8efa_a4193162571d> "T-2 L+2 M0 I0 T0 N0 J0" ;
                                                                             <http://emmo.info/emmo/top/annotations#EMMO_1f1b164d_ec6a_4faa_8d5e_88bda62316cc> "http://qudt.org/vocab/quantitykind/AbsorbedDose" ;
                                                                             <http://emmo.info/emmo/top/annotations#EMMO_6dd685dd_1895_46e4_b227_be9f7d643c25> "http://dbpedia.org/page/Absorbed_dose" ;
                                                                             <http://emmo.info/emmo/top/annotations#EMMO_70fe84ff_99b6_4206_a9fc_9a8931836d84> "Energy imparted to matter by ionizing radiation in a suitable small element of volume divided by the mass of that element of volume."@en ;
                                                                             <http://emmo.info/emmo/top/annotations#EMMO_fe015383_afb3_44a6_ae86_043628697aa2> "https://doi.org/10.1351/goldbook.A00031" ;
                                                                             <http://www.w3.org/2004/02/skos/core#prefLabel> "AbsorbedDose"@en .


###  http://emmo.info/emmo/middle/isq#EMMO_9141801c_c539_4c72_b423_8c74ff6b8f05
<http://emmo.info/emmo/middle/isq#EMMO_9141801c_c539_4c72_b423_8c74ff6b8f05> rdf:type owl:Class ;
                                                                             rdfs:subClassOf <http://emmo.info/emmo/middle/metrology#EMMO_9895a1b4_f0a5_4167_ac5e_97db40b8bfcc> ;
                                                                             <http://www.w3.org/2004/02/skos/core#prefLabel> "VolumeDimension"@en .


###  http://emmo.info/emmo/middle/isq#EMMO_92b2fb85_2143_4bc7_bbca_df3e6944bfc1
<http://emmo.info/emmo/middle/isq#EMMO_92b2fb85_2143_4bc7_bbca_df3e6944bfc1> rdf:type owl:Class ;
                                                                             rdfs:subClassOf <http://emmo.info/emmo/middle/isq#EMMO_e88f75d6_9a17_4cfc_bdf7_43d7cea5a9a1> ;
                                                                             <http://emmo.info/emmo/middle/isq#EMMO_de178b12_5d35_4bca_8efa_a4193162571d> "T-3 L+2 M+1 I-2 T0 N0 J0" ;
                                                                             <http://emmo.info/emmo/top/annotations#EMMO_1f1b164d_ec6a_4faa_8d5e_88bda62316cc> "http://qudt.org/vocab/quantitykind/Reactance" ;
                                                                             <http://emmo.info/emmo/top/annotations#EMMO_6dd685dd_1895_46e4_b227_be9f7d643c25> "http://dbpedia.org/page/Electrical_reactance" ;
                                                                             rdfs:comment "The opposition of a circuit element to a change in current or voltage, due to that element's inductance or capacitance."@en ;
                                                                             <http://www.w3.org/2004/02/skos/core#altLabel> "Reactance" ;
                                                                             <http://www.w3.org/2004/02/skos/core#prefLabel> "ElectricReactance"@en .


###  http://emmo.info/emmo/middle/isq#EMMO_961d1aba_f75e_4411_aaa4_457f7516ed6b
<http://emmo.info/emmo/middle/isq#EMMO_961d1aba_f75e_4411_aaa4_457f7516ed6b> rdf:type owl:Class ;
                                                                             rdfs:subClassOf <http://emmo.info/emmo/middle/isq#EMMO_2946d40b_24a1_47fa_8176_e3f79bb45064> ;
                                                                             <http://emmo.info/emmo/middle/isq#EMMO_de178b12_5d35_4bca_8efa_a4193162571d> "T-2 L0 M+1 I-1 T0 N0 J0" ;
                                                                             <http://emmo.info/emmo/top/annotations#EMMO_1f1b164d_ec6a_4faa_8d5e_88bda62316cc> "http://qudt.org/vocab/quantitykind/MagneticFluxDensity" ;
                                                                             <http://emmo.info/emmo/top/annotations#EMMO_6dd685dd_1895_46e4_b227_be9f7d643c25> "http://dbpedia.org/page/Magnetic_field" ;
                                                                             <http://emmo.info/emmo/top/annotations#EMMO_967080e5_2f42_4eb2_a3a9_c58143e835f9> "Strength of the magnetic field."@en ;
                                                                             <http://emmo.info/emmo/top/annotations#EMMO_fe015383_afb3_44a6_ae86_043628697aa2> "https://doi.org/10.1351/goldbook.M03686" ;
                                                                             rdfs:comment "Often denoted B."@en ;
                                                                             <http://www.w3.org/2004/02/skos/core#prefLabel> "MagneticFluxDensity"@en .


###  http://emmo.info/emmo/middle/isq#EMMO_96f39f77_44dc_491b_8fa7_30d887fe0890
<http://emmo.info/emmo/middle/isq#EMMO_96f39f77_44dc_491b_8fa7_30d887fe0890> rdf:type owl:Class ;
                                                                             rdfs:subClassOf <http://emmo.info/emmo/middle/isq#EMMO_2946d40b_24a1_47fa_8176_e3f79bb45064> ;
                                                                             <http://emmo.info/emmo/middle/isq#EMMO_de178b12_5d35_4bca_8efa_a4193162571d> "T0 L+2 M0 I0 T0 N0 J0" ;
                                                                             <http://emmo.info/emmo/top/annotations#EMMO_1f1b164d_ec6a_4faa_8d5e_88bda62316cc> "http://qudt.org/vocab/quantitykind/Area" ;
                                                                             <http://emmo.info/emmo/top/annotations#EMMO_6dd685dd_1895_46e4_b227_be9f7d643c25> "http://dbpedia.org/page/Area" ;
                                                                             <http://emmo.info/emmo/top/annotations#EMMO_fe015383_afb3_44a6_ae86_043628697aa2> "https://doi.org/10.1351/goldbook.A00429" ;
                                                                             rdfs:comment "Extent of a surface."@en ;
                                                                             <http://www.w3.org/2004/02/skos/core#prefLabel> "Area"@en .


###  http://emmo.info/emmo/middle/isq#EMMO_97589322_710c_4af4_9431_1e5027f2be42
<http://emmo.info/emmo/middle/isq#EMMO_97589322_710c_4af4_9431_1e5027f2be42> rdf:type owl:Class ;
                                                                             rdfs:subClassOf <http://emmo.info/emmo/middle/isq#EMMO_2946d40b_24a1_47fa_8176_e3f79bb45064> ;
                                                                             <http://emmo.info/emmo/middle/isq#EMMO_de178b12_5d35_4bca_8efa_a4193162571d> "T0 L-2 M0 I0 T0 N0 J+1" ;
                                                                             <http://emmo.info/emmo/top/annotations#EMMO_1f1b164d_ec6a_4faa_8d5e_88bda62316cc> "http://qudt.org/vocab/quantitykind/Luminance" ;
                                                                             <http://emmo.info/emmo/top/annotations#EMMO_6dd685dd_1895_46e4_b227_be9f7d643c25> "http://dbpedia.org/page/Luminance" ;
                                                                             <http://emmo.info/emmo/top/annotations#EMMO_fe015383_afb3_44a6_ae86_043628697aa2> "https://doi.org/10.1351/goldbook.L03640" ;
                                                                             rdfs:comment "Measured in cd/m. Not to confuse with Illuminance, which is measured in lux (cd sr/m)."@en ,
                                                                                          "a photometric measure of the luminous intensity per unit area of light travelling in a given direction."@en ;
                                                                             <http://www.w3.org/2004/02/skos/core#prefLabel> "Luminance"@en .


###  http://emmo.info/emmo/middle/isq#EMMO_99296e55_53f7_4333_9e06_760ad175a1b9
<http://emmo.info/emmo/middle/isq#EMMO_99296e55_53f7_4333_9e06_760ad175a1b9> rdf:type owl:Class ;
                                                                             rdfs:subClassOf <http://emmo.info/emmo/middle/isq#EMMO_81369540_1b0e_471b_9bae_6801af22800e> ,
                                                                                             <http://emmo.info/emmo/middle/isq#EMMO_f2ca6dd0_0e5f_4392_a92d_cafdae6cfc95> ;
                                                                             <http://emmo.info/emmo/middle/isq#EMMO_de178b12_5d35_4bca_8efa_a4193162571d> "T-1 L+1 M0 I0 T0 N0 J0" ;
                                                                             <http://emmo.info/emmo/top/annotations#EMMO_1f1b164d_ec6a_4faa_8d5e_88bda62316cc> "http://qudt.org/vocab/constant/SpeedOfLight_Vacuum" ;
                                                                             <http://emmo.info/emmo/top/annotations#EMMO_6dd685dd_1895_46e4_b227_be9f7d643c25> "http://dbpedia.org/page/Speed_of_light" ;
                                                                             <http://emmo.info/emmo/top/annotations#EMMO_967080e5_2f42_4eb2_a3a9_c58143e835f9> "The speed of light in vacuum. Defines the base unit metre in the SI system."@en ;
                                                                             <http://emmo.info/emmo/top/annotations#EMMO_a9b3d04c_7ceb_40a2_b8d3_28d514a770a8> "https://physics.nist.gov/cgi-bin/cuu/Value?c" ;
                                                                             <http://emmo.info/emmo/top/annotations#EMMO_fe015383_afb3_44a6_ae86_043628697aa2> "https://doi.org/10.1351/goldbook.S05854" ;
                                                                             <http://www.w3.org/2004/02/skos/core#prefLabel> "SpeedOfLightInVacuum"@en .


###  http://emmo.info/emmo/middle/isq#EMMO_99dba333_0dbd_4f75_8841_8c0f97fd58e2
<http://emmo.info/emmo/middle/isq#EMMO_99dba333_0dbd_4f75_8841_8c0f97fd58e2> rdf:type owl:Class ;
                                                                             rdfs:subClassOf <http://emmo.info/emmo/middle/isq#EMMO_2946d40b_24a1_47fa_8176_e3f79bb45064> ;
                                                                             <http://emmo.info/emmo/middle/isq#EMMO_de178b12_5d35_4bca_8efa_a4193162571d> "T+4 L-2 M-1 I+2 T0 N0 J0" ;
                                                                             <http://emmo.info/emmo/top/annotations#EMMO_1f1b164d_ec6a_4faa_8d5e_88bda62316cc> "http://qudt.org/vocab/quantitykind/Capacitance" ;
                                                                             <http://emmo.info/emmo/top/annotations#EMMO_6dd685dd_1895_46e4_b227_be9f7d643c25> "http://dbpedia.org/page/Capacitance" ;
                                                                             <http://emmo.info/emmo/top/annotations#EMMO_967080e5_2f42_4eb2_a3a9_c58143e835f9> "The derivative of the electric charge of a system with respect to the electric potential."@en ;
                                                                             <http://emmo.info/emmo/top/annotations#EMMO_fe015383_afb3_44a6_ae86_043628697aa2> "https://doi.org/10.1351/goldbook.C00791" ;
                                                                             <http://www.w3.org/2004/02/skos/core#altLabel> "ElectricCapacitance"@en ;
                                                                             <http://www.w3.org/2004/02/skos/core#prefLabel> "Capacitance"@en .


###  http://emmo.info/emmo/middle/isq#EMMO_9bbab0be_f9cc_4f46_9f46_0fd271911b79
<http://emmo.info/emmo/middle/isq#EMMO_9bbab0be_f9cc_4f46_9f46_0fd271911b79> rdf:type owl:Class ;
                                                                             rdfs:subClassOf <http://emmo.info/emmo/middle/isq#EMMO_2946d40b_24a1_47fa_8176_e3f79bb45064> ;
                                                                             <http://emmo.info/emmo/middle/isq#EMMO_de178b12_5d35_4bca_8efa_a4193162571d> "T-2 L+2 M+1 I0 T-1 N0 J0" ;
                                                                             <http://emmo.info/emmo/top/annotations#EMMO_1f1b164d_ec6a_4faa_8d5e_88bda62316cc> "http://qudt.org/vocab/quantitykind/Entropy" ;
                                                                             <http://emmo.info/emmo/top/annotations#EMMO_6dd685dd_1895_46e4_b227_be9f7d643c25> "http://dbpedia.org/page/Entropy" ;
                                                                             <http://emmo.info/emmo/top/annotations#EMMO_fe015383_afb3_44a6_ae86_043628697aa2> "https://doi.org/10.1351/goldbook.E02149" ;
                                                                             rdfs:comment "Logarithmic measure of the number of available states of a system."@en ,
                                                                                          "May also be referred to as a measure of order of  a system."@en ;
                                                                             <http://www.w3.org/2004/02/skos/core#prefLabel> "Entropy"@en .


###  http://emmo.info/emmo/middle/isq#EMMO_9d8f708a_f291_4d72_80ec_362c6e6bbca6
<http://emmo.info/emmo/middle/isq#EMMO_9d8f708a_f291_4d72_80ec_362c6e6bbca6> rdf:type owl:Class ;
                                                                             rdfs:subClassOf <http://emmo.info/emmo/middle/isq#EMMO_44da6d75_54a4_4aa8_bd3a_156f6e9abb8e> ;
                                                                             <http://emmo.info/emmo/middle/isq#EMMO_de178b12_5d35_4bca_8efa_a4193162571d> "T0 L+1 M0 I0 T0 N0 J0" ;
                                                                             <http://emmo.info/emmo/top/annotations#EMMO_50c298c2_55a2_4068_b3ac_4e948c33181f> "http://www.electropedia.org/iev/iev.nsf/display?openform&ievref=113-03-12" ;
                                                                             <http://emmo.info/emmo/top/annotations#EMMO_6dd685dd_1895_46e4_b227_be9f7d643c25> "http://dbpedia.org/page/Center_of_mass" ;
                                                                             <http://emmo.info/emmo/top/annotations#EMMO_967080e5_2f42_4eb2_a3a9_c58143e835f9> "The unique point where the weighted relative position of the distributed mass of an Item sums to zero. Equivalently, it is the point where if a force is applied to the Item, causes the Item to move in direction of force without rotation."@en ;
                                                                             <http://emmo.info/emmo/top/annotations#EMMO_c84c6752_6d64_48cc_9500_e54a3c34898d> "https://en.wikipedia.org/wiki/Center_of_mass" ;
                                                                             rdfs:comment "In non-relativistic physics, the centre of mass doesnt depend on the chosen reference frame."@en ;
                                                                             <http://www.w3.org/2004/02/skos/core#prefLabel> "CentreOfMass"@en .


###  http://emmo.info/emmo/middle/isq#EMMO_a3c78d6f_ae49_47c8_a634_9b6d86b79382
<http://emmo.info/emmo/middle/isq#EMMO_a3c78d6f_ae49_47c8_a634_9b6d86b79382> rdf:type owl:Class ;
                                                                             rdfs:subClassOf <http://emmo.info/emmo/middle/isq#EMMO_d859588d_44dc_4614_bc75_5fcd0058acc8> ,
                                                                                             <http://emmo.info/emmo/middle/metrology#EMMO_3f15d200_c97b_42c8_8ac0_d81d150361e2> ;
                                                                             <http://emmo.info/emmo/middle/isq#EMMO_de178b12_5d35_4bca_8efa_a4193162571d> "T0 L-1 M0 I0 T0 N0 J0" ;
                                                                             <http://emmo.info/emmo/top/annotations#EMMO_1f1b164d_ec6a_4faa_8d5e_88bda62316cc> "http://qudt.org/vocab/constant/RydbergConstant" ;
                                                                             <http://emmo.info/emmo/top/annotations#EMMO_6dd685dd_1895_46e4_b227_be9f7d643c25> "http://dbpedia.org/page/Rydberg_constant" ;
                                                                             <http://emmo.info/emmo/top/annotations#EMMO_a9b3d04c_7ceb_40a2_b8d3_28d514a770a8> "https://physics.nist.gov/cgi-bin/cuu/Value?ryd" ;
                                                                             <http://emmo.info/emmo/top/annotations#EMMO_fe015383_afb3_44a6_ae86_043628697aa2> "https://doi.org/10.1351/goldbook.R05430" ;
                                                                             rdfs:comment "The Rydberg constant represents the limiting value of the highest wavenumber (the inverse wavelength) of any photon that can be emitted from the hydrogen atom, or, alternatively, the wavenumber of the lowest-energy photon capable of ionizing the hydrogen atom from its ground state."@en ;
                                                                             <http://www.w3.org/2004/02/skos/core#prefLabel> "RybergConstant"@en .


###  http://emmo.info/emmo/middle/isq#EMMO_a66427d1_9932_4363_9ec5_7d91f2bfda1e
<http://emmo.info/emmo/middle/isq#EMMO_a66427d1_9932_4363_9ec5_7d91f2bfda1e> rdf:type owl:Class ;
                                                                             rdfs:subClassOf <http://emmo.info/emmo/middle/isq#EMMO_2946d40b_24a1_47fa_8176_e3f79bb45064> ;
                                                                             <http://emmo.info/emmo/middle/isq#EMMO_de178b12_5d35_4bca_8efa_a4193162571d> "T0 L0 M0 I0 T0 N0 J0" ;
                                                                             <http://emmo.info/emmo/top/annotations#EMMO_6dd685dd_1895_46e4_b227_be9f7d643c25> "http://dbpedia.org/page/Dimensionless_quantity" ;
                                                                             <http://emmo.info/emmo/top/annotations#EMMO_967080e5_2f42_4eb2_a3a9_c58143e835f9> "A quantity to which no physical dimension is assigned and with a corresponding unit of measurement in the SI of the unit one."@en ;
                                                                             <http://emmo.info/emmo/top/annotations#EMMO_c84c6752_6d64_48cc_9500_e54a3c34898d> "https://en.wikipedia.org/wiki/Dimensionless_quantity" ;
                                                                             <http://emmo.info/emmo/top/annotations#EMMO_fe015383_afb3_44a6_ae86_043628697aa2> "https://doi.org/10.1351/goldbook.D01742" ;
                                                                             <http://www.w3.org/2004/02/skos/core#prefLabel> "ISQDimensionlessQuantity"@en .


###  http://emmo.info/emmo/middle/isq#EMMO_a77a0a4b_6bd2_42b2_be27_4b63cebbb59e
<http://emmo.info/emmo/middle/isq#EMMO_a77a0a4b_6bd2_42b2_be27_4b63cebbb59e> rdf:type owl:Class ;
                                                                             rdfs:subClassOf <http://emmo.info/emmo/middle/metrology#EMMO_9895a1b4_f0a5_4167_ac5e_97db40b8bfcc> ;
                                                                             <http://www.w3.org/2004/02/skos/core#prefLabel> "TemperatureDimension"@en .


###  http://emmo.info/emmo/middle/isq#EMMO_a8eb87b5_4d10_4137_a75c_e04ee59ca095
<http://emmo.info/emmo/middle/isq#EMMO_a8eb87b5_4d10_4137_a75c_e04ee59ca095> rdf:type owl:Class ;
                                                                             rdfs:subClassOf <http://emmo.info/emmo/middle/chemistry#EMMO_a293f923_954c_4af5_9f97_9600ebd362cb> ,
                                                                                             <http://emmo.info/emmo/middle/isq#EMMO_faab3f84_e475_4a46_af9c_7d249f0b9aef> ;
                                                                             <http://emmo.info/emmo/middle/isq#EMMO_de178b12_5d35_4bca_8efa_a4193162571d> "T0 L0 M0 I0 T0 N0 J0" ;
                                                                             <http://emmo.info/emmo/top/annotations#EMMO_1f1b164d_ec6a_4faa_8d5e_88bda62316cc> "http://qudt.org/vocab/quantitykind/VolumeFraction" ;
                                                                             <http://emmo.info/emmo/top/annotations#EMMO_6dd685dd_1895_46e4_b227_be9f7d643c25> "http://dbpedia.org/page/Volume_fraction"@en ;
                                                                             <http://emmo.info/emmo/top/annotations#EMMO_967080e5_2f42_4eb2_a3a9_c58143e835f9> "Volume of a constituent of a mixture divided by the sum of volumes of all constituents prior to mixing."@en ;
                                                                             <http://emmo.info/emmo/top/annotations#EMMO_e55f2d7c_9893_48cd_b4a4_fdf38253bd20> "http://www.ontology-of-units-of-measure.org/resource/om-2/VolumeFraction"@en ;
                                                                             <http://emmo.info/emmo/top/annotations#EMMO_fe015383_afb3_44a6_ae86_043628697aa2> "https://doi.org/10.1351/goldbook.V06643"@en ;
                                                                             <http://www.w3.org/2004/02/skos/core#prefLabel> "VolumeFraction"@en .


###  http://emmo.info/emmo/middle/isq#EMMO_aaf9dd7f_0474_40d0_9606_02def8515249
<http://emmo.info/emmo/middle/isq#EMMO_aaf9dd7f_0474_40d0_9606_02def8515249> rdf:type owl:Class ;
                                                                             rdfs:subClassOf <http://emmo.info/emmo/middle/isq#EMMO_2946d40b_24a1_47fa_8176_e3f79bb45064> ;
                                                                             <http://emmo.info/emmo/middle/isq#EMMO_de178b12_5d35_4bca_8efa_a4193162571d> "T-2 L+2 M+1 I0 T0 N0 J0" ;
                                                                             <http://emmo.info/emmo/top/annotations#EMMO_1f1b164d_ec6a_4faa_8d5e_88bda62316cc> "http://qudt.org/vocab/quantitykind/Torque" ;
                                                                             <http://emmo.info/emmo/top/annotations#EMMO_50c298c2_55a2_4068_b3ac_4e948c33181f> "http://www.electropedia.org/iev/iev.nsf/display?openform&ievref=113-03-26" ;
                                                                             <http://emmo.info/emmo/top/annotations#EMMO_6dd685dd_1895_46e4_b227_be9f7d643c25> "http://dbpedia.org/page/Torque" ;
                                                                             <http://emmo.info/emmo/top/annotations#EMMO_967080e5_2f42_4eb2_a3a9_c58143e835f9> "The effectiveness of a force to produce rotation about an axis, measured by the product of the force and the perpendicular distance from the line of action of the force to the axis."@en ;
                                                                             <http://emmo.info/emmo/top/annotations#EMMO_e55f2d7c_9893_48cd_b4a4_fdf38253bd20> "http://www.ontology-of-units-of-measure.org/resource/om-2/Torque" ;
                                                                             <http://emmo.info/emmo/top/annotations#EMMO_fe015383_afb3_44a6_ae86_043628697aa2> "https://doi.org/10.1351/goldbook.T06400" ;
                                                                             rdfs:comment "Even though torque has the same physical dimension as energy, it is not of the same kind and can not be measured with energy units like joule or electron volt."@en ;
                                                                             <http://www.w3.org/2004/02/skos/core#prefLabel> "Torque"@en .


###  http://emmo.info/emmo/middle/isq#EMMO_ab79e92b_5377_454d_be06_d61b50db295a
<http://emmo.info/emmo/middle/isq#EMMO_ab79e92b_5377_454d_be06_d61b50db295a> rdf:type owl:Class ;
                                                                             rdfs:subClassOf <http://emmo.info/emmo/middle/metrology#EMMO_9895a1b4_f0a5_4167_ac5e_97db40b8bfcc> ;
                                                                             <http://www.w3.org/2004/02/skos/core#prefLabel> "ElectricChargeDimension"@en .


###  http://emmo.info/emmo/middle/isq#EMMO_ac540a9d_0131_43f6_a33b_17e5cfc432ed
<http://emmo.info/emmo/middle/isq#EMMO_ac540a9d_0131_43f6_a33b_17e5cfc432ed> rdf:type owl:Class ;
                                                                             rdfs:subClassOf <http://emmo.info/emmo/middle/isq#EMMO_31ec09ba_1713_42cb_83c7_b38bf6f9ced2> ;
                                                                             <http://emmo.info/emmo/middle/isq#EMMO_de178b12_5d35_4bca_8efa_a4193162571d> "T-2 L+2 M+1 I0 T0 N0 J0" ;
                                                                             <http://emmo.info/emmo/top/annotations#EMMO_1f1b164d_ec6a_4faa_8d5e_88bda62316cc> "http://qudt.org/vocab/quantitykind/KineticEnergy" ;
                                                                             <http://emmo.info/emmo/top/annotations#EMMO_50c298c2_55a2_4068_b3ac_4e948c33181f> "http://www.electropedia.org/iev/iev.nsf/display?openform&ievref=113-03-49" ;
                                                                             <http://emmo.info/emmo/top/annotations#EMMO_6dd685dd_1895_46e4_b227_be9f7d643c25> "http://dbpedia.org/page/Kinetic_energy" ;
                                                                             <http://emmo.info/emmo/top/annotations#EMMO_967080e5_2f42_4eb2_a3a9_c58143e835f9> "The energy of an object due to its motion."@en ;
                                                                             <http://emmo.info/emmo/top/annotations#EMMO_e55f2d7c_9893_48cd_b4a4_fdf38253bd20> "http://www.ontology-of-units-of-measure.org/resource/om-2/KineticEnergy" ;
                                                                             <http://emmo.info/emmo/top/annotations#EMMO_fe015383_afb3_44a6_ae86_043628697aa2> "https://doi.org/10.1351/goldbook.K03402" ;
                                                                             <http://www.w3.org/2004/02/skos/core#prefLabel> "KineticEnergy"@en .


###  http://emmo.info/emmo/middle/isq#EMMO_acf636d4_9ac2_4ce3_960a_d54338e6cae3
<http://emmo.info/emmo/middle/isq#EMMO_acf636d4_9ac2_4ce3_960a_d54338e6cae3> rdf:type owl:Class ;
                                                                             rdfs:subClassOf <http://emmo.info/emmo/middle/isq#EMMO_faab3f84_e475_4a46_af9c_7d249f0b9aef> ;
                                                                             <http://emmo.info/emmo/middle/isq#EMMO_de178b12_5d35_4bca_8efa_a4193162571d> "T0 L0 M0 I0 T0 N0 J0" ;
                                                                             <http://emmo.info/emmo/top/annotations#EMMO_1f1b164d_ec6a_4faa_8d5e_88bda62316cc> "http://qudt.org/vocab/quantitykind/Strain" ;
                                                                             <http://emmo.info/emmo/top/annotations#EMMO_50c298c2_55a2_4068_b3ac_4e948c33181f> "http://www.electropedia.org/iev/iev.nsf/display?openform&ievref=113-03-57" ;
                                                                             <http://emmo.info/emmo/top/annotations#EMMO_967080e5_2f42_4eb2_a3a9_c58143e835f9> "Change of the relative positions of parts of a body, excluding a displacement of the body as a whole."@en ;
                                                                             <http://emmo.info/emmo/top/annotations#EMMO_e55f2d7c_9893_48cd_b4a4_fdf38253bd20> "http://www.ontology-of-units-of-measure.org/resource/om-2/Strain" ;
                                                                             <http://www.w3.org/2004/02/skos/core#prefLabel> "Strain"@en .


###  http://emmo.info/emmo/middle/isq#EMMO_ad6c76cf_b400_423e_820f_cf0c4e77f455
<http://emmo.info/emmo/middle/isq#EMMO_ad6c76cf_b400_423e_820f_cf0c4e77f455> rdf:type owl:Class ;
                                                                             rdfs:subClassOf <http://emmo.info/emmo/middle/isq#EMMO_f2ca6dd0_0e5f_4392_a92d_cafdae6cfc95> ;
                                                                             <http://emmo.info/emmo/middle/isq#EMMO_de178b12_5d35_4bca_8efa_a4193162571d> "T-2 L+2 M+1 I0 T-1 N-1 J0" ;
                                                                             <http://emmo.info/emmo/top/annotations#EMMO_1f1b164d_ec6a_4faa_8d5e_88bda62316cc> "http://qudt.org/vocab/constant/MolarGasConstant" ;
                                                                             <http://emmo.info/emmo/top/annotations#EMMO_6dd685dd_1895_46e4_b227_be9f7d643c25> "http://dbpedia.org/page/Gas_constant" ;
                                                                             <http://emmo.info/emmo/top/annotations#EMMO_967080e5_2f42_4eb2_a3a9_c58143e835f9> "Equivalent to the Boltzmann constant, but expressed in units of energy per temperature increment per mole (rather than energy per temperature increment per particle)."@en ;
                                                                             <http://emmo.info/emmo/top/annotations#EMMO_a9b3d04c_7ceb_40a2_b8d3_28d514a770a8> "https://physics.nist.gov/cgi-bin/cuu/Value?r" ;
                                                                             <http://emmo.info/emmo/top/annotations#EMMO_fe015383_afb3_44a6_ae86_043628697aa2> "https://doi.org/10.1351/goldbook.G02579" ;
                                                                             <http://www.w3.org/2004/02/skos/core#prefLabel> "MolarGasConstant"@en .


###  http://emmo.info/emmo/middle/isq#EMMO_af24ae20_8ef2_435a_86a1_2ea44488b318
<http://emmo.info/emmo/middle/isq#EMMO_af24ae20_8ef2_435a_86a1_2ea44488b318> rdf:type owl:Class ;
                                                                             rdfs:subClassOf <http://emmo.info/emmo/middle/metrology#EMMO_9895a1b4_f0a5_4167_ac5e_97db40b8bfcc> ;
                                                                             <http://www.w3.org/2004/02/skos/core#prefLabel> "PerAmountDimension"@en .


###  http://emmo.info/emmo/middle/isq#EMMO_afea89af_ef16_4bdb_99d5_f3b2f4c85a6c
<http://emmo.info/emmo/middle/isq#EMMO_afea89af_ef16_4bdb_99d5_f3b2f4c85a6c> rdf:type owl:Class ;
                                                                             rdfs:subClassOf <http://emmo.info/emmo/middle/isq#EMMO_2946d40b_24a1_47fa_8176_e3f79bb45064> ;
                                                                             <http://emmo.info/emmo/middle/isq#EMMO_de178b12_5d35_4bca_8efa_a4193162571d> "T0 L-2 M+1 I0 T0 N0 J0" ;
                                                                             <http://emmo.info/emmo/top/annotations#EMMO_6dd685dd_1895_46e4_b227_be9f7d643c25> "http://dbpedia.org/page/Area_density" ;
                                                                             <http://emmo.info/emmo/top/annotations#EMMO_fe015383_afb3_44a6_ae86_043628697aa2> "https://doi.org/10.1351/goldbook.S06167" ;
                                                                             rdfs:comment "Mass per unit area."@en ;
                                                                             <http://www.w3.org/2004/02/skos/core#prefLabel> "AreaDensity"@en .


###  http://emmo.info/emmo/middle/isq#EMMO_affe07e4_e9bc_4852_86c6_69e26182a17f
<http://emmo.info/emmo/middle/isq#EMMO_affe07e4_e9bc_4852_86c6_69e26182a17f> rdf:type owl:Class ;
                                                                             rdfs:subClassOf <http://emmo.info/emmo/middle/isq#EMMO_1a4c1a97_88a7_4d8e_b2f9_2ca58e92dde4> ;
                                                                             <http://emmo.info/emmo/middle/isq#EMMO_de178b12_5d35_4bca_8efa_a4193162571d> "T0 L0 M0 I0 T+1 N0 J0" ;
                                                                             <http://emmo.info/emmo/top/annotations#EMMO_1f1b164d_ec6a_4faa_8d5e_88bda62316cc> "qudt.org/vocab/quantitykind/ThermodynamicTemperature" ;
                                                                             <http://emmo.info/emmo/top/annotations#EMMO_6dd685dd_1895_46e4_b227_be9f7d643c25> "http://dbpedia.org/page/Thermodynamic_temperature" ;
                                                                             <http://emmo.info/emmo/top/annotations#EMMO_967080e5_2f42_4eb2_a3a9_c58143e835f9> "Thermodynamic temperature is the absolute measure of temperature. It is defined by the third law of thermodynamics in which the theoretically lowest temperature is the null or zero point."@en ;
                                                                             <http://emmo.info/emmo/top/annotations#EMMO_fe015383_afb3_44a6_ae86_043628697aa2> "https://doi.org/10.1351/goldbook.T06321" ;
                                                                             <http://www.w3.org/2004/02/skos/core#prefLabel> "ThermodynamicTemperature"@en .


###  http://emmo.info/emmo/middle/isq#EMMO_b14d9be5_f81e_469b_abca_379c2e83feab
<http://emmo.info/emmo/middle/isq#EMMO_b14d9be5_f81e_469b_abca_379c2e83feab> rdf:type owl:Class ;
                                                                             rdfs:subClassOf <http://emmo.info/emmo/middle/metrology#EMMO_9895a1b4_f0a5_4167_ac5e_97db40b8bfcc> ;
                                                                             <http://www.w3.org/2004/02/skos/core#prefLabel> "CapacitanceDimension"@en .


###  http://emmo.info/emmo/middle/isq#EMMO_b3600e73_3e05_479d_9714_c041c3acf5cc
<http://emmo.info/emmo/middle/isq#EMMO_b3600e73_3e05_479d_9714_c041c3acf5cc> rdf:type owl:Class ;
                                                                             rdfs:subClassOf <http://emmo.info/emmo/middle/metrology#EMMO_9895a1b4_f0a5_4167_ac5e_97db40b8bfcc> ;
                                                                             <http://www.w3.org/2004/02/skos/core#prefLabel> "LengthDimension"@en .


###  http://emmo.info/emmo/middle/isq#EMMO_b4895f75_41c8_4fd9_b6d6_4d5f7c99c423
<http://emmo.info/emmo/middle/isq#EMMO_b4895f75_41c8_4fd9_b6d6_4d5f7c99c423> rdf:type owl:Class ;
                                                                             rdfs:subClassOf <http://emmo.info/emmo/middle/isq#EMMO_2946d40b_24a1_47fa_8176_e3f79bb45064> ;
                                                                             <http://emmo.info/emmo/middle/isq#EMMO_de178b12_5d35_4bca_8efa_a4193162571d> "T0 L-1 M0 I+1 T0 N0 J0" ;
                                                                             <http://emmo.info/emmo/top/annotations#EMMO_1f1b164d_ec6a_4faa_8d5e_88bda62316cc> "http://qudt.org/vocab/quantitykind/MagneticFieldStrength" ;
                                                                             <http://emmo.info/emmo/top/annotations#EMMO_6dd685dd_1895_46e4_b227_be9f7d643c25> "http://dbpedia.org/page/Magnetic_field" ;
                                                                             <http://emmo.info/emmo/top/annotations#EMMO_fe015383_afb3_44a6_ae86_043628697aa2> "https://doi.org/10.1351/goldbook.M03683" ;
                                                                             rdfs:comment "Strength of a magnetic field. Commonly denoted H."@en ;
                                                                             <http://www.w3.org/2004/02/skos/core#prefLabel> "MagneticFieldStrength"@en .


###  http://emmo.info/emmo/middle/isq#EMMO_b51fbd00_a857_4132_9711_0ef70e7bdd20
<http://emmo.info/emmo/middle/isq#EMMO_b51fbd00_a857_4132_9711_0ef70e7bdd20> rdf:type owl:Class ;
                                                                             rdfs:subClassOf <http://emmo.info/emmo/middle/isq#EMMO_2946d40b_24a1_47fa_8176_e3f79bb45064> ;
                                                                             <http://emmo.info/emmo/middle/isq#EMMO_de178b12_5d35_4bca_8efa_a4193162571d> "T0 L-2 M0 I0 T0 N0 J+1" ;
                                                                             <http://emmo.info/emmo/top/annotations#EMMO_1f1b164d_ec6a_4faa_8d5e_88bda62316cc> "http://qudt.org/vocab/quantitykind/Illuminance" ;
                                                                             <http://emmo.info/emmo/top/annotations#EMMO_6dd685dd_1895_46e4_b227_be9f7d643c25> "http://dbpedia.org/page/Illuminance" ;
                                                                             <http://emmo.info/emmo/top/annotations#EMMO_70fe84ff_99b6_4206_a9fc_9a8931836d84> "The total luminous flux incident on a surface, per unit area."@en ;
                                                                             <http://emmo.info/emmo/top/annotations#EMMO_fe015383_afb3_44a6_ae86_043628697aa2> "https://doi.org/10.1351/goldbook.I02941" ;
                                                                             <http://www.w3.org/2004/02/skos/core#prefLabel> "Illuminance"@en .


###  http://emmo.info/emmo/middle/isq#EMMO_ba380bc6_2bfd_4f11_94c7_b3cbaafd1631
<http://emmo.info/emmo/middle/isq#EMMO_ba380bc6_2bfd_4f11_94c7_b3cbaafd1631> rdf:type owl:Class ;
                                                                             rdfs:subClassOf <http://emmo.info/emmo/middle/isq#EMMO_f2ca6dd0_0e5f_4392_a92d_cafdae6cfc95> ;
                                                                             <http://emmo.info/emmo/middle/isq#EMMO_de178b12_5d35_4bca_8efa_a4193162571d> "T+2 L-1 M-1 I+1 T0 N0 J0" ;
                                                                             <http://emmo.info/emmo/top/annotations#EMMO_1f1b164d_ec6a_4faa_8d5e_88bda62316cc> "http://qudt.org/vocab/constant/JosephsonConstant" ;
                                                                             <http://emmo.info/emmo/top/annotations#EMMO_967080e5_2f42_4eb2_a3a9_c58143e835f9> "Inverse of the magnetic flux quantum."@en ;
                                                                             <http://emmo.info/emmo/top/annotations#EMMO_a9b3d04c_7ceb_40a2_b8d3_28d514a770a8> "https://physics.nist.gov/cgi-bin/cuu/Value?kjos" ;
                                                                             rdfs:comment "The DBpedia definition (http://dbpedia.org/page/Magnetic_flux_quantum) is outdated as May 20, 2019. It is now an exact quantity."@en ;
                                                                             <http://www.w3.org/2004/02/skos/core#prefLabel> "JosephsonConstant"@en .


###  http://emmo.info/emmo/middle/isq#EMMO_ba882f34_0d71_4e4f_9d92_0c076c633a2c
<http://emmo.info/emmo/middle/isq#EMMO_ba882f34_0d71_4e4f_9d92_0c076c633a2c> rdf:type owl:Class ;
                                                                             rdfs:subClassOf <http://emmo.info/emmo/middle/isq#EMMO_a66427d1_9932_4363_9ec5_7d91f2bfda1e> ;
                                                                             <http://emmo.info/emmo/middle/isq#EMMO_de178b12_5d35_4bca_8efa_a4193162571d> "T0 L0 M0 I0 T0 N0 J0" ;
                                                                             <http://emmo.info/emmo/top/annotations#EMMO_967080e5_2f42_4eb2_a3a9_c58143e835f9> "A pure number, typically the number of something."@en ;
                                                                             <http://emmo.info/emmo/top/annotations#EMMO_b432d2d5_25f4_4165_99c5_5935a7763c1a> """1, 
i, 
p,
the number of protons in the nucleus of an atom""" ;
                                                                             rdfs:comment """According to the SI brochure counting does not automatically qualify a quantity as an amount of substance.

This quantity is used only to describe the outcome of a counting process, without regard of the type of entities.

\"There are also some quantities that cannot be described in terms of the seven base quantities of the SI, but have the nature of a count. Examples are a number of molecules, a number of cellular or biomolecular entities (for example copies of a particular nucleic acid sequence), or degeneracy in quantum mechanics. Counting quantities are also quantities with the associated unit one.\""""@en ;
                                                                             <http://www.w3.org/2004/02/skos/core#prefLabel> "PureNumberQuantity"@en .


###  http://emmo.info/emmo/middle/isq#EMMO_bd67d149_24c2_4bc9_833a_c2bc26f98fd3
<http://emmo.info/emmo/middle/isq#EMMO_bd67d149_24c2_4bc9_833a_c2bc26f98fd3> rdf:type owl:Class ;
                                                                             rdfs:subClassOf <http://emmo.info/emmo/middle/isq#EMMO_2946d40b_24a1_47fa_8176_e3f79bb45064> ;
                                                                             <http://emmo.info/emmo/middle/isq#EMMO_de178b12_5d35_4bca_8efa_a4193162571d> "T-1 L0 M0 I0 T0 N+1 J0" ;
                                                                             <http://emmo.info/emmo/top/annotations#EMMO_1f1b164d_ec6a_4faa_8d5e_88bda62316cc> "http://qudt.org/vocab/quantitykind/CatalyticActivity" ;
                                                                             <http://emmo.info/emmo/top/annotations#EMMO_967080e5_2f42_4eb2_a3a9_c58143e835f9> "Increase in the rate of reaction of a specified chemical reaction that an enzyme produces in a specific assay system."@en ;
                                                                             <http://emmo.info/emmo/top/annotations#EMMO_fe015383_afb3_44a6_ae86_043628697aa2> "https://doi.org/10.1351/goldbook.C00881" ;
                                                                             <http://www.w3.org/2004/02/skos/core#prefLabel> "CatalyticActivity"@en .


###  http://emmo.info/emmo/middle/isq#EMMO_c8d084ad_f88e_4596_8e4d_982c6655ce6f
<http://emmo.info/emmo/middle/isq#EMMO_c8d084ad_f88e_4596_8e4d_982c6655ce6f> rdf:type owl:Class ;
                                                                             rdfs:subClassOf <http://emmo.info/emmo/middle/metrology#EMMO_9895a1b4_f0a5_4167_ac5e_97db40b8bfcc> ;
                                                                             <http://www.w3.org/2004/02/skos/core#prefLabel> "PowerDimension"@en .


###  http://emmo.info/emmo/middle/isq#EMMO_c995ae70_3b84_4ebb_bcfc_69e6a281bb88
<http://emmo.info/emmo/middle/isq#EMMO_c995ae70_3b84_4ebb_bcfc_69e6a281bb88> rdf:type owl:Class ;
                                                                             rdfs:subClassOf <http://emmo.info/emmo/middle/isq#EMMO_1a4c1a97_88a7_4d8e_b2f9_2ca58e92dde4> ;
                                                                             <http://emmo.info/emmo/middle/isq#EMMO_de178b12_5d35_4bca_8efa_a4193162571d> "T0 L0 M0 I+1 T0 N0 J0" ;
                                                                             <http://emmo.info/emmo/top/annotations#EMMO_1f1b164d_ec6a_4faa_8d5e_88bda62316cc> "http://qudt.org/vocab/quantitykind/ElectricCurrent" ;
                                                                             <http://emmo.info/emmo/top/annotations#EMMO_6dd685dd_1895_46e4_b227_be9f7d643c25> "http://dbpedia.org/page/Electric_current" ;
                                                                             <http://emmo.info/emmo/top/annotations#EMMO_967080e5_2f42_4eb2_a3a9_c58143e835f9> "A flow of electric charge."@en ;
                                                                             <http://emmo.info/emmo/top/annotations#EMMO_fe015383_afb3_44a6_ae86_043628697aa2> "https://doi.org/10.1351/goldbook.E01927" ;
                                                                             <http://www.w3.org/2004/02/skos/core#prefLabel> "ElectricCurrent"@en .


###  http://emmo.info/emmo/middle/isq#EMMO_cc01751d_dd05_429b_9d0c_1b7a74d1f277
<http://emmo.info/emmo/middle/isq#EMMO_cc01751d_dd05_429b_9d0c_1b7a74d1f277> rdf:type owl:Class ;
                                                                             rdfs:subClassOf <http://emmo.info/emmo/middle/isq#EMMO_1604f495_328a_4f28_9962_f4cc210739dd> ,
                                                                                             <http://emmo.info/emmo/middle/isq#EMMO_f2ca6dd0_0e5f_4392_a92d_cafdae6cfc95> ;
                                                                             <http://emmo.info/emmo/middle/isq#EMMO_de178b12_5d35_4bca_8efa_a4193162571d> "T+1 L0 M0 I+1 T0 N0 J0" ;
                                                                             <http://emmo.info/emmo/top/annotations#EMMO_70fe84ff_99b6_4206_a9fc_9a8931836d84> "The charge of an electron."@en ;
                                                                             <http://emmo.info/emmo/top/annotations#EMMO_fe015383_afb3_44a6_ae86_043628697aa2> "https://doi.org/10.1351/goldbook.E01982" ;
                                                                             rdfs:comment "The negative of ElementaryCharge."@en ;
                                                                             <http://www.w3.org/2004/02/skos/core#prefLabel> "ElectronCharge"@en .


###  http://emmo.info/emmo/middle/isq#EMMO_cd2cd0de_e0cc_4ef1_b27e_2e88db027bac
<http://emmo.info/emmo/middle/isq#EMMO_cd2cd0de_e0cc_4ef1_b27e_2e88db027bac> rdf:type owl:Class ;
                                                                             rdfs:subClassOf <http://emmo.info/emmo/middle/isq#EMMO_1a4c1a97_88a7_4d8e_b2f9_2ca58e92dde4> ;
                                                                             <http://emmo.info/emmo/middle/isq#EMMO_de178b12_5d35_4bca_8efa_a4193162571d> "T0 L+1 M0 I0 T0 N0 J0" ;
                                                                             <http://emmo.info/emmo/top/annotations#EMMO_50c298c2_55a2_4068_b3ac_4e948c33181f> "http://www.electropedia.org/iev/iev.nsf/display?openform&ievref=113-01-19" ;
                                                                             <http://emmo.info/emmo/top/annotations#EMMO_6dd685dd_1895_46e4_b227_be9f7d643c25> "http://dbpedia.org/page/Length" ;
                                                                             <http://emmo.info/emmo/top/annotations#EMMO_967080e5_2f42_4eb2_a3a9_c58143e835f9> "Extend of a spatial dimension."@en ;
                                                                             <http://emmo.info/emmo/top/annotations#EMMO_fe015383_afb3_44a6_ae86_043628697aa2> "https://doi.org/10.1351/goldbook.L03498" ;
                                                                             rdfs:comment "Length is a non-negative additive quantity attributed to a one-dimensional object in space."@en ;
                                                                             <http://www.w3.org/2004/02/skos/core#prefLabel> "Length"@en .


###  http://emmo.info/emmo/middle/isq#EMMO_cde4368c_1d4d_4c94_8548_604749523c6d
<http://emmo.info/emmo/middle/isq#EMMO_cde4368c_1d4d_4c94_8548_604749523c6d> rdf:type owl:Class ;
                                                                             rdfs:subClassOf <http://emmo.info/emmo/middle/isq#EMMO_2946d40b_24a1_47fa_8176_e3f79bb45064> ;
                                                                             <http://emmo.info/emmo/middle/isq#EMMO_de178b12_5d35_4bca_8efa_a4193162571d> "T+3 L-3 M-1 I+2 T0 N0 J0" ;
                                                                             <http://emmo.info/emmo/top/annotations#EMMO_1f1b164d_ec6a_4faa_8d5e_88bda62316cc> "http://qudt.org/vocab/quantitykind/ElectricConductivity" ;
                                                                             <http://emmo.info/emmo/top/annotations#EMMO_6dd685dd_1895_46e4_b227_be9f7d643c25> "http://dbpedia.org/page/Electrical_resistivity_and_conductivity" ;
                                                                             <http://emmo.info/emmo/top/annotations#EMMO_fe015383_afb3_44a6_ae86_043628697aa2> "https://doi.org/10.1351/goldbook.C01245" ;
                                                                             rdfs:comment """Measure of a material's ability to conduct an electric current. 

Conductivity is equeal to the resiprocal of resistivity."""@en ;
                                                                             <http://www.w3.org/2004/02/skos/core#altLabel> "Conductivity" ;
                                                                             <http://www.w3.org/2004/02/skos/core#prefLabel> "ElectricConductivity"@en .


###  http://emmo.info/emmo/middle/isq#EMMO_ce7d4720_aa20_4a8c_93e8_df41a35b6723
<http://emmo.info/emmo/middle/isq#EMMO_ce7d4720_aa20_4a8c_93e8_df41a35b6723> rdf:type owl:Class ;
                                                                             rdfs:subClassOf <http://emmo.info/emmo/middle/metrology#EMMO_9895a1b4_f0a5_4167_ac5e_97db40b8bfcc> ;
                                                                             <http://www.w3.org/2004/02/skos/core#prefLabel> "CatalyticActivityDimension"@en .


###  http://emmo.info/emmo/middle/isq#EMMO_d1917609_db5e_4b8a_9b76_ef1d6f860a81
<http://emmo.info/emmo/middle/isq#EMMO_d1917609_db5e_4b8a_9b76_ef1d6f860a81> rdf:type owl:Class ;
                                                                             rdfs:subClassOf <http://emmo.info/emmo/middle/isq#EMMO_2946d40b_24a1_47fa_8176_e3f79bb45064> ;
                                                                             <http://emmo.info/emmo/middle/isq#EMMO_de178b12_5d35_4bca_8efa_a4193162571d> "T-2 L-1 M+1 I0 T0 N0 J0" ;
                                                                             <http://emmo.info/emmo/top/annotations#EMMO_1f1b164d_ec6a_4faa_8d5e_88bda62316cc> "http://qudt.org/vocab/quantitykind/Stress" ;
                                                                             <http://emmo.info/emmo/top/annotations#EMMO_6dd685dd_1895_46e4_b227_be9f7d643c25> "http://dbpedia.org/page/Stress_(mechanics)" ;
                                                                             rdfs:comment "Force per unit oriented surface area ."@en ,
                                                                                          "Measure of the internal forces that neighboring particles of a continuous material exert on each other."@en ;
                                                                             <http://www.w3.org/2004/02/skos/core#prefLabel> "Stress"@en .


###  http://emmo.info/emmo/middle/isq#EMMO_d4f7d378_5e3b_468a_baa1_a7e98358cda7
<http://emmo.info/emmo/middle/isq#EMMO_d4f7d378_5e3b_468a_baa1_a7e98358cda7> rdf:type owl:Class ;
                                                                             rdfs:subClassOf <http://emmo.info/emmo/middle/isq#EMMO_1a4c1a97_88a7_4d8e_b2f9_2ca58e92dde4> ;
                                                                             <http://emmo.info/emmo/middle/isq#EMMO_de178b12_5d35_4bca_8efa_a4193162571d> "T+1 L0 M0 I0 T0 N0 J0" ;
                                                                             <http://emmo.info/emmo/top/annotations#EMMO_1f1b164d_ec6a_4faa_8d5e_88bda62316cc> "qudt.org/vocab/quantitykind/Time" ;
                                                                             <http://emmo.info/emmo/top/annotations#EMMO_50c298c2_55a2_4068_b3ac_4e948c33181f> "http://www.electropedia.org/iev/iev.nsf/display?openform&ievref=113-01-03" ;
                                                                             <http://emmo.info/emmo/top/annotations#EMMO_6dd685dd_1895_46e4_b227_be9f7d643c25> "http://dbpedia.org/page/Time" ;
                                                                             <http://emmo.info/emmo/top/annotations#EMMO_70fe84ff_99b6_4206_a9fc_9a8931836d84> "One-dimensional subspace of space-time, which is locally orthogonal to space."@en ;
                                                                             <http://emmo.info/emmo/top/annotations#EMMO_967080e5_2f42_4eb2_a3a9_c58143e835f9> "The indefinite continued progress of existence and events that occur in apparently irreversible succession from the past through the present to the future."@en ;
                                                                             <http://emmo.info/emmo/top/annotations#EMMO_fe015383_afb3_44a6_ae86_043628697aa2> "https://doi.org/10.1351/goldbook.T06375" ;
                                                                             rdfs:comment "Time can be seen as the duration of an event or, more operationally, as \"what clocks read\"."@en ;
                                                                             <http://www.w3.org/2004/02/skos/core#prefLabel> "Time"@en .


###  http://emmo.info/emmo/middle/isq#EMMO_d5be1faf_0c56_4f5a_9b78_581e6dee949f
<http://emmo.info/emmo/middle/isq#EMMO_d5be1faf_0c56_4f5a_9b78_581e6dee949f> rdf:type owl:Class ;
                                                                             rdfs:subClassOf <http://emmo.info/emmo/middle/chemistry#EMMO_a293f923_954c_4af5_9f97_9600ebd362cb> ,
                                                                                             <http://emmo.info/emmo/middle/isq#EMMO_2946d40b_24a1_47fa_8176_e3f79bb45064> ;
                                                                             <http://emmo.info/emmo/middle/isq#EMMO_de178b12_5d35_4bca_8efa_a4193162571d> "T0 L-3 M0 I0 T0 N+1 J0" ;
                                                                             <http://emmo.info/emmo/top/annotations#EMMO_1f1b164d_ec6a_4faa_8d5e_88bda62316cc> "http://qudt.org/vocab/quantitykind/AmountOfSubstanceConcentrationOfB" ;
                                                                             <http://emmo.info/emmo/top/annotations#EMMO_6dd685dd_1895_46e4_b227_be9f7d643c25> "http://dbpedia.org/page/Molar_concentration" ;
                                                                             <http://emmo.info/emmo/top/annotations#EMMO_fe015383_afb3_44a6_ae86_043628697aa2> "https://doi.org/10.1351/goldbook.A00295" ;
                                                                             rdfs:comment "The amount of a constituent divided by the volume of the mixture."@en ;
                                                                             <http://www.w3.org/2004/02/skos/core#altLabel> "Concentration"@en ,
                                                                                                                            "MolarConcentration"@en ,
                                                                                                                            "Molarity"@en ;
                                                                             <http://www.w3.org/2004/02/skos/core#prefLabel> "AmountConcentration"@en .


###  http://emmo.info/emmo/middle/isq#EMMO_d5f3e0e5_fc7d_4e64_86ad_555e74aaff84
<http://emmo.info/emmo/middle/isq#EMMO_d5f3e0e5_fc7d_4e64_86ad_555e74aaff84> rdf:type owl:Class ;
                                                                             rdfs:subClassOf <http://emmo.info/emmo/middle/metrology#EMMO_9895a1b4_f0a5_4167_ac5e_97db40b8bfcc> ;
                                                                             <http://www.w3.org/2004/02/skos/core#prefLabel> "ElectricCurrentDimension"@en .


###  http://emmo.info/emmo/middle/isq#EMMO_d7d2ca25_03e1_4099_9220_c1a58df13ad0
<http://emmo.info/emmo/middle/isq#EMMO_d7d2ca25_03e1_4099_9220_c1a58df13ad0> rdf:type owl:Class ;
                                                                             rdfs:subClassOf <http://emmo.info/emmo/middle/metrology#EMMO_3f15d200_c97b_42c8_8ac0_d81d150361e2> ;
                                                                             <http://emmo.info/emmo/middle/isq#EMMO_de178b12_5d35_4bca_8efa_a4193162571d> "T0 L0 M0 I0 T0 N0 J0" ;
                                                                             <http://emmo.info/emmo/top/annotations#EMMO_1f1b164d_ec6a_4faa_8d5e_88bda62316cc> "http://qudt.org/vocab/constant/FineStructureConstant" ;
                                                                             <http://emmo.info/emmo/top/annotations#EMMO_6dd685dd_1895_46e4_b227_be9f7d643c25> "http://dbpedia.org/page/Fine-structure_constant" ;
                                                                             <http://emmo.info/emmo/top/annotations#EMMO_a9b3d04c_7ceb_40a2_b8d3_28d514a770a8> "https://physics.nist.gov/cgi-bin/cuu/Value?alph" ;
                                                                             <http://emmo.info/emmo/top/annotations#EMMO_fe015383_afb3_44a6_ae86_043628697aa2> "https://doi.org/10.1351/goldbook.F02389" ;
                                                                             rdfs:comment "A fundamental physical constant characterizing the strength of the electromagnetic interaction between elementary charged particles."@en ;
                                                                             <http://www.w3.org/2004/02/skos/core#prefLabel> "FineStructureConstant"@en .


###  http://emmo.info/emmo/middle/isq#EMMO_d859588d_44dc_4614_bc75_5fcd0058acc8
<http://emmo.info/emmo/middle/isq#EMMO_d859588d_44dc_4614_bc75_5fcd0058acc8> rdf:type owl:Class ;
                                                                             rdfs:subClassOf <http://emmo.info/emmo/middle/isq#EMMO_ecec2983_7c26_4f8d_a981_51ca29668baf> ;
                                                                             <http://emmo.info/emmo/middle/isq#EMMO_de178b12_5d35_4bca_8efa_a4193162571d> "T0 L-1 M0 I0 T0 N0 J0" ;
                                                                             <http://emmo.info/emmo/top/annotations#EMMO_1f1b164d_ec6a_4faa_8d5e_88bda62316cc> "http://qudt.org/vocab/quantitykind/Wavenumber" ;
                                                                             <http://emmo.info/emmo/top/annotations#EMMO_6dd685dd_1895_46e4_b227_be9f7d643c25> "http://dbpedia.org/page/Wavenumber" ;
                                                                             <http://emmo.info/emmo/top/annotations#EMMO_e55f2d7c_9893_48cd_b4a4_fdf38253bd20> "http://www.ontology-of-units-of-measure.org/resource/om-2/Wavenumber" ;
                                                                             <http://emmo.info/emmo/top/annotations#EMMO_fe015383_afb3_44a6_ae86_043628697aa2> "https://doi.org/10.1351/goldbook.W06664" ;
                                                                             rdfs:comment "The number of waves per unit length along the direction of propagation."@en ;
                                                                             <http://www.w3.org/2004/02/skos/core#prefLabel> "Wavenumber"@en .


###  http://emmo.info/emmo/middle/isq#EMMO_da831168_975a_41f8_baae_279c298569da
<http://emmo.info/emmo/middle/isq#EMMO_da831168_975a_41f8_baae_279c298569da> rdf:type owl:Class ;
                                                                             rdfs:subClassOf <http://emmo.info/emmo/middle/metrology#EMMO_3f15d200_c97b_42c8_8ac0_d81d150361e2> ;
                                                                             <http://emmo.info/emmo/middle/isq#EMMO_de178b12_5d35_4bca_8efa_a4193162571d> "T-2 L+3 M-1 I0 T0 N0 J0" ;
                                                                             <http://emmo.info/emmo/top/annotations#EMMO_1f1b164d_ec6a_4faa_8d5e_88bda62316cc> "http://qudt.org/vocab/constant/NewtonianConstantOfGravitation" ;
                                                                             <http://emmo.info/emmo/top/annotations#EMMO_6dd685dd_1895_46e4_b227_be9f7d643c25> "http://dbpedia.org/page/Gravitational_constant" ;
                                                                             <http://emmo.info/emmo/top/annotations#EMMO_a9b3d04c_7ceb_40a2_b8d3_28d514a770a8> "https://physics.nist.gov/cgi-bin/cuu/Value?bg" ;
                                                                             <http://emmo.info/emmo/top/annotations#EMMO_fe015383_afb3_44a6_ae86_043628697aa2> "https://doi.org/10.1351/goldbook.G02695" ;
                                                                             rdfs:comment "Physical constant in Newton's law of gravitation and in Einstein's general theory of relativity."@en ;
                                                                             <http://www.w3.org/2004/02/skos/core#prefLabel> "NewtonianConstantOfGravity"@en .


###  http://emmo.info/emmo/middle/isq#EMMO_dc6c8de0_cfc4_4c66_a7dc_8f720e732d54
<http://emmo.info/emmo/middle/isq#EMMO_dc6c8de0_cfc4_4c66_a7dc_8f720e732d54> rdf:type owl:Class ;
                                                                             rdfs:subClassOf <http://emmo.info/emmo/middle/isq#EMMO_ba882f34_0d71_4e4f_9d92_0c076c633a2c> ;
                                                                             <http://emmo.info/emmo/middle/isq#EMMO_de178b12_5d35_4bca_8efa_a4193162571d> "T0 L0 M0 I0 T0 N0 J0" ;
                                                                             <http://emmo.info/emmo/top/annotations#EMMO_1f1b164d_ec6a_4faa_8d5e_88bda62316cc> "http://qudt.org/vocab/quantitykind/MassNumber" ;
                                                                             <http://emmo.info/emmo/top/annotations#EMMO_70fe84ff_99b6_4206_a9fc_9a8931836d84> "Number of nucleons in an atomic nucleus."@en ;
                                                                             <http://www.w3.org/2004/02/skos/core#altLabel> "AtomicMassNumber" ,
                                                                                                                            "NucleonNumber" ;
                                                                             <http://www.w3.org/2004/02/skos/core#prefLabel> "MassNumber"@en .


###  http://emmo.info/emmo/middle/isq#EMMO_de021e4f_918f_47ef_a67b_11120f56b9d7
<http://emmo.info/emmo/middle/isq#EMMO_de021e4f_918f_47ef_a67b_11120f56b9d7> rdf:type owl:Class ;
                                                                             rdfs:subClassOf <http://emmo.info/emmo/middle/isq#EMMO_09663630_1b84_4202_91e6_e641104f579e> ,
                                                                                             <http://emmo.info/emmo/middle/metrology#EMMO_3f15d200_c97b_42c8_8ac0_d81d150361e2> ;
                                                                             <http://emmo.info/emmo/middle/isq#EMMO_de178b12_5d35_4bca_8efa_a4193162571d> "T-2 L+1 M+1 I-2 T0 N0 J0" ;
                                                                             <http://emmo.info/emmo/top/annotations#EMMO_1f1b164d_ec6a_4faa_8d5e_88bda62316cc> "http://qudt.org/vocab/constant/ElectromagneticPermeabilityOfVacuum" ;
                                                                             <http://emmo.info/emmo/top/annotations#EMMO_a9b3d04c_7ceb_40a2_b8d3_28d514a770a8> "https://physics.nist.gov/cgi-bin/cuu/Value?mu0" ;
                                                                             rdfs:comment "The DBpedia and UIPAC Gold Book definitions (http://dbpedia.org/page/Vacuum_permeability,  https://doi.org/10.1351/goldbook.P04504) are outdated since May 20, 2019. It is now a measured constant."@en ,
                                                                                          "The value of magnetic permeability in a classical vacuum."@en ;
                                                                             <http://www.w3.org/2004/02/skos/core#prefLabel> "VacuumMagneticPermeability"@en .


###  http://emmo.info/emmo/middle/isq#EMMO_e150fa8d_06dc_4bb8_bf95_04e2aea529c1
<http://emmo.info/emmo/middle/isq#EMMO_e150fa8d_06dc_4bb8_bf95_04e2aea529c1> rdf:type owl:Class ;
                                                                             rdfs:subClassOf <http://emmo.info/emmo/middle/isq#EMMO_2946d40b_24a1_47fa_8176_e3f79bb45064> ;
                                                                             <http://emmo.info/emmo/middle/isq#EMMO_de178b12_5d35_4bca_8efa_a4193162571d> "T-3 L+3 M+1 I-2 T0 N0 J0" ;
                                                                             <http://emmo.info/emmo/top/annotations#EMMO_1f1b164d_ec6a_4faa_8d5e_88bda62316cc> "http://qudt.org/vocab/quantitykind/Resistivity" ;
                                                                             <http://emmo.info/emmo/top/annotations#EMMO_6dd685dd_1895_46e4_b227_be9f7d643c25> "http://dbpedia.org/page/Electrical_resistivity_and_conductivity" ;
                                                                             <http://emmo.info/emmo/top/annotations#EMMO_fe015383_afb3_44a6_ae86_043628697aa2> "https://doi.org/10.1351/goldbook.R05316" ;
                                                                             rdfs:comment "Electric field strength divided by the current density."@en ;
                                                                             <http://www.w3.org/2004/02/skos/core#altLabel> "Resistivity" ;
                                                                             <http://www.w3.org/2004/02/skos/core#prefLabel> "ElectricResistivity"@en .


###  http://emmo.info/emmo/middle/isq#EMMO_e2ee1c98_497a_4f66_b4ed_5711496a848e
<http://emmo.info/emmo/middle/isq#EMMO_e2ee1c98_497a_4f66_b4ed_5711496a848e> rdf:type owl:Class ;
                                                                             rdfs:subClassOf <http://emmo.info/emmo/middle/isq#EMMO_2946d40b_24a1_47fa_8176_e3f79bb45064> ;
                                                                             <http://emmo.info/emmo/middle/isq#EMMO_de178b12_5d35_4bca_8efa_a4193162571d> "T0 L0 M0 I0 T0 N0 J+1" ;
                                                                             <http://emmo.info/emmo/top/annotations#EMMO_1f1b164d_ec6a_4faa_8d5e_88bda62316cc> "http://qudt.org/vocab/quantitykind/LuminousFlux" ;
                                                                             <http://emmo.info/emmo/top/annotations#EMMO_6dd685dd_1895_46e4_b227_be9f7d643c25> "http://dbpedia.org/page/Luminous_flux" ;
                                                                             <http://emmo.info/emmo/top/annotations#EMMO_967080e5_2f42_4eb2_a3a9_c58143e835f9> "Perceived power of light."@en ;
                                                                             <http://emmo.info/emmo/top/annotations#EMMO_fe015383_afb3_44a6_ae86_043628697aa2> "https://doi.org/10.1351/goldbook.L03646" ;
                                                                             <http://www.w3.org/2004/02/skos/core#prefLabel> "LuminousFlux"@en .


###  http://emmo.info/emmo/middle/isq#EMMO_e37ac288_aa60_415a_8cb7_c375724ac8e1
<http://emmo.info/emmo/middle/isq#EMMO_e37ac288_aa60_415a_8cb7_c375724ac8e1> rdf:type owl:Class ;
                                                                             rdfs:subClassOf <http://emmo.info/emmo/middle/isq#EMMO_2946d40b_24a1_47fa_8176_e3f79bb45064> ;
                                                                             <http://emmo.info/emmo/middle/isq#EMMO_de178b12_5d35_4bca_8efa_a4193162571d> "T-2 L+1 M0 I0 T0 N0 J0" ;
                                                                             <http://emmo.info/emmo/top/annotations#EMMO_1f1b164d_ec6a_4faa_8d5e_88bda62316cc> "http://qudt.org/vocab/quantitykind/Acceleration" ;
                                                                             <http://emmo.info/emmo/top/annotations#EMMO_6dd685dd_1895_46e4_b227_be9f7d643c25> "http://dbpedia.org/page/Acceleration" ;
                                                                             <http://emmo.info/emmo/top/annotations#EMMO_fe015383_afb3_44a6_ae86_043628697aa2> "https://doi.org/10.1351/goldbook.A00051" ;
                                                                             rdfs:comment "Derivative of velocity with respect to time."@en ;
                                                                             <http://www.w3.org/2004/02/skos/core#prefLabel> "Acceleration"@en .


###  http://emmo.info/emmo/middle/isq#EMMO_e46f3f24_c2ec_4552_8dd4_cfc5c0a89c09
<http://emmo.info/emmo/middle/isq#EMMO_e46f3f24_c2ec_4552_8dd4_cfc5c0a89c09> rdf:type owl:Class ;
                                                                             rdfs:subClassOf <http://emmo.info/emmo/middle/isq#EMMO_09b9021b_f97b_43eb_b83d_0a764b472bc2> ;
                                                                             <http://emmo.info/emmo/middle/isq#EMMO_de178b12_5d35_4bca_8efa_a4193162571d> "T-3 L+2 M+1 I0 T0 N0 J0" ;
                                                                             <http://emmo.info/emmo/top/annotations#EMMO_1f1b164d_ec6a_4faa_8d5e_88bda62316cc> "http://qudt.org/vocab/quantitykind/RadiantFlux" ;
                                                                             <http://emmo.info/emmo/top/annotations#EMMO_6dd685dd_1895_46e4_b227_be9f7d643c25> "http://dbpedia.org/page/Radiant_flux" ;
                                                                             <http://emmo.info/emmo/top/annotations#EMMO_fe015383_afb3_44a6_ae86_043628697aa2> "https://doi.org/10.1351/goldbook.R05046" ;
                                                                             rdfs:comment "The radiant energy emitted, reflected, transmitted or received, per unit time."@en ;
                                                                             <http://www.w3.org/2004/02/skos/core#prefLabel> "RadiantFlux"@en .


###  http://emmo.info/emmo/middle/isq#EMMO_e501069c_34d3_4dc7_ac87_c90c7342192b
<http://emmo.info/emmo/middle/isq#EMMO_e501069c_34d3_4dc7_ac87_c90c7342192b> rdf:type owl:Class ;
                                                                             rdfs:subClassOf <http://emmo.info/emmo/middle/metrology#EMMO_9895a1b4_f0a5_4167_ac5e_97db40b8bfcc> ;
                                                                             <http://www.w3.org/2004/02/skos/core#prefLabel> "AmountDimension"@en .


###  http://emmo.info/emmo/middle/isq#EMMO_e7c9f7fd_e534_4441_88fe_1fec6cb20f26
<http://emmo.info/emmo/middle/isq#EMMO_e7c9f7fd_e534_4441_88fe_1fec6cb20f26> rdf:type owl:Class ;
                                                                             rdfs:subClassOf <http://emmo.info/emmo/middle/isq#EMMO_faab3f84_e475_4a46_af9c_7d249f0b9aef> ;
                                                                             <http://emmo.info/emmo/middle/isq#EMMO_de178b12_5d35_4bca_8efa_a4193162571d> "T0 L0 M0 I0 T0 N0 J0" ;
                                                                             <http://emmo.info/emmo/top/annotations#EMMO_1f1b164d_ec6a_4faa_8d5e_88bda62316cc> "http://qudt.org/vocab/quantitykind/SolidAngle" ;
                                                                             <http://emmo.info/emmo/top/annotations#EMMO_6dd685dd_1895_46e4_b227_be9f7d643c25> "http://dbpedia.org/page/Solid_angle" ;
                                                                             <http://emmo.info/emmo/top/annotations#EMMO_967080e5_2f42_4eb2_a3a9_c58143e835f9> "Ratio of area on a sphere to its radius squared."@en ;
                                                                             <http://emmo.info/emmo/top/annotations#EMMO_fe015383_afb3_44a6_ae86_043628697aa2> "https://doi.org/10.1351/goldbook.S05732" ;
                                                                             <http://www.w3.org/2004/02/skos/core#prefLabel> "SolidAngle"@en .


###  http://emmo.info/emmo/middle/isq#EMMO_e88f75d6_9a17_4cfc_bdf7_43d7cea5a9a1
<http://emmo.info/emmo/middle/isq#EMMO_e88f75d6_9a17_4cfc_bdf7_43d7cea5a9a1> rdf:type owl:Class ;
                                                                             rdfs:subClassOf <http://emmo.info/emmo/middle/isq#EMMO_2946d40b_24a1_47fa_8176_e3f79bb45064> ;
                                                                             <http://emmo.info/emmo/middle/isq#EMMO_de178b12_5d35_4bca_8efa_a4193162571d> "T-3 L+2 M+1 I-2 T0 N0 J0" ;
                                                                             <http://emmo.info/emmo/top/annotations#EMMO_1f1b164d_ec6a_4faa_8d5e_88bda62316cc> "http://qudt.org/vocab/quantitykind/Resistance" ;
                                                                             <http://emmo.info/emmo/top/annotations#EMMO_6dd685dd_1895_46e4_b227_be9f7d643c25> "http://dbpedia.org/page/Electrical_resistance_and_conductance" ;
                                                                             <http://emmo.info/emmo/top/annotations#EMMO_967080e5_2f42_4eb2_a3a9_c58143e835f9> "Measure of the difficulty to pass an electric current through a material."@en ;
                                                                             <http://emmo.info/emmo/top/annotations#EMMO_fe015383_afb3_44a6_ae86_043628697aa2> "https://doi.org/10.1351/goldbook.E01936" ;
                                                                             rdfs:comment "Inverse of 'ElectricalConductance'."@en ;
                                                                             <http://www.w3.org/2004/02/skos/core#altLabel> "Resistance"@en ;
                                                                             <http://www.w3.org/2004/02/skos/core#prefLabel> "ElectricResistance"@en .


###  http://emmo.info/emmo/middle/isq#EMMO_eb561764_276e_413d_a8cb_3a3154fd9bf8
<http://emmo.info/emmo/middle/isq#EMMO_eb561764_276e_413d_a8cb_3a3154fd9bf8> rdf:type owl:Class ;
                                                                             rdfs:subClassOf <http://emmo.info/emmo/middle/isq#EMMO_e88f75d6_9a17_4cfc_bdf7_43d7cea5a9a1> ,
                                                                                             <http://emmo.info/emmo/middle/isq#EMMO_f2ca6dd0_0e5f_4392_a92d_cafdae6cfc95> ;
                                                                             <http://emmo.info/emmo/middle/isq#EMMO_de178b12_5d35_4bca_8efa_a4193162571d> "T-3 L+2 M+1 I-2 T0 N0 J0" ;
                                                                             <http://emmo.info/emmo/top/annotations#EMMO_1f1b164d_ec6a_4faa_8d5e_88bda62316cc> "http://qudt.org/vocab/constant/VonKlitzingConstant" ;
                                                                             <http://emmo.info/emmo/top/annotations#EMMO_70fe84ff_99b6_4206_a9fc_9a8931836d84> "The von Klitzing constant is defined as Planck constant divided by the square of the elementary charge."@en ;
                                                                             <http://emmo.info/emmo/top/annotations#EMMO_a9b3d04c_7ceb_40a2_b8d3_28d514a770a8> "https://physics.nist.gov/cgi-bin/cuu/Value?rk" ;
                                                                             rdfs:comment "Resistance quantum."@en ;
                                                                             <http://www.w3.org/2004/02/skos/core#prefLabel> "VonKlitzingConstant"@en .


###  http://emmo.info/emmo/middle/isq#EMMO_ec903946_ddc9_464a_903c_7373e0d1eeb5
<http://emmo.info/emmo/middle/isq#EMMO_ec903946_ddc9_464a_903c_7373e0d1eeb5> rdf:type owl:Class ;
                                                                             rdfs:subClassOf <http://emmo.info/emmo/middle/metrology#EMMO_9895a1b4_f0a5_4167_ac5e_97db40b8bfcc> ;
                                                                             <http://www.w3.org/2004/02/skos/core#prefLabel> "MagneticFluxDensityDimension"@en .


###  http://emmo.info/emmo/middle/isq#EMMO_ecec2983_7c26_4f8d_a981_51ca29668baf
<http://emmo.info/emmo/middle/isq#EMMO_ecec2983_7c26_4f8d_a981_51ca29668baf> rdf:type owl:Class ;
                                                                             rdfs:subClassOf <http://emmo.info/emmo/middle/isq#EMMO_2946d40b_24a1_47fa_8176_e3f79bb45064> ;
                                                                             <http://emmo.info/emmo/middle/isq#EMMO_de178b12_5d35_4bca_8efa_a4193162571d> "T0 L-1 M0 I0 T0 N0 J0" ;
                                                                             <http://emmo.info/emmo/top/annotations#EMMO_1f1b164d_ec6a_4faa_8d5e_88bda62316cc> "http://qudt.org/vocab/quantitykind/InverseLength" ;
                                                                             <http://emmo.info/emmo/top/annotations#EMMO_6dd685dd_1895_46e4_b227_be9f7d643c25> "http://dbpedia.org/page/Reciprocal_length" ;
                                                                             <http://emmo.info/emmo/top/annotations#EMMO_967080e5_2f42_4eb2_a3a9_c58143e835f9> "The inverse of length."@en ;
                                                                             <http://emmo.info/emmo/top/annotations#EMMO_c84c6752_6d64_48cc_9500_e54a3c34898d> "https://en.wikipedia.org/wiki/Reciprocal_length" ;
                                                                             <http://www.w3.org/2004/02/skos/core#altLabel> "InverseLength" ;
                                                                             <http://www.w3.org/2004/02/skos/core#prefLabel> "ReciprocalLength"@en .


###  http://emmo.info/emmo/middle/isq#EMMO_ed4af7ae_63a2_497e_bb88_2309619ea405
<http://emmo.info/emmo/middle/isq#EMMO_ed4af7ae_63a2_497e_bb88_2309619ea405> rdf:type owl:Class ;
                                                                             rdfs:subClassOf <http://emmo.info/emmo/middle/isq#EMMO_1a4c1a97_88a7_4d8e_b2f9_2ca58e92dde4> ;
                                                                             <http://emmo.info/emmo/middle/isq#EMMO_de178b12_5d35_4bca_8efa_a4193162571d> "T0 L0 M+1 I0 T0 N0 J0" ;
                                                                             <http://emmo.info/emmo/top/annotations#EMMO_1f1b164d_ec6a_4faa_8d5e_88bda62316cc> "http://qudt.org/vocab/quantitykind/Mass" ;
                                                                             <http://emmo.info/emmo/top/annotations#EMMO_6dd685dd_1895_46e4_b227_be9f7d643c25> "http://dbpedia.org/page/Mass" ;
                                                                             <http://emmo.info/emmo/top/annotations#EMMO_967080e5_2f42_4eb2_a3a9_c58143e835f9> "Property of a physical body that express its resistance to acceleration (a change in its state of motion) when a force is applied."@en ;
                                                                             <http://emmo.info/emmo/top/annotations#EMMO_fe015383_afb3_44a6_ae86_043628697aa2> "https://doi.org/10.1351/goldbook.M03709" ;
                                                                             <http://www.w3.org/2004/02/skos/core#prefLabel> "Mass"@en .


###  http://emmo.info/emmo/middle/isq#EMMO_f1a51559_aa3d_43a0_9327_918039f0dfed
<http://emmo.info/emmo/middle/isq#EMMO_f1a51559_aa3d_43a0_9327_918039f0dfed> rdf:type owl:Class ;
                                                                             rdfs:subClassOf <http://emmo.info/emmo/middle/isq#EMMO_2946d40b_24a1_47fa_8176_e3f79bb45064> ;
                                                                             <http://emmo.info/emmo/middle/isq#EMMO_de178b12_5d35_4bca_8efa_a4193162571d> "T0 L-3 M0 I0 T0 N0 J0" ;
                                                                             <http://emmo.info/emmo/top/annotations#EMMO_1f1b164d_ec6a_4faa_8d5e_88bda62316cc> "http://qudt.org/vocab/quantitykind/Volume" ;
                                                                             <http://emmo.info/emmo/top/annotations#EMMO_6dd685dd_1895_46e4_b227_be9f7d643c25> "http://dbpedia.org/page/Volume" ;
                                                                             rdfs:comment "Extent of an object in space."@en ;
                                                                             <http://www.w3.org/2004/02/skos/core#prefLabel> "Volume"@en .


###  http://emmo.info/emmo/middle/isq#EMMO_f2ca6dd0_0e5f_4392_a92d_cafdae6cfc95
<http://emmo.info/emmo/middle/isq#EMMO_f2ca6dd0_0e5f_4392_a92d_cafdae6cfc95> rdf:type owl:Class ;
                                                                             rdfs:subClassOf <http://emmo.info/emmo/middle/metrology#EMMO_89762966_8076_4f7c_b745_f718d653e8e2> ;
                                                                             <http://emmo.info/emmo/top/annotations#EMMO_967080e5_2f42_4eb2_a3a9_c58143e835f9> "Physical constant that by definition (after the latest revision of the SI system that was enforsed May 2019) has a known exact numerical value when expressed in SI units."@en ;
                                                                             <http://www.w3.org/2004/02/skos/core#prefLabel> "SIExactConstant"@en .


###  http://emmo.info/emmo/middle/isq#EMMO_f35cff4d_dc09_44cf_a729_22fb79e3bfb2
<http://emmo.info/emmo/middle/isq#EMMO_f35cff4d_dc09_44cf_a729_22fb79e3bfb2> rdf:type owl:Class ;
                                                                             rdfs:subClassOf <http://emmo.info/emmo/middle/metrology#EMMO_02c0621e_a527_4790_8a0f_2bb51973c819> ;
                                                                             <http://emmo.info/emmo/top/annotations#EMMO_967080e5_2f42_4eb2_a3a9_c58143e835f9> "Quantities declared under the ISO 80000."@en ;
                                                                             <http://emmo.info/emmo/top/annotations#EMMO_c84c6752_6d64_48cc_9500_e54a3c34898d> "https://en.wikipedia.org/wiki/International_System_of_Quantities" ;
                                                                             rdfs:seeAlso "https://www.iso.org/obp/ui/#iso:std:iso:80000:-1:ed-1:v1:en:sec:3.1" ;
                                                                             <http://www.w3.org/2004/02/skos/core#prefLabel> "InternationalSystemOfQuantity"@en .


###  http://emmo.info/emmo/middle/isq#EMMO_f3dd74c0_f480_49e8_9764_33b78638c235
<http://emmo.info/emmo/middle/isq#EMMO_f3dd74c0_f480_49e8_9764_33b78638c235> rdf:type owl:Class ;
                                                                             rdfs:subClassOf <http://emmo.info/emmo/middle/isq#EMMO_faab3f84_e475_4a46_af9c_7d249f0b9aef> ;
                                                                             <http://emmo.info/emmo/middle/isq#EMMO_de178b12_5d35_4bca_8efa_a4193162571d> "T0 L0 M0 I0 T0 N0 J0" ;
                                                                             <http://emmo.info/emmo/top/annotations#EMMO_1f1b164d_ec6a_4faa_8d5e_88bda62316cc> "http://qudt.org/vocab/quantitykind/PlaneAngle" ;
                                                                             <http://emmo.info/emmo/top/annotations#EMMO_6dd685dd_1895_46e4_b227_be9f7d643c25> "http://dbpedia.org/page/Angle" ;
                                                                             <http://emmo.info/emmo/top/annotations#EMMO_70fe84ff_99b6_4206_a9fc_9a8931836d84> "Ratio of circular arc length to radius."@en ;
                                                                             <http://emmo.info/emmo/top/annotations#EMMO_fe015383_afb3_44a6_ae86_043628697aa2> "https://doi.org/10.1351/goldbook.A00346" ;
                                                                             <http://www.w3.org/2004/02/skos/core#altLabel> "PlaneAngle"@en ;
                                                                             <http://www.w3.org/2004/02/skos/core#prefLabel> "Angle"@en .


###  http://emmo.info/emmo/middle/isq#EMMO_f6070071_d054_4b17_9d2d_f446f7147d0f
<http://emmo.info/emmo/middle/isq#EMMO_f6070071_d054_4b17_9d2d_f446f7147d0f> rdf:type owl:Class ;
                                                                             rdfs:subClassOf <http://emmo.info/emmo/middle/metrology#EMMO_9895a1b4_f0a5_4167_ac5e_97db40b8bfcc> ;
                                                                             <http://www.w3.org/2004/02/skos/core#prefLabel> "EnergyDimension"@en .


###  http://emmo.info/emmo/middle/isq#EMMO_f84792eb_ec64_4a6b_941f_c9f3e9ef052c
<http://emmo.info/emmo/middle/isq#EMMO_f84792eb_ec64_4a6b_941f_c9f3e9ef052c> rdf:type owl:Class ;
                                                                             rdfs:subClassOf <http://emmo.info/emmo/middle/metrology#EMMO_9895a1b4_f0a5_4167_ac5e_97db40b8bfcc> ;
                                                                             <http://www.w3.org/2004/02/skos/core#prefLabel> "VelocityDimension"@en .


###  http://emmo.info/emmo/middle/isq#EMMO_f96feb3f_4438_4e43_aa44_7458c4d87fc2
<http://emmo.info/emmo/middle/isq#EMMO_f96feb3f_4438_4e43_aa44_7458c4d87fc2> rdf:type owl:Class ;
                                                                             rdfs:subClassOf <http://emmo.info/emmo/middle/isq#EMMO_852b4ab8_fc29_4749_a8c7_b92d4fca7d5a> ,
                                                                                             <http://emmo.info/emmo/middle/isq#EMMO_f2ca6dd0_0e5f_4392_a92d_cafdae6cfc95> ;
                                                                             <http://emmo.info/emmo/middle/isq#EMMO_de178b12_5d35_4bca_8efa_a4193162571d> "T-1 L0 M0 I0 T0 N0 J0" ;
                                                                             <http://emmo.info/emmo/top/annotations#EMMO_967080e5_2f42_4eb2_a3a9_c58143e835f9> """The frequency standard in the SI system in which the photon absorption by transitions between the two hyperfine ground states of caesium-133 atoms are used to control the output frequency.

It defines the base unit second in the SI system."""@en ;
                                                                             <http://emmo.info/emmo/top/annotations#EMMO_a9b3d04c_7ceb_40a2_b8d3_28d514a770a8> "https://physics.nist.gov/cgi-bin/cuu/Value?nucs" ;
                                                                             <http://www.w3.org/2004/02/skos/core#prefLabel> "HyperfineTransitionFrequencyOfCs"@en .


###  http://emmo.info/emmo/middle/isq#EMMO_faab3f84_e475_4a46_af9c_7d249f0b9aef
<http://emmo.info/emmo/middle/isq#EMMO_faab3f84_e475_4a46_af9c_7d249f0b9aef> rdf:type owl:Class ;
                                                                             rdfs:subClassOf <http://emmo.info/emmo/middle/isq#EMMO_a66427d1_9932_4363_9ec5_7d91f2bfda1e> ;
                                                                             <http://emmo.info/emmo/middle/isq#EMMO_de178b12_5d35_4bca_8efa_a4193162571d> "T0 L0 M0 I0 T0 N0 J0" ;
                                                                             <http://emmo.info/emmo/top/annotations#EMMO_967080e5_2f42_4eb2_a3a9_c58143e835f9> "The class of quantities that are the ratio of two quantities with the same physical dimensionality."@en ;
                                                                             <http://emmo.info/emmo/top/annotations#EMMO_b432d2d5_25f4_4165_99c5_5935a7763c1a> """refractive index,
volume fraction,
fine structure constant""" ;
                                                                             rdfs:comment """Quantities defined as ratios `Q=A/B` having equal dimensions in numerator and denominator are dimensionless quantities but still have a physical dimension defined as dim(A)/dim(B).

Johansson, Ingvar (2010). \"Metrological thinking needs the notions of parametric quantities, units and dimensions\". Metrologia. 47 (3): 219230. doi:10.1088/0026-1394/47/3/012. ISSN 0026-1394."""@en ;
                                                                             rdfs:seeAlso "https://iopscience.iop.org/article/10.1088/0026-1394/47/3/012" ;
                                                                             <http://www.w3.org/2004/02/skos/core#prefLabel> "RatioQuantity"@en .


###  http://emmo.info/emmo/middle/isq#EMMO_ffb73b1e_5786_43e4_a964_cb32ac7affb7
<http://emmo.info/emmo/middle/isq#EMMO_ffb73b1e_5786_43e4_a964_cb32ac7affb7> rdf:type owl:Class ;
                                                                             rdfs:subClassOf <http://emmo.info/emmo/middle/isq#EMMO_2946d40b_24a1_47fa_8176_e3f79bb45064> ;
                                                                             <http://emmo.info/emmo/middle/isq#EMMO_de178b12_5d35_4bca_8efa_a4193162571d> "T+3 L-2 M-1 I+2 T0 N0 J0" ;
                                                                             <http://emmo.info/emmo/top/annotations#EMMO_1f1b164d_ec6a_4faa_8d5e_88bda62316cc> "http://qudt.org/vocab/quantitykind/Conductance" ;
                                                                             <http://emmo.info/emmo/top/annotations#EMMO_6dd685dd_1895_46e4_b227_be9f7d643c25> "http://dbpedia.org/page/Electrical_resistance_and_conductance" ;
                                                                             <http://emmo.info/emmo/top/annotations#EMMO_967080e5_2f42_4eb2_a3a9_c58143e835f9> "Measure of the ease for electric current to pass through a material."@en ;
                                                                             <http://emmo.info/emmo/top/annotations#EMMO_fe015383_afb3_44a6_ae86_043628697aa2> "https://doi.org/10.1351/goldbook.E01925" ;
                                                                             rdfs:comment "Inverse of 'ElectricalResistance'."@en ;
                                                                             <http://www.w3.org/2004/02/skos/core#altLabel> "Conductance"@en ;
                                                                             <http://www.w3.org/2004/02/skos/core#prefLabel> "ElectricConductance"@en .


###  http://emmo.info/emmo/middle/isq#EMMO_ffc7735f_c177_46a4_98e9_a54440d29209
<http://emmo.info/emmo/middle/isq#EMMO_ffc7735f_c177_46a4_98e9_a54440d29209> rdf:type owl:Class ;
                                                                             rdfs:subClassOf <http://emmo.info/emmo/middle/isq#EMMO_9bbab0be_f9cc_4f46_9f46_0fd271911b79> ,
                                                                                             <http://emmo.info/emmo/middle/isq#EMMO_f2ca6dd0_0e5f_4392_a92d_cafdae6cfc95> ;
                                                                             <http://emmo.info/emmo/middle/isq#EMMO_de178b12_5d35_4bca_8efa_a4193162571d> "T-2 L+2 M+1 I0 T-1 N0 J0" ;
                                                                             <http://emmo.info/emmo/top/annotations#EMMO_1f1b164d_ec6a_4faa_8d5e_88bda62316cc> "http://qudt.org/vocab/constant/BoltzmannConstant" ;
                                                                             <http://emmo.info/emmo/top/annotations#EMMO_6dd685dd_1895_46e4_b227_be9f7d643c25> "http://dbpedia.org/page/Boltzmann_constant" ;
                                                                             <http://emmo.info/emmo/top/annotations#EMMO_967080e5_2f42_4eb2_a3a9_c58143e835f9> """A physical constant relating energy at the individual particle level with temperature. It is the gas constant R divided by the Avogadro constant.

It defines the Kelvin unit in the SI system."""@en ;
                                                                             <http://emmo.info/emmo/top/annotations#EMMO_a9b3d04c_7ceb_40a2_b8d3_28d514a770a8> "https://physics.nist.gov/cgi-bin/cuu/Value?k" ;
                                                                             <http://emmo.info/emmo/top/annotations#EMMO_fe015383_afb3_44a6_ae86_043628697aa2> "https://doi.org/10.1351/goldbook.B00695" ;
                                                                             rdfs:comment "The DBpedia definition (http://dbpedia.org/page/Boltzmann_constant) is outdated as May 20, 2019. It is now an exact quantity."@en ;
                                                                             <http://www.w3.org/2004/02/skos/core#prefLabel> "BoltzmannConstant"@en .


###  http://emmo.info/emmo/middle/isql#EMMO_7c055d65_2929_40e1_af4f_4bf10995ad50
<http://emmo.info/emmo/middle/isql#EMMO_7c055d65_2929_40e1_af4f_4bf10995ad50> rdf:type owl:Class ;
                                                                              rdfs:subClassOf <http://emmo.info/emmo/middle/chemistry#EMMO_a293f923_954c_4af5_9f97_9600ebd362cb> .


###  http://emmo.info/emmo/middle/manufacturing#EMMO_494b372c_cfdf_47d3_a4de_5e037c540de8
<http://emmo.info/emmo/middle/manufacturing#EMMO_494b372c_cfdf_47d3_a4de_5e037c540de8> rdf:type owl:Class ;
                                                                                       rdfs:subClassOf <http://emmo.info/emmo/middle/manufacturing#EMMO_86ca9b93_1183_4b65_81b8_c0fcd3bba5ad> ;
                                                                                       <http://emmo.info/emmo/top/annotations#EMMO_967080e5_2f42_4eb2_a3a9_c58143e835f9> "An engineered object which is instrumental for reaching a particular purpose through its characteristic functioning process, with particular reference to mechanical or electronic equipment."@en ;
                                                                                       rdfs:comment """From Old French \"deviser\", meaning: arrange, plan, contrive.

Literally \"dispose in portions,\" from Vulgar Latin \"divisare\", frequentative of Latin dividere, meaning \"to divide\""""@en ;
                                                                                       <http://www.w3.org/2004/02/skos/core#prefLabel> "Device"@en .


###  http://emmo.info/emmo/middle/manufacturing#EMMO_71d1c8f0_c6e3_44b5_a4b6_1b74ff35698a
<http://emmo.info/emmo/middle/manufacturing#EMMO_71d1c8f0_c6e3_44b5_a4b6_1b74ff35698a> rdf:type owl:Class ;
                                                                                       rdfs:subClassOf <http://emmo.info/emmo/middle/manufacturing#EMMO_a4d66059_5dd3_4b90_b4cb_10960559441b> ;
                                                                                       <http://emmo.info/emmo/top/annotations#EMMO_967080e5_2f42_4eb2_a3a9_c58143e835f9> "A manufacturing process whose product is the result of the combination of more substances."@en ;
                                                                                       <http://emmo.info/emmo/top/annotations#EMMO_b432d2d5_25f4_4165_99c5_5935a7763c1a> "Synthesis of materials, the preparation of a cake."@en ;
                                                                                       <http://www.w3.org/2004/02/skos/core#prefLabel> "ContinuumManufacturing"@en .


###  http://emmo.info/emmo/middle/manufacturing#EMMO_86ca9b93_1183_4b65_81b8_c0fcd3bba5ad
<http://emmo.info/emmo/middle/manufacturing#EMMO_86ca9b93_1183_4b65_81b8_c0fcd3bba5ad> rdf:type owl:Class ;
                                                                                       rdfs:subClassOf <http://emmo.info/emmo/middle/holistic#EMMO_49804605_c0fe_4538_abda_f70ba1dc8a5d> ;
                                                                                       <http://emmo.info/emmo/top/annotations#EMMO_967080e5_2f42_4eb2_a3a9_c58143e835f9> "A 'physical' that stands for a real world object that has been designed and manufactured for a particular purpose."@en ;
                                                                                       <http://emmo.info/emmo/top/annotations#EMMO_b432d2d5_25f4_4165_99c5_5935a7763c1a> "Car, tire, composite material."@en ;
                                                                                       rdfs:comment "The 'Engineered' branch represents real world objects that show some level of complexity/heterogeneity in their composition, and are made for a specific use."@en ;
                                                                                       <http://www.w3.org/2004/02/skos/core#prefLabel> "Engineered"@en .


###  http://emmo.info/emmo/middle/manufacturing#EMMO_8786cb47_8e1f_4968_9b15_f6d41fc51252
<http://emmo.info/emmo/middle/manufacturing#EMMO_8786cb47_8e1f_4968_9b15_f6d41fc51252> rdf:type owl:Class ;
                                                                                       rdfs:subClassOf <http://emmo.info/emmo/middle/manufacturing#EMMO_a4d66059_5dd3_4b90_b4cb_10960559441b> ;
                                                                                       <http://emmo.info/emmo/top/annotations#EMMO_967080e5_2f42_4eb2_a3a9_c58143e835f9> "A manufacturing process aimed to the production of a device made of specific components."@en ;
                                                                                       <http://emmo.info/emmo/top/annotations#EMMO_b432d2d5_25f4_4165_99c5_5935a7763c1a> "Assemblying a bicycle, building a car."@en ;
                                                                                       <http://www.w3.org/2004/02/skos/core#prefLabel> "DiscreteManufacturing"@en .


###  http://emmo.info/emmo/middle/manufacturing#EMMO_a4d66059_5dd3_4b90_b4cb_10960559441b
<http://emmo.info/emmo/middle/manufacturing#EMMO_a4d66059_5dd3_4b90_b4cb_10960559441b> rdf:type owl:Class ;
                                                                                       rdfs:subClassOf <http://emmo.info/emmo/middle/holistic#EMMO_43e9a05d_98af_41b4_92f6_00f79a09bfce> ;
                                                                                       <http://emmo.info/emmo/top/annotations#EMMO_967080e5_2f42_4eb2_a3a9_c58143e835f9> "The process of transforming raw materials into a product by the use of manual labor, machinery or chemical/biological processes."@en ;
                                                                                       rdfs:comment "From Latin manufacture: \"made by hand\"."@en ;
                                                                                       <http://www.w3.org/2004/02/skos/core#prefLabel> "Manufacturing"@en .


###  http://emmo.info/emmo/middle/manufacturing#EMMO_ec7464a9_d99d_45f8_965b_4e9230ea8356
<http://emmo.info/emmo/middle/manufacturing#EMMO_ec7464a9_d99d_45f8_965b_4e9230ea8356> rdf:type owl:Class ;
                                                                                       rdfs:subClassOf <http://emmo.info/emmo/middle/manufacturing#EMMO_86ca9b93_1183_4b65_81b8_c0fcd3bba5ad> ,
                                                                                                       <http://emmo.info/emmo/middle/physicalistic#EMMO_4207e895_8b83_4318_996a_72cfb32acd94> ;
                                                                                       rdfs:comment "A material that is synthesized within a manufacturing process."@en ;
                                                                                       <http://www.w3.org/2004/02/skos/core#prefLabel> "EngineeredMaterial"@en .


###  http://emmo.info/emmo/middle/materials#EMMO_04f2a2d5_e799_4692_a654_420e76f5acc1
<http://emmo.info/emmo/middle/materials#EMMO_04f2a2d5_e799_4692_a654_420e76f5acc1> rdf:type owl:Class ;
                                                                                   rdfs:subClassOf <http://emmo.info/emmo/middle/materials#EMMO_87ac88ff_8379_4f5a_8c7b_424a8fff1ee8> ,
                                                                                                   <http://emmo.info/emmo/middle/materials#EMMO_b9695e87_8261_412e_83cd_a86459426a28> ;
                                                                                   <http://emmo.info/emmo/top/annotations#EMMO_967080e5_2f42_4eb2_a3a9_c58143e835f9> "Gas is a compressible fluid, a state of matter that has no fixed shape and no fixed volume."@en ;
                                                                                   <http://www.w3.org/2004/02/skos/core#prefLabel> "Gas"@en .


###  http://emmo.info/emmo/middle/materials#EMMO_0b15f4ae_092e_4487_9100_3c44176c545c
<http://emmo.info/emmo/middle/materials#EMMO_0b15f4ae_092e_4487_9100_3c44176c545c> rdf:type owl:Class ;
                                                                                   rdfs:subClassOf <http://emmo.info/emmo/middle/materials#EMMO_ec2c8ac8_98c5_4c74_b85b_ff8e8ca6655c> ;
                                                                                   <http://emmo.info/emmo/top/annotations#EMMO_967080e5_2f42_4eb2_a3a9_c58143e835f9> "A material in which distributed particles of one phase are dispersed in a different continuous phase."@en ;
                                                                                   <http://www.w3.org/2004/02/skos/core#prefLabel> "Dispersion"@en .


###  http://emmo.info/emmo/middle/materials#EMMO_0e030040_98a7_49b2_a871_dced1f3a6131
<http://emmo.info/emmo/middle/materials#EMMO_0e030040_98a7_49b2_a871_dced1f3a6131> rdf:type owl:Class ;
                                                                                   rdfs:subClassOf <http://emmo.info/emmo/middle/materials#EMMO_ec2c8ac8_98c5_4c74_b85b_ff8e8ca6655c> ;
                                                                                   <http://emmo.info/emmo/top/annotations#EMMO_967080e5_2f42_4eb2_a3a9_c58143e835f9> "A mixture in which more than one phases of matter cohexists."@en ;
                                                                                   rdfs:comment """Phase heterogenous mixture may share the same state of matter.

For example, immiscibile liquid phases (e.g. oil and water) constitute a mixture whose phases are clearly separated but share the same state of matter."""@en ;
                                                                                   <http://www.w3.org/2004/02/skos/core#prefLabel> "PhaseHeterogeneousMixture"@en .


###  http://emmo.info/emmo/middle/materials#EMMO_0e6378df_1ce8_4321_b00c_ee9beea60a67
<http://emmo.info/emmo/middle/materials#EMMO_0e6378df_1ce8_4321_b00c_ee9beea60a67> rdf:type owl:Class ;
                                                                                   rdfs:subClassOf <http://emmo.info/emmo/middle/materials#EMMO_ec2c8ac8_98c5_4c74_b85b_ff8e8ca6655c> ;
                                                                                   <http://emmo.info/emmo/top/annotations#EMMO_967080e5_2f42_4eb2_a3a9_c58143e835f9> "A single phase mixture."@en ;
                                                                                   <http://www.w3.org/2004/02/skos/core#prefLabel> "PhaseHomogeneousMixture"@en .


###  http://emmo.info/emmo/middle/materials#EMMO_1067b97a_84f8_4d22_8ace_b842b8ce355c
<http://emmo.info/emmo/middle/materials#EMMO_1067b97a_84f8_4d22_8ace_b842b8ce355c> rdf:type owl:Class ;
                                                                                   rdfs:subClassOf <http://emmo.info/emmo/middle/materials#EMMO_7d66bde4_b68d_41cc_b5fc_6fd98c5e2ff0> ,
                                                                                                   <http://emmo.info/emmo/middle/reductionistic#EMMO_36c79456_e29c_400d_8bd3_0eedddb82652> ;
                                                                                   <http://emmo.info/emmo/top/annotations#EMMO_967080e5_2f42_4eb2_a3a9_c58143e835f9> "A 'spacetime' that stands for a quantum system made of electrons."@en ;
                                                                                   <http://www.w3.org/2004/02/skos/core#prefLabel> "ElectronCloud"@en .


###  http://emmo.info/emmo/middle/materials#EMMO_10dd1eed_da7d_45a3_860c_477ca9e152aa
<http://emmo.info/emmo/middle/materials#EMMO_10dd1eed_da7d_45a3_860c_477ca9e152aa> rdf:type owl:Class ;
                                                                                   rdfs:subClassOf <http://emmo.info/emmo/middle/materials#EMMO_5d659e25_a508_43ed_903c_3707c7c7cd4b> ;
                                                                                   <http://emmo.info/emmo/top/annotations#EMMO_967080e5_2f42_4eb2_a3a9_c58143e835f9> "Nanomaterials are Materials possessing all external dimension measuring 1-100nm"@en ;
                                                                                   <http://www.w3.org/2004/02/skos/core#prefLabel> "NanoParticle"@en .


###  http://emmo.info/emmo/middle/materials#EMMO_1f5e3e7e_72c9_40d4_91dd_ae432d7b7018
<http://emmo.info/emmo/middle/materials#EMMO_1f5e3e7e_72c9_40d4_91dd_ae432d7b7018> rdf:type owl:Class ;
                                                                                   rdfs:subClassOf <http://emmo.info/emmo/middle/materials#EMMO_6c487fb3_03d1_4e56_91ed_c2e16dcbef60> ;
                                                                                   <http://emmo.info/emmo/top/annotations#EMMO_967080e5_2f42_4eb2_a3a9_c58143e835f9> "A colloid formed by trapping pockets of gas in a liquid or solid."@en ;
                                                                                   <http://www.w3.org/2004/02/skos/core#prefLabel> "Foam"@en .


###  http://emmo.info/emmo/middle/materials#EMMO_2031516a_2be7_48e8_9af7_7e1270e308fe
<http://emmo.info/emmo/middle/materials#EMMO_2031516a_2be7_48e8_9af7_7e1270e308fe> rdf:type owl:Class ;
                                                                                   rdfs:subClassOf <http://emmo.info/emmo/middle/materials#EMMO_0b15f4ae_092e_4487_9100_3c44176c545c> ,
                                                                                                   <http://emmo.info/emmo/middle/materials#EMMO_0e6378df_1ce8_4321_b00c_ee9beea60a67> ;
                                                                                   <http://emmo.info/emmo/top/annotations#EMMO_967080e5_2f42_4eb2_a3a9_c58143e835f9> "A solution is a homogeneous mixture composed of two or more substances."@en ;
                                                                                   rdfs:comment "Solutions are characterized by the occurrence of Rayleigh scattering on light,"@en ;
                                                                                   <http://www.w3.org/2004/02/skos/core#prefLabel> "Solution"@en .


###  http://emmo.info/emmo/middle/materials#EMMO_21205421_5783_4d3e_81e5_10c5d894a88a
<http://emmo.info/emmo/middle/materials#EMMO_21205421_5783_4d3e_81e5_10c5d894a88a> rdf:type owl:Class ;
                                                                                   <http://emmo.info/emmo/middle/chemistry#example> "Hydrogen molecule is an adequate definition of a certain molecular entity for some purposes, whereas for others it is necessary to distinguish the electronic state and/or vibrational state and/or nuclear spin, etc. of the hydrogen molecule." ,
                                                                                                                                    "Methane, may mean a single molecule of CH4 (molecular entity) or a molar amount, specified or not (chemical species), participating in a reaction. The degree of precision necessary to describe a molecular entity depends on the context." ;
                                                                                   rdfs:comment """Molecular entity is used as a general term for singular entities, irrespective of their nature, while chemical species stands for sets or ensembles of molecular entities.

Note that the name of a compound may refer to the respective molecular entity or to the chemical species,""" .


###  http://emmo.info/emmo/middle/materials#EMMO_2dd512a1_5187_47cc_b0b8_141214e22b59
<http://emmo.info/emmo/middle/materials#EMMO_2dd512a1_5187_47cc_b0b8_141214e22b59> rdf:type owl:Class ;
                                                                                   rdfs:subClassOf <http://emmo.info/emmo/middle/materials#EMMO_4a464c8d_8895_44a8_a628_aed13509f1bd> ,
                                                                                                   <http://emmo.info/emmo/middle/materials#EMMO_a2b006f2_bbfd_4dba_bcaa_3fca20cd6be1> ;
                                                                                   <http://emmo.info/emmo/top/annotations#EMMO_967080e5_2f42_4eb2_a3a9_c58143e835f9> "A coarse dispersion of solid in a solid continuum phase."@en ;
                                                                                   <http://emmo.info/emmo/top/annotations#EMMO_b432d2d5_25f4_4165_99c5_5935a7763c1a> "Granite, sand, dried concrete."@en ;
                                                                                   <http://www.w3.org/2004/02/skos/core#prefLabel> "SolidSolidSuspension"@en .


###  http://emmo.info/emmo/middle/materials#EMMO_2fd3f574_5e93_47fe_afca_ed80b0a21ab4
<http://emmo.info/emmo/middle/materials#EMMO_2fd3f574_5e93_47fe_afca_ed80b0a21ab4> rdf:type owl:Class ;
                                                                                   rdfs:subClassOf <http://emmo.info/emmo/middle/materials#EMMO_eb77076b_a104_42ac_a065_798b2d2809ad> ;
                                                                                   <http://emmo.info/emmo/top/annotations#EMMO_967080e5_2f42_4eb2_a3a9_c58143e835f9> "An atom that does not share electrons with other atoms."@en ;
                                                                                   rdfs:comment "A standalone atom can be bonded with other atoms by intermolecular forces (i.e. dipoledipole, London dispersion force, hydrogen bonding), since this bonds does not involve electron sharing."@en ;
                                                                                   <http://www.w3.org/2004/02/skos/core#prefLabel> "StandaloneAtom"@en .


###  http://emmo.info/emmo/middle/materials#EMMO_31557fae_b039_491c_bcbb_0ccb8711d5a6
<http://emmo.info/emmo/middle/materials#EMMO_31557fae_b039_491c_bcbb_0ccb8711d5a6> rdf:type owl:Class ;
                                                                                   rdfs:subClassOf <http://emmo.info/emmo/middle/materials#EMMO_6c487fb3_03d1_4e56_91ed_c2e16dcbef60> ;
                                                                                   <http://emmo.info/emmo/top/annotations#EMMO_967080e5_2f42_4eb2_a3a9_c58143e835f9> "A colloid in which small particles (1 nm to 100 nm) are suspended in a continuum phase."@en ;
                                                                                   <http://www.w3.org/2004/02/skos/core#prefLabel> "Sol"@en .


###  http://emmo.info/emmo/middle/materials#EMMO_3397f270_dfc1_4500_8f6f_4d0d85ac5f71
<http://emmo.info/emmo/middle/materials#EMMO_3397f270_dfc1_4500_8f6f_4d0d85ac5f71> rdf:type owl:Class ;
                                                                                   rdfs:subClassOf <http://emmo.info/emmo/middle/physicalistic#EMMO_5b2222df_4da6_442f_8244_96e9e45887d1> ;
                                                                                   <http://emmo.info/emmo/top/annotations#EMMO_967080e5_2f42_4eb2_a3a9_c58143e835f9> "An atom_based state defined by an exact number of e-bonded atomic species and an electron cloud made of the shared electrons."@en ;
                                                                                   <http://emmo.info/emmo/top/annotations#EMMO_b432d2d5_25f4_4165_99c5_5935a7763c1a> "H20, C6H12O6, CH4"@en ;
                                                                                   rdfs:comment """An entity is called essential if removing one direct part will lead to a change in entity class.

An entity is called redundand if removing one direct part will not lead to a change in entity class."""@en ,
                                                                                                """This definition states that this object is a non-periodic set of atoms or a set with a finite periodicity.

Removing an atom from the state will result in another type of atom_based state.

e.g. you cannot remove H from H20 without changing the molecule type (essential). However, you can remove a C from a nanotube (redundant). C60 fullerene is a molecule, since it has a finite periodicity and is made of a well defined number of atoms (essential). A C nanotube is not a molecule, since it has an infinite periodicity (redundant)."""@en ;
                                                                                   <http://www.w3.org/2004/02/skos/core#prefLabel> "Molecule"@en .


###  http://emmo.info/emmo/middle/materials#EMMO_33e0ac8b_a318_4285_b1de_e95347784632
<http://emmo.info/emmo/middle/materials#EMMO_33e0ac8b_a318_4285_b1de_e95347784632> rdf:type owl:Class ;
                                                                                   rdfs:subClassOf <http://emmo.info/emmo/middle/materials#EMMO_4a464c8d_8895_44a8_a628_aed13509f1bd> ,
                                                                                                   <http://emmo.info/emmo/middle/materials#EMMO_a2b006f2_bbfd_4dba_bcaa_3fca20cd6be1> ;
                                                                                   <http://emmo.info/emmo/top/annotations#EMMO_967080e5_2f42_4eb2_a3a9_c58143e835f9> "A coarse dispersion of liquid in a solid continuum phase."@en ;
                                                                                   <http://www.w3.org/2004/02/skos/core#prefLabel> "SolidLiquidSuspension"@en .


###  http://emmo.info/emmo/middle/materials#EMMO_3995e22d_5720_4dcf_ba3b_d0ce03f514c6
<http://emmo.info/emmo/middle/materials#EMMO_3995e22d_5720_4dcf_ba3b_d0ce03f514c6> rdf:type owl:Class ;
                                                                                   rdfs:subClassOf <http://emmo.info/emmo/middle/materials#EMMO_6c487fb3_03d1_4e56_91ed_c2e16dcbef60> ,
                                                                                                   <http://emmo.info/emmo/middle/materials#EMMO_a2b006f2_bbfd_4dba_bcaa_3fca20cd6be1> ;
                                                                                   <http://emmo.info/emmo/top/annotations#EMMO_967080e5_2f42_4eb2_a3a9_c58143e835f9> "A soft, solid or solid-like colloid consisting of two or more components, one of which is a liquid, present in substantial quantity."@en ;
                                                                                   <http://www.w3.org/2004/02/skos/core#prefLabel> "Gel"@en .


###  http://emmo.info/emmo/middle/materials#EMMO_40e18c93_a1b5_49ff_b06a_d9d932d1fb65
<http://emmo.info/emmo/middle/materials#EMMO_40e18c93_a1b5_49ff_b06a_d9d932d1fb65> rdf:type owl:Class ;
                                                                                   rdfs:subClassOf <http://emmo.info/emmo/middle/materials#EMMO_6c487fb3_03d1_4e56_91ed_c2e16dcbef60> ,
                                                                                                   <http://emmo.info/emmo/middle/materials#EMMO_7509da43_56b1_4d7f_887a_65d1663df4ba> ;
                                                                                   <http://emmo.info/emmo/top/annotations#EMMO_967080e5_2f42_4eb2_a3a9_c58143e835f9> "An emulsion is a mixture of two or more liquids that are normally immiscible (a liquid-liquid heterogeneous mixture)."@en ;
                                                                                   <http://emmo.info/emmo/top/annotations#EMMO_b432d2d5_25f4_4165_99c5_5935a7763c1a> "Mayonnaise, milk."@en ;
                                                                                   <http://www.w3.org/2004/02/skos/core#prefLabel> "Emulsion"@en .


###  http://emmo.info/emmo/middle/materials#EMMO_42185fe7_122c_4e0c_a3cd_659d3e21c389
<http://emmo.info/emmo/middle/materials#EMMO_42185fe7_122c_4e0c_a3cd_659d3e21c389> rdf:type owl:Class ;
                                                                                   rdfs:subClassOf <http://emmo.info/emmo/middle/materials#EMMO_4a464c8d_8895_44a8_a628_aed13509f1bd> ,
                                                                                                   <http://emmo.info/emmo/middle/materials#EMMO_7509da43_56b1_4d7f_887a_65d1663df4ba> ;
                                                                                   <http://emmo.info/emmo/top/annotations#EMMO_967080e5_2f42_4eb2_a3a9_c58143e835f9> "A coarse dispersion of gas in a liquid continuum phase."@en ;
                                                                                   <http://emmo.info/emmo/top/annotations#EMMO_b432d2d5_25f4_4165_99c5_5935a7763c1a> "Sparkling water"@en ;
                                                                                   <http://www.w3.org/2004/02/skos/core#prefLabel> "LiquidGasSuspension"@en .


###  http://emmo.info/emmo/middle/materials#EMMO_4354ac74_7425_43ab_92e4_6dc19d1afee9
<http://emmo.info/emmo/middle/materials#EMMO_4354ac74_7425_43ab_92e4_6dc19d1afee9> rdf:type owl:Class ;
                                                                                   rdfs:subClassOf <http://emmo.info/emmo/middle/materials#EMMO_31557fae_b039_491c_bcbb_0ccb8711d5a6> ,
                                                                                                   <http://emmo.info/emmo/middle/materials#EMMO_7509da43_56b1_4d7f_887a_65d1663df4ba> ;
                                                                                   <http://emmo.info/emmo/top/annotations#EMMO_967080e5_2f42_4eb2_a3a9_c58143e835f9> "A type of sol in the form of one solid dispersed in liquid."@en ;
                                                                                   <http://www.w3.org/2004/02/skos/core#prefLabel> "LiquidSol"@en .


###  http://emmo.info/emmo/middle/materials#EMMO_4588526f_8553_4f4d_aa73_a483e88d599b
<http://emmo.info/emmo/middle/materials#EMMO_4588526f_8553_4f4d_aa73_a483e88d599b> rdf:type owl:Class ;
                                                                                   rdfs:subClassOf <http://emmo.info/emmo/middle/materials#EMMO_2fd3f574_5e93_47fe_afca_ed80b0a21ab4> ;
                                                                                   <http://emmo.info/emmo/top/annotations#EMMO_967080e5_2f42_4eb2_a3a9_c58143e835f9> "A standalone atom that has no net charge."@en ;
                                                                                   <http://www.w3.org/2004/02/skos/core#prefLabel> "NeutralAtom"@en .


###  http://emmo.info/emmo/middle/materials#EMMO_47fe2379_be21_48d1_9ede_402f0faf494b
<http://emmo.info/emmo/middle/materials#EMMO_47fe2379_be21_48d1_9ede_402f0faf494b> rdf:type owl:Class ;
                                                                                   rdfs:subClassOf <http://emmo.info/emmo/middle/materials#EMMO_4a464c8d_8895_44a8_a628_aed13509f1bd> ,
                                                                                                   <http://emmo.info/emmo/middle/materials#EMMO_7509da43_56b1_4d7f_887a_65d1663df4ba> ;
                                                                                   <http://emmo.info/emmo/top/annotations#EMMO_967080e5_2f42_4eb2_a3a9_c58143e835f9> "A coarse dispersion of liquid in a liquid continuum phase."@en ;
                                                                                   <http://www.w3.org/2004/02/skos/core#prefLabel> "LiquidLiquidSuspension"@en .


###  http://emmo.info/emmo/middle/materials#EMMO_498aad49_f8d4_40a4_a9eb_efd563a0115f
<http://emmo.info/emmo/middle/materials#EMMO_498aad49_f8d4_40a4_a9eb_efd563a0115f> rdf:type owl:Class ;
                                                                                   rdfs:subClassOf <http://emmo.info/emmo/middle/materials#EMMO_e0edfb9e_9a96_4fae_b942_831ffe27b84a> ;
                                                                                   <http://emmo.info/emmo/top/annotations#EMMO_967080e5_2f42_4eb2_a3a9_c58143e835f9> "A suspension of liquid droplets dispersed in a gas through an atomization process."@en ;
                                                                                   <http://www.w3.org/2004/02/skos/core#prefLabel> "Spray"@en .


###  http://emmo.info/emmo/middle/materials#EMMO_4a464c8d_8895_44a8_a628_aed13509f1bd
<http://emmo.info/emmo/middle/materials#EMMO_4a464c8d_8895_44a8_a628_aed13509f1bd> rdf:type owl:Class ;
                                                                                   rdfs:subClassOf <http://emmo.info/emmo/middle/materials#EMMO_0b15f4ae_092e_4487_9100_3c44176c545c> ,
                                                                                                   <http://emmo.info/emmo/middle/materials#EMMO_0e030040_98a7_49b2_a871_dced1f3a6131> ,
                                                                                                   <http://emmo.info/emmo/middle/materials#EMMO_b9695e87_8261_412e_83cd_a86459426a28> ;
                                                                                   <http://emmo.info/emmo/top/annotations#EMMO_967080e5_2f42_4eb2_a3a9_c58143e835f9> "An heterogeneous mixture that contains coarsly dispersed particles (no Tyndall effect), that generally tend to separate in time to the dispersion medium phase."@en ;
                                                                                   rdfs:comment "Suspensions show no significant effect on light."@en ;
                                                                                   <http://www.w3.org/2004/02/skos/core#prefLabel> "Suspension"@en .


###  http://emmo.info/emmo/middle/materials#EMMO_4b3e2374_52a1_4420_8e3f_3ae6b9bf7dff
<http://emmo.info/emmo/middle/materials#EMMO_4b3e2374_52a1_4420_8e3f_3ae6b9bf7dff> rdf:type owl:Class ;
                                                                                   rdfs:subClassOf <http://emmo.info/emmo/middle/materials#EMMO_2031516a_2be7_48e8_9af7_7e1270e308fe> ,
                                                                                                   <http://emmo.info/emmo/middle/materials#EMMO_7509da43_56b1_4d7f_887a_65d1663df4ba> ;
                                                                                   <http://emmo.info/emmo/top/annotations#EMMO_967080e5_2f42_4eb2_a3a9_c58143e835f9> "A liquid solution made of two or more component substances."@en ;
                                                                                   <http://www.w3.org/2004/02/skos/core#prefLabel> "LiquidSolution"@en .


###  http://emmo.info/emmo/middle/materials#EMMO_4c21fb86_fdcf_444e_b498_86fe656295af
<http://emmo.info/emmo/middle/materials#EMMO_4c21fb86_fdcf_444e_b498_86fe656295af> rdf:type owl:Class ;
                                                                                   rdfs:subClassOf <http://emmo.info/emmo/middle/materials#EMMO_87ac88ff_8379_4f5a_8c7b_424a8fff1ee8> ,
                                                                                                   <http://emmo.info/emmo/middle/materials#EMMO_b9695e87_8261_412e_83cd_a86459426a28> ;
                                                                                   <http://emmo.info/emmo/top/annotations#EMMO_967080e5_2f42_4eb2_a3a9_c58143e835f9> "A fluid in which a gas is ionized to a level where its electrical conductivity allows long-range electric and magnetic fields to dominate its behaviour."@en ;
                                                                                   <http://www.w3.org/2004/02/skos/core#prefLabel> "Plasma"@en .


###  http://emmo.info/emmo/middle/materials#EMMO_4d604a13_d1f6_42fd_818f_d3138d5e308c
<http://emmo.info/emmo/middle/materials#EMMO_4d604a13_d1f6_42fd_818f_d3138d5e308c> rdf:type owl:Class ;
                                                                                   rdfs:subClassOf <http://emmo.info/emmo/middle/materials#EMMO_94010cbc_c2a6_4cb9_b29a_83aa99d2ff70> ;
                                                                                   <http://emmo.info/emmo/top/annotations#EMMO_967080e5_2f42_4eb2_a3a9_c58143e835f9> "A liquid aerosol composed of water droplets in air or another gas."@en ;
                                                                                   <http://www.w3.org/2004/02/skos/core#prefLabel> "Vapor"@en .


###  http://emmo.info/emmo/middle/materials#EMMO_50781fd9_a9e4_46ad_b7be_4500371d188d
<http://emmo.info/emmo/middle/materials#EMMO_50781fd9_a9e4_46ad_b7be_4500371d188d> rdf:type owl:Class ;
                                                                                   rdfs:subClassOf <http://emmo.info/emmo/middle/materials#EMMO_7d66bde4_b68d_41cc_b5fc_6fd98c5e2ff0> ,
                                                                                                   <http://emmo.info/emmo/middle/reductionistic#EMMO_36c79456_e29c_400d_8bd3_0eedddb82652> ;
                                                                                   <http://www.w3.org/2004/02/skos/core#prefLabel> "Nucleon"@en .


###  http://emmo.info/emmo/middle/materials#EMMO_560d833a_6184_410c_859a_05d982712fd7
<http://emmo.info/emmo/middle/materials#EMMO_560d833a_6184_410c_859a_05d982712fd7> rdf:type owl:Class ;
                                                                                   rdfs:subClassOf <http://emmo.info/emmo/middle/materials#EMMO_04f2a2d5_e799_4692_a654_420e76f5acc1> ,
                                                                                                   <http://emmo.info/emmo/middle/materials#EMMO_6c487fb3_03d1_4e56_91ed_c2e16dcbef60> ;
                                                                                   <http://emmo.info/emmo/top/annotations#EMMO_967080e5_2f42_4eb2_a3a9_c58143e835f9> "A colloid composed of fine solid particles or liquid droplets in air or another gas."@en ;
                                                                                   <http://www.w3.org/2004/02/skos/core#prefLabel> "Aerosol"@en .


###  http://emmo.info/emmo/middle/materials#EMMO_5a2af26d_99de_4e5e_b1cd_514be71420c3
<http://emmo.info/emmo/middle/materials#EMMO_5a2af26d_99de_4e5e_b1cd_514be71420c3> rdf:type owl:Class ;
                                                                                   rdfs:subClassOf <http://emmo.info/emmo/middle/materials#EMMO_96c8d72f_b436_44e2_9f7f_085c24094292> ;
                                                                                   <http://emmo.info/emmo/top/annotations#EMMO_967080e5_2f42_4eb2_a3a9_c58143e835f9> "Smoke is a solid aerosol made of particles emitted when a material undergoes combustion or pyrolysis."@en ;
                                                                                   <http://www.w3.org/2004/02/skos/core#prefLabel> "Smoke"@en .


###  http://emmo.info/emmo/middle/materials#EMMO_5add9885_dc98_4fa5_8482_fdf9ba5e3889
<http://emmo.info/emmo/middle/materials#EMMO_5add9885_dc98_4fa5_8482_fdf9ba5e3889> rdf:type owl:Class ;
                                                                                   rdfs:subClassOf <http://emmo.info/emmo/middle/materials#EMMO_31557fae_b039_491c_bcbb_0ccb8711d5a6> ,
                                                                                                   <http://emmo.info/emmo/middle/materials#EMMO_a2b006f2_bbfd_4dba_bcaa_3fca20cd6be1> ;
                                                                                   <http://emmo.info/emmo/top/annotations#EMMO_967080e5_2f42_4eb2_a3a9_c58143e835f9> "A type of sol in the form of one solid dispersed in another continuous solid."@en ;
                                                                                   <http://www.w3.org/2004/02/skos/core#prefLabel> "SolidSol"@en .


###  http://emmo.info/emmo/middle/materials#EMMO_5be9c137_325a_43d8_b7cd_ea93e7721c2d
<http://emmo.info/emmo/middle/materials#EMMO_5be9c137_325a_43d8_b7cd_ea93e7721c2d> rdf:type owl:Class ;
                                                                                   rdfs:subClassOf <http://emmo.info/emmo/middle/materials#EMMO_04f2a2d5_e799_4692_a654_420e76f5acc1> ,
                                                                                                   <http://emmo.info/emmo/middle/materials#EMMO_2031516a_2be7_48e8_9af7_7e1270e308fe> ;
                                                                                   <http://emmo.info/emmo/top/annotations#EMMO_967080e5_2f42_4eb2_a3a9_c58143e835f9> "A gaseous solution made of more than one component type."@en ;
                                                                                   <http://www.w3.org/2004/02/skos/core#prefLabel> "GasMixture"@en .


###  http://emmo.info/emmo/middle/materials#EMMO_5cb107ba_7daa_46dd_8f9f_da22a6eac676
<http://emmo.info/emmo/middle/materials#EMMO_5cb107ba_7daa_46dd_8f9f_da22a6eac676> rdf:type owl:Class ;
                                                                                   rdfs:subClassOf <http://emmo.info/emmo/middle/materials#EMMO_4b3e2374_52a1_4420_8e3f_3ae6b9bf7dff> ;
                                                                                   <http://emmo.info/emmo/top/annotations#EMMO_967080e5_2f42_4eb2_a3a9_c58143e835f9> "A liquid solution in which the solvent is water."@en ;
                                                                                   <http://www.w3.org/2004/02/skos/core#prefLabel> "AcqueousSolution"@en .


###  http://emmo.info/emmo/middle/materials#EMMO_5d659e25_a508_43ed_903c_3707c7c7cd4b
<http://emmo.info/emmo/middle/materials#EMMO_5d659e25_a508_43ed_903c_3707c7c7cd4b> rdf:type owl:Class ;
                                                                                   rdfs:subClassOf <http://emmo.info/emmo/middle/physicalistic#EMMO_4207e895_8b83_4318_996a_72cfb32acd94> ;
                                                                                   <http://emmo.info/emmo/top/annotations#EMMO_967080e5_2f42_4eb2_a3a9_c58143e835f9> "Nanomaterials are Materials possessing, at minimum, one external dimension measuring 1-100nm"@en ;
                                                                                   <http://www.w3.org/2004/02/skos/core#prefLabel> "NanoMaterial"@en .


###  http://emmo.info/emmo/middle/materials#EMMO_5e77f00d_5c0a_44e7_baf1_2c2a4cb5b3ae
<http://emmo.info/emmo/middle/materials#EMMO_5e77f00d_5c0a_44e7_baf1_2c2a4cb5b3ae> rdf:type owl:Class ;
                                                                                   rdfs:subClassOf <http://emmo.info/emmo/middle/materials#EMMO_2031516a_2be7_48e8_9af7_7e1270e308fe> ,
                                                                                                   <http://emmo.info/emmo/middle/materials#EMMO_a2b006f2_bbfd_4dba_bcaa_3fca20cd6be1> ;
                                                                                   <http://emmo.info/emmo/top/annotations#EMMO_967080e5_2f42_4eb2_a3a9_c58143e835f9> "A solid solution made of two or more component substances."@en ;
                                                                                   <http://www.w3.org/2004/02/skos/core#prefLabel> "SolidSolution"@en .


###  http://emmo.info/emmo/middle/materials#EMMO_668fbd5b_6f1b_405c_9c6b_d6067bd0595a
<http://emmo.info/emmo/middle/materials#EMMO_668fbd5b_6f1b_405c_9c6b_d6067bd0595a> rdf:type owl:Class ;
                                                                                   rdfs:subClassOf <http://emmo.info/emmo/middle/materials#EMMO_8b0923ab_b500_477b_9ce9_8b3a3e4dc4f2> ;
                                                                                   <http://emmo.info/emmo/top/annotations#EMMO_967080e5_2f42_4eb2_a3a9_c58143e835f9> "A matter object throughout which all physical properties of a material are essentially uniform."@en ;
                                                                                   rdfs:comment """In the physical sciences, a phase is a region of space (a thermodynamic system), throughout which all physical properties of a material are essentially uniform. Examples of physical properties include density, index of refraction, magnetization and chemical composition. A simple description is that a phase is a region of material that is chemically uniform, physically distinct, and (often) mechanically separable. In a system consisting of ice and water in a glass jar, the ice cubes are one phase, the water is a second phase, and the humid air is a third phase over the ice and water. The glass of the jar is another separate phase.

The term phase is sometimes used as a synonym for state of matter, but there can be several immiscible phases of the same state of matter. Also, the term phase is sometimes used to refer to a set of equilibrium states demarcated in terms of state variables such as pressure and temperature by a phase boundary on a phase diagram. Because phase boundaries relate to changes in the organization of matter, such as a change from liquid to solid or a more subtle change from one crystal structure to another, this latter usage is similar to the use of \"phase\" as a synonym for state of matter. However, the state of matter and phase diagram usages are not commensurate with the formal definition given above and the intended meaning must be determined in part from the context in which the term is used.

[https://en.wikipedia.org/wiki/Phase_(matter)]"""@en ;
                                                                                   <http://www.w3.org/2004/02/skos/core#prefLabel> "PhaseOfMatter"@en .


###  http://emmo.info/emmo/middle/materials#EMMO_68390bfb_e307_479d_8f78_d66d8773cb1d
<http://emmo.info/emmo/middle/materials#EMMO_68390bfb_e307_479d_8f78_d66d8773cb1d> rdf:type owl:Class ;
                                                                                   rdfs:subClassOf <http://emmo.info/emmo/middle/physicalistic#EMMO_4207e895_8b83_4318_996a_72cfb32acd94> ;
                                                                                   <http://emmo.info/emmo/top/annotations#EMMO_967080e5_2f42_4eb2_a3a9_c58143e835f9> "A material that undergoes chemical changes."@en ;
                                                                                   <http://www.w3.org/2004/02/skos/core#prefLabel> "ReactiveMaterial"@en .


###  http://emmo.info/emmo/middle/materials#EMMO_6c487fb3_03d1_4e56_91ed_c2e16dcbef60
<http://emmo.info/emmo/middle/materials#EMMO_6c487fb3_03d1_4e56_91ed_c2e16dcbef60> rdf:type owl:Class ;
                                                                                   rdfs:subClassOf <http://emmo.info/emmo/middle/materials#EMMO_0b15f4ae_092e_4487_9100_3c44176c545c> ,
                                                                                                   <http://emmo.info/emmo/middle/materials#EMMO_0e030040_98a7_49b2_a871_dced1f3a6131> ;
                                                                                   <http://emmo.info/emmo/top/annotations#EMMO_967080e5_2f42_4eb2_a3a9_c58143e835f9> "A mixture in which one substance of microscopically dispersed insoluble or soluble particles (from 1 nm to 1 m) is suspended throughout another substance and that does not settle, or would take a very long time to settle appreciably."@en ;
                                                                                   rdfs:comment "Colloids are characterized by the occurring of the Tyndall effect on light."@en ;
                                                                                   <http://www.w3.org/2004/02/skos/core#prefLabel> "Colloid"@en .


###  http://emmo.info/emmo/middle/materials#EMMO_7509da43_56b1_4d7f_887a_65d1663df4ba
<http://emmo.info/emmo/middle/materials#EMMO_7509da43_56b1_4d7f_887a_65d1663df4ba> rdf:type owl:Class ;
                                                                                   rdfs:subClassOf <http://emmo.info/emmo/middle/materials#EMMO_87ac88ff_8379_4f5a_8c7b_424a8fff1ee8> ,
                                                                                                   <http://emmo.info/emmo/middle/materials#EMMO_b9695e87_8261_412e_83cd_a86459426a28> ;
                                                                                   <http://emmo.info/emmo/top/annotations#EMMO_967080e5_2f42_4eb2_a3a9_c58143e835f9> "A liquid is a nearly incompressible fluid that conforms to the shape of its container but retains a (nearly) constant volume independent of pressure."@en ;
                                                                                   <http://www.w3.org/2004/02/skos/core#prefLabel> "Liquid"@en .


###  http://emmo.info/emmo/middle/materials#EMMO_75fe4fd1_0f7e_429b_b91d_59d248561bae
<http://emmo.info/emmo/middle/materials#EMMO_75fe4fd1_0f7e_429b_b91d_59d248561bae> rdf:type owl:Class ;
                                                                                   rdfs:subClassOf <http://emmo.info/emmo/middle/physicalistic#EMMO_4207e895_8b83_4318_996a_72cfb32acd94> ;
                                                                                   <http://emmo.info/emmo/top/annotations#EMMO_967080e5_2f42_4eb2_a3a9_c58143e835f9> "A Material occurring in nature, without the need of human intervention."@en ;
                                                                                   <http://www.w3.org/2004/02/skos/core#prefLabel> "NaturalMaterial"@en .


###  http://emmo.info/emmo/middle/materials#EMMO_7d66bde4_b68d_41cc_b5fc_6fd98c5e2ff0
<http://emmo.info/emmo/middle/materials#EMMO_7d66bde4_b68d_41cc_b5fc_6fd98c5e2ff0> rdf:type owl:Class ;
                                                                                   rdfs:subClassOf <http://emmo.info/emmo/middle/physicalistic#EMMO_5b2222df_4da6_442f_8244_96e9e45887d1> ;
                                                                                   <http://www.w3.org/2004/02/skos/core#prefLabel> "Subatomic"@en .


###  http://emmo.info/emmo/middle/materials#EMMO_8303a247_f9d9_4616_bdcd_f5cbd7b298e3
<http://emmo.info/emmo/middle/materials#EMMO_8303a247_f9d9_4616_bdcd_f5cbd7b298e3> rdf:type owl:Class ;
                                                                                   rdfs:subClassOf <http://emmo.info/emmo/middle/materials#EMMO_eb77076b_a104_42ac_a065_798b2d2809ad> ;
                                                                                   <http://emmo.info/emmo/top/annotations#EMMO_967080e5_2f42_4eb2_a3a9_c58143e835f9> "An bonded atom that shares at least one electron to the atom-based entity of which is part of."@en ;
                                                                                   rdfs:comment """A real bond between atoms is always something hybrid between covalent, metallic and ionic.

In general, metallic and ionic bonds have atoms sharing electrons."""@en ,
                                                                                                "The bond types that are covered by this definition are the strong electonic bonds: covalent, metallic and ionic."@en ,
                                                                                                "This class can be used to represent molecules as simplified quantum systems, in which outer molecule shared electrons are un-entangled with the inner shells of the atoms composing the molecule."@en ;
                                                                                   <http://www.w3.org/2004/02/skos/core#prefLabel> "BondedAtom"@en .


###  http://emmo.info/emmo/middle/materials#EMMO_87ac88ff_8379_4f5a_8c7b_424a8fff1ee8
<http://emmo.info/emmo/middle/materials#EMMO_87ac88ff_8379_4f5a_8c7b_424a8fff1ee8> rdf:type owl:Class ;
                                                                                   rdfs:subClassOf <http://emmo.info/emmo/middle/materials#EMMO_8b0923ab_b500_477b_9ce9_8b3a3e4dc4f2> ;
                                                                                   <http://emmo.info/emmo/top/annotations#EMMO_967080e5_2f42_4eb2_a3a9_c58143e835f9> "A continuum that has no fixed shape and yields easily to external pressure."@en ;
                                                                                   <http://emmo.info/emmo/top/annotations#EMMO_b432d2d5_25f4_4165_99c5_5935a7763c1a> "Gas, liquid, plasma,"@en ;
                                                                                   <http://www.w3.org/2004/02/skos/core#prefLabel> "Fluid"@en .


###  http://emmo.info/emmo/middle/materials#EMMO_8b0923ab_b500_477b_9ce9_8b3a3e4dc4f2
<http://emmo.info/emmo/middle/materials#EMMO_8b0923ab_b500_477b_9ce9_8b3a3e4dc4f2> rdf:type owl:Class ;
                                                                                   rdfs:subClassOf <http://emmo.info/emmo/middle/physicalistic#EMMO_5b2222df_4da6_442f_8244_96e9e45887d1> ;
                                                                                   <http://emmo.info/emmo/top/annotations#EMMO_967080e5_2f42_4eb2_a3a9_c58143e835f9> """A state that is a collection of sufficiently large number of other parts such that:
- it is the bearer of qualities that can exists only by the fact that it is a sum of parts
- the smallest partition dV of the state volume in which we are interested in, contains enough parts to be statistically consistent: n [#/m3] x dV [m3] >> 1"""@en ;
                                                                                   rdfs:comment "A continuum is made of a sufficient number of parts that it continues to exists as continuum individual even after the loss of one of them i.e. a continuum is a redundant."@en ,
                                                                                                """A continuum is not necessarily small (i.e. composed by the minimum amount of sates to fulfill the definition).

A single continuum individual can be the whole fluid in a pipe."""@en ,
                                                                                                "A continuum is the bearer of properties that are generated by the interactions of parts such as viscosity and thermal or electrical conductivity."@en ;
                                                                                   <http://www.w3.org/2004/02/skos/core#prefLabel> "Continuum"@en .


###  http://emmo.info/emmo/middle/materials#EMMO_8f87e700_99a8_4427_8ffb_e493de05c217
<http://emmo.info/emmo/middle/materials#EMMO_8f87e700_99a8_4427_8ffb_e493de05c217> rdf:type owl:Class ;
                                                                                   rdfs:subClassOf <http://emmo.info/emmo/middle/materials#EMMO_50781fd9_a9e4_46ad_b7be_4500371d188d> ;
                                                                                   <http://www.w3.org/2004/02/skos/core#prefLabel> "Proton"@en .


###  http://emmo.info/emmo/middle/materials#EMMO_94010cbc_c2a6_4cb9_b29a_83aa99d2ff70
<http://emmo.info/emmo/middle/materials#EMMO_94010cbc_c2a6_4cb9_b29a_83aa99d2ff70> rdf:type owl:Class ;
                                                                                   rdfs:subClassOf <http://emmo.info/emmo/middle/materials#EMMO_560d833a_6184_410c_859a_05d982712fd7> ;
                                                                                   <http://emmo.info/emmo/top/annotations#EMMO_967080e5_2f42_4eb2_a3a9_c58143e835f9> "An aerosol composed of liquid droplets in air or another gas."@en ;
                                                                                   <http://www.w3.org/2004/02/skos/core#prefLabel> "LiquidAerosol"@en .


###  http://emmo.info/emmo/middle/materials#EMMO_96c8d72f_b436_44e2_9f7f_085c24094292
<http://emmo.info/emmo/middle/materials#EMMO_96c8d72f_b436_44e2_9f7f_085c24094292> rdf:type owl:Class ;
                                                                                   rdfs:subClassOf <http://emmo.info/emmo/middle/materials#EMMO_560d833a_6184_410c_859a_05d982712fd7> ;
                                                                                   <http://emmo.info/emmo/top/annotations#EMMO_967080e5_2f42_4eb2_a3a9_c58143e835f9> "An aerosol composed of fine solid particles in air or another gas."@en ;
                                                                                   <http://www.w3.org/2004/02/skos/core#prefLabel> "SolidAerosol"@en .


###  http://emmo.info/emmo/middle/materials#EMMO_9bed5d66_805a_4b3a_9153_beaf67143848
<http://emmo.info/emmo/middle/materials#EMMO_9bed5d66_805a_4b3a_9153_beaf67143848> rdf:type owl:Class ;
                                                                                   rdfs:subClassOf <http://emmo.info/emmo/middle/materials#EMMO_1f5e3e7e_72c9_40d4_91dd_ae432d7b7018> ,
                                                                                                   <http://emmo.info/emmo/middle/materials#EMMO_a2b006f2_bbfd_4dba_bcaa_3fca20cd6be1> ;
                                                                                   <http://emmo.info/emmo/top/annotations#EMMO_967080e5_2f42_4eb2_a3a9_c58143e835f9> "A foam of trapped gas in a solid."@en ;
                                                                                   <http://emmo.info/emmo/top/annotations#EMMO_b432d2d5_25f4_4165_99c5_5935a7763c1a> "Aerogel"@en ;
                                                                                   <http://www.w3.org/2004/02/skos/core#prefLabel> "SolidFoam"@en .


###  http://emmo.info/emmo/middle/materials#EMMO_a2b006f2_bbfd_4dba_bcaa_3fca20cd6be1
<http://emmo.info/emmo/middle/materials#EMMO_a2b006f2_bbfd_4dba_bcaa_3fca20cd6be1> rdf:type owl:Class ;
                                                                                   rdfs:subClassOf <http://emmo.info/emmo/middle/materials#EMMO_b9695e87_8261_412e_83cd_a86459426a28> ;
                                                                                   <http://emmo.info/emmo/top/annotations#EMMO_967080e5_2f42_4eb2_a3a9_c58143e835f9> "A continuum characterized by structural rigidity and resistance to changes of shape or volume, that retains its shape and density when not confined."@en ;
                                                                                   <http://www.w3.org/2004/02/skos/core#prefLabel> "Solid"@en .


###  http://emmo.info/emmo/middle/materials#EMMO_b9695e87_8261_412e_83cd_a86459426a28
<http://emmo.info/emmo/middle/materials#EMMO_b9695e87_8261_412e_83cd_a86459426a28> rdf:type owl:Class ;
                                                                                   rdfs:subClassOf <http://emmo.info/emmo/middle/materials#EMMO_8b0923ab_b500_477b_9ce9_8b3a3e4dc4f2> ;
                                                                                   <http://emmo.info/emmo/top/annotations#EMMO_967080e5_2f42_4eb2_a3a9_c58143e835f9> "A superclass made as the disjoint union of all the form under which matter can exist."@en ;
                                                                                   rdfs:comment """In physics, a state of matter is one of the distinct forms in which matter can exist. Four states of matter are observable in everyday life: solid, liquid, gas, and plasma.

https://en.wikipedia.org/wiki/State_of_matter"""@en ;
                                                                                   <http://www.w3.org/2004/02/skos/core#prefLabel> "StateOfMatter"@en .


###  http://emmo.info/emmo/middle/materials#EMMO_c457b6b9_5e73_4853_ae08_d776c12b8058
<http://emmo.info/emmo/middle/materials#EMMO_c457b6b9_5e73_4853_ae08_d776c12b8058> rdf:type owl:Class ;
                                                                                   rdfs:subClassOf <http://emmo.info/emmo/middle/materials#EMMO_4a464c8d_8895_44a8_a628_aed13509f1bd> ,
                                                                                                   <http://emmo.info/emmo/middle/materials#EMMO_a2b006f2_bbfd_4dba_bcaa_3fca20cd6be1> ;
                                                                                   <http://emmo.info/emmo/top/annotations#EMMO_967080e5_2f42_4eb2_a3a9_c58143e835f9> "A coarse dispersion of gas in a solid continuum phase."@en ;
                                                                                   <http://www.w3.org/2004/02/skos/core#prefLabel> "SolidGasSuspension"@en .


###  http://emmo.info/emmo/middle/materials#EMMO_d4f37e32_16ae_4cc6_b4cd_fd896b2449c4
<http://emmo.info/emmo/middle/materials#EMMO_d4f37e32_16ae_4cc6_b4cd_fd896b2449c4> rdf:type owl:Class ;
                                                                                   rdfs:subClassOf <http://emmo.info/emmo/middle/materials#EMMO_04f2a2d5_e799_4692_a654_420e76f5acc1> ,
                                                                                                   <http://emmo.info/emmo/middle/materials#EMMO_4a464c8d_8895_44a8_a628_aed13509f1bd> ;
                                                                                   <http://emmo.info/emmo/top/annotations#EMMO_967080e5_2f42_4eb2_a3a9_c58143e835f9> "A coarse dispersion of solid in a gas continuum phase."@en ;
                                                                                   <http://emmo.info/emmo/top/annotations#EMMO_b432d2d5_25f4_4165_99c5_5935a7763c1a> "Dust, sand storm."@en ;
                                                                                   <http://www.w3.org/2004/02/skos/core#prefLabel> "GasSolidSuspension"@en .


###  http://emmo.info/emmo/middle/materials#EMMO_d69d2e95_b22f_499a_a552_17fde0d778fc
<http://emmo.info/emmo/middle/materials#EMMO_d69d2e95_b22f_499a_a552_17fde0d778fc> rdf:type owl:Class ;
                                                                                   rdfs:subClassOf <http://emmo.info/emmo/middle/materials#EMMO_1f5e3e7e_72c9_40d4_91dd_ae432d7b7018> ,
                                                                                                   <http://emmo.info/emmo/middle/materials#EMMO_7509da43_56b1_4d7f_887a_65d1663df4ba> ;
                                                                                   <http://emmo.info/emmo/top/annotations#EMMO_967080e5_2f42_4eb2_a3a9_c58143e835f9> "A foam of trapped gas in a liquid."@en ;
                                                                                   <http://www.w3.org/2004/02/skos/core#prefLabel> "LiquidFoam"@en .


###  http://emmo.info/emmo/middle/materials#EMMO_db03061b_db31_4132_a47a_6a634846578b
<http://emmo.info/emmo/middle/materials#EMMO_db03061b_db31_4132_a47a_6a634846578b> rdf:type owl:Class ;
                                                                                   rdfs:subClassOf <http://emmo.info/emmo/middle/materials#EMMO_2fd3f574_5e93_47fe_afca_ed80b0a21ab4> ;
                                                                                   <http://emmo.info/emmo/top/annotations#EMMO_967080e5_2f42_4eb2_a3a9_c58143e835f9> "A standalone atom with an unbalanced number of electrons with respect to its atomic number."@en ;
                                                                                   rdfs:comment "The ion_atom is the basic part of a pure ionic bonded compound i.e. without eclectron sharing,"@en ;
                                                                                   <http://www.w3.org/2004/02/skos/core#prefLabel> "IonAtom"@en .


###  http://emmo.info/emmo/middle/materials#EMMO_df808271_df91_4f27_ba59_fa423c51896c
<http://emmo.info/emmo/middle/materials#EMMO_df808271_df91_4f27_ba59_fa423c51896c> rdf:type owl:Class ;
                                                                                   rdfs:subClassOf <http://emmo.info/emmo/middle/materials#EMMO_50781fd9_a9e4_46ad_b7be_4500371d188d> ;
                                                                                   <http://www.w3.org/2004/02/skos/core#prefLabel> "Neutron"@en .


###  http://emmo.info/emmo/middle/materials#EMMO_e0edfb9e_9a96_4fae_b942_831ffe27b84a
<http://emmo.info/emmo/middle/materials#EMMO_e0edfb9e_9a96_4fae_b942_831ffe27b84a> rdf:type owl:Class ;
                                                                                   rdfs:subClassOf <http://emmo.info/emmo/middle/materials#EMMO_04f2a2d5_e799_4692_a654_420e76f5acc1> ,
                                                                                                   <http://emmo.info/emmo/middle/materials#EMMO_4a464c8d_8895_44a8_a628_aed13509f1bd> ;
                                                                                   <http://emmo.info/emmo/top/annotations#EMMO_967080e5_2f42_4eb2_a3a9_c58143e835f9> "A coarse dispersion of liquid in a gas continuum phase."@en ;
                                                                                   <http://emmo.info/emmo/top/annotations#EMMO_b432d2d5_25f4_4165_99c5_5935a7763c1a> "Rain, spray."@en ;
                                                                                   <http://www.w3.org/2004/02/skos/core#prefLabel> "GasLiquidSuspension"@en .


###  http://emmo.info/emmo/middle/materials#EMMO_e4281979_2b07_4a43_a772_4903fb3696fe
<http://emmo.info/emmo/middle/materials#EMMO_e4281979_2b07_4a43_a772_4903fb3696fe> rdf:type owl:Class ;
                                                                                   rdfs:subClassOf <http://emmo.info/emmo/middle/materials#EMMO_d4f37e32_16ae_4cc6_b4cd_fd896b2449c4> ;
                                                                                   <http://emmo.info/emmo/top/annotations#EMMO_967080e5_2f42_4eb2_a3a9_c58143e835f9> "A suspension of fine particles in the atmosphere."@en ;
                                                                                   <http://www.w3.org/2004/02/skos/core#prefLabel> "Dust"@en .


###  http://emmo.info/emmo/middle/materials#EMMO_e9e02156_651f_41c8_9efb_d5da0d4ce5e2
<http://emmo.info/emmo/middle/materials#EMMO_e9e02156_651f_41c8_9efb_d5da0d4ce5e2> rdf:type owl:Class ;
                                                                                   rdfs:subClassOf <http://emmo.info/emmo/middle/materials#EMMO_4a464c8d_8895_44a8_a628_aed13509f1bd> ,
                                                                                                   <http://emmo.info/emmo/middle/materials#EMMO_7509da43_56b1_4d7f_887a_65d1663df4ba> ;
                                                                                   <http://emmo.info/emmo/top/annotations#EMMO_967080e5_2f42_4eb2_a3a9_c58143e835f9> "A coarse dispersion of solids in a liquid continuum phase."@en ;
                                                                                   <http://emmo.info/emmo/top/annotations#EMMO_b432d2d5_25f4_4165_99c5_5935a7763c1a> "Mud"@en ;
                                                                                   <http://www.w3.org/2004/02/skos/core#prefLabel> "LiquidSolidSuspension"@en .


###  http://emmo.info/emmo/middle/materials#EMMO_eb77076b_a104_42ac_a065_798b2d2809ad
<http://emmo.info/emmo/middle/materials#EMMO_eb77076b_a104_42ac_a065_798b2d2809ad> rdf:type owl:Class ;
                                                                                   rdfs:subClassOf <http://emmo.info/emmo/middle/physicalistic#EMMO_5b2222df_4da6_442f_8244_96e9e45887d1> ,
                                                                                                   <http://emmo.info/emmo/middle/reductionistic#EMMO_36c79456_e29c_400d_8bd3_0eedddb82652> ;
                                                                                   <http://emmo.info/emmo/top/annotations#EMMO_967080e5_2f42_4eb2_a3a9_c58143e835f9> """A standalone atom has direct part one 'nucleus' and one 'electron_cloud'. 

An O 'atom' within an O2 'molecule' is an 'e-bonded_atom'.

In this material branch, H atom is a particular case, with respect to higher atomic number atoms, since as soon as it shares its electron it has no nucleus entangled electron cloud.

We cannot say that H2 molecule has direct part two H atoms, but has direct part two H nucleus."""@en ;
                                                                                   rdfs:comment "An 'atom' is a 'nucleus' surrounded by an 'electron_cloud', i.e. a quantum system made of one or more bounded electrons."@en ;
                                                                                   <http://www.w3.org/2004/02/skos/core#altLabel> "ChemicalElement" ;
                                                                                   <http://www.w3.org/2004/02/skos/core#prefLabel> "Atom"@en .


###  http://emmo.info/emmo/middle/materials#EMMO_ec2c8ac8_98c5_4c74_b85b_ff8e8ca6655c
<http://emmo.info/emmo/middle/materials#EMMO_ec2c8ac8_98c5_4c74_b85b_ff8e8ca6655c> rdf:type owl:Class ;
                                                                                   rdfs:subClassOf <http://emmo.info/emmo/middle/materials#EMMO_8b0923ab_b500_477b_9ce9_8b3a3e4dc4f2> ;
                                                                                   <http://emmo.info/emmo/top/annotations#EMMO_967080e5_2f42_4eb2_a3a9_c58143e835f9> "A Miixture is a material made up of two or more different substances which are physically (not chemically) combined."@en ;
                                                                                   <http://www.w3.org/2004/02/skos/core#prefLabel> "Mixture"@en .


###  http://emmo.info/emmo/middle/materials#EMMO_f835f4d4_c665_403d_ab25_dca5cc74be52
<http://emmo.info/emmo/middle/materials#EMMO_f835f4d4_c665_403d_ab25_dca5cc74be52> rdf:type owl:Class ;
                                                                                   rdfs:subClassOf <http://emmo.info/emmo/middle/materials#EMMO_7d66bde4_b68d_41cc_b5fc_6fd98c5e2ff0> ,
                                                                                                   <http://emmo.info/emmo/middle/reductionistic#EMMO_36c79456_e29c_400d_8bd3_0eedddb82652> ;
                                                                                   <http://www.w3.org/2004/02/skos/core#prefLabel> "Nucleus"@en .


###  http://emmo.info/emmo/middle/math#EMMO_048a14e3_65fb_457d_8695_948965c89492
<http://emmo.info/emmo/middle/math#EMMO_048a14e3_65fb_457d_8695_948965c89492> rdf:type owl:Class ;
                                                                              rdfs:subClassOf <http://emmo.info/emmo/middle/math#EMMO_f8a2fe9f_458b_4771_9aba_a50e76afc52d> ;
                                                                              <http://www.w3.org/2004/02/skos/core#prefLabel> "Laplacian"@en .


###  http://emmo.info/emmo/middle/math#EMMO_06658d8d_dcde_4fc9_aae1_17f71c0bcdec
<http://emmo.info/emmo/middle/math#EMMO_06658d8d_dcde_4fc9_aae1_17f71c0bcdec> rdf:type owl:Class ;
                                                                              rdfs:subClassOf <http://emmo.info/emmo/middle/math#EMMO_28fbea28_2204_4613_87ff_6d877b855fcd> ;
                                                                              <http://www.w3.org/2004/02/skos/core#prefLabel> "Vector"@en .


###  http://emmo.info/emmo/middle/math#EMMO_0b6ebe5a_0026_4bef_a1c1_5be00df9f98e
<http://emmo.info/emmo/middle/math#EMMO_0b6ebe5a_0026_4bef_a1c1_5be00df9f98e> rdf:type owl:Class ;
                                                                              rdfs:subClassOf <http://emmo.info/emmo/middle/math#EMMO_88470739_03d3_4c47_a03e_b30a1288d50c> ;
                                                                              <http://emmo.info/emmo/top/annotations#EMMO_967080e5_2f42_4eb2_a3a9_c58143e835f9> "A relation which makes a non-equal comparison between two numbers or other mathematical expressions."@en ;
                                                                              <http://emmo.info/emmo/top/annotations#EMMO_b432d2d5_25f4_4165_99c5_5935a7763c1a> "f(x) > 0"@en ;
                                                                              <http://www.w3.org/2004/02/skos/core#prefLabel> "Inequality"@en .


###  http://emmo.info/emmo/middle/math#EMMO_18d180e4_5e3e_42f7_820c_e08951223486
<http://emmo.info/emmo/middle/math#EMMO_18d180e4_5e3e_42f7_820c_e08951223486> rdf:type owl:Class ;
                                                                              rdfs:subClassOf <http://emmo.info/emmo/middle/math#EMMO_21f56795_ee72_4858_b571_11cfaa59c1a8> ;
                                                                              <http://www.w3.org/2004/02/skos/core#prefLabel> "Real"@en .


###  http://emmo.info/emmo/middle/math#EMMO_1aed91a3_d00c_48af_8f43_a0c958b2512a
<http://emmo.info/emmo/middle/math#EMMO_1aed91a3_d00c_48af_8f43_a0c958b2512a> rdf:type owl:Class ;
                                                                              rdfs:subClassOf <http://emmo.info/emmo/middle/math#EMMO_f9bc8b52_85e9_4b53_b969_dd7724d5b8e4> ;
                                                                              <http://emmo.info/emmo/top/annotations#EMMO_b432d2d5_25f4_4165_99c5_5935a7763c1a> "2x+3"@en ;
                                                                              rdfs:comment "An expression that has parts only integer constants, variables, and the algebraic operations (addition, subtraction, multiplication, division and exponentiation by an exponent that is a rational number)"@en ;
                                                                              <http://www.w3.org/2004/02/skos/core#prefLabel> "AlgebricExpression"@en .


###  http://emmo.info/emmo/middle/math#EMMO_1cba0b27_15d0_4326_933f_379d0b3565b6
<http://emmo.info/emmo/middle/math#EMMO_1cba0b27_15d0_4326_933f_379d0b3565b6> rdf:type owl:Class ;
                                                                              rdfs:subClassOf <http://emmo.info/emmo/middle/math#EMMO_28fbea28_2204_4613_87ff_6d877b855fcd> ;
                                                                              <http://www.w3.org/2004/02/skos/core#prefLabel> "Matrix"@en .


###  http://emmo.info/emmo/middle/math#EMMO_1eed0732_e3f1_4b2c_a9c4_b4e75eeb5895
<http://emmo.info/emmo/middle/math#EMMO_1eed0732_e3f1_4b2c_a9c4_b4e75eeb5895> rdf:type owl:Class ;
                                                                              rdfs:subClassOf <http://emmo.info/emmo/middle/math#EMMO_54ee6b5e_5261_44a8_86eb_5717e7fdb9d0> ,
                                                                                              <http://emmo.info/emmo/middle/semiotics#EMMO_35d2e130_6e01_41ed_94f7_00b333d46cf9> ;
                                                                              <http://emmo.info/emmo/top/annotations#EMMO_967080e5_2f42_4eb2_a3a9_c58143e835f9> "A 'Variable' is a symbolic object that stands for a numerical defined 'Mathematical' object like e.g. a number, a vector, a matrix."@en ;
                                                                              <http://emmo.info/emmo/top/annotations#EMMO_b432d2d5_25f4_4165_99c5_5935a7763c1a> """x
k"""@en ;
                                                                              <http://www.w3.org/2004/02/skos/core#prefLabel> "Variable"@en .


###  http://emmo.info/emmo/middle/math#EMMO_21f56795_ee72_4858_b571_11cfaa59c1a8
<http://emmo.info/emmo/middle/math#EMMO_21f56795_ee72_4858_b571_11cfaa59c1a8> rdf:type owl:Class ;
                                                                              rdfs:subClassOf <http://emmo.info/emmo/middle/math#EMMO_4ce76d7f_03f8_45b6_9003_90052a79bfaa> ,
                                                                                              <http://emmo.info/emmo/middle/math#EMMO_5be83f9c_a4ba_4b9a_be1a_5bfc6e891231> ;
                                                                              <http://emmo.info/emmo/top/annotations#EMMO_967080e5_2f42_4eb2_a3a9_c58143e835f9> "A numerical data value."@en ;
                                                                              rdfs:comment """A number is actually a string (e.g. 1.4, 1e-8) of numerical digits and other symbols. However, in order not to increase complexity of the taxonomy and relations, here we take a number as an \"atomic\" object (i.e. we do not include digits in the EMMO as alphabet for numbers).

A 'Number' individual provide the link between the ontology and the actual data, through the data property hasNumericalValue."""@en ,
                                                                                           """In math usually number and numeral are distinct concepts, the numeral being the symbol or a composition of symbols (e.g. 3.14, 010010, three) and the number is the idea behind it.

More than one numeral stand for the same number.

In the EMMO abstract entities does not exists, and numbers are simply defined by other numerals, so that a number is the class of all the numerals that are equivalent (e.g. 3 and 0011 are numerals that stands for the same number).

Or alternatively, an integer numeral may also stands for a set of a specific cardinality (e.g. 3 stands for a set of three apples). Rational and real numbers are simply a syntactic arrangment of integers (digits, in decimal system).

The fact that you can't give a name to a number without using a numeral or, in case of positive integers, without referring to a real world objects set with specific cardinality, suggests that the abstract concept of number is not a concept that can be practically used.

For these reasons, the EMMO will consider numerals and numbers as the same concept."""@en ;
                                                                              <http://www.w3.org/2004/02/skos/core#prefLabel> "Number"@en .


###  http://emmo.info/emmo/middle/math#EMMO_223d9523_4169_4ecd_b8af_acad1215e1ff
<http://emmo.info/emmo/middle/math#EMMO_223d9523_4169_4ecd_b8af_acad1215e1ff> rdf:type owl:Class ;
                                                                              rdfs:subClassOf <http://emmo.info/emmo/middle/math#EMMO_3c424d37_cf62_41b1_ac9d_a316f8d113d6> ;
                                                                              <http://www.w3.org/2004/02/skos/core#prefLabel> "Exponent"@en .


###  http://emmo.info/emmo/middle/math#EMMO_29afdf54_90ae_4c98_8845_fa9ea3f143a8
<http://emmo.info/emmo/middle/math#EMMO_29afdf54_90ae_4c98_8845_fa9ea3f143a8> rdf:type owl:Class ;
                                                                              rdfs:subClassOf <http://emmo.info/emmo/middle/math#EMMO_e56ee3eb_7609_4ae1_8bed_51974f0960a6> ;
                                                                              <http://emmo.info/emmo/top/annotations#EMMO_967080e5_2f42_4eb2_a3a9_c58143e835f9> "An equation that define a new variable in terms of other mathematical entities."@en ;
                                                                              <http://emmo.info/emmo/top/annotations#EMMO_b432d2d5_25f4_4165_99c5_5935a7763c1a> """The definition of velocity as v = dx/dt.

The definition of density as mass/volume.

y = f(x)"""@en ;
                                                                              <http://www.w3.org/2004/02/skos/core#prefLabel> "DefiningEquation"@en .


###  http://emmo.info/emmo/middle/math#EMMO_2b1303e8_d4c3_453b_9918_76f1d009543f
<http://emmo.info/emmo/middle/math#EMMO_2b1303e8_d4c3_453b_9918_76f1d009543f> rdf:type owl:Class ;
                                                                              rdfs:subClassOf <http://emmo.info/emmo/middle/math#EMMO_707f0cd1_941c_4b57_9f20_d0ba30cd6ff3> ;
                                                                              <http://www.w3.org/2004/02/skos/core#prefLabel> "Multiplication"@en .


###  http://emmo.info/emmo/middle/math#EMMO_3c424d37_cf62_41b1_ac9d_a316f8d113d6
<http://emmo.info/emmo/middle/math#EMMO_3c424d37_cf62_41b1_ac9d_a316f8d113d6> rdf:type owl:Class ;
                                                                              rdfs:subClassOf <http://emmo.info/emmo/middle/math#EMMO_f6d0c26a_98b6_4cf8_8632_aa259131faaa> ;
                                                                              <http://www.w3.org/2004/02/skos/core#prefLabel> "AlgebricOperator"@en .


###  http://emmo.info/emmo/middle/math#EMMO_46d5643b_9706_4b67_8bea_ed77d6026539
<http://emmo.info/emmo/middle/math#EMMO_46d5643b_9706_4b67_8bea_ed77d6026539> rdf:type owl:Class ;
                                                                              rdfs:subClassOf <http://emmo.info/emmo/middle/math#EMMO_707f0cd1_941c_4b57_9f20_d0ba30cd6ff3> ;
                                                                              <http://www.w3.org/2004/02/skos/core#prefLabel> "Minus"@en .


###  http://emmo.info/emmo/middle/math#EMMO_4bc29b0f_8fcc_4026_a291_f9774a66d9b8
<http://emmo.info/emmo/middle/math#EMMO_4bc29b0f_8fcc_4026_a291_f9774a66d9b8> rdf:type owl:Class ;
                                                                              rdfs:subClassOf <http://emmo.info/emmo/middle/math#EMMO_29afdf54_90ae_4c98_8845_fa9ea3f143a8> ;
                                                                              <http://emmo.info/emmo/top/annotations#EMMO_967080e5_2f42_4eb2_a3a9_c58143e835f9> "A function defined using functional notation."@en ;
                                                                              <http://emmo.info/emmo/top/annotations#EMMO_b432d2d5_25f4_4165_99c5_5935a7763c1a> "y = f(x)"@en ;
                                                                              <http://www.w3.org/2004/02/skos/core#prefLabel> "FunctionDefinition"@en .


###  http://emmo.info/emmo/middle/math#EMMO_4ce76d7f_03f8_45b6_9003_90052a79bfaa
<http://emmo.info/emmo/middle/math#EMMO_4ce76d7f_03f8_45b6_9003_90052a79bfaa> rdf:type owl:Class ;
                                                                              rdfs:subClassOf <http://emmo.info/emmo/middle/math#EMMO_54ee6b5e_5261_44a8_86eb_5717e7fdb9d0> ;
                                                                              <http://emmo.info/emmo/top/annotations#EMMO_967080e5_2f42_4eb2_a3a9_c58143e835f9> "A 'Mathematical' that has no unknown value, i.e. all its 'Variable\"-s parts refers to a 'Number' (for scalars that have a built-in datatype) or to another 'Numerical' (for complex numerical data structures that should rely on external implementations)."@en ;
                                                                              <http://www.w3.org/2004/02/skos/core#prefLabel> "Numerical"@en .


###  http://emmo.info/emmo/middle/math#EMMO_535d75a4_1972_40bc_88c6_ca566386934f
<http://emmo.info/emmo/middle/math#EMMO_535d75a4_1972_40bc_88c6_ca566386934f> rdf:type owl:Class ;
                                                                              rdfs:subClassOf <http://emmo.info/emmo/middle/math#EMMO_5be83f9c_a4ba_4b9a_be1a_5bfc6e891231> ;
                                                                              <http://emmo.info/emmo/top/annotations#EMMO_967080e5_2f42_4eb2_a3a9_c58143e835f9> "The equals symbol."@en ;
                                                                              <http://www.w3.org/2004/02/skos/core#prefLabel> "Equals"@en .


###  http://emmo.info/emmo/middle/math#EMMO_54dc83cb_06e1_4739_9e45_bc09cead7f48
<http://emmo.info/emmo/middle/math#EMMO_54dc83cb_06e1_4739_9e45_bc09cead7f48> rdf:type owl:Class ;
                                                                              rdfs:subClassOf <http://emmo.info/emmo/middle/math#EMMO_21f56795_ee72_4858_b571_11cfaa59c1a8> ;
                                                                              <http://www.w3.org/2004/02/skos/core#prefLabel> "Boolean"@en .


###  http://emmo.info/emmo/middle/math#EMMO_54ee6b5e_5261_44a8_86eb_5717e7fdb9d0
<http://emmo.info/emmo/middle/math#EMMO_54ee6b5e_5261_44a8_86eb_5717e7fdb9d0> rdf:type owl:Class ;
                                                                              rdfs:subClassOf <http://emmo.info/emmo/middle/perceptual#EMMO_d8d2144e_5c8d_455d_a643_5caf4d8d9df8> ;
                                                                              <http://emmo.info/emmo/top/annotations#EMMO_967080e5_2f42_4eb2_a3a9_c58143e835f9> "The class of general mathematical symbolic objects respecting mathematical syntactic rules."@en ;
                                                                              <http://www.w3.org/2004/02/skos/core#prefLabel> "Mathematical"@en .


###  http://emmo.info/emmo/middle/math#EMMO_5be83f9c_a4ba_4b9a_be1a_5bfc6e891231
<http://emmo.info/emmo/middle/math#EMMO_5be83f9c_a4ba_4b9a_be1a_5bfc6e891231> rdf:type owl:Class ;
                                                                              rdfs:subClassOf <http://emmo.info/emmo/middle/math#EMMO_54ee6b5e_5261_44a8_86eb_5717e7fdb9d0> ,
                                                                                              <http://emmo.info/emmo/middle/perceptual#EMMO_a1083d0a_c1fb_471f_8e20_a98f881ad527> ;
                                                                              <http://www.w3.org/2004/02/skos/core#prefLabel> "MathematicalSymbol"@en .


###  http://emmo.info/emmo/middle/math#EMMO_707f0cd1_941c_4b57_9f20_d0ba30cd6ff3
<http://emmo.info/emmo/middle/math#EMMO_707f0cd1_941c_4b57_9f20_d0ba30cd6ff3> rdf:type owl:Class ;
                                                                              rdfs:subClassOf <http://emmo.info/emmo/middle/math#EMMO_3c424d37_cf62_41b1_ac9d_a316f8d113d6> ;
                                                                              <http://www.w3.org/2004/02/skos/core#prefLabel> "ArithmeticOperator"@en .


###  http://emmo.info/emmo/middle/math#EMMO_88470739_03d3_4c47_a03e_b30a1288d50c
<http://emmo.info/emmo/middle/math#EMMO_88470739_03d3_4c47_a03e_b30a1288d50c> rdf:type owl:Class ;
                                                                              rdfs:subClassOf <http://emmo.info/emmo/middle/math#EMMO_54ee6b5e_5261_44a8_86eb_5717e7fdb9d0> ,
                                                                                              <http://emmo.info/emmo/middle/perceptual#EMMO_89a0c87c_0804_4013_937a_6fe234d9499c> ;
                                                                              <http://emmo.info/emmo/top/annotations#EMMO_967080e5_2f42_4eb2_a3a9_c58143e835f9> "A mathematical string that can be evaluated as true or false."@en ;
                                                                              <http://www.w3.org/2004/02/skos/core#prefLabel> "MathematicalFormula"@en .


###  http://emmo.info/emmo/middle/math#EMMO_89083bab_f69c_4d06_bf6d_62973b56cdc7
<http://emmo.info/emmo/middle/math#EMMO_89083bab_f69c_4d06_bf6d_62973b56cdc7> rdf:type owl:Class ;
                                                                              rdfs:subClassOf <http://emmo.info/emmo/middle/math#EMMO_1aed91a3_d00c_48af_8f43_a0c958b2512a> ;
                                                                              <http://emmo.info/emmo/top/annotations#EMMO_b432d2d5_25f4_4165_99c5_5935a7763c1a> "2+2"@en ;
                                                                              <http://www.w3.org/2004/02/skos/core#prefLabel> "ArithmeticExpression"@en .


###  http://emmo.info/emmo/middle/math#EMMO_8de14a59_660b_454f_aff8_76a07ce185f4
<http://emmo.info/emmo/middle/math#EMMO_8de14a59_660b_454f_aff8_76a07ce185f4> rdf:type owl:Class ;
                                                                              rdfs:subClassOf <http://emmo.info/emmo/middle/math#EMMO_707f0cd1_941c_4b57_9f20_d0ba30cd6ff3> ;
                                                                              <http://www.w3.org/2004/02/skos/core#prefLabel> "Plus"@en .


###  http://emmo.info/emmo/middle/math#EMMO_91447ec0_fb55_49f2_85a5_3172dff6482c
<http://emmo.info/emmo/middle/math#EMMO_91447ec0_fb55_49f2_85a5_3172dff6482c> rdf:type owl:Class ;
                                                                              rdfs:subClassOf <http://emmo.info/emmo/middle/math#EMMO_1aed91a3_d00c_48af_8f43_a0c958b2512a> ;
                                                                              <http://emmo.info/emmo/top/annotations#EMMO_b432d2d5_25f4_4165_99c5_5935a7763c1a> "2 * x^2 + x + 3"@en ;
                                                                              <http://www.w3.org/2004/02/skos/core#prefLabel> "Polynomial"@en .


###  http://emmo.info/emmo/middle/math#EMMO_98d65021_4574_4890_b2fb_46430841077f
<http://emmo.info/emmo/middle/math#EMMO_98d65021_4574_4890_b2fb_46430841077f> rdf:type owl:Class ;
                                                                              rdfs:subClassOf <http://emmo.info/emmo/middle/math#EMMO_e56ee3eb_7609_4ae1_8bed_51974f0960a6> ;
                                                                              <http://emmo.info/emmo/top/annotations#EMMO_b432d2d5_25f4_4165_99c5_5935a7763c1a> "2 * a - b = c"@en ;
                                                                              rdfs:comment "An 'equation' that has parts two 'polynomial'-s"@en ;
                                                                              <http://www.w3.org/2004/02/skos/core#prefLabel> "AlgebricEquation"@en .


###  http://emmo.info/emmo/middle/math#EMMO_a365b3c1_7bde_41d7_a15b_2820762e85f4
<http://emmo.info/emmo/middle/math#EMMO_a365b3c1_7bde_41d7_a15b_2820762e85f4> rdf:type owl:Class ;
                                                                              rdfs:subClassOf <http://emmo.info/emmo/middle/math#EMMO_707f0cd1_941c_4b57_9f20_d0ba30cd6ff3> ;
                                                                              <http://www.w3.org/2004/02/skos/core#prefLabel> "Division"@en .


###  http://emmo.info/emmo/middle/math#EMMO_a6138ba7_e365_4f2d_b6b4_fe5a5918d403
<http://emmo.info/emmo/middle/math#EMMO_a6138ba7_e365_4f2d_b6b4_fe5a5918d403> rdf:type owl:Class ;
                                                                              rdfs:subClassOf <http://emmo.info/emmo/middle/math#EMMO_e56ee3eb_7609_4ae1_8bed_51974f0960a6> ;
                                                                              <http://emmo.info/emmo/top/annotations#EMMO_b432d2d5_25f4_4165_99c5_5935a7763c1a> "1 + 1 = 2"@en ;
                                                                              <http://www.w3.org/2004/02/skos/core#prefLabel> "ArithmeticEquation"@en .


###  http://emmo.info/emmo/middle/math#EMMO_ae15fb4f_8e4d_41de_a0f9_3997f89ba6a2
<http://emmo.info/emmo/middle/math#EMMO_ae15fb4f_8e4d_41de_a0f9_3997f89ba6a2> rdf:type owl:Class ;
                                                                              rdfs:subClassOf <http://emmo.info/emmo/middle/math#EMMO_1eed0732_e3f1_4b2c_a9c4_b4e75eeb5895> ;
                                                                              <http://emmo.info/emmo/top/annotations#EMMO_967080e5_2f42_4eb2_a3a9_c58143e835f9> "A 'varaible' that stand for a well known constant."@en ;
                                                                              <http://emmo.info/emmo/top/annotations#EMMO_b432d2d5_25f4_4165_99c5_5935a7763c1a> "p refers to the constant number ~3.14"@en ;
                                                                              <http://www.w3.org/2004/02/skos/core#prefLabel> "Constant"@en .


###  http://emmo.info/emmo/middle/math#EMMO_b5c58790_fb2d_42eb_b184_2a3f6ca60acb
<http://emmo.info/emmo/middle/math#EMMO_b5c58790_fb2d_42eb_b184_2a3f6ca60acb> rdf:type owl:Class ;
                                                                              rdfs:subClassOf <http://emmo.info/emmo/middle/math#EMMO_f8a2fe9f_458b_4771_9aba_a50e76afc52d> ;
                                                                              <http://www.w3.org/2004/02/skos/core#prefLabel> "Gradient"@en .


###  http://emmo.info/emmo/middle/math#EMMO_d1d436e7_72fc_49cd_863b_7bfb4ba5276a
<http://emmo.info/emmo/middle/math#EMMO_d1d436e7_72fc_49cd_863b_7bfb4ba5276a> rdf:type owl:Class ;
                                                                              rdfs:subClassOf <http://emmo.info/emmo/middle/math#EMMO_1eed0732_e3f1_4b2c_a9c4_b4e75eeb5895> ;
                                                                              <http://emmo.info/emmo/top/annotations#EMMO_b432d2d5_25f4_4165_99c5_5935a7763c1a> "viscosity in the Navier-Stokes equation"@en ;
                                                                              rdfs:comment "A 'variable' whose value is assumed to be known independently from the equation, but whose value is not explicitated in the equation."@en ;
                                                                              <http://www.w3.org/2004/02/skos/core#prefLabel> "Parameter"@en .


###  http://emmo.info/emmo/middle/math#EMMO_e56ee3eb_7609_4ae1_8bed_51974f0960a6
<http://emmo.info/emmo/middle/math#EMMO_e56ee3eb_7609_4ae1_8bed_51974f0960a6> rdf:type owl:Class ;
                                                                              rdfs:subClassOf <http://emmo.info/emmo/middle/math#EMMO_88470739_03d3_4c47_a03e_b30a1288d50c> ,
                                                                                              <http://emmo.info/emmo/middle/reductionistic#EMMO_36c79456_e29c_400d_8bd3_0eedddb82652> ;
                                                                              <http://emmo.info/emmo/top/annotations#EMMO_967080e5_2f42_4eb2_a3a9_c58143e835f9> "The class of 'mathematical'-s that stand for a statement of equality between two mathematical expressions."@en ;
                                                                              <http://emmo.info/emmo/top/annotations#EMMO_b432d2d5_25f4_4165_99c5_5935a7763c1a> """2+3 = 5
x^2 +3x  = 5x
dv/dt = a
sin(x) = y"""@en ;
                                                                              rdfs:comment """An equation with variables can always be represented as:

f(v0, v1, ..., vn) = g(v0, v1, ..., vn)

where f is the left hand and g the right hand  side expressions and v0, v1, ..., vn are the variables."""@en ;
                                                                              <http://www.w3.org/2004/02/skos/core#prefLabel> "Equation"@en .


###  http://emmo.info/emmo/middle/math#EMMO_f6d0c26a_98b6_4cf8_8632_aa259131faaa
<http://emmo.info/emmo/middle/math#EMMO_f6d0c26a_98b6_4cf8_8632_aa259131faaa> rdf:type owl:Class ;
                                                                              rdfs:subClassOf <http://emmo.info/emmo/middle/math#EMMO_5be83f9c_a4ba_4b9a_be1a_5bfc6e891231> ;
                                                                              <http://www.w3.org/2004/02/skos/core#prefLabel> "MathematicalOperator"@en .


###  http://emmo.info/emmo/middle/math#EMMO_f8a2fe9f_458b_4771_9aba_a50e76afc52d
<http://emmo.info/emmo/middle/math#EMMO_f8a2fe9f_458b_4771_9aba_a50e76afc52d> rdf:type owl:Class ;
                                                                              rdfs:subClassOf <http://emmo.info/emmo/middle/math#EMMO_f6d0c26a_98b6_4cf8_8632_aa259131faaa> ;
                                                                              <http://www.w3.org/2004/02/skos/core#prefLabel> "DifferentialOperator"@en .


###  http://emmo.info/emmo/middle/math#EMMO_f8bd64d5_5d3e_4ad4_a46e_c30714fecb7f
<http://emmo.info/emmo/middle/math#EMMO_f8bd64d5_5d3e_4ad4_a46e_c30714fecb7f> rdf:type owl:Class ;
                                                                              rdfs:subClassOf <http://emmo.info/emmo/middle/math#EMMO_21f56795_ee72_4858_b571_11cfaa59c1a8> ;
                                                                              <http://www.w3.org/2004/02/skos/core#prefLabel> "Integer"@en .


###  http://emmo.info/emmo/middle/math#EMMO_f9bc8b52_85e9_4b53_b969_dd7724d5b8e4
<http://emmo.info/emmo/middle/math#EMMO_f9bc8b52_85e9_4b53_b969_dd7724d5b8e4> rdf:type owl:Class ;
                                                                              rdfs:subClassOf <http://emmo.info/emmo/middle/math#EMMO_54ee6b5e_5261_44a8_86eb_5717e7fdb9d0> ,
                                                                                              <http://emmo.info/emmo/middle/perceptual#EMMO_89a0c87c_0804_4013_937a_6fe234d9499c> ;
                                                                              <http://emmo.info/emmo/top/annotations#EMMO_967080e5_2f42_4eb2_a3a9_c58143e835f9> "A well-formed finite combination of mathematical symbols according to some specific rules."@en ;
                                                                              <http://www.w3.org/2004/02/skos/core#prefLabel> "Expression"@en .


###  http://emmo.info/emmo/middle/math#EMMO_fe7e56ce_118b_4243_9aad_20eb9f4f31f6
<http://emmo.info/emmo/middle/math#EMMO_fe7e56ce_118b_4243_9aad_20eb9f4f31f6> rdf:type owl:Class ;
                                                                              rdfs:subClassOf <http://emmo.info/emmo/middle/math#EMMO_1eed0732_e3f1_4b2c_a9c4_b4e75eeb5895> ;
                                                                              <http://emmo.info/emmo/top/annotations#EMMO_967080e5_2f42_4eb2_a3a9_c58143e835f9> "The dependent variable for which an equation has been written."@en ;
                                                                              <http://emmo.info/emmo/top/annotations#EMMO_b432d2d5_25f4_4165_99c5_5935a7763c1a> "Velocity, for the Navier-Stokes equation."@en ;
                                                                              <http://www.w3.org/2004/02/skos/core#prefLabel> "Unknown"@en .


###  http://emmo.info/emmo/middle/math#EMMO_28fbea28_2204_4613_87ff_6d877b855fcd
<http://emmo.info/emmo/middle/math#EMMO_28fbea28_2204_4613_87ff_6d877b855fcd> rdf:type owl:Class ;
                                                                                 rdfs:subClassOf <http://emmo.info/emmo/middle/math#EMMO_54ee6b5e_5261_44a8_86eb_5717e7fdb9d0> ;
                                                                                 <http://www.w3.org/2004/02/skos/core#prefLabel> "Array"@en .


###  http://emmo.info/emmo/middle/metrology#EMMO_02c0621e_a527_4790_8a0f_2bb51973c819
<http://emmo.info/emmo/middle/metrology#EMMO_02c0621e_a527_4790_8a0f_2bb51973c819> rdf:type owl:Class ;
                                                                                   rdfs:subClassOf <http://emmo.info/emmo/middle/math#EMMO_54ee6b5e_5261_44a8_86eb_5717e7fdb9d0> ,
                                                                                                   <http://emmo.info/emmo/middle/metrology#EMMO_f658c301_ce93_46cf_9639_4eace2c5d1d5> ;
                                                                                   <http://emmo.info/emmo/top/annotations#EMMO_967080e5_2f42_4eb2_a3a9_c58143e835f9> "A 'Mathematical' entity that is made of a 'Numeral' and a 'MeasurementUnit' defined by a physical law, connected to a physical entity through a model perspective. Measurement is done according to the same model."@en ;
                                                                                   rdfs:comment """In the same system of quantities, dim ?B = ML-3 is the quantity dimension of mass concentration of component B, and ML-3 is also the quantity dimension of mass density, ?.
ISO 80000-1"""@en ,
                                                                                                """Measured or simulated 'physical propertiy'-s are always defined by a physical law, connected to a physical entity through a model perspective and measurement is done according to the same model.

Systems of units suggests that this is the correct approach, since except for the fundamental units (length, time, charge) every other unit is derived by mathematical relations between these fundamental units, implying a physical laws or definitions."""@en ,
                                                                                                """Measurement units of quantities of the same quantity dimension may be designated by the same name and symbol even when the quantities are not of the same kind. 

For example, joule per kelvin and J/K are respectively the name and symbol of both a measurement unit of heat capacity and a measurement unit of entropy, which are generally not considered to be quantities of the same kind. 

However, in some cases special measurement unit names are restricted to be used with quantities of specific kind only. 

For example, the measurement unit second to the power minus one (1/s) is called hertz (Hz) when used for frequencies and becquerel (Bq) when used for activities of radionuclides. 

As another example, the joule (J) is used as a unit of energy, but never as a unit of moment of force, i.e. the newton metre (N  m)."""@en ,
                                                                                                """ quantities of the same kind have the same quantity dimension,
 quantities of different quantity dimensions are always of different kinds, and
 quantities having the same quantity dimension are not necessarily of the same kind.
ISO 80000-1"""@en ;
                                                                                   <http://www.w3.org/2004/02/skos/core#prefLabel> "PhysicalQuantity"@en .


###  http://emmo.info/emmo/middle/metrology#EMMO_08b308d4_31cd_4779_a784_aa92fc730f39
<http://emmo.info/emmo/middle/metrology#EMMO_08b308d4_31cd_4779_a784_aa92fc730f39> rdf:type owl:Class ;
                                                                                   rdfs:subClassOf <http://emmo.info/emmo/middle/metrology#EMMO_868ae137_4d25_493e_b270_21ea3d94849e> ;
                                                                                   <http://emmo.info/emmo/top/annotations#EMMO_967080e5_2f42_4eb2_a3a9_c58143e835f9> "Derived units are defined as products of powers of the base units corresponding to the relations defining the derived quantities in terms of the base quantities."@en ;
                                                                                   <http://www.w3.org/2004/02/skos/core#prefLabel> "DerivedUnit"@en .


###  http://emmo.info/emmo/middle/metrology#EMMO_0a318776_b067_4de0_a2a6_cba2cf6333f8
<http://emmo.info/emmo/middle/metrology#EMMO_0a318776_b067_4de0_a2a6_cba2cf6333f8> rdf:type owl:Class ;
                                                                                   rdfs:subClassOf <http://emmo.info/emmo/middle/perceptual#EMMO_48716718_225f_4c88_89e2_d819d30c90a2> ,
                                                                                                   <http://emmo.info/emmo/middle/perceptual#EMMO_a1083d0a_c1fb_471f_8e20_a98f881ad527> ;
                                                                                   <http://www.w3.org/2004/02/skos/core#prefLabel> "IdiomaticSymbol"@en .


###  http://emmo.info/emmo/middle/metrology#EMMO_18ce5200_00f5_45bb_8c6f_6fb128cd41ae
<http://emmo.info/emmo/middle/metrology#EMMO_18ce5200_00f5_45bb_8c6f_6fb128cd41ae> rdf:type owl:Class ;
                                                                                   rdfs:subClassOf <http://emmo.info/emmo/middle/metrology#EMMO_985bec21_989f_4b9e_a4b3_735d88099c3c> ;
                                                                                   rdfs:comment """A reference can be a measurement unit, a measurement procedure, a reference material, or a combination of such.
International vocabulary of metrology (VIM)"""@en ,
                                                                                                """A symbolic is recognized as reference unit also if it is not part of a quatity (e.g. as in the sentence \"the Bq is the reference unit of Becquerel\").

For this reason we can't declare the axiom:
ReferenceUnit SubClassOf: inverse(hasReferenceUnit) some Quantity
because there exist reference units without being part of a quantity.

This is peculiar to EMMO, where quantities (symbolic) are distinct with properties (semiotics)."""@en ;
                                                                                   <http://www.w3.org/2004/02/skos/core#prefLabel> "ReferenceUnit"@en .


###  http://emmo.info/emmo/middle/metrology#EMMO_216f448e_cdbc_4aeb_a529_7a5fe7fc38bb
<http://emmo.info/emmo/middle/metrology#EMMO_216f448e_cdbc_4aeb_a529_7a5fe7fc38bb> rdf:type owl:Class ;
                                                                                   rdfs:subClassOf <http://emmo.info/emmo/middle/metrology#EMMO_50a3552e_859a_4ff7_946d_76d537cabce6> ,
                                                                                                   <http://emmo.info/emmo/middle/metrology#EMMO_868ae137_4d25_493e_b270_21ea3d94849e> ;
                                                                                   <http://emmo.info/emmo/top/annotations#EMMO_967080e5_2f42_4eb2_a3a9_c58143e835f9> "A symbol that stands for a single unit."@en ;
                                                                                   <http://emmo.info/emmo/top/annotations#EMMO_b432d2d5_25f4_4165_99c5_5935a7763c1a> "Some examples are \"Pa\", \"m\" and \"J\"."@en ;
                                                                                   <http://www.w3.org/2004/02/skos/core#prefLabel> "UnitSymbol"@en .


###  http://emmo.info/emmo/middle/metrology#EMMO_3227b821_26a5_4c7c_9c01_5c24483e0bd0
<http://emmo.info/emmo/middle/metrology#EMMO_3227b821_26a5_4c7c_9c01_5c24483e0bd0> rdf:type owl:Class ;
                                                                                   rdfs:subClassOf <http://emmo.info/emmo/middle/metrology#EMMO_9895a1b4_f0a5_4167_ac5e_97db40b8bfcc> ;
                                                                                   rdfs:comment """\"The unit one is the neutral element of any system of units  necessary and present automatically.\"
SI Brochure"""@en ;
                                                                                   <http://www.w3.org/2004/02/skos/core#prefLabel> "DimensionOne"@en .


###  http://emmo.info/emmo/middle/metrology#EMMO_3ee80521_3c23_4dd1_935d_9d522614a3e2
<http://emmo.info/emmo/middle/metrology#EMMO_3ee80521_3c23_4dd1_935d_9d522614a3e2> rdf:type owl:Class ;
                                                                                   rdfs:subClassOf <http://emmo.info/emmo/middle/metrology#EMMO_08b308d4_31cd_4779_a784_aa92fc730f39> ,
                                                                                                   <http://emmo.info/emmo/middle/metrology#EMMO_216f448e_cdbc_4aeb_a529_7a5fe7fc38bb> ,
                                                                                                   <http://emmo.info/emmo/middle/semiotics#EMMO_b21a56ed_f969_4612_a6ec_cb7766f7f31d> ;
                                                                                   <http://emmo.info/emmo/top/annotations#EMMO_967080e5_2f42_4eb2_a3a9_c58143e835f9> "A unit symbol that stands for a derived unit."@en ;
                                                                                   <http://emmo.info/emmo/top/annotations#EMMO_b432d2d5_25f4_4165_99c5_5935a7763c1a> """Pa stands for N/m2
J stands for N m"""@en ;
                                                                                   rdfs:comment "Special units are semiotic shortcuts to more complex composed symbolic objects."@en ;
                                                                                   <http://www.w3.org/2004/02/skos/core#prefLabel> "SpecialUnit"@en .


###  http://emmo.info/emmo/middle/metrology#EMMO_3f15d200_c97b_42c8_8ac0_d81d150361e2
<http://emmo.info/emmo/middle/metrology#EMMO_3f15d200_c97b_42c8_8ac0_d81d150361e2> rdf:type owl:Class ;
                                                                                   rdfs:subClassOf <http://emmo.info/emmo/middle/metrology#EMMO_b953f2b1_c8d1_4dd9_b630_d3ef6580c2bb> ;
                                                                                   <http://emmo.info/emmo/top/annotations#EMMO_967080e5_2f42_4eb2_a3a9_c58143e835f9> "For a given unit system, measured constants are physical constants that are not used to define the unit system. Hence, these constants have to be measured and will therefore be associated with an uncertainty."@en ;
                                                                                   <http://www.w3.org/2004/02/skos/core#prefLabel> "MeasuredConstant"@en .


###  http://emmo.info/emmo/middle/metrology#EMMO_50a3552e_859a_4ff7_946d_76d537cabce6
<http://emmo.info/emmo/middle/metrology#EMMO_50a3552e_859a_4ff7_946d_76d537cabce6> rdf:type owl:Class ;
                                                                                   rdfs:subClassOf <http://emmo.info/emmo/middle/metrology#EMMO_985bec21_989f_4b9e_a4b3_735d88099c3c> ,
                                                                                                   <http://emmo.info/emmo/middle/perceptual#EMMO_a1083d0a_c1fb_471f_8e20_a98f881ad527> ;
                                                                                   <http://emmo.info/emmo/top/annotations#EMMO_967080e5_2f42_4eb2_a3a9_c58143e835f9> "A symbol that stands for a concept in the language of the meterological domain of ISO 80000."@en ;
                                                                                   <http://www.w3.org/2004/02/skos/core#prefLabel> "MetrologicalSymbol"@en .


###  http://emmo.info/emmo/middle/metrology#EMMO_591e02fd_8d37_45a6_9d11_bb21cef391a0
<http://emmo.info/emmo/middle/metrology#EMMO_591e02fd_8d37_45a6_9d11_bb21cef391a0> rdf:type owl:Class ;
                                                                                   rdfs:subClassOf <http://emmo.info/emmo/middle/metrology#EMMO_b081b346_7279_46ef_9a3d_2c088fcd79f4> ;
                                                                                   <http://emmo.info/emmo/top/annotations#EMMO_967080e5_2f42_4eb2_a3a9_c58143e835f9> "A unit that does not belong to any system of units."@en ;
                                                                                   <http://emmo.info/emmo/top/annotations#EMMO_b432d2d5_25f4_4165_99c5_5935a7763c1a> """eV
barn"""@en ;
                                                                                   <http://www.w3.org/2004/02/skos/core#prefLabel> "OffSystemUnit"@en .


###  http://emmo.info/emmo/middle/metrology#EMMO_5ebd5e01_0ed3_49a2_a30d_cd05cbe72978
<http://emmo.info/emmo/middle/metrology#EMMO_5ebd5e01_0ed3_49a2_a30d_cd05cbe72978> rdf:type owl:Class ;
                                                                                   rdfs:subClassOf <http://emmo.info/emmo/middle/metrology#EMMO_08b308d4_31cd_4779_a784_aa92fc730f39> ;
                                                                                   <http://emmo.info/emmo/top/annotations#EMMO_1f1b164d_ec6a_4faa_8d5e_88bda62316cc> "http://qudt.org/vocab/unit/UNITLESS" ;
                                                                                   <http://emmo.info/emmo/top/annotations#EMMO_967080e5_2f42_4eb2_a3a9_c58143e835f9> "Represents the number 1, used as an explicit unit to say something has no units."@en ;
                                                                                   <http://emmo.info/emmo/top/annotations#EMMO_b432d2d5_25f4_4165_99c5_5935a7763c1a> "Refractive index or volume fraction."@en ,
                                                                                                                                                                     "Typically used for ratios of two units whos dimensions cancels out."@en ;
                                                                                   <http://www.w3.org/2004/02/skos/core#prefLabel> "UnitOne"@en .


###  http://emmo.info/emmo/middle/metrology#EMMO_62f0d847_3603_45b4_bfc4_dd4511355ff2
<http://emmo.info/emmo/middle/metrology#EMMO_62f0d847_3603_45b4_bfc4_dd4511355ff2> rdf:type owl:Class ;
                                                                                   rdfs:subClassOf <http://emmo.info/emmo/middle/metrology#EMMO_c6d4a5e0_7e95_44df_a6db_84ee0a8bbc8e> ;
                                                                                   <http://emmo.info/emmo/top/annotations#EMMO_967080e5_2f42_4eb2_a3a9_c58143e835f9> "Measurement unit obtained by multiplying a given measurement unit by an integer greater than one."@en ;
                                                                                   <http://www.w3.org/2004/02/skos/core#prefLabel> "MultipleUnit"@en .


###  http://emmo.info/emmo/middle/metrology#EMMO_71f6ab56_342c_484b_bbe0_de86b7367cb3
<http://emmo.info/emmo/middle/metrology#EMMO_71f6ab56_342c_484b_bbe0_de86b7367cb3> rdf:type owl:Class ;
                                                                                   rdfs:subClassOf <http://emmo.info/emmo/middle/metrology#EMMO_02c0621e_a527_4790_8a0f_2bb51973c819> ;
                                                                                   <http://emmo.info/emmo/top/annotations#EMMO_967080e5_2f42_4eb2_a3a9_c58143e835f9> "\"Quantity, in a system of quantities, defined in terms of the base quantities of that system\"."@en ;
                                                                                   <http://www.w3.org/2004/02/skos/core#prefLabel> "DerivedQuantity"@en .


###  http://emmo.info/emmo/middle/metrology#EMMO_79751276_b2d0_4e2f_bbd4_99d412f43d55
<http://emmo.info/emmo/middle/metrology#EMMO_79751276_b2d0_4e2f_bbd4_99d412f43d55> rdf:type owl:Class ;
                                                                                   rdfs:subClassOf <http://emmo.info/emmo/middle/metrology#EMMO_02c0621e_a527_4790_8a0f_2bb51973c819> ;
                                                                                   <http://www.w3.org/2004/02/skos/core#prefLabel> "CategorizedPhysicalQuantity"@en .


###  http://emmo.info/emmo/middle/metrology#EMMO_7d2afa66_ae9e_4095_a9bf_421d0be401b6
<http://emmo.info/emmo/middle/metrology#EMMO_7d2afa66_ae9e_4095_a9bf_421d0be401b6> rdf:type owl:Class ;
                                                                                   rdfs:subClassOf <http://emmo.info/emmo/middle/math#EMMO_5be83f9c_a4ba_4b9a_be1a_5bfc6e891231> ,
                                                                                                   <http://emmo.info/emmo/middle/math#EMMO_ae15fb4f_8e4d_41de_a0f9_3997f89ba6a2> ,
                                                                                                   <http://emmo.info/emmo/middle/metrology#EMMO_50a3552e_859a_4ff7_946d_76d537cabce6> ;
                                                                                   <http://emmo.info/emmo/top/annotations#EMMO_967080e5_2f42_4eb2_a3a9_c58143e835f9> "Dimensionless multiplicative unit prefix."@en ;
                                                                                   rdfs:seeAlso "https://en.wikipedia.org/wiki/Metric_prefix" ;
                                                                                   <http://www.w3.org/2004/02/skos/core#prefLabel> "MetricPrefix"@en .


###  http://emmo.info/emmo/middle/metrology#EMMO_868ae137_4d25_493e_b270_21ea3d94849e
<http://emmo.info/emmo/middle/metrology#EMMO_868ae137_4d25_493e_b270_21ea3d94849e> rdf:type owl:Class ;
                                                                                   rdfs:subClassOf <http://emmo.info/emmo/middle/metrology#EMMO_b081b346_7279_46ef_9a3d_2c088fcd79f4> ;
                                                                                   <http://emmo.info/emmo/top/annotations#EMMO_967080e5_2f42_4eb2_a3a9_c58143e835f9> "A measurement unit symbol that do not have a metric prefix as a direct spatial part."@en ;
                                                                                   <http://www.w3.org/2004/02/skos/core#prefLabel> "NonPrefixedUnit"@en .


###  http://emmo.info/emmo/middle/metrology#EMMO_89762966_8076_4f7c_b745_f718d653e8e2
<http://emmo.info/emmo/middle/metrology#EMMO_89762966_8076_4f7c_b745_f718d653e8e2> rdf:type owl:Class ;
                                                                                   rdfs:subClassOf <http://emmo.info/emmo/middle/metrology#EMMO_b953f2b1_c8d1_4dd9_b630_d3ef6580c2bb> ;
                                                                                   rdfs:comment "Physical constant used to define a unit system. Hence, when expressed in that unit system they have an exact value with no associated uncertainty."@en ;
                                                                                   <http://www.w3.org/2004/02/skos/core#prefLabel> "ExactConstant"@en .


###  http://emmo.info/emmo/middle/metrology#EMMO_985bec21_989f_4b9e_a4b3_735d88099c3c
<http://emmo.info/emmo/middle/metrology#EMMO_985bec21_989f_4b9e_a4b3_735d88099c3c> rdf:type owl:Class ;
                                                                                   rdfs:subClassOf <http://emmo.info/emmo/middle/perceptual#EMMO_d8d2144e_5c8d_455d_a643_5caf4d8d9df8> ;
                                                                                   <http://emmo.info/emmo/top/annotations#EMMO_967080e5_2f42_4eb2_a3a9_c58143e835f9> "A language object used in metrology."@en ;
                                                                                   rdfs:comment """Metrology includes all theoretical and practical aspects of measurement, whatever the measurement uncertainty and field of application.

-- International vocabulary of metrology (VIM)"""@en ,
                                                                                                "This language domain makes use of ISO 80000 concepts."@en ;
                                                                                   <http://www.w3.org/2004/02/skos/core#prefLabel> "Metrological"@en .


###  http://emmo.info/emmo/middle/metrology#EMMO_9895a1b4_f0a5_4167_ac5e_97db40b8bfcc
<http://emmo.info/emmo/middle/metrology#EMMO_9895a1b4_f0a5_4167_ac5e_97db40b8bfcc> rdf:type owl:Class ;
                                                                                   rdfs:subClassOf <http://emmo.info/emmo/middle/metrology#EMMO_50a3552e_859a_4ff7_946d_76d537cabce6> ;
                                                                                   <http://emmo.info/emmo/top/annotations#EMMO_967080e5_2f42_4eb2_a3a9_c58143e835f9> "A symbol that, following SI specifications, describe the physical dimensionality of a physical quantity and the exponents of the base units in a measurement unit."@en ;
                                                                                   rdfs:comment """All physical quantities, with the exception of counts, are derived quantities, which may be written in terms of base quantities according to the equations of physics. The dimensions of the derived quantities are written as products of powers of the dimensions of the base quantities using the equations that relate the derived quantities to the base quantities.
In general the dimension of any quantity Q is written in the form of a dimensional product,

dim Q = T^a L^ M^? I^d T^e N^? J^?

where the exponents a, , ?, d, e, ? and ?, which are generally small integers, which can be positive, negative, or zero, are called the dimensional exponents.
(SI brochure)"""@en ,
                                                                                                """The conventional symbolic representation of the dimension of a base quantity is a single upper case letter in roman (upright) type. The conventional symbolic representation of the dimension of a derived quantity is the product of powers of the dimensions of the base quantities according to the definition of the derived quantity. The dimension of a quantity Q is denoted by dim Q.
ISO 80000-1"""@en ,
                                                                                                """The expression used by the EMMO for physical dimensions is a metrological symbol (but a string at meta level, i.e. the ontologist level) like this:
 
Ta Lb Mc Id Te Nf Jg

where a, b, c, d, e, f and g are 0 or signed integers.

Regex for the physical dimension symbol for the EMMO is:
^T([+-][1-9]|0) L([+-][1-9]|0) M([+-][1-9]|0) I([+-][1-9]|0) T([+-][1-9]|0) N([+-][1-9]|0) J([+-][1-9]|0)$

Examples of correspondance between base units and physical dimensions are:
mol -> T0 L0 M0 I0 T0 N+1 J0
s -> T+1 L0 M0 I0 T0 N0 J0
A/m2 -> T0 L0 M-2 I+1 T0 N0 J0"""@en ;
                                                                                   <http://www.w3.org/2004/02/skos/core#prefLabel> "PhysicalDimension"@en .


###  http://emmo.info/emmo/middle/metrology#EMMO_a2f94f33_71fa_443c_a1fb_d1685fc537ec
<http://emmo.info/emmo/middle/metrology#EMMO_a2f94f33_71fa_443c_a1fb_d1685fc537ec> rdf:type owl:Class ;
                                                                                   rdfs:subClassOf <http://emmo.info/emmo/middle/metrology#EMMO_c6d4a5e0_7e95_44df_a6db_84ee0a8bbc8e> ;
                                                                                   <http://emmo.info/emmo/top/annotations#EMMO_967080e5_2f42_4eb2_a3a9_c58143e835f9> "Measurement unit obtained by dividing a given measurement unit by an integer greater than one."@en ;
                                                                                   <http://www.w3.org/2004/02/skos/core#prefLabel> "SubMultipleUnit"@en .


###  http://emmo.info/emmo/middle/metrology#EMMO_acaaa124_3dde_48b6_86e6_6ec6f364f408
<http://emmo.info/emmo/middle/metrology#EMMO_acaaa124_3dde_48b6_86e6_6ec6f364f408> rdf:type owl:Class ;
                                                                                   rdfs:subClassOf <http://emmo.info/emmo/middle/metrology#EMMO_02c0621e_a527_4790_8a0f_2bb51973c819> ;
                                                                                   <http://emmo.info/emmo/top/annotations#EMMO_967080e5_2f42_4eb2_a3a9_c58143e835f9> """\"Quantity in a conventionally chosen subset of a given system of quantities, where no quantity in the subset can be expressed in terms of the other quantities within that subset\"
ISO 80000-1"""@en ;
                                                                                   <http://www.w3.org/2004/02/skos/core#prefLabel> "BaseQuantity"@en .


###  http://emmo.info/emmo/middle/metrology#EMMO_acd1a504_ca32_4f30_86ad_0b62cea5bc02
<http://emmo.info/emmo/middle/metrology#EMMO_acd1a504_ca32_4f30_86ad_0b62cea5bc02> rdf:type owl:Class ;
                                                                                   rdfs:subClassOf <http://emmo.info/emmo/middle/metrology#EMMO_18ce5200_00f5_45bb_8c6f_6fb128cd41ae> ;
                                                                                   <http://emmo.info/emmo/top/annotations#EMMO_967080e5_2f42_4eb2_a3a9_c58143e835f9> """A reference unit provided by a reference material.
International vocabulary of metrology (VIM)"""@en ;
                                                                                   <http://emmo.info/emmo/top/annotations#EMMO_b432d2d5_25f4_4165_99c5_5935a7763c1a> "Arbitrary amount-of-substance concentration of lutropin in a given sample of plasma (WHO international standard 80/552): 5.0 International Unit/l"@en ;
                                                                                   <http://www.w3.org/2004/02/skos/core#prefLabel> "StandardUnit"@en .


###  http://emmo.info/emmo/middle/metrology#EMMO_b081b346_7279_46ef_9a3d_2c088fcd79f4
<http://emmo.info/emmo/middle/metrology#EMMO_b081b346_7279_46ef_9a3d_2c088fcd79f4> rdf:type owl:Class ;
                                                                                   rdfs:subClassOf <http://emmo.info/emmo/middle/metrology#EMMO_18ce5200_00f5_45bb_8c6f_6fb128cd41ae> ,
                                                                                                   <http://emmo.info/emmo/middle/semiotics#EMMO_6f5af708_f825_4feb_a0d1_a8d813d3022b> ;
                                                                                   <http://emmo.info/emmo/top/annotations#EMMO_967080e5_2f42_4eb2_a3a9_c58143e835f9> """A 'Quantity' that stands for the standard reference magnitude of a specific class of measurement processes, defined and adopted by convention or by law.

The numerical quantity value of the 'MeasurementUnit' is conventionally 1 and does not appear.

Quantitative measurement results are expressed as a multiple of the 'MeasurementUnit'."""@en ;
                                                                                   rdfs:comment """\"Real scalar quantity, defined and adopted by convention, with which any other quantity of the same kind can be compared to express the ratio of the second quantity to the first one as a number\"
ISO 80000-1"""@en ,
                                                                                                """\"Unit symbols are mathematical entities and not abbreviations.\"

\"Symbols for units are treated as mathematical entities. In expressing the value of a quantity as the product of a numerical value and a unit, both the numerical value and the unit may be treated by the ordinary rules of algebra.\"

https://www.bipm.org/utils/common/pdf/si-brochure/SI-Brochure-9-EN.pdf"""@en ,
                                                                                                """While the SI brochure treats 'MeasurementUnit' as a 'PhysicalQuantity', in the EMMO this is not possible since the latter always has two direct parts, a 'Numerical' and a 'MeasurementUnit', while the former a single 'Symbol'.

SI distinguishes between a quantity (an abstract concept) and the quantity value (a number and a reference). The EMMO, following strict nominalism, considers a SI quantity as a SI quantity value, collapsing the two concepts into one: the 'Quantity'.

So, for the EMMO the symbol \"kg\" is not a physical quantity but a 'MeasurementUnit', while the string \"1 kg\" is 'Physical Quantity'."""@en ;
                                                                                   <http://www.w3.org/2004/02/skos/core#prefLabel> "MeasurementUnit"@en .


###  http://emmo.info/emmo/middle/metrology#EMMO_b953f2b1_c8d1_4dd9_b630_d3ef6580c2bb
<http://emmo.info/emmo/middle/metrology#EMMO_b953f2b1_c8d1_4dd9_b630_d3ef6580c2bb> rdf:type owl:Class ;
                                                                                   rdfs:subClassOf <http://emmo.info/emmo/middle/metrology#EMMO_02c0621e_a527_4790_8a0f_2bb51973c819> ;
                                                                                   <http://emmo.info/emmo/top/annotations#EMMO_c84c6752_6d64_48cc_9500_e54a3c34898d> "https://en.wikipedia.org/wiki/List_of_physical_constants" ;
                                                                                   rdfs:comment """Physical constants are categorised into \"exact\" and measured constants. 

With \"exact\" constants, we refer to physical constants that have an exact numerical value after the revision of the SI system that was enforsed May 2019."""@en ;
                                                                                   <http://www.w3.org/2004/02/skos/core#prefLabel> "PhysicalConstant"@en .


###  http://emmo.info/emmo/middle/metrology#EMMO_c46f091c_0420_4c1a_af30_0a2c8ebcf7d7
<http://emmo.info/emmo/middle/metrology#EMMO_c46f091c_0420_4c1a_af30_0a2c8ebcf7d7> rdf:type owl:Class ;
                                                                                   rdfs:subClassOf <http://emmo.info/emmo/middle/metrology#EMMO_f658c301_ce93_46cf_9639_4eace2c5d1d5> ;
                                                                                   <http://emmo.info/emmo/top/annotations#EMMO_967080e5_2f42_4eb2_a3a9_c58143e835f9> """\"Quantity, defined by a conventional measurement procedure, for which a total ordering relation can be established, according to magnitude, with other quantities of the same kind, but for which no algebraic operations among those quantities exist\"
International vocabulary of metrology (VIM)"""@en ;
                                                                                   <http://emmo.info/emmo/top/annotations#EMMO_b432d2d5_25f4_4165_99c5_5935a7763c1a> """Hardness
Resilience"""@en ;
                                                                                   rdfs:comment """\"Ordinal quantities, such as Rockwell C hardness, are usually not considered to be part of a system of quantities because they are related to other quantities through empirical relations only.\"
International vocabulary of metrology (VIM)"""@en ;
                                                                                   <http://www.w3.org/2004/02/skos/core#prefLabel> "OrdinalQuantity"@en .


###  http://emmo.info/emmo/middle/metrology#EMMO_c6d4a5e0_7e95_44df_a6db_84ee0a8bbc8e
<http://emmo.info/emmo/middle/metrology#EMMO_c6d4a5e0_7e95_44df_a6db_84ee0a8bbc8e> rdf:type owl:Class ;
                                                                                   rdfs:subClassOf <http://emmo.info/emmo/middle/metrology#EMMO_b081b346_7279_46ef_9a3d_2c088fcd79f4> ,
                                                                                                   <http://emmo.info/emmo/middle/reductionistic#EMMO_36c79456_e29c_400d_8bd3_0eedddb82652> ;
                                                                                   <http://emmo.info/emmo/top/annotations#EMMO_967080e5_2f42_4eb2_a3a9_c58143e835f9> "A measurement unit that is made of a metric prefix and a unit symbol."@en ;
                                                                                   <http://www.w3.org/2004/02/skos/core#prefLabel> "PrefixedUnit"@en .


###  http://emmo.info/emmo/middle/metrology#EMMO_c9c8f824_9127_4f93_bc21_69fe78a7f6f2
<http://emmo.info/emmo/middle/metrology#EMMO_c9c8f824_9127_4f93_bc21_69fe78a7f6f2> rdf:type owl:Class ;
                                                                                   rdfs:subClassOf <http://emmo.info/emmo/middle/metrology#EMMO_18ce5200_00f5_45bb_8c6f_6fb128cd41ae> ;
                                                                                   <http://emmo.info/emmo/top/annotations#EMMO_967080e5_2f42_4eb2_a3a9_c58143e835f9> "A reference unit provided by a measurement procedure."@en ;
                                                                                   <http://emmo.info/emmo/top/annotations#EMMO_b432d2d5_25f4_4165_99c5_5935a7763c1a> "Rockwell C hardness of a given sample (150 kg load): 43.5HRC(150 kg)"@en ;
                                                                                   <http://www.w3.org/2004/02/skos/core#prefLabel> "ProcedureUnit"@en .


###  http://emmo.info/emmo/middle/metrology#EMMO_daf05011_df3f_44a0_bb31_f8d565d7a854
<http://emmo.info/emmo/middle/metrology#EMMO_daf05011_df3f_44a0_bb31_f8d565d7a854> rdf:type owl:Class ;
                                                                                   rdfs:subClassOf <http://emmo.info/emmo/middle/metrology#EMMO_79751276_b2d0_4e2f_bbd4_99d412f43d55> ;
                                                                                   <http://www.w3.org/2004/02/skos/core#prefLabel> "PhysicoChemical"@en .


###  http://emmo.info/emmo/middle/metrology#EMMO_db716151_6b73_45ff_910c_d182fdcbb4f5
<http://emmo.info/emmo/middle/metrology#EMMO_db716151_6b73_45ff_910c_d182fdcbb4f5> rdf:type owl:Class ;
                                                                                   rdfs:subClassOf <http://emmo.info/emmo/middle/metrology#EMMO_216f448e_cdbc_4aeb_a529_7a5fe7fc38bb> ;
                                                                                   <http://emmo.info/emmo/top/annotations#EMMO_967080e5_2f42_4eb2_a3a9_c58143e835f9> "A set of units that correspond to the base quantities in a system of units."@en ;
                                                                                   <http://www.w3.org/2004/02/skos/core#prefLabel> "BaseUnit"@en .


###  http://emmo.info/emmo/middle/metrology#EMMO_dd4a7f3e_ef56_466c_ac1a_d2716b5f87ec
<http://emmo.info/emmo/middle/metrology#EMMO_dd4a7f3e_ef56_466c_ac1a_d2716b5f87ec> rdf:type owl:Class ;
                                                                                   rdfs:subClassOf <http://emmo.info/emmo/middle/metrology#EMMO_f658c301_ce93_46cf_9639_4eace2c5d1d5> ,
                                                                                                   <http://emmo.info/emmo/middle/properties#EMMO_2a888cdf_ec4a_4ec5_af1c_0343372fc978> ;
                                                                                   <http://emmo.info/emmo/top/annotations#EMMO_70fe84ff_99b6_4206_a9fc_9a8931836d84> """\"A property of a phenomenon, body, or substance, where the property has a magnitude that can be expressed by means of a number and a reference\"
ISO 80000-1

\"A reference can be a measurement unit, a measurement procedure, a reference material, or a combination of such.\"
International vocabulary of metrology (VIM)"""@en ;
                                                                                   <http://emmo.info/emmo/top/annotations#EMMO_967080e5_2f42_4eb2_a3a9_c58143e835f9> "A 'Quantity' that can be quantified with respect to a standardized reference physical instance (e.g. the prototype meter bar, the kg prototype) or method (e.g. resilience) through a measurement process."@en ;
                                                                                   rdfs:comment """A quantitative property is always expresssed as a quantity (i.e. a number and a reference unit). For the EMMO, a nominalistic ontology, there is no property as abstract object.

A property is a sign that stands for an object according to a specific code shared by some observers.

For quantititative properties, one possible code that is shared between the scientific community (the observers) is the SI system of units."""@en ,
                                                                                                "Subclasses of 'QuantitativeProperty' classify objects according to the type semiosis that is used to connect the property to the object (e.g. by measurement, by convention, by modelling)."@en ;
                                                                                   <http://www.w3.org/2004/02/skos/core#prefLabel> "QuantitativeProperty"@en .


###  http://emmo.info/emmo/middle/metrology#EMMO_f658c301_ce93_46cf_9639_4eace2c5d1d5
<http://emmo.info/emmo/middle/metrology#EMMO_f658c301_ce93_46cf_9639_4eace2c5d1d5> rdf:type owl:Class ;
                                                                                   rdfs:subClassOf <http://emmo.info/emmo/middle/metrology#EMMO_985bec21_989f_4b9e_a4b3_735d88099c3c> ,
                                                                                                   <http://emmo.info/emmo/middle/reductionistic#EMMO_36c79456_e29c_400d_8bd3_0eedddb82652> ;
                                                                                   <http://emmo.info/emmo/top/annotations#EMMO_967080e5_2f42_4eb2_a3a9_c58143e835f9> "A symbolic that has parts a reference unit and a numerical object separated by a space expressing the value of a quantitative property (expressed as the product of the numerical and the unit)."@en ;
                                                                                   <http://emmo.info/emmo/top/annotations#EMMO_b432d2d5_25f4_4165_99c5_5935a7763c1a> """6.8 m
0.9 km
8 K
6 MeV
43.5 HRC(150 kg)"""@en ;
                                                                                   rdfs:comment """A quantity is not necessarily a property, since it is possible to write \"10 kg\", without assigning this quantity to a specific object.

However, a quantitative property is always a quantity."""@en ,
                                                                                                "Referred as Quantity Value in International vocabulary of metrology (VIM)"@en ,
                                                                                                """SI distinguishes between a quantity (an abstract concept) and the quantity value (a number and a reference). 

The EMMO, following strict nominalism, denies the existence of abstract objects and then collapses the two concepts of SI quantity and SI quantity value into a single one: the 'Quantity'.

So, for the EMMO the symbol \"kg\" is not a physical quantity but simply a 'Symbolic' object categorized as a 'MeasurementUnit'.

While the string \"1 kg\" is a 'Physical Quantity'."""@en ;
                                                                                   <http://www.w3.org/2004/02/skos/core#prefLabel> "Quantity"@en .


###  http://emmo.info/emmo/middle/models#EMMO_22522299_4091_4d1f_82a2_3890492df6db
<http://emmo.info/emmo/middle/models#EMMO_22522299_4091_4d1f_82a2_3890492df6db> rdf:type owl:Class ;
                                                                                rdfs:subClassOf <http://emmo.info/emmo/middle/properties#EMMO_10a5fd39_06aa_4648_9e70_f962a9cb2069> ;
                                                                                <http://emmo.info/emmo/top/annotations#EMMO_967080e5_2f42_4eb2_a3a9_c58143e835f9> "An experiment is a process that is intended to replicate a physical phenomenon in a controlled environment."@en ;
                                                                                <http://www.w3.org/2004/02/skos/core#prefLabel> "Experiment"@en .


###  http://emmo.info/emmo/middle/models#EMMO_27c5d8c6_8af7_4d63_beb1_ec37cd8b3fa3
<http://emmo.info/emmo/middle/models#EMMO_27c5d8c6_8af7_4d63_beb1_ec37cd8b3fa3> rdf:type owl:Class ;
                                                                                rdfs:subClassOf <http://emmo.info/emmo/middle/math#EMMO_e56ee3eb_7609_4ae1_8bed_51974f0960a6> ,
                                                                                                <http://emmo.info/emmo/middle/models#EMMO_f7ed665b_c2e1_42bc_889b_6b42ed3a36f0> ;
                                                                                <http://emmo.info/emmo/top/annotations#EMMO_967080e5_2f42_4eb2_a3a9_c58143e835f9> "An 'equation' that stands for a 'physical_law' by mathematically defining the relations between physics_quantities."@en ;
                                                                                <http://emmo.info/emmo/top/annotations#EMMO_b432d2d5_25f4_4165_99c5_5935a7763c1a> """The Newton's equation of motion.

The Schrdinger equation.

The Navier-Stokes equation."""@en ;
                                                                                <http://www.w3.org/2004/02/skos/core#prefLabel> "PhysicsEquation"@en .


###  http://emmo.info/emmo/middle/models#EMMO_314d0bd5_67ed_437e_a609_36d46147cea7
<http://emmo.info/emmo/middle/models#EMMO_314d0bd5_67ed_437e_a609_36d46147cea7> rdf:type owl:Class ;
                                                                                rdfs:subClassOf <http://emmo.info/emmo/middle/holistic#EMMO_43e9a05d_98af_41b4_92f6_00f79a09bfce> ;
                                                                                <http://emmo.info/emmo/top/annotations#EMMO_967080e5_2f42_4eb2_a3a9_c58143e835f9> "A 'process' that is recognized by physical sciences and is catogrized accordingly."@en ;
                                                                                rdfs:comment "While every 'process' in the EMMO involves physical objects, this class is devoted to represent real world objects that express a phenomenon relevant for the ontologist."@en ;
                                                                                <http://www.w3.org/2004/02/skos/core#prefLabel> "PhysicalPhenomenon"@en .


###  http://emmo.info/emmo/middle/models#EMMO_4456a5d2_16a6_4ee1_9a8e_5c75956b28ea
<http://emmo.info/emmo/middle/models#EMMO_4456a5d2_16a6_4ee1_9a8e_5c75956b28ea> rdf:type owl:Class ;
                                                                                rdfs:subClassOf <http://emmo.info/emmo/middle/models#EMMO_b29fd350_39aa_4af7_9459_3faa0544cba6> ;
                                                                                <http://emmo.info/emmo/top/annotations#EMMO_967080e5_2f42_4eb2_a3a9_c58143e835f9> "A physics-based model based on a physics equation describing the behaviour of continuum volume."@en ;
                                                                                <http://www.w3.org/2004/02/skos/core#prefLabel> "ContinuumModel"@en .


###  http://emmo.info/emmo/middle/models#EMMO_53935db0_af45_4426_b9e9_244a0d77db00
<http://emmo.info/emmo/middle/models#EMMO_53935db0_af45_4426_b9e9_244a0d77db00> rdf:type owl:Class ;
                                                                                rdfs:subClassOf <http://emmo.info/emmo/middle/models#EMMO_b29fd350_39aa_4af7_9459_3faa0544cba6> ;
                                                                                <http://emmo.info/emmo/top/annotations#EMMO_967080e5_2f42_4eb2_a3a9_c58143e835f9> "A physics-based model based on a physics equation describing the behaviour of mesoscopic entities, i.e. a set of bounded atoms like a molecule, bead or nanoparticle."@en ;
                                                                                <http://www.w3.org/2004/02/skos/core#prefLabel> "MesoscopicModel"@en .


###  http://emmo.info/emmo/middle/models#EMMO_6c739b1a_a774_4416_bb31_1961486fa9ed
<http://emmo.info/emmo/middle/models#EMMO_6c739b1a_a774_4416_bb31_1961486fa9ed> rdf:type owl:Class ;
                                                                                rdfs:subClassOf <http://emmo.info/emmo/middle/properties#EMMO_10a5fd39_06aa_4648_9e70_f962a9cb2069> ;
                                                                                <http://emmo.info/emmo/top/annotations#EMMO_967080e5_2f42_4eb2_a3a9_c58143e835f9> "The 'semiosis' process of interpreting a 'physical' and provide a complec sign, 'theory' that stands for it and explain it to another interpreter."@en ;
                                                                                <http://www.w3.org/2004/02/skos/core#prefLabel> "Theorization"@en .


###  http://emmo.info/emmo/middle/models#EMMO_6eca09be_17e9_445e_abc9_000aa61b7a11
<http://emmo.info/emmo/middle/models#EMMO_6eca09be_17e9_445e_abc9_000aa61b7a11> rdf:type owl:Class ;
                                                                                rdfs:subClassOf <http://emmo.info/emmo/middle/models#EMMO_b29fd350_39aa_4af7_9459_3faa0544cba6> ;
                                                                                <http://emmo.info/emmo/top/annotations#EMMO_967080e5_2f42_4eb2_a3a9_c58143e835f9> "A physics-based model based on a physics equation describing the behaviour of electrons."@en ;
                                                                                <http://emmo.info/emmo/top/annotations#EMMO_b432d2d5_25f4_4165_99c5_5935a7763c1a> """Density functional theory.
Hartree-Fock."""@en ;
                                                                                <http://www.w3.org/2004/02/skos/core#prefLabel> "ElectronicModel"@en .


###  http://emmo.info/emmo/middle/models#EMMO_84cadc45_6758_46f2_ba2a_5ead65c70213
<http://emmo.info/emmo/middle/models#EMMO_84cadc45_6758_46f2_ba2a_5ead65c70213> rdf:type owl:Class ;
                                                                                rdfs:subClassOf <http://emmo.info/emmo/middle/models#EMMO_b29fd350_39aa_4af7_9459_3faa0544cba6> ;
                                                                                <http://emmo.info/emmo/top/annotations#EMMO_967080e5_2f42_4eb2_a3a9_c58143e835f9> "A physics-based model based on a physics equation describing the behaviour of atoms."@en ;
                                                                                <http://www.w3.org/2004/02/skos/core#prefLabel> "AtomisticModel"@en .


###  http://emmo.info/emmo/middle/models#EMMO_8d2d9374_ef3a_47e6_8595_6bc208e07519
<http://emmo.info/emmo/middle/models#EMMO_8d2d9374_ef3a_47e6_8595_6bc208e07519> rdf:type owl:Class ;
                                                                                rdfs:subClassOf <http://emmo.info/emmo/middle/semiotics#EMMO_35d2e130_6e01_41ed_94f7_00b333d46cf9> ;
                                                                                <http://emmo.info/emmo/top/annotations#EMMO_967080e5_2f42_4eb2_a3a9_c58143e835f9> "A 'conventional' that stand for a 'physical'."@en ;
                                                                                rdfs:comment """The 'theory' is e.g. a proposition, a book or a paper whose sub-symbols suggest in the mind of the interpreter an interpretant structure that can represent a 'physical'.

It is not an 'icon' (like a math equation), because it has no common resemblance or logical structure with the 'physical'.

In Peirce semiotics: legisign-symbol-argument"""@en ;
                                                                                <http://www.w3.org/2004/02/skos/core#prefLabel> "Theory"@en .


###  http://emmo.info/emmo/middle/models#EMMO_939483b1_0148_43d1_8b35_851d2cd5d939
<http://emmo.info/emmo/middle/models#EMMO_939483b1_0148_43d1_8b35_851d2cd5d939> rdf:type owl:Class ;
                                                                                rdfs:subClassOf <http://emmo.info/emmo/middle/semiotics#EMMO_d7788d1a_020d_4c78_85a1_13563fcec168> ;
                                                                                <http://emmo.info/emmo/top/annotations#EMMO_967080e5_2f42_4eb2_a3a9_c58143e835f9> """A 'sign' that not only stands for a 'physical' or a 'process', but it is also a simplified representation, aimed to assist calculations for its description or for predictions of its behaviour.

A 'model' represents a 'physical' or a 'process' by direct similitude (e.g. small scale replica) or by capturing in a logical framework the relations between its properties (e.g. mathematical model)."""@en ;
                                                                                rdfs:comment "A 'model' prediction is always a prediction of the properties of an entity, since an entity is known by an interpreter only through perception."@en ;
                                                                                <http://www.w3.org/2004/02/skos/core#prefLabel> "Model"@en .


###  http://emmo.info/emmo/middle/models#EMMO_9c32fd69_f480_4130_83b3_fb25d9face14
<http://emmo.info/emmo/middle/models#EMMO_9c32fd69_f480_4130_83b3_fb25d9face14> rdf:type owl:Class ;
                                                                                rdfs:subClassOf <http://emmo.info/emmo/middle/models#EMMO_db9a009e_f097_43f5_9520_6cbc07e7610b> ;
                                                                                <http://www.w3.org/2004/02/skos/core#prefLabel> "PhysicalLaw"@en .


###  http://emmo.info/emmo/middle/models#EMMO_a4b14b83_9392_4a5f_a2e8_b2b58793f59b
<http://emmo.info/emmo/middle/models#EMMO_a4b14b83_9392_4a5f_a2e8_b2b58793f59b> rdf:type owl:Class ;
                                                                                rdfs:subClassOf <http://emmo.info/emmo/middle/models#EMMO_f7ed665b_c2e1_42bc_889b_6b42ed3a36f0> ;
                                                                                <http://emmo.info/emmo/top/annotations#EMMO_967080e5_2f42_4eb2_a3a9_c58143e835f9> "A computational model that uses existing data to create new insight into the behaviour of a system."@en ;
                                                                                <http://www.w3.org/2004/02/skos/core#prefLabel> "DataBasedModel"@en .


###  http://emmo.info/emmo/middle/models#EMMO_b29fd350_39aa_4af7_9459_3faa0544cba6
<http://emmo.info/emmo/middle/models#EMMO_b29fd350_39aa_4af7_9459_3faa0544cba6> rdf:type owl:Class ;
                                                                                rdfs:subClassOf <http://emmo.info/emmo/middle/models#EMMO_f7ed665b_c2e1_42bc_889b_6b42ed3a36f0> ;
                                                                                <http://emmo.info/emmo/top/annotations#EMMO_967080e5_2f42_4eb2_a3a9_c58143e835f9> "A solvable set of one Physics Equation and one or more Materials Relations."@en ;
                                                                                <http://www.w3.org/2004/02/skos/core#prefLabel> "PhysicsBasedModel"@en .


###  http://emmo.info/emmo/middle/models#EMMO_db9a009e_f097_43f5_9520_6cbc07e7610b
<http://emmo.info/emmo/middle/models#EMMO_db9a009e_f097_43f5_9520_6cbc07e7610b> rdf:type owl:Class ;
                                                                                rdfs:subClassOf <http://emmo.info/emmo/middle/models#EMMO_8d2d9374_ef3a_47e6_8595_6bc208e07519> ;
                                                                                <http://www.w3.org/2004/02/skos/core#prefLabel> "NaturalLaw"@en .


###  http://emmo.info/emmo/middle/models#EMMO_e5438930_04e7_4d42_ade5_3700d4a52ab7
<http://emmo.info/emmo/middle/models#EMMO_e5438930_04e7_4d42_ade5_3700d4a52ab7> rdf:type owl:Class ;
                                                                                rdfs:subClassOf <http://emmo.info/emmo/middle/math#EMMO_e56ee3eb_7609_4ae1_8bed_51974f0960a6> ;
                                                                                <http://emmo.info/emmo/top/annotations#EMMO_967080e5_2f42_4eb2_a3a9_c58143e835f9> "An 'equation' that stands for a physical assumption specific to a material, and provides an expression for a 'physics_quantity' (the dependent variable) as function of other variables, physics_quantity or data (independent variables)."@en ;
                                                                                <http://emmo.info/emmo/top/annotations#EMMO_b432d2d5_25f4_4165_99c5_5935a7763c1a> """The Lennard-Jones potential.

A force field.

An Hamiltonian."""@en ;
                                                                                rdfs:comment "A material_relation can e.g. return a predefined number, return a database query, be an equation that depends on other physics_quantities."@en ;
                                                                                <http://www.w3.org/2004/02/skos/core#prefLabel> "MaterialRelation"@en .


###  http://emmo.info/emmo/middle/models#EMMO_f19ff3b4_6bfe_4c41_a2b2_9affd39c140b
<http://emmo.info/emmo/middle/models#EMMO_f19ff3b4_6bfe_4c41_a2b2_9affd39c140b> rdf:type owl:Class ;
                                                                                rdfs:subClassOf <http://emmo.info/emmo/middle/models#EMMO_db9a009e_f097_43f5_9520_6cbc07e7610b> ;
                                                                                <http://www.w3.org/2004/02/skos/core#prefLabel> "MaterialLaw"@en .


###  http://emmo.info/emmo/middle/models#EMMO_f7ed665b_c2e1_42bc_889b_6b42ed3a36f0
<http://emmo.info/emmo/middle/models#EMMO_f7ed665b_c2e1_42bc_889b_6b42ed3a36f0> rdf:type owl:Class ;
                                                                                rdfs:subClassOf <http://emmo.info/emmo/middle/math#EMMO_54ee6b5e_5261_44a8_86eb_5717e7fdb9d0> ,
                                                                                                <http://emmo.info/emmo/middle/models#EMMO_939483b1_0148_43d1_8b35_851d2cd5d939> ;
                                                                                rdfs:comment """A mathematical model can be defined as a description of a system using mathematical concepts and language to facilitate proper explanation of a system or to study the effects of different components and to make predictions on patterns of behaviour. 

Abramowitz and Stegun, 1968"""@en ;
                                                                                <http://www.w3.org/2004/02/skos/core#prefLabel> "MathematicalModel"@en .


###  http://emmo.info/emmo/middle/perceptual#EMMO_057e7d57_aff0_49de_911a_8861d85cef40
<http://emmo.info/emmo/middle/perceptual#EMMO_057e7d57_aff0_49de_911a_8861d85cef40> rdf:type owl:Class ;
                                                                                    rdfs:subClassOf <http://emmo.info/emmo/middle/perceptual#EMMO_c74da218_9147_4f03_92d1_8894abca55f3> ;
                                                                                    <http://emmo.info/emmo/top/annotations#EMMO_967080e5_2f42_4eb2_a3a9_c58143e835f9> "An 'Graphical' that stands for a token or a composition of tokens from one or more alphabets, without necessarily respecting syntactic rules."@en ;
                                                                                    <http://emmo.info/emmo/top/annotations#EMMO_b432d2d5_25f4_4165_99c5_5935a7763c1a> """fe780
emmo
!5*a
cat
for(i=0;i<N;++i)"""@en ;
                                                                                    <http://www.w3.org/2004/02/skos/core#prefLabel> "Symbolic"@en .


###  http://emmo.info/emmo/middle/perceptual#EMMO_09007bc0_b5f2_4fb9_af01_caf948cf2044
<http://emmo.info/emmo/middle/perceptual#EMMO_09007bc0_b5f2_4fb9_af01_caf948cf2044> rdf:type owl:Class ;
                                                                                    rdfs:subClassOf <http://emmo.info/emmo/middle/perceptual#EMMO_8681074a_e225_4e38_b586_e85b0f43ce38> ;
                                                                                    <http://www.w3.org/2004/02/skos/core#prefLabel> "Java"@en .


###  http://emmo.info/emmo/middle/perceptual#EMMO_0ab0485c_9e5b_4257_a679_90a2dfba5c7c
<http://emmo.info/emmo/middle/perceptual#EMMO_0ab0485c_9e5b_4257_a679_90a2dfba5c7c> rdf:type owl:Class ;
                                                                                    rdfs:subClassOf <http://emmo.info/emmo/middle/perceptual#EMMO_b5957cef_a287_442d_a3ce_fd39f20ba1cd> ;
                                                                                    <http://www.w3.org/2004/02/skos/core#prefLabel> "0-manifold"@en .


###  http://emmo.info/emmo/middle/perceptual#EMMO_0c576e13_4ee7_4f3d_bfe9_1614243df018
<http://emmo.info/emmo/middle/perceptual#EMMO_0c576e13_4ee7_4f3d_bfe9_1614243df018> rdf:type owl:Class ;
                                                                                    rdfs:subClassOf <http://emmo.info/emmo/middle/perceptual#EMMO_b5957cef_a287_442d_a3ce_fd39f20ba1cd> ;
                                                                                    <http://www.w3.org/2004/02/skos/core#prefLabel> "1-manifold"@en .


###  http://emmo.info/emmo/middle/perceptual#EMMO_0ef4ff4a_5458_4f2a_b51f_4689d472a3f2
<http://emmo.info/emmo/middle/perceptual#EMMO_0ef4ff4a_5458_4f2a_b51f_4689d472a3f2> rdf:type owl:Class ;
                                                                                    rdfs:subClassOf <http://emmo.info/emmo/middle/perceptual#EMMO_0c576e13_4ee7_4f3d_bfe9_1614243df018> ;
                                                                                    <http://www.w3.org/2004/02/skos/core#prefLabel> "Curve"@en .


###  http://emmo.info/emmo/middle/perceptual#EMMO_1da53c06_9577_4008_8652_272fa3b62be7
<http://emmo.info/emmo/middle/perceptual#EMMO_1da53c06_9577_4008_8652_272fa3b62be7> rdf:type owl:Class ;
                                                                                    rdfs:subClassOf <http://emmo.info/emmo/middle/perceptual#EMMO_c74da218_9147_4f03_92d1_8894abca55f3> ;
                                                                                    <http://emmo.info/emmo/top/annotations#EMMO_967080e5_2f42_4eb2_a3a9_c58143e835f9> "A 'Graphical' that stands for a real world object that shows a recognizable pictorial pattern without being necessarily associated to a symbolic language."@en ;
                                                                                    <http://emmo.info/emmo/top/annotations#EMMO_b432d2d5_25f4_4165_99c5_5935a7763c1a> """A drawing of a cat.
A circle on a paper sheet.
The Mona Lisa."""@en ;
                                                                                    <http://www.w3.org/2004/02/skos/core#prefLabel> "Pictorial"@en .


###  http://emmo.info/emmo/middle/perceptual#EMMO_25f5ca8e_8f7f_44d8_a392_bd3fe8894458
<http://emmo.info/emmo/middle/perceptual#EMMO_25f5ca8e_8f7f_44d8_a392_bd3fe8894458> rdf:type owl:Class ;
                                                                                    rdfs:subClassOf <http://emmo.info/emmo/middle/perceptual#EMMO_9268958f_7f54_48ab_a693_febe2645892b> ;
                                                                                    <http://www.w3.org/2004/02/skos/core#prefLabel> "Plane"@en .


###  http://emmo.info/emmo/middle/perceptual#EMMO_39362460_2a97_4367_8f93_0418c2ac9a08
<http://emmo.info/emmo/middle/perceptual#EMMO_39362460_2a97_4367_8f93_0418c2ac9a08> rdf:type owl:Class ;
                                                                                    rdfs:subClassOf <http://emmo.info/emmo/middle/perceptual#EMMO_0ab0485c_9e5b_4257_a679_90a2dfba5c7c> ;
                                                                                    <http://www.w3.org/2004/02/skos/core#prefLabel> "Point"@en .


###  http://emmo.info/emmo/middle/perceptual#EMMO_3e309118_e8b7_4021_80f4_642d2df65d94
<http://emmo.info/emmo/middle/perceptual#EMMO_3e309118_e8b7_4021_80f4_642d2df65d94> rdf:type owl:Class ;
                                                                                    rdfs:subClassOf <http://emmo.info/emmo/middle/perceptual#EMMO_0c576e13_4ee7_4f3d_bfe9_1614243df018> ;
                                                                                    <http://www.w3.org/2004/02/skos/core#prefLabel> "Line"@en .


###  http://emmo.info/emmo/middle/perceptual#EMMO_432192c4_111f_4e80_b7cd_c6ce1c1129ea
<http://emmo.info/emmo/middle/perceptual#EMMO_432192c4_111f_4e80_b7cd_c6ce1c1129ea> rdf:type owl:Class ;
                                                                                    rdfs:subClassOf <http://emmo.info/emmo/middle/perceptual#EMMO_a1083d0a_c1fb_471f_8e20_a98f881ad527> ;
                                                                                    <http://www.w3.org/2004/02/skos/core#prefLabel> "Spacing"@en .


###  http://emmo.info/emmo/middle/perceptual#EMMO_46f0f8df_4dc6_418f_8036_10427a3a288e
<http://emmo.info/emmo/middle/perceptual#EMMO_46f0f8df_4dc6_418f_8036_10427a3a288e> rdf:type owl:Class ;
                                                                                    rdfs:subClassOf <http://emmo.info/emmo/middle/perceptual#EMMO_b5957cef_a287_442d_a3ce_fd39f20ba1cd> ;
                                                                                    <http://www.w3.org/2004/02/skos/core#prefLabel> "3-manifold"@en .


###  http://emmo.info/emmo/middle/perceptual#EMMO_48716718_225f_4c88_89e2_d819d30c90a2
<http://emmo.info/emmo/middle/perceptual#EMMO_48716718_225f_4c88_89e2_d819d30c90a2> rdf:type owl:Class ;
                                                                                    rdfs:subClassOf <http://emmo.info/emmo/middle/perceptual#EMMO_d8d2144e_5c8d_455d_a643_5caf4d8d9df8> ;
                                                                                    <http://emmo.info/emmo/top/annotations#EMMO_967080e5_2f42_4eb2_a3a9_c58143e835f9> "A language object that follows syntactic rules of a an idiom (e.g. english, italian)."@en ;
                                                                                    <http://www.w3.org/2004/02/skos/core#prefLabel> "Idiomatic"@en .


###  http://emmo.info/emmo/middle/perceptual#EMMO_4b3afb22_27cf_4ce3_88bc_492bfccb546b
<http://emmo.info/emmo/middle/perceptual#EMMO_4b3afb22_27cf_4ce3_88bc_492bfccb546b> rdf:type owl:Class ;
                                                                                    rdfs:subClassOf <http://emmo.info/emmo/middle/perceptual#EMMO_649bf97b_4397_4005_90d9_219755d92e34> ;
                                                                                    <http://emmo.info/emmo/top/annotations#EMMO_967080e5_2f42_4eb2_a3a9_c58143e835f9> "A 'Perceptual' which stands for a real world object whose spatiotemporal pattern makes it identifiable by an observer as a sound."@en ;
                                                                                    rdfs:comment "'acoustical' refers to the perception mechanism of the observer that can occur through a microphone, a ear."@en ;
                                                                                    <http://www.w3.org/2004/02/skos/core#prefLabel> "Acoustical"@en .


###  http://emmo.info/emmo/middle/perceptual#EMMO_50ea1ec5_f157_41b0_b46b_a9032f17ca10
<http://emmo.info/emmo/middle/perceptual#EMMO_50ea1ec5_f157_41b0_b46b_a9032f17ca10> rdf:type owl:Class ;
                                                                                    rdfs:subClassOf <http://emmo.info/emmo/middle/perceptual#EMMO_89a0c87c_0804_4013_937a_6fe234d9499c> ,
                                                                                                    <http://emmo.info/emmo/middle/reductionistic#EMMO_36c79456_e29c_400d_8bd3_0eedddb82652> ;
                                                                                    <http://emmo.info/emmo/top/annotations#EMMO_967080e5_2f42_4eb2_a3a9_c58143e835f9> "A physical made of more than one symbol sequentially arranged."@en ;
                                                                                    <http://emmo.info/emmo/top/annotations#EMMO_b432d2d5_25f4_4165_99c5_5935a7763c1a> """The word \"cat\" considered as a collection of 'symbol'-s respecting the rules of english language. 

In this example the 'symbolic' entity \"cat\" is not related to the real cat, but it is only a word (like it would be to an italian person that ignores the meaning of this english word).

If an 'interpreter' skilled in english language is involved in a 'semiotic' process with this word, that \"cat\" became also a 'sign' i.e. it became for the 'interpreter' a representation for a real cat."""@en ;
                                                                                    rdfs:comment "A string is made of concatenated symbols whose arrangement is one-dimensional. Each symbol can have only one previous and one next neighborhood (bidirectional list)."@en ,
                                                                                                 "A string is not requested to respect any syntactic rule: it's simply directly made of symbols."@en ;
                                                                                    <http://www.w3.org/2004/02/skos/core#prefLabel> "String"@en .


###  http://emmo.info/emmo/middle/perceptual#EMMO_5f278af9_8593_4e27_a717_ccc9e07a0ddf
<http://emmo.info/emmo/middle/perceptual#EMMO_5f278af9_8593_4e27_a717_ccc9e07a0ddf> rdf:type owl:Class ;
                                                                                    rdfs:subClassOf <http://emmo.info/emmo/middle/perceptual#EMMO_46f0f8df_4dc6_418f_8036_10427a3a288e> ;
                                                                                    <http://www.w3.org/2004/02/skos/core#prefLabel> "EuclideanSpace"@en .


###  http://emmo.info/emmo/middle/perceptual#EMMO_649bf97b_4397_4005_90d9_219755d92e34
<http://emmo.info/emmo/middle/perceptual#EMMO_649bf97b_4397_4005_90d9_219755d92e34> rdf:type owl:Class ;
                                                                                    rdfs:subClassOf <http://emmo.info/emmo/top#EMMO_49267eba_5548_4163_8f36_518d65b583f9> ;
                                                                                    <http://emmo.info/emmo/top/annotations#EMMO_967080e5_2f42_4eb2_a3a9_c58143e835f9> "A 'Physical' which stands for a real world object that can stimulate a perception (e.g. a mental impression, the excitation of a sensor) to an interpreter (human or non-human)."@en ;
                                                                                    <http://emmo.info/emmo/top/annotations#EMMO_b432d2d5_25f4_4165_99c5_5935a7763c1a> """A line scratched on a surface.
A sound.
A smell.
The word 'cat' and the sound of the word 'cat' (the first one is graphical and the second acoustical)."""@en ,
                                                                                                                                                                      """The meta-semiotic process:
I see a cloud in the sky. Since I'm an EMMO ontologist, I create an individual named Cloud under the 'Impression' class.  This semiotic process occurs at meta-level: it's how I use the EMMO as tool for a direct representation of the world.

The semiotic process within EMMO:
My friend looks at the same cloud and says: \"It is an elephant\".
I use the EMMO to record this experience by declaring:
    - my friend as MyFriend individual, belonging to 'Interpreter' classes
    - the sound of the word \"elephant\" as an acoustical impression individual named ElephantWord, belonging to 'Impression'
    - a relation hasSign between Cloud and ElephantWord, that makes ElephantWord also belonging to 'Sign' class and Cloud belonging also to 'Object' class
    - a 'Semiosis' individual called MyFriendElephantCloud that hasParticipant: Cloud, ElephantWord and MyFriend, respectively as object, sign and interpreter."""@en ;
                                                                                    rdfs:comment """'Perceptual' includes real world objects that:
- are part of a communication system (e.g. words, speech, alphabets)
- are not part of a communication system, but can be identified and referred by an interpreter"""@en ,
                                                                                                 """A 'Perceptual' is a meta-object, meaning that is addressed by the ontologist (the meta-interpreter) in a meta-semiotic process occurring outside the EMMO.

A 'Perceptual' becomes an 'Object', when it is part of a 'Semiotic' process described by the ontologist through the EMMO."""@en ,
                                                                                                 "From Latin perceptio (a receiving or collecting, perception, comprehension), from perceptus (perceived, observed)."@en ,
                                                                                                 """This class is the most general superclass for the categorization of real world objects that are recognizable by an interpreter (agent).

A 'Perceptual' can stand for something else in a semiotic process (acting as sign or as object). 

However, a perceptual is not necessarily a 'Sign' (e.g. a line sketched on a blackboard is a recognizable 'Perceptual' but it may stand for nothing)."""@en ;
                                                                                    <http://www.w3.org/2004/02/skos/core#prefLabel> "Perceptual"@en .


###  http://emmo.info/emmo/middle/perceptual#EMMO_64aba1e5_24b7_4140_8eb4_676c35698e79
<http://emmo.info/emmo/middle/perceptual#EMMO_64aba1e5_24b7_4140_8eb4_676c35698e79> rdf:type owl:Class ;
                                                                                    rdfs:subClassOf <http://emmo.info/emmo/middle/perceptual#EMMO_8681074a_e225_4e38_b586_e85b0f43ce38> ;
                                                                                    <http://emmo.info/emmo/top/annotations#EMMO_967080e5_2f42_4eb2_a3a9_c58143e835f9> "A language object respectin the syntactic rules of C++."@en ;
                                                                                    <http://www.w3.org/2004/02/skos/core#prefLabel> "C++"@en .


###  http://emmo.info/emmo/middle/perceptual#EMMO_74b05aed_66bf_43c8_aa2c_752a9ca8be03
<http://emmo.info/emmo/middle/perceptual#EMMO_74b05aed_66bf_43c8_aa2c_752a9ca8be03> rdf:type owl:Class ;
                                                                                    rdfs:subClassOf <http://emmo.info/emmo/middle/perceptual#EMMO_a1083d0a_c1fb_471f_8e20_a98f881ad527> ;
                                                                                    <http://www.w3.org/2004/02/skos/core#prefLabel> "Numeral"@en .


###  http://emmo.info/emmo/middle/perceptual#EMMO_86060335_31c2_4820_b433_27c64aea0366
<http://emmo.info/emmo/middle/perceptual#EMMO_86060335_31c2_4820_b433_27c64aea0366> rdf:type owl:Class ;
                                                                                    rdfs:subClassOf <http://emmo.info/emmo/middle/perceptual#EMMO_9268958f_7f54_48ab_a693_febe2645892b> ;
                                                                                    <http://www.w3.org/2004/02/skos/core#prefLabel> "Torus"@en .


###  http://emmo.info/emmo/middle/perceptual#EMMO_8681074a_e225_4e38_b586_e85b0f43ce38
<http://emmo.info/emmo/middle/perceptual#EMMO_8681074a_e225_4e38_b586_e85b0f43ce38> rdf:type owl:Class ;
                                                                                    rdfs:subClassOf <http://emmo.info/emmo/middle/perceptual#EMMO_d8d2144e_5c8d_455d_a643_5caf4d8d9df8> ;
                                                                                    <http://emmo.info/emmo/top/annotations#EMMO_967080e5_2f42_4eb2_a3a9_c58143e835f9> "A language object that follows syntactic rules of a programming language."@en ;
                                                                                    <http://www.w3.org/2004/02/skos/core#prefLabel> "Software"@en .


###  http://emmo.info/emmo/middle/perceptual#EMMO_89a0c87c_0804_4013_937a_6fe234d9499c
<http://emmo.info/emmo/middle/perceptual#EMMO_89a0c87c_0804_4013_937a_6fe234d9499c> rdf:type owl:Class ;
                                                                                    rdfs:subClassOf <http://emmo.info/emmo/middle/perceptual#EMMO_057e7d57_aff0_49de_911a_8861d85cef40> ;
                                                                                    <http://emmo.info/emmo/top/annotations#EMMO_967080e5_2f42_4eb2_a3a9_c58143e835f9> "A symbolic entity made of other symbolic entities according to a specific spatial configuration."@en ;
                                                                                    rdfs:comment "This class collects individuals that represents arrangements of strings, or other symbolic compositions, without any particular predifined arrangement schema."@en ;
                                                                                    <http://www.w3.org/2004/02/skos/core#prefLabel> "SymbolicComposition"@en .


###  http://emmo.info/emmo/middle/perceptual#EMMO_9268958f_7f54_48ab_a693_febe2645892b
<http://emmo.info/emmo/middle/perceptual#EMMO_9268958f_7f54_48ab_a693_febe2645892b> rdf:type owl:Class ;
                                                                                    rdfs:subClassOf <http://emmo.info/emmo/middle/perceptual#EMMO_b5957cef_a287_442d_a3ce_fd39f20ba1cd> ;
                                                                                    <http://www.w3.org/2004/02/skos/core#prefLabel> "2-manifold"@en .


###  http://emmo.info/emmo/middle/perceptual#EMMO_a1083d0a_c1fb_471f_8e20_a98f881ad527
<http://emmo.info/emmo/middle/perceptual#EMMO_a1083d0a_c1fb_471f_8e20_a98f881ad527> rdf:type owl:Class ;
                                                                                    rdfs:subClassOf <http://emmo.info/emmo/middle/perceptual#EMMO_057e7d57_aff0_49de_911a_8861d85cef40> ;
                                                                                    <http://emmo.info/emmo/top/annotations#EMMO_967080e5_2f42_4eb2_a3a9_c58143e835f9> "The class of individuals that stand for an elementary mark of a specific symbolic code (alphabet)."@en ;
                                                                                    <http://emmo.info/emmo/top/annotations#EMMO_b432d2d5_25f4_4165_99c5_5935a7763c1a> "The class of letter \"A\" is the symbol as idea and the letter A that you see on the screen is the mark."@en ;
                                                                                    rdfs:comment """Subclasses of 'Symbol' are alphabets, in formal languages terminology.

A 'Symbol' is atomic for that alphabet, i.e. it has no parts that are symbols for the same alphabet.
e.g. a math symbol is not made of other math symbols

A Symbol may be a String in another language.
e.g. \"Bq\" is the symbol for Becquerel units when dealing with metrology, or a string of \"B\" and \"q\" symbols when dealing with characters."""@en ,
                                                                                                 """Symbols of a formal language need not be symbols of anything. For instance there are logical constants which do not refer to any idea, but rather serve as a form of punctuation in the language (e.g. parentheses). 

Symbols of a formal language must be capable of being specified without any reference to any interpretation of them. 
(Wikipedia)"""@en ,
                                                                                                 "The class is the idea of the symbol, while the individual of that class stands for a specific mark (or token) of that idea."@en ;
                                                                                    <http://www.w3.org/2004/02/skos/core#prefLabel> "Symbol"@en .


###  http://emmo.info/emmo/middle/perceptual#EMMO_a817035a_3e3c_4709_8ede_3205df3031a3
<http://emmo.info/emmo/middle/perceptual#EMMO_a817035a_3e3c_4709_8ede_3205df3031a3> rdf:type owl:Class ;
                                                                                    rdfs:subClassOf <http://emmo.info/emmo/middle/perceptual#EMMO_a1083d0a_c1fb_471f_8e20_a98f881ad527> ;
                                                                                    <http://www.w3.org/2004/02/skos/core#prefLabel> "Punctuation"@en .


###  http://emmo.info/emmo/middle/perceptual#EMMO_add2e29d_6d87_4b78_9706_588e25557093
<http://emmo.info/emmo/middle/perceptual#EMMO_add2e29d_6d87_4b78_9706_588e25557093> rdf:type owl:Class ;
                                                                                    rdfs:subClassOf <http://emmo.info/emmo/middle/perceptual#EMMO_8681074a_e225_4e38_b586_e85b0f43ce38> ;
                                                                                    <http://www.w3.org/2004/02/skos/core#prefLabel> "Python"@en .


###  http://emmo.info/emmo/middle/perceptual#EMMO_b2a234a8_579a_422c_9305_b8f7e72c76cd
<http://emmo.info/emmo/middle/perceptual#EMMO_b2a234a8_579a_422c_9305_b8f7e72c76cd> rdf:type owl:Class ;
                                                                                    rdfs:subClassOf <http://emmo.info/emmo/middle/perceptual#EMMO_0c576e13_4ee7_4f3d_bfe9_1614243df018> ;
                                                                                    <http://www.w3.org/2004/02/skos/core#prefLabel> "Circle"@en .


###  http://emmo.info/emmo/middle/perceptual#EMMO_b5957cef_a287_442d_a3ce_fd39f20ba1cd
<http://emmo.info/emmo/middle/perceptual#EMMO_b5957cef_a287_442d_a3ce_fd39f20ba1cd> rdf:type owl:Class ;
                                                                                    rdfs:subClassOf <http://emmo.info/emmo/middle/perceptual#EMMO_c74da218_9147_4f03_92d1_8894abca55f3> ;
                                                                                    <http://emmo.info/emmo/top/annotations#EMMO_967080e5_2f42_4eb2_a3a9_c58143e835f9> "A 'graphical' aimed to represent a geometrical concept."@en ;
                                                                                    rdfs:comment """A 'geometrical' stands for real world objects that express a geometrical concept.

This can be achieved in many different ways. For example, a line can be expressed by:
a) an equation like y=mx+q, which is both an 'equation' and a 'geometrical'
b) a line drawn with a pencil on a paper, which is simply a 'graphical' object
c) a set of axioms, when the properties of a line are inferred by the interpreter reading them, that are both 'graphical' and also 'formula'

The case a) is a geometrical and mathematical, b) is geometrical and pictorial, while c) is geometrical and a composition of idiomatic strings."""@en ;
                                                                                    <http://www.w3.org/2004/02/skos/core#prefLabel> "Geometrical"@en .


###  http://emmo.info/emmo/middle/perceptual#EMMO_bed2fe4c_dc7e_43a8_8200_6aac44030bff
<http://emmo.info/emmo/middle/perceptual#EMMO_bed2fe4c_dc7e_43a8_8200_6aac44030bff> rdf:type owl:Class ;
                                                                                    rdfs:subClassOf <http://emmo.info/emmo/middle/perceptual#EMMO_a1083d0a_c1fb_471f_8e20_a98f881ad527> ;
                                                                                    <http://www.w3.org/2004/02/skos/core#prefLabel> "Letter"@en .


###  http://emmo.info/emmo/middle/perceptual#EMMO_c74da218_9147_4f03_92d1_8894abca55f3
<http://emmo.info/emmo/middle/perceptual#EMMO_c74da218_9147_4f03_92d1_8894abca55f3> rdf:type owl:Class ;
                                                                                    rdfs:subClassOf <http://emmo.info/emmo/middle/perceptual#EMMO_649bf97b_4397_4005_90d9_219755d92e34> ;
                                                                                    <http://emmo.info/emmo/top/annotations#EMMO_967080e5_2f42_4eb2_a3a9_c58143e835f9> "A 'Perceptual' which stands for a real world object whose spatial configuration shows a pattern identifiable by an observer."@en ;
                                                                                    <http://emmo.info/emmo/top/annotations#EMMO_b432d2d5_25f4_4165_99c5_5935a7763c1a> "'Graphical' objects include writings, pictures, sketches ..."@en ;
                                                                                    rdfs:comment "From the Ancient Greek ??af? (graph?) which means drawing, painting, writing, a writing, description, and from ???f? (grpho) which means scratch, carve."@en ;
                                                                                    <http://www.w3.org/2004/02/skos/core#prefLabel> "Graphical"@en .


###  http://emmo.info/emmo/middle/perceptual#EMMO_d7bf784a_db94_4dd9_861c_54f262846fbf
<http://emmo.info/emmo/middle/perceptual#EMMO_d7bf784a_db94_4dd9_861c_54f262846fbf> rdf:type owl:Class ;
                                                                                    rdfs:subClassOf <http://emmo.info/emmo/middle/perceptual#EMMO_9268958f_7f54_48ab_a693_febe2645892b> ;
                                                                                    <http://www.w3.org/2004/02/skos/core#prefLabel> "Sphere"@en .


###  http://emmo.info/emmo/middle/perceptual#EMMO_d8d2144e_5c8d_455d_a643_5caf4d8d9df8
<http://emmo.info/emmo/middle/perceptual#EMMO_d8d2144e_5c8d_455d_a643_5caf4d8d9df8> rdf:type owl:Class ;
                                                                                    rdfs:subClassOf <http://emmo.info/emmo/middle/perceptual#EMMO_057e7d57_aff0_49de_911a_8861d85cef40> ;
                                                                                    <http://emmo.info/emmo/top/annotations#EMMO_967080e5_2f42_4eb2_a3a9_c58143e835f9> "A language object is a symbolic object respecting a specific language syntactic rules (a well-formed formula)."@en ;
                                                                                    <http://www.w3.org/2004/02/skos/core#prefLabel> "Language"@en .


###  http://emmo.info/emmo/middle/perceptual#EMMO_e13b2173_1dec_4b97_9ac1_1dc4b418612a
<http://emmo.info/emmo/middle/perceptual#EMMO_e13b2173_1dec_4b97_9ac1_1dc4b418612a> rdf:type owl:Class ;
                                                                                    rdfs:subClassOf <http://emmo.info/emmo/middle/perceptual#EMMO_a1083d0a_c1fb_471f_8e20_a98f881ad527> ;
                                                                                    <http://www.w3.org/2004/02/skos/core#prefLabel> "UTF8"@en .


###  http://emmo.info/emmo/middle/physicalistic#EMMO_25f8b804_9a0b_4387_a3e7_b35bce5365ee
<http://emmo.info/emmo/middle/physicalistic#EMMO_25f8b804_9a0b_4387_a3e7_b35bce5365ee> rdf:type owl:Class ;
                                                                                       rdfs:subClassOf <http://emmo.info/emmo/middle/physicalistic#EMMO_e5488299_8dab_4ebb_900a_26d2abed8396> ;
                                                                                       <http://emmo.info/emmo/top/annotations#EMMO_967080e5_2f42_4eb2_a3a9_c58143e835f9> "The class of individuals that stand for photons elementary particles."@en ;
                                                                                       <http://www.w3.org/2004/02/skos/core#prefLabel> "Photon"@en .


###  http://emmo.info/emmo/middle/physicalistic#EMMO_385b8f6e_43ac_4596_ad76_ac322c68b7ca
<http://emmo.info/emmo/middle/physicalistic#EMMO_385b8f6e_43ac_4596_ad76_ac322c68b7ca> rdf:type owl:Class ;
                                                                                       rdfs:subClassOf <http://emmo.info/emmo/middle/physicalistic#EMMO_c26a0340_d619_4928_b1a1_1a04e88bb89d> ;
                                                                                       <http://emmo.info/emmo/top/annotations#EMMO_967080e5_2f42_4eb2_a3a9_c58143e835f9> "The union of classes of elementary particles that possess mass."@en ;
                                                                                       <http://www.w3.org/2004/02/skos/core#prefLabel> "Massive"@en .


###  http://emmo.info/emmo/middle/physicalistic#EMMO_3c218fbe_60c9_4597_8bcf_41eb1773af1f
<http://emmo.info/emmo/middle/physicalistic#EMMO_3c218fbe_60c9_4597_8bcf_41eb1773af1f> rdf:type owl:Class ;
                                                                                       rdfs:subClassOf <http://emmo.info/emmo/middle/physicalistic#EMMO_70dac51e_bddd_48c2_8a98_7d8395e91fc2> ;
                                                                                       <http://emmo.info/emmo/top/annotations#EMMO_967080e5_2f42_4eb2_a3a9_c58143e835f9> "A 'Physical' with no 'Massive' parts."@en ;
                                                                                       <http://www.w3.org/2004/02/skos/core#prefLabel> "Vacuum"@en .


###  http://emmo.info/emmo/middle/physicalistic#EMMO_4207e895_8b83_4318_996a_72cfb32acd94
<http://emmo.info/emmo/middle/physicalistic#EMMO_4207e895_8b83_4318_996a_72cfb32acd94> rdf:type owl:Class ;
                                                                                       rdfs:subClassOf <http://emmo.info/emmo/middle/physicalistic#EMMO_5b2222df_4da6_442f_8244_96e9e45887d1> ;
                                                                                       <http://emmo.info/emmo/top/annotations#EMMO_967080e5_2f42_4eb2_a3a9_c58143e835f9> "A matter individual that stands for a real world object representing an amount of a physical substance (or mixture of substances) in different states of matter or phases."@en ;
                                                                                       rdfs:comment "A instance of a material (e.g. nitrogen) can represent different states of matter. The fact that the individual also belongs to other classes (e.g. Gas) would reveal the actual form in which the material is found."@en ,
                                                                                                    "Material usually means some definite kind, quality, or quantity of matter, especially as intended for use."@en ;
                                                                                       <http://www.w3.org/2004/02/skos/core#prefLabel> "Material"@en .


###  http://emmo.info/emmo/middle/physicalistic#EMMO_5b2222df_4da6_442f_8244_96e9e45887d1
<http://emmo.info/emmo/middle/physicalistic#EMMO_5b2222df_4da6_442f_8244_96e9e45887d1> rdf:type owl:Class ;
                                                                                       rdfs:subClassOf <http://emmo.info/emmo/middle/physicalistic#EMMO_98ada9d8_f1c8_4f13_99b5_d890f5354152> ;
                                                                                       <http://emmo.info/emmo/top/annotations#EMMO_967080e5_2f42_4eb2_a3a9_c58143e835f9> "A 'Physical' that possesses some 'Massive' parts."@en ;
                                                                                       <http://www.w3.org/2004/02/skos/core#prefLabel> "Matter"@en .


###  http://emmo.info/emmo/middle/physicalistic#EMMO_70dac51e_bddd_48c2_8a98_7d8395e91fc2
<http://emmo.info/emmo/middle/physicalistic#EMMO_70dac51e_bddd_48c2_8a98_7d8395e91fc2> rdf:type owl:Class ;
                                                                                       rdfs:subClassOf <http://emmo.info/emmo/middle/physicalistic#EMMO_98ada9d8_f1c8_4f13_99b5_d890f5354152> ;
                                                                                       <http://emmo.info/emmo/top/annotations#EMMO_967080e5_2f42_4eb2_a3a9_c58143e835f9> "A 'Physical' with 'Massless' parts that are mediators of interactions."@en ;
                                                                                       rdfs:comment """The concepts of matter and field for classical physics, upon which we can categorize physical entities, are replaced in quantum physics by the more general concepts of quantum field.

Here the class 'Field' refers to the quantum field of massless bosonic particles (i.e. photons, gluons), while the class 'Matter' refers to the quantum field of massive fermionic or bosonic particles (e.g. quarks, electrons)."""@en ;
                                                                                       <http://www.w3.org/2004/02/skos/core#prefLabel> "Field"@en .


###  http://emmo.info/emmo/middle/physicalistic#EMMO_72d53756_7fb1_46ed_980f_83f47efbe105
<http://emmo.info/emmo/middle/physicalistic#EMMO_72d53756_7fb1_46ed_980f_83f47efbe105> rdf:type owl:Class ;
                                                                                       rdfs:subClassOf <http://emmo.info/emmo/middle/physicalistic#EMMO_385b8f6e_43ac_4596_ad76_ac322c68b7ca> ;
                                                                                       <http://emmo.info/emmo/top/annotations#EMMO_967080e5_2f42_4eb2_a3a9_c58143e835f9> "The class of individuals that stand for quarks elementary particles."@en ;
                                                                                       <http://www.w3.org/2004/02/skos/core#prefLabel> "Quark"@en .


###  http://emmo.info/emmo/middle/physicalistic#EMMO_7db59e56_f68b_48b7_ae99_891c35ae5c3b
<http://emmo.info/emmo/middle/physicalistic#EMMO_7db59e56_f68b_48b7_ae99_891c35ae5c3b> rdf:type owl:Class ;
                                                                                       rdfs:subClassOf <http://emmo.info/emmo/middle/physicalistic#EMMO_e5488299_8dab_4ebb_900a_26d2abed8396> ;
                                                                                       <http://emmo.info/emmo/top/annotations#EMMO_967080e5_2f42_4eb2_a3a9_c58143e835f9> "The class of individuals that stand for gluons elementary particles."@en ;
                                                                                       <http://www.w3.org/2004/02/skos/core#prefLabel> "Gluon"@en .


###  http://emmo.info/emmo/middle/physicalistic#EMMO_8043d3c6_a4c1_4089_ba34_9744e28e5b3d
<http://emmo.info/emmo/middle/physicalistic#EMMO_8043d3c6_a4c1_4089_ba34_9744e28e5b3d> rdf:type owl:Class ;
                                                                                       rdfs:subClassOf <http://emmo.info/emmo/middle/physicalistic#EMMO_385b8f6e_43ac_4596_ad76_ac322c68b7ca> ;
                                                                                       <http://emmo.info/emmo/top/annotations#EMMO_967080e5_2f42_4eb2_a3a9_c58143e835f9> "The class of individuals that stand for electrons elemntary particles."@en ;
                                                                                       <http://www.w3.org/2004/02/skos/core#prefLabel> "Electron"@en .


###  http://emmo.info/emmo/middle/physicalistic#EMMO_98ada9d8_f1c8_4f13_99b5_d890f5354152
<http://emmo.info/emmo/middle/physicalistic#EMMO_98ada9d8_f1c8_4f13_99b5_d890f5354152> rdf:type owl:Class ;
                                                                                       rdfs:subClassOf <http://emmo.info/emmo/top#EMMO_49267eba_5548_4163_8f36_518d65b583f9> ;
                                                                                       <http://emmo.info/emmo/top/annotations#EMMO_967080e5_2f42_4eb2_a3a9_c58143e835f9> "The perspective for which physical objects are categorized only by concepts coming from applied physical sciences."@en ;
                                                                                       <http://www.w3.org/2004/02/skos/core#prefLabel> "Physicalistic"@en .


###  http://emmo.info/emmo/middle/physicalistic#EMMO_c26a0340_d619_4928_b1a1_1a04e88bb89d
<http://emmo.info/emmo/middle/physicalistic#EMMO_c26a0340_d619_4928_b1a1_1a04e88bb89d> rdf:type owl:Class ;
                                                                                       rdfs:subClassOf <http://emmo.info/emmo/middle/physicalistic#EMMO_98ada9d8_f1c8_4f13_99b5_d890f5354152> ,
                                                                                                       <http://emmo.info/emmo/top/physical#EMMO_0f795e3e_c602_4577_9a43_d5a231aa1360> ;
                                                                                       <http://emmo.info/emmo/top/annotations#EMMO_967080e5_2f42_4eb2_a3a9_c58143e835f9> "The union of all classes categorizing elementary particles according to the Standard Model."@en ;
                                                                                       rdfs:comment "Only a subset of elementary particles from the Standard Model are here included for the sake of simplicity."@en ;
                                                                                       <http://www.w3.org/2004/02/skos/core#prefLabel> "ElementaryParticle"@en .


###  http://emmo.info/emmo/middle/physicalistic#EMMO_e5488299_8dab_4ebb_900a_26d2abed8396
<http://emmo.info/emmo/middle/physicalistic#EMMO_e5488299_8dab_4ebb_900a_26d2abed8396> rdf:type owl:Class ;
                                                                                       rdfs:subClassOf <http://emmo.info/emmo/middle/physicalistic#EMMO_c26a0340_d619_4928_b1a1_1a04e88bb89d> ;
                                                                                       <http://emmo.info/emmo/top/annotations#EMMO_967080e5_2f42_4eb2_a3a9_c58143e835f9> "The union of classes of elementary particles that do not possess mass."@en ;
                                                                                       <http://www.w3.org/2004/02/skos/core#prefLabel> "Massless"@en .


###  http://emmo.info/emmo/middle/physicalistic#EMMO_eb3c61f0_3983_4346_a0c6_e7f6b90a67a8
<http://emmo.info/emmo/middle/physicalistic#EMMO_eb3c61f0_3983_4346_a0c6_e7f6b90a67a8> rdf:type owl:Class ;
                                                                                       rdfs:subClassOf <http://emmo.info/emmo/middle/physicalistic#EMMO_e5488299_8dab_4ebb_900a_26d2abed8396> ;
                                                                                       <http://emmo.info/emmo/top/annotations#EMMO_967080e5_2f42_4eb2_a3a9_c58143e835f9> "The class of individuals that stand for gravitons elementary particles."@en ;
                                                                                       rdfs:comment """While this particle is only supposed to exist, the EMMO approach to classical and quantum systems represents fields as made of particles.

For this reason graviton is an useful concept to homogenize the approach between different fields."""@en ;
                                                                                       <http://www.w3.org/2004/02/skos/core#prefLabel> "Graviton"@en .


###  http://emmo.info/emmo/middle/properties#EMMO_10a5fd39_06aa_4648_9e70_f962a9cb2069
<http://emmo.info/emmo/middle/properties#EMMO_10a5fd39_06aa_4648_9e70_f962a9cb2069> rdf:type owl:Class ;
                                                                                    rdfs:subClassOf <http://emmo.info/emmo/middle/semiotics#EMMO_008fd3b2_4013_451f_8827_52bceab11841> ;
                                                                                    <http://emmo.info/emmo/top/annotations#EMMO_967080e5_2f42_4eb2_a3a9_c58143e835f9> "A 'Semiosis' that involves an 'Observer' that perceives another 'Physical' (the 'Object') through a specific perception mechanism and produces a 'Property' (the 'Sign') that stands for the result of that particular perception."@en ;
                                                                                    <http://www.w3.org/2004/02/skos/core#prefLabel> "Observation"@en .


###  http://emmo.info/emmo/middle/properties#EMMO_1b52ee70_121e_4d8d_8419_3f97cd0bd89c
<http://emmo.info/emmo/middle/properties#EMMO_1b52ee70_121e_4d8d_8419_3f97cd0bd89c> rdf:type owl:Class ;
                                                                                    rdfs:subClassOf <http://emmo.info/emmo/middle/semiotics#EMMO_0527413c_b286_4e9c_b2d0_03fb2a038dee> ;
                                                                                    <http://emmo.info/emmo/top/annotations#EMMO_967080e5_2f42_4eb2_a3a9_c58143e835f9> "An 'interpreter' that perceives another 'entity' (the 'object') through a specific perception mechanism and produces a 'property' (the 'sign') that stands for the result of that particular perception."@en ;
                                                                                    <http://www.w3.org/2004/02/skos/core#prefLabel> "Observer"@en .


###  http://emmo.info/emmo/middle/properties#EMMO_251cfb4f_5c75_4778_91ed_6c8395212fd8
<http://emmo.info/emmo/middle/properties#EMMO_251cfb4f_5c75_4778_91ed_6c8395212fd8> rdf:type owl:Class ;
                                                                                    rdfs:subClassOf <http://emmo.info/emmo/middle/properties#EMMO_b7bcff25_ffc3_474e_9ab5_01b1664bd4ba> ;
                                                                                    <http://emmo.info/emmo/top/annotations#EMMO_967080e5_2f42_4eb2_a3a9_c58143e835f9> "A 'Property' that cannot be univocally determined and depends on an agent (e.g. a human individual, a community) acting as black-box."@en ;
                                                                                    <http://emmo.info/emmo/top/annotations#EMMO_b432d2d5_25f4_4165_99c5_5935a7763c1a> """The beauty of that girl.
The style of your clothing."""@en ;
                                                                                    rdfs:comment """The word subjective means that a non-well defined or an unknown procedure is used for the definition of the property.

This happens due to e.g. the complexity of the object, the lack of a underlying model for the representation of the object, the non-well specified meaning of the property symbols. 

A 'SubjectiveProperty' cannot be used to univocally compare 'Object'-s.

e.g. you cannot evaluate the beauty of a person on objective basis."""@en ;
                                                                                    <http://www.w3.org/2004/02/skos/core#prefLabel> "SubjectiveProperty"@en .


###  http://emmo.info/emmo/middle/properties#EMMO_2a888cdf_ec4a_4ec5_af1c_0343372fc978
<http://emmo.info/emmo/middle/properties#EMMO_2a888cdf_ec4a_4ec5_af1c_0343372fc978> rdf:type owl:Class ;
                                                                                    rdfs:subClassOf <http://emmo.info/emmo/middle/properties#EMMO_b7bcff25_ffc3_474e_9ab5_01b1664bd4ba> ;
                                                                                    <http://emmo.info/emmo/top/annotations#EMMO_967080e5_2f42_4eb2_a3a9_c58143e835f9> "A 'Property' that is determined by each 'Observer' following a well defined 'Observation' procedure through a specific perception channel."@en ;
                                                                                    rdfs:comment "The word objective does not mean that each observation will provide the same results. It means that the observation followed a well defined procedure."@en ,
                                                                                                 "This class refers to what is commonly known as physical property, i.e. a measurable property of physical system, whether is quantifiable or not."@en ;
                                                                                    <http://www.w3.org/2004/02/skos/core#prefLabel> "ObjectiveProperty"@en .


###  http://emmo.info/emmo/middle/properties#EMMO_463bcfda_867b_41d9_a967_211d4d437cfb
<http://emmo.info/emmo/middle/properties#EMMO_463bcfda_867b_41d9_a967_211d4d437cfb> rdf:type owl:Class ;
                                                                                    rdfs:subClassOf <http://emmo.info/emmo/middle/properties#EMMO_10a5fd39_06aa_4648_9e70_f962a9cb2069> ;
                                                                                    <http://emmo.info/emmo/top/annotations#EMMO_967080e5_2f42_4eb2_a3a9_c58143e835f9> "An 'observation' that results in a quantitative comparison of a 'property' of an 'object' with a standard reference."@en ;
                                                                                    <http://www.w3.org/2004/02/skos/core#prefLabel> "Measurement"@en .


###  http://emmo.info/emmo/middle/properties#EMMO_873b0ab3_88e6_4054_b901_5531e01f14a4
<http://emmo.info/emmo/middle/properties#EMMO_873b0ab3_88e6_4054_b901_5531e01f14a4> rdf:type owl:Class ;
                                                                                    rdfs:subClassOf <http://emmo.info/emmo/middle/metrology#EMMO_dd4a7f3e_ef56_466c_ac1a_d2716b5f87ec> ;
                                                                                    <http://www.w3.org/2004/02/skos/core#prefLabel> "MeasuredQuantitativeProperty"@en .


###  http://emmo.info/emmo/middle/properties#EMMO_909415d1_7c43_4d5e_bbeb_7e1910159f66
<http://emmo.info/emmo/middle/properties#EMMO_909415d1_7c43_4d5e_bbeb_7e1910159f66> rdf:type owl:Class ;
                                                                                    rdfs:subClassOf <http://emmo.info/emmo/middle/properties#EMMO_2a888cdf_ec4a_4ec5_af1c_0343372fc978> ;
                                                                                    <http://emmo.info/emmo/top/annotations#EMMO_967080e5_2f42_4eb2_a3a9_c58143e835f9> "An 'ObjectiveProperty' that cannot be quantified."@en ;
                                                                                    <http://emmo.info/emmo/top/annotations#EMMO_b432d2d5_25f4_4165_99c5_5935a7763c1a> """CFC is a 'sign' that stands for the fact that the morphology of atoms composing the microstructure of an entity is predominantly Cubic Face Centered

A color is a nominal property.

Sex of a human being."""@en ;
                                                                                    rdfs:comment """\"Property of a phenomenon, body, or substance, where the property has no magnitude.\"

\"A nominal property has a value, which can be expressed in words, by alphanumerical codes, or by other means.\"

International vocabulary of metrology (VIM)"""@en ;
                                                                                    <http://www.w3.org/2004/02/skos/core#prefLabel> "NominalProperty"@en .


###  http://emmo.info/emmo/middle/properties#EMMO_b7bcff25_ffc3_474e_9ab5_01b1664bd4ba
<http://emmo.info/emmo/middle/properties#EMMO_b7bcff25_ffc3_474e_9ab5_01b1664bd4ba> rdf:type owl:Class ;
                                                                                    rdfs:subClassOf <http://emmo.info/emmo/middle/semiotics#EMMO_35d2e130_6e01_41ed_94f7_00b333d46cf9> ;
                                                                                    <http://emmo.info/emmo/top/annotations#EMMO_967080e5_2f42_4eb2_a3a9_c58143e835f9> """A 'Perceptual' referring to a specific code that is used as 'Conventional' sign to represent an 'Object' according to a specific interaction mechanism by an 'Observer'.

(A property is always a partial representation of an 'Object' since it reflects the 'Object' capability to be part of a specific 'Observation' process)"""@en ;
                                                                                    <http://emmo.info/emmo/top/annotations#EMMO_b432d2d5_25f4_4165_99c5_5935a7763c1a> """Hardness is a subclass of properties.

Vickers hardness is a subclass of hardness that involves the procedures and instruments defined by the standard hardness test."""@en ,
                                                                                                                                                                      """Let's define the class 'colour' as the subclass of the properties that involve photon emission and an electromagnetic radiation sensible observer.

An individual C of this class 'colour' can be defined be declaring the process individual (e.g. daylight illumination) and the observer (e.g. my eyes)

Stating that an entity E hasProperty C, we mean that it can be observed by such setup of process + observer (i.e. observed by my eyes under daylight).

This definition can be generalized by using a generic human eye, so that the observer can be a generic human.

This can be used in material characterization, to define exactly the type of measurement done, including the instrument type."""@en ;
                                                                                    rdfs:comment """A 'Property' is a sort of name or label that we put upon objects that interact with an observer in the same specific way.

e.g. \"hot\" objects are objects that interact with an observer through a perception mechanism aimed to perceive an heat source."""@en ,
                                                                                                 """We know real world entities through observation/perception.

A non-perceivable real world entity does not exist (or it exists on a plane of existance that has no intersection with us and we can say nothing about it).

Perception/observation of a real wolrd entity occurs when the entity stimulate an observer in a peculiar way through a well defined perception channel.

For this reason each property is related to a specific observation process which involves a specific observer with its own perception mechanisms.

The observation process (e.g. a look, a photo shot, a measurement) is performed  by an observer (e.g. you, a camera, an instrument) through a specific perception mechanism (e.g. retina impression, CMOS excitation, piezoelectric sensor activation) and involves an observed entity.

An observation is a semiotic process, since it stimulate an interpretant within the interpreter who can communicate the perception result to other interpreters through a sign which is the property. 

Property subclasses are specializations that depend on the type of observation processes.

e.g. the property 'colour' is related to a process that involves emission or interaction of photon and an observer who can perceive electromagnetic radiation in the visible frequency range. 

Properties usually relies on symbolic systems (e.g. for colour it can be palette or RGB)."""@en ;
                                                                                    <http://www.w3.org/2004/02/skos/core#prefLabel> "Property"@en .


###  http://emmo.info/emmo/middle/properties#EMMO_d0200cf1_e4f4_45ae_873f_b9359daea3cd
<http://emmo.info/emmo/middle/properties#EMMO_d0200cf1_e4f4_45ae_873f_b9359daea3cd> rdf:type owl:Class ;
                                                                                    rdfs:subClassOf <http://emmo.info/emmo/middle/metrology#EMMO_dd4a7f3e_ef56_466c_ac1a_d2716b5f87ec> ;
                                                                                    <http://www.w3.org/2004/02/skos/core#prefLabel> "ModelledQuantitativeProperty"@en .


###  http://emmo.info/emmo/middle/properties#EMMO_d8aa8e1f_b650_416d_88a0_5118de945456
<http://emmo.info/emmo/middle/properties#EMMO_d8aa8e1f_b650_416d_88a0_5118de945456> rdf:type owl:Class ;
                                                                                    rdfs:subClassOf <http://emmo.info/emmo/middle/metrology#EMMO_dd4a7f3e_ef56_466c_ac1a_d2716b5f87ec> ;
                                                                                    <http://emmo.info/emmo/top/annotations#EMMO_967080e5_2f42_4eb2_a3a9_c58143e835f9> "A quantitative property attributed by agreement to a quantity for a given purpose."@en ;
                                                                                    <http://emmo.info/emmo/top/annotations#EMMO_b432d2d5_25f4_4165_99c5_5935a7763c1a> """The thermal conductivity of a copper sample in my laboratory can be assumed to be the conductivity that appears in the vendor specification. This value has been obtained by measurement of a sample which is not the one I have in my laboratory. This conductivity value is then a conventional quantitiative property assigned to my sample through a semiotic process in which no actual measurement is done by my laboratory.

If I don't believe the vendor, then I can measure the actual thermal conductivity. I then perform a measurement process that semiotically assign another value for the conductivity, which is a measured property, since is part of a measurement process.

Then I have two different physical quantities that are properties thanks to two different semiotic processes."""@en ;
                                                                                    rdfs:comment "A property that is associated to an object by convention, or assumption."@en ;
                                                                                    <http://www.w3.org/2004/02/skos/core#prefLabel> "ConventionalQuantitativeProperty"@en .


###  http://emmo.info/emmo/middle/properties#EMMO_f2d5d3ad_2e00_417f_8849_686f3988d929
<http://emmo.info/emmo/middle/properties#EMMO_f2d5d3ad_2e00_417f_8849_686f3988d929> rdf:type owl:Class ;
                                                                                    rdfs:subClassOf <http://emmo.info/emmo/middle/properties#EMMO_1b52ee70_121e_4d8d_8419_3f97cd0bd89c> ;
                                                                                    <http://www.w3.org/2004/02/skos/core#prefLabel> "MeasurementInstrument"@en .


###  http://emmo.info/emmo/middle/reductionistic#EMMO_15db234d_ecaf_4715_9838_4b4ec424fb13
<http://emmo.info/emmo/middle/reductionistic#EMMO_15db234d_ecaf_4715_9838_4b4ec424fb13> rdf:type owl:Class ;
                                                                                        rdfs:subClassOf <http://emmo.info/emmo/top#EMMO_49267eba_5548_4163_8f36_518d65b583f9> ;
                                                                                        <http://emmo.info/emmo/top/annotations#EMMO_967080e5_2f42_4eb2_a3a9_c58143e835f9> "A class devoted to categorize 'Physical'-s according to their granularity relations, first in terms of time evolution (Existent) and then in terms of their composition (State), up to the spatial a-tomistic element (Elementary)."@en ;
                                                                                        rdfs:comment "Direct parthood is the relation used to build the class hierarchy (and the granularity hierarchy) for this perspective." ;
                                                                                        <http://www.w3.org/2004/02/skos/core#prefLabel> "Reductionistic"@en .


###  http://emmo.info/emmo/middle/reductionistic#EMMO_36c79456_e29c_400d_8bd3_0eedddb82652
<http://emmo.info/emmo/middle/reductionistic#EMMO_36c79456_e29c_400d_8bd3_0eedddb82652> rdf:type owl:Class ;
                                                                                        rdfs:subClassOf <http://emmo.info/emmo/middle/reductionistic#EMMO_15db234d_ecaf_4715_9838_4b4ec424fb13> ;
                                                                                        <http://emmo.info/emmo/top/annotations#EMMO_967080e5_2f42_4eb2_a3a9_c58143e835f9> "A 'Physical' which is a tessellation of spatial direct parts."@en ;
                                                                                        <http://emmo.info/emmo/top/annotations#EMMO_b432d2d5_25f4_4165_99c5_5935a7763c1a> """e.g. the existent in my glass is declared at t = t_start as made of two direct parts: the ice and the water. It will continue to exists as state as long as the ice is completely melt at t = t_end. The new state will be completely made of water. Between t_start and t_end there is an exchange of molecules between the ice and the water, but this does not affect the existence of the two states.

If we partition the existent in my glass as ice surrounded by several molecules (we do not use the object water as direct part) then the appearance of a molecule coming from the ice will cause a state to end and another state to begin."""@en ;
                                                                                        rdfs:comment """Direct partitions declaration is a choice of the ontologist that choses the classes to be used as direct parts, according to its own world view.

A 'State' can always be direct partitioned in 'Elementary'-s and 'Void' or 'Physical'.

e.g. the water in my glass can be seen as a single object without declaring direct parts, or as made of H2O molecules direct parts."""@en ,
                                                                                                     """The definition of 'State' implies that its spatial direct parts (i.e. 'physicals') are not gained or lost during its temporal extension (they exist from the left to the right side of the time interval), so that the cardinality of spatial direct parts in a 'State' is constant.

This does not mean that there cannot be a change in the internal structure of the 'State' direct parts. It means only that this change must not affect the existence of the direct part itself.

There is no change in granularity or cardinality of direct parts of a 'State'.

The use of spatial direct parthood in 'State' definition means that a 'State' cannot overlap in space another 'State'."""@en ,
                                                                                                     """The usefulness of 'State' is that it makes it possible to describe the evolution in time of an 'Existent' in terms of series of 'State'-s that can take into account the disappearance or appearance of parts within a 'Physical'. 

A 'State' is a recognizable granularity level of matter, in the sense that its direct parts do not appear or disappear within its lifetime as it can be for a generic 'Existent'."""@en ,
                                                                                                     """There is no change in granularity or cardinality of parts within a state.

The use of spatial direct parthood in state definition means that a state cannot overlap in space another state that is direct part of the same whole."""@en ;
                                                                                        <http://www.w3.org/2004/02/skos/core#prefLabel> "State"@en .


###  http://emmo.info/emmo/middle/reductionistic#EMMO_52211e5e_d767_4812_845e_eb6b402c476a
<http://emmo.info/emmo/middle/reductionistic#EMMO_52211e5e_d767_4812_845e_eb6b402c476a> rdf:type owl:Class ;
                                                                                        rdfs:subClassOf <http://emmo.info/emmo/middle/reductionistic#EMMO_15db234d_ecaf_4715_9838_4b4ec424fb13> ;
                                                                                        <http://emmo.info/emmo/top/annotations#EMMO_967080e5_2f42_4eb2_a3a9_c58143e835f9> "A 'Physical' which is a tessellation of 'State' temporal direct parts."@en ;
                                                                                        rdfs:comment """'Existent' is the EMMO class to be used for representing real world physical objects under a reductionistic perspective (i.e. objects come from the composition of sub-part objects, both in time and space). 

'Existent' class collects all individuals that stand for physical objects that can be structured in well defined temporal sub-parts called states, through the temporal direct parthood relation.

This class provides a first granularity hierarchy in time, and a way to axiomatize tessellation principles for a specific whole with a non-transitivity relation (direct parthood) that helps to retain the granularity levels.

e.g. a car, a supersaturated gas with nucleating nanoparticles, an atom that becomes ionized and then recombines with an electron."""@en ,
                                                                                                     """An 'Existent' individual stands for a real world object for which the ontologist wants to provide univocal tessellation in time.

By definition, the tiles are represented by 'State'-s individual.

Tiles are related to the 'Existent' through temporal direct parthood, enforcing non-transitivity and inverse-functionality."""@en ,
                                                                                                     """Being hasTemporalDirectPart a proper parthood relation, there cannot be 'Existent' made of a single 'State'.

Moreover, due to inverse functionality, a 'State' can be part of only one 'Existent', preventing overlapping between 'Existent'-s."""@en ,
                                                                                                     "ex-sistere (latin): to stay (to persist through time) outside others of the same type (to be distinct from the rest)."@en ;
                                                                                        <http://www.w3.org/2004/02/skos/core#prefLabel> "Existent"@en .


###  http://emmo.info/emmo/middle/semiotics#EMMO_008fd3b2_4013_451f_8827_52bceab11841
<http://emmo.info/emmo/middle/semiotics#EMMO_008fd3b2_4013_451f_8827_52bceab11841> rdf:type owl:Class ;
                                                                                   rdfs:subClassOf <http://emmo.info/emmo/middle/holistic#EMMO_43e9a05d_98af_41b4_92f6_00f79a09bfce> ;
                                                                                   <http://emmo.info/emmo/top/annotations#EMMO_967080e5_2f42_4eb2_a3a9_c58143e835f9> "A 'Process', that has participant an 'Interpreter', that is aimed to produce a 'Sign' representing another participant, the 'Object'."@en ;
                                                                                   <http://emmo.info/emmo/top/annotations#EMMO_b432d2d5_25f4_4165_99c5_5935a7763c1a> """Me looking a cat and saying loud: \"Cat!\" -> the semiosis process

me -> interpreter
cat -> object (in Peirce semiotics)
the cat perceived by my mind -> interpretant
\"Cat!\" -> sign, the produced sign"""@en ;
                                                                                   <http://www.w3.org/2004/02/skos/core#prefLabel> "Semiosis"@en .


###  http://emmo.info/emmo/middle/semiotics#EMMO_0527413c_b286_4e9c_b2d0_03fb2a038dee
<http://emmo.info/emmo/middle/semiotics#EMMO_0527413c_b286_4e9c_b2d0_03fb2a038dee> rdf:type owl:Class ;
                                                                                   rdfs:subClassOf <http://emmo.info/emmo/middle/semiotics#EMMO_b803f122_4acb_4064_9d71_c1e5fd091fc9> ;
                                                                                   <http://emmo.info/emmo/top/annotations#EMMO_967080e5_2f42_4eb2_a3a9_c58143e835f9> "The entity (or agent, or observer, or cognitive entity) who connects 'Sign', 'Interpretant' and 'Object'."@en ;
                                                                                   <http://www.w3.org/2004/02/skos/core#prefLabel> "Interpreter"@en .


###  http://emmo.info/emmo/middle/semiotics#EMMO_054af807_85cd_4a13_8eba_119dfdaaf38b
<http://emmo.info/emmo/middle/semiotics#EMMO_054af807_85cd_4a13_8eba_119dfdaaf38b> rdf:type owl:Class ;
                                                                                   rdfs:subClassOf <http://emmo.info/emmo/middle/semiotics#EMMO_b21a56ed_f969_4612_a6ec_cb7766f7f31d> ;
                                                                                   <http://emmo.info/emmo/top/annotations#EMMO_967080e5_2f42_4eb2_a3a9_c58143e835f9> "The interpreter's internal representation of the object in a semiosis process."@en ;
                                                                                   <http://www.w3.org/2004/02/skos/core#prefLabel> "Interpretant"@en .


###  http://emmo.info/emmo/middle/semiotics#EMMO_0cd58641_824c_4851_907f_f4c3be76630c
<http://emmo.info/emmo/middle/semiotics#EMMO_0cd58641_824c_4851_907f_f4c3be76630c> rdf:type owl:Class ;
                                                                                   rdfs:subClassOf <http://emmo.info/emmo/middle/semiotics#EMMO_b21a56ed_f969_4612_a6ec_cb7766f7f31d> ;
                                                                                   <http://emmo.info/emmo/top/annotations#EMMO_967080e5_2f42_4eb2_a3a9_c58143e835f9> "A 'Sign' that stands for an 'Object' due to causal continguity."@en ;
                                                                                   <http://emmo.info/emmo/top/annotations#EMMO_b432d2d5_25f4_4165_99c5_5935a7763c1a> """Smoke stands for a combustion process (a fire).
My facial expression stands for my emotional status."""@en ;
                                                                                   <http://www.w3.org/2004/02/skos/core#prefLabel> "Index"@en .


###  http://emmo.info/emmo/middle/semiotics#EMMO_35d2e130_6e01_41ed_94f7_00b333d46cf9
<http://emmo.info/emmo/middle/semiotics#EMMO_35d2e130_6e01_41ed_94f7_00b333d46cf9> rdf:type owl:Class ;
                                                                                   rdfs:subClassOf <http://emmo.info/emmo/middle/semiotics#EMMO_b21a56ed_f969_4612_a6ec_cb7766f7f31d> ;
                                                                                   <http://emmo.info/emmo/top/annotations#EMMO_967080e5_2f42_4eb2_a3a9_c58143e835f9> "A 'Sign' that stands for an 'Object' through convention, norm or habit, without any resemblance to it."@en ;
                                                                                   rdfs:comment "In Peirce semiotics this kind of sign category is called symbol. However, since symbol is also used in formal languages, the name is changed in conventional."@en ;
                                                                                   <http://www.w3.org/2004/02/skos/core#prefLabel> "Conventional"@en .


###  http://emmo.info/emmo/middle/semiotics#EMMO_6f5af708_f825_4feb_a0d1_a8d813d3022b
<http://emmo.info/emmo/middle/semiotics#EMMO_6f5af708_f825_4feb_a0d1_a8d813d3022b> rdf:type owl:Class ;
                                                                                   rdfs:subClassOf <http://emmo.info/emmo/middle/semiotics#EMMO_b803f122_4acb_4064_9d71_c1e5fd091fc9> ;
                                                                                   <http://emmo.info/emmo/top/annotations#EMMO_967080e5_2f42_4eb2_a3a9_c58143e835f9> "The object, in Peirce semiotics."@en ;
                                                                                   rdfs:comment """Here is assumed that the concept of 'object' is always relative to a 'semiotic' process. An 'object' does not exists per se, but it's always part of an interpretation.

The EMMO relies on strong reductionism, i.e. everything real is a formless collection of elementary particles: we give a meaning to real world entities only by giving them boundaries and defining them using 'sign'-s. 

In this way the 'sign'-ed entity become and 'object', and the 'object' is the basic entity needed in order to apply a logical formalism to the real world entities (i.e. we can speak of it through its sign, and use logics on it through its sign)."""@en ;
                                                                                   <http://www.w3.org/2004/02/skos/core#prefLabel> "Object"@en .


###  http://emmo.info/emmo/middle/semiotics#EMMO_b21a56ed_f969_4612_a6ec_cb7766f7f31d
<http://emmo.info/emmo/middle/semiotics#EMMO_b21a56ed_f969_4612_a6ec_cb7766f7f31d> rdf:type owl:Class ;
                                                                                   rdfs:subClassOf <http://emmo.info/emmo/middle/semiotics#EMMO_b803f122_4acb_4064_9d71_c1e5fd091fc9> ;
                                                                                   <http://emmo.info/emmo/top/annotations#EMMO_967080e5_2f42_4eb2_a3a9_c58143e835f9> "An 'Physical' that is used as sign (\"semeion\" in greek) that stands for another 'Physical' through an semiotic process."@en ;
                                                                                   <http://emmo.info/emmo/top/annotations#EMMO_b432d2d5_25f4_4165_99c5_5935a7763c1a> """A novel is made of chapters, paragraphs, sentences, words and characters (in a direct parthood mereological hierarchy). 

Each of them are 'sign'-s. 

A character can be the a-tomistic 'sign' for the class of texts.

The horizontal segment in the character \"A\" is direct part of \"A\" but it is not a 'sign' itself.

For plain text we can propose the ASCII symbols, for math the fundamental math symbols."""@en ;
                                                                                   rdfs:comment """A 'Sign' can have temporal-direct-parts which are 'Sign' themselves.

A 'Sign' usually have 'sign' spatial direct parts only up to a certain elementary semiotic level, in which the part is only a 'Physical' and no more a 'Sign' (i.e. it stands for nothing). This elementary semiotic level is peculiar to each particular system of signs (e.g. text, painting).

Just like an 'Elementary' in the 'Physical' branch, each 'Sign' branch should have an a-tomistic mereological part."""@en ,
                                                                                                """According to Peirce, 'Sign' includes three subcategories:
- symbols: that stand for an object through convention
- indeces: that stand for an object due to causal continguity
- icon: that stand for an object due to similitudes e.g. in shape or composition"""@en ;
                                                                                   <http://www.w3.org/2004/02/skos/core#prefLabel> "Sign"@en .


###  http://emmo.info/emmo/middle/semiotics#EMMO_b803f122_4acb_4064_9d71_c1e5fd091fc9
<http://emmo.info/emmo/middle/semiotics#EMMO_b803f122_4acb_4064_9d71_c1e5fd091fc9> rdf:type owl:Class ;
                                                                                   rdfs:subClassOf <http://emmo.info/emmo/middle/holistic#EMMO_49804605_c0fe_4538_abda_f70ba1dc8a5d> ;
                                                                                   <http://emmo.info/emmo/top/annotations#EMMO_967080e5_2f42_4eb2_a3a9_c58143e835f9> "The class of individuals that stands for semiotic objects, i.e. objects that take part on a semiotic process."@en ;
                                                                                   rdfs:comment """Semiotic subclasse are defined using Peirce's semiotic theory.

\"Namely, a sign is something, A, which brings something, B, its interpretant sign determined or created by it, into the same sort of correspondence with something, C, its object, as that in which itself stands to C.\" (Peirce 1902, NEM 4, 2021).

The triadic elements:
- 'sign': the sign A (e.g. a name)
- 'interpretant': the sign B as the effects of the sign A on the interpreter (e.g. the mental concept of what a name means)
- 'object': the object C (e.g. the entity to which the sign A and B refer to)

This class includes also the 'interpeter' i.e. the entity that connects the 'sign' to the 'object'"""@en ;
                                                                                   <http://www.w3.org/2004/02/skos/core#prefLabel> "Semiotic"@en .


###  http://emmo.info/emmo/middle/semiotics#EMMO_d7788d1a_020d_4c78_85a1_13563fcec168
<http://emmo.info/emmo/middle/semiotics#EMMO_d7788d1a_020d_4c78_85a1_13563fcec168> rdf:type owl:Class ;
                                                                                   rdfs:subClassOf <http://emmo.info/emmo/middle/semiotics#EMMO_b21a56ed_f969_4612_a6ec_cb7766f7f31d> ;
                                                                                   <http://emmo.info/emmo/top/annotations#EMMO_967080e5_2f42_4eb2_a3a9_c58143e835f9> "A 'Sign' that stands for an 'Object' by resembling or imitating it, in shape or by sharing a similar logical structure."@en ;
                                                                                   <http://emmo.info/emmo/top/annotations#EMMO_b432d2d5_25f4_4165_99c5_5935a7763c1a> """A picture that reproduces the aspect of a person. 

An equation that reproduces the logical connection of the properties of a physical entity."""@en ;
                                                                                   rdfs:comment """Three subtypes of icon are possible:
 
(a) the image, which depends on a simple quality (e.g. picture)

(b) the diagram, whose internal relations, mainly dyadic or so taken, represent by analogy the relations in something (e.g. math formula, geometric flowchart)

(c) the metaphor, which represents the representative character of a sign by representing a parallelism in something else

[Wikipedia]"""@en ;
                                                                                   <http://www.w3.org/2004/02/skos/core#prefLabel> "Icon"@en .


###  http://emmo.info/emmo/middle/siunits#EMMO_00199e76_69dc_45b6_a9c6_98cc90cdc0f5
<http://emmo.info/emmo/middle/siunits#EMMO_00199e76_69dc_45b6_a9c6_98cc90cdc0f5> rdf:type owl:Class ;
                                                                                 rdfs:subClassOf <http://emmo.info/emmo/middle/siunits#EMMO_e9ffc696_5228_4ff9_8a60_0f5e05e9931b> ;
                                                                                 <http://emmo.info/emmo/top/annotations#EMMO_1f1b164d_ec6a_4faa_8d5e_88bda62316cc> "http://qudt.org/vocab/unit/GRAY" ;
                                                                                 <http://emmo.info/emmo/top/annotations#EMMO_fe015383_afb3_44a6_ae86_043628697aa2> "https://doi.org/10.1351/goldbook.G02696" ;
                                                                                 rdfs:comment "Measurement unit for absorbed dose."@en ;
                                                                                 <http://www.w3.org/2004/02/skos/core#prefLabel> "Gray"@en .


###  http://emmo.info/emmo/middle/siunits#EMMO_068c4e58_2470_4b1c_8454_010dd4906100
<http://emmo.info/emmo/middle/siunits#EMMO_068c4e58_2470_4b1c_8454_010dd4906100> rdf:type owl:Class ;
                                                                                 rdfs:subClassOf <http://emmo.info/emmo/middle/siunits#EMMO_471cb92b_edca_4cf9_bce8_a75084d876b8> ;
                                                                                 <http://www.w3.org/2004/02/skos/core#prefLabel> "Pico"@en .


###  http://emmo.info/emmo/middle/siunits#EMMO_080052a1_f295_44be_a60f_1326ce13f1ba
<http://emmo.info/emmo/middle/siunits#EMMO_080052a1_f295_44be_a60f_1326ce13f1ba> rdf:type owl:Class ;
                                                                                 rdfs:subClassOf <http://emmo.info/emmo/middle/siunits#EMMO_e9ffc696_5228_4ff9_8a60_0f5e05e9931b> ;
                                                                                 <http://emmo.info/emmo/top/annotations#EMMO_1f1b164d_ec6a_4faa_8d5e_88bda62316cc> "http://qudt.org/vocab/unit/W" ;
                                                                                 <http://emmo.info/emmo/top/annotations#EMMO_fe015383_afb3_44a6_ae86_043628697aa2> "https://doi.org/10.1351/goldbook.W06656" ;
                                                                                 rdfs:comment "Measurement unit for power."@en ;
                                                                                 <http://www.w3.org/2004/02/skos/core#prefLabel> "Watt"@en .


###  http://emmo.info/emmo/middle/siunits#EMMO_1181c938_c8f0_4ad6_bc7a_2bfdc0903d29
<http://emmo.info/emmo/middle/siunits#EMMO_1181c938_c8f0_4ad6_bc7a_2bfdc0903d29> rdf:type owl:Class ;
                                                                                 rdfs:subClassOf <http://emmo.info/emmo/middle/siunits#EMMO_471cb92b_edca_4cf9_bce8_a75084d876b8> ;
                                                                                 <http://www.w3.org/2004/02/skos/core#prefLabel> "Deci"@en .


###  http://emmo.info/emmo/middle/siunits#EMMO_1273eb34_de48_43a9_925f_104110469dd2
<http://emmo.info/emmo/middle/siunits#EMMO_1273eb34_de48_43a9_925f_104110469dd2> rdf:type owl:Class ;
                                                                                 rdfs:subClassOf <http://emmo.info/emmo/middle/metrology#EMMO_08b308d4_31cd_4779_a784_aa92fc730f39> ,
                                                                                                 <http://emmo.info/emmo/middle/siunits#EMMO_707c6032_e272_4a20_98b5_d35c4f67be68> ;
                                                                                 <http://emmo.info/emmo/top/annotations#EMMO_967080e5_2f42_4eb2_a3a9_c58143e835f9> "A SI derived unit whos numerical factor in front of the product of SI base units is one."@en ;
                                                                                 <http://emmo.info/emmo/top/annotations#EMMO_b432d2d5_25f4_4165_99c5_5935a7763c1a> """m/s
kg/m^3""" ;
                                                                                 rdfs:comment "This class collects all units that are products or powers of SI base or SI special units only."@en ;
                                                                                 <http://www.w3.org/2004/02/skos/core#prefLabel> "SICoherentDerivedUnit"@en .


###  http://emmo.info/emmo/middle/siunits#EMMO_1d8b370b_c672_4d0c_964e_eaafcbf2f51f
<http://emmo.info/emmo/middle/siunits#EMMO_1d8b370b_c672_4d0c_964e_eaafcbf2f51f> rdf:type owl:Class ;
                                                                                 rdfs:subClassOf <http://emmo.info/emmo/middle/siunits#EMMO_471cb92b_edca_4cf9_bce8_a75084d876b8> ;
                                                                                 <http://www.w3.org/2004/02/skos/core#prefLabel> "Deka"@en .


###  http://emmo.info/emmo/middle/siunits#EMMO_21aaefc1_3f86_4208_b7db_a755f31f0f8c
<http://emmo.info/emmo/middle/siunits#EMMO_21aaefc1_3f86_4208_b7db_a755f31f0f8c> rdf:type owl:Class ;
                                                                                 rdfs:subClassOf <http://emmo.info/emmo/middle/siunits#EMMO_471cb92b_edca_4cf9_bce8_a75084d876b8> ;
                                                                                 <http://www.w3.org/2004/02/skos/core#prefLabel> "Hecto"@en .


###  http://emmo.info/emmo/middle/siunits#EMMO_23bfe79a_cade_48f1_9a8c_fd96e6bac8ba
<http://emmo.info/emmo/middle/siunits#EMMO_23bfe79a_cade_48f1_9a8c_fd96e6bac8ba> rdf:type owl:Class ;
                                                                                 rdfs:subClassOf <http://emmo.info/emmo/middle/siunits#EMMO_471cb92b_edca_4cf9_bce8_a75084d876b8> ;
                                                                                 <http://www.w3.org/2004/02/skos/core#prefLabel> "Femto"@en .


###  http://emmo.info/emmo/middle/siunits#EMMO_254472c6_3dbd_4f02_bc43_571389cd281f
<http://emmo.info/emmo/middle/siunits#EMMO_254472c6_3dbd_4f02_bc43_571389cd281f> rdf:type owl:Class ;
                                                                                 rdfs:subClassOf <http://emmo.info/emmo/middle/siunits#EMMO_471cb92b_edca_4cf9_bce8_a75084d876b8> ;
                                                                                 <http://www.w3.org/2004/02/skos/core#prefLabel> "Zepto"@en .


###  http://emmo.info/emmo/middle/siunits#EMMO_2e5e45fc_f52c_4294_bdc2_5ed7a06dfce7
<http://emmo.info/emmo/middle/siunits#EMMO_2e5e45fc_f52c_4294_bdc2_5ed7a06dfce7> rdf:type owl:Class ;
                                                                                 rdfs:subClassOf <http://emmo.info/emmo/middle/siunits#EMMO_3a185e6c_9e19_4776_b583_19c978156aa0> ;
                                                                                 <http://emmo.info/emmo/top/annotations#EMMO_1f1b164d_ec6a_4faa_8d5e_88bda62316cc> "http://qudt.org/vocab/unit/K" ;
                                                                                 <http://emmo.info/emmo/top/annotations#EMMO_70fe84ff_99b6_4206_a9fc_9a8931836d84> "The kelvin, symbol K, is the SI unit of thermodynamic temperature. It is defined by taking the fixed numerical value of the Boltzmann constant k to be 1.38064910-23 when expressed in the unit J K-1, which is equal to kg m2 s-2 K-1, where the kilogram, metre and second are defined in terms of h, c and ??Cs."@en ;
                                                                                 <http://emmo.info/emmo/top/annotations#EMMO_fe015383_afb3_44a6_ae86_043628697aa2> "https://doi.org/10.1351/goldbook.K03374" ;
                                                                                 <http://www.w3.org/2004/02/skos/core#prefLabel> "Kelvin"@en .


###  http://emmo.info/emmo/middle/siunits#EMMO_314ba716_2d3d_4462_9a4f_d3419ae1df43
<http://emmo.info/emmo/middle/siunits#EMMO_314ba716_2d3d_4462_9a4f_d3419ae1df43> rdf:type owl:Class ;
                                                                                 rdfs:subClassOf <http://emmo.info/emmo/middle/siunits#EMMO_3a185e6c_9e19_4776_b583_19c978156aa0> ;
                                                                                 <http://emmo.info/emmo/top/annotations#EMMO_1f1b164d_ec6a_4faa_8d5e_88bda62316cc> "http://qudt.org/vocab/unit/SEC" ;
                                                                                 <http://emmo.info/emmo/top/annotations#EMMO_70fe84ff_99b6_4206_a9fc_9a8931836d84> "The second, symbol s, is the SI unit of time. It is defined by taking the fixed numerical value of the caesium frequency ??Cs, the unperturbed ground-state hyperfine transition frequency of the caesium 133 atom, to be 9192631770 when expressed in the unit Hz, which is equal to s-1."@en ;
                                                                                 <http://emmo.info/emmo/top/annotations#EMMO_fe015383_afb3_44a6_ae86_043628697aa2> "https://doi.org/10.1351/goldbook.S05513" ;
                                                                                 <http://www.w3.org/2004/02/skos/core#prefLabel> "Second"@en .


###  http://emmo.info/emmo/middle/siunits#EMMO_32129fb5_df25_48fd_a29c_18a2f22a2dd5
<http://emmo.info/emmo/middle/siunits#EMMO_32129fb5_df25_48fd_a29c_18a2f22a2dd5> rdf:type owl:Class ;
                                                                                 rdfs:subClassOf <http://emmo.info/emmo/middle/metrology#EMMO_216f448e_cdbc_4aeb_a529_7a5fe7fc38bb> ,
                                                                                                 <http://emmo.info/emmo/middle/siunits#EMMO_707c6032_e272_4a20_98b5_d35c4f67be68> ;
                                                                                 <http://www.w3.org/2004/02/skos/core#prefLabel> "SIUnitSymbol"@en .


###  http://emmo.info/emmo/middle/siunits#EMMO_33b67e69_3645_4c73_b100_5ea6759221b4
<http://emmo.info/emmo/middle/siunits#EMMO_33b67e69_3645_4c73_b100_5ea6759221b4> rdf:type owl:Class ;
                                                                                 rdfs:subClassOf <http://emmo.info/emmo/middle/siunits#EMMO_e9ffc696_5228_4ff9_8a60_0f5e05e9931b> ;
                                                                                 <http://emmo.info/emmo/top/annotations#EMMO_1f1b164d_ec6a_4faa_8d5e_88bda62316cc> "http://qudt.org/vocab/unit/KAT" ;
                                                                                 <http://emmo.info/emmo/top/annotations#EMMO_fe015383_afb3_44a6_ae86_043628697aa2> "https://doi.org/10.1351/goldbook.K03372" ;
                                                                                 rdfs:comment "Measurement unit for catalytic activity."@en ;
                                                                                 <http://www.w3.org/2004/02/skos/core#prefLabel> "Katal"@en .


###  http://emmo.info/emmo/middle/siunits#EMMO_3a185e6c_9e19_4776_b583_19c978156aa0
<http://emmo.info/emmo/middle/siunits#EMMO_3a185e6c_9e19_4776_b583_19c978156aa0> rdf:type owl:Class ;
                                                                                 rdfs:subClassOf <http://emmo.info/emmo/middle/metrology#EMMO_db716151_6b73_45ff_910c_d182fdcbb4f5> ,
                                                                                                 <http://emmo.info/emmo/middle/siunits#EMMO_32129fb5_df25_48fd_a29c_18a2f22a2dd5> ;
                                                                                 <http://emmo.info/emmo/top/annotations#EMMO_967080e5_2f42_4eb2_a3a9_c58143e835f9> "The base units in the SI system."@en ;
                                                                                 rdfs:seeAlso "https://www.bipm.org/utils/common/pdf/si-brochure/SI-Brochure-9-EN.pdf" ;
                                                                                 <http://www.w3.org/2004/02/skos/core#prefLabel> "SIBaseUnit"@en .


###  http://emmo.info/emmo/middle/siunits#EMMO_3a204900_2b33_47d1_b444_815cc4c8cffa
<http://emmo.info/emmo/middle/siunits#EMMO_3a204900_2b33_47d1_b444_815cc4c8cffa> rdf:type owl:Class ;
                                                                                 rdfs:subClassOf <http://emmo.info/emmo/middle/siunits#EMMO_471cb92b_edca_4cf9_bce8_a75084d876b8> ;
                                                                                 <http://www.w3.org/2004/02/skos/core#prefLabel> "Tera"@en .


###  http://emmo.info/emmo/middle/siunits#EMMO_42955b2d_b465_4666_86cc_ea3c2d685753
<http://emmo.info/emmo/middle/siunits#EMMO_42955b2d_b465_4666_86cc_ea3c2d685753> rdf:type owl:Class ;
                                                                                 rdfs:subClassOf <http://emmo.info/emmo/middle/siunits#EMMO_471cb92b_edca_4cf9_bce8_a75084d876b8> ;
                                                                                 <http://www.w3.org/2004/02/skos/core#prefLabel> "Atto"@en .


###  http://emmo.info/emmo/middle/siunits#EMMO_43a6b269_da31_4bb6_a537_c97df4fff32a
<http://emmo.info/emmo/middle/siunits#EMMO_43a6b269_da31_4bb6_a537_c97df4fff32a> rdf:type owl:Class ;
                                                                                 rdfs:subClassOf <http://emmo.info/emmo/middle/siunits#EMMO_471cb92b_edca_4cf9_bce8_a75084d876b8> ;
                                                                                 <http://www.w3.org/2004/02/skos/core#prefLabel> "Peta"@en .


###  http://emmo.info/emmo/middle/siunits#EMMO_471cb92b_edca_4cf9_bce8_a75084d876b8
<http://emmo.info/emmo/middle/siunits#EMMO_471cb92b_edca_4cf9_bce8_a75084d876b8> rdf:type owl:Class ;
                                                                                 rdfs:subClassOf <http://emmo.info/emmo/middle/metrology#EMMO_7d2afa66_ae9e_4095_a9bf_421d0be401b6> ;
                                                                                 <http://www.w3.org/2004/02/skos/core#prefLabel> "SIMetricPrefix"@en .


###  http://emmo.info/emmo/middle/siunits#EMMO_59c10c5c_47bd_4348_ba39_38836607dfa1
<http://emmo.info/emmo/middle/siunits#EMMO_59c10c5c_47bd_4348_ba39_38836607dfa1> rdf:type owl:Class ;
                                                                                 rdfs:subClassOf <http://emmo.info/emmo/middle/siunits#EMMO_e9ffc696_5228_4ff9_8a60_0f5e05e9931b> ;
                                                                                 <http://emmo.info/emmo/top/annotations#EMMO_1f1b164d_ec6a_4faa_8d5e_88bda62316cc> "http://qudt.org/vocab/unit/OHM" ;
                                                                                 <http://emmo.info/emmo/top/annotations#EMMO_fe015383_afb3_44a6_ae86_043628697aa2> "https://doi.org/10.1351/goldbook.O04280" ;
                                                                                 rdfs:comment "Measurement unit for resistance."@en ;
                                                                                 <http://www.w3.org/2004/02/skos/core#prefLabel> "Ohm"@en .


###  http://emmo.info/emmo/middle/siunits#EMMO_5cf9f86c_86f5_40c4_846d_60371f670e0a
<http://emmo.info/emmo/middle/siunits#EMMO_5cf9f86c_86f5_40c4_846d_60371f670e0a> rdf:type owl:Class ;
                                                                                 rdfs:subClassOf <http://emmo.info/emmo/middle/siunits#EMMO_471cb92b_edca_4cf9_bce8_a75084d876b8> ;
                                                                                 <http://www.w3.org/2004/02/skos/core#prefLabel> "Exa"@en .


###  http://emmo.info/emmo/middle/siunits#EMMO_5eaecadc_4f0d_4a3a_afc7_1fc0b83cc928
<http://emmo.info/emmo/middle/siunits#EMMO_5eaecadc_4f0d_4a3a_afc7_1fc0b83cc928> rdf:type owl:Class ;
                                                                                 rdfs:subClassOf <http://emmo.info/emmo/middle/siunits#EMMO_471cb92b_edca_4cf9_bce8_a75084d876b8> ;
                                                                                 <http://www.w3.org/2004/02/skos/core#prefLabel> "Mega"@en .


###  http://emmo.info/emmo/middle/siunits#EMMO_60b78cc3_6011_4134_95ab_956f56d4bdc1
<http://emmo.info/emmo/middle/siunits#EMMO_60b78cc3_6011_4134_95ab_956f56d4bdc1> rdf:type owl:Class ;
                                                                                 rdfs:subClassOf <http://emmo.info/emmo/middle/siunits#EMMO_8246541a_f1f6_4d03_8bd7_fc6b76d17375> ;
                                                                                 <http://emmo.info/emmo/top/annotations#EMMO_967080e5_2f42_4eb2_a3a9_c58143e835f9> "A derived unit whos numerical factor in front of the product of base units is NOT equal to one."@en ;
                                                                                 <http://www.w3.org/2004/02/skos/core#prefLabel> "SINonCoherentDerivedUnit"@en .


###  http://emmo.info/emmo/middle/siunits#EMMO_696ed548_9477_45ea_993c_6a8f5271914a
<http://emmo.info/emmo/middle/siunits#EMMO_696ed548_9477_45ea_993c_6a8f5271914a> rdf:type owl:Class ;
                                                                                 rdfs:subClassOf <http://emmo.info/emmo/middle/siunits#EMMO_e9ffc696_5228_4ff9_8a60_0f5e05e9931b> ;
                                                                                 <http://emmo.info/emmo/top/annotations#EMMO_1f1b164d_ec6a_4faa_8d5e_88bda62316cc> "http://qudt.org/vocab/unit/C" ;
                                                                                 <http://emmo.info/emmo/top/annotations#EMMO_fe015383_afb3_44a6_ae86_043628697aa2> "https://doi.org/10.1351/goldbook.C01365" ;
                                                                                 rdfs:comment "Measurement unit for electric charge."@en ;
                                                                                 <http://www.w3.org/2004/02/skos/core#prefLabel> "Coulomb"@en .


###  http://emmo.info/emmo/middle/siunits#EMMO_707c6032_e272_4a20_98b5_d35c4f67be68
<http://emmo.info/emmo/middle/siunits#EMMO_707c6032_e272_4a20_98b5_d35c4f67be68> rdf:type owl:Class ;
                                                                                 rdfs:subClassOf <http://emmo.info/emmo/middle/metrology#EMMO_868ae137_4d25_493e_b270_21ea3d94849e> ,
                                                                                                 <http://emmo.info/emmo/middle/siunits#EMMO_feb03a8a_bbb6_4918_a891_46713ef557f4> ;
                                                                                 rdfs:comment "Derived units are defined as products of powers of the base units. When the numerical factor of this product is one, the derived units are called coherent derived units. The base and coherent derived units of the SI form a coherent set, designated the set of coherent SI units."@en ;
                                                                                 <http://www.w3.org/2004/02/skos/core#prefLabel> "SICoherentUnit"@en .


###  http://emmo.info/emmo/middle/siunits#EMMO_74931b1b_c133_4e59_9a75_1bf0e1626201
<http://emmo.info/emmo/middle/siunits#EMMO_74931b1b_c133_4e59_9a75_1bf0e1626201> rdf:type owl:Class ;
                                                                                 rdfs:subClassOf <http://emmo.info/emmo/middle/siunits#EMMO_471cb92b_edca_4cf9_bce8_a75084d876b8> ;
                                                                                 <http://www.w3.org/2004/02/skos/core#prefLabel> "Kilo"@en .


###  http://emmo.info/emmo/middle/siunits#EMMO_7db11dbf_a643_464a_9b56_07eabcc3e9c5
<http://emmo.info/emmo/middle/siunits#EMMO_7db11dbf_a643_464a_9b56_07eabcc3e9c5> rdf:type owl:Class ;
                                                                                 rdfs:subClassOf <http://emmo.info/emmo/middle/siunits#EMMO_3a185e6c_9e19_4776_b583_19c978156aa0> ;
                                                                                 <http://emmo.info/emmo/top/annotations#EMMO_1f1b164d_ec6a_4faa_8d5e_88bda62316cc> "http://qudt.org/vocab/unit/M" ;
                                                                                 <http://emmo.info/emmo/top/annotations#EMMO_70fe84ff_99b6_4206_a9fc_9a8931836d84> "The metre, symbol m, is the SI unit of length. It is defined by taking the fixed numerical value of the speed of light in vacuum c to be 299792458 when expressed in the unit m s-1, where the second is defined in terms of ??Cs."@en ;
                                                                                 <http://emmo.info/emmo/top/annotations#EMMO_fe015383_afb3_44a6_ae86_043628697aa2> "https://doi.org/10.1351/goldbook.M03884" ;
                                                                                 <http://www.w3.org/2004/02/skos/core#prefLabel> "Metre"@en .


###  http://emmo.info/emmo/middle/siunits#EMMO_8246541a_f1f6_4d03_8bd7_fc6b76d17375
<http://emmo.info/emmo/middle/siunits#EMMO_8246541a_f1f6_4d03_8bd7_fc6b76d17375> rdf:type owl:Class ;
                                                                                 rdfs:subClassOf <http://emmo.info/emmo/middle/siunits#EMMO_feb03a8a_bbb6_4918_a891_46713ef557f4> ;
                                                                                 <http://www.w3.org/2004/02/skos/core#prefLabel> "SINonCoherentUnit"@en .


###  http://emmo.info/emmo/middle/siunits#EMMO_8a70dea4_d6ab_4260_b931_a3e990982416
<http://emmo.info/emmo/middle/siunits#EMMO_8a70dea4_d6ab_4260_b931_a3e990982416> rdf:type owl:Class ;
                                                                                 rdfs:subClassOf <http://emmo.info/emmo/middle/siunits#EMMO_e9ffc696_5228_4ff9_8a60_0f5e05e9931b> ;
                                                                                 <http://emmo.info/emmo/top/annotations#EMMO_1f1b164d_ec6a_4faa_8d5e_88bda62316cc> "http://qudt.org/vocab/unit/J" ;
                                                                                 <http://emmo.info/emmo/top/annotations#EMMO_fe015383_afb3_44a6_ae86_043628697aa2> "https://doi.org/10.1351/goldbook.J03363" ;
                                                                                 rdfs:comment "Measurement unit for energy."@en ;
                                                                                 <http://www.w3.org/2004/02/skos/core#prefLabel> "Joule"@en .


###  http://emmo.info/emmo/middle/siunits#EMMO_8d00f093_3f45_4ea3_986c_b3545c3c2f4c
<http://emmo.info/emmo/middle/siunits#EMMO_8d00f093_3f45_4ea3_986c_b3545c3c2f4c> rdf:type owl:Class ;
                                                                                 rdfs:subClassOf <http://emmo.info/emmo/middle/siunits#EMMO_3a185e6c_9e19_4776_b583_19c978156aa0> ;
                                                                                 <http://emmo.info/emmo/top/annotations#EMMO_1f1b164d_ec6a_4faa_8d5e_88bda62316cc> "http://qudt.org/vocab/unit/CD" ;
                                                                                 <http://emmo.info/emmo/top/annotations#EMMO_70fe84ff_99b6_4206_a9fc_9a8931836d84> "The candela, symbol cd, is the SI unit of luminous intensity in a given direction. It is defined by taking the fixed numerical value of the luminous efficacy of monochromatic radiation of frequency 5401012 Hz, Kcd, to be 683 when expressed in the unit lm W-1, which is equal to cd sr W-1, or cd sr kg-1 m-2 s3, where the kilogram, metre and second are defined in terms of h, c and ??Cs."@en ;
                                                                                 <http://emmo.info/emmo/top/annotations#EMMO_fe015383_afb3_44a6_ae86_043628697aa2> "https://doi.org/10.1351/goldbook.C00787" ;
                                                                                 <http://www.w3.org/2004/02/skos/core#prefLabel> "Candela"@en .


###  http://emmo.info/emmo/middle/siunits#EMMO_9bfd6f1e_b0ce_459c_beb7_8f1f41708bba
<http://emmo.info/emmo/middle/siunits#EMMO_9bfd6f1e_b0ce_459c_beb7_8f1f41708bba> rdf:type owl:Class ;
                                                                                 rdfs:subClassOf <http://emmo.info/emmo/middle/siunits#EMMO_3a185e6c_9e19_4776_b583_19c978156aa0> ;
                                                                                 <http://emmo.info/emmo/top/annotations#EMMO_1f1b164d_ec6a_4faa_8d5e_88bda62316cc> "http://qudt.org/vocab/unit/KiloGM" ;
                                                                                 <http://emmo.info/emmo/top/annotations#EMMO_70fe84ff_99b6_4206_a9fc_9a8931836d84> "The kilogram, symbol kg, is the SI unit of mass. It is defined by taking the fixed numerical value of the Planck constant h to be 6.6260701510-34 when expressed in the unit J s, which is equal to kg m2 s-1, where the metre and the second are defined in terms of c and ??Cs."@en ;
                                                                                 <http://emmo.info/emmo/top/annotations#EMMO_fe015383_afb3_44a6_ae86_043628697aa2> "https://doi.org/10.1351/goldbook.K03391" ;
                                                                                 <http://www.w3.org/2004/02/skos/core#prefLabel> "Kilogram"@en .


###  http://emmo.info/emmo/middle/siunits#EMMO_9ff3bf8e_2168_406e_8251_1d158fc948ae
<http://emmo.info/emmo/middle/siunits#EMMO_9ff3bf8e_2168_406e_8251_1d158fc948ae> rdf:type owl:Class ;
                                                                                 rdfs:subClassOf <http://emmo.info/emmo/middle/siunits#EMMO_471cb92b_edca_4cf9_bce8_a75084d876b8> ;
                                                                                 <http://www.w3.org/2004/02/skos/core#prefLabel> "Micro"@en .


###  http://emmo.info/emmo/middle/siunits#EMMO_a121bb1d_5225_4c78_809b_0268c3012208
<http://emmo.info/emmo/middle/siunits#EMMO_a121bb1d_5225_4c78_809b_0268c3012208> rdf:type owl:Class ;
                                                                                 rdfs:subClassOf <http://emmo.info/emmo/middle/siunits#EMMO_e9ffc696_5228_4ff9_8a60_0f5e05e9931b> ,
                                                                                                 <http://emmo.info/emmo/middle/units-extension#EMMO_cdc962d8_f3ea_4764_a57a_c7caa4859179> ;
                                                                                 <http://emmo.info/emmo/top/annotations#EMMO_1f1b164d_ec6a_4faa_8d5e_88bda62316cc> "http://qudt.org/vocab/unit/RAD" ;
                                                                                 <http://emmo.info/emmo/top/annotations#EMMO_967080e5_2f42_4eb2_a3a9_c58143e835f9> "Measure of plane angle."@en ;
                                                                                 <http://emmo.info/emmo/top/annotations#EMMO_fe015383_afb3_44a6_ae86_043628697aa2> "https://doi.org/10.1351/goldbook.R05036" ;
                                                                                 rdfs:comment "Dimensionless measurement unit for plane angle."@en ;
                                                                                 <http://www.w3.org/2004/02/skos/core#prefLabel> "Radian"@en .


###  http://emmo.info/emmo/middle/siunits#EMMO_a3a701ed_6f7d_4a10_9aee_dfa1961fc7b7
<http://emmo.info/emmo/middle/siunits#EMMO_a3a701ed_6f7d_4a10_9aee_dfa1961fc7b7> rdf:type owl:Class ;
                                                                                 rdfs:subClassOf <http://emmo.info/emmo/middle/siunits#EMMO_471cb92b_edca_4cf9_bce8_a75084d876b8> ;
                                                                                 <http://www.w3.org/2004/02/skos/core#prefLabel> "Milli"@en .


###  http://emmo.info/emmo/middle/siunits#EMMO_a80dc6f5_b1aa_41a7_a3a8_cd5040da2162
<http://emmo.info/emmo/middle/siunits#EMMO_a80dc6f5_b1aa_41a7_a3a8_cd5040da2162> rdf:type owl:Class ;
                                                                                 rdfs:subClassOf <http://emmo.info/emmo/middle/siunits#EMMO_e9ffc696_5228_4ff9_8a60_0f5e05e9931b> ;
                                                                                 <http://emmo.info/emmo/top/annotations#EMMO_1f1b164d_ec6a_4faa_8d5e_88bda62316cc> "http://qudt.org/vocab/unit/PA" ;
                                                                                 <http://emmo.info/emmo/top/annotations#EMMO_fe015383_afb3_44a6_ae86_043628697aa2> "https://doi.org/10.1351/goldbook.P04442" ;
                                                                                 rdfs:comment "Measurement unit for pressure."@en ;
                                                                                 <http://www.w3.org/2004/02/skos/core#prefLabel> "Pascal"@en .


###  http://emmo.info/emmo/middle/siunits#EMMO_a8eb4bbb_1bd3_4ad4_b114_2789bcbd2134
<http://emmo.info/emmo/middle/siunits#EMMO_a8eb4bbb_1bd3_4ad4_b114_2789bcbd2134> rdf:type owl:Class ;
                                                                                 rdfs:subClassOf <http://emmo.info/emmo/middle/siunits#EMMO_471cb92b_edca_4cf9_bce8_a75084d876b8> ;
                                                                                 <http://www.w3.org/2004/02/skos/core#prefLabel> "Giga"@en .


###  http://emmo.info/emmo/middle/siunits#EMMO_a9201b2f_e6de_442a_b3a6_d292a5820bc5
<http://emmo.info/emmo/middle/siunits#EMMO_a9201b2f_e6de_442a_b3a6_d292a5820bc5> rdf:type owl:Class ;
                                                                                 rdfs:subClassOf <http://emmo.info/emmo/middle/siunits#EMMO_e9ffc696_5228_4ff9_8a60_0f5e05e9931b> ;
                                                                                 <http://emmo.info/emmo/top/annotations#EMMO_1f1b164d_ec6a_4faa_8d5e_88bda62316cc> "http://qudt.org/vocab/unit/FARAD" ;
                                                                                 <http://emmo.info/emmo/top/annotations#EMMO_fe015383_afb3_44a6_ae86_043628697aa2> "https://doi.org/10.1351/goldbook.F02320" ;
                                                                                 rdfs:comment "Measurement unit for electric capacitance."@en ;
                                                                                 <http://www.w3.org/2004/02/skos/core#prefLabel> "Farad"@en .


###  http://emmo.info/emmo/middle/siunits#EMMO_a979c531_f9fa_4a6e_93c1_a2960241ca64
<http://emmo.info/emmo/middle/siunits#EMMO_a979c531_f9fa_4a6e_93c1_a2960241ca64> rdf:type owl:Class ;
                                                                                 rdfs:subClassOf <http://emmo.info/emmo/middle/siunits#EMMO_e9ffc696_5228_4ff9_8a60_0f5e05e9931b> ;
                                                                                 <http://emmo.info/emmo/top/annotations#EMMO_1f1b164d_ec6a_4faa_8d5e_88bda62316cc> "http://qudt.org/vocab/unit/N" ;
                                                                                 <http://emmo.info/emmo/top/annotations#EMMO_fe015383_afb3_44a6_ae86_043628697aa2> "https://doi.org/10.1351/goldbook.N04135" ;
                                                                                 rdfs:comment "Measurement unit for force."@en ;
                                                                                 <http://www.w3.org/2004/02/skos/core#prefLabel> "Newton"@en .


###  http://emmo.info/emmo/middle/siunits#EMMO_acb50123_87a2_4753_b36c_f87114ad4de2
<http://emmo.info/emmo/middle/siunits#EMMO_acb50123_87a2_4753_b36c_f87114ad4de2> rdf:type owl:Class ;
                                                                                 rdfs:subClassOf <http://emmo.info/emmo/middle/siunits#EMMO_e9ffc696_5228_4ff9_8a60_0f5e05e9931b> ;
                                                                                 <http://emmo.info/emmo/top/annotations#EMMO_1f1b164d_ec6a_4faa_8d5e_88bda62316cc> "http://qudt.org/vocab/unit/T" ;
                                                                                 <http://emmo.info/emmo/top/annotations#EMMO_fe015383_afb3_44a6_ae86_043628697aa2> "https://doi.org/10.1351/goldbook.T06283" ;
                                                                                 rdfs:comment "Measurement unit for magnetic flux density or induction."@en ;
                                                                                 <http://www.w3.org/2004/02/skos/core#prefLabel> "Tesla"@en .


###  http://emmo.info/emmo/middle/siunits#EMMO_b20be325_8bfd_4237_bee7_201ab0fd9c75
<http://emmo.info/emmo/middle/siunits#EMMO_b20be325_8bfd_4237_bee7_201ab0fd9c75> rdf:type owl:Class ;
                                                                                 rdfs:subClassOf <http://emmo.info/emmo/middle/siunits#EMMO_e9ffc696_5228_4ff9_8a60_0f5e05e9931b> ;
                                                                                 <http://emmo.info/emmo/top/annotations#EMMO_1f1b164d_ec6a_4faa_8d5e_88bda62316cc> "http://qudt.org/vocab/unit/DEG_C" ;
                                                                                 <http://emmo.info/emmo/top/annotations#EMMO_fe015383_afb3_44a6_ae86_043628697aa2> "https://doi.org/10.1351/goldbook.D01561" ;
                                                                                 rdfs:comment "Measurement unit for Celsius temperature. This unit can only be used for expressing temperature differences."@en ;
                                                                                 <http://www.w3.org/2004/02/skos/core#prefLabel> "DegreeCelsius"@en .


###  http://emmo.info/emmo/middle/siunits#EMMO_b55cd09a_e54d_4eb1_81dd_03c29d1b878e
<http://emmo.info/emmo/middle/siunits#EMMO_b55cd09a_e54d_4eb1_81dd_03c29d1b878e> rdf:type owl:Class ;
                                                                                 rdfs:subClassOf <http://emmo.info/emmo/middle/siunits#EMMO_471cb92b_edca_4cf9_bce8_a75084d876b8> ;
                                                                                 <http://www.w3.org/2004/02/skos/core#prefLabel> "Centi"@en .


###  http://emmo.info/emmo/middle/siunits#EMMO_b71e4ba5_8f73_4199_8c96_7ea7f94d9e2a
<http://emmo.info/emmo/middle/siunits#EMMO_b71e4ba5_8f73_4199_8c96_7ea7f94d9e2a> rdf:type owl:Class ;
                                                                                 rdfs:subClassOf <http://emmo.info/emmo/middle/siunits#EMMO_e9ffc696_5228_4ff9_8a60_0f5e05e9931b> ;
                                                                                 <http://emmo.info/emmo/top/annotations#EMMO_1f1b164d_ec6a_4faa_8d5e_88bda62316cc> "http://qudt.org/vocab/unit/BQ" ;
                                                                                 <http://emmo.info/emmo/top/annotations#EMMO_70fe84ff_99b6_4206_a9fc_9a8931836d84> "Radioactive decays per second."@en ;
                                                                                 <http://emmo.info/emmo/top/annotations#EMMO_fe015383_afb3_44a6_ae86_043628697aa2> "https://doi.org/10.1351/goldbook.B00624" ;
                                                                                 rdfs:comment "Unit for radioactive activity."@en ;
                                                                                 <http://www.w3.org/2004/02/skos/core#prefLabel> "Becquerel"@en .


###  http://emmo.info/emmo/middle/siunits#EMMO_cf3dd6cc_c5d6_4b3d_aef4_82f3b7a361af
<http://emmo.info/emmo/middle/siunits#EMMO_cf3dd6cc_c5d6_4b3d_aef4_82f3b7a361af> rdf:type owl:Class ;
                                                                                 rdfs:subClassOf <http://emmo.info/emmo/middle/siunits#EMMO_e9ffc696_5228_4ff9_8a60_0f5e05e9931b> ,
                                                                                                 <http://emmo.info/emmo/middle/units-extension#EMMO_6f4d704a_a7c6_4c07_b8a7_ea0bab04128f> ;
                                                                                 <http://emmo.info/emmo/top/annotations#EMMO_1f1b164d_ec6a_4faa_8d5e_88bda62316cc> "http://qudt.org/vocab/unit/SR" ;
                                                                                 <http://emmo.info/emmo/top/annotations#EMMO_967080e5_2f42_4eb2_a3a9_c58143e835f9> "Dimensionless measurement unit for solid angle."@en ;
                                                                                 <http://emmo.info/emmo/top/annotations#EMMO_fe015383_afb3_44a6_ae86_043628697aa2> "https://doi.org/10.1351/goldbook.S05971" ;
                                                                                 <http://www.w3.org/2004/02/skos/core#prefLabel> "Steradian"@en .


###  http://emmo.info/emmo/middle/siunits#EMMO_d41ce84b_4317_41fb_a5d1_6cd281fca106
<http://emmo.info/emmo/middle/siunits#EMMO_d41ce84b_4317_41fb_a5d1_6cd281fca106> rdf:type owl:Class ;
                                                                                 rdfs:subClassOf <http://emmo.info/emmo/middle/metrology#EMMO_c6d4a5e0_7e95_44df_a6db_84ee0a8bbc8e> ,
                                                                                                 <http://emmo.info/emmo/middle/siunits#EMMO_8246541a_f1f6_4d03_8bd7_fc6b76d17375> ;
                                                                                 <http://emmo.info/emmo/top/annotations#EMMO_967080e5_2f42_4eb2_a3a9_c58143e835f9> "A SI base or special unit with a metric prefix."@en ;
                                                                                 rdfs:comment "The presence of the prefix makes this units non-coherent with SI system."@en ;
                                                                                 <http://www.w3.org/2004/02/skos/core#prefLabel> "SIPrefixedUnit"@en .


###  http://emmo.info/emmo/middle/siunits#EMMO_d7b7fd1e_645a_42cb_8f40_85f0d034d3ae
<http://emmo.info/emmo/middle/siunits#EMMO_d7b7fd1e_645a_42cb_8f40_85f0d034d3ae> rdf:type owl:Class ;
                                                                                 rdfs:subClassOf <http://emmo.info/emmo/middle/siunits#EMMO_e9ffc696_5228_4ff9_8a60_0f5e05e9931b> ;
                                                                                 <http://emmo.info/emmo/top/annotations#EMMO_1f1b164d_ec6a_4faa_8d5e_88bda62316cc> "http://qudt.org/vocab/unit/LM" ;
                                                                                 <http://emmo.info/emmo/top/annotations#EMMO_fe015383_afb3_44a6_ae86_043628697aa2> "https://doi.org/10.1351/goldbook.L03639" ;
                                                                                 rdfs:comment "Measurement unit for luminous flux."@en ;
                                                                                 <http://www.w3.org/2004/02/skos/core#prefLabel> "Lumen"@en .


###  http://emmo.info/emmo/middle/siunits#EMMO_d7f11b34_a121_4519_87c0_aa754f1c4737
<http://emmo.info/emmo/middle/siunits#EMMO_d7f11b34_a121_4519_87c0_aa754f1c4737> rdf:type owl:Class ;
                                                                                 rdfs:subClassOf <http://emmo.info/emmo/middle/siunits#EMMO_e9ffc696_5228_4ff9_8a60_0f5e05e9931b> ;
                                                                                 <http://emmo.info/emmo/top/annotations#EMMO_1f1b164d_ec6a_4faa_8d5e_88bda62316cc> "http://qudt.org/vocab/unit/WB" ;
                                                                                 <http://emmo.info/emmo/top/annotations#EMMO_fe015383_afb3_44a6_ae86_043628697aa2> "https://doi.org/10.1351/goldbook.W06666" ;
                                                                                 rdfs:comment "Measurement unit for magnetic flux."@en ;
                                                                                 <http://www.w3.org/2004/02/skos/core#prefLabel> "Weber"@en .


###  http://emmo.info/emmo/middle/siunits#EMMO_da1dd4a7_c611_4ad4_bef6_7646f28aa598
<http://emmo.info/emmo/middle/siunits#EMMO_da1dd4a7_c611_4ad4_bef6_7646f28aa598> rdf:type owl:Class ;
                                                                                 rdfs:subClassOf <http://emmo.info/emmo/middle/siunits#EMMO_e9ffc696_5228_4ff9_8a60_0f5e05e9931b> ;
                                                                                 <http://emmo.info/emmo/top/annotations#EMMO_1f1b164d_ec6a_4faa_8d5e_88bda62316cc> "http://qudt.org/vocab/unit/LUX" ;
                                                                                 <http://emmo.info/emmo/top/annotations#EMMO_fe015383_afb3_44a6_ae86_043628697aa2> "https://doi.org/10.1351/goldbook.L03651" ;
                                                                                 rdfs:comment "Measurement unit for illuminance."@en ;
                                                                                 <http://www.w3.org/2004/02/skos/core#prefLabel> "Lux"@en .


###  http://emmo.info/emmo/middle/siunits#EMMO_daa9ee97_4c5f_42e5_918c_44d7523e8958
<http://emmo.info/emmo/middle/siunits#EMMO_daa9ee97_4c5f_42e5_918c_44d7523e8958> rdf:type owl:Class ;
                                                                                 rdfs:subClassOf <http://emmo.info/emmo/middle/siunits#EMMO_471cb92b_edca_4cf9_bce8_a75084d876b8> ;
                                                                                 <http://www.w3.org/2004/02/skos/core#prefLabel> "Zetta"@en .


###  http://emmo.info/emmo/middle/siunits#EMMO_db5dd38d_ac79_4af6_8782_fee7e7150ae8
<http://emmo.info/emmo/middle/siunits#EMMO_db5dd38d_ac79_4af6_8782_fee7e7150ae8> rdf:type owl:Class ;
                                                                                 rdfs:subClassOf <http://emmo.info/emmo/middle/siunits#EMMO_3a185e6c_9e19_4776_b583_19c978156aa0> ;
                                                                                 <http://emmo.info/emmo/top/annotations#EMMO_1f1b164d_ec6a_4faa_8d5e_88bda62316cc> "http://qudt.org/vocab/unit/A" ;
                                                                                 <http://emmo.info/emmo/top/annotations#EMMO_70fe84ff_99b6_4206_a9fc_9a8931836d84> "The ampere, symbol A, is the SI unit of electric current. It is defined by taking the fixed numerical value of the elementary charge e to be 1.60217663410-19 when expressed in the unit C, which is equal to A s, where the second is defined in terms of ??Cs."@en ;
                                                                                 <http://emmo.info/emmo/top/annotations#EMMO_fe015383_afb3_44a6_ae86_043628697aa2> "https://doi.org/10.1351/goldbook.A00300" ;
                                                                                 <http://www.w3.org/2004/02/skos/core#prefLabel> "Ampere"@en .


###  http://emmo.info/emmo/middle/siunits#EMMO_dc232f53_8ed8_4ddd_9f41_cc057985eadb
<http://emmo.info/emmo/middle/siunits#EMMO_dc232f53_8ed8_4ddd_9f41_cc057985eadb> rdf:type owl:Class ;
                                                                                 rdfs:subClassOf <http://emmo.info/emmo/middle/siunits#EMMO_e9ffc696_5228_4ff9_8a60_0f5e05e9931b> ;
                                                                                 <http://emmo.info/emmo/top/annotations#EMMO_1f1b164d_ec6a_4faa_8d5e_88bda62316cc> "http://qudt.org/vocab/unit/SV" ;
                                                                                 <http://emmo.info/emmo/top/annotations#EMMO_c84c6752_6d64_48cc_9500_e54a3c34898d> "https://en.wikipedia.org/wiki/Equivalent_dose" ;
                                                                                 <http://emmo.info/emmo/top/annotations#EMMO_fe015383_afb3_44a6_ae86_043628697aa2> "https://doi.org/10.1351/goldbook.S05658" ;
                                                                                 rdfs:comment """Measurement unit for equivalent doseof ionizing radiation. 

Sievert is derived from absorbed dose, but takes into account the biological effectiveness of the radiation, which is dependent on the radiation type and energy."""@en ;
                                                                                 <http://www.w3.org/2004/02/skos/core#prefLabel> "Sievert"@en .


###  http://emmo.info/emmo/middle/siunits#EMMO_df6eeb01_1b41_4bd8_9257_a04fbd7cf000
<http://emmo.info/emmo/middle/siunits#EMMO_df6eeb01_1b41_4bd8_9257_a04fbd7cf000> rdf:type owl:Class ;
                                                                                 rdfs:subClassOf <http://emmo.info/emmo/middle/siunits#EMMO_3a185e6c_9e19_4776_b583_19c978156aa0> ;
                                                                                 <http://emmo.info/emmo/top/annotations#EMMO_1f1b164d_ec6a_4faa_8d5e_88bda62316cc> "http://qudt.org/vocab/unit/MOL" ;
                                                                                 <http://emmo.info/emmo/top/annotations#EMMO_70fe84ff_99b6_4206_a9fc_9a8931836d84> "The mole, symbol mol, is the SI unit of amount of substance. One mole contains exactly 6.022 140 76  1023 elementary entities. This number is the fixed numerical value of the Avogadro constant, NA, when expressed in the unit mol-1 and is called the Avogadro number. The amount of substance, symbol n, of a system is a measure of the number of specified elementary entities. An elementary entity may be an atom, a molecule, an ion, an electron, any other particle or specified group of particles."@en ;
                                                                                 <http://emmo.info/emmo/top/annotations#EMMO_fe015383_afb3_44a6_ae86_043628697aa2> "https://doi.org/10.1351/goldbook.M03980" ;
                                                                                 <http://www.w3.org/2004/02/skos/core#prefLabel> "Mole"@en .


###  http://emmo.info/emmo/middle/siunits#EMMO_e1981c25_7c55_4020_aa7a_d2e14ced86d4
<http://emmo.info/emmo/middle/siunits#EMMO_e1981c25_7c55_4020_aa7a_d2e14ced86d4> rdf:type owl:Class ;
                                                                                 rdfs:subClassOf <http://emmo.info/emmo/middle/siunits#EMMO_471cb92b_edca_4cf9_bce8_a75084d876b8> ;
                                                                                 <http://www.w3.org/2004/02/skos/core#prefLabel> "Nano"@en .


###  http://emmo.info/emmo/middle/siunits#EMMO_e2207e91_02b0_4a8a_b13e_61d2a2a839f1
<http://emmo.info/emmo/middle/siunits#EMMO_e2207e91_02b0_4a8a_b13e_61d2a2a839f1> rdf:type owl:Class ;
                                                                                 rdfs:subClassOf <http://emmo.info/emmo/middle/siunits#EMMO_e9ffc696_5228_4ff9_8a60_0f5e05e9931b> ;
                                                                                 <http://emmo.info/emmo/top/annotations#EMMO_1f1b164d_ec6a_4faa_8d5e_88bda62316cc> "http://qudt.org/vocab/unit/V" ;
                                                                                 <http://emmo.info/emmo/top/annotations#EMMO_fe015383_afb3_44a6_ae86_043628697aa2> "https://doi.org/10.1351/goldbook.V06634" ;
                                                                                 rdfs:comment "Measurement unit for voltage."@en ;
                                                                                 <http://www.w3.org/2004/02/skos/core#prefLabel> "Volt"@en .


###  http://emmo.info/emmo/middle/siunits#EMMO_e75f580e_52bf_4dd5_af70_df409cec08fd
<http://emmo.info/emmo/middle/siunits#EMMO_e75f580e_52bf_4dd5_af70_df409cec08fd> rdf:type owl:Class ;
                                                                                 rdfs:subClassOf <http://emmo.info/emmo/middle/siunits#EMMO_e9ffc696_5228_4ff9_8a60_0f5e05e9931b> ;
                                                                                 <http://emmo.info/emmo/top/annotations#EMMO_1f1b164d_ec6a_4faa_8d5e_88bda62316cc> "http://qudt.org/vocab/unit/HZ" ;
                                                                                 <http://emmo.info/emmo/top/annotations#EMMO_fe015383_afb3_44a6_ae86_043628697aa2> "https://doi.org/10.1351/goldbook.H02785" ;
                                                                                 rdfs:comment "Measurement unit for frequence."@en ;
                                                                                 <http://www.w3.org/2004/02/skos/core#prefLabel> "Hertz"@en .


###  http://emmo.info/emmo/middle/siunits#EMMO_e79c62ff_10ad_4ec0_baba_c19ddd4eaa11
<http://emmo.info/emmo/middle/siunits#EMMO_e79c62ff_10ad_4ec0_baba_c19ddd4eaa11> rdf:type owl:Class ;
                                                                                 rdfs:subClassOf <http://emmo.info/emmo/middle/siunits#EMMO_471cb92b_edca_4cf9_bce8_a75084d876b8> ;
                                                                                 <http://www.w3.org/2004/02/skos/core#prefLabel> "Yotta"@en .


###  http://emmo.info/emmo/middle/siunits#EMMO_e9ffc696_5228_4ff9_8a60_0f5e05e9931b
<http://emmo.info/emmo/middle/siunits#EMMO_e9ffc696_5228_4ff9_8a60_0f5e05e9931b> rdf:type owl:Class ;
                                                                                 rdfs:subClassOf <http://emmo.info/emmo/middle/metrology#EMMO_3ee80521_3c23_4dd1_935d_9d522614a3e2> ,
                                                                                                 <http://emmo.info/emmo/middle/siunits#EMMO_32129fb5_df25_48fd_a29c_18a2f22a2dd5> ;
                                                                                 <http://emmo.info/emmo/top/annotations#EMMO_967080e5_2f42_4eb2_a3a9_c58143e835f9> "The 22 derived units that are given a special name in the SI system that stands for units derived by SI base units."@en ;
                                                                                 <http://emmo.info/emmo/top/annotations#EMMO_c84c6752_6d64_48cc_9500_e54a3c34898d> "https://en.wikipedia.org/wiki/International_System_of_Units#Derived_units" ;
                                                                                 rdfs:comment "These units are SI coherent by definition."@en ;
                                                                                 <http://www.w3.org/2004/02/skos/core#prefLabel> "SISpecialUnit"@en .


###  http://emmo.info/emmo/middle/siunits#EMMO_f2523820_04a6_44ab_bb67_8237dda2b0c2
<http://emmo.info/emmo/middle/siunits#EMMO_f2523820_04a6_44ab_bb67_8237dda2b0c2> rdf:type owl:Class ;
                                                                                 rdfs:subClassOf <http://emmo.info/emmo/middle/siunits#EMMO_e9ffc696_5228_4ff9_8a60_0f5e05e9931b> ;
                                                                                 rdfs:comment "Measurement unit for electrical conductance."@en ;
                                                                                 <http://www.w3.org/2004/02/skos/core#prefLabel> "Siemens"@en .


###  http://emmo.info/emmo/middle/siunits#EMMO_f5769206_9257_4b08_bf7b_dad7868c6afc
<http://emmo.info/emmo/middle/siunits#EMMO_f5769206_9257_4b08_bf7b_dad7868c6afc> rdf:type owl:Class ;
                                                                                 rdfs:subClassOf <http://emmo.info/emmo/middle/siunits#EMMO_471cb92b_edca_4cf9_bce8_a75084d876b8> ;
                                                                                 <http://www.w3.org/2004/02/skos/core#prefLabel> "Yocto"@en .


###  http://emmo.info/emmo/middle/siunits#EMMO_fab003c8_f7a6_4346_9988_7161325ed7a3
<http://emmo.info/emmo/middle/siunits#EMMO_fab003c8_f7a6_4346_9988_7161325ed7a3> rdf:type owl:Class ;
                                                                                 rdfs:subClassOf <http://emmo.info/emmo/middle/siunits#EMMO_e9ffc696_5228_4ff9_8a60_0f5e05e9931b> ;
                                                                                 <http://emmo.info/emmo/top/annotations#EMMO_1f1b164d_ec6a_4faa_8d5e_88bda62316cc> "http://qudt.org/vocab/unit/H" ;
                                                                                 <http://emmo.info/emmo/top/annotations#EMMO_fe015383_afb3_44a6_ae86_043628697aa2> "https://doi.org/10.1351/goldbook.H02782" ;
                                                                                 rdfs:comment "Measurement unit for electrical inductance."@en ;
                                                                                 <http://www.w3.org/2004/02/skos/core#prefLabel> "Henry"@en .


###  http://emmo.info/emmo/middle/siunits#EMMO_feb03a8a_bbb6_4918_a891_46713ef557f4
<http://emmo.info/emmo/middle/siunits#EMMO_feb03a8a_bbb6_4918_a891_46713ef557f4> rdf:type owl:Class ;
                                                                                 rdfs:subClassOf <http://emmo.info/emmo/middle/metrology#EMMO_b081b346_7279_46ef_9a3d_2c088fcd79f4> ;
                                                                                 <http://emmo.info/emmo/top/annotations#EMMO_967080e5_2f42_4eb2_a3a9_c58143e835f9> "The set of units provided by the SI referring to the ISQ."@en ;
                                                                                 rdfs:comment "The complete set of SI units includes both the coherent set and the multiples and sub-multiples formed by using the SI prefixes."@en ,
                                                                                              """The names, symbols and prefixes of SI units are defined by the General Conference on Weights and Measures (CGPM).

https://en.wikipedia.org/wiki/General_Conference_on_Weights_and_Measures"""@en ;
                                                                                 <http://www.w3.org/2004/02/skos/core#prefLabel> "SIUnit"@en .


###  http://emmo.info/emmo/middle/units-extension#EMMO_00dd79e0_31a6_427e_9b9c_90f3097e4a96
<http://emmo.info/emmo/middle/units-extension#EMMO_00dd79e0_31a6_427e_9b9c_90f3097e4a96> rdf:type owl:Class ;
                                                                                         rdfs:subClassOf <http://emmo.info/emmo/middle/units-extension#EMMO_6795a4b8_ffd0_4588_a581_a9413fe49cac> ;
                                                                                         <http://emmo.info/emmo/top/annotations#EMMO_1f1b164d_ec6a_4faa_8d5e_88bda62316cc> "http://qudt.org/vocab/unit/Dalton" ;
                                                                                         <http://emmo.info/emmo/top/annotations#EMMO_6dd685dd_1895_46e4_b227_be9f7d643c25> "http://dbpedia.org/page/Unified_atomic_mass_unit" ;
                                                                                         <http://emmo.info/emmo/top/annotations#EMMO_70fe84ff_99b6_4206_a9fc_9a8931836d84> "One dalton is defined as one twelfth of the mass of an unbound neutral atom of carbon-12 in its nuclear and electronic ground state."@en ;
                                                                                         <http://emmo.info/emmo/top/annotations#EMMO_fe015383_afb3_44a6_ae86_043628697aa2> "https://doi.org/10.1351/goldbook.D01514" ;
                                                                                         <http://www.w3.org/2004/02/skos/core#prefLabel> "Dalton"@en .


###  http://emmo.info/emmo/middle/units-extension#EMMO_053648ea_3c0a_468c_89cb_eb009239323a
<http://emmo.info/emmo/middle/units-extension#EMMO_053648ea_3c0a_468c_89cb_eb009239323a> rdf:type owl:Class ;
                                                                                         rdfs:subClassOf <http://emmo.info/emmo/middle/units-extension#EMMO_6795a4b8_ffd0_4588_a581_a9413fe49cac> ;
                                                                                         <http://emmo.info/emmo/top/annotations#EMMO_1f1b164d_ec6a_4faa_8d5e_88bda62316cc> "http://qudt.org/vocab/unit/PARSEC" ;
                                                                                         <http://emmo.info/emmo/top/annotations#EMMO_6dd685dd_1895_46e4_b227_be9f7d643c25> "http://dbpedia.org/page/Astronomical_unit" ;
                                                                                         <http://emmo.info/emmo/top/annotations#EMMO_70fe84ff_99b6_4206_a9fc_9a8931836d84> "One astronomical unit is defined as exactly 149597870700 m, which is roughly the distance from earth to sun."@en ;
                                                                                         <http://emmo.info/emmo/top/annotations#EMMO_c84c6752_6d64_48cc_9500_e54a3c34898d> "https://en.wikipedia.org/wiki/Astronomical_unit" ;
                                                                                         <http://www.w3.org/2004/02/skos/core#prefLabel> "AstronomicalUnit"@en .


###  http://emmo.info/emmo/middle/units-extension#EMMO_15d62b55_38ea_4aec_b7c4_25db1a2e5a01
<http://emmo.info/emmo/middle/units-extension#EMMO_15d62b55_38ea_4aec_b7c4_25db1a2e5a01> rdf:type owl:Class ;
                                                                                         rdfs:subClassOf <http://emmo.info/emmo/middle/metrology#EMMO_5ebd5e01_0ed3_49a2_a30d_cd05cbe72978> ;
                                                                                         <http://emmo.info/emmo/top/annotations#EMMO_967080e5_2f42_4eb2_a3a9_c58143e835f9> "Unit for dimensionless units that cannot be expressed as a 'FractionUnit'."@en ;
                                                                                         <http://emmo.info/emmo/top/annotations#EMMO_b432d2d5_25f4_4165_99c5_5935a7763c1a> "Unit of AtomicNumber"@en ;
                                                                                         <http://www.w3.org/2004/02/skos/core#prefLabel> "PureNumberUnit"@en .


###  http://emmo.info/emmo/middle/units-extension#EMMO_18448443_dcf1_49b8_a321_cf46e2c393e1
<http://emmo.info/emmo/middle/units-extension#EMMO_18448443_dcf1_49b8_a321_cf46e2c393e1> rdf:type owl:Class ;
                                                                                         rdfs:subClassOf <http://emmo.info/emmo/middle/units-extension#EMMO_c2f5ee66_579c_44c6_a2e9_fa2eaa9fa4da> ;
                                                                                         <http://emmo.info/emmo/top/annotations#EMMO_967080e5_2f42_4eb2_a3a9_c58143e835f9> "Unit for quantities of dimension one that are the fraction of two masses."@en ;
                                                                                         <http://emmo.info/emmo/top/annotations#EMMO_b432d2d5_25f4_4165_99c5_5935a7763c1a> "Unit for mass fraction."@en ;
                                                                                         <http://www.w3.org/2004/02/skos/core#prefLabel> "MassFractionUnit"@en .


###  http://emmo.info/emmo/middle/units-extension#EMMO_1e0b665d_db6c_4752_a6d4_262d3a8dbb46
<http://emmo.info/emmo/middle/units-extension#EMMO_1e0b665d_db6c_4752_a6d4_262d3a8dbb46> rdf:type owl:Class ;
                                                                                         rdfs:subClassOf <http://emmo.info/emmo/middle/units-extension#EMMO_6795a4b8_ffd0_4588_a581_a9413fe49cac> ;
                                                                                         <http://emmo.info/emmo/top/annotations#EMMO_1f1b164d_ec6a_4faa_8d5e_88bda62316cc> "http://qudt.org/vocab/unit/ARCMIN" ;
                                                                                         <http://emmo.info/emmo/top/annotations#EMMO_70fe84ff_99b6_4206_a9fc_9a8931836d84> "Measure of plane angle defined as 1/60 or a degree."@en ;
                                                                                         <http://www.w3.org/2004/02/skos/core#altLabel> "MinuteOfArc"@en ;
                                                                                         <http://www.w3.org/2004/02/skos/core#prefLabel> "ArcMinute"@en .


###  http://emmo.info/emmo/middle/units-extension#EMMO_21ef2ed6_c086_4d24_8a75_980d2bcc9282
<http://emmo.info/emmo/middle/units-extension#EMMO_21ef2ed6_c086_4d24_8a75_980d2bcc9282> rdf:type owl:Class ;
                                                                                         rdfs:subClassOf <http://emmo.info/emmo/middle/units-extension#EMMO_6795a4b8_ffd0_4588_a581_a9413fe49cac> ;
                                                                                         <http://emmo.info/emmo/top/annotations#EMMO_1f1b164d_ec6a_4faa_8d5e_88bda62316cc> "http://qudt.org/vocab/unit/HR" ;
                                                                                         <http://emmo.info/emmo/top/annotations#EMMO_70fe84ff_99b6_4206_a9fc_9a8931836d84> "Measure of time defined as 3600 seconds."@en ;
                                                                                         <http://emmo.info/emmo/top/annotations#EMMO_fe015383_afb3_44a6_ae86_043628697aa2> "https://doi.org/10.1351/goldbook.H02866" ;
                                                                                         <http://www.w3.org/2004/02/skos/core#prefLabel> "Hour"@en .


###  http://emmo.info/emmo/middle/units-extension#EMMO_27c530c4_dfcd_486e_b324_54ad4448cd26
<http://emmo.info/emmo/middle/units-extension#EMMO_27c530c4_dfcd_486e_b324_54ad4448cd26> rdf:type owl:Class ;
                                                                                         rdfs:subClassOf <http://emmo.info/emmo/middle/metrology#EMMO_216f448e_cdbc_4aeb_a529_7a5fe7fc38bb> ,
                                                                                                         <http://emmo.info/emmo/middle/metrology#EMMO_591e02fd_8d37_45a6_9d11_bb21cef391a0> ;
                                                                                         <http://emmo.info/emmo/top/annotations#EMMO_1f1b164d_ec6a_4faa_8d5e_88bda62316cc> "http://qudt.org/vocab/unit/ANGSTROM" ;
                                                                                         <http://emmo.info/emmo/top/annotations#EMMO_6dd685dd_1895_46e4_b227_be9f7d643c25> "http://dbpedia.org/page/%C3%85ngstr%C3%B6m" ;
                                                                                         <http://emmo.info/emmo/top/annotations#EMMO_70fe84ff_99b6_4206_a9fc_9a8931836d84> "Measure of length defined as 1e-10 metres."@en ;
                                                                                         <http://emmo.info/emmo/top/annotations#EMMO_c84c6752_6d64_48cc_9500_e54a3c34898d> "https://en.wikipedia.org/wiki/Angstrom" ;
                                                                                         <http://emmo.info/emmo/top/annotations#EMMO_fe015383_afb3_44a6_ae86_043628697aa2> "https://doi.org/10.1351/goldbook.N00350" ;
                                                                                         rdfs:comment """ngstrm is not mentioned in the SI system and deprecated by the International Bureau of Weights and Measures (BIPM).

Dispite of that, it is often used in the natural sciences and technology."""@en ;
                                                                                         <http://www.w3.org/2004/02/skos/core#altLabel> "Angstrom"@en ;
                                                                                         <http://www.w3.org/2004/02/skos/core#prefLabel> "ngstrm"@en .


###  http://emmo.info/emmo/middle/units-extension#EMMO_28ef05a7_ecc1_4df6_8116_c53251fbd4a8
<http://emmo.info/emmo/middle/units-extension#EMMO_28ef05a7_ecc1_4df6_8116_c53251fbd4a8> rdf:type owl:Class ;
                                                                                         rdfs:subClassOf <http://emmo.info/emmo/middle/units-extension#EMMO_6795a4b8_ffd0_4588_a581_a9413fe49cac> ;
                                                                                         <http://emmo.info/emmo/top/annotations#EMMO_1f1b164d_ec6a_4faa_8d5e_88bda62316cc> "http://qudt.org/vocab/unit/DAY" ;
                                                                                         <http://emmo.info/emmo/top/annotations#EMMO_6dd685dd_1895_46e4_b227_be9f7d643c25> "http://dbpedia.org/page/Day" ;
                                                                                         <http://emmo.info/emmo/top/annotations#EMMO_70fe84ff_99b6_4206_a9fc_9a8931836d84> "A measure of time defined as 86 400 seconds."@en ;
                                                                                         <http://emmo.info/emmo/top/annotations#EMMO_fe015383_afb3_44a6_ae86_043628697aa2> "https://doi.org/10.1351/goldbook.D01527" ;
                                                                                         <http://www.w3.org/2004/02/skos/core#prefLabel> "Day"@en .


###  http://emmo.info/emmo/middle/units-extension#EMMO_4a27950a_0d31_4175_bd4e_14995aa94702
<http://emmo.info/emmo/middle/units-extension#EMMO_4a27950a_0d31_4175_bd4e_14995aa94702> rdf:type owl:Class ;
                                                                                         rdfs:subClassOf <http://emmo.info/emmo/middle/siunits#EMMO_1273eb34_de48_43a9_925f_104110469dd2> ;
                                                                                         <http://emmo.info/emmo/top/annotations#EMMO_1f1b164d_ec6a_4faa_8d5e_88bda62316cc> "http://qudt.org/vocab/unit/M-PER-SEC" ;
                                                                                         <http://emmo.info/emmo/top/annotations#EMMO_967080e5_2f42_4eb2_a3a9_c58143e835f9> "SI coherent measurement unit for speed."@en ;
                                                                                         <http://emmo.info/emmo/top/annotations#EMMO_e55f2d7c_9893_48cd_b4a4_fdf38253bd20> "http://www.ontology-of-units-of-measure.org/resource/om-2/metrePerSecond-Time" ;
                                                                                         <http://www.w3.org/2004/02/skos/core#prefLabel> "MetrePerSecond"@en .


###  http://emmo.info/emmo/middle/units-extension#EMMO_52e4cb25_da39_45e2_a6db_063ec5730499
<http://emmo.info/emmo/middle/units-extension#EMMO_52e4cb25_da39_45e2_a6db_063ec5730499> rdf:type owl:Class ;
                                                                                         rdfs:subClassOf <http://emmo.info/emmo/middle/metrology#EMMO_b081b346_7279_46ef_9a3d_2c088fcd79f4> ;
                                                                                         <http://emmo.info/emmo/top/annotations#EMMO_967080e5_2f42_4eb2_a3a9_c58143e835f9> "The centimetregramsecond (CGS) system of units."@en ;
                                                                                         <http://emmo.info/emmo/top/annotations#EMMO_c84c6752_6d64_48cc_9500_e54a3c34898d> "https://en.wikipedia.org/wiki/Centimetre%E2%80%93gram%E2%80%93second_system_of_units" ;
                                                                                         rdfs:comment "CGS is a variant of the metric system."@en ;
                                                                                         <http://www.w3.org/2004/02/skos/core#prefLabel> "CGSUnit"@en .


###  http://emmo.info/emmo/middle/units-extension#EMMO_6795a4b8_ffd0_4588_a581_a9413fe49cac
<http://emmo.info/emmo/middle/units-extension#EMMO_6795a4b8_ffd0_4588_a581_a9413fe49cac> rdf:type owl:Class ;
                                                                                         rdfs:subClassOf <http://emmo.info/emmo/middle/metrology#EMMO_3ee80521_3c23_4dd1_935d_9d522614a3e2> ,
                                                                                                         <http://emmo.info/emmo/middle/metrology#EMMO_591e02fd_8d37_45a6_9d11_bb21cef391a0> ;
                                                                                         <http://emmo.info/emmo/top/annotations#EMMO_967080e5_2f42_4eb2_a3a9_c58143e835f9> "Non-SI units mentioned in the SI."@en ;
                                                                                         <http://emmo.info/emmo/top/annotations#EMMO_c84c6752_6d64_48cc_9500_e54a3c34898d> "https://en.wikipedia.org/wiki/Non-SI_units_mentioned_in_the_SI" ;
                                                                                         rdfs:comment "This is a list of units that are not defined as part of the International System of Units (SI), but are otherwise mentioned in the SI brouchure, because either the General Conference on Weights and Measures (CGPM) accepts their use as being multiples or submultiples of SI-units, they have important contemporary application worldwide, or are otherwise commonly encountered worldwide."@en ;
                                                                                         <http://www.w3.org/2004/02/skos/core#prefLabel> "SIAcceptedSpecialUnit"@en .


###  http://emmo.info/emmo/middle/units-extension#EMMO_6a4547ab_3abb_430d_b81b_ce32d47729f5
<http://emmo.info/emmo/middle/units-extension#EMMO_6a4547ab_3abb_430d_b81b_ce32d47729f5> rdf:type owl:Class ;
                                                                                         rdfs:subClassOf <http://emmo.info/emmo/middle/units-extension#EMMO_6795a4b8_ffd0_4588_a581_a9413fe49cac> ;
                                                                                         <http://emmo.info/emmo/top/annotations#EMMO_1f1b164d_ec6a_4faa_8d5e_88bda62316cc> "http://qudt.org/vocab/unit/ARCSEC" ;
                                                                                         <http://emmo.info/emmo/top/annotations#EMMO_70fe84ff_99b6_4206_a9fc_9a8931836d84> "Measure of plane angle defined as 1/3600 or a degree."@en ;
                                                                                         <http://www.w3.org/2004/02/skos/core#altLabel> "SecondOfArc"@en ;
                                                                                         <http://www.w3.org/2004/02/skos/core#prefLabel> "ArcSecond"@en .


###  http://emmo.info/emmo/middle/units-extension#EMMO_6c7160fc_cc64_46f0_b43b_aba65e9952e3
<http://emmo.info/emmo/middle/units-extension#EMMO_6c7160fc_cc64_46f0_b43b_aba65e9952e3> rdf:type owl:Class ;
                                                                                         rdfs:subClassOf <http://emmo.info/emmo/middle/units-extension#EMMO_6795a4b8_ffd0_4588_a581_a9413fe49cac> ;
                                                                                         <http://emmo.info/emmo/top/annotations#EMMO_1f1b164d_ec6a_4faa_8d5e_88bda62316cc> "http://qudt.org/vocab/unit/B" ;
                                                                                         <http://emmo.info/emmo/top/annotations#EMMO_70fe84ff_99b6_4206_a9fc_9a8931836d84> "One bel is defined as `1/2 ln(10) neper`."@en ;
                                                                                         <http://emmo.info/emmo/top/annotations#EMMO_967080e5_2f42_4eb2_a3a9_c58143e835f9> "Unit of measurement for quantities of type level or level difference."@en ;
                                                                                         <http://emmo.info/emmo/top/annotations#EMMO_c84c6752_6d64_48cc_9500_e54a3c34898d> "https://en.wikipedia.org/wiki/Decibel" ;
                                                                                         rdfs:comment "Today decibel (one tenth of a bel) is commonly used instead of bel."@en ,
                                                                                                      "bel is used to express the ratio of one value of a power or field quantity to another, on a logarithmic scale, the logarithmic quantity being called the power level or field level, respectively."@en ;
                                                                                         <http://www.w3.org/2004/02/skos/core#prefLabel> "Bel"@en .


###  http://emmo.info/emmo/middle/units-extension#EMMO_6f4d704a_a7c6_4c07_b8a7_ea0bab04128f
<http://emmo.info/emmo/middle/units-extension#EMMO_6f4d704a_a7c6_4c07_b8a7_ea0bab04128f> rdf:type owl:Class ;
                                                                                         rdfs:subClassOf <http://emmo.info/emmo/middle/units-extension#EMMO_c2f5ee66_579c_44c6_a2e9_fa2eaa9fa4da> ;
                                                                                         <http://emmo.info/emmo/top/annotations#EMMO_967080e5_2f42_4eb2_a3a9_c58143e835f9> "Unit for quantities of dimension one that are the fraction of two areas."@en ;
                                                                                         <http://emmo.info/emmo/top/annotations#EMMO_b432d2d5_25f4_4165_99c5_5935a7763c1a> "Unit for solid angle."@en ;
                                                                                         <http://www.w3.org/2004/02/skos/core#prefLabel> "AreaFractionUnit"@en .


###  http://emmo.info/emmo/middle/units-extension#EMMO_9fd1e79d_41d1_44f8_8142_66dbdf0fc7ad
<http://emmo.info/emmo/middle/units-extension#EMMO_9fd1e79d_41d1_44f8_8142_66dbdf0fc7ad> rdf:type owl:Class ;
                                                                                         rdfs:subClassOf <http://emmo.info/emmo/middle/units-extension#EMMO_c2f5ee66_579c_44c6_a2e9_fa2eaa9fa4da> ;
                                                                                         <http://emmo.info/emmo/top/annotations#EMMO_967080e5_2f42_4eb2_a3a9_c58143e835f9> "Unit for quantities of dimension one that are the fraction of two volumes."@en ;
                                                                                         <http://emmo.info/emmo/top/annotations#EMMO_b432d2d5_25f4_4165_99c5_5935a7763c1a> "Unit for volume fraction."@en ;
                                                                                         <http://www.w3.org/2004/02/skos/core#prefLabel> "VolumeFractionUnit"@en .


###  http://emmo.info/emmo/middle/units-extension#EMMO_a055d311_9990_40a5_b2f2_288412f5d6a5
<http://emmo.info/emmo/middle/units-extension#EMMO_a055d311_9990_40a5_b2f2_288412f5d6a5> rdf:type owl:Class ;
                                                                                         rdfs:subClassOf <http://emmo.info/emmo/middle/siunits#EMMO_1273eb34_de48_43a9_925f_104110469dd2> ;
                                                                                         <http://emmo.info/emmo/top/annotations#EMMO_1f1b164d_ec6a_4faa_8d5e_88bda62316cc> "http://qudt.org/vocab/unit/M3" ;
                                                                                         <http://emmo.info/emmo/top/annotations#EMMO_967080e5_2f42_4eb2_a3a9_c58143e835f9> "SI coherent measurement unit for volume."@en ;
                                                                                         <http://emmo.info/emmo/top/annotations#EMMO_e55f2d7c_9893_48cd_b4a4_fdf38253bd20> "http://www.ontology-of-units-of-measure.org/resource/om-2/cubicMetre" ;
                                                                                         <http://www.w3.org/2004/02/skos/core#prefLabel> "CubicMetre"@en .


###  http://emmo.info/emmo/middle/units-extension#EMMO_a155dc93_d266_487e_b5e7_2a2c72d5ebf9
<http://emmo.info/emmo/middle/units-extension#EMMO_a155dc93_d266_487e_b5e7_2a2c72d5ebf9> rdf:type owl:Class ;
                                                                                         rdfs:subClassOf <http://emmo.info/emmo/middle/units-extension#EMMO_6795a4b8_ffd0_4588_a581_a9413fe49cac> ;
                                                                                         <http://emmo.info/emmo/top/annotations#EMMO_1f1b164d_ec6a_4faa_8d5e_88bda62316cc> "http://qudt.org/vocab/unit/L" ;
                                                                                         <http://emmo.info/emmo/top/annotations#EMMO_70fe84ff_99b6_4206_a9fc_9a8931836d84> "A non-SI unit of volume defined as 1 cubic decimetre (dm3),"@en ;
                                                                                         <http://emmo.info/emmo/top/annotations#EMMO_fe015383_afb3_44a6_ae86_043628697aa2> "https://doi.org/10.1351/goldbook.L03594" ;
                                                                                         <http://www.w3.org/2004/02/skos/core#prefLabel> "Litre"@en .


###  http://emmo.info/emmo/middle/units-extension#EMMO_b0d1c460_d06b_4c7f_8832_148bc1c8e7dc
<http://emmo.info/emmo/middle/units-extension#EMMO_b0d1c460_d06b_4c7f_8832_148bc1c8e7dc> rdf:type owl:Class ;
                                                                                         rdfs:subClassOf <http://emmo.info/emmo/middle/siunits#EMMO_1273eb34_de48_43a9_925f_104110469dd2> ;
                                                                                         <http://emmo.info/emmo/top/annotations#EMMO_1f1b164d_ec6a_4faa_8d5e_88bda62316cc> "http://qudt.org/vocab/unit/M2" ;
                                                                                         <http://emmo.info/emmo/top/annotations#EMMO_967080e5_2f42_4eb2_a3a9_c58143e835f9> "SI coherent measurement unit for area."@en ;
                                                                                         <http://emmo.info/emmo/top/annotations#EMMO_e55f2d7c_9893_48cd_b4a4_fdf38253bd20> "http://www.ontology-of-units-of-measure.org/resource/om-2/squareMetre" ;
                                                                                         <http://www.w3.org/2004/02/skos/core#prefLabel> "SquareMetre"@en .


###  http://emmo.info/emmo/middle/units-extension#EMMO_b41515a9_28d8_4d78_8165_74b2fc72f89e
<http://emmo.info/emmo/middle/units-extension#EMMO_b41515a9_28d8_4d78_8165_74b2fc72f89e> rdf:type owl:Class ;
                                                                                         rdfs:subClassOf <http://emmo.info/emmo/middle/units-extension#EMMO_6795a4b8_ffd0_4588_a581_a9413fe49cac> ;
                                                                                         <http://emmo.info/emmo/top/annotations#EMMO_1f1b164d_ec6a_4faa_8d5e_88bda62316cc> "http://qudt.org/vocab/unit/NP" ;
                                                                                         <http://emmo.info/emmo/top/annotations#EMMO_6dd685dd_1895_46e4_b227_be9f7d643c25> "http://dbpedia.org/page/Neper" ;
                                                                                         <http://emmo.info/emmo/top/annotations#EMMO_70fe84ff_99b6_4206_a9fc_9a8931836d84> """Unit of measurement for quantities of type level or level difference, which are defined as the natural logarithm of the ratio of power- or field-type quantities.

The value of a ratio in nepers is given by `ln(x1/x2)` where `x1` and `x2` are the values of interest (amplitudes), and ln is the natural logarithm. When the values are quadratic in the amplitude (e.g. power), they are first linearised by taking the square root before the logarithm is taken, or equivalently the result is halved.

Wikipedia"""@en ;
                                                                                         <http://emmo.info/emmo/top/annotations#EMMO_c84c6752_6d64_48cc_9500_e54a3c34898d> "https://en.wikipedia.org/wiki/Neper" ;
                                                                                         <http://emmo.info/emmo/top/annotations#EMMO_fe015383_afb3_44a6_ae86_043628697aa2> "https://doi.org/10.1351/goldbook.N04106" ;
                                                                                         <http://www.w3.org/2004/02/skos/core#prefLabel> "Neper"@en .


###  http://emmo.info/emmo/middle/units-extension#EMMO_b8830065_3809_41b7_be3c_e33795567fd9
<http://emmo.info/emmo/middle/units-extension#EMMO_b8830065_3809_41b7_be3c_e33795567fd9> rdf:type owl:Class ;
                                                                                         rdfs:subClassOf <http://emmo.info/emmo/middle/units-extension#EMMO_6795a4b8_ffd0_4588_a581_a9413fe49cac> ;
                                                                                         <http://emmo.info/emmo/top/annotations#EMMO_1f1b164d_ec6a_4faa_8d5e_88bda62316cc> "http://qudt.org/vocab/unit/DEG" ;
                                                                                         <http://emmo.info/emmo/top/annotations#EMMO_6dd685dd_1895_46e4_b227_be9f7d643c25> "http://dbpedia.org/page/Degree_(angle)" ;
                                                                                         <http://emmo.info/emmo/top/annotations#EMMO_70fe84ff_99b6_4206_a9fc_9a8931836d84> "Degree is a measurement of plane angle, defined by representing a full rotation as 360 degrees."@en ;
                                                                                         <http://emmo.info/emmo/top/annotations#EMMO_fe015383_afb3_44a6_ae86_043628697aa2> "https://doi.org/10.1351/goldbook.D01560" ;
                                                                                         <http://www.w3.org/2004/02/skos/core#prefLabel> "Degree"@en .


###  http://emmo.info/emmo/middle/units-extension#EMMO_c10b7090_7284_4719_8e15_c743b13ca6ad
<http://emmo.info/emmo/middle/units-extension#EMMO_c10b7090_7284_4719_8e15_c743b13ca6ad> rdf:type owl:Class ;
                                                                                         rdfs:subClassOf <http://emmo.info/emmo/middle/siunits#EMMO_1273eb34_de48_43a9_925f_104110469dd2> ;
                                                                                         <http://emmo.info/emmo/top/annotations#EMMO_1f1b164d_ec6a_4faa_8d5e_88bda62316cc> "http://qudt.org/vocab/unit/N-M" ;
                                                                                         <http://emmo.info/emmo/top/annotations#EMMO_967080e5_2f42_4eb2_a3a9_c58143e835f9> "SI coherent measurement unit for torque."@en ;
                                                                                         <http://emmo.info/emmo/top/annotations#EMMO_e55f2d7c_9893_48cd_b4a4_fdf38253bd20> "http://www.ontology-of-units-of-measure.org/resource/om-2/newtonMetre" ;
                                                                                         rdfs:comment "Note that the physical dimension is the same as for Joule."@en ;
                                                                                         <http://www.w3.org/2004/02/skos/core#prefLabel> "NewtonMetre"@en .


###  http://emmo.info/emmo/middle/units-extension#EMMO_c2f5ee66_579c_44c6_a2e9_fa2eaa9fa4da
<http://emmo.info/emmo/middle/units-extension#EMMO_c2f5ee66_579c_44c6_a2e9_fa2eaa9fa4da> rdf:type owl:Class ;
                                                                                         rdfs:subClassOf <http://emmo.info/emmo/middle/metrology#EMMO_5ebd5e01_0ed3_49a2_a30d_cd05cbe72978> ;
                                                                                         <http://emmo.info/emmo/top/annotations#EMMO_967080e5_2f42_4eb2_a3a9_c58143e835f9> "Unit for fractions of quantities of the same kind, to aid the understanding of the quantity being expressed."@en ;
                                                                                         rdfs:comment """Quantities that are ratios of quantities of the same kind (for example length ratios and amount fractions) have the option of being expressed with units (m/m, mol/mol to aid the understanding of the quantity being expressed and also allow the use of SI prefixes, if this
is desirable (m/m, nmol/mol).
-- SI Brochure"""@en ;
                                                                                         <http://www.w3.org/2004/02/skos/core#prefLabel> "FractionUnit"@en .


###  http://emmo.info/emmo/middle/units-extension#EMMO_cabb20f0_05c7_448f_9485_e129725f15a4
<http://emmo.info/emmo/middle/units-extension#EMMO_cabb20f0_05c7_448f_9485_e129725f15a4> rdf:type owl:Class ;
                                                                                         rdfs:subClassOf <http://emmo.info/emmo/middle/units-extension#EMMO_6795a4b8_ffd0_4588_a581_a9413fe49cac> ;
                                                                                         <http://emmo.info/emmo/top/annotations#EMMO_1f1b164d_ec6a_4faa_8d5e_88bda62316cc> "http://qudt.org/vocab/unit/MIN" ;
                                                                                         <http://emmo.info/emmo/top/annotations#EMMO_6dd685dd_1895_46e4_b227_be9f7d643c25> "http://dbpedia.org/page/Minute" ;
                                                                                         <http://emmo.info/emmo/top/annotations#EMMO_70fe84ff_99b6_4206_a9fc_9a8931836d84> "Non-SI time unit defined as 60 seconds."@en ;
                                                                                         <http://www.w3.org/2004/02/skos/core#prefLabel> "Minute"@en .


###  http://emmo.info/emmo/middle/units-extension#EMMO_cdc962d8_f3ea_4764_a57a_c7caa4859179
<http://emmo.info/emmo/middle/units-extension#EMMO_cdc962d8_f3ea_4764_a57a_c7caa4859179> rdf:type owl:Class ;
                                                                                         rdfs:subClassOf <http://emmo.info/emmo/middle/units-extension#EMMO_c2f5ee66_579c_44c6_a2e9_fa2eaa9fa4da> ;
                                                                                         <http://emmo.info/emmo/top/annotations#EMMO_967080e5_2f42_4eb2_a3a9_c58143e835f9> "Unit for quantities of dimension one that are the fraction of two lengths."@en ;
                                                                                         <http://emmo.info/emmo/top/annotations#EMMO_b432d2d5_25f4_4165_99c5_5935a7763c1a> "Unit for plane angle."@en ;
                                                                                         <http://www.w3.org/2004/02/skos/core#prefLabel> "LengthFractionUnit"@en .


###  http://emmo.info/emmo/middle/units-extension#EMMO_d6eb0176_a0d7_4b4e_8df0_50e912be2342
<http://emmo.info/emmo/middle/units-extension#EMMO_d6eb0176_a0d7_4b4e_8df0_50e912be2342> rdf:type owl:Class ;
                                                                                         rdfs:subClassOf <http://emmo.info/emmo/middle/units-extension#EMMO_6795a4b8_ffd0_4588_a581_a9413fe49cac> ;
                                                                                         <http://emmo.info/emmo/top/annotations#EMMO_1f1b164d_ec6a_4faa_8d5e_88bda62316cc> "http://qudt.org/vocab/unit/HA" ;
                                                                                         <http://emmo.info/emmo/top/annotations#EMMO_6dd685dd_1895_46e4_b227_be9f7d643c25> "http://dbpedia.org/page/Hectare" ;
                                                                                         <http://emmo.info/emmo/top/annotations#EMMO_70fe84ff_99b6_4206_a9fc_9a8931836d84> "A non-SI metric unit of area defined as the square with 100-metre sides."@en ;
                                                                                         <http://emmo.info/emmo/top/annotations#EMMO_c84c6752_6d64_48cc_9500_e54a3c34898d> "https://en.wikipedia.org/wiki/Hectare" ;
                                                                                         <http://www.w3.org/2004/02/skos/core#prefLabel> "Hectare"@en .


###  http://emmo.info/emmo/middle/units-extension#EMMO_e29f84db_4c1c_46ae_aa38_c4d47536b972
<http://emmo.info/emmo/middle/units-extension#EMMO_e29f84db_4c1c_46ae_aa38_c4d47536b972> rdf:type owl:Class ;
                                                                                         rdfs:subClassOf <http://emmo.info/emmo/middle/units-extension#EMMO_6795a4b8_ffd0_4588_a581_a9413fe49cac> ;
                                                                                         <http://emmo.info/emmo/top/annotations#EMMO_1f1b164d_ec6a_4faa_8d5e_88bda62316cc> "http://qudt.org/vocab/unit/EV" ;
                                                                                         <http://emmo.info/emmo/top/annotations#EMMO_6dd685dd_1895_46e4_b227_be9f7d643c25> "http://dbpedia.org/page/Electronvolt" ;
                                                                                         <http://emmo.info/emmo/top/annotations#EMMO_70fe84ff_99b6_4206_a9fc_9a8931836d84> "The amount of energy gained (or lost) by the charge of a single electron moving across an electric potential difference of one volt."@en ;
                                                                                         <http://emmo.info/emmo/top/annotations#EMMO_fe015383_afb3_44a6_ae86_043628697aa2> "https://doi.org/10.1351/goldbook.E02014" ;
                                                                                         <http://www.w3.org/2004/02/skos/core#prefLabel> "ElectronVolt"@en .


###  http://emmo.info/emmo/middle/units-extension#EMMO_e7bc8939_7ff8_4917_beb5_c42730b390f3
<http://emmo.info/emmo/middle/units-extension#EMMO_e7bc8939_7ff8_4917_beb5_c42730b390f3> rdf:type owl:Class ;
                                                                                         rdfs:subClassOf <http://emmo.info/emmo/middle/units-extension#EMMO_c2f5ee66_579c_44c6_a2e9_fa2eaa9fa4da> ;
                                                                                         <http://emmo.info/emmo/top/annotations#EMMO_967080e5_2f42_4eb2_a3a9_c58143e835f9> "Unit for quantities of dimension one that are the fraction of two speeds."@en ;
                                                                                         <http://emmo.info/emmo/top/annotations#EMMO_b432d2d5_25f4_4165_99c5_5935a7763c1a> "Unit for refractive index."@en ;
                                                                                         <http://www.w3.org/2004/02/skos/core#prefLabel> "SpeedFractionUnit"@en .


###  http://emmo.info/emmo/middle/units-extension#EMMO_e9eaeeb5_620c_4dab_8f72_269ff85d0634
<http://emmo.info/emmo/middle/units-extension#EMMO_e9eaeeb5_620c_4dab_8f72_269ff85d0634> rdf:type owl:Class ;
                                                                                         rdfs:subClassOf <http://emmo.info/emmo/middle/siunits#EMMO_1273eb34_de48_43a9_925f_104110469dd2> ;
                                                                                         <http://emmo.info/emmo/top/annotations#EMMO_967080e5_2f42_4eb2_a3a9_c58143e835f9> "Measurement unit for electric dipole moment."@en ;
                                                                                         <http://www.w3.org/2004/02/skos/core#prefLabel> "CoulombMetre"@en .


###  http://emmo.info/emmo/middle/units-extension#EMMO_f76f5a24_d703_4e8c_b368_f9a7777cb73a
<http://emmo.info/emmo/middle/units-extension#EMMO_f76f5a24_d703_4e8c_b368_f9a7777cb73a> rdf:type owl:Class ;
                                                                                         rdfs:subClassOf <http://emmo.info/emmo/middle/units-extension#EMMO_c2f5ee66_579c_44c6_a2e9_fa2eaa9fa4da> ;
                                                                                         <http://emmo.info/emmo/top/annotations#EMMO_967080e5_2f42_4eb2_a3a9_c58143e835f9> "Unit for quantities of dimension one that are the fraction of two amount of substance."@en ;
                                                                                         <http://emmo.info/emmo/top/annotations#EMMO_b432d2d5_25f4_4165_99c5_5935a7763c1a> "Unit for amount fraction."@en ;
                                                                                         <http://www.w3.org/2004/02/skos/core#prefLabel> "AmountFractionUnit"@en .


###  http://emmo.info/emmo/middle/units-extension#EMMO_f8b92999_3cde_46e3_99d5_664da3090a02
<http://emmo.info/emmo/middle/units-extension#EMMO_f8b92999_3cde_46e3_99d5_664da3090a02> rdf:type owl:Class ;
                                                                                         rdfs:subClassOf <http://emmo.info/emmo/middle/units-extension#EMMO_6795a4b8_ffd0_4588_a581_a9413fe49cac> ;
                                                                                         <http://emmo.info/emmo/top/annotations#EMMO_1f1b164d_ec6a_4faa_8d5e_88bda62316cc> "http://qudt.org/vocab/unit/TON_M" ;
                                                                                         <http://emmo.info/emmo/top/annotations#EMMO_70fe84ff_99b6_4206_a9fc_9a8931836d84> "A non-SI unit defined as 1000 kg."@en ;
                                                                                         <http://emmo.info/emmo/top/annotations#EMMO_c84c6752_6d64_48cc_9500_e54a3c34898d> "https://en.wikipedia.org/wiki/Tonne" ;
                                                                                         <http://emmo.info/emmo/top/annotations#EMMO_fe015383_afb3_44a6_ae86_043628697aa2> "https://doi.org/10.1351/goldbook.T06394" ;
                                                                                         <http://www.w3.org/2004/02/skos/core#prefLabel> "Tonne"@en .


###  http://emmo.info/emmo/middle/units-extension#EMMO_f992dc76_f9a6_45f6_8873_c8e20d16fbbe
<http://emmo.info/emmo/middle/units-extension#EMMO_f992dc76_f9a6_45f6_8873_c8e20d16fbbe> rdf:type owl:Class ;
                                                                                         rdfs:subClassOf <http://emmo.info/emmo/middle/metrology#EMMO_216f448e_cdbc_4aeb_a529_7a5fe7fc38bb> ,
                                                                                                         <http://emmo.info/emmo/middle/units-extension#EMMO_52e4cb25_da39_45e2_a6db_063ec5730499> ;
                                                                                         <http://emmo.info/emmo/top/annotations#EMMO_1f1b164d_ec6a_4faa_8d5e_88bda62316cc> "http://qudt.org/vocab/unit/GM" ;
                                                                                         <http://emmo.info/emmo/top/annotations#EMMO_70fe84ff_99b6_4206_a9fc_9a8931836d84> "Gram is defined as one thousandth of the SI unit kilogram."@en ;
                                                                                         <http://emmo.info/emmo/top/annotations#EMMO_c84c6752_6d64_48cc_9500_e54a3c34898d> "https://en.wikipedia.org/wiki/Gram" ;
                                                                                         <http://emmo.info/emmo/top/annotations#EMMO_fe015383_afb3_44a6_ae86_043628697aa2> "https://doi.org/10.1351/goldbook.G02680" ;
                                                                                         <http://www.w3.org/2004/02/skos/core#prefLabel> "Gram"@en .


###  http://emmo.info/emmo/top#EMMO_49267eba_5548_4163_8f36_518d65b583f9
<http://emmo.info/emmo/top#EMMO_49267eba_5548_4163_8f36_518d65b583f9> rdf:type owl:Class ;
                                                                      rdfs:subClassOf <http://emmo.info/emmo/top/physical#EMMO_c5ddfdba_c074_4aa4_ad6b_1ac4942d300d> ;
                                                                      <http://emmo.info/emmo/top/annotations#EMMO_967080e5_2f42_4eb2_a3a9_c58143e835f9> "The class of individuals that stand for real world objects according to a specific representational perspective."@en ;
                                                                      rdfs:comment """This class is the practical implementation of the EMMO pluralistic approach for which the only objective categorization is provided by the Universe individual and all the Quantum individuals.

Between these two extremes, there are several subjective ways to categorize real world objects, each one provide under a 'Perspective' subclass."""@en ;
                                                                      <http://www.w3.org/2004/02/skos/core#prefLabel> "Perspective"@en .


###  http://emmo.info/emmo/top/mereotopology#EMMO_2d2ecd97_067f_4d0e_950c_d746b7700a31
<http://emmo.info/emmo/top/mereotopology#EMMO_2d2ecd97_067f_4d0e_950c_d746b7700a31> rdf:type owl:Class ;
                                                                                    rdfs:subClassOf <http://emmo.info/emmo/top/mereotopology#EMMO_802d3e92_8770_4f98_a289_ccaaab7fdddf> ;
                                                                                    <http://emmo.info/emmo/top/annotations#EMMO_967080e5_2f42_4eb2_a3a9_c58143e835f9> "The class of all individuals that stand for a real world not self-connected object."@en ;
                                                                                    rdfs:comment """A 'Collection' individual stands for a non-self-connected real world object.

A 'Collection' individual is related to each 'Item' individuals of the collection (i.e. the members) through the membership relation.

An 'Item' individual stands for a real world self-connected object which can be represented as a whole made of connected parts (e.g. a car made of components)."""@en ,
                                                                                                 """Formally, 'Collection' is axiomatized as the class of individuals that hasMember some 'Item'.

A 'Collection' cannot have as member another 'Collection'."""@en ,
                                                                                                 "From Latin collectio, from colligere gather together."@en ,
                                                                                                 "e.g. the collection of users of a particular software, the collection of atoms that have been part of that just dissociated molecule, or even the collection of atoms that are part of a molecule considered as single individual non-connected objects and not as a mereotopological self-connected fusion."@en ;
                                                                                    <http://www.w3.org/2004/02/skos/core#prefLabel> "Collection"@en .


###  http://emmo.info/emmo/top/mereotopology#EMMO_3f9ae00e_810c_4518_aec2_7200e424cf68
<http://emmo.info/emmo/top/mereotopology#EMMO_3f9ae00e_810c_4518_aec2_7200e424cf68> rdf:type owl:Class ;
                                                                                    rdfs:subClassOf <http://emmo.info/emmo/top/mereotopology#EMMO_eb3a768e_d53e_4be9_a23b_0714833c36de> ;
                                                                                    <http://emmo.info/emmo/top/annotations#EMMO_967080e5_2f42_4eb2_a3a9_c58143e835f9> "The class of 'EMMO' individuals that stand for real world objects that can't be further divided in time nor in space."@en ;
                                                                                    <http://emmo.info/emmo/top/annotations#EMMO_b432d2d5_25f4_4165_99c5_5935a7763c1a> """For a physics based ontology the 'Quantum' can stand for the smallest identifiable portion of spacetime defined by the Planck limit in length (1.616e-35 m) and time (5.39e-44 s).

However, the quantum mereotopology approach is not restricted only to physics. For example, in a manpower management ontology, a 'Quantum' can stand for an hour (time) of a worker (space) activity."""@en ;
                                                                                    rdfs:comment """A 'Quantum' is the most fundamental subclass of 'Item', since its individuals stand for the smallest possible self-connected 4D real world objects.

The quantum concept recalls the fact that there is lower epistemological limit to our knowledge of the universe, related to the uncertainity principle."""@en ,
                                                                                                 "A 'Quantum' stands for a 4D real world object."@en ,
                                                                                                 """A quantum is the EMMO mereological 4D a-tomic entity. 

To avoid confusion with the concept of atom coming from physics, we will use the expression quantum mereology, instead of a-tomistic mereology."""@en ,
                                                                                                 "From Latin quantum (plural quanta) \"as much as, so much as;\", introduced in physics directly from Latin by Max Planck, 1900."@en ;
                                                                                    <http://www.w3.org/2004/02/skos/core#prefLabel> "Quantum"@en .


###  http://emmo.info/emmo/top/mereotopology#EMMO_802d3e92_8770_4f98_a289_ccaaab7fdddf
<http://emmo.info/emmo/top/mereotopology#EMMO_802d3e92_8770_4f98_a289_ccaaab7fdddf> rdf:type owl:Class ;
                                                                                    <http://emmo.info/emmo/top/annotations#EMMO_967080e5_2f42_4eb2_a3a9_c58143e835f9> "The class representing the collection of all the individuals declared in this ontology standing for real world objects."@en ;
                                                                                    rdfs:comment """'EMMO' is the disjoint union of 'Item' and 'Collection' (covering axiom).

The union implies that 'EMMO' individuals can only be 'Item' individuals (standing for self-connected real world objects) or 'Collection' individuals (standing for a collection of disconnected items).

Disjointness means that a 'Collection' individual cannot be an 'Item' individual and viceversa, representing the fact that a real world object cannot be self-connected and non-self connected at the same time."""@en ,
                                                                                                 """For the EMMO ontologist the whole universe is represented as a 4D path-connected topological manifold (i.e. the spacetime).

A real world object is then a 4D topological sub-region of the universe. 

A universe sub-region is isolated and defined as a real world object by the ontologist. Then, through a semiotic process that occurs at meta-ontological level (i.e. outside the ontology). an EMMO ontology entity (e.g. an OWL individual) is assigned to represent that real world object.

The fundamental distinction between real world objects, upon which the EMMO is based, is self-connectedness: a real world object can be self-connected xor not self-connected."""@en ,
                                                                                                 "In the EMMO we will refer to the universe as a Minkowski space, restricting the ontology to special relativity only. However, exension to general relativity, will adding more complexity, should not change the overall approach."@en ,
                                                                                                 """Mereotopology is the fundamental logical representation used by the EMMO ontologist to characterize the universe and to provide the definitions to connect real world objects to the EMMO concepts.

Parthood relations do not change dimensionality of the real world object referred by an 'EMMO' individual, i.e. every part of a real world object always retains its 4D dimensionality. 

The smallest part of a real world object (i.e. a part that has no proper parts) is referred in the EMMO by a 'Quantum' individual.

It follows that, for the EMMO, real world objects of dimensionality lower than 4D (e.g. surfaces, lines) do not exist."""@en ;
                                                                                    <http://www.w3.org/2004/02/skos/core#prefLabel> "EMMO"@en .


###  http://emmo.info/emmo/top/mereotopology#EMMO_eb3a768e_d53e_4be9_a23b_0714833c36de
<http://emmo.info/emmo/top/mereotopology#EMMO_eb3a768e_d53e_4be9_a23b_0714833c36de> rdf:type owl:Class ;
                                                                                    rdfs:subClassOf <http://emmo.info/emmo/top/mereotopology#EMMO_802d3e92_8770_4f98_a289_ccaaab7fdddf> ;
                                                                                    rdfs:comment """A real world object is self-connected if any two parts that make up the whole are connected to each other (here the concept of connection is primitive). 

Alternatively, using the primitive path-connectivity concept we can define a self-connected real world object as an object for which each couple of points is path-connected."""@en ,
                                                                                                 """An 'Item' individual stands for a real world self-connected object which can be represented as a whole made of connected parts (e.g. a car made of components).

In the EMMO, connectivity is the topological foundation of causality.

All physical systems, i.e. systems whose behaviour is explained by physics laws, are represented only by 'Item'-s.

Members of a 'Collection' lack of causality connection, i.e. they do not constitute a physical system as a whole."""@en ,
                                                                                                 "From Latin item, \"likewise, just so, moreover\"."@en ;
                                                                                    <http://www.w3.org/2004/02/skos/core#prefLabel> "Item"@en .


###  http://emmo.info/emmo/top/physical#EMMO_0f795e3e_c602_4577_9a43_d5a231aa1360
<http://emmo.info/emmo/top/physical#EMMO_0f795e3e_c602_4577_9a43_d5a231aa1360> rdf:type owl:Class ;
                                                                               rdfs:subClassOf <http://emmo.info/emmo/top/physical#EMMO_c5ddfdba_c074_4aa4_ad6b_1ac4942d300d> ;
                                                                               <http://emmo.info/emmo/top/annotations#EMMO_967080e5_2f42_4eb2_a3a9_c58143e835f9> "The basic constituent of 'item'-s that can be proper partitioned only in time up to quantum level."@en ;
                                                                               rdfs:comment """According to mereology, this should be call 'a-tomistic' in the strict etimological sense of the word (from greek, a-tomos: un-divisible).

Mereology based on such items is called atomistic mereology.

However, in order not to confuse the lexicon between mereology and physics (in which an atom is a divisible physical entity) we prefer to call it 'elementary', recalling the concept of elementary particle coming from the standard particles model."""@en ,
                                                                                            "From Latin elementarius (elementary), from elementum (one of the four elements of antiquity; fundamentals)"@en ,
                                                                                            "While a 'Quantum' is a-tomistic in time and space, an 'elementary' is a-tomistic only in space, recalling the concept of elementary particle."@en ;
                                                                               <http://www.w3.org/2004/02/skos/core#prefLabel> "Elementary"@en .


###  http://emmo.info/emmo/top/physical#EMMO_29072ec4_ffcb_42fb_bdc7_26f05a2e9873
<http://emmo.info/emmo/top/physical#EMMO_29072ec4_ffcb_42fb_bdc7_26f05a2e9873> rdf:type owl:Class ;
                                                                               rdfs:subClassOf <http://emmo.info/emmo/top/mereotopology#EMMO_eb3a768e_d53e_4be9_a23b_0714833c36de> ;
                                                                               <http://emmo.info/emmo/top/annotations#EMMO_967080e5_2f42_4eb2_a3a9_c58143e835f9> "A 'Item' that has no 'Physical' parts."@en ;
                                                                               rdfs:comment "From Latin vacuus, empty."@en ,
                                                                                            "The void concept is paramount for the representation of physical systems according to quantum theory."@en ;
                                                                               <http://www.w3.org/2004/02/skos/core#prefLabel> "Void"@en .


###  http://emmo.info/emmo/top/physical#EMMO_c5ddfdba_c074_4aa4_ad6b_1ac4942d300d
<http://emmo.info/emmo/top/physical#EMMO_c5ddfdba_c074_4aa4_ad6b_1ac4942d300d> rdf:type owl:Class ;
                                                                               rdfs:subClassOf <http://emmo.info/emmo/top/mereotopology#EMMO_eb3a768e_d53e_4be9_a23b_0714833c36de> ;
                                                                               <http://emmo.info/emmo/top/annotations#EMMO_967080e5_2f42_4eb2_a3a9_c58143e835f9> "A 'Item' that has part some 'Elementary' and whose temporal proper parts are only 'Physical'-s (i.e. it can be perceived without interruptions in time)."@en ;
                                                                               rdfs:comment """A 'Physical' is the class that contains all the individuals that stand for real world objects that interact physically with the ontologist, i.e. physical objects.

A physical object must be perceived through physical interaction by the ontologist. Then the ontologist can declare an individual standing for the physical object just perceived.

Perception is a subcategory of physical interactions. It is an interaction that stimulate a representation of the physical object within the ontologist (the agent)."""@en ,
                                                                                            """A 'Physical' must include at least an 'Elementary' part, and can include 'Void' parts.

A 'Physical' may include as part also the 'Void' surrounding or enclosed by its 'Physical' sub parts.

There are no particular criteria for 'Physical'-s structure, except that is made of some 'Elementary'-s as proper parts and not only 'Void'.

This is done in order to take into account the quantum nature of physical systems, in which the actual position of sub-components (e.g. electrons in an atom) is not known except for its probability distribution function (according to the Copenhagen interpretation.)

e.g. a real world object that has spatial parts an atom and a cubic light year of void, extending for some time, can be a physical object."""@en ,
                                                                                            """A 'Physical' with dimensions other than 4D cannot exist, following the restriction of the parent 'EMMO' class.

It follows from the fact that perception is always unfolding in time.

e.g. you always have an aperture time when you take a picture or measure a property. Instantaneous perceptions are idealizations (abstractions) or a very small time measurement."""@en ,
                                                                                            """From Latin physica \"study of nature\" (and Ancient Greek f?s????, natural). 

Here the word relates to things perceived through the senses as opposed to the mind; tangible or concrete."""@en ,
                                                                                            "In the EMMO there are no relations such as occupiesSpace, since 'Physical'-s are themselves the 4D regions."@en ,
                                                                                            """The EMMO can be used to represent real world entities as 'Physical'-s that are easy to connect to classical or quantum mechanical based models.

Classical mechanics poses no representational issues, for the EMMO: the 4D representation of 'Physical'-s is consistent with classical physics systems.

However, the representation of 'Physical'-s that are typically analized through quantum mechanics (e.g. molecules, atoms, clusters), is not straightforward.

1) De Broglie - Bohm interpretation
The most simple approach is to rely on Bohmian mechanics, in which each particle is supposed to exists in a specific position between measurements (hidden variables approach), while its trajectory is calculated using a Guiding Equation based on a quantum field calculated with the Schroedinger Equation.

While this approach is really easy to implement in an ontology, since each entity has its own well defined 4D region, its mathematical representation failed to receive large consensus due to the difficulties to include relativistic effects, to be extended to subnuclear scale and the strong non-locality assumtpion of the quantum field.

Nevertheless, the Bohmian mechanics is a numerical approach that is used in electronic models to reduce the computational effort of the solution of Schroedinger Equation.

In practice, an EMMO user can declare a 'physical' individual that stand for the whole quantum system to be described, and at the same time all sub-parts individuals can be declared, having them a well defined position in time, according to De Broglie - Bohm interpretation. The Hamiltonian can be calculated by considering the sub-part individuals.

'physical'-s are then made of 'physical' parts and 'void' parts that stand for the space between 'physical'-s (e.g. the void between electrons and nucleus in an atom).

2) Copenhagen interpretation
In this interpretation the properties (e.g. energy level, position, spin) of a particle are not defined in the interval between two measurements and the quantum system is entangled (i.e. properties of particles in the sysyem are correlated) and described by a global wavefunction obtained solving the Schroedinger Equation. 

Upon measurement, the wavefunction collapses to a combination of close eigenstates that provide information about bservables of the system components (e.g. position, energy).

The EMMO can be used to represent 'physical'-s that can be related to Copenhagen based models. In practice, the user should follow these steps:

a) define the quantum system as a 'physical' individual (e.g. an H2 molecule) under a specific class (e.g. 'h2_molecule'). This individual is the whole.

b) define the axioms of the  class that describe how many sub-parts are expected for the whole and their class types (e.g. 'h2_molecule' has axioms 'has_proper_part exactly 2 electron' and 'has_proper_part exactly 2 nucleus)

c) the user can now connect the whole to a Schroedinger equation based model whose Hamiltonian is calculated trough the information coming only from the axioms. No individuals are declared for the subparts!

d) a measurement done on the quantum system that provides information on the sub-part observables is interpreted as wavefunction collapse and leads to the end of the whole and the declaration of the sub-parts individuals which can be themselves other quantum systems 

e.g. if the outer electron of the H2 molecule interacts with another entity defining its state, then the whole that stands for the entangled H2 molecule becomes a 'physical' made of an electron individual, a quantum system made of one electron and two nuclei and the void between them.

e.g. in the Born-Oppenheimer approximation the user represent the atom by un-entangling nucleus and electronic cloud. The un-entanglement comes in the form of declaration of individual as parts.

e.g. the double slit experiment can be represent in the EMMO as:
a) before the slit: a 'physical' that extend in space and has parts 'electron' and 'void', called 'single_electron_wave_function'. 'electron' and 'void' are only in the axioms and not decalred individuals.
b) during slit passage: a 'physical' made of one declared individual, the 'electron'.
c) after the slit: again 'single_electron_wave_function'
d) upon collision with the detector:  'physical' made of one declared individual, the 'electron'."""@en ,
                                                                                            """The purpose of the 'Physical' branch is to provide a representation of the real world objects, while the models used to name, explain or predict the behaviour of the real world objects lay under the 'Semiotic' branch.

More than one semiotic representation can be connected to the same 'Physical'.

e.g. Navier-Stokes or Euler equation applied to the same fluid are an example of mathematical model used to represent a physical object for some specific interpreter."""@en ;
                                                                               <http://www.w3.org/2004/02/skos/core#prefLabel> "Physical"@en .


[ owl:qualifiedCardinality "1"^^xsd:nonNegativeInteger
] .

[ owl:minQualifiedCardinality "1"^^xsd:nonNegativeInteger
 ] .

[ owl:minQualifiedCardinality "2"^^xsd:nonNegativeInteger
 ] .

[ owl:minQualifiedCardinality "2"^^xsd:nonNegativeInteger
 ] .

[ owl:minQualifiedCardinality "1"^^xsd:nonNegativeInteger
 ] .

[ owl:qualifiedCardinality "1"^^xsd:nonNegativeInteger
 ] .

[ owl:qualifiedCardinality "1"^^xsd:nonNegativeInteger
 ] .

[ owl:qualifiedCardinality "1"^^xsd:nonNegativeInteger
 ] .

[ owl:qualifiedCardinality "1"^^xsd:nonNegativeInteger
 ] .

[ owl:qualifiedCardinality "1"^^xsd:nonNegativeInteger
 ] .

#################################################################
#    Annotations
#################################################################

<http://emmo.info/emmo/domain/mechanical-testing#EMMO_474a5489_aad9_418c_9aef_e3873017c43b> rdfs:comment "a data propery introduced to be able to describe very simply the existing dataset that categorizes runout into 3 categories - true, false and unknown.To be changed!" ;
                                                                                             <http://www.w3.org/2004/02/skos/core#prefLabel> "hasRunOut"@en ;
                                                                                             rdfs:comment "A run out is a specimen that survives a certain amount of cycles (cycle limit e. g. 10^7) without failure." .


<http://emmo.info/emmo/domain/mechanical-testing#EMMO_52813850_bc0e_450f_8a62_4832288ca1b2> rdfs:comment "a data propery introduced to be able to describe very simply the existing dataset that categorizes hardening into 3 categories - true, false and unknown.To be changed!" ;
                                                                                            <http://www.w3.org/2004/02/skos/core#prefLabel> "hasHardening"@en .


<http://emmo.info/emmo/domain/mechanical-testing#EMMO_a7dddd8f_51f4_4cf5_a8a2_a7aba83e8a72> rdfs:comment "a data propery introduced to be able to describe very simply the existing dataset that categorizes case hardening into 3 categories - true, false and unknown.To be changed!" ;
                                                                                            <http://www.w3.org/2004/02/skos/core#prefLabel> "hasCaseHardening"@en .


<http://emmo.info/emmo/middle/math#EMMO_faf79f53_749d_40b2_807c_d34244c192f4> <http://www.w3.org/2004/02/skos/core#prefLabel> "hasNumericalData"@en .


<http://emmo.info/emmo/middle/perceptual#EMMO_23b579e1_8088_45b5_9975_064014026c42> <http://www.w3.org/2004/02/skos/core#prefLabel> "hasSymbolData"@en .


<http://emmo.info/emmo/top/annotations#EMMO_21ae69b4_235e_479d_8dd8_4f756f694c1b> owl:deprecated "Replaced by skos:altLabel" ;
                                                                                  <http://www.w3.org/2004/02/skos/core#prefLabel> "altLabel"@en .


<http://emmo.info/emmo/top/annotations#EMMO_5525a055_dda5_4556_8b91_f0d22fa676cc> <http://www.w3.org/2004/02/skos/core#prefLabel> "license"@en ;
                                                                                  owl:deprecated "Replaced by dcterms:license" .


<http://emmo.info/emmo/top/annotations#EMMO_b306ae38_938e_48fe_83e9_6141e08b596f> rdfs:comment "URL to corresponding concept in the Basic Datatype Ontology (DBO)"@en ;
                                                                                  rdfs:seeAlso "https://github.com/TechnicalBuildingSystems/Ontologies/blob/master/BasicDataTypeOntology/ontology.ttl"^^xsd:anyURI ;
                                                                                  <http://www.w3.org/2004/02/skos/core#prefLabel> "bdoMatch"@en .


<http://emmo.info/emmo/top/annotations#EMMO_cd5fb112_7ee7_4120_a35d_3ca3e6c3f4ab> owl:deprecated "Replaced by dcterms:creator" ;
                                                                                  <http://www.w3.org/2004/02/skos/core#prefLabel> "author"@en .


<http://emmo.info/emmo/top/mereotopology#EMMO_08cb807c_e626_447b_863f_e2835540e918> <http://www.w3.org/2004/02/skos/core#prefLabel> "Universe"@en .


###  Generated by the OWL API (version 4.5.9.2019-02-01T07:24:44Z) https://github.com/owlcs/owlapi
